@prefix dc: <http://purl.org/dc/elements/1.1/> .
@prefix rdakit: <http://metadataregistry.org/uri/profile/rdakit/> .
@prefix rdf: <http://www.w3.org/1999/02/22-rdf-syntax-ns#> .
@prefix rdfs: <http://www.w3.org/2000/01/rdf-schema#> .
@prefix reg: <http://metadataregistry.org/uri/profile/regap/> .
@prefix skos: <http://www.w3.org/2004/02/skos/core#> .
@prefix xml: <http://www.w3.org/XML/1998/namespace> .
@prefix xsd: <http://www.w3.org/2001/XMLSchema#> .

<http://rdaregistry.info/termList/formatNoteMus/1001> a skos:Concept ;
    rdakit:toolkitDefinition "A format of notated music consisting of a large music book made to be placed on a stand in front of a choir."@en,
        "Un libro grande de música creado para ser colocado en un atril enfrente de un coro. Cada parte tiene notación separada, usualmente en la configuración que presenta, cuando el libro está abierto, las partes de la soprano y el tenor en el reverso de una hoja y las partes del alto y el bajo en el anverso de la siguiente hoja."@es,
        "Grand livre de musique fait pour être placé sur un pupitre devant un chœur. Chaque partie est notée séparément, généralement selon une configuration présentant, quand le livre est ouvert, les parties de soprano et de ténor sur le verso d’un feuillet, et les parties d’alto et de basse sur le recto du feuillet suivant."@fr,
        "放在唱诗班前面立架上的大型乐谱，每部分的乐谱是分开的，通常的编排为，当乐谱打开时，女高音和男高音部分在反面的页上，女低音和男低音部分在下一个正面的页上。"@zh ;
    rdakit:toolkitLabel "choir book"@en,
        "libro de coro"@es,
        "livre de chœur"@fr,
        "唱诗班乐谱"@zh ;
    reg:identifier <http://metadataregistry.org/concepts/1153> ;
    reg:status <http://metadataregistry.org/uri/RegStatus/1001> ;
    skos:definition "Ein großes Musikbuch, das gemacht wurde, um auf einem Ständer vor dem Chor platziert zu werden. Jede Stimme ist separat notiert, normalerweise in der Zusammenstellung, die die Sopran- und Tenorstimmen auf der Rückseite eines Blattes und die Alt- und Bass-Stimmen auf der Vorderseite des nächsten Blattes präsentiert, wenn das Buch geöffnet ist."@de,
        "A format of notated music consisting of a large music book made to be placed on a stand in front of a choir."@en,
        "Un libro grande de música creado para ser colocado en un atril enfrente de un coro. Cada parte tiene notación separada, usualmente en la configuración que presenta, cuando el libro está abierto, las partes de la soprano y el tenor en el reverso de una hoja y las partes del alto y el bajo en el anverso de la siguiente hoja."@es,
        "Grand livre de musique fait pour être placé sur un pupitre devant un chœur. Chaque partie est notée séparément, généralement selon une configuration présentant, quand le livre est ouvert, les parties de soprano et de ténor sur le verso d’un feuillet, et les parties d’alto et de basse sur le recto du feuillet suivant."@fr,
        "放在唱诗班前面立架上的大型乐谱，每部分的乐谱是分开的，通常的编排为，当乐谱打开时，女高音和男高音部分在反面的页上，女低音和男低音部分在下一个正面的页上。"@zh ;
    skos:inScheme <http://rdaregistry.info/termList/formatNoteMus> ;
    skos:prefLabel "Chorbuch"@de,
        "choir book"@en,
        "libro de coro"@es,
        "livre de chœur"@fr,
        "唱诗班乐谱"@zh ;
    skos:scopeNote "Each part is notated separately, usually in the configuration that presents, when the book is open, the soprano and tenor parts on the verso of a leaf, and the alto and bass parts on the recto of the next leaf."@en .

<http://rdaregistry.info/termList/formatNoteMus/1003> a skos:Concept ;
    rdakit:toolkitDefinition "A format of notated music consisting of a score in which the number of staves is reduced to two or a few, generally organized by instrumental sections or vocal parts, and often with cues for individual parts."@en,
        "Partitura en la que el número de pentagramas se ha reducido a dos, o a unos pocos, generalmente organizada en secciones instrumentales o partes vocales y con frecuencia con indicaciones para partes individuales."@es,
        "Partition dans laquelle le nombre de portées est réduit à deux ou à quelques-unes, généralement organisées par sections instrumentales ou parties vocales, et souvent avec des repères pour les parties individuelles."@fr,
        "五线谱的数量被缩减为两个或更少的总谱，通常按乐器演奏部分编排，并附有对各个部分的提示。"@zh ;
    rdakit:toolkitLabel "condensed score"@en,
        "partitura abreviada"@es,
        "partition réduite"@fr,
        "缩写谱"@zh ;
    reg:identifier <http://metadataregistry.org/concepts/1155> ;
    reg:status <http://metadataregistry.org/uri/RegStatus/1001> ;
    skos:altLabel "close score"@en,
        "reduced score"@en,
        "short score"@en,
        "partitura breve"@es,
        "partitura cerrada"@es,
        "partitura reducida"@es,
        "particelle"@fr,
        "partition condensée"@fr,
        "简化谱"@zh ;
    skos:definition "A format of notated music consisting of a score in which the number of staves is reduced to two or a few, generally organized by instrumental sections or vocal parts, and often with cues for individual parts."@en,
        "Partitura en la que el número de pentagramas se ha reducido a dos, o a unos pocos, generalmente organizada en secciones instrumentales o partes vocales y con frecuencia con indicaciones para partes individuales."@es,
        "Partition dans laquelle le nombre de portées est réduit à deux ou à quelques-unes, généralement organisées par sections instrumentales ou parties vocales, et souvent avec des repères pour les parties individuelles."@fr,
        "五线谱的数量被缩减为两个或更少的总谱，通常按乐器演奏部分编排，并附有对各个部分的提示。"@zh ;
    skos:inScheme <http://rdaregistry.info/termList/formatNoteMus> ;
    skos:prefLabel "condensed score"@en,
        "partitura abreviada"@es,
        "partition réduite"@fr,
        "缩写谱"@zh .

<http://rdaregistry.info/termList/formatNoteMus/1004> a skos:Concept ;
    rdakit:toolkitDefinition "A format of notated music consisting of the music for the use of one or more, but not all, performers."@en,
        "En el contexto de la música notada, un componente que consiste en la música para el uso de uno o más, pero no todos, los intérpretes."@es,
        "Dans le contexte de la musique notée, partie composante consistant en musique à destination d’un ou plusieurs interprètes, mais non de tous."@fr,
        "就音乐乐谱而言，指由一个或多个，但不是所有表演者使用的音乐组成的部分。"@zh ;
    rdakit:toolkitLabel "part"@en,
        "parte"@es,
        "partie"@fr,
        "分谱"@zh ;
    reg:identifier <http://metadataregistry.org/concepts/1156> ;
    reg:status <http://metadataregistry.org/uri/RegStatus/1001> ;
    skos:definition "Im Zusammenhang mit Noten handelt es sich um einen Bestandteil, der aus der Musik für die Verwendung durch einen oder mehrere, aber nicht alle Ausführende besteht."@de,
        "A format of notated music consisting of the music for the use of one or more, but not all, performers."@en,
        "En el contexto de la música notada, un componente que consiste en la música para el uso de uno o más, pero no todos, los intérpretes."@es,
        "Dans le contexte de la musique notée, partie composante consistant en musique à destination d’un ou plusieurs interprètes, mais non de tous."@fr,
        "就音乐乐谱而言，指由一个或多个，但不是所有表演者使用的音乐组成的部分。"@zh ;
    skos:inScheme <http://rdaregistry.info/termList/formatNoteMus> ;
    skos:prefLabel "Stimme"@de,
        "part"@en,
        "parte"@es,
        "partie"@fr,
        "分谱"@zh .

<http://rdaregistry.info/termList/formatNoteMus/1005> a skos:Concept ;
    rdakit:toolkitDefinition "A format of notated music consisting of a performance part for a piano performer in an ensemble, with cues for the other instruments that enable the performer of that part also to conduct."@en,
        "Parte de interpretación de piano para un pianista en un conjunto de músicos que contiene indicaciones para los otros instrumentos, que también permiten conducir al intérprete de esa parte."@es,
        "Partie d’exécution pour un pianiste dans un ensemble avec l’indication de l’entrée des autres instruments permettant également à l’exécutant de cette partie de diriger l’ensemble."@fr,
        "在集体演奏中由钢琴演奏的部分，它对其他乐器的演奏可起到提示和指挥的作用。"@zh ;
    rdakit:toolkitLabel "piano conductor part"@en,
        "parte de piano del director"@es,
        "partie de piano conducteur"@fr,
        "钢琴指挥分谱"@zh ;
    reg:identifier <http://metadataregistry.org/concepts/1157> ;
    reg:status <http://metadataregistry.org/uri/RegStatus/1001> ;
    skos:definition "Eine Aufführungsstimme für einen Ausführenden am Klavier in einem Ensemble mit Einsätzen für die anderen Instrumente, die den Ausführenden dieser Stimme ebenfalls in die Lage versetzen zu dirigieren."@de,
        "A format of notated music consisting of a performance part for a piano performer in an ensemble, with cues for the other instruments that enable the performer of that part also to conduct."@en,
        "Parte de interpretación de piano para un pianista en un conjunto de músicos que contiene indicaciones para los otros instrumentos, que también permiten conducir al intérprete de esa parte."@es,
        "Partie d’exécution pour un pianiste dans un ensemble avec l’indication de l’entrée des autres instruments permettant également à l’exécutant de cette partie de diriger l’ensemble."@fr,
        "在集体演奏中由钢琴演奏的部分，它对其他乐器的演奏可起到提示和指挥的作用。"@zh ;
    skos:inScheme <http://rdaregistry.info/termList/formatNoteMus> ;
    skos:prefLabel "Klavier-Direktionsstimme"@de,
        "piano conductor part"@en,
        "parte de piano del director"@es,
        "partie de piano conducteur"@fr,
        "钢琴指挥分谱"@zh .

<http://rdaregistry.info/termList/formatNoteMus/1006> a skos:Concept ;
    rdakit:toolkitDefinition "A format of notated music consisting of a reduction of an instrumental work or a vocal work with instruments to a version for piano."@en,
        "Reducción de una obra musical (o de una obra vocal) con instrumentos a una versión para piano."@es,
        "Réduction à une version pour piano d’une œuvre instrumentale ou d’une œuvre vocale avec instruments."@fr,
        "对器乐或声乐作品进行缩减，使之成为钢琴演奏版，"@zh ;
    rdakit:toolkitLabel "piano score"@en,
        "partitura para piano"@es,
        "partition de piano"@fr,
        "钢琴总谱"@zh ;
    reg:identifier <http://metadataregistry.org/concepts/1158> ;
    reg:status <http://metadataregistry.org/uri/RegStatus/1001> ;
    skos:definition "Eine Aufführungsstimme für einen Ausführenden am Klavier in einem Ensemble mit Einsätzen für die anderen Instrumente, die den Ausführenden dieser Stimme ebenfalls in die Lage versetzen zu dirigieren."@de,
        "A format of notated music consisting of a reduction of an instrumental work or a vocal work with instruments to a version for piano."@en,
        "Reducción de una obra musical (o de una obra vocal) con instrumentos a una versión para piano."@es,
        "Réduction à une version pour piano d’une œuvre instrumentale ou d’une œuvre vocale avec instruments."@fr,
        "对器乐或声乐作品进行缩减，使之成为钢琴演奏版，"@zh ;
    skos:inScheme <http://rdaregistry.info/termList/formatNoteMus> ;
    skos:prefLabel "Klavierbearbeitung"@de,
        "piano score"@en,
        "partitura para piano"@es,
        "partition de piano"@fr,
        "钢琴总谱"@zh ;
    skos:scopeNote "Peut inclure les paroles d’une œuvre vocale."@fr,
        "可包含声乐作品的词。"@zh .

<http://rdaregistry.info/termList/formatNoteMus/1007> a skos:Concept ;
    rdakit:toolkitDefinition "A format of notated music consisting of graphical, symbolic, or word-based musical notation representing the sounds of all the parts of an ensemble or a work for solo performer or electronic media."@en,
        "Notación gráfica, simbólica o basada en palabras, que representa los sonidos de todas las partes de un conjunto o de una obra para un solista o para medios electrónicos."@es,
        "Notation musicale graphique, symbolique ou basée sur des mots, représentant les sons de toutes les parties d’un ensemble ou d’une œuvre pour soliste ou pour média électronique."@fr,
        "表现合唱/合奏各声部、独唱/独奏表演或电子音乐作品声音的图形、符号或文字的音乐标记。"@zh ;
    rdakit:toolkitLabel "score"@en,
        "partitura"@es,
        "partition"@fr,
        "总谱"@zh ;
    reg:identifier <http://metadataregistry.org/concepts/1159> ;
    reg:status <http://metadataregistry.org/uri/RegStatus/1001> ;
    skos:altLabel "full score"@en,
        "partitura completa"@es,
        "总谱"@zh ;
    skos:definition "Grafische, zeichen- oder wort-basierte Musiknotation, die die Töne für alle Stimmen eines Ensembles oder eines Werks für Solisten oder elektronische Medien repräsentiert."@de,
        "A format of notated music consisting of graphical, symbolic, or word-based musical notation representing the sounds of all the parts of an ensemble or a work for solo performer or electronic media."@en,
        "Notación gráfica, simbólica o basada en palabras, que representa los sonidos de todas las partes de un conjunto o de una obra para un solista o para medios electrónicos."@es,
        "Notation musicale graphique, symbolique ou basée sur des mots, représentant les sons de toutes les parties d’un ensemble ou d’une œuvre pour soliste ou pour média électronique."@fr,
        "表现合唱/合奏各声部、独唱/独奏表演或电子音乐作品声音的图形、符号或文字的音乐标记。"@zh ;
    skos:inScheme <http://rdaregistry.info/termList/formatNoteMus> ;
    skos:prefLabel "Partitur"@de,
        "score"@en,
        "partitura"@es,
        "partition"@fr,
        "总谱"@zh ;
    skos:scopeNote "Do not confuse with Part."@en,
        "不要与术语“分谱”（Part）相混淆。"@zh .

<http://rdaregistry.info/termList/formatNoteMus/1008> a skos:Concept ;
    rdakit:toolkitDefinition "A format of notated music consisting of a score issued in a musical image of reduced size, not primarily intended for use in performance."@en,
        "Partitura publicada como una imagen musical de tamaño reducido, que no tiene como propósito principal ser utilizada para la interpretación. Normalmente aparece en el recurso una frase descriptiva tal como \"Partitura de estudio\", \"Miniature score\", \"Taschenpartitur\", \"Partition de poche\", etc. normalmente aparece en el recurso."@es,
        "Partition publiée comme une image musicale réduite, qui n’est pas d’abord prévue pour être utilisée lors de l’exécution d’une œuvre."@fr,
        "以小尺寸出版的乐谱翻版，不是主要用于演奏的。"@zh ;
    rdakit:toolkitLabel "study score"@en,
        "partitura para estudiar"@es,
        "partition de travail"@fr,
        "研习总谱"@zh ;
    reg:identifier <http://metadataregistry.org/concepts/1160> ;
    reg:status <http://metadataregistry.org/uri/RegStatus/1001> ;
    skos:altLabel "miniature score"@en,
        "partitura miniatura"@es ;
    skos:definition "Eine Partitur, die als eine musikalische Abbildung in reduzierter Größe erscheint und die nicht in erster Linie für den Gebrauch in der Aufführung vorgesehen ist und normalerweise eine beschreibende Phrase aufweist wie \"Studienpartitur\", \"Miniature score\", \"Taschenpartitur\", \"Partition de poche\" usw."@de,
        "A format of notated music consisting of a score issued in a musical image of reduced size, not primarily intended for use in performance."@en,
        "Partitura publicada como una imagen musical de tamaño reducido, que no tiene como propósito principal ser utilizada para la interpretación. Normalmente aparece en el recurso una frase descriptiva tal como \"Partitura de estudio\", \"Miniature score\", \"Taschenpartitur\", \"Partition de poche\", etc. normalmente aparece en el recurso."@es,
        "Partition publiée comme une image musicale réduite, qui n’est pas d’abord prévue pour être utilisée lors de l’exécution d’une œuvre."@fr,
        "以小尺寸出版的乐谱翻版，不是主要用于演奏的。"@zh ;
    skos:inScheme <http://rdaregistry.info/termList/formatNoteMus> ;
    skos:prefLabel "Studienpartitur"@de,
        "study score"@en,
        "partitura para estudiar"@es,
        "partition de travail"@fr,
        "研习总谱"@zh .

<http://rdaregistry.info/termList/formatNoteMus/1009> a skos:Concept ;
    rdakit:toolkitDefinition "A format of notated music consisting of a music book made to be placed on a table and displayed in such a way that the performers can read their parts while seated or standing across or around the table."@en,
        "Un libro de música, creado para ser colocado en una mesa y mostrado de tal manera que los intérpretes puedan leer sus partes mientras están sentados o de pie a lo largo o alrededor de la mesa. Cada parte tiene notación independiente, normalmente en una configuración que presenta, cuando el libro está abierto, diferentes partes en posiciones invertidas y/o perpendiculares."@es,
        "Livre de musique conçu pour être posé sur une table et disposé de façon que les interprètes puissent lire leur partie assis ou debout des deux côtés ou autour de la table. Chaque partie est notée séparément, habituellement dans une configuration qui présente, lorsque le livre est ouvert, les différentes parties inversées et/ou perpendiculaires les unes par rapport aux autres."@fr,
        "用于放在桌上或以这种方式陈列，使得面对面或围成一圈坐着或站立的演奏者可看到他们所演奏的部分的乐谱。每个部分是分别记谱的，通常的编排为，当乐谱打开时，不同的部分相对倒置和/或相对垂直排序。"@zh ;
    rdakit:toolkitLabel "table book"@en,
        "libro de mesa"@es,
        "livre de table"@fr,
        "桌谱"@zh ;
    reg:identifier <http://metadataregistry.org/concepts/1161> ;
    reg:status <http://metadataregistry.org/uri/RegStatus/1001> ;
    skos:definition "Ein Musikbuch, das dazu gedacht ist, auf einem Tisch platziert und so gelegt zu werden, dass die Ausführenden ihre Stimmen lesen können, während sie am oder um den Tisch sitzen oder stehen. Jede Stimme ist getrennt notiert, normalerweise in einer Anordnung, die wenn das Buch geöffnet ist, verschiedene Stimmen in seitenverkehrten und senkrechten Positionen präsentiert."@de,
        "A format of notated music consisting of a music book made to be placed on a table and displayed in such a way that the performers can read their parts while seated or standing across or around the table."@en,
        "Un libro de música, creado para ser colocado en una mesa y mostrado de tal manera que los intérpretes puedan leer sus partes mientras están sentados o de pie a lo largo o alrededor de la mesa. Cada parte tiene notación independiente, normalmente en una configuración que presenta, cuando el libro está abierto, diferentes partes en posiciones invertidas y/o perpendiculares."@es,
        "Livre de musique conçu pour être posé sur une table et disposé de façon que les interprètes puissent lire leur partie assis ou debout des deux côtés ou autour de la table. Chaque partie est notée séparément, habituellement dans une configuration qui présente, lorsque le livre est ouvert, les différentes parties inversées et/ou perpendiculaires les unes par rapport aux autres."@fr,
        "用于放在桌上或以这种方式陈列，使得面对面或围成一圈坐着或站立的演奏者可看到他们所演奏的部分的乐谱。每个部分是分别记谱的，通常的编排为，当乐谱打开时，不同的部分相对倒置和/或相对垂直排序。"@zh ;
    skos:inScheme <http://rdaregistry.info/termList/formatNoteMus> ;
    skos:prefLabel "Table Book"@de,
        "table book"@en,
        "libro de mesa"@es,
        "livre de table"@fr,
        "桌谱"@zh ;
    skos:scopeNote "Each part is notated separately, usually in a configuration that presents, when the book is open, different parts in inverted and/or perpendicular positions."@en .

<http://rdaregistry.info/termList/formatNoteMus/1010> a skos:Concept ;
    rdakit:toolkitDefinition "A format of notated music consisting of a performance part for a violin performer in an ensemble, with cues for the other instruments that enable the performer of that part also to conduct."@en,
        "Parte de interpretación para un violinista en un grupo instrumental, que contiene indicaciones para los otros instrumentos, que permiten al intérprete de esa parte también dirigir."@es,
        "Partie d’exécution pour un violoniste dans un ensemble avec l’indication de l’entrée des autres instruments permettant également à l’exécutant de cette partie de diriger l’ensemble."@fr,
        "在集体演奏中由小提琴演奏的部分，它对其他乐器的演奏可起到提示和指挥的作用。"@zh ;
    rdakit:toolkitLabel "violin conductor part"@en,
        "parte de violín del director"@es,
        "partie de violon conducteur"@fr,
        "小提琴指挥分谱"@zh ;
    reg:identifier <http://metadataregistry.org/concepts/1162> ;
    reg:status <http://metadataregistry.org/uri/RegStatus/1001> ;
    skos:definition "Eine Aufführungsstimme für einen Violinenspieler in einem Ensemble mit Einsätzen für die anderen Instrumente, die dem Musiker ermöglichen, auch zu dirigieren."@de,
        "A format of notated music consisting of a performance part for a violin performer in an ensemble, with cues for the other instruments that enable the performer of that part also to conduct."@en,
        "Parte de interpretación para un violinista en un grupo instrumental, que contiene indicaciones para los otros instrumentos, que permiten al intérprete de esa parte también dirigir."@es,
        "Partie d’exécution pour un violoniste dans un ensemble avec l’indication de l’entrée des autres instruments permettant également à l’exécutant de cette partie de diriger l’ensemble."@fr,
        "在集体演奏中由小提琴演奏的部分，它对其他乐器的演奏可起到提示和指挥的作用。"@zh ;
    skos:inScheme <http://rdaregistry.info/termList/formatNoteMus> ;
    skos:prefLabel "Violin-Direktionsstimme"@de,
        "violin conductor part"@en,
        "parte de violín del director"@es,
        "partie de violon conducteur"@fr,
        "小提琴指挥分谱"@zh .

<http://rdaregistry.info/termList/formatNoteMus/1002> a skos:Concept ;
    rdakit:toolkitDefinition "A format of notated music consisting of a score of a work for solo voices and chorus showing only the parts for chorus, at least in those portions of the work in which the chorus sings, with the instrumental accompaniment either arranged for keyboard or other chordal instruments or omitted."@en,
        "Partitura de una obra para solos de voces y coro mostrando solo las partes del coro, al menos en aquellas porciones de la obra en las que canta el coro, con el acompañamiento instrumental ya sea arreglado para teclado(s) u otros instrumentos de cuerda u omitidos."@es,
        "Partition d’une œuvre pour voix solistes et chœur présentant seulement la partie pour chœur (au moins pour les parties de l’œuvre où le chœur chante) avec l’accompagnement instrumental arrangé pour un ou plusieurs instruments à clavier ou autres instruments harmoniques ou sans l’accompagnement instrumental."@fr,
        "本身包括独唱和合唱的乐谱，但只显示合唱部分。在这部分中至少包括合唱和键盘或其他弦乐乐器的伴奏，伴奏部分也可能省略。"@zh ;
    rdakit:toolkitLabel "chorus score"@en,
        "partitura coral"@es,
        "partition de chœur"@fr,
        "合唱总谱"@zh ;
    reg:identifier <http://metadataregistry.org/concepts/1154> ;
    reg:status <http://metadataregistry.org/uri/RegStatus/1001> ;
    skos:definition "A format of notated music consisting of a score of a work for solo voices and chorus showing only the parts for chorus, at least in those portions of the work in which the chorus sings, with the instrumental accompaniment either arranged for keyboard or other chordal instruments or omitted."@en,
        "Partitura de una obra para solos de voces y coro mostrando solo las partes del coro, al menos en aquellas porciones de la obra en las que canta el coro, con el acompañamiento instrumental ya sea arreglado para teclado(s) u otros instrumentos de cuerda u omitidos."@es,
        "Partition d’une œuvre pour voix solistes et chœur présentant seulement la partie pour chœur (au moins pour les parties de l’œuvre où le chœur chante) avec l’accompagnement instrumental arrangé pour un ou plusieurs instruments à clavier ou autres instruments harmoniques ou sans l’accompagnement instrumental."@fr,
        "本身包括独唱和合唱的乐谱，但只显示合唱部分。在这部分中至少包括合唱和键盘或其他弦乐乐器的伴奏，伴奏部分也可能省略。"@zh ;
    skos:inScheme <http://rdaregistry.info/termList/formatNoteMus> ;
    skos:prefLabel "Chorpartitur"@de,
        "chorus score"@en,
        "partitura coral"@es,
        "partition de chœur"@fr,
        "合唱总谱"@zh ;
    skos:related <http://rdaregistry.info/termList/formatNoteMus/1011> .

<http://rdaregistry.info/termList/formatNoteMus/1011> a skos:Concept ;
    rdakit:toolkitDefinition "A format of notated music consisting of a score showing all vocal parts, with the instrumental accompaniment either omitted or arranged for a keyboard or other chordal instrument or instruments."@en,
        "Partitura que presenta todas las partes vocales, con el acompañamiento instrumental ya sea arreglado para teclados u otros instrumentos de cuerda u omitidos."@es,
        "Partition montrant toutes les parties vocales avec l’accompagnement arrangé pour un ou deux instruments à clavier ou autres instruments harmoniques ou sans l’accompagnement instrumental."@fr,
        "显示所有人声声部的乐谱，包括键盘或其他弦乐乐器的伴奏，伴奏部分也可能省略。"@zh ;
    rdakit:toolkitLabel "vocal score"@en,
        "partitura vocal"@es,
        "partition de chant"@fr,
        "声乐缩编谱"@zh ;
    reg:identifier <http://metadataregistry.org/concepts/1163> ;
    reg:status <http://metadataregistry.org/uri/RegStatus/1001> ;
    skos:definition "A format of notated music consisting of a score showing all vocal parts, with the instrumental accompaniment either omitted or arranged for a keyboard or other chordal instrument or instruments."@en,
        "Partitura que presenta todas las partes vocales, con el acompañamiento instrumental ya sea arreglado para teclados u otros instrumentos de cuerda u omitidos."@es,
        "Partition montrant toutes les parties vocales avec l’accompagnement arrangé pour un ou deux instruments à clavier ou autres instruments harmoniques ou sans l’accompagnement instrumental."@fr,
        "显示所有人声声部的乐谱，包括键盘或其他弦乐乐器的伴奏，伴奏部分也可能省略。"@zh ;
    skos:inScheme <http://rdaregistry.info/termList/formatNoteMus> ;
    skos:prefLabel "Gesangspartitur"@de,
        "vocal score"@en,
        "partitura vocal"@es,
        "partition de chant"@fr,
        "声乐缩编谱"@zh ;
    skos:related <http://rdaregistry.info/termList/formatNoteMus/1002> .

<http://metadataregistry.org/uri/RegStatus/1001> a skos:Concept ;
    skos:prefLabel "Published"@en .

<http://rdaregistry.info/termList/formatNoteMus> a skos:ConceptScheme ;
    dc:title "RDA Format of Notated Music" .

