@prefix dc: <http://purl.org/dc/elements/1.1/> .
@prefix rdakit: <http://metadataregistry.org/uri/profile/rdakit/> .
@prefix rdf: <http://www.w3.org/1999/02/22-rdf-syntax-ns#> .
@prefix rdfs: <http://www.w3.org/2000/01/rdf-schema#> .
@prefix reg: <http://metadataregistry.org/uri/profile/regap/> .
@prefix skos: <http://www.w3.org/2004/02/skos/core#> .
@prefix xml: <http://www.w3.org/XML/1998/namespace> .
@prefix xsd: <http://www.w3.org/2001/XMLSchema#> .

<http://rdaregistry.info/termList/noteMove/1001> a skos:Concept ;
    rdakit:toolkitDefinition "Eine Form der Bewegungsnotation für Tanz, die Musiknoten verwendet, um die Bewegungen der einzelnen Teile des Körpers darzustellen. Sie wird auf horizontalen neunzeiligen Notenlinien erfasst, die den Körper darstellen."@de,
        "A form of notated movement for dance using musical notation to represent movements by single parts of the body."@en,
        "Forma de movimiento notado para danza que utiliza notación musical para representar movimientos de partes individuales del cuerpo. Es registrado en un pentagrama horizontal de nueve líneas que representa el cuerpo."@es,
        "Forme de notation du mouvement pour la danse qui emploie la notation musicale pour décrire les mouvements des parties individuelles du corps. Cette notation utilise une portée horizontale de 9 lignes qui représente le corps."@fr,
        "Een vorm van bewegingsnotatie voor dans waarbij muzieknotatie gebruikt wordt om bewegingen voor te stellen per lichaamsdeel. Deze is vastgelegd op een horizontale balk van negen lijntjes, die het lichaam voorstelt."@nl,
        "一种用乐谱表示身体各部分运动的动作谱形式。它在水平方向的九条谱线上记录身体的表现。"@zh ;
    rdakit:toolkitLabel "Notation nach Stepanov"@de,
        "Stepanov dance notation"@en,
        "notación Stepanov para danza"@es,
        "Stepanov -tanssinotaatio"@fi,
        "notation Stepanov"@fr,
        "Notazione coreografica Stepanov"@it,
        "Stepanov dansnotatie"@nl,
        "斯捷潘诺夫舞谱"@zh ;
    reg:identifier <http://metadataregistry.org/concepts/1027> ;
    reg:status <http://metadataregistry.org/uri/RegStatus/1001> ;
    skos:definition "Eine Form der Bewegungsnotation für Tanz, die Musiknoten verwendet, um die Bewegungen der einzelnen Teile des Körpers darzustellen. Sie wird auf horizontalen neunzeiligen Notenlinien erfasst, die den Körper darstellen."@de,
        "A form of notated movement for dance using musical notation to represent movements by single parts of the body."@en,
        "Forma de movimiento notado para danza que utiliza notación musical para representar movimientos de partes individuales del cuerpo. Es registrado en un pentagrama horizontal de nueve líneas que representa el cuerpo."@es,
        "Forme de notation du mouvement pour la danse qui emploie la notation musicale pour décrire les mouvements des parties individuelles du corps. Cette notation utilise une portée horizontale de 9 lignes qui représente le corps."@fr,
        "Een vorm van bewegingsnotatie voor dans waarbij muzieknotatie gebruikt wordt om bewegingen voor te stellen per lichaamsdeel. Deze is vastgelegd op een horizontale balk van negen lijntjes, die het lichaam voorstelt."@nl,
        "一种用乐谱表示身体各部分运动的动作谱形式。它在水平方向的九条谱线上记录身体的表现。"@zh ;
    skos:inScheme <http://rdaregistry.info/termList/noteMove> ;
    skos:prefLabel "Notation nach Stepanov"@de,
        "Stepanov dance notation"@en,
        "notación Stepanov para danza"@es,
        "Stepanov -tanssinotaatio"@fi,
        "notation Stepanov"@fr,
        "Notazione coreografica Stepanov"@it,
        "Stepanov dansnotatie"@nl,
        "斯捷潘诺夫舞谱"@zh ;
    skos:scopeNote "It is recorded on a horizontal nine-line staff that represents the body."@en .

<http://rdaregistry.info/termList/noteMove/1004> a skos:Concept ;
    rdakit:toolkitDefinition "Eine Form der Bewegungsnotation, die taktische Bewegungen während eines Spiels wie zum Beispiel Schach aufzeichnet."@de,
        "A form of notated movement for recording the position of players or pieces during the course of a game."@en,
        "Forma de movimiento notado que registra los movimientos tácticos durante el curso de un juego, como el ajedrez."@es,
        "Forme de notation du mouvement servant à enregistrer les mouvements tactiques pendant le déroulement d’un jeu, comme les échecs."@fr,
        "Een vorm van bewegingsnotatie waarbij tactische zetten bijgehouden worden gedurende het verloop van een spel, zoals schaken."@nl,
        "在诸如下棋的游戏过程中记录战术步骤的动作谱形式。"@zh ;
    rdakit:toolkitLabel "Spielnotation"@de,
        "game play notation"@en,
        "notación de jugabilidad"@es,
        "pelinotaatio"@fi,
        "notation de jeu"@fr,
        "Notazione di gioco"@it,
        "Spelnotatie"@nl,
        "spelnotation"@sv,
        "游戏谱"@zh ;
    reg:identifier <http://metadataregistry.org/concepts/1030> ;
    reg:status <http://metadataregistry.org/uri/RegStatus/1001> ;
    skos:altLabel "Speldiagrammen"@nl ;
    skos:definition "Eine Form der Bewegungsnotation, die taktische Bewegungen während eines Spiels wie zum Beispiel Schach aufzeichnet."@de,
        "A form of notated movement for recording the position of players or pieces during the course of a game."@en,
        "Forma de movimiento notado que registra los movimientos tácticos durante el curso de un juego, como el ajedrez."@es,
        "Forme de notation du mouvement servant à enregistrer les mouvements tactiques pendant le déroulement d’un jeu, comme les échecs."@fr,
        "Een vorm van bewegingsnotatie waarbij tactische zetten bijgehouden worden gedurende het verloop van een spel, zoals schaken."@nl,
        "在诸如下棋的游戏过程中记录战术步骤的动作谱形式。"@zh ;
    skos:inScheme <http://rdaregistry.info/termList/noteMove> ;
    skos:prefLabel "Spielnotation"@de,
        "game play notation"@en,
        "notación de jugabilidad"@es,
        "pelinotaatio"@fi,
        "notation de jeu"@fr,
        "Notazione di gioco"@it,
        "Spelnotatie"@nl,
        "spelnotation"@sv,
        "游戏谱"@zh .

<http://rdaregistry.info/termList/noteMove/1005> a skos:Concept ;
    rdakit:toolkitDefinition "Eine Form der Bewegungsnotation, die ein sphärisches Koordinatensystem verwendet, um die Positionen des Körpers und der Gliedmaßen anzuzeigen. Sie wird auf einem Gitternetz erfasst, das den Körper darstellt."@de,
        "A form of notated movement using a spherical coordinate system to denote body and limb positions."@en,
        "Forma de movimiento notado que utiliza un sistema esférico coordinado para denotar las posiciones del cuerpo y las extremidades. Es registrado en una rejilla que representa el cuerpo."@es,
        "Forme de notation du mouvement qui emploie un système sphérique de coordonnées pour représenter les positions du corps et des membres. Le système utilise une grille qui représente le corps."@fr,
        "Een vorm van bewegingsnotatie waarbij een bolvormig coördinatensysteem gebruikt wordt om de positie van lichaam en ledematen voor te stellen. Deze is vastgelegd op een raster dat het lichaam voorstelt."@nl,
        "一种用球面坐标体系指出身体和四肢位置的动作谱形式。它在一个网格上记录身体的表现。"@zh ;
    rdakit:toolkitLabel "Eshkol-Wachmann-Notation"@de,
        "Eshkol-Wachman movement notation"@en,
        "notación de movimientos Eshkol-Wachman"@es,
        "Eshkol-Wachman-liikenotaatio"@fi,
        "notation Eshkol-Wachman"@fr,
        "Notazione di movimento Eshkol-Wachman"@it,
        "Eshkol-Wachman bewegingsnotatie"@nl,
        "Eshkol-Wachmnnotation"@sv,
        "埃什科尔-瓦克曼动作谱"@zh ;
    reg:identifier <http://metadataregistry.org/concepts/1031> ;
    reg:status <http://metadataregistry.org/uri/RegStatus/1001> ;
    skos:definition "Eine Form der Bewegungsnotation, die ein sphärisches Koordinatensystem verwendet, um die Positionen des Körpers und der Gliedmaßen anzuzeigen. Sie wird auf einem Gitternetz erfasst, das den Körper darstellt."@de,
        "A form of notated movement using a spherical coordinate system to denote body and limb positions."@en,
        "Forma de movimiento notado que utiliza un sistema esférico coordinado para denotar las posiciones del cuerpo y las extremidades. Es registrado en una rejilla que representa el cuerpo."@es,
        "Forme de notation du mouvement qui emploie un système sphérique de coordonnées pour représenter les positions du corps et des membres. Le système utilise une grille qui représente le corps."@fr,
        "Een vorm van bewegingsnotatie waarbij een bolvormig coördinatensysteem gebruikt wordt om de positie van lichaam en ledematen voor te stellen. Deze is vastgelegd op een raster dat het lichaam voorstelt."@nl,
        "一种用球面坐标体系指出身体和四肢位置的动作谱形式。它在一个网格上记录身体的表现。"@zh ;
    skos:inScheme <http://rdaregistry.info/termList/noteMove> ;
    skos:prefLabel "Eshkol-Wachmann-Notation"@de,
        "Eshkol-Wachman movement notation"@en,
        "notación de movimientos Eshkol-Wachman"@es,
        "Eshkol-Wachman-liikenotaatio"@fi,
        "notation Eshkol-Wachman"@fr,
        "Notazione di movimento Eshkol-Wachman"@it,
        "Eshkol-Wachman bewegingsnotatie"@nl,
        "Eshkol-Wachmnnotation"@sv,
        "埃什科尔-瓦克曼动作谱"@zh ;
    skos:scopeNote "It is recorded on a grid that represents the body."@en .

<http://rdaregistry.info/termList/noteMove/1006> a skos:Concept ;
    rdakit:toolkitDefinition "Eine Form der Bewegungsnotation, die figurative und abstrakte Symbole verwendet, um die Positionen des Körpers und der Gliedmaßen und die Bewegungen darzustellen. Sie wird auf fünfzeiligen horizontalen Notenlinien erfasst, die den Körper darstellen."@de,
        "A form of notated movement using figurative and abstract symbols to represent body and limb positions and movements."@en,
        "Forma de movimiento notado que utiliza símbolos figurativos y abstractos para representar posiciones y movimientos del cuerpo y las extremidades. Es registrado en un pentagrama horizontal de cinco líneas que representa el cuerpo."@es,
        "Forme de notation du mouvement qui emploie des symboles figuratifs et abstraits pour représenter les positions et les mouvements du corps et des membres. Cette notation utilise une portée horizontale de cinq lignes qui représente le corps."@fr,
        "Een vorm van bewegingsnotatie waarbij figuratieve en abstracte symbolen gebruikt worden om posities en bewegingen voor te stellen van lichaam en ledematen. Deze is vastgelegd op een horizontale balk van vijf lijntjes, die het lichaam voorstelt."@nl,
        "一种用形象的和抽象的符号表示身体和四肢位置及运动的动作谱形式。它在水平方向的五条谱线上记录身体的表现。"@zh ;
    rdakit:toolkitLabel "Sutton Dance-Writing"@de,
        "DanceWriting"@en,
        "DanceWriting"@es,
        "DanceWriting"@fi,
        "DanceWriting"@fr,
        "DanceWriting"@it,
        "DanceWriting"@nl,
        "[萨顿] 舞谱"@zh ;
    reg:identifier <http://metadataregistry.org/concepts/1032> ;
    reg:status <http://metadataregistry.org/uri/RegStatus/1001> ;
    skos:definition "Eine Form der Bewegungsnotation, die figurative und abstrakte Symbole verwendet, um die Positionen des Körpers und der Gliedmaßen und die Bewegungen darzustellen. Sie wird auf fünfzeiligen horizontalen Notenlinien erfasst, die den Körper darstellen."@de,
        "A form of notated movement using figurative and abstract symbols to represent body and limb positions and movements."@en,
        "Forma de movimiento notado que utiliza símbolos figurativos y abstractos para representar posiciones y movimientos del cuerpo y las extremidades. Es registrado en un pentagrama horizontal de cinco líneas que representa el cuerpo."@es,
        "Forme de notation du mouvement qui emploie des symboles figuratifs et abstraits pour représenter les positions et les mouvements du corps et des membres. Cette notation utilise une portée horizontale de cinq lignes qui représente le corps."@fr,
        "Een vorm van bewegingsnotatie waarbij figuratieve en abstracte symbolen gebruikt worden om posities en bewegingen voor te stellen van lichaam en ledematen. Deze is vastgelegd op een horizontale balk van vijf lijntjes, die het lichaam voorstelt."@nl,
        "一种用形象的和抽象的符号表示身体和四肢位置及运动的动作谱形式。它在水平方向的五条谱线上记录身体的表现。"@zh ;
    skos:inScheme <http://rdaregistry.info/termList/noteMove> ;
    skos:prefLabel "Sutton Dance-Writing"@de,
        "DanceWriting"@en,
        "DanceWriting"@es,
        "DanceWriting"@fi,
        "DanceWriting"@fr,
        "DanceWriting"@it,
        "DanceWriting"@nl,
        "[萨顿] 舞谱"@zh ;
    skos:scopeNote "It is recorded on a five-line horizontal staff that represents the body."@en .

<http://rdaregistry.info/termList/noteMove/1007> a skos:Concept ;
    rdakit:toolkitDefinition "Eine Form der Bewegungsnotation, die abstrakte Symbole verwendet, um die Positionen des Körpers und der Gliedmaßen darzustellen, wie sie von hinten zu sehen sind. Sie wird auf fünfzeiligen horizontalen Notenlinien erfasst, die den Körper darstellen."@de,
        "A form of notated movement using abstract symbols to represent body and limb positions as seen from the back."@en,
        "Forma de movimiento notado que utiliza símbolos abstractos para representar posiciones del cuerpo y miembros vistos desde atrás. Es registrado en un pentagrama horizontal de cinco líneas que representa el cuerpo."@es,
        "Forme de notation du mouvement qui emploie des symboles abstraits pour représenter les positions du corps et des membres vus de dos. Cette notation utilise une portée horizontale de cinq lignes qui représente le corps."@fr,
        "Een vorm van bewegingsnotatie waarbij abstracte symbolen gebruikt worden om de posities van lichaam en ledematen voor te stellen gezien vanaf de rug. Deze is vastgelegd op een horizontale balk van vijf lijntjes, die het lichaam voorstelt."@nl,
        "一种用抽象的符号表示从背后所看到的身体和四肢位置的动作谱形式。它在五条水平谱线上记录身体的表现。"@zh ;
    rdakit:toolkitLabel "Choreologie"@de,
        "Benesh movement notation"@en,
        "notación de movimientos Benesh"@es,
        "Benesh-liikenotaatio"@fi,
        "notation Benesh"@fr,
        "Notazione Benesh"@it,
        "Benesh bewegingsnotatie"@nl,
        "Beneshnotation"@sv,
        "班尼斯动作谱"@zh ;
    reg:identifier <http://metadataregistry.org/concepts/1033> ;
    reg:status <http://metadataregistry.org/uri/RegStatus/1001> ;
    skos:altLabel "Choreologie"@nl ;
    skos:definition "Eine Form der Bewegungsnotation, die abstrakte Symbole verwendet, um die Positionen des Körpers und der Gliedmaßen darzustellen, wie sie von hinten zu sehen sind. Sie wird auf fünfzeiligen horizontalen Notenlinien erfasst, die den Körper darstellen."@de,
        "A form of notated movement using abstract symbols to represent body and limb positions as seen from the back."@en,
        "Forma de movimiento notado que utiliza símbolos abstractos para representar posiciones del cuerpo y miembros vistos desde atrás. Es registrado en un pentagrama horizontal de cinco líneas que representa el cuerpo."@es,
        "Forme de notation du mouvement qui emploie des symboles abstraits pour représenter les positions du corps et des membres vus de dos. Cette notation utilise une portée horizontale de cinq lignes qui représente le corps."@fr,
        "Een vorm van bewegingsnotatie waarbij abstracte symbolen gebruikt worden om de posities van lichaam en ledematen voor te stellen gezien vanaf de rug. Deze is vastgelegd op een horizontale balk van vijf lijntjes, die het lichaam voorstelt."@nl,
        "一种用抽象的符号表示从背后所看到的身体和四肢位置的动作谱形式。它在五条水平谱线上记录身体的表现。"@zh ;
    skos:inScheme <http://rdaregistry.info/termList/noteMove> ;
    skos:prefLabel "Choreologie"@de,
        "Benesh movement notation"@en,
        "notación de movimientos Benesh"@es,
        "Benesh-liikenotaatio"@fi,
        "notation Benesh"@fr,
        "Notazione Benesh"@it,
        "Benesh bewegingsnotatie"@nl,
        "Beneshnotation"@sv,
        "班尼斯动作谱"@zh ;
    skos:scopeNote "It is recorded on a five-line horizontal staff that represents the body."@en .

<http://rdaregistry.info/termList/noteMove/1008> a skos:Concept ;
    rdakit:toolkitDefinition "Eine Form der Bewegungsnotation, die abstrakte Symbole verwendet, um die Bewegungen der Füße während einer damit in Verbindung stehenden Musikpassage darzustellen. Sie wird auf einer Spur erfasst, die den Weg des Tänzers auf dem Fußboden nachzeichnet."@de,
        "A form of notated movement using abstract symbols to represent movements of the feet during an associated passage of music."@en,
        "Forma de movimiento notado que utiliza símbolos abstractos para representar los movimientos del pie durante un pasaje asociado de música. Es registrado en un dibujo de pista que traza el camino del bailarín a lo largo del piso."@es,
        "Forme de notation du mouvement qui emploie des symboles abstraits pour représenter les mouvements des pieds pendant un passage de musique associé. Les mouvements sont notés à l’aide d’un dessin montrant le parcours du danseur sur le plancher."@fr,
        "Een vorm van bewegingsnotatie waarbij abstracte symbolen gebruikt worden om de bewegingen van de voeten voor te stellen gedurende een bijpassend stuk muziek. Deze is vastgelegd in een tekening die het spoor van de danser volgt over de vloer."@nl,
        "一种用抽象的符号表示与一段音乐相关的脚步运动的动作谱形式。它记录舞者在地面上的足迹或跨越的轨迹。"@zh ;
    rdakit:toolkitLabel "Beauchamp-Feuillet-Notation"@de,
        "Beauchamp-Feuillet notation"@en,
        "notación Beauchamp-Feuillet"@es,
        "Beauchamp-Feuillet-notaatio"@fi,
        "notation Beauchamp-Feuillet"@fr,
        "Notazione Beauchamp-Feuillet"@it,
        "Beauchamp-Feuillet notatie"@nl,
        "Feuilletnotation"@sv,
        "博尚-傅叶舞谱"@zh ;
    reg:identifier <http://metadataregistry.org/concepts/1034> ;
    reg:status <http://metadataregistry.org/uri/RegStatus/1001> ;
    skos:definition "Eine Form der Bewegungsnotation, die abstrakte Symbole verwendet, um die Bewegungen der Füße während einer damit in Verbindung stehenden Musikpassage darzustellen. Sie wird auf einer Spur erfasst, die den Weg des Tänzers auf dem Fußboden nachzeichnet."@de,
        "A form of notated movement using abstract symbols to represent movements of the feet during an associated passage of music."@en,
        "Forma de movimiento notado que utiliza símbolos abstractos para representar los movimientos del pie durante un pasaje asociado de música. Es registrado en un dibujo de pista que traza el camino del bailarín a lo largo del piso."@es,
        "Forme de notation du mouvement qui emploie des symboles abstraits pour représenter les mouvements des pieds pendant un passage de musique associé. Les mouvements sont notés à l’aide d’un dessin montrant le parcours du danseur sur le plancher."@fr,
        "Een vorm van bewegingsnotatie waarbij abstracte symbolen gebruikt worden om de bewegingen van de voeten voor te stellen gedurende een bijpassend stuk muziek. Deze is vastgelegd in een tekening die het spoor van de danser volgt over de vloer."@nl,
        "一种用抽象的符号表示与一段音乐相关的脚步运动的动作谱形式。它记录舞者在地面上的足迹或跨越的轨迹。"@zh ;
    skos:inScheme <http://rdaregistry.info/termList/noteMove> ;
    skos:prefLabel "Beauchamp-Feuillet-Notation"@de,
        "Beauchamp-Feuillet notation"@en,
        "notación Beauchamp-Feuillet"@es,
        "Beauchamp-Feuillet-notaatio"@fi,
        "notation Beauchamp-Feuillet"@fr,
        "Notazione Beauchamp-Feuillet"@it,
        "Beauchamp-Feuillet notatie"@nl,
        "Feuilletnotation"@sv,
        "博尚-傅叶舞谱"@zh ;
    skos:scopeNote "It is recorded on a track drawing that traces the path of the dancer across the floor."@en .

<http://rdaregistry.info/termList/noteMove/1009> a skos:Concept ;
    rdakit:toolkitDefinition "Eine Form der Bewegungsnotation, die abstrakte Symbole verwendet, um die Positionen des Körpers und der Gliedmaßen und die Bewegungen darzustellen. Sie wird auf getrennten vertikalen Linien erfasst, die die Arme, Beine und den Körper darstellen."@de,
        "A form of notated movement using abstract symbols to represent body and limb positions and movements."@en,
        "Forma de movimiento notado que utiliza símbolos abstractos para representar las posiciones y los movimientos del cuerpo y las extremidades. Se registra en un pentagrama vertical que representa los brazos, las piernas y el tronco."@es,
        "Forme de notation du mouvement qui emploie des symboles abstraits pour représenter les positions et les mouvements du corps et des membres. Cette notation utilise des portées verticales séparées représentant les bras, les jambes et le tronc."@fr,
        "Een vorm van bewegingsnotatie waarbij abstracte symbolen gebruikt worden om posities en bewegingen voor te stellen van lichaam en ledematen. Deze is vastgelegd op aparte verticale balken voor armen, benen en romp."@nl,
        "一种用抽象的符号表示身体和四肢位置及运动的动作谱形式。它在不同的垂直谱线上分别记录上肢、下肢和躯干的表现。"@zh ;
    rdakit:toolkitLabel "Action Stroke Dance Notation"@de,
        "action stroke dance notation"@en,
        "notación de movimientos para danza"@es,
        "action stroke dance notation"@fi,
        "Notazione coreografica Action Stroke"@it,
        "Action Stroke Dance-notatie"@nl,
        "动作分解舞谱"@zh ;
    reg:identifier <http://metadataregistry.org/concepts/1035> ;
    reg:status <http://metadataregistry.org/uri/RegStatus/1001> ;
    skos:definition "Eine Form der Bewegungsnotation, die abstrakte Symbole verwendet, um die Positionen des Körpers und der Gliedmaßen und die Bewegungen darzustellen. Sie wird auf getrennten vertikalen Linien erfasst, die die Arme, Beine und den Körper darstellen."@de,
        "A form of notated movement using abstract symbols to represent body and limb positions and movements."@en,
        "Forma de movimiento notado que utiliza símbolos abstractos para representar las posiciones y los movimientos del cuerpo y las extremidades. Se registra en un pentagrama vertical que representa los brazos, las piernas y el tronco."@es,
        "Forme de notation du mouvement qui emploie des symboles abstraits pour représenter les positions et les mouvements du corps et des membres. Cette notation utilise des portées verticales séparées représentant les bras, les jambes et le tronc."@fr,
        "notation de la danse par traits d’action"@fr,
        "Een vorm van bewegingsnotatie waarbij abstracte symbolen gebruikt worden om posities en bewegingen voor te stellen van lichaam en ledematen. Deze is vastgelegd op aparte verticale balken voor armen, benen en romp."@nl,
        "一种用抽象的符号表示身体和四肢位置及运动的动作谱形式。它在不同的垂直谱线上分别记录上肢、下肢和躯干的表现。"@zh ;
    skos:inScheme <http://rdaregistry.info/termList/noteMove> ;
    skos:prefLabel "Action Stroke Dance Notation"@de,
        "action stroke dance notation"@en,
        "notación de movimientos para danza"@es,
        "action stroke dance notation"@fi,
        "Notazione coreografica Action Stroke"@it,
        "Action Stroke Dance-notatie"@nl,
        "动作分解舞谱"@zh ;
    skos:scopeNote "It is recorded on separate vertical staffs representing the arms, legs, and trunk."@en .

<http://rdaregistry.info/termList/noteMove/1002> a skos:Concept ;
    rdakit:toolkitDefinition "Eine Form der Bewegungsnotation, die abstrakte Symbole verwendet, um die Positionen des Körpers und der Gliedmaßen darzustellen, wie sie von hinten zu sehen sind. Sie wird auf vertikalen dreizeiligen Notenlinien erfasst, die den Körper darstellen. Ähnlich wie Kinetografie Laban."@de,
        "A form of notated movement using abstract symbols on a vertical three-line staff to represent movement of the body and limbs as seen from the back, developed in the United States and the United Kingdom in the middle of the 20th century."@en,
        "Forma de movimiento notado que utiliza símbolos abstractos para representar el movimiento del cuerpo y extremidades vistos desde atrás. Se registra en un pentagrama vertical de tres líneas que representa el cuerpo. Similar a la Kinetografía Laban."@es,
        "Forme de notation du mouvement qui emploie des symboles abstraits pour représenter les mouvements du corps et des membres vus de dos. Cette notation utilise une portée verticale de trois lignes qui représente le corps. Similaire à la Cinétographie Laban."@fr,
        "Een vorm van bewegingsnotatie waarbij abstracte symbolen gebruikt worden om beweging voor te stellen van lichaam en ledematen gezien vanaf de rug. Deze is vastgelegd op een verticale balk van drie lijntjes, die het lichaam voorstelt. Gebaseerd op Kinetography Laban."@nl,
        "一种用抽象的符号表示从背后所看到的身体和四肢运动的动作谱形式。它在垂直的三条谱线上记录身体的表现，与拉班书面舞谱类似。"@zh ;
    rdakit:toolkitLabel "Labanotation"@de,
        "Labanotation"@en,
        "Labanotación"@es,
        "Laban-notaatio"@fi,
        "Labanotation"@fr,
        "Notazione Laban"@it,
        "Labannotatie"@nl,
        "labanotation"@sv,
        "拉班舞谱"@zh ;
    reg:identifier <http://metadataregistry.org/concepts/1028> ;
    reg:status <http://metadataregistry.org/uri/RegStatus/1001> ;
    skos:altLabel "Labanotatie"@nl ;
    skos:definition "Eine Form der Bewegungsnotation, die abstrakte Symbole verwendet, um die Positionen des Körpers und der Gliedmaßen darzustellen, wie sie von hinten zu sehen sind. Sie wird auf vertikalen dreizeiligen Notenlinien erfasst, die den Körper darstellen. Ähnlich wie Kinetografie Laban."@de,
        "A form of notated movement using abstract symbols on a vertical three-line staff to represent movement of the body and limbs as seen from the back, developed in the United States and the United Kingdom in the middle of the 20th century."@en,
        "Forma de movimiento notado que utiliza símbolos abstractos para representar el movimiento del cuerpo y extremidades vistos desde atrás. Se registra en un pentagrama vertical de tres líneas que representa el cuerpo. Similar a la Kinetografía Laban."@es,
        "Forme de notation du mouvement qui emploie des symboles abstraits pour représenter les mouvements du corps et des membres vus de dos. Cette notation utilise une portée verticale de trois lignes qui représente le corps. Similaire à la Cinétographie Laban."@fr,
        "Een vorm van bewegingsnotatie waarbij abstracte symbolen gebruikt worden om beweging voor te stellen van lichaam en ledematen gezien vanaf de rug. Deze is vastgelegd op een verticale balk van drie lijntjes, die het lichaam voorstelt. Gebaseerd op Kinetography Laban."@nl,
        "一种用抽象的符号表示从背后所看到的身体和四肢运动的动作谱形式。它在垂直的三条谱线上记录身体的表现，与拉班书面舞谱类似。"@zh ;
    skos:inScheme <http://rdaregistry.info/termList/noteMove> ;
    skos:note "与拉班书面舞谱类似。"@zh ;
    skos:prefLabel "Labanotation"@de,
        "Labanotation"@en,
        "Labanotación"@es,
        "Laban-notaatio"@fi,
        "Labanotation"@fr,
        "Notazione Laban"@it,
        "Labannotatie"@nl,
        "labanotation"@sv,
        "拉班舞谱"@zh ;
    skos:related <http://rdaregistry.info/termList/noteMove/1010> ;
    skos:scopeNote "Labanotation is now harmonized with, while remaining distinct from, Kineography Laban."@en,
        "与拉班书面舞谱类似。"@zh .

<http://rdaregistry.info/termList/noteMove/1010> a skos:Concept ;
    rdakit:toolkitDefinition "Eine Form der Bewegungsnotation, die abstrakte Symbole verwendet, um die Positionen des Körpers und der Gliedmaßen darzustellen, wie sie von hinten zu sehen sind. Sie wird auf vertikalen dreizeiligen Notenlinien erfasst, die den Körper darstellen. Ähnlich wie Labanotation."@de,
        "A form of notated movement using abstract symbols on a vertical three-line staff to represent movement of the body and limbs as seen from the back, developed in Europe in the middle of the 20th century."@en,
        "Forma de movimiento notado que utiliza símbolos abstractos para representar el movimiento del cuerpo y extremidades vistos desde atrás. Se registra en un pentagrama vertical de tres líneas que representa el cuerpo. Similar a la Labanotación."@es,
        "Forme de notation du mouvement qui emploie des symboles abstraits pour représenter les mouvements du corps et des membres vus de dos. Cette notation utilise une portée verticale de trois lignes qui représente le corps. Similaire à la Labanotation."@fr,
        "Een vorm van bewegingsnotatie waarbij abstracte symbolen gebruikt worden om bewegingen voor te stellen van lichaam en ledematen vanaf de rug. Deze is vastgelegd op een verticale balk van drie lijntjes, die het lichaam voorstelt. Vergelijkbaar met Labanotation."@nl,
        "一种用抽象的符号表示从背后所看到的身体和四肢运动的动作谱形式。它在垂直的三条谱线上记录身体的表现，与拉班舞谱类似。"@zh ;
    rdakit:toolkitLabel "Kinetography Laban"@de,
        "Kinetography Laban"@en,
        "Kinetografía Laban"@es,
        "Kinetography Laban -notaatio"@fi,
        "Cinétographie Laban"@fr,
        "Cinetografia Laban"@it,
        "Kinetography Laban"@nl,
        "拉班书面舞谱"@zh ;
    reg:identifier <http://metadataregistry.org/concepts/5924> ;
    reg:status <http://metadataregistry.org/uri/RegStatus/1001> ;
    skos:definition "Eine Form der Bewegungsnotation, die abstrakte Symbole verwendet, um die Positionen des Körpers und der Gliedmaßen darzustellen, wie sie von hinten zu sehen sind. Sie wird auf vertikalen dreizeiligen Notenlinien erfasst, die den Körper darstellen. Ähnlich wie Labanotation."@de,
        "A form of notated movement using abstract symbols on a vertical three-line staff to represent movement of the body and limbs as seen from the back, developed in Europe in the middle of the 20th century."@en,
        "Forma de movimiento notado que utiliza símbolos abstractos para representar el movimiento del cuerpo y extremidades vistos desde atrás. Se registra en un pentagrama vertical de tres líneas que representa el cuerpo. Similar a la Labanotación."@es,
        "Forme de notation du mouvement qui emploie des symboles abstraits pour représenter les mouvements du corps et des membres vus de dos. Cette notation utilise une portée verticale de trois lignes qui représente le corps. Similaire à la Labanotation."@fr,
        "Een vorm van bewegingsnotatie waarbij abstracte symbolen gebruikt worden om bewegingen voor te stellen van lichaam en ledematen vanaf de rug. Deze is vastgelegd op een verticale balk van drie lijntjes, die het lichaam voorstelt. Vergelijkbaar met Labanotation."@nl,
        "一种用抽象的符号表示从背后所看到的身体和四肢运动的动作谱形式。它在垂直的三条谱线上记录身体的表现，与拉班舞谱类似。"@zh ;
    skos:inScheme <http://rdaregistry.info/termList/noteMove> ;
    skos:note "与拉班舞谱类似。"@zh ;
    skos:prefLabel "Kinetography Laban"@de,
        "Kinetography Laban"@en,
        "Kinetografía Laban"@es,
        "Kinetography Laban -notaatio"@fi,
        "Cinétographie Laban"@fr,
        "Cinetografia Laban"@it,
        "Kinetography Laban"@nl,
        "拉班书面舞谱"@zh ;
    skos:related <http://rdaregistry.info/termList/noteMove/1002> ;
    skos:scopeNote "Kineography Laban is now harmonized with, while remaining distinct from, Labanotation."@en,
        "与拉班舞谱类似。"@zh .

<http://metadataregistry.org/uri/RegStatus/1001> a skos:Concept ;
    skos:prefLabel "Published"@en .

<http://rdaregistry.info/termList/noteMove> a skos:ConceptScheme ;
    dc:title "RDA Form of Notated Movement" .

