@prefix rdf: <http://www.w3.org/1999/02/22-rdf-syntax-ns#> .
@prefix dc: <http://purl.org/dc/elements/1.1/> .
@prefix foaf: <http://xmlns.com/foaf/0.1/> .
@prefix owl: <http://www.w3.org/2002/07/owl#> .
@prefix rdakit: <http://metadataregistry.org/uri/profile/rdakit/> .
@prefix rdfs: <http://www.w3.org/2000/01/rdf-schema#> .
@prefix reg: <http://metadataregistry.org/uri/profile/regap/> .
@prefix skos: <http://www.w3.org/2004/02/skos/core#> .

<http://metadataregistry.org/uri/RegStatus/1001>
    a skos:Concept ;
    skos:prefLabel "Published"@en .

<http://metadataregistry.org/uri/RegStatus/1008>
    a skos:Concept ;
    skos:prefLabel "Deprecated"@en .

<http://rdaregistry.info/Elements/u/>
    dc:title "RDA Unconstrained properties"@en ;
    skos:note "Properties derived from RDA elements and relationship designators without specific or implicit restrictions to RDA entities."@en ;
    foaf:homepage <http://www.rdaregistry.info/Elements/u/> .

<http://rdaregistry.info/Elements/u/P60001>
    reg:hasSubproperty <http://rdaregistry.info/Elements/a/P50001> ;
    reg:lexicalAlias <http://rdaregistry.info/Elements/u/respondentOf.en> ;
    reg:name "respondentOf"@en ;
    reg:status <http://metadataregistry.org/uri/RegStatus/1001> ;
    a rdf:Property ;
    rdfs:isDefinedBy <http://rdaregistry.info/Elements/u/> ;
    rdfs:label "is respondent of"@en ;
    rdfs:subPropertyOf <http://rdaregistry.info/Elements/u/P60672> ;
    owl:inverseOf <http://rdaregistry.info/Elements/u/P60045> ;
    skos:definition "Relates a candidate for a degree who defends or opposes a thesis provided by a praeses in an academic disputation to a resource."@en .

<http://rdaregistry.info/Elements/u/P60002>
    reg:hasSubproperty <http://rdaregistry.info/Elements/a/P50003> ;
    reg:lexicalAlias <http://rdaregistry.info/Elements/u/degreeGrantingInstitutionOf.en> ;
    reg:name "degreeGrantingInstitutionOf"@en ;
    reg:status <http://metadataregistry.org/uri/RegStatus/1001> ;
    a rdf:Property ;
    rdfs:isDefinedBy <http://rdaregistry.info/Elements/u/> ;
    rdfs:label "is degree granting institution of"@en ;
    rdfs:subPropertyOf <http://rdaregistry.info/Elements/u/P60602> ;
    owl:inverseOf <http://rdaregistry.info/Elements/u/P60060> ;
    skos:definition "Relates an agent granting an academic degree to a resource."@en .

<http://rdaregistry.info/Elements/u/P60003>
    reg:hasSubproperty <http://rdaregistry.info/Elements/a/P50004> ;
    reg:lexicalAlias <http://rdaregistry.info/Elements/u/hostInstitutionOf.en> ;
    reg:name "hostInstitutionOf"@en ;
    reg:status <http://metadataregistry.org/uri/RegStatus/1001> ;
    a rdf:Property ;
    rdfs:isDefinedBy <http://rdaregistry.info/Elements/u/> ;
    rdfs:label "is host institution of"@en ;
    rdfs:subPropertyOf <http://rdaregistry.info/Elements/u/P60602> ;
    owl:inverseOf <http://rdaregistry.info/Elements/u/P60061> ;
    skos:definition "Relates an agent hosting an event, exhibit, conference, etc., which gave rise to a resource to a resource."@en .

<http://rdaregistry.info/Elements/u/P60004>
    reg:hasSubproperty <http://rdaregistry.info/Elements/a/P50005> ;
    reg:lexicalAlias <http://rdaregistry.info/Elements/u/productionCompanyOf.en> ;
    reg:name "productionCompanyOf"@en ;
    reg:status <http://metadataregistry.org/uri/RegStatus/1001> ;
    a rdf:Property ;
    rdfs:isDefinedBy <http://rdaregistry.info/Elements/u/> ;
    rdfs:label "is production company of"@en ;
    rdfs:subPropertyOf <http://rdaregistry.info/Elements/u/P60602> ;
    owl:inverseOf <http://rdaregistry.info/Elements/u/P60062> ;
    skos:definition "Relates an agent that is responsible for financial, technical, and organizational management of a production for stage, screen, sound recording, television, webcast, etc. to a resource."@en .

<http://rdaregistry.info/Elements/u/P60005>
    reg:hasSubproperty <http://rdaregistry.info/Elements/a/P50044> ;
    reg:lexicalAlias <http://rdaregistry.info/Elements/u/courtGovernedOf.en> ;
    reg:name "courtGovernedOf"@en ;
    reg:status <http://metadataregistry.org/uri/RegStatus/1001> ;
    a rdf:Property ;
    rdfs:isDefinedBy <http://rdaregistry.info/Elements/u/> ;
    rdfs:label "is court governed of"@en ;
    rdfs:subPropertyOf <http://rdaregistry.info/Elements/u/P60602> ;
    owl:inverseOf <http://rdaregistry.info/Elements/u/P60065> ;
    skos:definition "Relates a court governed by court rules, regardless of their official nature to a resource."@en .

<http://rdaregistry.info/Elements/u/P60006>
    reg:hasSubproperty <http://rdaregistry.info/Elements/a/P50045> ;
    reg:lexicalAlias <http://rdaregistry.info/Elements/u/collectorOf.en> ;
    reg:name "collectorOf"@en ;
    reg:status <http://metadataregistry.org/uri/RegStatus/1001> ;
    a rdf:Property ;
    rdfs:isDefinedBy <http://rdaregistry.info/Elements/u/> ;
    rdfs:label "is collector of"@en ;
    rdfs:subPropertyOf <http://rdaregistry.info/Elements/u/P60604> ;
    owl:inverseOf <http://rdaregistry.info/Elements/u/P60066> ;
    skos:definition "Relates a curator who brings together resources from various sources that are then arranged, described, and cataloged as a collection to a resource."@en .

<http://rdaregistry.info/Elements/u/P60007>
    reg:hasSubproperty <http://rdaregistry.info/Elements/a/P50046> ;
    reg:lexicalAlias <http://rdaregistry.info/Elements/u/collectionRegistrarOf.en> ;
    reg:name "collectionRegistrarOf"@en ;
    reg:status <http://metadataregistry.org/uri/RegStatus/1001> ;
    a rdf:Property ;
    rdfs:isDefinedBy <http://rdaregistry.info/Elements/u/> ;
    rdfs:label "is collection registrar of"@en ;
    rdfs:subPropertyOf <http://rdaregistry.info/Elements/u/P60604> ;
    owl:inverseOf <http://rdaregistry.info/Elements/u/P60067> ;
    skos:definition "Relates a curator who lists or inventories resources in an aggregate resource such as a collection of resources to a resource."@en .

<http://rdaregistry.info/Elements/u/P60008>
    reg:hasSubproperty <http://rdaregistry.info/Elements/a/P50047> ;
    reg:lexicalAlias <http://rdaregistry.info/Elements/u/depositorOf.en> ;
    reg:name "depositorOf"@en ;
    reg:status <http://metadataregistry.org/uri/RegStatus/1001> ;
    a rdf:Property ;
    rdfs:isDefinedBy <http://rdaregistry.info/Elements/u/> ;
    rdfs:label "is depositor of"@en ;
    rdfs:subPropertyOf <http://rdaregistry.info/Elements/u/P60628> ;
    owl:inverseOf <http://rdaregistry.info/Elements/u/P60068> ;
    skos:definition "Relates a current owner of a resource who deposited a resource into the custody of another agent, while still retaining ownership to a resource."@en .

<http://rdaregistry.info/Elements/u/P60009>
    reg:hasSubproperty <http://rdaregistry.info/Elements/a/P50048> ;
    reg:lexicalAlias <http://rdaregistry.info/Elements/u/filmDirectorOf.en> ;
    reg:name "filmDirectorOf"@en ;
    reg:status <http://metadataregistry.org/uri/RegStatus/1001> ;
    a rdf:Property ;
    rdfs:isDefinedBy <http://rdaregistry.info/Elements/u/> ;
    rdfs:label "is film director of"@en ;
    rdfs:subPropertyOf <http://rdaregistry.info/Elements/u/P60673> ;
    owl:inverseOf <http://rdaregistry.info/Elements/u/P60084> ;
    skos:definition "Relates a director responsible for the general management and supervision of a filmed performance to a resource."@en .

<http://rdaregistry.info/Elements/u/P60010>
    reg:hasSubproperty <http://rdaregistry.info/Elements/a/P50049> ;
    reg:lexicalAlias <http://rdaregistry.info/Elements/u/radioDirectorOf.en> ;
    reg:name "radioDirectorOf"@en ;
    reg:status <http://metadataregistry.org/uri/RegStatus/1001> ;
    a rdf:Property ;
    rdfs:isDefinedBy <http://rdaregistry.info/Elements/u/> ;
    rdfs:label "is radio director of"@en ;
    rdfs:subPropertyOf <http://rdaregistry.info/Elements/u/P60673> ;
    owl:inverseOf <http://rdaregistry.info/Elements/u/P60085> ;
    skos:definition "Relates a director responsible for the general management and supervision of a radio program to a resource."@en .

<http://rdaregistry.info/Elements/u/P60011>
    reg:hasSubproperty <http://rdaregistry.info/Elements/a/P50050> ;
    reg:lexicalAlias <http://rdaregistry.info/Elements/u/televisionDirectorOf.en> ;
    reg:name "televisionDirectorOf"@en ;
    reg:status <http://metadataregistry.org/uri/RegStatus/1001> ;
    a rdf:Property ;
    rdfs:isDefinedBy <http://rdaregistry.info/Elements/u/> ;
    rdfs:label "is television director of"@en ;
    rdfs:subPropertyOf <http://rdaregistry.info/Elements/u/P60673> ;
    owl:inverseOf <http://rdaregistry.info/Elements/u/P60086> ;
    skos:definition "Relates a director responsible for the general management and supervision of a television program to a resource."@en .

<http://rdaregistry.info/Elements/u/P60012>
    reg:hasSubproperty <http://rdaregistry.info/Elements/a/P50066> ;
    reg:lexicalAlias <http://rdaregistry.info/Elements/u/donorOf.en> ;
    reg:name "donorOf"@en ;
    reg:status <http://metadataregistry.org/uri/RegStatus/1001> ;
    a rdf:Property ;
    rdfs:isDefinedBy <http://rdaregistry.info/Elements/u/> ;
    rdfs:label "is donor of"@en ;
    rdfs:subPropertyOf <http://rdaregistry.info/Elements/u/P60630> ;
    owl:inverseOf <http://rdaregistry.info/Elements/u/P60091> ;
    skos:definition "Relates a former owner of a resource who donated that resource to another owner to a resource."@en .

<http://rdaregistry.info/Elements/u/P60013>
    reg:hasSubproperty <http://rdaregistry.info/Elements/a/P50067> ;
    reg:lexicalAlias <http://rdaregistry.info/Elements/u/sellerOf.en> ;
    reg:name "sellerOf"@en ;
    reg:status <http://metadataregistry.org/uri/RegStatus/1001> ;
    a rdf:Property ;
    rdfs:isDefinedBy <http://rdaregistry.info/Elements/u/> ;
    rdfs:label "is seller of"@en ;
    rdfs:subPropertyOf <http://rdaregistry.info/Elements/u/P60630> ;
    owl:inverseOf <http://rdaregistry.info/Elements/u/P60092> ;
    skos:definition "Relates a former owner of a resource who sold that resource to another owner to a resource."@en .

<http://rdaregistry.info/Elements/u/P60014>
    reg:hasSubproperty <http://rdaregistry.info/Elements/a/P50068> ;
    reg:lexicalAlias <http://rdaregistry.info/Elements/u/enactingJurisdictionOf.en> ;
    reg:name "enactingJurisdictionOf"@en ;
    reg:status <http://metadataregistry.org/uri/RegStatus/1001> ;
    a rdf:Property ;
    rdfs:isDefinedBy <http://rdaregistry.info/Elements/u/> ;
    rdfs:label "is enacting jurisdiction of"@en ;
    rdfs:subPropertyOf <http://rdaregistry.info/Elements/u/P60672> ;
    owl:inverseOf <http://rdaregistry.info/Elements/u/P60096> ;
    skos:definition "Relates a jurisdiction enacting a law, regulation, constitution, court rule, etc. to a resource."@en .

<http://rdaregistry.info/Elements/u/P60015>
    reg:hasSubproperty <http://rdaregistry.info/Elements/a/P50069> ;
    reg:lexicalAlias <http://rdaregistry.info/Elements/u/jurisdictionGovernedOf.en> ;
    reg:name "jurisdictionGovernedOf"@en ;
    reg:status <http://metadataregistry.org/uri/RegStatus/1001> ;
    a rdf:Property ;
    rdfs:isDefinedBy <http://rdaregistry.info/Elements/u/> ;
    rdfs:label "is jurisdiction governed of"@en ;
    rdfs:subPropertyOf <http://rdaregistry.info/Elements/u/P60602> ;
    owl:inverseOf <http://rdaregistry.info/Elements/u/P60097> ;
    skos:definition "Relates a jurisdiction governed by a law, regulation, etc., that was enacted by another jurisdiction to a resource."@en .

<http://rdaregistry.info/Elements/u/P60016>
    reg:hasSubproperty <http://rdaregistry.info/Elements/a/P50070>, <http://rdaregistry.info/Elements/u/P60843>, <http://rdaregistry.info/Elements/u/P60845> ;
    reg:lexicalAlias <http://rdaregistry.info/Elements/u/conductorOf.en> ;
    reg:name "conductorOf"@en ;
    reg:status <http://metadataregistry.org/uri/RegStatus/1001> ;
    a rdf:Property ;
    rdfs:isDefinedBy <http://rdaregistry.info/Elements/u/> ;
    rdfs:label "is conductor of"@en ;
    rdfs:subPropertyOf <http://rdaregistry.info/Elements/u/P60615> ;
    owl:inverseOf <http://rdaregistry.info/Elements/u/P60141> ;
    skos:definition "Relates a performer contributing to a musical resource by leading a performing group in a musical or dramatic presentation, etc. to a resource."@en .

<http://rdaregistry.info/Elements/u/P60017>
    reg:hasSubproperty <http://rdaregistry.info/Elements/a/P50071>, <http://rdaregistry.info/Elements/u/P60027> ;
    reg:lexicalAlias <http://rdaregistry.info/Elements/u/actorOf.en> ;
    reg:name "actorOf"@en ;
    reg:status <http://metadataregistry.org/uri/RegStatus/1001> ;
    a rdf:Property ;
    rdfs:isDefinedBy <http://rdaregistry.info/Elements/u/> ;
    rdfs:label "is actor of"@en ;
    rdfs:subPropertyOf <http://rdaregistry.info/Elements/u/P60615> ;
    owl:inverseOf <http://rdaregistry.info/Elements/u/P60142> ;
    skos:definition "Relates a performer contributing to a resource by acting as a cast member or player in a musical or dramatic presentation, etc. to a resource."@en .

<http://rdaregistry.info/Elements/u/P60018>
    rdakit:seeAlso <http://rdaregistry.info/Elements/u/P60825> ;
    reg:hasSubproperty <http://rdaregistry.info/Elements/a/P50072> ;
    reg:lexicalAlias <http://rdaregistry.info/Elements/u/onScreenPresenterOf.en> ;
    reg:name "onScreenPresenterOf"@en ;
    reg:status <http://metadataregistry.org/uri/RegStatus/1001> ;
    a rdf:Property ;
    rdfs:isDefinedBy <http://rdaregistry.info/Elements/u/> ;
    rdfs:label "is on-screen presenter of"@en ;
    rdfs:subPropertyOf <http://rdaregistry.info/Elements/u/P60615> ;
    owl:inverseOf <http://rdaregistry.info/Elements/u/P60143> ;
    skos:definition "Relates a performer contributing to a resource by appearing on screen to provide contextual or background information. an on-screen presenter may appear in nonfiction moving image materials or in introductions to fiction moving image materials to a resource."@en ;
    skos:scopeNote "Appearance in nonfiction moving image materials or in introductions to fiction moving image materials is included. Appearance on screen in a non-performing role is excluded."@en .

<http://rdaregistry.info/Elements/u/P60019>
    reg:hasSubproperty <http://rdaregistry.info/Elements/a/P50073> ;
    reg:lexicalAlias <http://rdaregistry.info/Elements/u/dancerOf.en> ;
    reg:name "dancerOf"@en ;
    reg:status <http://metadataregistry.org/uri/RegStatus/1001> ;
    a rdf:Property ;
    rdfs:isDefinedBy <http://rdaregistry.info/Elements/u/> ;
    rdfs:label "is dancer of"@en ;
    rdfs:subPropertyOf <http://rdaregistry.info/Elements/u/P60615> ;
    owl:inverseOf <http://rdaregistry.info/Elements/u/P60144> ;
    skos:definition "Relates a performer contributing to a resource by dancing in a musical, dramatic, etc., presentation to a resource."@en .

<http://rdaregistry.info/Elements/u/P60020>
    reg:hasSubproperty <http://rdaregistry.info/Elements/a/P50074> ;
    reg:lexicalAlias <http://rdaregistry.info/Elements/u/teacherOf.en> ;
    reg:name "teacherOf"@en ;
    reg:status <http://metadataregistry.org/uri/RegStatus/1001> ;
    a rdf:Property ;
    rdfs:isDefinedBy <http://rdaregistry.info/Elements/u/> ;
    rdfs:label "is teacher of"@en ;
    rdfs:subPropertyOf <http://rdaregistry.info/Elements/u/P60615> ;
    owl:inverseOf <http://rdaregistry.info/Elements/u/P60145> ;
    skos:definition "Relates a performer contributing to a resource by giving instruction or providing a demonstration to a resource."@en .

<http://rdaregistry.info/Elements/u/P60021>
    reg:hasSubproperty <http://rdaregistry.info/Elements/a/P50075> ;
    reg:lexicalAlias <http://rdaregistry.info/Elements/u/hostOf.en> ;
    reg:name "hostOf"@en ;
    reg:status <http://metadataregistry.org/uri/RegStatus/1001> ;
    a rdf:Property ;
    rdfs:isDefinedBy <http://rdaregistry.info/Elements/u/> ;
    rdfs:label "is host of"@en ;
    rdfs:subPropertyOf <http://rdaregistry.info/Elements/u/P60615> ;
    owl:inverseOf <http://rdaregistry.info/Elements/u/P60146> ;
    skos:definition "Relates a performer contributing to a resource by leading a program, often broadcast, that includes other guests, performers, etc., to a resource."@en .

<http://rdaregistry.info/Elements/u/P60022>
    reg:hasSubproperty <http://rdaregistry.info/Elements/a/P50076> ;
    reg:lexicalAlias <http://rdaregistry.info/Elements/u/moderatorOf.en> ;
    reg:name "moderatorOf"@en ;
    reg:status <http://metadataregistry.org/uri/RegStatus/1001> ;
    a rdf:Property ;
    rdfs:isDefinedBy <http://rdaregistry.info/Elements/u/> ;
    rdfs:label "is moderator of"@en ;
    rdfs:subPropertyOf <http://rdaregistry.info/Elements/u/P60615> ;
    owl:inverseOf <http://rdaregistry.info/Elements/u/P60147> ;
    skos:definition "Relates a performer contributing to a resource by leading a program, often broadcast, where topics are discussed, usually with participation of experts in fields related to the discussion to a resource."@en .

<http://rdaregistry.info/Elements/u/P60023>
    reg:hasSubproperty <http://rdaregistry.info/Elements/a/P50077> ;
    reg:lexicalAlias <http://rdaregistry.info/Elements/u/puppeteerOf.en> ;
    reg:name "puppeteerOf"@en ;
    reg:status <http://metadataregistry.org/uri/RegStatus/1001> ;
    a rdf:Property ;
    rdfs:isDefinedBy <http://rdaregistry.info/Elements/u/> ;
    rdfs:label "is puppeteer of"@en ;
    rdfs:subPropertyOf <http://rdaregistry.info/Elements/u/P60615> ;
    owl:inverseOf <http://rdaregistry.info/Elements/u/P60148> ;
    skos:definition "Relates a performer contributing to a resource by manipulating, controlling, or directing puppets or marionettes in a moving image production or a musical or dramatic presentation or entertainment to a resource."@en .

<http://rdaregistry.info/Elements/u/P60024>
    reg:hasSubproperty <http://rdaregistry.info/Elements/a/P50078> ;
    reg:lexicalAlias <http://rdaregistry.info/Elements/u/panelistOf.en> ;
    reg:name "panelistOf"@en ;
    reg:status <http://metadataregistry.org/uri/RegStatus/1001> ;
    a rdf:Property ;
    rdfs:isDefinedBy <http://rdaregistry.info/Elements/u/> ;
    rdfs:label "is panelist of"@en ;
    rdfs:subPropertyOf <http://rdaregistry.info/Elements/u/P60615> ;
    owl:inverseOf <http://rdaregistry.info/Elements/u/P60149> ;
    skos:definition "Relates a performer contributing to a resource by participating in a program, often broadcast, where topics are discussed, usually with participation of experts in fields related to the discussion to a resource."@en .

<http://rdaregistry.info/Elements/u/P60025>
    reg:hasSubproperty <http://rdaregistry.info/Elements/a/P50079> ;
    reg:lexicalAlias <http://rdaregistry.info/Elements/u/instrumentalistOf.en> ;
    reg:name "instrumentalistOf"@en ;
    reg:status <http://metadataregistry.org/uri/RegStatus/1001> ;
    a rdf:Property ;
    rdfs:isDefinedBy <http://rdaregistry.info/Elements/u/> ;
    rdfs:label "is instrumentalist of"@en ;
    rdfs:subPropertyOf <http://rdaregistry.info/Elements/u/P60615> ;
    owl:inverseOf <http://rdaregistry.info/Elements/u/P60150> ;
    skos:definition "Relates a performer contributing to a resource by playing a musical instrument to a resource."@en .

<http://rdaregistry.info/Elements/u/P60026>
    reg:hasSubproperty <http://rdaregistry.info/Elements/a/P50080> ;
    reg:lexicalAlias <http://rdaregistry.info/Elements/u/commentatorOf.en> ;
    reg:name "commentatorOf"@en ;
    reg:status <http://metadataregistry.org/uri/RegStatus/1001> ;
    a rdf:Property ;
    rdfs:isDefinedBy <http://rdaregistry.info/Elements/u/> ;
    rdfs:label "is commentator of"@en ;
    rdfs:subPropertyOf <http://rdaregistry.info/Elements/u/P60615> ;
    owl:inverseOf <http://rdaregistry.info/Elements/u/P60151> ;
    skos:definition "Relates a performer contributing to a resource by providing interpretation, analysis, or a discussion of the subject matter on a recording, film, or other audiovisual medium to a resource."@en .

<http://rdaregistry.info/Elements/u/P60027>
    reg:hasSubproperty <http://rdaregistry.info/Elements/a/P50217> ;
    reg:lexicalAlias <http://rdaregistry.info/Elements/u/voiceActorOf.en> ;
    reg:name "voiceActorOf"@en ;
    reg:status <http://metadataregistry.org/uri/RegStatus/1001> ;
    a rdf:Property ;
    rdfs:isDefinedBy <http://rdaregistry.info/Elements/u/> ;
    rdfs:label "is voice actor of"@en ;
    rdfs:subPropertyOf <http://rdaregistry.info/Elements/u/P60017> ;
    owl:inverseOf <http://rdaregistry.info/Elements/u/P60152> ;
    skos:definition "Relates a performer contributing to a resource by providing the voice for characters in radio and audio productions and for animated characters in moving image resources as well as by providing voice-overs in radio and television commercials, dubbed resources, etc. to a resource."@en .

<http://rdaregistry.info/Elements/u/P60028>
    reg:hasSubproperty <http://rdaregistry.info/Elements/a/P50081> ;
    reg:lexicalAlias <http://rdaregistry.info/Elements/u/narratorOf.en> ;
    reg:name "narratorOf"@en ;
    reg:status <http://metadataregistry.org/uri/RegStatus/1001> ;
    a rdf:Property ;
    rdfs:isDefinedBy <http://rdaregistry.info/Elements/u/> ;
    rdfs:label "is narrator of"@en ;
    rdfs:subPropertyOf <http://rdaregistry.info/Elements/u/P60615> ;
    owl:inverseOf <http://rdaregistry.info/Elements/u/P60153> ;
    skos:definition "Relates a performer contributing to a resource by reading aloud or giving an account of an act, occurrence, course of events, etc. to a resource."@en .

<http://rdaregistry.info/Elements/u/P60029>
    reg:hasSubproperty <http://rdaregistry.info/Elements/a/P50082> ;
    reg:lexicalAlias <http://rdaregistry.info/Elements/u/storytellerOf.en> ;
    reg:name "storytellerOf"@en ;
    reg:status <http://metadataregistry.org/uri/RegStatus/1001> ;
    a rdf:Property ;
    rdfs:isDefinedBy <http://rdaregistry.info/Elements/u/> ;
    rdfs:label "is storyteller of"@en ;
    rdfs:subPropertyOf <http://rdaregistry.info/Elements/u/P60615> ;
    owl:inverseOf <http://rdaregistry.info/Elements/u/P60154> ;
    skos:definition "Relates a performer contributing to a resource by relaying a creator's original story with dramatic or theatrical interpretation to a resource."@en .

<http://rdaregistry.info/Elements/u/P60030>
    reg:hasSubproperty <http://rdaregistry.info/Elements/a/P50083> ;
    reg:lexicalAlias <http://rdaregistry.info/Elements/u/speakerOf.en> ;
    reg:name "speakerOf"@en ;
    reg:status <http://metadataregistry.org/uri/RegStatus/1001> ;
    a rdf:Property ;
    rdfs:isDefinedBy <http://rdaregistry.info/Elements/u/> ;
    rdfs:label "is speaker of"@en ;
    rdfs:subPropertyOf <http://rdaregistry.info/Elements/u/P60615> ;
    owl:inverseOf <http://rdaregistry.info/Elements/u/P60155> ;
    skos:definition "Relates a performer contributing to a resource by speaking words, such as a lecture, speech, etc. to a resource."@en .

<http://rdaregistry.info/Elements/u/P60031>
    reg:hasSubproperty <http://rdaregistry.info/Elements/a/P50084> ;
    reg:lexicalAlias <http://rdaregistry.info/Elements/u/singerOf.en> ;
    reg:name "singerOf"@en ;
    reg:status <http://metadataregistry.org/uri/RegStatus/1001> ;
    a rdf:Property ;
    rdfs:isDefinedBy <http://rdaregistry.info/Elements/u/> ;
    rdfs:label "is singer of"@en ;
    rdfs:subPropertyOf <http://rdaregistry.info/Elements/u/P60615> ;
    owl:inverseOf <http://rdaregistry.info/Elements/u/P60156> ;
    skos:definition "Relates a performer contributing to a resource by using his/her/their voice, with or without instrumental accompaniment, to produce music. a singer's performance may or may not include actual words to a resource."@en .

<http://rdaregistry.info/Elements/u/P60032>
    reg:hasSubproperty <http://rdaregistry.info/Elements/a/P50086> ;
    reg:lexicalAlias <http://rdaregistry.info/Elements/u/mediumOf.en> ;
    reg:name "mediumOf"@en ;
    reg:status <http://metadataregistry.org/uri/RegStatus/1001> ;
    a rdf:Property ;
    rdfs:isDefinedBy <http://rdaregistry.info/Elements/u/> ;
    rdfs:label "is medium of"@en ;
    rdfs:subPropertyOf <http://rdaregistry.info/Elements/u/P60602> ;
    owl:inverseOf <http://rdaregistry.info/Elements/u/P60157> ;
    skos:definition "Relates an agent held to be a channel of communication between the earthly world and a world of spirits to a resource."@en .

<http://rdaregistry.info/Elements/u/P60033>
    reg:hasSubproperty <http://rdaregistry.info/Elements/a/P50213> ;
    reg:lexicalAlias <http://rdaregistry.info/Elements/u/filmProducerOf.en> ;
    reg:name "filmProducerOf"@en ;
    reg:status <http://metadataregistry.org/uri/RegStatus/1001> ;
    a rdf:Property ;
    rdfs:isDefinedBy <http://rdaregistry.info/Elements/u/> ;
    rdfs:label "is film producer of"@en ;
    rdfs:subPropertyOf <http://rdaregistry.info/Elements/u/P60668> ;
    owl:inverseOf <http://rdaregistry.info/Elements/u/P60169> ;
    skos:definition "Relates a producer responsible for most of the business aspects of a film to a resource."@en .

<http://rdaregistry.info/Elements/u/P60034>
    reg:hasSubproperty <http://rdaregistry.info/Elements/a/P50214> ;
    reg:lexicalAlias <http://rdaregistry.info/Elements/u/radioProducerOf.en> ;
    reg:name "radioProducerOf"@en ;
    reg:status <http://metadataregistry.org/uri/RegStatus/1001> ;
    a rdf:Property ;
    rdfs:isDefinedBy <http://rdaregistry.info/Elements/u/> ;
    rdfs:label "is radio producer of"@en ;
    rdfs:subPropertyOf <http://rdaregistry.info/Elements/u/P60668> ;
    owl:inverseOf <http://rdaregistry.info/Elements/u/P60170> ;
    skos:definition "Relates a producer responsible for most of the business aspects of a radio program to a resource."@en .

<http://rdaregistry.info/Elements/u/P60035>
    reg:hasSubproperty <http://rdaregistry.info/Elements/a/P50215> ;
    reg:lexicalAlias <http://rdaregistry.info/Elements/u/televisionProducerOf.en> ;
    reg:name "televisionProducerOf"@en ;
    reg:status <http://metadataregistry.org/uri/RegStatus/1001> ;
    a rdf:Property ;
    rdfs:isDefinedBy <http://rdaregistry.info/Elements/u/> ;
    rdfs:label "is television producer of"@en ;
    rdfs:subPropertyOf <http://rdaregistry.info/Elements/u/P60668> ;
    owl:inverseOf <http://rdaregistry.info/Elements/u/P60171> ;
    skos:definition "Relates a producer responsible for most of the business aspects of a television program to a resource."@en .

<http://rdaregistry.info/Elements/u/P60036>
    reg:hasSubproperty <http://rdaregistry.info/Elements/a/P50105> ;
    reg:lexicalAlias <http://rdaregistry.info/Elements/u/alternateIdentity.en> ;
    reg:name "alternateIdentity"@en ;
    reg:status <http://metadataregistry.org/uri/RegStatus/1001> ;
    a rdf:Property ;
    rdfs:isDefinedBy <http://rdaregistry.info/Elements/u/> ;
    rdfs:label "has alternate identity"@en ;
    owl:inverseOf <http://rdaregistry.info/Elements/u/P60037> ;
    skos:definition "Relates a pseudonymous or other identity assumed by an agent to an agent."@en .

<http://rdaregistry.info/Elements/u/P60037>
    reg:hasSubproperty <http://rdaregistry.info/Elements/a/P50106> ;
    reg:lexicalAlias <http://rdaregistry.info/Elements/u/realIdentity.en> ;
    reg:name "realIdentity"@en ;
    reg:status <http://metadataregistry.org/uri/RegStatus/1001> ;
    a rdf:Property ;
    rdfs:isDefinedBy <http://rdaregistry.info/Elements/u/> ;
    rdfs:label "has real identity"@en ;
    owl:inverseOf <http://rdaregistry.info/Elements/u/P60036> ;
    skos:definition "Relates a real agent who assumes an alternate identity to an agent."@en .

<http://rdaregistry.info/Elements/u/P60045>
    reg:lexicalAlias <http://rdaregistry.info/Elements/u/respondent.en> ;
    reg:name "respondent"@en ;
    reg:status <http://metadataregistry.org/uri/RegStatus/1001> ;
    a rdf:Property ;
    rdfs:isDefinedBy <http://rdaregistry.info/Elements/u/> ;
    rdfs:label "has respondent"@en ;
    rdfs:subPropertyOf <http://rdaregistry.info/Elements/u/P60447> ;
    owl:inverseOf <http://rdaregistry.info/Elements/u/P60001> ;
    skos:definition "Relates a resource to a candidate for a degree who defends or opposes a thesis provided by a praeses in an academic disputation."@en .

<http://rdaregistry.info/Elements/u/P60046>
    reg:hasSubproperty <http://rdaregistry.info/Elements/a/P50093> ;
    reg:lexicalAlias <http://rdaregistry.info/Elements/u/undifferentiatedNameIndicator.en> ;
    reg:name "undifferentiatedNameIndicator"@en ;
    reg:status <http://metadataregistry.org/uri/RegStatus/1001> ;
    a rdf:Property ;
    rdfs:isDefinedBy <http://rdaregistry.info/Elements/u/> ;
    rdfs:label "has undifferentiated name indicator"@en ;
    skos:definition "Relates a resource to a categorization indicating that the core elements recorded are insufficient to differentiate between two or more agents with the same name."@en .

<http://rdaregistry.info/Elements/u/P60047>
    reg:hasSubproperty <http://rdaregistry.info/Elements/a/P50051>, <http://rdaregistry.info/Elements/a/P50237>, <http://rdaregistry.info/Elements/a/P50238> ;
    reg:lexicalAlias <http://rdaregistry.info/Elements/u/typeOfAgent.en> ;
    reg:name "typeOfAgent"@en ;
    reg:status <http://metadataregistry.org/uri/RegStatus/1001> ;
    a rdf:Property ;
    rdfs:isDefinedBy <http://rdaregistry.info/Elements/u/> ;
    rdfs:label "has type of agent"@en ;
    skos:definition "Relates a resource to a categorization or generic descriptor for a type of agent."@en .

<http://rdaregistry.info/Elements/u/P60048>
    reg:hasSubproperty <http://rdaregistry.info/Elements/m/P30001> ;
    reg:lexicalAlias <http://rdaregistry.info/Elements/u/carrierType.en> ;
    reg:name "carrierType"@en ;
    reg:status <http://metadataregistry.org/uri/RegStatus/1001> ;
    a rdf:Property ;
    rdfs:isDefinedBy <http://rdaregistry.info/Elements/u/> ;
    rdfs:label "has carrier type"@en ;
    skos:definition "Relates a resource to a categorization reflecting a format of a storage medium and housing of a carrier in combination with a type of intermediation device required to view, play, run, etc., the content of a resource."@en .

<http://rdaregistry.info/Elements/u/P60049>
    reg:hasSubproperty <http://rdaregistry.info/Elements/e/P20001> ;
    reg:lexicalAlias <http://rdaregistry.info/Elements/u/contentType.en> ;
    reg:name "contentType"@en ;
    reg:status <http://metadataregistry.org/uri/RegStatus/1001> ;
    a rdf:Property ;
    rdfs:isDefinedBy <http://rdaregistry.info/Elements/u/> ;
    rdfs:label "has content type"@en ;
    skos:definition "Relates a resource to a categorization reflecting a fundamental form of communication in which a content is expressed and a human sense through which it is intended to be perceived."@en ;
    skos:scopeNote "Content type also reflects the number of spatial dimensions and the presence or absence of movement in which content expressed in the form of an image or images is intended to be perceived."@en .

<http://rdaregistry.info/Elements/u/P60050>
    reg:hasSubproperty <http://rdaregistry.info/Elements/m/P30002> ;
    reg:lexicalAlias <http://rdaregistry.info/Elements/u/mediaType.en> ;
    reg:name "mediaType"@en ;
    reg:status <http://metadataregistry.org/uri/RegStatus/1001> ;
    a rdf:Property ;
    rdfs:isDefinedBy <http://rdaregistry.info/Elements/u/> ;
    rdfs:label "has media type"@en ;
    skos:definition "Relates a resource to a categorization reflecting a general type of intermediation device required to view, play, run, etc., the content of a resource."@en .

<http://rdaregistry.info/Elements/u/P60051>
    reg:hasSubproperty <http://rdaregistry.info/Elements/m/P30003> ;
    reg:lexicalAlias <http://rdaregistry.info/Elements/u/modeOfIssuance.en> ;
    reg:name "modeOfIssuance"@en ;
    reg:status <http://metadataregistry.org/uri/RegStatus/1001> ;
    a rdf:Property ;
    rdfs:isDefinedBy <http://rdaregistry.info/Elements/u/> ;
    rdfs:label "has mode of issuance"@en ;
    skos:definition "Relates a resource to a categorization reflecting whether a resource is issued in one or more parts, the way it is updated, and its intended termination."@en .

<http://rdaregistry.info/Elements/u/P60052>
    reg:hasSubproperty <http://rdaregistry.info/Elements/e/P20002>, <http://rdaregistry.info/Elements/i/P40001>, <http://rdaregistry.info/Elements/m/P30004>, <http://rdaregistry.info/Elements/u/P60139>, <http://rdaregistry.info/Elements/u/P60140> ;
    reg:lexicalAlias <http://rdaregistry.info/Elements/u/identifierForResource.en> ;
    reg:name "identifierForResource"@en ;
    reg:status <http://metadataregistry.org/uri/RegStatus/1001> ;
    a rdf:Property ;
    rdfs:isDefinedBy <http://rdaregistry.info/Elements/u/> ;
    rdfs:label "has identifier for resource"@en ;
    skos:definition "Relates a resource to a character string associated with a resource that serves to differentiate a resource from other resources."@en .

<http://rdaregistry.info/Elements/u/P60053>
    reg:hasSubproperty <http://rdaregistry.info/Elements/a/P50006>, <http://rdaregistry.info/Elements/a/P50052>, <http://rdaregistry.info/Elements/a/P50094> ;
    reg:lexicalAlias <http://rdaregistry.info/Elements/u/identifierForAgent.en> ;
    reg:name "identifierForAgent"@en ;
    reg:status <http://metadataregistry.org/uri/RegStatus/1001> ;
    a rdf:Property ;
    rdfs:isDefinedBy <http://rdaregistry.info/Elements/u/> ;
    rdfs:label "has identifier for agent"@en ;
    skos:definition "Relates a resource to a character string uniquely associated with an agent, or with a surrogate for an agent such as an authority record."@en .

<http://rdaregistry.info/Elements/u/P60054>
    reg:hasSubproperty <http://rdaregistry.info/Elements/e/P20003> ;
    reg:lexicalAlias <http://rdaregistry.info/Elements/u/otherDistinguishingCharacteristicOfResource.en> ;
    reg:name "otherDistinguishingCharacteristicOfResource"@en ;
    reg:status <http://metadataregistry.org/uri/RegStatus/1001> ;
    a rdf:Property ;
    rdfs:isDefinedBy <http://rdaregistry.info/Elements/u/> ;
    rdfs:label "has other distinguishing characteristic of resource"@en ;
    skos:definition "Relates a resource to a characteristic other than form of resource, date of resource, place of origin of a resource, content type, or language of resource serving to differentiate a resource from another resource with the same title or from a name of an agent."@en .

<http://rdaregistry.info/Elements/u/P60055>
    reg:status <http://metadataregistry.org/uri/RegStatus/1008> ;
    rdfs:isDefinedBy <http://rdaregistry.info/Elements/u/> .

<http://rdaregistry.info/Elements/u/P60056>
    reg:hasSubproperty <http://rdaregistry.info/Elements/i/P40003>, <http://rdaregistry.info/Elements/u/P60055> ;
    reg:lexicalAlias <http://rdaregistry.info/Elements/u/noteOnResourceSpecificCarrierCharacteristic.en> ;
    reg:name "noteOnResourceSpecificCarrierCharacteristic"@en ;
    reg:status <http://metadataregistry.org/uri/RegStatus/1001> ;
    a rdf:Property ;
    rdfs:isDefinedBy <http://rdaregistry.info/Elements/u/> ;
    rdfs:label "has note on resource-specific carrier characteristic"@en ;
    skos:definition "Relates a resource to a note providing information about additional characteristics that are specific to a resource being described and are assumed not to apply to other resources exemplifying the same resource."@en .

<http://rdaregistry.info/Elements/u/P60057>
    reg:hasSubproperty <http://rdaregistry.info/Elements/m/P30005> ;
    reg:lexicalAlias <http://rdaregistry.info/Elements/u/preferredCitation.en> ;
    reg:name "preferredCitation"@en ;
    reg:status <http://metadataregistry.org/uri/RegStatus/1001> ;
    a rdf:Property ;
    rdfs:isDefinedBy <http://rdaregistry.info/Elements/u/> ;
    rdfs:label "has preferred citation"@en ;
    skos:definition "Relates a resource to a citation for a resource in a form preferred by a creator, publisher, custodian, indexing or abstracting service, etc."@en .

<http://rdaregistry.info/Elements/u/P60058>
    reg:lexicalAlias <http://rdaregistry.info/Elements/u/formOfResource.en> ;
    reg:name "formOfResource"@en ;
    reg:status <http://metadataregistry.org/uri/RegStatus/1001> ;
    a rdf:Property ;
    rdfs:isDefinedBy <http://rdaregistry.info/Elements/u/> ;
    rdfs:label "has form of resource"@en ;
    skos:definition "Relates a resource to a class or genre to which a resource belongs."@en .

<http://rdaregistry.info/Elements/u/P60059>
    reg:hasSubproperty <http://rdaregistry.info/Elements/m/P30006> ;
    reg:lexicalAlias <http://rdaregistry.info/Elements/u/regionalEncoding.en> ;
    reg:name "regionalEncoding"@en ;
    reg:status <http://metadataregistry.org/uri/RegStatus/1001> ;
    a rdf:Property ;
    rdfs:isDefinedBy <http://rdaregistry.info/Elements/u/> ;
    rdfs:label "has regional encoding"@en ;
    rdfs:subPropertyOf <http://rdaregistry.info/Elements/u/P60350> ;
    skos:definition "Relates a resource to a designation for one or more regions of the world for which a videodisc or video game carrier has been encoded, indicating that playback is restricted to a device configured to decode it."@en .

<http://rdaregistry.info/Elements/u/P60060>
    reg:lexicalAlias <http://rdaregistry.info/Elements/u/degreeGrantingInstitution.en> ;
    reg:name "degreeGrantingInstitution"@en ;
    reg:status <http://metadataregistry.org/uri/RegStatus/1001> ;
    a rdf:Property ;
    rdfs:isDefinedBy <http://rdaregistry.info/Elements/u/> ;
    rdfs:label "has degree granting institution"@en ;
    rdfs:subPropertyOf <http://rdaregistry.info/Elements/u/P60374> ;
    owl:inverseOf <http://rdaregistry.info/Elements/u/P60002> ;
    skos:definition "Relates a resource to an agent granting an academic degree."@en .

<http://rdaregistry.info/Elements/u/P60061>
    reg:lexicalAlias <http://rdaregistry.info/Elements/u/hostInstitution.en> ;
    reg:name "host institution"@en ;
    reg:status <http://metadataregistry.org/uri/RegStatus/1001> ;
    a rdf:Property ;
    rdfs:isDefinedBy <http://rdaregistry.info/Elements/u/> ;
    rdfs:label "has host institution"@en ;
    rdfs:subPropertyOf <http://rdaregistry.info/Elements/u/P60374> ;
    owl:inverseOf <http://rdaregistry.info/Elements/u/P60003> ;
    skos:definition "Relates a resource to an agent hosting the event, exhibit, conference, etc., which gave rise to a resource, but having little or no responsibility for the content."@en .

<http://rdaregistry.info/Elements/u/P60062>
    reg:lexicalAlias <http://rdaregistry.info/Elements/u/productionCompany.en> ;
    reg:name "productionCompany"@en ;
    reg:status <http://metadataregistry.org/uri/RegStatus/1001> ;
    a rdf:Property ;
    rdfs:isDefinedBy <http://rdaregistry.info/Elements/u/> ;
    rdfs:label "has production company"@en ;
    rdfs:subPropertyOf <http://rdaregistry.info/Elements/u/P60374> ;
    owl:inverseOf <http://rdaregistry.info/Elements/u/P60004> ;
    skos:definition "Relates a resource to an agent that is responsible for financial, technical, and organizational management of a production for stage, screen, sound recording, television, webcast, etc."@en .

<http://rdaregistry.info/Elements/u/P60063>
    reg:hasSubproperty <http://rdaregistry.info/Elements/a/P50097> ;
    reg:lexicalAlias <http://rdaregistry.info/Elements/u/countryAssociatedWithPerson.en> ;
    reg:name "countryAssociatedWithAgent"@en ;
    reg:status <http://metadataregistry.org/uri/RegStatus/1001> ;
    a rdf:Property ;
    rdfs:isDefinedBy <http://rdaregistry.info/Elements/u/> ;
    rdfs:label "has country associated with agent"@en ;
    skos:definition "Relates a resource to a country with which an agent is identified."@en .

<http://rdaregistry.info/Elements/u/P60064>
    reg:lexicalAlias <http://rdaregistry.info/Elements/u/locationOfHeadquarters.en> ;
    reg:name "locationOfHeadquarters"@en ;
    reg:status <http://metadataregistry.org/uri/RegStatus/1008> ;
    a rdf:Property ;
    rdfs:isDefinedBy <http://rdaregistry.info/Elements/u/> ;
    rdfs:subPropertyOf <http://rdaregistry.info/Elements/u/P60325> .

<http://rdaregistry.info/Elements/u/P60065>
    reg:lexicalAlias <http://rdaregistry.info/Elements/u/courtGoverned.en> ;
    reg:name "courtGoverned"@en ;
    reg:status <http://metadataregistry.org/uri/RegStatus/1001> ;
    a rdf:Property ;
    rdfs:isDefinedBy <http://rdaregistry.info/Elements/u/> ;
    rdfs:label "has court governed"@en ;
    rdfs:subPropertyOf <http://rdaregistry.info/Elements/u/P60374> ;
    owl:inverseOf <http://rdaregistry.info/Elements/u/P60005> ;
    skos:definition "Relates a resource to a court governed by court rules, regardless of their official nature."@en .

<http://rdaregistry.info/Elements/u/P60066>
    reg:hasSubproperty <http://rdaregistry.info/Elements/i/P40004> ;
    reg:lexicalAlias <http://rdaregistry.info/Elements/u/collector.en> ;
    reg:name "collector"@en ;
    reg:status <http://metadataregistry.org/uri/RegStatus/1001> ;
    a rdf:Property ;
    rdfs:isDefinedBy <http://rdaregistry.info/Elements/u/> ;
    rdfs:label "has collector"@en ;
    rdfs:subPropertyOf <http://rdaregistry.info/Elements/u/P60376> ;
    owl:inverseOf <http://rdaregistry.info/Elements/u/P60006> ;
    skos:definition "Relates a resource to a curator who brings together resources from various sources that are then arranged, described, and cataloged as a collection."@en .

<http://rdaregistry.info/Elements/u/P60067>
    reg:hasSubproperty <http://rdaregistry.info/Elements/i/P40005> ;
    reg:lexicalAlias <http://rdaregistry.info/Elements/u/collectionRegistrar.en> ;
    reg:name "collectionRegistrar"@en ;
    reg:status <http://metadataregistry.org/uri/RegStatus/1001> ;
    a rdf:Property ;
    rdfs:isDefinedBy <http://rdaregistry.info/Elements/u/> ;
    rdfs:label "has collection registrar"@en ;
    rdfs:subPropertyOf <http://rdaregistry.info/Elements/u/P60376> ;
    owl:inverseOf <http://rdaregistry.info/Elements/u/P60007> ;
    skos:definition "Relates a resource to a curator who lists or inventories resources in an aggregate resource such as a collection of resources."@en .

<http://rdaregistry.info/Elements/u/P60068>
    reg:hasSubproperty <http://rdaregistry.info/Elements/i/P40006> ;
    reg:lexicalAlias <http://rdaregistry.info/Elements/u/depositor.en> ;
    reg:name "depositor"@en ;
    reg:status <http://metadataregistry.org/uri/RegStatus/1001> ;
    a rdf:Property ;
    rdfs:isDefinedBy <http://rdaregistry.info/Elements/u/> ;
    rdfs:label "has depositor"@en ;
    rdfs:subPropertyOf <http://rdaregistry.info/Elements/u/P60400> ;
    owl:inverseOf <http://rdaregistry.info/Elements/u/P60008> ;
    skos:definition "Relates a resource to a current owner of a resource who deposited a resource into the custody of another agent, while still retaining ownership."@en .

<http://rdaregistry.info/Elements/u/P60069>
    reg:hasSubproperty <http://rdaregistry.info/Elements/m/P30007> ;
    reg:lexicalAlias <http://rdaregistry.info/Elements/u/copyrightDate.en> ;
    reg:name "copyrightDate"@en ;
    reg:status <http://metadataregistry.org/uri/RegStatus/1001> ;
    a rdf:Property ;
    rdfs:isDefinedBy <http://rdaregistry.info/Elements/u/> ;
    rdfs:label "has copyright date"@en ;
    skos:definition "Relates a resource to a date associated with a claim of protection under copyright or a similar regime."@en .

<http://rdaregistry.info/Elements/u/P60070>
    reg:hasSubproperty <http://rdaregistry.info/Elements/m/P30008> ;
    reg:lexicalAlias <http://rdaregistry.info/Elements/u/dateOfDistribution.en> ;
    reg:name "dateOfDistribution"@en ;
    reg:status <http://metadataregistry.org/uri/RegStatus/1001> ;
    a rdf:Property ;
    rdfs:isDefinedBy <http://rdaregistry.info/Elements/u/> ;
    rdfs:label "has date of distribution"@en ;
    skos:definition "Relates a resource to a date associated with the distribution of a resource in a published form."@en .

<http://rdaregistry.info/Elements/u/P60071>
    reg:hasSubproperty <http://rdaregistry.info/Elements/m/P30009> ;
    reg:lexicalAlias <http://rdaregistry.info/Elements/u/dateOfProduction.en> ;
    reg:name "dateOfProduction"@en ;
    reg:status <http://metadataregistry.org/uri/RegStatus/1001> ;
    a rdf:Property ;
    rdfs:isDefinedBy <http://rdaregistry.info/Elements/u/> ;
    rdfs:label "has date of production"@en ;
    skos:definition "Relates a resource to a date associated with the inscription, fabrication, construction, etc., of a resource in an unpublished form."@en .

<http://rdaregistry.info/Elements/u/P60072>
    reg:hasSubproperty <http://rdaregistry.info/Elements/m/P30010> ;
    reg:lexicalAlias <http://rdaregistry.info/Elements/u/dateOfManufacture.en> ;
    reg:name "dateOfManufacture"@en ;
    reg:status <http://metadataregistry.org/uri/RegStatus/1001> ;
    a rdf:Property ;
    rdfs:isDefinedBy <http://rdaregistry.info/Elements/u/> ;
    rdfs:label "has date of manufacture"@en ;
    skos:definition "Relates a resource to a date associated with the printing, duplicating, casting, etc., of a resource in a published form."@en .

<http://rdaregistry.info/Elements/u/P60073>
    reg:hasSubproperty <http://rdaregistry.info/Elements/m/P30011> ;
    reg:lexicalAlias <http://rdaregistry.info/Elements/u/dateOfPublication.en> ;
    reg:name "dateOfPublication"@en ;
    reg:status <http://metadataregistry.org/uri/RegStatus/1001> ;
    a rdf:Property ;
    rdfs:isDefinedBy <http://rdaregistry.info/Elements/u/> ;
    rdfs:label "has date of publication"@en ;
    skos:definition "Relates a resource to a date associated with the publication, release, or issuing of a resource."@en .

<http://rdaregistry.info/Elements/u/P60074>
    reg:hasSubproperty <http://rdaregistry.info/Elements/e/P20004> ;
    reg:lexicalAlias <http://rdaregistry.info/Elements/u/dateOfCapture.en> ;
    reg:name "dateOfCapture"@en ;
    reg:status <http://metadataregistry.org/uri/RegStatus/1001> ;
    a rdf:Property ;
    rdfs:isDefinedBy <http://rdaregistry.info/Elements/u/> ;
    rdfs:label "has date of capture"@en ;
    skos:definition "Relates a resource to a date associated with the recording, filming, etc., of the content of a resource."@en .

<http://rdaregistry.info/Elements/u/P60075>
    reg:lexicalAlias <http://rdaregistry.info/Elements/u/dateOfUsage.en> ;
    reg:name "dateOfUsage"@en ;
    reg:status <http://metadataregistry.org/uri/RegStatus/1001> ;
    a rdf:Property ;
    rdfs:isDefinedBy <http://rdaregistry.info/Elements/u/> ;
    rdfs:label "has date of usage"@en ;
    skos:definition "Relates a name to a date or range of dates associated with the use of the name chosen as a preferred name for an agent."@en .

<http://rdaregistry.info/Elements/u/P60076>
    reg:hasSubproperty <http://rdaregistry.info/Elements/a/P50098>, <http://rdaregistry.info/Elements/a/P50236> ;
    reg:lexicalAlias <http://rdaregistry.info/Elements/u/periodOfActivityOfAgent.en> ;
    reg:name "periodOfActivityOfAgent"@en ;
    reg:status <http://metadataregistry.org/uri/RegStatus/1001> ;
    a rdf:Property ;
    rdfs:isDefinedBy <http://rdaregistry.info/Elements/u/> ;
    rdfs:label "has period of activity of agent"@en ;
    rdfs:subPropertyOf <http://rdaregistry.info/Elements/u/P60324> ;
    skos:definition "Relates a resource to a date or range of dates indicative of a period in which an agent was active in its primary field of endeavour."@en .

<http://rdaregistry.info/Elements/u/P60077>
    reg:hasSubproperty <http://rdaregistry.info/Elements/m/P30012> ;
    reg:lexicalAlias <http://rdaregistry.info/Elements/u/parallelDesignationOfNamedRevisionOfEdition.en> ;
    reg:name "parallelDesignationOfNamedRevisionOfEdition"@en ;
    reg:status <http://metadataregistry.org/uri/RegStatus/1001> ;
    a rdf:Property ;
    rdfs:isDefinedBy <http://rdaregistry.info/Elements/u/> ;
    rdfs:label "has parallel designation of named revision of edition"@en ;
    skos:definition "Relates a resource to a designation of a named revision of an edition in a language or script that differs from that recorded in a designation of a named revision of an edition element."@en .

<http://rdaregistry.info/Elements/u/P60078>
    reg:hasSubproperty <http://rdaregistry.info/Elements/m/P30013> ;
    reg:lexicalAlias <http://rdaregistry.info/Elements/u/parallelDesignationOfEdition.en> ;
    reg:name "parallelDesignationOfEdition"@en ;
    reg:status <http://metadataregistry.org/uri/RegStatus/1001> ;
    a rdf:Property ;
    rdfs:isDefinedBy <http://rdaregistry.info/Elements/u/> ;
    rdfs:label "has parallel designation of edition"@en ;
    skos:definition "Relates a resource to a designation of edition in a language or script that differs from that recorded in a designation of edition element."@en .

<http://rdaregistry.info/Elements/u/P60079>
    reg:hasSubproperty <http://rdaregistry.info/Elements/a/P50019> ;
    reg:lexicalAlias <http://rdaregistry.info/Elements/u/numberOfConferenceEtc.en> ;
    reg:name "numberOfConferenceEtc"@en ;
    reg:status <http://metadataregistry.org/uri/RegStatus/1001> ;
    a rdf:Property ;
    rdfs:isDefinedBy <http://rdaregistry.info/Elements/u/> ;
    rdfs:label "has number of conference, etc."@en ;
    skos:definition "Relates a resource to a designation of a sequencing of a conference, etc., within a series of conferences, etc."@en .

<http://rdaregistry.info/Elements/u/P60080>
    reg:lexicalAlias <http://rdaregistry.info/Elements/u/numberingOfPart.en> ;
    reg:name "numberingOfPart"@en ;
    reg:status <http://metadataregistry.org/uri/RegStatus/1001> ;
    a rdf:Property ;
    rdfs:isDefinedBy <http://rdaregistry.info/Elements/u/> ;
    rdfs:label "has numbering of part"@en ;
    skos:definition "Relates a resource to a designation of a sequencing of a part or parts within a larger resource."@en ;
    skos:scopeNote "Numbering includes a numeral, a letter, any other character, or the combination of these with or without an accompanying caption, and/or a chronological designation."@en .

<http://rdaregistry.info/Elements/u/P60081>
    reg:hasSubproperty <http://rdaregistry.info/Elements/m/P30014> ;
    reg:lexicalAlias <http://rdaregistry.info/Elements/u/numberingWithinSeries.en> ;
    reg:name "numberingWithinSeries"@en ;
    reg:status <http://metadataregistry.org/uri/RegStatus/1001> ;
    a rdf:Property ;
    rdfs:isDefinedBy <http://rdaregistry.info/Elements/u/> ;
    rdfs:label "has numbering within series"@en ;
    skos:definition "Relates a resource to a designation of a sequencing of a part or parts within a series."@en ;
    skos:scopeNote "Numbering includes a numeral, a letter, any other character, or the combination of these with or without an accompanying caption and/or a chronological designation."@en .

<http://rdaregistry.info/Elements/u/P60082>
    reg:hasSubproperty <http://rdaregistry.info/Elements/m/P30015> ;
    reg:lexicalAlias <http://rdaregistry.info/Elements/u/numberingWithinSubseries.en> ;
    reg:name "numberingWithinSubseries"@en ;
    reg:status <http://metadataregistry.org/uri/RegStatus/1001> ;
    a rdf:Property ;
    rdfs:isDefinedBy <http://rdaregistry.info/Elements/u/> ;
    rdfs:label "has numbering within subseries"@en ;
    skos:definition "Relates a resource to a designation of a sequencing of a part or parts within a subseries."@en ;
    skos:scopeNote "Numbering includes a numeral, a letter, any other character, or the combination of these with or without an accompanying caption and/or a chronological designation."@en .

<http://rdaregistry.info/Elements/u/P60083>
    reg:hasSubproperty <http://rdaregistry.info/Elements/i/P40057>, <http://rdaregistry.info/Elements/m/P30016> ;
    reg:lexicalAlias <http://rdaregistry.info/Elements/u/electronicReproduction.en> ;
    reg:name "electronicReproduction"@en ;
    reg:status <http://metadataregistry.org/uri/RegStatus/1001> ;
    a rdf:Property ;
    rdfs:isDefinedBy <http://rdaregistry.info/Elements/u/> ;
    rdfs:label "has electronic reproduction"@en ;
    rdfs:subPropertyOf <http://rdaregistry.info/Elements/u/P60272> ;
    owl:inverseOf <http://rdaregistry.info/Elements/u/P60469> ;
    skos:definition "Relates a resource to a resource in a digital format that is a result of a transfer of a resource in an analog format."@en .

<http://rdaregistry.info/Elements/u/P60084>
    reg:lexicalAlias <http://rdaregistry.info/Elements/u/filmDirector.en> ;
    reg:name "filmDirector"@en ;
    reg:status <http://metadataregistry.org/uri/RegStatus/1001> ;
    a rdf:Property ;
    rdfs:isDefinedBy <http://rdaregistry.info/Elements/u/> ;
    rdfs:label "has film director"@en ;
    rdfs:subPropertyOf <http://rdaregistry.info/Elements/u/P60449> ;
    owl:inverseOf <http://rdaregistry.info/Elements/u/P60009> ;
    skos:definition "Relates a resource to a director responsible for the general management and supervision of a filmed performance."@en .

<http://rdaregistry.info/Elements/u/P60085>
    reg:lexicalAlias <http://rdaregistry.info/Elements/u/radioDirector.en> ;
    reg:name "radioDirector"@en ;
    reg:status <http://metadataregistry.org/uri/RegStatus/1001> ;
    a rdf:Property ;
    rdfs:isDefinedBy <http://rdaregistry.info/Elements/u/> ;
    rdfs:label "has radio director"@en ;
    rdfs:subPropertyOf <http://rdaregistry.info/Elements/u/P60449> ;
    owl:inverseOf <http://rdaregistry.info/Elements/u/P60010> ;
    skos:definition "Relates a resource to a director responsible for the general management and supervision of a radio program."@en .

<http://rdaregistry.info/Elements/u/P60086>
    reg:lexicalAlias <http://rdaregistry.info/Elements/u/televisionDirector.en> ;
    reg:name "televisionDirector"@en ;
    reg:status <http://metadataregistry.org/uri/RegStatus/1001> ;
    a rdf:Property ;
    rdfs:isDefinedBy <http://rdaregistry.info/Elements/u/> ;
    rdfs:label "has television director"@en ;
    rdfs:subPropertyOf <http://rdaregistry.info/Elements/u/P60449> ;
    owl:inverseOf <http://rdaregistry.info/Elements/u/P60011> ;
    skos:definition "Relates a resource to a director responsible for the general management and supervision of a television program."@en .

<http://rdaregistry.info/Elements/u/P60087>
    reg:hasSubproperty <http://rdaregistry.info/Elements/m/P30017> ;
    reg:lexicalAlias <http://rdaregistry.info/Elements/u/parallelDistributorsName.en> ;
    reg:name "parallelDistributorsName"@en ;
    reg:status <http://metadataregistry.org/uri/RegStatus/1001> ;
    a rdf:Property ;
    rdfs:isDefinedBy <http://rdaregistry.info/Elements/u/> ;
    rdfs:label "has parallel distributors name"@en ;
    skos:definition "Relates a resource to a distributor's name in a language or script that differs from that recorded in a distributor's name element."@en .

<http://rdaregistry.info/Elements/u/P60088>
    reg:hasSubproperty <http://rdaregistry.info/Elements/e/P20073> ;
    reg:lexicalAlias <http://rdaregistry.info/Elements/u/dramatizedAs.en> ;
    reg:name "dramatizedAs"@en ;
    reg:status <http://metadataregistry.org/uri/RegStatus/1001> ;
    a rdf:Property ;
    rdfs:isDefinedBy <http://rdaregistry.info/Elements/u/> ;
    rdfs:label "is dramatized as"@en ;
    rdfs:subPropertyOf <http://rdaregistry.info/Elements/u/P60260> ;
    owl:inverseOf <http://rdaregistry.info/Elements/u/P60225> ;
    skos:definition "Relates a resource to a dramatic resource adapted from a source resource."@en .

<http://rdaregistry.info/Elements/u/P60089>
    reg:hasSubproperty <http://rdaregistry.info/Elements/a/P50022>, <http://rdaregistry.info/Elements/a/P50100> ;
    reg:lexicalAlias <http://rdaregistry.info/Elements/u/fieldOfActivityOfAgent.en> ;
    reg:name "fieldOfActivityOfAgent"@en ;
    reg:status <http://metadataregistry.org/uri/RegStatus/1001> ;
    a rdf:Property ;
    rdfs:isDefinedBy <http://rdaregistry.info/Elements/u/> ;
    rdfs:label "has field of activity of agent"@en ;
    skos:definition "Relates a resource to a field of endeavour, area of expertise, competence, responsibility, jurisdiction etc., in which an agent is engaged or was engaged."@en .

<http://rdaregistry.info/Elements/u/P60090>
    reg:hasSubproperty <http://rdaregistry.info/Elements/e/P20005> ;
    reg:lexicalAlias <http://rdaregistry.info/Elements/u/award.en> ;
    reg:name "award"@en ;
    reg:status <http://metadataregistry.org/uri/RegStatus/1001> ;
    a rdf:Property ;
    rdfs:isDefinedBy <http://rdaregistry.info/Elements/u/> ;
    rdfs:label "has award"@en ;
    skos:definition "Relates a resource to a formal recognition of excellence, etc., given by an award- or prize-granting body, for the content of a resource."@en .

<http://rdaregistry.info/Elements/u/P60091>
    reg:hasSubproperty <http://rdaregistry.info/Elements/i/P40007> ;
    reg:lexicalAlias <http://rdaregistry.info/Elements/u/donor.en> ;
    reg:name "donor"@en ;
    reg:status <http://metadataregistry.org/uri/RegStatus/1001> ;
    a rdf:Property ;
    rdfs:isDefinedBy <http://rdaregistry.info/Elements/u/> ;
    rdfs:label "has donor"@en ;
    rdfs:subPropertyOf <http://rdaregistry.info/Elements/u/P60401> ;
    owl:inverseOf <http://rdaregistry.info/Elements/u/P60012> ;
    skos:definition "Relates a resource to a former owner of a resource who donated that resource to another owner."@en .

<http://rdaregistry.info/Elements/u/P60092>
    reg:hasSubproperty <http://rdaregistry.info/Elements/i/P40008> ;
    reg:lexicalAlias <http://rdaregistry.info/Elements/u/seller.en> ;
    reg:name "seller"@en ;
    reg:status <http://metadataregistry.org/uri/RegStatus/1001> ;
    a rdf:Property ;
    rdfs:isDefinedBy <http://rdaregistry.info/Elements/u/> ;
    rdfs:label "has seller"@en ;
    rdfs:subPropertyOf <http://rdaregistry.info/Elements/u/P60401> ;
    owl:inverseOf <http://rdaregistry.info/Elements/u/P60013> ;
    skos:definition "Relates a resource to a former owner of a resource who sold that resource to another owner."@en .

<http://rdaregistry.info/Elements/u/P60093>
    reg:hasSubproperty <http://rdaregistry.info/Elements/m/P30018> ;
    reg:lexicalAlias <http://rdaregistry.info/Elements/u/fileType.en> ;
    reg:name "fileType"@en ;
    reg:status <http://metadataregistry.org/uri/RegStatus/1001> ;
    a rdf:Property ;
    rdfs:isDefinedBy <http://rdaregistry.info/Elements/u/> ;
    rdfs:label "has file type"@en ;
    rdfs:subPropertyOf <http://rdaregistry.info/Elements/u/P60350> ;
    skos:definition "Relates a resource to a general type of data content encoded in a computer file."@en .

<http://rdaregistry.info/Elements/u/P60095>
    reg:hasSubproperty <http://rdaregistry.info/Elements/a/P50101> ;
    reg:lexicalAlias <http://rdaregistry.info/Elements/u/affiliation.en> ;
    reg:name "affiliation"@en ;
    reg:status <http://metadataregistry.org/uri/RegStatus/1001> ;
    a rdf:Property ;
    rdfs:isDefinedBy <http://rdaregistry.info/Elements/u/> ;
    rdfs:label "has affiliation"@en ;
    skos:definition "Relates a resource to a group with which an agent is affiliated or has been affiliated through employment, membership, cultural identity, etc."@en .

<http://rdaregistry.info/Elements/u/P60096>
    reg:lexicalAlias <http://rdaregistry.info/Elements/u/enactingJurisdiction.en> ;
    reg:name "enactingJurisdiction"@en ;
    reg:status <http://metadataregistry.org/uri/RegStatus/1001> ;
    a rdf:Property ;
    rdfs:isDefinedBy <http://rdaregistry.info/Elements/u/> ;
    rdfs:label "has enacting jurisdiction"@en ;
    rdfs:subPropertyOf <http://rdaregistry.info/Elements/u/P60447> ;
    owl:inverseOf <http://rdaregistry.info/Elements/u/P60014> ;
    skos:definition "Relates a resource to a jurisdiction enacting a law, regulation, constitution, court rule, etc."@en .

<http://rdaregistry.info/Elements/u/P60097>
    reg:lexicalAlias <http://rdaregistry.info/Elements/u/jurisdictionGoverned.en> ;
    reg:name "jurisdictionGoverned"@en ;
    reg:status <http://metadataregistry.org/uri/RegStatus/1001> ;
    a rdf:Property ;
    rdfs:isDefinedBy <http://rdaregistry.info/Elements/u/> ;
    rdfs:label "has jurisdiction governed"@en ;
    rdfs:subPropertyOf <http://rdaregistry.info/Elements/u/P60374> ;
    owl:inverseOf <http://rdaregistry.info/Elements/u/P60015> ;
    skos:definition "Relates a resource to a jurisdiction governed by a law, regulation, etc., that was enacted by another jurisdiction."@en .

<http://rdaregistry.info/Elements/u/P60098>
    reg:hasSubproperty <http://rdaregistry.info/Elements/a/P50023>, <http://rdaregistry.info/Elements/a/P50102>, <http://rdaregistry.info/Elements/a/P50235> ;
    reg:lexicalAlias <http://rdaregistry.info/Elements/u/languageOfAgent.en> ;
    reg:name "languageOfAgent"@en ;
    reg:status <http://metadataregistry.org/uri/RegStatus/1001> ;
    a rdf:Property ;
    rdfs:isDefinedBy <http://rdaregistry.info/Elements/u/> ;
    rdfs:label "has language of agent"@en ;
    skos:definition "Relates a resource to a language an agent uses in its communications, when writing for publication, broadcasting, etc."@en .

<http://rdaregistry.info/Elements/u/P60099>
    reg:hasSubproperty <http://rdaregistry.info/Elements/e/P20006>, <http://rdaregistry.info/Elements/e/P20007> ;
    reg:lexicalAlias <http://rdaregistry.info/Elements/u/languageOfContent.en> ;
    reg:name "languageOfContent"@en ;
    reg:status <http://metadataregistry.org/uri/RegStatus/1001> ;
    a rdf:Property ;
    rdfs:isDefinedBy <http://rdaregistry.info/Elements/u/> ;
    rdfs:label "has language of content"@en ;
    skos:definition "Relates a resource to a language used to express the content of a resource."@en .

<http://rdaregistry.info/Elements/u/P60100>
    reg:hasSubproperty <http://rdaregistry.info/Elements/m/P30019> ;
    reg:lexicalAlias <http://rdaregistry.info/Elements/u/facsimileContainedIn.en> ;
    reg:name "facsimileContainedIn"@en ;
    reg:status <http://metadataregistry.org/uri/RegStatus/1001> ;
    a rdf:Property ;
    rdfs:isDefinedBy <http://rdaregistry.info/Elements/u/> ;
    rdfs:label "is facsimile contained in"@en ;
    rdfs:subPropertyOf <http://rdaregistry.info/Elements/u/P60101> ;
    owl:inverseOf <http://rdaregistry.info/Elements/u/P60300> ;
    skos:definition "Relates a resource to a larger resource of which a part is a discrete component that exactly reproduces another resource embodying a resource."@en .

<http://rdaregistry.info/Elements/u/P60101>
    reg:hasSubproperty <http://rdaregistry.info/Elements/e/P20074>, <http://rdaregistry.info/Elements/i/P40009>, <http://rdaregistry.info/Elements/m/P30020>, <http://rdaregistry.info/Elements/u/P60100>, <http://rdaregistry.info/Elements/u/P60192>, <http://rdaregistry.info/Elements/u/P60193>, <http://rdaregistry.info/Elements/u/P60194>, <http://rdaregistry.info/Elements/u/P60317> ;
    reg:lexicalAlias <http://rdaregistry.info/Elements/u/containedIn.en> ;
    reg:name "containedIn"@en ;
    reg:status <http://metadataregistry.org/uri/RegStatus/1001> ;
    a rdf:Property ;
    rdfs:isDefinedBy <http://rdaregistry.info/Elements/u/> ;
    rdfs:label "is contained in"@en ;
    rdfs:subPropertyOf <http://rdaregistry.info/Elements/u/P60714> ;
    owl:inverseOf <http://rdaregistry.info/Elements/u/P60249> ;
    skos:definition "Relates a resource to a larger resource of which a part is a discrete component."@en .

<http://rdaregistry.info/Elements/u/P60102>
    reg:lexicalAlias <http://rdaregistry.info/Elements/u/sequel.en> ;
    reg:name "sequel"@en ;
    reg:status <http://metadataregistry.org/uri/RegStatus/1001> ;
    a rdf:Property ;
    rdfs:isDefinedBy <http://rdaregistry.info/Elements/u/> ;
    rdfs:label "is sequel"@en ;
    rdfs:subPropertyOf <http://rdaregistry.info/Elements/u/P60278> ;
    owl:inverseOf <http://rdaregistry.info/Elements/u/P60577> ;
    skos:definition "Relates a resource to a later resource that continues the narrative of an earlier resource."@en .

<http://rdaregistry.info/Elements/u/P60103>
    reg:hasSubproperty <http://rdaregistry.info/Elements/e/P20075> ;
    reg:lexicalAlias <http://rdaregistry.info/Elements/u/replacedInPartBy.en> ;
    reg:name "replacedInPartBy"@en ;
    reg:status <http://metadataregistry.org/uri/RegStatus/1001> ;
    a rdf:Property ;
    rdfs:isDefinedBy <http://rdaregistry.info/Elements/u/> ;
    rdfs:label "is replaced in part by"@en ;
    rdfs:subPropertyOf <http://rdaregistry.info/Elements/u/P60278> ;
    owl:inverseOf <http://rdaregistry.info/Elements/u/P60479> ;
    skos:definition "Relates a resource to a later resource used in part in place of an earlier resource, usually because the later resource contains updated or new information that makes part of the earlier resource obsolete."@en ;
    skos:scopeNote "This relationship applies generally to single-part units, multipart monographs, and integrating resources."@en .

<http://rdaregistry.info/Elements/u/P60104>
    reg:hasSubproperty <http://rdaregistry.info/Elements/e/P20076> ;
    reg:lexicalAlias <http://rdaregistry.info/Elements/u/replacedBy.en> ;
    reg:name "replacedBy"@en ;
    reg:status <http://metadataregistry.org/uri/RegStatus/1001> ;
    a rdf:Property ;
    rdfs:isDefinedBy <http://rdaregistry.info/Elements/u/> ;
    rdfs:label "is replaced by"@en ;
    rdfs:subPropertyOf <http://rdaregistry.info/Elements/u/P60278> ;
    owl:inverseOf <http://rdaregistry.info/Elements/u/P60480> ;
    skos:definition "Relates a resource to a later resource used in place of an earlier resource, usually because the later resource contains updated or new information that makes the earlier resource obsolete."@en ;
    skos:scopeNote "This relationship applies generally to single-part units, multipart monographs, and integrating resources."@en .

<http://rdaregistry.info/Elements/u/P60105>
    reg:status <http://metadataregistry.org/uri/RegStatus/1008> ;
    rdfs:isDefinedBy <http://rdaregistry.info/Elements/u/> .

<http://rdaregistry.info/Elements/u/P60106>
    reg:hasSubproperty <http://rdaregistry.info/Elements/e/P20077> ;
    reg:lexicalAlias <http://rdaregistry.info/Elements/u/adaptedInVerseAs.en> ;
    reg:name "adaptedInVerseAs"@en ;
    reg:status <http://metadataregistry.org/uri/RegStatus/1001> ;
    a rdf:Property ;
    rdfs:isDefinedBy <http://rdaregistry.info/Elements/u/> ;
    rdfs:label "is adapted in verse as"@en ;
    rdfs:subPropertyOf <http://rdaregistry.info/Elements/u/P60260> ;
    owl:inverseOf <http://rdaregistry.info/Elements/u/P60226> ;
    skos:definition "Relates a resource to a literary composition in verse form adapted from a source resource."@en .

<http://rdaregistry.info/Elements/u/P60107>
    reg:hasSubproperty <http://rdaregistry.info/Elements/a/P50024> ;
    reg:lexicalAlias <http://rdaregistry.info/Elements/u/locationOfConferenceEtc.en> ;
    reg:name "locationOfConferenceEtc"@en ;
    reg:status <http://metadataregistry.org/uri/RegStatus/1001> ;
    a rdf:Property ;
    rdfs:isDefinedBy <http://rdaregistry.info/Elements/u/> ;
    rdfs:label "has location of conference, etc."@en ;
    rdfs:subPropertyOf <http://rdaregistry.info/Elements/u/P60325> ;
    skos:definition "Relates a resource to a local place in which a conference, congress, meeting, exhibition, fair, festival, etc., was held."@en .

<http://rdaregistry.info/Elements/u/P60108>
    reg:hasSubproperty <http://rdaregistry.info/Elements/m/P30049> ;
    reg:lexicalAlias <http://rdaregistry.info/Elements/u/parallelManufacturersName.en> ;
    reg:name "parallelManufacturersName"@en ;
    reg:status <http://metadataregistry.org/uri/RegStatus/1001> ;
    a rdf:Property ;
    rdfs:isDefinedBy <http://rdaregistry.info/Elements/u/> ;
    rdfs:label "has parallel manufacturers name"@en ;
    skos:definition "Relates a resource to a manufacturer's name in a language or script that differs from that recorded in a manufacturer's name element."@en .

<http://rdaregistry.info/Elements/u/P60109>
    reg:hasSubproperty <http://rdaregistry.info/Elements/u/P60345>, <http://rdaregistry.info/Elements/u/P60346>, <http://rdaregistry.info/Elements/u/P60347> ;
    reg:lexicalAlias <http://rdaregistry.info/Elements/u/coordinatesOfCartographicContent.en> ;
    reg:name "coordinatesOfCartographicContent"@en ;
    reg:status <http://metadataregistry.org/uri/RegStatus/1001> ;
    a rdf:Property ;
    rdfs:isDefinedBy <http://rdaregistry.info/Elements/u/> ;
    rdfs:label "has coordinates of cartographic content"@en ;
    skos:definition "Relates a resource to a mathematical system for identifying an area covered by the cartographic content of a resource."@en .

<http://rdaregistry.info/Elements/u/P60110>
    reg:hasSubproperty <http://rdaregistry.info/Elements/e/P20009> ;
    reg:lexicalAlias <http://rdaregistry.info/Elements/u/adaptedAsAMotionPicture.en> ;
    reg:name "adaptedAsAMotionPicture"@en ;
    reg:status <http://metadataregistry.org/uri/RegStatus/1001> ;
    a rdf:Property ;
    rdfs:isDefinedBy <http://rdaregistry.info/Elements/u/> ;
    rdfs:label "is adapted as motion picture"@en ;
    rdfs:subPropertyOf <http://rdaregistry.info/Elements/u/P60260> ;
    owl:inverseOf <http://rdaregistry.info/Elements/u/P60227> ;
    skos:definition "Relates a resource to a motion picture based on the source resource."@en .

<http://rdaregistry.info/Elements/u/P60111>
    reg:hasSubproperty <http://rdaregistry.info/Elements/e/P20078> ;
    reg:lexicalAlias <http://rdaregistry.info/Elements/u/dubbedVersionOf.en> ;
    reg:name "dubbedVersionOf"@en ;
    reg:status <http://metadataregistry.org/uri/RegStatus/1001> ;
    a rdf:Property ;
    rdfs:isDefinedBy <http://rdaregistry.info/Elements/u/> ;
    rdfs:label "is dubbed version of"@en ;
    rdfs:subPropertyOf <http://rdaregistry.info/Elements/u/P60244> ;
    owl:inverseOf <http://rdaregistry.info/Elements/u/P60112> ;
    skos:definition "Relates a resource to a moving image resource in which spoken dialogue has been translated into a language different from that of an original resource."@en .

<http://rdaregistry.info/Elements/u/P60112>
    reg:hasSubproperty <http://rdaregistry.info/Elements/e/P20079> ;
    reg:lexicalAlias <http://rdaregistry.info/Elements/u/dubbedVersion.en> ;
    reg:name "dubbedVersion"@en ;
    reg:status <http://metadataregistry.org/uri/RegStatus/1001> ;
    a rdf:Property ;
    rdfs:isDefinedBy <http://rdaregistry.info/Elements/u/> ;
    rdfs:label "is dubbed version"@en ;
    rdfs:subPropertyOf <http://rdaregistry.info/Elements/u/P60280> ;
    owl:inverseOf <http://rdaregistry.info/Elements/u/P60111> ;
    skos:definition "Relates a resource to a moving image resource that translates spoken dialogue of an original resource into a different language."@en .

<http://rdaregistry.info/Elements/u/P60113>
    reg:hasSubproperty <http://rdaregistry.info/Elements/e/P20080> ;
    reg:lexicalAlias <http://rdaregistry.info/Elements/u/cadenza.en> ;
    reg:name "cadenza"@en ;
    reg:status <http://metadataregistry.org/uri/RegStatus/1001> ;
    a rdf:Property ;
    rdfs:isDefinedBy <http://rdaregistry.info/Elements/u/> ;
    rdfs:label "is cadenza"@en ;
    rdfs:subPropertyOf <http://rdaregistry.info/Elements/u/P60204> ;
    owl:inverseOf <http://rdaregistry.info/Elements/u/P60116> ;
    skos:definition "Relates a resource to a musical resource consisting of an ornamental passage for a soloist, added to a musical resource such as a concerto, either by the same or a different composer."@en .

<http://rdaregistry.info/Elements/u/P60114>
    reg:hasSubproperty <http://rdaregistry.info/Elements/e/P20081> ;
    reg:lexicalAlias <http://rdaregistry.info/Elements/u/variationsBasedOn.en> ;
    reg:name "variationsBasedOn"@en ;
    reg:status <http://metadataregistry.org/uri/RegStatus/1001> ;
    a rdf:Property ;
    rdfs:isDefinedBy <http://rdaregistry.info/Elements/u/> ;
    rdfs:label "is variations based on"@en ;
    rdfs:subPropertyOf <http://rdaregistry.info/Elements/u/P60305> ;
    owl:inverseOf <http://rdaregistry.info/Elements/u/P60115> ;
    skos:definition "Relates a resource to a musical resource from which melodic, thematic, or harmonic material is taken to form a discrete theme, which is repeated one or more times with subsequent modifications."@en .

<http://rdaregistry.info/Elements/u/P60115>
    reg:hasSubproperty <http://rdaregistry.info/Elements/e/P20082> ;
    reg:lexicalAlias <http://rdaregistry.info/Elements/u/modifiedByVariationAs.en> ;
    reg:name "modifiedByVariationAs"@en ;
    reg:status <http://metadataregistry.org/uri/RegStatus/1001> ;
    a rdf:Property ;
    rdfs:isDefinedBy <http://rdaregistry.info/Elements/u/> ;
    rdfs:label "is modified by variation as"@en ;
    rdfs:subPropertyOf <http://rdaregistry.info/Elements/u/P60250> ;
    owl:inverseOf <http://rdaregistry.info/Elements/u/P60114> ;
    skos:definition "Relates a resource to a musical resource in which melodic, thematic, or harmonic material taken from a source resource forms a discrete theme, which is repeated one or more times with subsequent modifications."@en .

<http://rdaregistry.info/Elements/u/P60116>
    reg:hasSubproperty <http://rdaregistry.info/Elements/e/P20083> ;
    reg:lexicalAlias <http://rdaregistry.info/Elements/u/cadenzaComposedFor.en> ;
    reg:name "cadenzaComposedFor"@en ;
    reg:status <http://metadataregistry.org/uri/RegStatus/1001> ;
    a rdf:Property ;
    rdfs:isDefinedBy <http://rdaregistry.info/Elements/u/> ;
    rdfs:label "is cadenza composed for"@en ;
    rdfs:subPropertyOf <http://rdaregistry.info/Elements/u/P60307> ;
    owl:inverseOf <http://rdaregistry.info/Elements/u/P60113> ;
    skos:definition "Relates a resource to a musical resource such as a concerto for which an ornamental passage for a soloist has been composed, either by the same or a different composer."@en .

<http://rdaregistry.info/Elements/u/P60117>
    reg:hasSubproperty <http://rdaregistry.info/Elements/e/P20084> ;
    reg:lexicalAlias <http://rdaregistry.info/Elements/u/librettoFor.en> ;
    reg:name "librettoFor"@en ;
    reg:status <http://metadataregistry.org/uri/RegStatus/1001> ;
    a rdf:Property ;
    rdfs:isDefinedBy <http://rdaregistry.info/Elements/u/> ;
    rdfs:label "is libretto for"@en ;
    rdfs:subPropertyOf <http://rdaregistry.info/Elements/u/P60198> ;
    owl:inverseOf <http://rdaregistry.info/Elements/u/P60270> ;
    skos:definition "Relates a resource to a musical resource such as an opera or other resource for the musical stage, or an oratorio, that uses a text of a related resource."@en .

<http://rdaregistry.info/Elements/u/P60118>
    reg:hasSubproperty <http://rdaregistry.info/Elements/e/P20085> ;
    reg:lexicalAlias <http://rdaregistry.info/Elements/u/incidentalMusic.en> ;
    reg:name "incidentalMusic"@en ;
    reg:status <http://metadataregistry.org/uri/RegStatus/1001> ;
    a rdf:Property ;
    rdfs:isDefinedBy <http://rdaregistry.info/Elements/u/> ;
    rdfs:label "is incidental music"@en ;
    rdfs:subPropertyOf <http://rdaregistry.info/Elements/u/P60723> ;
    owl:inverseOf <http://rdaregistry.info/Elements/u/P60202> ;
    skos:definition "Relates a resource to a musical resource that provides incidental music for a play or other spoken resource for the stage."@en .

<http://rdaregistry.info/Elements/u/P60119>
    reg:hasSubproperty <http://rdaregistry.info/Elements/a/P50025>, <http://rdaregistry.info/Elements/a/P50054>, <http://rdaregistry.info/Elements/a/P50103> ;
    reg:lexicalAlias <http://rdaregistry.info/Elements/u/variantNameForAgent.en> ;
    reg:name "variantNameForAgent"@en ;
    reg:status <http://metadataregistry.org/uri/RegStatus/1001> ;
    a rdf:Property ;
    rdfs:isDefinedBy <http://rdaregistry.info/Elements/u/> ;
    rdfs:label "has variant name for agent"@en ;
    rdfs:subPropertyOf <http://rdaregistry.info/Elements/u/P60368> ;
    skos:definition "Relates a resource to a name or form of name by which an agent is known that differs from a name or form of name chosen as a preferred name."@en .

<http://rdaregistry.info/Elements/u/P60120>
    reg:hasSubproperty <http://rdaregistry.info/Elements/e/P20086> ;
    reg:lexicalAlias <http://rdaregistry.info/Elements/u/remadeAs.en> ;
    reg:name "remadeAs"@en ;
    reg:status <http://metadataregistry.org/uri/RegStatus/1001> ;
    a rdf:Property ;
    rdfs:isDefinedBy <http://rdaregistry.info/Elements/u/> ;
    rdfs:label "is remade as"@en ;
    rdfs:subPropertyOf <http://rdaregistry.info/Elements/u/P60250> ;
    owl:inverseOf <http://rdaregistry.info/Elements/u/P60295> ;
    skos:definition "Relates a resource to a motion picture, radio program, television program, or video based on an earlier resource."@en .

<http://rdaregistry.info/Elements/u/P60121>
    reg:hasSubproperty <http://rdaregistry.info/Elements/e/P20087> ;
    reg:lexicalAlias <http://rdaregistry.info/Elements/u/setToMusicAs.en> ;
    reg:name "setToMusicAs"@en ;
    reg:status <http://metadataregistry.org/uri/RegStatus/1001> ;
    a rdf:Property ;
    rdfs:isDefinedBy <http://rdaregistry.info/Elements/u/> ;
    rdfs:label "is set to music as"@en ;
    rdfs:subPropertyOf <http://rdaregistry.info/Elements/u/P60250> ;
    owl:inverseOf <http://rdaregistry.info/Elements/u/P60266> ;
    skos:definition "Relates a resource to a non-dramatic musical resource, other than an oratorio, that uses a text of a source resource."@en .

<http://rdaregistry.info/Elements/u/P60122>
    reg:hasSubproperty <http://rdaregistry.info/Elements/m/P30050> ;
    reg:lexicalAlias <http://rdaregistry.info/Elements/u/noteOnIssuePartOrIterationUsedAsBasisForIdentificationOfResource.en> ;
    reg:name "noteOnIssuePartOrIterationUsedAsBasisForIdentificationOfResource"@en ;
    reg:status <http://metadataregistry.org/uri/RegStatus/1001> ;
    a rdf:Property ;
    rdfs:isDefinedBy <http://rdaregistry.info/Elements/u/> ;
    rdfs:label "has note on issue, part, or iteration used as basis for identification of resource"@en ;
    rdfs:subPropertyOf <http://rdaregistry.info/Elements/u/P60470> ;
    skos:definition "Relates a resource to a note identifying an issue or part of a multipart monograph or serial, or an iteration of an integrating resource that has been used as a basis for the identification of a resource."@en .

<http://rdaregistry.info/Elements/u/P60123>
    reg:hasSubproperty <http://rdaregistry.info/Elements/e/P20010> ;
    reg:lexicalAlias <http://rdaregistry.info/Elements/u/noteOnChangesInContentCharacteristics.en> ;
    reg:name "noteOnChangesInContentCharacteristics"@en ;
    reg:status <http://metadataregistry.org/uri/RegStatus/1001> ;
    a rdf:Property ;
    rdfs:isDefinedBy <http://rdaregistry.info/Elements/u/> ;
    rdfs:label "has note on changes in content characteristics"@en ;
    rdfs:subPropertyOf <http://rdaregistry.info/Elements/u/P60470> ;
    skos:definition "Relates a resource to a note on changes in content characteristics that occur in subsequent issues or parts of a resource issued in successive parts or between iterations of an integrating resource."@en .

<http://rdaregistry.info/Elements/u/P60124>
    reg:hasSubproperty <http://rdaregistry.info/Elements/m/P30051> ;
    reg:lexicalAlias <http://rdaregistry.info/Elements/u/noteOnChangesInCarrierCharacteristics.en> ;
    reg:name "noteOnChangesInCarrierCharacteristics"@en ;
    reg:status <http://metadataregistry.org/uri/RegStatus/1001> ;
    a rdf:Property ;
    rdfs:isDefinedBy <http://rdaregistry.info/Elements/u/> ;
    rdfs:label "has note on changes in carrier characteristics"@en ;
    rdfs:subPropertyOf <http://rdaregistry.info/Elements/u/P60470> ;
    skos:definition "Relates a resource to a note on changes in the characteristics of a carrier that occur in subsequent issues or parts of a resource issued in successive parts or between iterations of an integrating resource."@en .

<http://rdaregistry.info/Elements/u/P60125>
    reg:hasSubproperty <http://rdaregistry.info/Elements/m/P30052> ;
    reg:lexicalAlias <http://rdaregistry.info/Elements/u/noteOnDistributionStatement.en> ;
    reg:name "noteOnDistributionStatement"@en ;
    reg:status <http://metadataregistry.org/uri/RegStatus/1001> ;
    a rdf:Property ;
    rdfs:isDefinedBy <http://rdaregistry.info/Elements/u/> ;
    rdfs:label "has note on distribution statement"@en ;
    rdfs:subPropertyOf <http://rdaregistry.info/Elements/u/P60470> ;
    skos:definition "Relates a resource to a note providing details on place of distribution, distributor, or date of distribution, or information on changes in the place of distribution, distributor, or distributors name."@en .

<http://rdaregistry.info/Elements/u/P60126>
    reg:hasSubproperty <http://rdaregistry.info/Elements/m/P30053> ;
    reg:lexicalAlias <http://rdaregistry.info/Elements/u/noteOnManufactureStatement.en> ;
    reg:name "noteOnManufactureStatement"@en ;
    reg:status <http://metadataregistry.org/uri/RegStatus/1001> ;
    a rdf:Property ;
    rdfs:isDefinedBy <http://rdaregistry.info/Elements/u/> ;
    rdfs:label "has note on manufacture statement"@en ;
    rdfs:subPropertyOf <http://rdaregistry.info/Elements/u/P60470> ;
    skos:definition "Relates a resource to a note providing details on place of manufacture, manufacturer, or date of manufacture, or information on changes in place of manufacture, manufacturer, or manufacturers name."@en .

<http://rdaregistry.info/Elements/u/P60127>
    reg:hasSubproperty <http://rdaregistry.info/Elements/m/P30054> ;
    reg:lexicalAlias <http://rdaregistry.info/Elements/u/noteOnProductionStatement.en> ;
    reg:name "noteOnProductionStatement"@en ;
    reg:status <http://metadataregistry.org/uri/RegStatus/1001> ;
    a rdf:Property ;
    rdfs:isDefinedBy <http://rdaregistry.info/Elements/u/> ;
    rdfs:label "has note on production statement"@en ;
    rdfs:subPropertyOf <http://rdaregistry.info/Elements/u/P60470> ;
    skos:definition "Relates a resource to a note providing details on place of production, producer, or date of production, or information on changes in place of production, producer, or producers name."@en .

<http://rdaregistry.info/Elements/u/P60128>
    reg:hasSubproperty <http://rdaregistry.info/Elements/m/P30055> ;
    reg:lexicalAlias <http://rdaregistry.info/Elements/u/noteOnPublicationStatement.en> ;
    reg:name "noteOnPublicationStatement"@en ;
    reg:status <http://metadataregistry.org/uri/RegStatus/1001> ;
    a rdf:Property ;
    rdfs:isDefinedBy <http://rdaregistry.info/Elements/u/> ;
    rdfs:label "has note on publication statement"@en ;
    rdfs:subPropertyOf <http://rdaregistry.info/Elements/u/P60470> ;
    skos:definition "Relates a resource to a note providing details on place of publication, publisher, or date of publication, information on changes in place of publication, publisher, or publishers name, or on suspension of publication."@en .

<http://rdaregistry.info/Elements/u/P60129>
    reg:hasSubproperty <http://rdaregistry.info/Elements/m/P30056> ;
    reg:lexicalAlias <http://rdaregistry.info/Elements/u/noteOnFrequency.en> ;
    reg:name "noteOnFrequency"@en ;
    reg:status <http://metadataregistry.org/uri/RegStatus/1001> ;
    a rdf:Property ;
    rdfs:isDefinedBy <http://rdaregistry.info/Elements/u/> ;
    rdfs:label "has note on frequency"@en ;
    rdfs:subPropertyOf <http://rdaregistry.info/Elements/u/P60470> ;
    skos:definition "Relates a resource to a note providing details on the currency of the contents, on the frequency of release of issues or parts of a serial or the frequency of updates to an integrating resource, or on changes in frequency."@en .

<http://rdaregistry.info/Elements/u/P60130>
    reg:hasSubproperty <http://rdaregistry.info/Elements/m/P30057> ;
    reg:lexicalAlias <http://rdaregistry.info/Elements/u/noteOnStatementOfResponsibility.en> ;
    reg:name "noteOnStatementOfResponsibility"@en ;
    reg:status <http://metadataregistry.org/uri/RegStatus/1001> ;
    a rdf:Property ;
    rdfs:isDefinedBy <http://rdaregistry.info/Elements/u/> ;
    rdfs:label "has note on statement of responsibility"@en ;
    rdfs:subPropertyOf <http://rdaregistry.info/Elements/u/P60470> ;
    skos:definition "Relates a resource to a note providing information on an agent not named in a statement of responsibility to whom responsibility for the creation of, or contribution to a realization of, the intellectual or artistic content of a resource has been attributed, on variant forms of names appearing in the resource, on changes in statements of responsibility, or on other details relating to a statement of responsibility."@en .

<http://rdaregistry.info/Elements/u/P60131>
    reg:hasSubproperty <http://rdaregistry.info/Elements/m/P30058> ;
    reg:lexicalAlias <http://rdaregistry.info/Elements/u/noteOnSeriesStatement.en> ;
    reg:name "noteOnSeriesStatement"@en ;
    reg:status <http://metadataregistry.org/uri/RegStatus/1001> ;
    a rdf:Property ;
    rdfs:isDefinedBy <http://rdaregistry.info/Elements/u/> ;
    rdfs:label "has note on series statement"@en ;
    rdfs:subPropertyOf <http://rdaregistry.info/Elements/u/P60470> ;
    skos:definition "Relates a resource to a note providing information on complex series statements, incorrect numbering within series, or changes in series statements."@en .

<http://rdaregistry.info/Elements/u/P60132>
    reg:hasSubproperty <http://rdaregistry.info/Elements/m/P30059> ;
    reg:lexicalAlias <http://rdaregistry.info/Elements/u/noteOnCopyrightDate.en> ;
    reg:name "noteOnCopyrightDate"@en ;
    reg:status <http://metadataregistry.org/uri/RegStatus/1001> ;
    a rdf:Property ;
    rdfs:isDefinedBy <http://rdaregistry.info/Elements/u/> ;
    rdfs:label "has note on copyright date"@en ;
    rdfs:subPropertyOf <http://rdaregistry.info/Elements/u/P60470> ;
    skos:definition "Relates a resource to a note providing information on copyright dates not recorded as part of a copyright date element."@en .

<http://rdaregistry.info/Elements/u/P60133>
    reg:hasSubproperty <http://rdaregistry.info/Elements/i/P40010>, <http://rdaregistry.info/Elements/m/P30060> ;
    reg:lexicalAlias <http://rdaregistry.info/Elements/u/noteOnDimensionsOfResource.en> ;
    reg:name "noteOnDimensionsOfResource"@en ;
    reg:status <http://metadataregistry.org/uri/RegStatus/1001> ;
    a rdf:Property ;
    rdfs:isDefinedBy <http://rdaregistry.info/Elements/u/> ;
    rdfs:label "has note on dimensions of resource"@en ;
    rdfs:subPropertyOf <http://rdaregistry.info/Elements/u/P60470> ;
    skos:definition "Relates a resource to a note providing information on the dimensions of a resource that is not recorded as part of a dimensions element."@en .

<http://rdaregistry.info/Elements/u/P60134>
    reg:hasSubproperty <http://rdaregistry.info/Elements/i/P40011>, <http://rdaregistry.info/Elements/m/P30061> ;
    reg:lexicalAlias <http://rdaregistry.info/Elements/u/noteOnExtentOfResource.en> ;
    reg:name "noteOnExtentOfResource"@en ;
    reg:status <http://metadataregistry.org/uri/RegStatus/1001> ;
    a rdf:Property ;
    rdfs:isDefinedBy <http://rdaregistry.info/Elements/u/> ;
    rdfs:label "has note on extent of resource"@en ;
    rdfs:subPropertyOf <http://rdaregistry.info/Elements/u/P60470> ;
    skos:definition "Relates a resource to a note providing information on the extent of a resource that is not recorded as part of an extent element."@en .

<http://rdaregistry.info/Elements/u/P60135>
    reg:hasSubproperty <http://rdaregistry.info/Elements/m/P30062> ;
    reg:lexicalAlias <http://rdaregistry.info/Elements/u/noteOnNumberingOfSerials.en> ;
    reg:name "noteOnNumberingOfSerials"@en ;
    reg:status <http://metadataregistry.org/uri/RegStatus/1001> ;
    a rdf:Property ;
    rdfs:isDefinedBy <http://rdaregistry.info/Elements/u/> ;
    rdfs:label "has note on numbering of serials"@en ;
    rdfs:subPropertyOf <http://rdaregistry.info/Elements/u/P60470> ;
    skos:definition "Relates a resource to a note providing information on the numbering of the first or last issue or part, on complex or irregular numbering including numbering errors, on a period covered by a volume, issue, part, etc., or on other information relating to numbering of serials."@en .

<http://rdaregistry.info/Elements/u/P60136>
    reg:hasSubproperty <http://rdaregistry.info/Elements/m/P30063> ;
    reg:lexicalAlias <http://rdaregistry.info/Elements/u/noteOnTitle.en> ;
    reg:name "noteOnTitle"@en ;
    reg:status <http://metadataregistry.org/uri/RegStatus/1001> ;
    a rdf:Property ;
    rdfs:isDefinedBy <http://rdaregistry.info/Elements/u/> ;
    rdfs:label "has note on title"@en ;
    rdfs:subPropertyOf <http://rdaregistry.info/Elements/u/P60470> ;
    skos:definition "Relates a resource to a note providing information on a source from which a title was taken, on the date a title was viewed, on variations in titles, on inaccuracies, deletions, etc., or other information relating to a title."@en .

<http://rdaregistry.info/Elements/u/P60137>
    reg:hasSubproperty <http://rdaregistry.info/Elements/m/P30064> ;
    reg:lexicalAlias <http://rdaregistry.info/Elements/u/noteOnEditionStatement.en> ;
    reg:name "noteOnEditionStatement"@en ;
    reg:status <http://metadataregistry.org/uri/RegStatus/1001> ;
    a rdf:Property ;
    rdfs:isDefinedBy <http://rdaregistry.info/Elements/u/> ;
    rdfs:label "has note on edition statement"@en ;
    rdfs:subPropertyOf <http://rdaregistry.info/Elements/u/P60470> ;
    skos:definition "Relates a resource to a note providing information on a source of an edition statement, on edition statements relating to issues, parts, etc., on changes in edition statements, or other information relating to an edition statement."@en .

<http://rdaregistry.info/Elements/u/P60138>
    reg:hasSubproperty <http://rdaregistry.info/Elements/e/P20088> ;
    reg:lexicalAlias <http://rdaregistry.info/Elements/u/adaptedAsNovel.en> ;
    reg:name "novelization"@en ;
    reg:status <http://metadataregistry.org/uri/RegStatus/1001> ;
    a rdf:Property ;
    rdfs:isDefinedBy <http://rdaregistry.info/Elements/u/> ;
    rdfs:label "is adapted as novel"@en ;
    rdfs:subPropertyOf <http://rdaregistry.info/Elements/u/P60260> ;
    owl:inverseOf <http://rdaregistry.info/Elements/u/P60228> ;
    skos:definition "Relates a resource to a novel adapted from a source resource."@en .

<http://rdaregistry.info/Elements/u/P60139>
    reg:hasSubproperty <http://rdaregistry.info/Elements/m/P30065> ;
    reg:lexicalAlias <http://rdaregistry.info/Elements/u/publishersNumberForMusic.en> ;
    reg:name "publishersNumberForMusic"@en ;
    reg:status <http://metadataregistry.org/uri/RegStatus/1001> ;
    a rdf:Property ;
    rdfs:isDefinedBy <http://rdaregistry.info/Elements/u/> ;
    rdfs:label "has publishers number for music"@en ;
    rdfs:subPropertyOf <http://rdaregistry.info/Elements/u/P60052> ;
    skos:definition "Relates a resource to a numbering designation assigned to a notated music resource by a publisher."@en ;
    skos:scopeNote "A publishers number for notated music sometimes includes initials, abbreviations, or words identifying the publisher."@en .

<http://rdaregistry.info/Elements/u/P60140>
    reg:hasSubproperty <http://rdaregistry.info/Elements/m/P30066> ;
    reg:lexicalAlias <http://rdaregistry.info/Elements/u/plateNumberForMusic.en> ;
    reg:name "plateNumberForMusic"@en ;
    reg:status <http://metadataregistry.org/uri/RegStatus/1001> ;
    a rdf:Property ;
    rdfs:isDefinedBy <http://rdaregistry.info/Elements/u/> ;
    rdfs:label "has plate number for music"@en ;
    rdfs:subPropertyOf <http://rdaregistry.info/Elements/u/P60052> ;
    skos:definition "Relates a resource to a numbering designation assigned to a notated music resource by a publisher."@en ;
    skos:scopeNote "A plate number for notated music sometimes includes initials, abbreviations, or words identifying the publisher. It is sometimes followed by a number corresponding to the number of pages or plates or a number corresponding to an individual page or plate."@en .

<http://rdaregistry.info/Elements/u/P60141>
    reg:hasSubproperty <http://rdaregistry.info/Elements/e/P20011>, <http://rdaregistry.info/Elements/u/P60842>, <http://rdaregistry.info/Elements/u/P60844> ;
    reg:lexicalAlias <http://rdaregistry.info/Elements/u/conductor.en> ;
    reg:name "conductor"@en ;
    reg:status <http://metadataregistry.org/uri/RegStatus/1001> ;
    a rdf:Property ;
    rdfs:isDefinedBy <http://rdaregistry.info/Elements/u/> ;
    rdfs:label "has conductor"@en ;
    rdfs:subPropertyOf <http://rdaregistry.info/Elements/u/P60387> ;
    owl:inverseOf <http://rdaregistry.info/Elements/u/P60016> ;
    skos:definition "Relates a resource to a performer contributing to a musical resource by leading a performing group in a musical or dramatic presentation, etc."@en .

<http://rdaregistry.info/Elements/u/P60142>
    reg:hasSubproperty <http://rdaregistry.info/Elements/e/P20012>, <http://rdaregistry.info/Elements/u/P60152> ;
    reg:lexicalAlias <http://rdaregistry.info/Elements/u/actor.en> ;
    reg:name "actor"@en ;
    reg:status <http://metadataregistry.org/uri/RegStatus/1001> ;
    a rdf:Property ;
    rdfs:isDefinedBy <http://rdaregistry.info/Elements/u/> ;
    rdfs:label "has actor"@en ;
    rdfs:subPropertyOf <http://rdaregistry.info/Elements/u/P60387> ;
    owl:inverseOf <http://rdaregistry.info/Elements/u/P60017> ;
    skos:definition "Relates a resource to a performer contributing to a resource by acting as a cast member or player in a musical or dramatic presentation, etc."@en .

<http://rdaregistry.info/Elements/u/P60143>
    rdakit:seeAlso <http://rdaregistry.info/Elements/u/P60824> ;
    reg:hasSubproperty <http://rdaregistry.info/Elements/e/P20013> ;
    reg:lexicalAlias <http://rdaregistry.info/Elements/u/onScreenPresenter.en> ;
    reg:name "onScreenPresenter"@en ;
    reg:status <http://metadataregistry.org/uri/RegStatus/1001> ;
    a rdf:Property ;
    rdfs:isDefinedBy <http://rdaregistry.info/Elements/u/> ;
    rdfs:label "has on-screen presenter"@en ;
    rdfs:subPropertyOf <http://rdaregistry.info/Elements/u/P60387> ;
    owl:inverseOf <http://rdaregistry.info/Elements/u/P60018> ;
    skos:definition "Relates a resource to a performer contributing to a resource by appearing on screen to provide contextual or background information. an on-screen presenter may appear in nonfiction moving image materials or in introductions to fiction moving image materials."@en ;
    skos:scopeNote "Appearance in nonfiction moving image materials or in introductions to fiction moving image materials is included. Appearance on screen in a non-performing role is excluded."@en .

<http://rdaregistry.info/Elements/u/P60144>
    reg:hasSubproperty <http://rdaregistry.info/Elements/e/P20014> ;
    reg:lexicalAlias <http://rdaregistry.info/Elements/u/dancer.en> ;
    reg:name "dancer"@en ;
    reg:status <http://metadataregistry.org/uri/RegStatus/1001> ;
    a rdf:Property ;
    rdfs:isDefinedBy <http://rdaregistry.info/Elements/u/> ;
    rdfs:label "has dancer"@en ;
    rdfs:subPropertyOf <http://rdaregistry.info/Elements/u/P60387> ;
    owl:inverseOf <http://rdaregistry.info/Elements/u/P60019> ;
    skos:definition "Relates a resource to a performer contributing to a resource by dancing in a musical, dramatic, etc., presentation."@en .

<http://rdaregistry.info/Elements/u/P60145>
    reg:hasSubproperty <http://rdaregistry.info/Elements/e/P20015> ;
    reg:lexicalAlias <http://rdaregistry.info/Elements/u/teacher.en> ;
    reg:name "teacher"@en ;
    reg:status <http://metadataregistry.org/uri/RegStatus/1001> ;
    a rdf:Property ;
    rdfs:isDefinedBy <http://rdaregistry.info/Elements/u/> ;
    rdfs:label "has teacher"@en ;
    rdfs:subPropertyOf <http://rdaregistry.info/Elements/u/P60387> ;
    owl:inverseOf <http://rdaregistry.info/Elements/u/P60020> ;
    skos:definition "Relates a resource to a performer contributing to a resource by giving instruction or providing a demonstration."@en .

<http://rdaregistry.info/Elements/u/P60146>
    reg:hasSubproperty <http://rdaregistry.info/Elements/e/P20016> ;
    reg:lexicalAlias <http://rdaregistry.info/Elements/u/host.en> ;
    reg:name "host"@en ;
    reg:status <http://metadataregistry.org/uri/RegStatus/1001> ;
    a rdf:Property ;
    rdfs:isDefinedBy <http://rdaregistry.info/Elements/u/> ;
    rdfs:label "has host"@en ;
    rdfs:subPropertyOf <http://rdaregistry.info/Elements/u/P60387> ;
    owl:inverseOf <http://rdaregistry.info/Elements/u/P60021> ;
    skos:definition "Relates a resource to a performer contributing to a resource by leading a program, often broadcast, that includes other guests, performers, etc."@en .

<http://rdaregistry.info/Elements/u/P60147>
    reg:hasSubproperty <http://rdaregistry.info/Elements/e/P20017> ;
    reg:lexicalAlias <http://rdaregistry.info/Elements/u/moderator.en> ;
    reg:name "moderator"@en ;
    reg:status <http://metadataregistry.org/uri/RegStatus/1001> ;
    a rdf:Property ;
    rdfs:isDefinedBy <http://rdaregistry.info/Elements/u/> ;
    rdfs:label "has moderator"@en ;
    rdfs:subPropertyOf <http://rdaregistry.info/Elements/u/P60387> ;
    owl:inverseOf <http://rdaregistry.info/Elements/u/P60022> ;
    skos:definition "Relates a resource to a performer contributing to a resource by leading a program, often broadcast, where topics are discussed, usually with participation of experts in fields related to the discussion."@en .

<http://rdaregistry.info/Elements/u/P60148>
    reg:hasSubproperty <http://rdaregistry.info/Elements/e/P20018> ;
    reg:lexicalAlias <http://rdaregistry.info/Elements/u/puppeteer.en> ;
    reg:name "puppeteer"@en ;
    reg:status <http://metadataregistry.org/uri/RegStatus/1001> ;
    a rdf:Property ;
    rdfs:isDefinedBy <http://rdaregistry.info/Elements/u/> ;
    rdfs:label "has puppeteer"@en ;
    rdfs:subPropertyOf <http://rdaregistry.info/Elements/u/P60387> ;
    owl:inverseOf <http://rdaregistry.info/Elements/u/P60023> ;
    skos:definition "Relates a resource to a performer contributing to a resource by manipulating, controlling, or directing puppets or marionettes in a moving image production or a musical or dramatic presentation or entertainment."@en .

<http://rdaregistry.info/Elements/u/P60149>
    reg:hasSubproperty <http://rdaregistry.info/Elements/e/P20019> ;
    reg:lexicalAlias <http://rdaregistry.info/Elements/u/panelist.en> ;
    reg:name "panelist"@en ;
    reg:status <http://metadataregistry.org/uri/RegStatus/1001> ;
    a rdf:Property ;
    rdfs:isDefinedBy <http://rdaregistry.info/Elements/u/> ;
    rdfs:label "has panelist"@en ;
    rdfs:subPropertyOf <http://rdaregistry.info/Elements/u/P60387> ;
    owl:inverseOf <http://rdaregistry.info/Elements/u/P60024> ;
    skos:definition "Relates a resource to a performer contributing to a resource by participating in a program, often broadcast, where topics are discussed, usually with participation of experts in fields related to the discussion."@en .

<http://rdaregistry.info/Elements/u/P60150>
    reg:hasSubproperty <http://rdaregistry.info/Elements/e/P20020> ;
    reg:lexicalAlias <http://rdaregistry.info/Elements/u/instrumentalist.en> ;
    reg:name "instrumentalist"@en ;
    reg:status <http://metadataregistry.org/uri/RegStatus/1001> ;
    a rdf:Property ;
    rdfs:isDefinedBy <http://rdaregistry.info/Elements/u/> ;
    rdfs:label "has instrumentalist"@en ;
    rdfs:subPropertyOf <http://rdaregistry.info/Elements/u/P60387> ;
    owl:inverseOf <http://rdaregistry.info/Elements/u/P60025> ;
    skos:definition "Relates a resource to a performer contributing to a resource by playing a musical instrument."@en .

<http://rdaregistry.info/Elements/u/P60151>
    reg:hasSubproperty <http://rdaregistry.info/Elements/e/P20021> ;
    reg:lexicalAlias <http://rdaregistry.info/Elements/u/commentator.en> ;
    reg:name "commentator"@en ;
    reg:status <http://metadataregistry.org/uri/RegStatus/1001> ;
    a rdf:Property ;
    rdfs:isDefinedBy <http://rdaregistry.info/Elements/u/> ;
    rdfs:label "has commentator"@en ;
    rdfs:subPropertyOf <http://rdaregistry.info/Elements/u/P60387> ;
    owl:inverseOf <http://rdaregistry.info/Elements/u/P60026> ;
    skos:definition "Relates a resource to a performer contributing to a resource by providing interpretation, analysis, or a discussion of the subject matter on a recording, film, or other audiovisual medium."@en .

<http://rdaregistry.info/Elements/u/P60152>
    reg:hasSubproperty <http://rdaregistry.info/Elements/e/P20070> ;
    reg:lexicalAlias <http://rdaregistry.info/Elements/u/voiceActor.en> ;
    reg:name "voiceActor"@en ;
    reg:status <http://metadataregistry.org/uri/RegStatus/1001> ;
    a rdf:Property ;
    rdfs:isDefinedBy <http://rdaregistry.info/Elements/u/> ;
    rdfs:label "has voice actor"@en ;
    rdfs:subPropertyOf <http://rdaregistry.info/Elements/u/P60142> ;
    owl:inverseOf <http://rdaregistry.info/Elements/u/P60027> ;
    skos:definition "Relates a resource to a performer contributing to a resource by providing a voice for characters in radio and audio productions and for animated characters in moving image resources as well as by providing voice-overs in radio and television commercials, dubbed resources, etc."@en .

<http://rdaregistry.info/Elements/u/P60153>
    reg:hasSubproperty <http://rdaregistry.info/Elements/e/P20022> ;
    reg:lexicalAlias <http://rdaregistry.info/Elements/u/narrator.en> ;
    reg:name "narrator"@en ;
    reg:status <http://metadataregistry.org/uri/RegStatus/1001> ;
    a rdf:Property ;
    rdfs:isDefinedBy <http://rdaregistry.info/Elements/u/> ;
    rdfs:label "has narrator"@en ;
    rdfs:subPropertyOf <http://rdaregistry.info/Elements/u/P60387> ;
    owl:inverseOf <http://rdaregistry.info/Elements/u/P60028> ;
    skos:definition "Relates a resource to a performer contributing to a resource by reading aloud or giving an account of an act, occurrence, course of events, etc."@en .

<http://rdaregistry.info/Elements/u/P60154>
    reg:hasSubproperty <http://rdaregistry.info/Elements/e/P20023> ;
    reg:lexicalAlias <http://rdaregistry.info/Elements/u/storyteller.en> ;
    reg:name "storyteller"@en ;
    reg:status <http://metadataregistry.org/uri/RegStatus/1001> ;
    a rdf:Property ;
    rdfs:isDefinedBy <http://rdaregistry.info/Elements/u/> ;
    rdfs:label "has storyteller"@en ;
    rdfs:subPropertyOf <http://rdaregistry.info/Elements/u/P60387> ;
    owl:inverseOf <http://rdaregistry.info/Elements/u/P60029> ;
    skos:definition "Relates a resource to a performer contributing to a resource by relaying a creator's original story with dramatic or theatrical interpretation."@en .

<http://rdaregistry.info/Elements/u/P60155>
    reg:hasSubproperty <http://rdaregistry.info/Elements/e/P20024> ;
    reg:lexicalAlias <http://rdaregistry.info/Elements/u/speaker.en> ;
    reg:name "speaker"@en ;
    reg:status <http://metadataregistry.org/uri/RegStatus/1001> ;
    a rdf:Property ;
    rdfs:isDefinedBy <http://rdaregistry.info/Elements/u/> ;
    rdfs:label "has speaker"@en ;
    rdfs:subPropertyOf <http://rdaregistry.info/Elements/u/P60387> ;
    owl:inverseOf <http://rdaregistry.info/Elements/u/P60030> ;
    skos:definition "Relates a resource to a performer contributing to a resource by speaking words, such as a lecture, speech, etc."@en .

<http://rdaregistry.info/Elements/u/P60156>
    reg:hasSubproperty <http://rdaregistry.info/Elements/e/P20025> ;
    reg:lexicalAlias <http://rdaregistry.info/Elements/u/singer.en> ;
    reg:name "singer"@en ;
    reg:status <http://metadataregistry.org/uri/RegStatus/1001> ;
    a rdf:Property ;
    rdfs:isDefinedBy <http://rdaregistry.info/Elements/u/> ;
    rdfs:label "has singer"@en ;
    rdfs:subPropertyOf <http://rdaregistry.info/Elements/u/P60387> ;
    owl:inverseOf <http://rdaregistry.info/Elements/u/P60031> ;
    skos:definition "Relates a resource to a performer contributing to a resource by using his/her/their voice, with or without instrumental accompaniment, to produce music. a singers performance may or may not include actual words."@en .

<http://rdaregistry.info/Elements/u/P60157>
    reg:lexicalAlias <http://rdaregistry.info/Elements/u/medium.en> ;
    reg:name "medium"@en ;
    reg:status <http://metadataregistry.org/uri/RegStatus/1001> ;
    a rdf:Property ;
    rdfs:isDefinedBy <http://rdaregistry.info/Elements/u/> ;
    rdfs:label "has medium"@en ;
    rdfs:subPropertyOf <http://rdaregistry.info/Elements/u/P60374> ;
    owl:inverseOf <http://rdaregistry.info/Elements/u/P60032> ;
    skos:definition "Relates a resource to an agent held to be a channel of communication between the earthly world and a world of spirits."@en .

<http://rdaregistry.info/Elements/u/P60158>
    reg:hasSubproperty <http://rdaregistry.info/Elements/u/P60884>, <http://rdaregistry.info/Elements/u/P60886>, <http://rdaregistry.info/Elements/u/P60887>, <http://rdaregistry.info/Elements/u/P60888>, <http://rdaregistry.info/Elements/u/P60890> ;
    reg:status <http://metadataregistry.org/uri/RegStatus/1008> ;
    rdfs:isDefinedBy <http://rdaregistry.info/Elements/u/> .

<http://rdaregistry.info/Elements/u/P60159>
    reg:hasSubproperty <http://rdaregistry.info/Elements/m/P30084>, <http://rdaregistry.info/Elements/u/P60344> ;
    reg:lexicalAlias <http://rdaregistry.info/Elements/u/appliedMaterial.en> ;
    reg:name "appliedMaterial"@en ;
    reg:status <http://metadataregistry.org/uri/RegStatus/1001> ;
    a rdf:Property ;
    rdfs:isDefinedBy <http://rdaregistry.info/Elements/u/> ;
    rdfs:label "has applied material"@en ;
    skos:definition "Relates a resource to a physical or chemical substance applied to a base material of a resource."@en .

<http://rdaregistry.info/Elements/u/P60160>
    reg:hasSubproperty <http://rdaregistry.info/Elements/m/P30085> ;
    reg:lexicalAlias <http://rdaregistry.info/Elements/u/placeOfDistribution.en> ;
    reg:name "placeOfDistribution"@en ;
    reg:status <http://metadataregistry.org/uri/RegStatus/1001> ;
    a rdf:Property ;
    rdfs:isDefinedBy <http://rdaregistry.info/Elements/u/> ;
    rdfs:label "has place of distribution"@en ;
    skos:definition "Relates a resource to a place associated with a distribution of a resource in a published form."@en .

<http://rdaregistry.info/Elements/u/P60161>
    reg:hasSubproperty <http://rdaregistry.info/Elements/m/P30086> ;
    reg:lexicalAlias <http://rdaregistry.info/Elements/u/placeOfProduction.en> ;
    reg:name "placeOfProduction"@en ;
    reg:status <http://metadataregistry.org/uri/RegStatus/1001> ;
    a rdf:Property ;
    rdfs:isDefinedBy <http://rdaregistry.info/Elements/u/> ;
    rdfs:label "has place of production"@en ;
    skos:definition "Relates a resource to a place associated with the inscription, fabrication, construction, etc., of a resource in an unpublished form."@en .

<http://rdaregistry.info/Elements/u/P60162>
    reg:hasSubproperty <http://rdaregistry.info/Elements/m/P30087> ;
    reg:lexicalAlias <http://rdaregistry.info/Elements/u/placeOfManufacture.en> ;
    reg:name "placeOfManufacture"@en ;
    reg:status <http://metadataregistry.org/uri/RegStatus/1001> ;
    a rdf:Property ;
    rdfs:isDefinedBy <http://rdaregistry.info/Elements/u/> ;
    rdfs:label "has place of manufacture"@en ;
    skos:definition "Relates a resource to a place associated with the printing, duplicating, casting, etc., of a resource in a published form."@en .

<http://rdaregistry.info/Elements/u/P60163>
    reg:hasSubproperty <http://rdaregistry.info/Elements/m/P30088> ;
    reg:lexicalAlias <http://rdaregistry.info/Elements/u/placeOfPublication.en> ;
    reg:name "placeOfPublication"@en ;
    reg:status <http://metadataregistry.org/uri/RegStatus/1001> ;
    a rdf:Property ;
    rdfs:isDefinedBy <http://rdaregistry.info/Elements/u/> ;
    rdfs:label "has place of publication"@en ;
    skos:definition "Relates a resource to a place associated with the publication, release, or issuing of a resource."@en .

<http://rdaregistry.info/Elements/u/P60164>
    reg:hasSubproperty <http://rdaregistry.info/Elements/m/P30089> ;
    reg:lexicalAlias <http://rdaregistry.info/Elements/u/parallelPlaceOfDistribution.en> ;
    reg:name "parallelPlaceOfDistribution"@en ;
    reg:status <http://metadataregistry.org/uri/RegStatus/1001> ;
    a rdf:Property ;
    rdfs:isDefinedBy <http://rdaregistry.info/Elements/u/> ;
    rdfs:label "has parallel place of distribution"@en ;
    skos:definition "Relates a resource to a place of distribution in a language or script that differs from that recorded in a place of distribution element."@en .

<http://rdaregistry.info/Elements/u/P60165>
    reg:hasSubproperty <http://rdaregistry.info/Elements/m/P30090> ;
    reg:lexicalAlias <http://rdaregistry.info/Elements/u/parallelPlaceOfManufacture.en> ;
    reg:name "parallelPlaceOfManufacture"@en ;
    reg:status <http://metadataregistry.org/uri/RegStatus/1001> ;
    a rdf:Property ;
    rdfs:isDefinedBy <http://rdaregistry.info/Elements/u/> ;
    rdfs:label "has parallel place of manufacture"@en ;
    skos:definition "Relates a resource to a place of manufacture in a language or script that differs from that recorded in a place of manufacture element."@en .

<http://rdaregistry.info/Elements/u/P60166>
    reg:hasSubproperty <http://rdaregistry.info/Elements/m/P30091> ;
    reg:lexicalAlias <http://rdaregistry.info/Elements/u/parallelPlaceOfProduction.en> ;
    reg:name "parallelPlaceOfProduction"@en ;
    reg:status <http://metadataregistry.org/uri/RegStatus/1001> ;
    a rdf:Property ;
    rdfs:isDefinedBy <http://rdaregistry.info/Elements/u/> ;
    rdfs:label "has parallel place of production"@en ;
    skos:definition "Relates a resource to a place of production in a language or script that differs from that recorded in a place of production element."@en .

<http://rdaregistry.info/Elements/u/P60167>
    reg:hasSubproperty <http://rdaregistry.info/Elements/m/P30092> ;
    reg:lexicalAlias <http://rdaregistry.info/Elements/u/parallelPlaceOfPublication.en> ;
    reg:name "parallelPlaceOfPublication"@en ;
    reg:status <http://metadataregistry.org/uri/RegStatus/1001> ;
    a rdf:Property ;
    rdfs:isDefinedBy <http://rdaregistry.info/Elements/u/> ;
    rdfs:label "has parallel place of publication"@en ;
    skos:definition "Relates a resource to a place of publication in a language or script that differs from that recorded in a place of publication element."@en .

<http://rdaregistry.info/Elements/u/P60168>
    reg:hasSubproperty <http://rdaregistry.info/Elements/i/P40038>, <http://rdaregistry.info/Elements/m/P30093> ;
    reg:lexicalAlias <http://rdaregistry.info/Elements/u/reprintOf.en> ;
    reg:name "reprintOf"@en ;
    reg:status <http://metadataregistry.org/uri/RegStatus/1001> ;
    a rdf:Property ;
    rdfs:isDefinedBy <http://rdaregistry.info/Elements/u/> ;
    rdfs:label "is reprint of"@en ;
    rdfs:subPropertyOf <http://rdaregistry.info/Elements/u/P60297> ;
    owl:inverseOf <http://rdaregistry.info/Elements/u/P60271> ;
    skos:definition "Relates a resource to a resource that reissues the same resource as a printed resource being described."@en .

<http://rdaregistry.info/Elements/u/P60169>
    reg:lexicalAlias <http://rdaregistry.info/Elements/u/filmProducer.en> ;
    reg:name "filmProducer"@en ;
    reg:status <http://metadataregistry.org/uri/RegStatus/1001> ;
    a rdf:Property ;
    rdfs:isDefinedBy <http://rdaregistry.info/Elements/u/> ;
    rdfs:label "has film producer"@en ;
    rdfs:subPropertyOf <http://rdaregistry.info/Elements/u/P60441> ;
    owl:inverseOf <http://rdaregistry.info/Elements/u/P60033> ;
    skos:definition "Relates a resource to a producer responsible for most of the business aspects of a film."@en .

<http://rdaregistry.info/Elements/u/P60170>
    reg:lexicalAlias <http://rdaregistry.info/Elements/u/radioProducer.en> ;
    reg:name "radioProducer"@en ;
    reg:status <http://metadataregistry.org/uri/RegStatus/1001> ;
    a rdf:Property ;
    rdfs:isDefinedBy <http://rdaregistry.info/Elements/u/> ;
    rdfs:label "has radio producer"@en ;
    rdfs:subPropertyOf <http://rdaregistry.info/Elements/u/P60441> ;
    owl:inverseOf <http://rdaregistry.info/Elements/u/P60034> ;
    skos:definition "Relates a resource to a producer responsible for most of the business aspects of a radio program."@en .

<http://rdaregistry.info/Elements/u/P60171>
    reg:lexicalAlias <http://rdaregistry.info/Elements/u/televisionProducer.en> ;
    reg:name "televisionProducer"@en ;
    reg:status <http://metadataregistry.org/uri/RegStatus/1001> ;
    a rdf:Property ;
    rdfs:isDefinedBy <http://rdaregistry.info/Elements/u/> ;
    rdfs:label "has television producer"@en ;
    rdfs:subPropertyOf <http://rdaregistry.info/Elements/u/P60441> ;
    owl:inverseOf <http://rdaregistry.info/Elements/u/P60035> ;
    skos:definition "Relates a resource to a producer responsible for most of the business aspects of a television program."@en .

<http://rdaregistry.info/Elements/u/P60172>
    reg:hasSubproperty <http://rdaregistry.info/Elements/m/P30094> ;
    reg:lexicalAlias <http://rdaregistry.info/Elements/u/parallelProducersName.en> ;
    reg:name "parallelProducersName"@en ;
    reg:status <http://metadataregistry.org/uri/RegStatus/1001> ;
    a rdf:Property ;
    rdfs:isDefinedBy <http://rdaregistry.info/Elements/u/> ;
    rdfs:label "has parallel producers name"@en ;
    skos:definition "Relates a resource to a producer's name in a language or script that differs from that recorded in a producer's name element."@en .

<http://rdaregistry.info/Elements/u/P60173>
    reg:hasSubproperty <http://rdaregistry.info/Elements/m/P30095> ;
    reg:lexicalAlias <http://rdaregistry.info/Elements/u/parallelPublishersName.en> ;
    reg:name "parallelPublishersName"@en ;
    reg:status <http://metadataregistry.org/uri/RegStatus/1001> ;
    a rdf:Property ;
    rdfs:isDefinedBy <http://rdaregistry.info/Elements/u/> ;
    rdfs:label "has parallel publishers name"@en ;
    skos:definition "Relates a resource to a publisher's name in a language or script that differs from that recorded in a publisher's name element."@en .

<http://rdaregistry.info/Elements/u/P60174>
    reg:hasSubproperty <http://rdaregistry.info/Elements/e/P20060> ;
    reg:lexicalAlias <http://rdaregistry.info/Elements/u/adaptedAsARadioProgram.en> ;
    reg:name "adaptedAsARadioProgram"@en ;
    reg:status <http://metadataregistry.org/uri/RegStatus/1001> ;
    a rdf:Property ;
    rdfs:isDefinedBy <http://rdaregistry.info/Elements/u/> ;
    rdfs:label "is adapted as radio program"@en ;
    rdfs:subPropertyOf <http://rdaregistry.info/Elements/u/P60260> ;
    owl:inverseOf <http://rdaregistry.info/Elements/u/P60229> ;
    skos:definition "Relates a resource to a radio program based on a source resource."@en .

<http://rdaregistry.info/Elements/u/P60175>
    reg:lexicalAlias <http://rdaregistry.info/Elements/u/academicDegree.en> ;
    reg:name "academicDegree"@en ;
    reg:status <http://metadataregistry.org/uri/RegStatus/1001> ;
    a rdf:Property ;
    rdfs:isDefinedBy <http://rdaregistry.info/Elements/u/> ;
    rdfs:label "has academic degree"@en ;
    skos:definition "Relates a resource to a rank conferred as a guarantee of academic proficiency."@en .

<http://rdaregistry.info/Elements/u/P60176>
    reg:hasSubproperty <http://rdaregistry.info/Elements/i/P40026> ;
    reg:lexicalAlias <http://rdaregistry.info/Elements/u/custodialHistoryOfResource.en> ;
    reg:name "custodialHistoryOfResource"@en ;
    reg:status <http://metadataregistry.org/uri/RegStatus/1001> ;
    a rdf:Property ;
    rdfs:isDefinedBy <http://rdaregistry.info/Elements/u/> ;
    rdfs:label "has custodial history of resource"@en ;
    skos:definition "Relates a resource to a record of previous ownership or custodianship of a resource."@en .

<http://rdaregistry.info/Elements/u/P60177>
    reg:hasSubproperty <http://rdaregistry.info/Elements/e/P20090> ;
    reg:lexicalAlias <http://rdaregistry.info/Elements/u/abstractedIn.en> ;
    reg:name "abstractedIn"@en ;
    reg:status <http://metadataregistry.org/uri/RegStatus/1001> ;
    a rdf:Property ;
    rdfs:isDefinedBy <http://rdaregistry.info/Elements/u/> ;
    rdfs:label "is abstracted in"@en ;
    rdfs:subPropertyOf <http://rdaregistry.info/Elements/u/P60250> ;
    owl:inverseOf <http://rdaregistry.info/Elements/u/P60308> ;
    skos:definition "Relates a resource to a resource that is an abstracting and indexing service that abstracts the contents of a source entity."@en .

<http://rdaregistry.info/Elements/u/P60178>
    reg:hasSubproperty <http://rdaregistry.info/Elements/e/P20091> ;
    reg:lexicalAlias <http://rdaregistry.info/Elements/u/indexedIn.en> ;
    reg:name "indexedIn"@en ;
    reg:status <http://metadataregistry.org/uri/RegStatus/1001> ;
    a rdf:Property ;
    rdfs:isDefinedBy <http://rdaregistry.info/Elements/u/> ;
    rdfs:label "is indexed in"@en ;
    rdfs:subPropertyOf <http://rdaregistry.info/Elements/u/P60250> ;
    owl:inverseOf <http://rdaregistry.info/Elements/u/P60309> ;
    skos:definition "Relates a resource to a resource that is an abstracting and indexing service that indexes the contents of a source resource."@en .

<http://rdaregistry.info/Elements/u/P60179>
    reg:hasSubproperty <http://rdaregistry.info/Elements/i/P40059>, <http://rdaregistry.info/Elements/m/P30021> ;
    reg:lexicalAlias <http://rdaregistry.info/Elements/u/preservationFacsimile.en> ;
    reg:name "preservationFacsimile"@en ;
    reg:status <http://metadataregistry.org/uri/RegStatus/1001> ;
    a rdf:Property ;
    rdfs:isDefinedBy <http://rdaregistry.info/Elements/u/> ;
    rdfs:label "has preservation facsimile"@en ;
    rdfs:subPropertyOf <http://rdaregistry.info/Elements/u/P60217> ;
    owl:inverseOf <http://rdaregistry.info/Elements/u/P60299> ;
    skos:definition "Relates a resource to a resource that consists of an exact reproduction on preservation-quality media, such as acid-free permanent or archival paper."@en .

<http://rdaregistry.info/Elements/u/P60180>
    reg:hasSubproperty <http://rdaregistry.info/Elements/e/P20092> ;
    reg:lexicalAlias <http://rdaregistry.info/Elements/u/adaptedAsChoreography.en> ;
    reg:name "adaptedAsChoreography"@en ;
    reg:status <http://metadataregistry.org/uri/RegStatus/1001> ;
    a rdf:Property ;
    rdfs:isDefinedBy <http://rdaregistry.info/Elements/u/> ;
    rdfs:label "is adapted as choreography"@en ;
    rdfs:subPropertyOf <http://rdaregistry.info/Elements/u/P60250> ;
    owl:inverseOf <http://rdaregistry.info/Elements/u/P60293> ;
    skos:definition "Relates a resource to a resource consisting of movement based on a source resource."@en .

<http://rdaregistry.info/Elements/u/P60181>
    reg:hasSubproperty <http://rdaregistry.info/Elements/e/P20093> ;
    reg:lexicalAlias <http://rdaregistry.info/Elements/u/errata.en> ;
    reg:name "errata"@en ;
    reg:status <http://metadataregistry.org/uri/RegStatus/1001> ;
    a rdf:Property ;
    rdfs:isDefinedBy <http://rdaregistry.info/Elements/u/> ;
    rdfs:label "is errata"@en ;
    rdfs:subPropertyOf <http://rdaregistry.info/Elements/u/P60204> ;
    owl:inverseOf <http://rdaregistry.info/Elements/u/P60251> ;
    skos:definition "Relates a resource to a resource consisting of errors discovered after the publication of a predominant resource, with their corrections."@en .

<http://rdaregistry.info/Elements/u/P60182>
    reg:hasSubproperty <http://rdaregistry.info/Elements/e/P20094> ;
    reg:lexicalAlias <http://rdaregistry.info/Elements/u/illustrations.en> ;
    reg:name "illustrations"@en ;
    reg:status <http://metadataregistry.org/uri/RegStatus/1001> ;
    a rdf:Property ;
    rdfs:isDefinedBy <http://rdaregistry.info/Elements/u/> ;
    rdfs:label "is illustrations"@en ;
    rdfs:subPropertyOf <http://rdaregistry.info/Elements/u/P60204> ;
    owl:inverseOf <http://rdaregistry.info/Elements/u/P60254> ;
    skos:definition "Relates a resource to a resource consisting of pictorial content designed to explain or decorate an augmented resource."@en .

<http://rdaregistry.info/Elements/u/P60183>
    reg:hasSubproperty <http://rdaregistry.info/Elements/m/P30022> ;
    reg:lexicalAlias <http://rdaregistry.info/Elements/u/insert.en> ;
    reg:name "insert"@en ;
    reg:status <http://metadataregistry.org/uri/RegStatus/1001> ;
    a rdf:Property ;
    rdfs:isDefinedBy <http://rdaregistry.info/Elements/u/> ;
    rdfs:label "is insert"@en ;
    rdfs:subPropertyOf <http://rdaregistry.info/Elements/u/P60249> ;
    owl:inverseOf <http://rdaregistry.info/Elements/u/P60194> ;
    skos:definition "Relates a resource to a resource in which a part has been issued; a title of a larger resource appears on a part."@en .

<http://rdaregistry.info/Elements/u/P60184>
    reg:hasSubproperty <http://rdaregistry.info/Elements/e/P20095> ;
    reg:lexicalAlias <http://rdaregistry.info/Elements/u/adaptedAsAMotionPictureScreenplay.en> ;
    reg:name "adaptedAsAMotionPictureScreenplay"@en ;
    reg:status <http://metadataregistry.org/uri/RegStatus/1001> ;
    a rdf:Property ;
    rdfs:isDefinedBy <http://rdaregistry.info/Elements/u/> ;
    rdfs:label "is adapted as motion picture screenplay"@en ;
    rdfs:subPropertyOf <http://rdaregistry.info/Elements/u/P60185> ;
    owl:inverseOf <http://rdaregistry.info/Elements/u/P60232> ;
    skos:definition "Relates a resource to a resource consisting of a screenplay for a motion picture, based on a source resource."@en .

<http://rdaregistry.info/Elements/u/P60185>
    reg:hasSubproperty <http://rdaregistry.info/Elements/e/P20096>, <http://rdaregistry.info/Elements/u/P60184>, <http://rdaregistry.info/Elements/u/P60186>, <http://rdaregistry.info/Elements/u/P60187> ;
    reg:lexicalAlias <http://rdaregistry.info/Elements/u/adaptedAsScreenplay.en> ;
    reg:name "adaptedAsScreenplay"@en ;
    reg:status <http://metadataregistry.org/uri/RegStatus/1001> ;
    a rdf:Property ;
    rdfs:isDefinedBy <http://rdaregistry.info/Elements/u/> ;
    rdfs:label "is adapted as screenplay"@en ;
    rdfs:subPropertyOf <http://rdaregistry.info/Elements/u/P60260> ;
    owl:inverseOf <http://rdaregistry.info/Elements/u/P60231> ;
    skos:definition "Relates a resource to a resource consisting of a screenplay for a motion picture, television program, or video, based on a source resource."@en .

<http://rdaregistry.info/Elements/u/P60186>
    reg:hasSubproperty <http://rdaregistry.info/Elements/e/P20097> ;
    reg:lexicalAlias <http://rdaregistry.info/Elements/u/adaptedAsATelevisionScreenplay.en> ;
    reg:name "adaptedAsATelevisionScreenplay"@en ;
    reg:status <http://metadataregistry.org/uri/RegStatus/1001> ;
    a rdf:Property ;
    rdfs:isDefinedBy <http://rdaregistry.info/Elements/u/> ;
    rdfs:label "is adapted as television screenplay"@en ;
    rdfs:subPropertyOf <http://rdaregistry.info/Elements/u/P60185> ;
    owl:inverseOf <http://rdaregistry.info/Elements/u/P60233> ;
    skos:definition "Relates a resource to a resource consisting of a screenplay for a television program, based on a source resource."@en .

<http://rdaregistry.info/Elements/u/P60187>
    reg:hasSubproperty <http://rdaregistry.info/Elements/e/P20098> ;
    reg:lexicalAlias <http://rdaregistry.info/Elements/u/adaptedAsAVideoScreenplay.en> ;
    reg:name "adaptedAsAVideoScreenplay"@en ;
    reg:status <http://metadataregistry.org/uri/RegStatus/1001> ;
    a rdf:Property ;
    rdfs:isDefinedBy <http://rdaregistry.info/Elements/u/> ;
    rdfs:label "is adapted as video screenplay"@en ;
    rdfs:subPropertyOf <http://rdaregistry.info/Elements/u/P60185> ;
    owl:inverseOf <http://rdaregistry.info/Elements/u/P60234> ;
    skos:definition "Relates a resource to a resource consisting of a screenplay for a video, based on a source resource."@en .

<http://rdaregistry.info/Elements/u/P60188>
    reg:hasSubproperty <http://rdaregistry.info/Elements/e/P20099> ;
    reg:lexicalAlias <http://rdaregistry.info/Elements/u/adaptedAsARadioScript.en> ;
    reg:name "adaptedAsARadioScript"@en ;
    reg:status <http://metadataregistry.org/uri/RegStatus/1001> ;
    a rdf:Property ;
    rdfs:isDefinedBy <http://rdaregistry.info/Elements/u/> ;
    rdfs:label "is adapted as radio script"@en ;
    rdfs:subPropertyOf <http://rdaregistry.info/Elements/u/P60260> ;
    owl:inverseOf <http://rdaregistry.info/Elements/u/P60235> ;
    skos:definition "Relates a resource to a resource consisting of a script for a radio program, based on a source resource."@en .

<http://rdaregistry.info/Elements/u/P60189>
    reg:hasSubproperty <http://rdaregistry.info/Elements/e/P20119> ;
    reg:lexicalAlias <http://rdaregistry.info/Elements/u/freelyTranslatedAs.en> ;
    reg:name "freelyTranslatedAs"@en ;
    reg:status <http://metadataregistry.org/uri/RegStatus/1001> ;
    a rdf:Property ;
    rdfs:isDefinedBy <http://rdaregistry.info/Elements/u/> ;
    rdfs:label "is freely translated as"@en ;
    rdfs:subPropertyOf <http://rdaregistry.info/Elements/u/P60250> ;
    owl:inverseOf <http://rdaregistry.info/Elements/u/P60243> ;
    skos:definition "Relates a resource to a resource that is both an adaptation and a translation into another language of a source resource."@en .

<http://rdaregistry.info/Elements/u/P60190>
    reg:hasSubproperty <http://rdaregistry.info/Elements/u/P60239>, <http://rdaregistry.info/Elements/u/P60255>, <http://rdaregistry.info/Elements/u/P60288>, <http://rdaregistry.info/Elements/u/P60292>, <http://rdaregistry.info/Elements/u/P60298>, <http://rdaregistry.info/Elements/w/P10265>, <http://rdaregistry.info/Elements/w/P10271>, <http://rdaregistry.info/Elements/w/P10277>, <http://rdaregistry.info/Elements/w/P10325>, <http://rdaregistry.info/Elements/w/P10326>, <http://rdaregistry.info/Elements/w/P10327> ;
    reg:lexicalAlias <http://rdaregistry.info/Elements/u/descriptionOf.en> ;
    reg:name "descriptionOf"@en ;
    reg:status <http://metadataregistry.org/uri/RegStatus/1001> ;
    a rdf:Property ;
    rdfs:isDefinedBy <http://rdaregistry.info/Elements/u/> ;
    rdfs:label "is description of"@en ;
    rdfs:subPropertyOf <http://rdaregistry.info/Elements/u/P60805> ;
    owl:inverseOf <http://rdaregistry.info/Elements/u/P60215> ;
    skos:definition "Relates a resource to a resource described by a describing entity."@en .

<http://rdaregistry.info/Elements/u/P60191>
    reg:hasSubproperty <http://rdaregistry.info/Elements/i/P40031>, <http://rdaregistry.info/Elements/m/P30024>, <http://rdaregistry.info/Elements/u/P60195>, <http://rdaregistry.info/Elements/u/P60197>, <http://rdaregistry.info/Elements/u/P60272>, <http://rdaregistry.info/Elements/u/P60297> ;
    reg:lexicalAlias <http://rdaregistry.info/Elements/u/equivalent.en> ;
    reg:name "equivalent"@en ;
    reg:status <http://metadataregistry.org/uri/RegStatus/1001> ;
    a rdf:Property ;
    rdfs:isDefinedBy <http://rdaregistry.info/Elements/u/> ;
    rdfs:label "has equivalent"@en ;
    rdfs:subPropertyOf <http://rdaregistry.info/Elements/u/P60712> ;
    owl:inverseOf <http://rdaregistry.info/Elements/u/P60191> ;
    skos:definition "Relates a resource to a resource that carries the same content as a resource."@en .

<http://rdaregistry.info/Elements/u/P60192>
    reg:lexicalAlias <http://rdaregistry.info/Elements/u/subseriesOf.en> ;
    reg:name "subseriesOf"@en ;
    reg:status <http://metadataregistry.org/uri/RegStatus/1001> ;
    a rdf:Property ;
    rdfs:isDefinedBy <http://rdaregistry.info/Elements/u/> ;
    rdfs:label "is subseries of"@en ;
    rdfs:subPropertyOf <http://rdaregistry.info/Elements/u/P60101> ;
    owl:inverseOf <http://rdaregistry.info/Elements/u/P60316> ;
    skos:definition "Relates a resource to a resource in which a part consistently appears; a title of the larger resource appears on all issues or parts of a subseries."@en .

<http://rdaregistry.info/Elements/u/P60193>
    reg:lexicalAlias <http://rdaregistry.info/Elements/u/inSeries.en> ;
    reg:name "inSeries"@en ;
    reg:status <http://metadataregistry.org/uri/RegStatus/1001> ;
    a rdf:Property ;
    rdfs:isDefinedBy <http://rdaregistry.info/Elements/u/> ;
    rdfs:label "is in series"@en ;
    rdfs:subPropertyOf <http://rdaregistry.info/Elements/u/P60101> ;
    owl:inverseOf <http://rdaregistry.info/Elements/u/P60240> ;
    skos:definition "Relates a resource to a resource in which a part has been issued; a title of a larger resource appears on a part."@en .

<http://rdaregistry.info/Elements/u/P60194>
    reg:hasSubproperty <http://rdaregistry.info/Elements/m/P30025> ;
    reg:lexicalAlias <http://rdaregistry.info/Elements/u/insertedIn.en> ;
    reg:name "insertedIn"@en ;
    reg:status <http://metadataregistry.org/uri/RegStatus/1001> ;
    a rdf:Property ;
    rdfs:isDefinedBy <http://rdaregistry.info/Elements/u/> ;
    rdfs:label "is inserted in"@en ;
    rdfs:subPropertyOf <http://rdaregistry.info/Elements/u/P60101> ;
    owl:inverseOf <http://rdaregistry.info/Elements/u/P60183> ;
    skos:definition "Relates a resource to a resource into which material has been inserted that is not an integral part of the publication."@en .

<http://rdaregistry.info/Elements/u/P60195>
    reg:hasSubproperty <http://rdaregistry.info/Elements/m/P30026> ;
    reg:lexicalAlias <http://rdaregistry.info/Elements/u/alsoIssuedAs.en> ;
    reg:name "alsoIssuedAs"@en ;
    reg:status <http://metadataregistry.org/uri/RegStatus/1001> ;
    a rdf:Property ;
    rdfs:isDefinedBy <http://rdaregistry.info/Elements/u/> ;
    rdfs:label "is also issued as"@en ;
    rdfs:subPropertyOf <http://rdaregistry.info/Elements/u/P60191> ;
    owl:inverseOf <http://rdaregistry.info/Elements/u/P60195> ;
    skos:definition "Relates a resource to a resource that carries the same content of a resource in a different format."@en .

<http://rdaregistry.info/Elements/u/P60196>
    reg:hasSubproperty <http://rdaregistry.info/Elements/i/P40029>, <http://rdaregistry.info/Elements/m/P30027>, <http://rdaregistry.info/Elements/u/P60237>, <http://rdaregistry.info/Elements/u/P60256> ;
    reg:lexicalAlias <http://rdaregistry.info/Elements/u/accompaniedBy.en> ;
    reg:name "accompaniedBy"@en ;
    reg:status <http://metadataregistry.org/uri/RegStatus/1001> ;
    a rdf:Property ;
    rdfs:isDefinedBy <http://rdaregistry.info/Elements/u/> ;
    rdfs:label "is accompanied by"@en ;
    rdfs:subPropertyOf <http://rdaregistry.info/Elements/u/P60709> ;
    owl:inverseOf <http://rdaregistry.info/Elements/u/P60196> ;
    skos:definition "Relates a resource to a resource issued with another resource, without any relationship to its content."@en .

<http://rdaregistry.info/Elements/u/P60197>
    reg:hasSubproperty <http://rdaregistry.info/Elements/m/P30028> ;
    reg:lexicalAlias <http://rdaregistry.info/Elements/u/mirrorSite.en> ;
    reg:name "mirrorSite"@en ;
    reg:status <http://metadataregistry.org/uri/RegStatus/1001> ;
    a rdf:Property ;
    rdfs:isDefinedBy <http://rdaregistry.info/Elements/u/> ;
    rdfs:label "is mirror site"@en ;
    rdfs:subPropertyOf <http://rdaregistry.info/Elements/u/P60191> ;
    owl:inverseOf <http://rdaregistry.info/Elements/u/P60197> ;
    skos:definition "Relates a resource to a resource that is an exact copy of a website, used to reduce network traffic or improve the availability of the content of the original site."@en .

<http://rdaregistry.info/Elements/u/P60198>
    reg:hasSubproperty <http://rdaregistry.info/Elements/e/P20100>, <http://rdaregistry.info/Elements/u/P60117>, <http://rdaregistry.info/Elements/u/P60201>, <http://rdaregistry.info/Elements/u/P60264>, <http://rdaregistry.info/Elements/u/P60267>, <http://rdaregistry.info/Elements/u/P60270>, <http://rdaregistry.info/Elements/u/P60285>, <http://rdaregistry.info/Elements/u/P60740>, <http://rdaregistry.info/Elements/u/P60741> ;
    reg:lexicalAlias <http://rdaregistry.info/Elements/u/complementedBy.en> ;
    reg:name "complementedBy"@en ;
    reg:status <http://metadataregistry.org/uri/RegStatus/1001> ;
    a rdf:Property ;
    rdfs:isDefinedBy <http://rdaregistry.info/Elements/u/> ;
    rdfs:label "is complemented by"@en ;
    rdfs:subPropertyOf <http://rdaregistry.info/Elements/u/P60709> ;
    owl:inverseOf <http://rdaregistry.info/Elements/u/P60198> ;
    skos:definition "Relates a resource to a resource paired with another resource without either resource being considered to predominate."@en .

<http://rdaregistry.info/Elements/u/P60199>
    reg:hasSubproperty <http://rdaregistry.info/Elements/e/P20101> ;
    reg:lexicalAlias <http://rdaregistry.info/Elements/u/continuedInPartBy.en> ;
    reg:name "continuedInPartBy"@en ;
    reg:status <http://metadataregistry.org/uri/RegStatus/1001> ;
    a rdf:Property ;
    rdfs:isDefinedBy <http://rdaregistry.info/Elements/u/> ;
    rdfs:label "is continued in part by"@en ;
    rdfs:subPropertyOf <http://rdaregistry.info/Elements/u/P60278> ;
    owl:inverseOf <http://rdaregistry.info/Elements/u/P60277> ;
    skos:definition "Relates a resource to a resource part of whose content separated from an earlier resource to form a new resource."@en ;
    skos:scopeNote "This relationship applies generally to serials."@en .

<http://rdaregistry.info/Elements/u/P60200>
    reg:hasSubproperty <http://rdaregistry.info/Elements/i/P40056>, <http://rdaregistry.info/Elements/m/P30029> ;
    reg:lexicalAlias <http://rdaregistry.info/Elements/u/digitalTransfer.en> ;
    reg:name "digitalTransfer"@en ;
    reg:status <http://metadataregistry.org/uri/RegStatus/1001> ;
    a rdf:Property ;
    rdfs:isDefinedBy <http://rdaregistry.info/Elements/u/> ;
    rdfs:label "has digital transfer"@en ;
    rdfs:subPropertyOf <http://rdaregistry.info/Elements/u/P60272> ;
    owl:inverseOf <http://rdaregistry.info/Elements/u/P60287> ;
    skos:definition "Relates a resource to a resource in a digital format that results from a transfer of a resource in another digital format."@en .

<http://rdaregistry.info/Elements/u/P60201>
    reg:hasSubproperty <http://rdaregistry.info/Elements/e/P20102>, <http://rdaregistry.info/Elements/u/P60282>, <http://rdaregistry.info/Elements/u/P60283>, <http://rdaregistry.info/Elements/u/P60284> ;
    reg:lexicalAlias <http://rdaregistry.info/Elements/u/screenplayFor.en> ;
    reg:name "screenplayFor"@en ;
    reg:status <http://metadataregistry.org/uri/RegStatus/1001> ;
    a rdf:Property ;
    rdfs:isDefinedBy <http://rdaregistry.info/Elements/u/> ;
    rdfs:label "is screenplay for"@en ;
    rdfs:subPropertyOf <http://rdaregistry.info/Elements/u/P60198> ;
    owl:inverseOf <http://rdaregistry.info/Elements/u/P60264> ;
    skos:definition "Relates a resource to a resource such as a motion picture, television program, or video, that uses a text of a resource as a screenplay."@en .

<http://rdaregistry.info/Elements/u/P60202>
    reg:hasSubproperty <http://rdaregistry.info/Elements/e/P20103> ;
    reg:lexicalAlias <http://rdaregistry.info/Elements/u/incidentalMusicFor.en> ;
    reg:name "incidentalMusicFor"@en ;
    reg:status <http://metadataregistry.org/uri/RegStatus/1001> ;
    a rdf:Property ;
    rdfs:isDefinedBy <http://rdaregistry.info/Elements/u/> ;
    rdfs:label "is incidental music for"@en ;
    rdfs:subPropertyOf <http://rdaregistry.info/Elements/u/P60724> ;
    owl:inverseOf <http://rdaregistry.info/Elements/u/P60118> ;
    skos:definition "Relates a resource to a resource such as a play or other spoken resource for the stage that uses a musical resource as incidental music."@en .

<http://rdaregistry.info/Elements/u/P60203>
    reg:hasSubproperty <http://rdaregistry.info/Elements/e/P20104> ;
    reg:lexicalAlias <http://rdaregistry.info/Elements/u/abstractedAs.en> ;
    reg:name "abstractedAs"@en ;
    reg:status <http://metadataregistry.org/uri/RegStatus/1001> ;
    a rdf:Property ;
    rdfs:isDefinedBy <http://rdaregistry.info/Elements/u/> ;
    rdfs:label "is abstracted as"@en ;
    rdfs:subPropertyOf <http://rdaregistry.info/Elements/u/P60250> ;
    owl:inverseOf <http://rdaregistry.info/Elements/u/P60224> ;
    skos:definition "Relates a resource to a resource that abbreviates a source resource in a brief, objective manner."@en .

<http://rdaregistry.info/Elements/u/P60204>
    reg:hasSubproperty <http://rdaregistry.info/Elements/e/P20105>, <http://rdaregistry.info/Elements/u/P60113>, <http://rdaregistry.info/Elements/u/P60181>, <http://rdaregistry.info/Elements/u/P60182>, <http://rdaregistry.info/Elements/u/P60206>, <http://rdaregistry.info/Elements/u/P60208>, <http://rdaregistry.info/Elements/u/P60209>, <http://rdaregistry.info/Elements/u/P60221>, <http://rdaregistry.info/Elements/u/P60222>, <http://rdaregistry.info/Elements/u/P60262>, <http://rdaregistry.info/Elements/u/P60263>, <http://rdaregistry.info/Elements/u/P60281> ;
    reg:lexicalAlias <http://rdaregistry.info/Elements/u/augmentedBy.en> ;
    reg:name "augmentedBy"@en ;
    reg:status <http://metadataregistry.org/uri/RegStatus/1001> ;
    a rdf:Property ;
    rdfs:isDefinedBy <http://rdaregistry.info/Elements/u/> ;
    rdfs:label "is augmented by"@en ;
    rdfs:subPropertyOf <http://rdaregistry.info/Elements/u/P60709> ;
    owl:inverseOf <http://rdaregistry.info/Elements/u/P60307> ;
    skos:definition "Relates a resource to a resource that adds to the content of a predominant resource."@en .

<http://rdaregistry.info/Elements/u/P60205>
    reg:hasSubproperty <http://rdaregistry.info/Elements/e/P20106> ;
    reg:lexicalAlias <http://rdaregistry.info/Elements/u/summarizedAs.en> ;
    reg:name "summarizedAs"@en ;
    reg:status <http://metadataregistry.org/uri/RegStatus/1001> ;
    a rdf:Property ;
    rdfs:isDefinedBy <http://rdaregistry.info/Elements/u/> ;
    rdfs:label "is summarized as"@en ;
    rdfs:subPropertyOf <http://rdaregistry.info/Elements/u/P60250> ;
    owl:inverseOf <http://rdaregistry.info/Elements/u/P60289> ;
    skos:definition "Relates a resource to a resource that consists of a brief recapitulation of the content of a source resource."@en .

<http://rdaregistry.info/Elements/u/P60206>
    reg:hasSubproperty <http://rdaregistry.info/Elements/e/P20107> ;
    reg:lexicalAlias <http://rdaregistry.info/Elements/u/catalogue.en> ;
    reg:name "catalogue"@en ;
    reg:status <http://metadataregistry.org/uri/RegStatus/1001> ;
    a rdf:Property ;
    rdfs:isDefinedBy <http://rdaregistry.info/Elements/u/> ;
    rdfs:label "is catalogue"@en ;
    rdfs:subPropertyOf <http://rdaregistry.info/Elements/u/P60204> ;
    owl:inverseOf <http://rdaregistry.info/Elements/u/P60290> ;
    skos:definition "Relates a resource to a resource that consists of a complete enumeration of resources arranged systematically."@en .

<http://rdaregistry.info/Elements/u/P60207>
    reg:hasSubproperty <http://rdaregistry.info/Elements/m/P30030> ;
    reg:lexicalAlias <http://rdaregistry.info/Elements/u/specialIssue.en> ;
    reg:name "specialIssue"@en ;
    reg:status <http://metadataregistry.org/uri/RegStatus/1001> ;
    a rdf:Property ;
    rdfs:isDefinedBy <http://rdaregistry.info/Elements/u/> ;
    rdfs:label "is special issue"@en ;
    rdfs:subPropertyOf <http://rdaregistry.info/Elements/u/P60249> ;
    owl:inverseOf <http://rdaregistry.info/Elements/u/P60317> ;
    skos:definition "Relates a resource to a resource that consists of a single issue or a supplementary section of a periodical or newspaper devoted to a special subject, with or without serial numbering."@en .

<http://rdaregistry.info/Elements/u/P60208>
    reg:hasSubproperty <http://rdaregistry.info/Elements/e/P20108> ;
    reg:lexicalAlias <http://rdaregistry.info/Elements/u/concordance.en> ;
    reg:name "concordance"@en ;
    reg:status <http://metadataregistry.org/uri/RegStatus/1001> ;
    a rdf:Property ;
    rdfs:isDefinedBy <http://rdaregistry.info/Elements/u/> ;
    rdfs:label "is concordance"@en ;
    rdfs:subPropertyOf <http://rdaregistry.info/Elements/u/P60204> ;
    owl:inverseOf <http://rdaregistry.info/Elements/u/P60291> ;
    skos:definition "Relates a resource to a resource that consists of an index of all a words in a predominant resource."@en .

<http://rdaregistry.info/Elements/u/P60209>
    reg:hasSubproperty <http://rdaregistry.info/Elements/e/P20109> ;
    reg:lexicalAlias <http://rdaregistry.info/Elements/u/addenda.en> ;
    reg:name "addenda"@en ;
    reg:status <http://metadataregistry.org/uri/RegStatus/1001> ;
    a rdf:Property ;
    rdfs:isDefinedBy <http://rdaregistry.info/Elements/u/> ;
    rdfs:label "is addenda"@en ;
    rdfs:subPropertyOf <http://rdaregistry.info/Elements/u/P60204> ;
    owl:inverseOf <http://rdaregistry.info/Elements/u/P60286> ;
    skos:definition "Relates a resource to a resource consisting of brief content that is essential for the completeness of another resource."@en .

<http://rdaregistry.info/Elements/u/P60210>
    reg:hasSubproperty <http://rdaregistry.info/Elements/e/P20110> ;
    reg:lexicalAlias <http://rdaregistry.info/Elements/u/adaptedAsLibretto.en> ;
    reg:name "adaptedAsLibretto"@en ;
    reg:status <http://metadataregistry.org/uri/RegStatus/1001> ;
    a rdf:Property ;
    rdfs:isDefinedBy <http://rdaregistry.info/Elements/u/> ;
    rdfs:label "is adapted as libretto"@en ;
    rdfs:subPropertyOf <http://rdaregistry.info/Elements/u/P60250> ;
    owl:inverseOf <http://rdaregistry.info/Elements/u/P60304> ;
    skos:definition "Relates a resource to a resource consisting of a text of an opera or other resource for a musical stage, or an oratorio, based on a source resource."@en .

<http://rdaregistry.info/Elements/u/P60211>
    reg:hasSubproperty <http://rdaregistry.info/Elements/e/P20274>, <http://rdaregistry.info/Elements/i/P40067>, <http://rdaregistry.info/Elements/m/P30259> ;
    reg:lexicalAlias <http://rdaregistry.info/Elements/u/reviewedIn.en> ;
    reg:name "reviewedIn"@en ;
    reg:status <http://metadataregistry.org/uri/RegStatus/1001> ;
    a rdf:Property ;
    rdfs:isDefinedBy <http://rdaregistry.info/Elements/u/> ;
    rdfs:label "is reviewed in"@en ;
    rdfs:subPropertyOf <http://rdaregistry.info/Elements/u/P60215> ;
    owl:inverseOf <http://rdaregistry.info/Elements/u/P60288> ;
    skos:definition "Relates a resource to a resource that contains a brief evaluation of a described resource."@en .

<http://rdaregistry.info/Elements/u/P60212>
    reg:hasSubproperty <http://rdaregistry.info/Elements/e/P20272>, <http://rdaregistry.info/Elements/i/P40065>, <http://rdaregistry.info/Elements/m/P30257> ;
    reg:lexicalAlias <http://rdaregistry.info/Elements/u/critiquedIn.en> ;
    reg:name "critiquedIn"@en ;
    reg:status <http://metadataregistry.org/uri/RegStatus/1001> ;
    a rdf:Property ;
    rdfs:isDefinedBy <http://rdaregistry.info/Elements/u/> ;
    rdfs:label "is critiqued in"@en ;
    rdfs:subPropertyOf <http://rdaregistry.info/Elements/u/P60215> ;
    owl:inverseOf <http://rdaregistry.info/Elements/u/P60292> ;
    skos:definition "Relates a resource to a resource that contains a critical evaluation of a described resource."@en .

<http://rdaregistry.info/Elements/u/P60213>
    reg:hasSubproperty <http://rdaregistry.info/Elements/e/P20271>, <http://rdaregistry.info/Elements/i/P40064>, <http://rdaregistry.info/Elements/m/P30256> ;
    reg:lexicalAlias <http://rdaregistry.info/Elements/u/commentaryIn.en> ;
    reg:name "commentaryIn"@en ;
    reg:status <http://metadataregistry.org/uri/RegStatus/1001> ;
    a rdf:Property ;
    rdfs:isDefinedBy <http://rdaregistry.info/Elements/u/> ;
    rdfs:label "is commentary in"@en ;
    rdfs:subPropertyOf <http://rdaregistry.info/Elements/u/P60215> ;
    owl:inverseOf <http://rdaregistry.info/Elements/u/P60298> ;
    skos:definition "Relates a resource to a resource that contains a set of explanatory or critical notes on a described resource"@en .

<http://rdaregistry.info/Elements/u/P60214>
    reg:hasSubproperty <http://rdaregistry.info/Elements/e/P20114>, <http://rdaregistry.info/Elements/u/P60246> ;
    reg:lexicalAlias <http://rdaregistry.info/Elements/u/imitatedAs.en> ;
    reg:name "imitatedAs"@en ;
    reg:status <http://metadataregistry.org/uri/RegStatus/1001> ;
    a rdf:Property ;
    rdfs:isDefinedBy <http://rdaregistry.info/Elements/u/> ;
    rdfs:label "is imitated as"@en ;
    rdfs:subPropertyOf <http://rdaregistry.info/Elements/u/P60250> ;
    owl:inverseOf <http://rdaregistry.info/Elements/u/P60311> ;
    skos:definition "Relates a resource to a resource that copies the style or content of a source resource."@en .

<http://rdaregistry.info/Elements/u/P60215>
    reg:hasSubproperty <http://rdaregistry.info/Elements/a/P50368>, <http://rdaregistry.info/Elements/a/P50369>, <http://rdaregistry.info/Elements/a/P50370>, <http://rdaregistry.info/Elements/e/P20269>, <http://rdaregistry.info/Elements/i/P40062>, <http://rdaregistry.info/Elements/m/P30254>, <http://rdaregistry.info/Elements/u/P60211>, <http://rdaregistry.info/Elements/u/P60212>, <http://rdaregistry.info/Elements/u/P60213>, <http://rdaregistry.info/Elements/u/P60218>, <http://rdaregistry.info/Elements/u/P60219> ;
    reg:lexicalAlias <http://rdaregistry.info/Elements/u/describedIn.en> ;
    reg:name "describedIn"@en ;
    reg:status <http://metadataregistry.org/uri/RegStatus/1001> ;
    a rdf:Property ;
    rdfs:isDefinedBy <http://rdaregistry.info/Elements/u/> ;
    rdfs:label "is described in"@en ;
    rdfs:subPropertyOf <http://rdaregistry.info/Elements/u/P60806> ;
    owl:inverseOf <http://rdaregistry.info/Elements/u/P60190> ;
    skos:definition "Relates a resource to a resource that describes a described entity."@en .

<http://rdaregistry.info/Elements/u/P60216>
    reg:hasSubproperty <http://rdaregistry.info/Elements/e/P20115> ;
    reg:lexicalAlias <http://rdaregistry.info/Elements/u/expandedAs.en> ;
    reg:name "expandedAs"@en ;
    reg:status <http://metadataregistry.org/uri/RegStatus/1001> ;
    a rdf:Property ;
    rdfs:isDefinedBy <http://rdaregistry.info/Elements/u/> ;
    rdfs:label "is expanded as"@en ;
    rdfs:subPropertyOf <http://rdaregistry.info/Elements/u/P60250> ;
    owl:inverseOf <http://rdaregistry.info/Elements/u/P60294> ;
    skos:definition "Relates a resource to a resource that enlarges upon the content of a source resource."@en .

<http://rdaregistry.info/Elements/u/P60217>
    reg:hasSubproperty <http://rdaregistry.info/Elements/i/P40058>, <http://rdaregistry.info/Elements/m/P30031>, <http://rdaregistry.info/Elements/u/P60179> ;
    reg:lexicalAlias <http://rdaregistry.info/Elements/u/facsimile.en> ;
    reg:name "facsimile"@en ;
    reg:status <http://metadataregistry.org/uri/RegStatus/1001> ;
    a rdf:Property ;
    rdfs:isDefinedBy <http://rdaregistry.info/Elements/u/> ;
    rdfs:label "has facsimile"@en ;
    rdfs:subPropertyOf <http://rdaregistry.info/Elements/u/P60272> ;
    owl:inverseOf <http://rdaregistry.info/Elements/u/P60301> ;
    skos:definition "Relates a resource to a resource that exactly reproduces another resource embodying a resource."@en .

<http://rdaregistry.info/Elements/u/P60218>
    reg:hasSubproperty <http://rdaregistry.info/Elements/e/P20273>, <http://rdaregistry.info/Elements/i/P40066>, <http://rdaregistry.info/Elements/m/P30258> ;
    reg:lexicalAlias <http://rdaregistry.info/Elements/u/evaluatedIn.en> ;
    reg:name "evaluatedIn"@en ;
    reg:status <http://metadataregistry.org/uri/RegStatus/1001> ;
    a rdf:Property ;
    rdfs:isDefinedBy <http://rdaregistry.info/Elements/u/> ;
    rdfs:label "is evaluated in"@en ;
    rdfs:subPropertyOf <http://rdaregistry.info/Elements/u/P60215> ;
    owl:inverseOf <http://rdaregistry.info/Elements/u/P60255> ;
    skos:definition "Relates a resource to a resource that examines or judges a described resource."@en .

<http://rdaregistry.info/Elements/u/P60219>
    reg:hasSubproperty <http://rdaregistry.info/Elements/e/P20270>, <http://rdaregistry.info/Elements/i/P40063>, <http://rdaregistry.info/Elements/m/P30255> ;
    reg:lexicalAlias <http://rdaregistry.info/Elements/u/analysedIn.en> ;
    reg:name "analysedIn"@en ;
    reg:status <http://metadataregistry.org/uri/RegStatus/1001> ;
    a rdf:Property ;
    rdfs:isDefinedBy <http://rdaregistry.info/Elements/u/> ;
    rdfs:label "is analysed in"@en ;
    rdfs:subPropertyOf <http://rdaregistry.info/Elements/u/P60215> ;
    owl:inverseOf <http://rdaregistry.info/Elements/u/P60239> ;
    skos:definition "Relates a resource to a resource that examines a source resource to identify its components and their relations."@en .

<http://rdaregistry.info/Elements/u/P60220>
    reg:lexicalAlias <http://rdaregistry.info/Elements/u/prequel.en> ;
    reg:name "prequel"@en ;
    reg:status <http://metadataregistry.org/uri/RegStatus/1001> ;
    a rdf:Property ;
    rdfs:isDefinedBy <http://rdaregistry.info/Elements/u/> ;
    rdfs:label "is prequel"@en ;
    rdfs:subPropertyOf <http://rdaregistry.info/Elements/u/P60261> ;
    owl:inverseOf <http://rdaregistry.info/Elements/u/P60310> ;
    skos:definition "Relates a resource to a resource that extends the narrative of an earlier resource backwards in time."@en .

<http://rdaregistry.info/Elements/u/P60221>
    reg:hasSubproperty <http://rdaregistry.info/Elements/e/P20118> ;
    reg:lexicalAlias <http://rdaregistry.info/Elements/u/appendix.en> ;
    reg:name "appendix"@en ;
    reg:status <http://metadataregistry.org/uri/RegStatus/1001> ;
    a rdf:Property ;
    rdfs:isDefinedBy <http://rdaregistry.info/Elements/u/> ;
    rdfs:label "is appendix"@en ;
    rdfs:subPropertyOf <http://rdaregistry.info/Elements/u/P60204> ;
    owl:inverseOf <http://rdaregistry.info/Elements/u/P60253> ;
    skos:definition "Relates a resource to a resource whose content augments another resource."@en .

<http://rdaregistry.info/Elements/u/P60222>
    reg:hasSubproperty <http://rdaregistry.info/Elements/e/P20120> ;
    reg:lexicalAlias <http://rdaregistry.info/Elements/u/guide.en> ;
    reg:name "guide"@en ;
    reg:status <http://metadataregistry.org/uri/RegStatus/1001> ;
    a rdf:Property ;
    rdfs:isDefinedBy <http://rdaregistry.info/Elements/u/> ;
    rdfs:label "is guide"@en ;
    rdfs:subPropertyOf <http://rdaregistry.info/Elements/u/P60204> ;
    owl:inverseOf <http://rdaregistry.info/Elements/u/P60252> ;
    skos:definition "Relates a resource to a resource that guides a user through the use of a predominant resource, using notes, learning and study aids, exercises, problems, questions and answers, instructor or student materials, etc."@en .

<http://rdaregistry.info/Elements/u/P60223>
    reg:hasSubproperty <http://rdaregistry.info/Elements/e/P20121> ;
    reg:lexicalAlias <http://rdaregistry.info/Elements/u/abridgementOf.en> ;
    reg:name "abridgementOf"@en ;
    reg:status <http://metadataregistry.org/uri/RegStatus/1001> ;
    a rdf:Property ;
    rdfs:isDefinedBy <http://rdaregistry.info/Elements/u/> ;
    rdfs:label "is abridgement of"@en ;
    rdfs:subPropertyOf <http://rdaregistry.info/Elements/u/P60305> ;
    owl:inverseOf <http://rdaregistry.info/Elements/u/P60275> ;
    skos:definition "Relates a resource to a resource that has been abridged, i.e., shortened without changing a general meaning or manner of presentation of a source resource."@en .

<http://rdaregistry.info/Elements/u/P60224>
    reg:hasSubproperty <http://rdaregistry.info/Elements/e/P20122> ;
    reg:lexicalAlias <http://rdaregistry.info/Elements/u/abstractOf.en> ;
    reg:name "abstractOf"@en ;
    reg:status <http://metadataregistry.org/uri/RegStatus/1001> ;
    a rdf:Property ;
    rdfs:isDefinedBy <http://rdaregistry.info/Elements/u/> ;
    rdfs:label "is abstract of"@en ;
    rdfs:subPropertyOf <http://rdaregistry.info/Elements/u/P60305> ;
    owl:inverseOf <http://rdaregistry.info/Elements/u/P60203> ;
    skos:definition "Relates a resource to a resource that has been abstracted, i.e., abbreviated in a brief, objective manner."@en .

<http://rdaregistry.info/Elements/u/P60225>
    reg:hasSubproperty <http://rdaregistry.info/Elements/e/P20123> ;
    reg:lexicalAlias <http://rdaregistry.info/Elements/u/dramatizationOf.en> ;
    reg:name "dramatizationOf"@en ;
    reg:status <http://metadataregistry.org/uri/RegStatus/1001> ;
    a rdf:Property ;
    rdfs:isDefinedBy <http://rdaregistry.info/Elements/u/> ;
    rdfs:label "is dramatization of"@en ;
    rdfs:subPropertyOf <http://rdaregistry.info/Elements/u/P60241> ;
    owl:inverseOf <http://rdaregistry.info/Elements/u/P60088> ;
    skos:definition "Relates a resource to a resource that has been adapted as a drama."@en .

<http://rdaregistry.info/Elements/u/P60226>
    reg:hasSubproperty <http://rdaregistry.info/Elements/e/P20124> ;
    reg:lexicalAlias <http://rdaregistry.info/Elements/u/verseAdaptationOf.en> ;
    reg:name "verseAdaptationOf"@en ;
    reg:status <http://metadataregistry.org/uri/RegStatus/1001> ;
    a rdf:Property ;
    rdfs:isDefinedBy <http://rdaregistry.info/Elements/u/> ;
    rdfs:label "is verse adaptation of"@en ;
    rdfs:subPropertyOf <http://rdaregistry.info/Elements/u/P60241> ;
    owl:inverseOf <http://rdaregistry.info/Elements/u/P60106> ;
    skos:definition "Relates a resource to a resource that has been adapted as a literary composition in verse form."@en .

<http://rdaregistry.info/Elements/u/P60227>
    reg:hasSubproperty <http://rdaregistry.info/Elements/e/P20125> ;
    reg:lexicalAlias <http://rdaregistry.info/Elements/u/motionPictureAdaptationOf.en> ;
    reg:name "motionPictureAdaptationOf"@en ;
    reg:status <http://metadataregistry.org/uri/RegStatus/1001> ;
    a rdf:Property ;
    rdfs:isDefinedBy <http://rdaregistry.info/Elements/u/> ;
    rdfs:label "is motion picture adaptation of"@en ;
    rdfs:subPropertyOf <http://rdaregistry.info/Elements/u/P60241> ;
    owl:inverseOf <http://rdaregistry.info/Elements/u/P60110> ;
    skos:definition "Relates a resource to a resource that has been adapted as a motion picture."@en .

<http://rdaregistry.info/Elements/u/P60228>
    reg:hasSubproperty <http://rdaregistry.info/Elements/e/P20126> ;
    reg:lexicalAlias <http://rdaregistry.info/Elements/u/novelizationOf.en> ;
    reg:name "novelizationOf"@en ;
    reg:status <http://metadataregistry.org/uri/RegStatus/1001> ;
    a rdf:Property ;
    rdfs:isDefinedBy <http://rdaregistry.info/Elements/u/> ;
    rdfs:label "is novelization of"@en ;
    rdfs:subPropertyOf <http://rdaregistry.info/Elements/u/P60241> ;
    owl:inverseOf <http://rdaregistry.info/Elements/u/P60138> ;
    skos:definition "Relates a resource to a resource that has been adapted as a novel."@en .

<http://rdaregistry.info/Elements/u/P60229>
    reg:hasSubproperty <http://rdaregistry.info/Elements/e/P20127> ;
    reg:lexicalAlias <http://rdaregistry.info/Elements/u/radioAdaptationOf.en> ;
    reg:name "radioAdaptationOf"@en ;
    reg:status <http://metadataregistry.org/uri/RegStatus/1001> ;
    a rdf:Property ;
    rdfs:isDefinedBy <http://rdaregistry.info/Elements/u/> ;
    rdfs:label "is radio adaptation of"@en ;
    rdfs:subPropertyOf <http://rdaregistry.info/Elements/u/P60241> ;
    owl:inverseOf <http://rdaregistry.info/Elements/u/P60174> ;
    skos:definition "Relates a resource to a resource that has been adapted as a radio program."@en .

<http://rdaregistry.info/Elements/u/P60230>
    reg:hasSubproperty <http://rdaregistry.info/Elements/e/P20128> ;
    reg:lexicalAlias <http://rdaregistry.info/Elements/u/televisionAdaptationOf.en> ;
    reg:name "televisionAdaptationOf"@en ;
    reg:status <http://metadataregistry.org/uri/RegStatus/1001> ;
    a rdf:Property ;
    rdfs:isDefinedBy <http://rdaregistry.info/Elements/u/> ;
    rdfs:label "is television adaptation of"@en ;
    rdfs:subPropertyOf <http://rdaregistry.info/Elements/u/P60241> ;
    owl:inverseOf <http://rdaregistry.info/Elements/u/P60354> ;
    skos:definition "Relates a resource to a resource that has been adapted as a television program."@en .

<http://rdaregistry.info/Elements/u/P60231>
    reg:hasSubproperty <http://rdaregistry.info/Elements/e/P20129>, <http://rdaregistry.info/Elements/u/P60232>, <http://rdaregistry.info/Elements/u/P60233>, <http://rdaregistry.info/Elements/u/P60234> ;
    reg:lexicalAlias <http://rdaregistry.info/Elements/u/screenplayBasedOn.en> ;
    reg:name "screenplayBasedOn"@en ;
    reg:status <http://metadataregistry.org/uri/RegStatus/1001> ;
    a rdf:Property ;
    rdfs:isDefinedBy <http://rdaregistry.info/Elements/u/> ;
    rdfs:label "is screenplay based on"@en ;
    rdfs:subPropertyOf <http://rdaregistry.info/Elements/u/P60241> ;
    owl:inverseOf <http://rdaregistry.info/Elements/u/P60185> ;
    skos:definition "Relates a resource to a resource that has been adapted as a screenplay for a motion picture, television program, or video."@en .

<http://rdaregistry.info/Elements/u/P60232>
    reg:hasSubproperty <http://rdaregistry.info/Elements/e/P20130> ;
    reg:lexicalAlias <http://rdaregistry.info/Elements/u/motionPictureScreenplayBasedOn.en> ;
    reg:name "motionPictureScreenplayBasedOn"@en ;
    reg:status <http://metadataregistry.org/uri/RegStatus/1001> ;
    a rdf:Property ;
    rdfs:isDefinedBy <http://rdaregistry.info/Elements/u/> ;
    rdfs:label "is motion picture screenplay based on"@en ;
    rdfs:subPropertyOf <http://rdaregistry.info/Elements/u/P60231> ;
    owl:inverseOf <http://rdaregistry.info/Elements/u/P60184> ;
    skos:definition "Relates a resource to a resource that has been adapted as a screenplay for a motion picture."@en .

<http://rdaregistry.info/Elements/u/P60233>
    reg:hasSubproperty <http://rdaregistry.info/Elements/e/P20131> ;
    reg:lexicalAlias <http://rdaregistry.info/Elements/u/televisionScreenplayBasedOn.en> ;
    reg:name "televisionScreenplayBasedOn"@en ;
    reg:status <http://metadataregistry.org/uri/RegStatus/1001> ;
    a rdf:Property ;
    rdfs:isDefinedBy <http://rdaregistry.info/Elements/u/> ;
    rdfs:label "is television screenplay based on"@en ;
    rdfs:subPropertyOf <http://rdaregistry.info/Elements/u/P60231> ;
    owl:inverseOf <http://rdaregistry.info/Elements/u/P60186> ;
    skos:definition "Relates a resource to a resource that has been adapted as a screenplay for a television program."@en .

<http://rdaregistry.info/Elements/u/P60234>
    reg:hasSubproperty <http://rdaregistry.info/Elements/e/P20132> ;
    reg:lexicalAlias <http://rdaregistry.info/Elements/u/videoScreenplayBasedOn.en> ;
    reg:name "videoScreenplayBasedOn"@en ;
    reg:status <http://metadataregistry.org/uri/RegStatus/1001> ;
    a rdf:Property ;
    rdfs:isDefinedBy <http://rdaregistry.info/Elements/u/> ;
    rdfs:label "is video screenplay based on"@en ;
    rdfs:subPropertyOf <http://rdaregistry.info/Elements/u/P60231> ;
    owl:inverseOf <http://rdaregistry.info/Elements/u/P60187> ;
    skos:definition "Relates a resource to a resource that has been adapted as a screenplay for a video."@en .

<http://rdaregistry.info/Elements/u/P60235>
    reg:hasSubproperty <http://rdaregistry.info/Elements/e/P20133> ;
    reg:lexicalAlias <http://rdaregistry.info/Elements/u/radioScriptBasedOn.en> ;
    reg:name "radioScriptBasedOn"@en ;
    reg:status <http://metadataregistry.org/uri/RegStatus/1001> ;
    a rdf:Property ;
    rdfs:isDefinedBy <http://rdaregistry.info/Elements/u/> ;
    rdfs:label "is radio script based on"@en ;
    rdfs:subPropertyOf <http://rdaregistry.info/Elements/u/P60241> ;
    owl:inverseOf <http://rdaregistry.info/Elements/u/P60188> ;
    skos:definition "Relates a resource to a resource that has been adapted as a script for a radio program."@en .

<http://rdaregistry.info/Elements/u/P60236>
    reg:hasSubproperty <http://rdaregistry.info/Elements/e/P20134> ;
    reg:lexicalAlias <http://rdaregistry.info/Elements/u/videoAdaptationOf.en> ;
    reg:name "videoAdaptationOf"@en ;
    reg:status <http://metadataregistry.org/uri/RegStatus/1001> ;
    a rdf:Property ;
    rdfs:isDefinedBy <http://rdaregistry.info/Elements/u/> ;
    rdfs:label "is video adaptation of"@en ;
    rdfs:subPropertyOf <http://rdaregistry.info/Elements/u/P60241> ;
    owl:inverseOf <http://rdaregistry.info/Elements/u/P60361> ;
    skos:definition "Relates a resource to a resource that has been adapted for video."@en .

<http://rdaregistry.info/Elements/u/P60237>
    reg:hasSubproperty <http://rdaregistry.info/Elements/i/P40032> ;
    reg:lexicalAlias <http://rdaregistry.info/Elements/u/boundWith.en> ;
    reg:name "boundWith"@en ;
    reg:status <http://metadataregistry.org/uri/RegStatus/1001> ;
    a rdf:Property ;
    rdfs:isDefinedBy <http://rdaregistry.info/Elements/u/> ;
    rdfs:label "is bound with"@en ;
    rdfs:subPropertyOf <http://rdaregistry.info/Elements/u/P60196> ;
    owl:inverseOf <http://rdaregistry.info/Elements/u/P60237> ;
    skos:definition "Relates a resource to a resource that has been bound within the same binding as a resource being described."@en .

<http://rdaregistry.info/Elements/u/P60238>
    reg:hasSubproperty <http://rdaregistry.info/Elements/e/P20135> ;
    reg:lexicalAlias <http://rdaregistry.info/Elements/u/digestOf.en> ;
    reg:name "digestOf"@en ;
    reg:status <http://metadataregistry.org/uri/RegStatus/1001> ;
    a rdf:Property ;
    rdfs:isDefinedBy <http://rdaregistry.info/Elements/u/> ;
    rdfs:label "is digest of"@en ;
    rdfs:subPropertyOf <http://rdaregistry.info/Elements/u/P60305> ;
    owl:inverseOf <http://rdaregistry.info/Elements/u/P60279> ;
    skos:definition "Relates a resource to a resource that has been digested, i.e., systematically and comprehensively condensed."@en .

<http://rdaregistry.info/Elements/u/P60239>
    reg:hasSubproperty <http://rdaregistry.info/Elements/w/P10266>, <http://rdaregistry.info/Elements/w/P10272>, <http://rdaregistry.info/Elements/w/P10278> ;
    reg:lexicalAlias <http://rdaregistry.info/Elements/u/analysisOf.en> ;
    reg:name "analysisOf"@en ;
    reg:status <http://metadataregistry.org/uri/RegStatus/1001> ;
    a rdf:Property ;
    rdfs:isDefinedBy <http://rdaregistry.info/Elements/u/> ;
    rdfs:label "is analysis of"@en ;
    rdfs:subPropertyOf <http://rdaregistry.info/Elements/u/P60190> ;
    owl:inverseOf <http://rdaregistry.info/Elements/u/P60219> ;
    skos:definition "Relates a resource to a resource that has been examined to identify its components and their relations."@en .

<http://rdaregistry.info/Elements/u/P60240>
    reg:lexicalAlias <http://rdaregistry.info/Elements/u/seriesContainerOf.en> ;
    reg:name "seriesContainerOf"@en ;
    reg:status <http://metadataregistry.org/uri/RegStatus/1001> ;
    a rdf:Property ;
    rdfs:isDefinedBy <http://rdaregistry.info/Elements/u/> ;
    rdfs:label "is series container of"@en ;
    rdfs:subPropertyOf <http://rdaregistry.info/Elements/u/P60249> ;
    owl:inverseOf <http://rdaregistry.info/Elements/u/P60193> ;
    skos:definition "Relates a resource to a resource that has been issued as part of a series."@en .

<http://rdaregistry.info/Elements/u/P60241>
    reg:hasSubproperty <http://rdaregistry.info/Elements/e/P20152>, <http://rdaregistry.info/Elements/u/P60225>, <http://rdaregistry.info/Elements/u/P60226>, <http://rdaregistry.info/Elements/u/P60227>, <http://rdaregistry.info/Elements/u/P60228>, <http://rdaregistry.info/Elements/u/P60229>, <http://rdaregistry.info/Elements/u/P60230>, <http://rdaregistry.info/Elements/u/P60231>, <http://rdaregistry.info/Elements/u/P60235>, <http://rdaregistry.info/Elements/u/P60236>, <http://rdaregistry.info/Elements/u/P60743>, <http://rdaregistry.info/Elements/u/P60745> ;
    reg:lexicalAlias <http://rdaregistry.info/Elements/u/adaptationOf.en> ;
    reg:name "adaptationOf"@en ;
    reg:status <http://metadataregistry.org/uri/RegStatus/1001> ;
    a rdf:Property ;
    rdfs:isDefinedBy <http://rdaregistry.info/Elements/u/> ;
    rdfs:label "is adaptation of"@en ;
    rdfs:subPropertyOf <http://rdaregistry.info/Elements/u/P60305> ;
    owl:inverseOf <http://rdaregistry.info/Elements/u/P60260> ;
    skos:definition "Relates a resource to a resource that has been modified for a purpose, use, or medium other than that for which it was originally intended."@en ;
    skos:scopeNote "This relationship applies to changes in form or to resources completely rewritten in the same form."@en .

<http://rdaregistry.info/Elements/u/P60242>
    reg:hasSubproperty <http://rdaregistry.info/Elements/e/P20139> ;
    reg:lexicalAlias <http://rdaregistry.info/Elements/u/arrangementOf.en> ;
    reg:name "arrangementOf"@en ;
    reg:status <http://metadataregistry.org/uri/RegStatus/1001> ;
    a rdf:Property ;
    rdfs:isDefinedBy <http://rdaregistry.info/Elements/u/> ;
    rdfs:label "is arrangement of"@en ;
    rdfs:subPropertyOf <http://rdaregistry.info/Elements/u/P60305> ;
    owl:inverseOf <http://rdaregistry.info/Elements/u/P60274> ;
    skos:definition "Relates a resource to a musical resource that has been rewritten for a medium of performance different from that for which a resource was originally intended."@en .

<http://rdaregistry.info/Elements/u/P60243>
    reg:hasSubproperty <http://rdaregistry.info/Elements/e/P20140> ;
    reg:lexicalAlias <http://rdaregistry.info/Elements/u/freeTranslationOf.en> ;
    reg:name "freeTranslationOf"@en ;
    reg:status <http://metadataregistry.org/uri/RegStatus/1001> ;
    a rdf:Property ;
    rdfs:isDefinedBy <http://rdaregistry.info/Elements/u/> ;
    rdfs:label "is free translation of"@en ;
    rdfs:subPropertyOf <http://rdaregistry.info/Elements/u/P60305> ;
    owl:inverseOf <http://rdaregistry.info/Elements/u/P60189> ;
    skos:definition "Relates a resource to a resource that has been adapted and translated into another language."@en .

<http://rdaregistry.info/Elements/u/P60244>
    reg:hasSubproperty <http://rdaregistry.info/Elements/e/P20141>, <http://rdaregistry.info/Elements/u/P60111> ;
    reg:lexicalAlias <http://rdaregistry.info/Elements/u/translationOf.en> ;
    reg:name "translationOf"@en ;
    reg:status <http://metadataregistry.org/uri/RegStatus/1001> ;
    a rdf:Property ;
    rdfs:isDefinedBy <http://rdaregistry.info/Elements/u/> ;
    rdfs:label "is translation of"@en ;
    rdfs:subPropertyOf <http://rdaregistry.info/Elements/u/P60305> ;
    owl:inverseOf <http://rdaregistry.info/Elements/u/P60280> ;
    skos:definition "Relates a resource to a resource that has been translated, i.e., the text expressed in a language different from that of an original resource."@en .

<http://rdaregistry.info/Elements/u/P60245>
    reg:hasSubproperty <http://rdaregistry.info/Elements/e/P20211> ;
    reg:lexicalAlias <http://rdaregistry.info/Elements/u/revisedAs.en> ;
    reg:name "revisedAs"@en ;
    reg:status <http://metadataregistry.org/uri/RegStatus/1001> ;
    a rdf:Property ;
    rdfs:isDefinedBy <http://rdaregistry.info/Elements/u/> ;
    rdfs:label "is revised as"@en ;
    rdfs:subPropertyOf <http://rdaregistry.info/Elements/u/P60250> ;
    owl:inverseOf <http://rdaregistry.info/Elements/u/P60303> ;
    skos:definition "Relates a resource to a resource that has been updated, corrected, or expanded."@en .

<http://rdaregistry.info/Elements/u/P60246>
    reg:hasSubproperty <http://rdaregistry.info/Elements/e/P20142> ;
    reg:lexicalAlias <http://rdaregistry.info/Elements/u/parodiedAs.en> ;
    reg:name "parodiedAs"@en ;
    reg:status <http://metadataregistry.org/uri/RegStatus/1001> ;
    a rdf:Property ;
    rdfs:isDefinedBy <http://rdaregistry.info/Elements/u/> ;
    rdfs:label "is parodied as"@en ;
    rdfs:subPropertyOf <http://rdaregistry.info/Elements/u/P60214> ;
    owl:inverseOf <http://rdaregistry.info/Elements/u/P60312> ;
    skos:definition "Relates a resource to a resource that imitates the style or content of the source resource for comic effect."@en .

<http://rdaregistry.info/Elements/u/P60247>
    reg:hasSubproperty <http://rdaregistry.info/Elements/e/P20143> ;
    reg:lexicalAlias <http://rdaregistry.info/Elements/u/absorbedBy.en> ;
    reg:name "absorbedBy"@en ;
    reg:status <http://metadataregistry.org/uri/RegStatus/1001> ;
    a rdf:Property ;
    rdfs:isDefinedBy <http://rdaregistry.info/Elements/u/> ;
    rdfs:label "is absorbed by"@en ;
    rdfs:subPropertyOf <http://rdaregistry.info/Elements/u/P60278> ;
    owl:inverseOf <http://rdaregistry.info/Elements/u/P60574> ;
    skos:definition "Relates a resource to a resource that incorporates another resource."@en .

<http://rdaregistry.info/Elements/u/P60248>
    reg:hasSubproperty <http://rdaregistry.info/Elements/e/P20144> ;
    reg:lexicalAlias <http://rdaregistry.info/Elements/u/absorbedInPartBy.en> ;
    reg:name "absorbedInPartBy"@en ;
    reg:status <http://metadataregistry.org/uri/RegStatus/1001> ;
    a rdf:Property ;
    rdfs:isDefinedBy <http://rdaregistry.info/Elements/u/> ;
    rdfs:label "is absorbed in part by"@en ;
    rdfs:subPropertyOf <http://rdaregistry.info/Elements/u/P60278> ;
    owl:inverseOf <http://rdaregistry.info/Elements/u/P60575> ;
    skos:definition "Relates a resource to a resource that incorporates part of the content of another resource."@en .

<http://rdaregistry.info/Elements/u/P60249>
    reg:hasSubproperty <http://rdaregistry.info/Elements/e/P20145>, <http://rdaregistry.info/Elements/i/P40034>, <http://rdaregistry.info/Elements/m/P30033>, <http://rdaregistry.info/Elements/u/P60183>, <http://rdaregistry.info/Elements/u/P60207>, <http://rdaregistry.info/Elements/u/P60240>, <http://rdaregistry.info/Elements/u/P60300>, <http://rdaregistry.info/Elements/u/P60316> ;
    reg:lexicalAlias <http://rdaregistry.info/Elements/u/containerOf.en> ;
    reg:name "containerOf"@en ;
    reg:status <http://metadataregistry.org/uri/RegStatus/1001> ;
    a rdf:Property ;
    rdfs:isDefinedBy <http://rdaregistry.info/Elements/u/> ;
    rdfs:label "is container of"@en ;
    rdfs:subPropertyOf <http://rdaregistry.info/Elements/u/P60714> ;
    owl:inverseOf <http://rdaregistry.info/Elements/u/P60101> ;
    skos:definition "Relates a resource to a resource that is a discrete component of a larger resource."@en .

<http://rdaregistry.info/Elements/u/P60250>
    reg:hasSubproperty <http://rdaregistry.info/Elements/e/P20203>, <http://rdaregistry.info/Elements/u/P60115>, <http://rdaregistry.info/Elements/u/P60120>, <http://rdaregistry.info/Elements/u/P60121>, <http://rdaregistry.info/Elements/u/P60177>, <http://rdaregistry.info/Elements/u/P60178>, <http://rdaregistry.info/Elements/u/P60180>, <http://rdaregistry.info/Elements/u/P60189>, <http://rdaregistry.info/Elements/u/P60203>, <http://rdaregistry.info/Elements/u/P60205>, <http://rdaregistry.info/Elements/u/P60210>, <http://rdaregistry.info/Elements/u/P60214>, <http://rdaregistry.info/Elements/u/P60216>, <http://rdaregistry.info/Elements/u/P60245>, <http://rdaregistry.info/Elements/u/P60260>, <http://rdaregistry.info/Elements/u/P60273>, <http://rdaregistry.info/Elements/u/P60274>, <http://rdaregistry.info/Elements/u/P60275>, <http://rdaregistry.info/Elements/u/P60279>, <http://rdaregistry.info/Elements/u/P60280>, <http://rdaregistry.info/Elements/u/P60831>, <http://rdaregistry.info/Elements/u/P60833> ;
    reg:lexicalAlias <http://rdaregistry.info/Elements/u/derivative.en> ;
    reg:name "derivative"@en ;
    reg:status <http://metadataregistry.org/uri/RegStatus/1001> ;
    a rdf:Property ;
    rdfs:isDefinedBy <http://rdaregistry.info/Elements/u/> ;
    rdfs:label "is derivative"@en ;
    rdfs:subPropertyOf <http://rdaregistry.info/Elements/u/P60710> ;
    owl:inverseOf <http://rdaregistry.info/Elements/u/P60305> ;
    skos:definition "Relates a resource to a resource that is a modification of a source resource."@en .

<http://rdaregistry.info/Elements/u/P60251>
    reg:hasSubproperty <http://rdaregistry.info/Elements/e/P20146> ;
    reg:lexicalAlias <http://rdaregistry.info/Elements/u/errataTo.en> ;
    reg:name "errataTo"@en ;
    reg:status <http://metadataregistry.org/uri/RegStatus/1001> ;
    a rdf:Property ;
    rdfs:isDefinedBy <http://rdaregistry.info/Elements/u/> ;
    rdfs:label "is errata to"@en ;
    rdfs:subPropertyOf <http://rdaregistry.info/Elements/u/P60307> ;
    owl:inverseOf <http://rdaregistry.info/Elements/u/P60181> ;
    skos:definition "Relates a resource to a resource that is augmented by a list of errors in a predominant resource, discovered after publication, with their corrections."@en .

<http://rdaregistry.info/Elements/u/P60252>
    reg:hasSubproperty <http://rdaregistry.info/Elements/e/P20147> ;
    reg:lexicalAlias <http://rdaregistry.info/Elements/u/guideTo.en> ;
    reg:name "guideTo"@en ;
    reg:status <http://metadataregistry.org/uri/RegStatus/1001> ;
    a rdf:Property ;
    rdfs:isDefinedBy <http://rdaregistry.info/Elements/u/> ;
    rdfs:label "is guide to"@en ;
    rdfs:subPropertyOf <http://rdaregistry.info/Elements/u/P60307> ;
    owl:inverseOf <http://rdaregistry.info/Elements/u/P60222> ;
    skos:definition "Relates a resource to a resource that is augmented by another resource consisting of material, such as notes, learning and study aids, exercises, problems, questions and answers, instructor or student materials, etc., to help a user of a predominant resource."@en .

<http://rdaregistry.info/Elements/u/P60253>
    reg:hasSubproperty <http://rdaregistry.info/Elements/e/P20089> ;
    reg:lexicalAlias <http://rdaregistry.info/Elements/u/appendixTo.en> ;
    reg:name "appendixTo"@en ;
    reg:status <http://metadataregistry.org/uri/RegStatus/1001> ;
    a rdf:Property ;
    rdfs:isDefinedBy <http://rdaregistry.info/Elements/u/> ;
    rdfs:label "is appendix to"@en ;
    rdfs:subPropertyOf <http://rdaregistry.info/Elements/u/P60307> ;
    owl:inverseOf <http://rdaregistry.info/Elements/u/P60221> ;
    skos:definition "Relates a resource to a resource whose content is augmented with content from another resource."@en .

<http://rdaregistry.info/Elements/u/P60254>
    reg:hasSubproperty <http://rdaregistry.info/Elements/e/P20148> ;
    reg:lexicalAlias <http://rdaregistry.info/Elements/u/illustrationsFor.en> ;
    reg:name "illustrationsFor"@en ;
    reg:status <http://metadataregistry.org/uri/RegStatus/1001> ;
    a rdf:Property ;
    rdfs:isDefinedBy <http://rdaregistry.info/Elements/u/> ;
    rdfs:label "is illustrations for"@en ;
    rdfs:subPropertyOf <http://rdaregistry.info/Elements/u/P60307> ;
    owl:inverseOf <http://rdaregistry.info/Elements/u/P60182> ;
    skos:definition "Relates a resource to a resource that is augmented by pictorial content designed to explain or decorate it."@en .

<http://rdaregistry.info/Elements/u/P60255>
    reg:hasSubproperty <http://rdaregistry.info/Elements/w/P10267>, <http://rdaregistry.info/Elements/w/P10273>, <http://rdaregistry.info/Elements/w/P10279> ;
    reg:lexicalAlias <http://rdaregistry.info/Elements/u/evaluationOf.en> ;
    reg:name "evaluationOf"@en ;
    reg:status <http://metadataregistry.org/uri/RegStatus/1001> ;
    a rdf:Property ;
    rdfs:isDefinedBy <http://rdaregistry.info/Elements/u/> ;
    rdfs:label "is evaluation of"@en ;
    rdfs:subPropertyOf <http://rdaregistry.info/Elements/u/P60190> ;
    owl:inverseOf <http://rdaregistry.info/Elements/u/P60218> ;
    skos:definition "Relates a resource to a resource that is examined or judged."@en .

<http://rdaregistry.info/Elements/u/P60256>
    reg:hasSubproperty <http://rdaregistry.info/Elements/m/P30035>, <http://rdaregistry.info/Elements/u/P60257>, <http://rdaregistry.info/Elements/u/P60258> ;
    reg:lexicalAlias <http://rdaregistry.info/Elements/u/issuedWith.en> ;
    reg:name "issuedWith"@en ;
    reg:status <http://metadataregistry.org/uri/RegStatus/1001> ;
    a rdf:Property ;
    rdfs:isDefinedBy <http://rdaregistry.info/Elements/u/> ;
    rdfs:label "is issued with"@en ;
    rdfs:subPropertyOf <http://rdaregistry.info/Elements/u/P60196> ;
    owl:inverseOf <http://rdaregistry.info/Elements/u/P60256> ;
    skos:definition "Relates a resource to a resource that is issued on the same carrier as a resource being described."@en .

<http://rdaregistry.info/Elements/u/P60257>
    reg:hasSubproperty <http://rdaregistry.info/Elements/i/P40035>, <http://rdaregistry.info/Elements/m/P30036> ;
    reg:lexicalAlias <http://rdaregistry.info/Elements/u/onDiscWith.en> ;
    reg:name "onDiscWith"@en ;
    reg:status <http://metadataregistry.org/uri/RegStatus/1001> ;
    a rdf:Property ;
    rdfs:isDefinedBy <http://rdaregistry.info/Elements/u/> ;
    rdfs:label "is on disc with"@en ;
    rdfs:subPropertyOf <http://rdaregistry.info/Elements/u/P60256> ;
    owl:inverseOf <http://rdaregistry.info/Elements/u/P60257> ;
    skos:definition "Relates a resource to a resource that is issued on the same disc with a resource being described."@en .

<http://rdaregistry.info/Elements/u/P60258>
    reg:hasSubproperty <http://rdaregistry.info/Elements/i/P40036>, <http://rdaregistry.info/Elements/m/P30037> ;
    reg:lexicalAlias <http://rdaregistry.info/Elements/u/filmedWith.en> ;
    reg:name "filmedWith"@en ;
    reg:status <http://metadataregistry.org/uri/RegStatus/1001> ;
    a rdf:Property ;
    rdfs:isDefinedBy <http://rdaregistry.info/Elements/u/> ;
    rdfs:label "is filmed with"@en ;
    rdfs:subPropertyOf <http://rdaregistry.info/Elements/u/P60256> ;
    owl:inverseOf <http://rdaregistry.info/Elements/u/P60258> ;
    skos:definition "Relates a resource to a resource that is issued on the same microform with a resource being described."@en .

<http://rdaregistry.info/Elements/u/P60259>
    reg:hasSubproperty <http://rdaregistry.info/Elements/e/P20151> ;
    reg:lexicalAlias <http://rdaregistry.info/Elements/u/supplementTo.en> ;
    reg:name "supplementTo"@en ;
    reg:status <http://metadataregistry.org/uri/RegStatus/1001> ;
    a rdf:Property ;
    rdfs:isDefinedBy <http://rdaregistry.info/Elements/u/> ;
    rdfs:label "is supplement to"@en ;
    rdfs:subPropertyOf <http://rdaregistry.info/Elements/u/P60307> ;
    owl:inverseOf <http://rdaregistry.info/Elements/u/P60281> ;
    skos:definition "Relates a resource to a resource that is updated or otherwise complemented by an augmenting resource."@en .

<http://rdaregistry.info/Elements/u/P60260>
    reg:hasSubproperty <http://rdaregistry.info/Elements/e/P20153>, <http://rdaregistry.info/Elements/u/P60088>, <http://rdaregistry.info/Elements/u/P60106>, <http://rdaregistry.info/Elements/u/P60110>, <http://rdaregistry.info/Elements/u/P60138>, <http://rdaregistry.info/Elements/u/P60174>, <http://rdaregistry.info/Elements/u/P60185>, <http://rdaregistry.info/Elements/u/P60188>, <http://rdaregistry.info/Elements/u/P60354>, <http://rdaregistry.info/Elements/u/P60361>, <http://rdaregistry.info/Elements/u/P60742>, <http://rdaregistry.info/Elements/u/P60744> ;
    reg:lexicalAlias <http://rdaregistry.info/Elements/u/adaptedAs.en> ;
    reg:name "adaptedAs"@en ;
    reg:status <http://metadataregistry.org/uri/RegStatus/1001> ;
    a rdf:Property ;
    rdfs:isDefinedBy <http://rdaregistry.info/Elements/u/> ;
    rdfs:label "is adapted as"@en ;
    rdfs:subPropertyOf <http://rdaregistry.info/Elements/u/P60250> ;
    owl:inverseOf <http://rdaregistry.info/Elements/u/P60241> ;
    skos:definition "Relates a resource to a resource that modifies a source resource for a purpose, use, or medium other than that for which it was originally intended."@en ;
    skos:scopeNote "This relationship applies to changes in form or to resources completely rewritten in the same form."@en .

<http://rdaregistry.info/Elements/u/P60261>
    reg:hasSubproperty <http://rdaregistry.info/Elements/e/P20154>, <http://rdaregistry.info/Elements/u/P60220>, <http://rdaregistry.info/Elements/u/P60276>, <http://rdaregistry.info/Elements/u/P60277>, <http://rdaregistry.info/Elements/u/P60479>, <http://rdaregistry.info/Elements/u/P60480>, <http://rdaregistry.info/Elements/u/P60505>, <http://rdaregistry.info/Elements/u/P60574>, <http://rdaregistry.info/Elements/u/P60575>, <http://rdaregistry.info/Elements/u/P60576>, <http://rdaregistry.info/Elements/u/P60577> ;
    reg:lexicalAlias <http://rdaregistry.info/Elements/u/precededBy.en> ;
    reg:name "precededBy"@en ;
    reg:status <http://metadataregistry.org/uri/RegStatus/1001> ;
    a rdf:Property ;
    rdfs:isDefinedBy <http://rdaregistry.info/Elements/u/> ;
    rdfs:label "is preceded by"@en ;
    rdfs:subPropertyOf <http://rdaregistry.info/Elements/u/P60713> ;
    owl:inverseOf <http://rdaregistry.info/Elements/u/P60278> ;
    skos:definition "Relates a resource to a resource that precedes, that is, is earlier in time or before in a narrative, etc., a succeeding resource."@en .

<http://rdaregistry.info/Elements/u/P60262>
    reg:hasSubproperty <http://rdaregistry.info/Elements/e/P20155> ;
    reg:lexicalAlias <http://rdaregistry.info/Elements/u/findingAid.en> ;
    reg:name "findingAid"@en ;
    reg:status <http://metadataregistry.org/uri/RegStatus/1001> ;
    a rdf:Property ;
    rdfs:isDefinedBy <http://rdaregistry.info/Elements/u/> ;
    rdfs:label "is finding aid"@en ;
    rdfs:subPropertyOf <http://rdaregistry.info/Elements/u/P60204> ;
    owl:inverseOf <http://rdaregistry.info/Elements/u/P60474> ;
    skos:definition "Relates a resource to a resource that provides a guide to an organization, arrangement, and contents of an archival collection."@en .

<http://rdaregistry.info/Elements/u/P60263>
    reg:hasSubproperty <http://rdaregistry.info/Elements/e/P20156> ;
    reg:lexicalAlias <http://rdaregistry.info/Elements/u/index.en> ;
    reg:name "index"@en ;
    reg:status <http://metadataregistry.org/uri/RegStatus/1001> ;
    a rdf:Property ;
    rdfs:isDefinedBy <http://rdaregistry.info/Elements/u/> ;
    rdfs:label "is index"@en ;
    rdfs:subPropertyOf <http://rdaregistry.info/Elements/u/P60204> ;
    owl:inverseOf <http://rdaregistry.info/Elements/u/P60302> ;
    skos:definition "Relates a resource to a resource that provides a systematic, alphabetical guide to the contents of a predominant resource, usually keyed to page numbers or other reference codes."@en .

<http://rdaregistry.info/Elements/u/P60264>
    reg:hasSubproperty <http://rdaregistry.info/Elements/e/P20157>, <http://rdaregistry.info/Elements/u/P60265>, <http://rdaregistry.info/Elements/u/P60268>, <http://rdaregistry.info/Elements/u/P60269> ;
    reg:lexicalAlias <http://rdaregistry.info/Elements/u/screenplay.en> ;
    reg:name "screenplay"@en ;
    reg:status <http://metadataregistry.org/uri/RegStatus/1001> ;
    a rdf:Property ;
    rdfs:isDefinedBy <http://rdaregistry.info/Elements/u/> ;
    rdfs:label "is screenplay"@en ;
    rdfs:subPropertyOf <http://rdaregistry.info/Elements/u/P60198> ;
    owl:inverseOf <http://rdaregistry.info/Elements/u/P60201> ;
    skos:definition "Relates a resource to a resource that provides text for a motion picture, television program or video."@en .

<http://rdaregistry.info/Elements/u/P60265>
    reg:hasSubproperty <http://rdaregistry.info/Elements/e/P20158> ;
    reg:lexicalAlias <http://rdaregistry.info/Elements/u/motionPictureScreenplay.en> ;
    reg:name "motionPictureScreenplay"@en ;
    reg:status <http://metadataregistry.org/uri/RegStatus/1001> ;
    a rdf:Property ;
    rdfs:isDefinedBy <http://rdaregistry.info/Elements/u/> ;
    rdfs:label "is motion picture screenplay"@en ;
    rdfs:subPropertyOf <http://rdaregistry.info/Elements/u/P60264> ;
    owl:inverseOf <http://rdaregistry.info/Elements/u/P60282> ;
    skos:definition "Relates a resource to a resource that provides text for a motion picture."@en .

<http://rdaregistry.info/Elements/u/P60266>
    reg:hasSubproperty <http://rdaregistry.info/Elements/e/P20159> ;
    reg:lexicalAlias <http://rdaregistry.info/Elements/u/musicalSettingOf.en> ;
    reg:name "musicalSettingOf"@en ;
    reg:status <http://metadataregistry.org/uri/RegStatus/1001> ;
    a rdf:Property ;
    rdfs:isDefinedBy <http://rdaregistry.info/Elements/u/> ;
    rdfs:label "is musical setting of"@en ;
    rdfs:subPropertyOf <http://rdaregistry.info/Elements/u/P60305> ;
    owl:inverseOf <http://rdaregistry.info/Elements/u/P60121> ;
    skos:definition "Relates a resource to a resource that provides text for a non-dramatic musical resource, other than an oratorio."@en .

<http://rdaregistry.info/Elements/u/P60267>
    reg:hasSubproperty <http://rdaregistry.info/Elements/e/P20160> ;
    reg:lexicalAlias <http://rdaregistry.info/Elements/u/radioScript.en> ;
    reg:name "radioScript"@en ;
    reg:status <http://metadataregistry.org/uri/RegStatus/1001> ;
    a rdf:Property ;
    rdfs:isDefinedBy <http://rdaregistry.info/Elements/u/> ;
    rdfs:label "is radio script"@en ;
    rdfs:subPropertyOf <http://rdaregistry.info/Elements/u/P60198> ;
    owl:inverseOf <http://rdaregistry.info/Elements/u/P60285> ;
    skos:definition "Relates a resource to a resource that provides text for a radio program."@en .

<http://rdaregistry.info/Elements/u/P60268>
    reg:hasSubproperty <http://rdaregistry.info/Elements/e/P20161> ;
    reg:lexicalAlias <http://rdaregistry.info/Elements/u/televisionScreenplay.en> ;
    reg:name "televisionScreenplay"@en ;
    reg:status <http://metadataregistry.org/uri/RegStatus/1001> ;
    a rdf:Property ;
    rdfs:isDefinedBy <http://rdaregistry.info/Elements/u/> ;
    rdfs:label "is television screenplay"@en ;
    rdfs:subPropertyOf <http://rdaregistry.info/Elements/u/P60264> ;
    owl:inverseOf <http://rdaregistry.info/Elements/u/P60283> ;
    skos:definition "Relates a resource to a resource that provides text for a television program."@en .

<http://rdaregistry.info/Elements/u/P60269>
    reg:hasSubproperty <http://rdaregistry.info/Elements/e/P20162> ;
    reg:lexicalAlias <http://rdaregistry.info/Elements/u/videoScreenplay.en> ;
    reg:name "videoScreenplay"@en ;
    reg:status <http://metadataregistry.org/uri/RegStatus/1001> ;
    a rdf:Property ;
    rdfs:isDefinedBy <http://rdaregistry.info/Elements/u/> ;
    rdfs:label "is video screenplay"@en ;
    rdfs:subPropertyOf <http://rdaregistry.info/Elements/u/P60264> ;
    owl:inverseOf <http://rdaregistry.info/Elements/u/P60284> ;
    skos:definition "Relates a resource to a resource that provides text for a video."@en .

<http://rdaregistry.info/Elements/u/P60270>
    reg:hasSubproperty <http://rdaregistry.info/Elements/e/P20163> ;
    reg:lexicalAlias <http://rdaregistry.info/Elements/u/libretto.en> ;
    reg:name "libretto"@en ;
    reg:status <http://metadataregistry.org/uri/RegStatus/1001> ;
    a rdf:Property ;
    rdfs:isDefinedBy <http://rdaregistry.info/Elements/u/> ;
    rdfs:label "is libretto"@en ;
    rdfs:subPropertyOf <http://rdaregistry.info/Elements/u/P60198> ;
    owl:inverseOf <http://rdaregistry.info/Elements/u/P60117> ;
    skos:definition "Relates a resource to a resource that provides a text of an opera or other resource for the musical stage, or an oratorio."@en .

<http://rdaregistry.info/Elements/u/P60271>
    reg:hasSubproperty <http://rdaregistry.info/Elements/i/P40060>, <http://rdaregistry.info/Elements/m/P30038> ;
    reg:lexicalAlias <http://rdaregistry.info/Elements/u/reprintedAs.en> ;
    reg:name "reprintedAs"@en ;
    reg:status <http://metadataregistry.org/uri/RegStatus/1001> ;
    a rdf:Property ;
    rdfs:isDefinedBy <http://rdaregistry.info/Elements/u/> ;
    rdfs:label "is reprinted as"@en ;
    rdfs:subPropertyOf <http://rdaregistry.info/Elements/u/P60272> ;
    owl:inverseOf <http://rdaregistry.info/Elements/u/P60168> ;
    skos:definition "Relates a resource to a resource that reissues the same resource as a printed resource being described."@en .

<http://rdaregistry.info/Elements/u/P60272>
    reg:hasSubproperty <http://rdaregistry.info/Elements/i/P40055>, <http://rdaregistry.info/Elements/m/P30039>, <http://rdaregistry.info/Elements/u/P60083>, <http://rdaregistry.info/Elements/u/P60200>, <http://rdaregistry.info/Elements/u/P60217>, <http://rdaregistry.info/Elements/u/P60271> ;
    reg:lexicalAlias <http://rdaregistry.info/Elements/u/reproducedAs.en> ;
    reg:name "reproducedAs"@en ;
    reg:status <http://metadataregistry.org/uri/RegStatus/1001> ;
    a rdf:Property ;
    rdfs:isDefinedBy <http://rdaregistry.info/Elements/u/> ;
    rdfs:label "is reproduced as"@en ;
    rdfs:subPropertyOf <http://rdaregistry.info/Elements/u/P60191> ;
    owl:inverseOf <http://rdaregistry.info/Elements/u/P60297> ;
    skos:definition "Relates a resource to a resource that reproduces another resource."@en .

<http://rdaregistry.info/Elements/u/P60273>
    reg:hasSubproperty <http://rdaregistry.info/Elements/e/P20164> ;
    reg:lexicalAlias <http://rdaregistry.info/Elements/u/paraphrasedAs.en> ;
    reg:name "paraphrasedAs"@en ;
    reg:status <http://metadataregistry.org/uri/RegStatus/1001> ;
    a rdf:Property ;
    rdfs:isDefinedBy <http://rdaregistry.info/Elements/u/> ;
    rdfs:label "is paraphrased as"@en ;
    rdfs:subPropertyOf <http://rdaregistry.info/Elements/u/P60250> ;
    owl:inverseOf <http://rdaregistry.info/Elements/u/P60296> ;
    skos:definition "Relates a resource to a resource that restates a content of a source resource in a different form."@en .

<http://rdaregistry.info/Elements/u/P60274>
    reg:hasSubproperty <http://rdaregistry.info/Elements/e/P20165> ;
    reg:lexicalAlias <http://rdaregistry.info/Elements/u/arrangedAs.en> ;
    reg:name "arrangedAs"@en ;
    reg:status <http://metadataregistry.org/uri/RegStatus/1001> ;
    a rdf:Property ;
    rdfs:isDefinedBy <http://rdaregistry.info/Elements/u/> ;
    rdfs:label "is arranged as"@en ;
    rdfs:subPropertyOf <http://rdaregistry.info/Elements/u/P60250> ;
    owl:inverseOf <http://rdaregistry.info/Elements/u/P60242> ;
    skos:definition "Relates a resource to a musical resource that rewrites a source resource for a medium of performance different from that for which a resource was originally intended."@en .

<http://rdaregistry.info/Elements/u/P60275>
    reg:hasSubproperty <http://rdaregistry.info/Elements/e/P20166> ;
    reg:lexicalAlias <http://rdaregistry.info/Elements/u/abridgedAs.en> ;
    reg:name "abridgedAs"@en ;
    reg:status <http://metadataregistry.org/uri/RegStatus/1001> ;
    a rdf:Property ;
    rdfs:isDefinedBy <http://rdaregistry.info/Elements/u/> ;
    rdfs:label "is abridged as"@en ;
    rdfs:subPropertyOf <http://rdaregistry.info/Elements/u/P60250> ;
    owl:inverseOf <http://rdaregistry.info/Elements/u/P60223> ;
    skos:definition "Relates a resource to a resource that shortens a source resource without changing a general meaning or manner of presentation."@en .

<http://rdaregistry.info/Elements/u/P60276>
    reg:hasSubproperty <http://rdaregistry.info/Elements/e/P20167> ;
    reg:lexicalAlias <http://rdaregistry.info/Elements/u/continuationInPartOf.en> ;
    reg:name "continuationInPartOf"@en ;
    reg:status <http://metadataregistry.org/uri/RegStatus/1001> ;
    a rdf:Property ;
    rdfs:isDefinedBy <http://rdaregistry.info/Elements/u/> ;
    rdfs:label "is continuation in part of"@en ;
    rdfs:subPropertyOf <http://rdaregistry.info/Elements/u/P60261> ;
    owl:inverseOf <http://rdaregistry.info/Elements/u/P60503> ;
    skos:definition "Relates a resource to a resource that split into two or more separate resources with new titles."@en ;
    skos:scopeNote "This relationship applies generally to serials."@en .

<http://rdaregistry.info/Elements/u/P60277>
    reg:hasSubproperty <http://rdaregistry.info/Elements/e/P20168> ;
    reg:lexicalAlias <http://rdaregistry.info/Elements/u/separatedFrom.en> ;
    reg:name "separatedFrom"@en ;
    reg:status <http://metadataregistry.org/uri/RegStatus/1001> ;
    a rdf:Property ;
    rdfs:isDefinedBy <http://rdaregistry.info/Elements/u/> ;
    rdfs:label "is separated from"@en ;
    rdfs:subPropertyOf <http://rdaregistry.info/Elements/u/P60261> ;
    owl:inverseOf <http://rdaregistry.info/Elements/u/P60199> ;
    skos:definition "Relates a resource to a resource that spun off a part of its content to form a new resource."@en .

<http://rdaregistry.info/Elements/u/P60278>
    reg:hasSubproperty <http://rdaregistry.info/Elements/e/P20169>, <http://rdaregistry.info/Elements/u/P60102>, <http://rdaregistry.info/Elements/u/P60103>, <http://rdaregistry.info/Elements/u/P60104>, <http://rdaregistry.info/Elements/u/P60199>, <http://rdaregistry.info/Elements/u/P60247>, <http://rdaregistry.info/Elements/u/P60248>, <http://rdaregistry.info/Elements/u/P60306>, <http://rdaregistry.info/Elements/u/P60310>, <http://rdaregistry.info/Elements/u/P60503>, <http://rdaregistry.info/Elements/u/P60504> ;
    reg:lexicalAlias <http://rdaregistry.info/Elements/u/succeededBy.en> ;
    reg:name "succeededBy"@en ;
    reg:status <http://metadataregistry.org/uri/RegStatus/1001> ;
    a rdf:Property ;
    rdfs:isDefinedBy <http://rdaregistry.info/Elements/u/> ;
    rdfs:label "is succeeded by"@en ;
    rdfs:subPropertyOf <http://rdaregistry.info/Elements/u/P60713> ;
    owl:inverseOf <http://rdaregistry.info/Elements/u/P60261> ;
    skos:definition "Relates a resource to a resource that succeeds, that is, is later in time or after in a narrative, etc., a preceding resource."@en .

<http://rdaregistry.info/Elements/u/P60279>
    reg:hasSubproperty <http://rdaregistry.info/Elements/e/P20170> ;
    reg:lexicalAlias <http://rdaregistry.info/Elements/u/digestedAs.en> ;
    reg:name "digestedAs"@en ;
    reg:status <http://metadataregistry.org/uri/RegStatus/1001> ;
    a rdf:Property ;
    rdfs:isDefinedBy <http://rdaregistry.info/Elements/u/> ;
    rdfs:label "is digested as"@en ;
    rdfs:subPropertyOf <http://rdaregistry.info/Elements/u/P60250> ;
    owl:inverseOf <http://rdaregistry.info/Elements/u/P60238> ;
    skos:definition "Relates a resource to a resource that systematically and comprehensively condenses a source resource."@en .

<http://rdaregistry.info/Elements/u/P60280>
    reg:hasSubproperty <http://rdaregistry.info/Elements/e/P20171>, <http://rdaregistry.info/Elements/u/P60112> ;
    reg:lexicalAlias <http://rdaregistry.info/Elements/u/translatedAs.en> ;
    reg:name "translatedAs"@en ;
    reg:status <http://metadataregistry.org/uri/RegStatus/1001> ;
    a rdf:Property ;
    rdfs:isDefinedBy <http://rdaregistry.info/Elements/u/> ;
    rdfs:label "is translated as"@en ;
    rdfs:subPropertyOf <http://rdaregistry.info/Elements/u/P60250> ;
    owl:inverseOf <http://rdaregistry.info/Elements/u/P60244> ;
    skos:definition "Relates a resource to a resource that translates the text of a source entity into a language different from that of an original resource."@en .

<http://rdaregistry.info/Elements/u/P60281>
    reg:hasSubproperty <http://rdaregistry.info/Elements/e/P20172> ;
    reg:lexicalAlias <http://rdaregistry.info/Elements/u/supplement.en> ;
    reg:name "supplement"@en ;
    reg:status <http://metadataregistry.org/uri/RegStatus/1001> ;
    a rdf:Property ;
    rdfs:isDefinedBy <http://rdaregistry.info/Elements/u/> ;
    rdfs:label "is supplement"@en ;
    rdfs:subPropertyOf <http://rdaregistry.info/Elements/u/P60204> ;
    owl:inverseOf <http://rdaregistry.info/Elements/u/P60259> ;
    skos:definition "Relates a resource to a resource that updates or otherwise complements a predominant resource."@en .

<http://rdaregistry.info/Elements/u/P60282>
    reg:hasSubproperty <http://rdaregistry.info/Elements/e/P20173> ;
    reg:lexicalAlias <http://rdaregistry.info/Elements/u/screenplayForMotionPicture.en> ;
    reg:name "screenplayForMotionPicture"@en ;
    reg:status <http://metadataregistry.org/uri/RegStatus/1001> ;
    a rdf:Property ;
    rdfs:isDefinedBy <http://rdaregistry.info/Elements/u/> ;
    rdfs:label "is screenplay for motion picture"@en ;
    rdfs:subPropertyOf <http://rdaregistry.info/Elements/u/P60201> ;
    owl:inverseOf <http://rdaregistry.info/Elements/u/P60265> ;
    skos:definition "Relates a resource to a resource that uses a text as a screenplay for a motion picture."@en .

<http://rdaregistry.info/Elements/u/P60283>
    reg:hasSubproperty <http://rdaregistry.info/Elements/e/P20174> ;
    reg:lexicalAlias <http://rdaregistry.info/Elements/u/screenplayForTelevisionProgram.en> ;
    reg:name "screenplayForTelevisionProgram"@en ;
    reg:status <http://metadataregistry.org/uri/RegStatus/1001> ;
    a rdf:Property ;
    rdfs:isDefinedBy <http://rdaregistry.info/Elements/u/> ;
    rdfs:label "is screenplay for television program"@en ;
    rdfs:subPropertyOf <http://rdaregistry.info/Elements/u/P60201> ;
    owl:inverseOf <http://rdaregistry.info/Elements/u/P60268> ;
    skos:definition "Relates a resource to a resource that uses a text as a screenplay for a television program."@en .

<http://rdaregistry.info/Elements/u/P60284>
    reg:hasSubproperty <http://rdaregistry.info/Elements/e/P20175> ;
    reg:lexicalAlias <http://rdaregistry.info/Elements/u/screenplayForVideo.en> ;
    reg:name "screenplayForVideo"@en ;
    reg:status <http://metadataregistry.org/uri/RegStatus/1001> ;
    a rdf:Property ;
    rdfs:isDefinedBy <http://rdaregistry.info/Elements/u/> ;
    rdfs:label "is screenplay for video"@en ;
    rdfs:subPropertyOf <http://rdaregistry.info/Elements/u/P60201> ;
    owl:inverseOf <http://rdaregistry.info/Elements/u/P60269> ;
    skos:definition "Relates a resource to a resource that uses a text as a screenplay for a video."@en .

<http://rdaregistry.info/Elements/u/P60285>
    reg:hasSubproperty <http://rdaregistry.info/Elements/e/P20176> ;
    reg:lexicalAlias <http://rdaregistry.info/Elements/u/scriptForRadioProgram.en> ;
    reg:name "scriptForRadioProgram"@en ;
    reg:status <http://metadataregistry.org/uri/RegStatus/1001> ;
    a rdf:Property ;
    rdfs:isDefinedBy <http://rdaregistry.info/Elements/u/> ;
    rdfs:label "is script for radio program"@en ;
    rdfs:subPropertyOf <http://rdaregistry.info/Elements/u/P60198> ;
    owl:inverseOf <http://rdaregistry.info/Elements/u/P60267> ;
    skos:definition "Relates a resource to a resource that uses a text of a source resource as a script for a radio program."@en .

<http://rdaregistry.info/Elements/u/P60286>
    reg:hasSubproperty <http://rdaregistry.info/Elements/e/P20177> ;
    reg:lexicalAlias <http://rdaregistry.info/Elements/u/addendaTo.en> ;
    reg:name "addendaTo"@en ;
    reg:status <http://metadataregistry.org/uri/RegStatus/1001> ;
    a rdf:Property ;
    rdfs:isDefinedBy <http://rdaregistry.info/Elements/u/> ;
    rdfs:label "is addenda to"@en ;
    rdfs:subPropertyOf <http://rdaregistry.info/Elements/u/P60307> ;
    owl:inverseOf <http://rdaregistry.info/Elements/u/P60209> ;
    skos:definition "Relates a resource to a resource whose content is completed with brief content from another resource."@en .

<http://rdaregistry.info/Elements/u/P60287>
    reg:hasSubproperty <http://rdaregistry.info/Elements/i/P40039>, <http://rdaregistry.info/Elements/m/P30040> ;
    reg:lexicalAlias <http://rdaregistry.info/Elements/u/digitalTransferOf.en> ;
    reg:name "digitalTransferOf"@en ;
    reg:status <http://metadataregistry.org/uri/RegStatus/1001> ;
    a rdf:Property ;
    rdfs:isDefinedBy <http://rdaregistry.info/Elements/u/> ;
    rdfs:label "is digital transfer of"@en ;
    rdfs:subPropertyOf <http://rdaregistry.info/Elements/u/P60297> ;
    owl:inverseOf <http://rdaregistry.info/Elements/u/P60200> ;
    skos:definition "Relates a resource to a resource in a digital format that is transferred to another digital format."@en .

<http://rdaregistry.info/Elements/u/P60288>
    reg:hasSubproperty <http://rdaregistry.info/Elements/w/P10268>, <http://rdaregistry.info/Elements/w/P10274>, <http://rdaregistry.info/Elements/w/P10280> ;
    reg:lexicalAlias <http://rdaregistry.info/Elements/u/reviewOf.en> ;
    reg:name "reviewOf"@en ;
    reg:status <http://metadataregistry.org/uri/RegStatus/1001> ;
    a rdf:Property ;
    rdfs:isDefinedBy <http://rdaregistry.info/Elements/u/> ;
    rdfs:label "is review of"@en ;
    rdfs:subPropertyOf <http://rdaregistry.info/Elements/u/P60190> ;
    owl:inverseOf <http://rdaregistry.info/Elements/u/P60211> ;
    skos:definition "Relates a resource to a resource used as a basis for a brief evaluation."@en .

<http://rdaregistry.info/Elements/u/P60289>
    reg:hasSubproperty <http://rdaregistry.info/Elements/e/P20179> ;
    reg:lexicalAlias <http://rdaregistry.info/Elements/u/summaryOf.en> ;
    reg:name "summaryOf"@en ;
    reg:status <http://metadataregistry.org/uri/RegStatus/1001> ;
    a rdf:Property ;
    rdfs:isDefinedBy <http://rdaregistry.info/Elements/u/> ;
    rdfs:label "is summary of"@en ;
    rdfs:subPropertyOf <http://rdaregistry.info/Elements/u/P60305> ;
    owl:inverseOf <http://rdaregistry.info/Elements/u/P60205> ;
    skos:definition "Relates a resource to a resource used as a basis for a brief recapitulation of its content."@en .

<http://rdaregistry.info/Elements/u/P60290>
    reg:hasSubproperty <http://rdaregistry.info/Elements/e/P20180> ;
    reg:lexicalAlias <http://rdaregistry.info/Elements/u/catalogueOf.en> ;
    reg:name "catalogueOf"@en ;
    reg:status <http://metadataregistry.org/uri/RegStatus/1001> ;
    a rdf:Property ;
    rdfs:isDefinedBy <http://rdaregistry.info/Elements/u/> ;
    rdfs:label "is catalogue of"@en ;
    rdfs:subPropertyOf <http://rdaregistry.info/Elements/u/P60307> ;
    owl:inverseOf <http://rdaregistry.info/Elements/u/P60206> ;
    skos:definition "Relates a resource to a resource used as a basis for a catalogue, i.e., a complete enumeration of resources arranged systematically."@en .

<http://rdaregistry.info/Elements/u/P60291>
    reg:hasSubproperty <http://rdaregistry.info/Elements/e/P20181> ;
    reg:lexicalAlias <http://rdaregistry.info/Elements/u/concordanceTo.en> ;
    reg:name "concordanceTo"@en ;
    reg:status <http://metadataregistry.org/uri/RegStatus/1001> ;
    a rdf:Property ;
    rdfs:isDefinedBy <http://rdaregistry.info/Elements/u/> ;
    rdfs:label "is concordance to"@en ;
    rdfs:subPropertyOf <http://rdaregistry.info/Elements/u/P60307> ;
    owl:inverseOf <http://rdaregistry.info/Elements/u/P60208> ;
    skos:definition "Relates a resource to a resource used as a basis for a concordance, i.e. an index of all the words in the predominant resource."@en .

<http://rdaregistry.info/Elements/u/P60292>
    reg:hasSubproperty <http://rdaregistry.info/Elements/w/P10269>, <http://rdaregistry.info/Elements/w/P10275>, <http://rdaregistry.info/Elements/w/P10281> ;
    reg:lexicalAlias <http://rdaregistry.info/Elements/u/critiqueOf.en> ;
    reg:name "critiqueOf"@en ;
    reg:status <http://metadataregistry.org/uri/RegStatus/1001> ;
    a rdf:Property ;
    rdfs:isDefinedBy <http://rdaregistry.info/Elements/u/> ;
    rdfs:label "is critique of"@en ;
    rdfs:subPropertyOf <http://rdaregistry.info/Elements/u/P60190> ;
    owl:inverseOf <http://rdaregistry.info/Elements/u/P60212> ;
    skos:definition "Relates a resource to a resource used as a basis for a critical evaluation."@en .

<http://rdaregistry.info/Elements/u/P60293>
    reg:hasSubproperty <http://rdaregistry.info/Elements/e/P20183> ;
    reg:lexicalAlias <http://rdaregistry.info/Elements/u/choreographicAdaptationOf.en> ;
    reg:name "choreographicAdaptationOf"@en ;
    reg:status <http://metadataregistry.org/uri/RegStatus/1001> ;
    a rdf:Property ;
    rdfs:isDefinedBy <http://rdaregistry.info/Elements/u/> ;
    rdfs:label "is choreographic adaptation of"@en ;
    rdfs:subPropertyOf <http://rdaregistry.info/Elements/u/P60305> ;
    owl:inverseOf <http://rdaregistry.info/Elements/u/P60180> ;
    skos:definition "Relates a resource to a resource that has been adapted as a resource consisting of movement."@en .

<http://rdaregistry.info/Elements/u/P60294>
    reg:hasSubproperty <http://rdaregistry.info/Elements/e/P20184> ;
    reg:lexicalAlias <http://rdaregistry.info/Elements/u/expandedVersionOf.en> ;
    reg:name "expandedVersionOf"@en ;
    reg:status <http://metadataregistry.org/uri/RegStatus/1001> ;
    a rdf:Property ;
    rdfs:isDefinedBy <http://rdaregistry.info/Elements/u/> ;
    rdfs:label "is expanded version of"@en ;
    rdfs:subPropertyOf <http://rdaregistry.info/Elements/u/P60305> ;
    owl:inverseOf <http://rdaregistry.info/Elements/u/P60216> ;
    skos:definition "Relates a resource to a resource used as a basis for a derivative resource that enlarges upon the content of a source resource."@en .

<http://rdaregistry.info/Elements/u/P60295>
    reg:hasSubproperty <http://rdaregistry.info/Elements/e/P20185> ;
    reg:lexicalAlias <http://rdaregistry.info/Elements/u/remakeOf.en> ;
    reg:name "remakeOf"@en ;
    reg:status <http://metadataregistry.org/uri/RegStatus/1001> ;
    a rdf:Property ;
    rdfs:isDefinedBy <http://rdaregistry.info/Elements/u/> ;
    rdfs:label "is remake of"@en ;
    rdfs:subPropertyOf <http://rdaregistry.info/Elements/u/P60305> ;
    owl:inverseOf <http://rdaregistry.info/Elements/u/P60120> ;
    skos:definition "Relates a resource to a resource used as a basis for a new motion picture, radio program, television program, or video."@en .

<http://rdaregistry.info/Elements/u/P60296>
    reg:hasSubproperty <http://rdaregistry.info/Elements/e/P20186> ;
    reg:lexicalAlias <http://rdaregistry.info/Elements/u/paraphraseOf.en> ;
    reg:name "paraphraseOf"@en ;
    reg:status <http://metadataregistry.org/uri/RegStatus/1001> ;
    a rdf:Property ;
    rdfs:isDefinedBy <http://rdaregistry.info/Elements/u/> ;
    rdfs:label "is paraphrase of"@en ;
    rdfs:subPropertyOf <http://rdaregistry.info/Elements/u/P60305> ;
    owl:inverseOf <http://rdaregistry.info/Elements/u/P60273> ;
    skos:definition "Relates a resource to a resource used as a basis for a paraphrase, i.e., a restating of the content of the source resource in a different form."@en .

<http://rdaregistry.info/Elements/u/P60297>
    reg:hasSubproperty <http://rdaregistry.info/Elements/i/P40042>, <http://rdaregistry.info/Elements/m/P30043>, <http://rdaregistry.info/Elements/u/P60168>, <http://rdaregistry.info/Elements/u/P60287>, <http://rdaregistry.info/Elements/u/P60301>, <http://rdaregistry.info/Elements/u/P60469> ;
    reg:lexicalAlias <http://rdaregistry.info/Elements/u/reproductionOf.en> ;
    reg:name "reproductionOf"@en ;
    reg:status <http://metadataregistry.org/uri/RegStatus/1001> ;
    a rdf:Property ;
    rdfs:isDefinedBy <http://rdaregistry.info/Elements/u/> ;
    rdfs:label "is reproduction of"@en ;
    rdfs:subPropertyOf <http://rdaregistry.info/Elements/u/P60191> ;
    owl:inverseOf <http://rdaregistry.info/Elements/u/P60272> ;
    skos:definition "Relates a resource to a resource that is used as a basis for a reproduction."@en .

<http://rdaregistry.info/Elements/u/P60298>
    reg:hasSubproperty <http://rdaregistry.info/Elements/w/P10270>, <http://rdaregistry.info/Elements/w/P10276>, <http://rdaregistry.info/Elements/w/P10282> ;
    reg:lexicalAlias <http://rdaregistry.info/Elements/u/commentaryOn.en> ;
    reg:name "commentaryOn"@en ;
    reg:status <http://metadataregistry.org/uri/RegStatus/1001> ;
    a rdf:Property ;
    rdfs:isDefinedBy <http://rdaregistry.info/Elements/u/> ;
    rdfs:label "is commentary on"@en ;
    rdfs:subPropertyOf <http://rdaregistry.info/Elements/u/P60190> ;
    owl:inverseOf <http://rdaregistry.info/Elements/u/P60213> ;
    skos:definition "Relates a resource to a resource used as a basis for a set of explanatory or critical notes."@en .

<http://rdaregistry.info/Elements/u/P60299>
    reg:hasSubproperty <http://rdaregistry.info/Elements/i/P40044>, <http://rdaregistry.info/Elements/m/P30045> ;
    reg:lexicalAlias <http://rdaregistry.info/Elements/u/preservationFacsimileOf.en> ;
    reg:name "preservationFacsimileOf"@en ;
    reg:status <http://metadataregistry.org/uri/RegStatus/1001> ;
    a rdf:Property ;
    rdfs:isDefinedBy <http://rdaregistry.info/Elements/u/> ;
    rdfs:label "is preservation facsimile of"@en ;
    rdfs:subPropertyOf <http://rdaregistry.info/Elements/u/P60301> ;
    owl:inverseOf <http://rdaregistry.info/Elements/u/P60179> ;
    skos:definition "Relates a resource to a resource that is used as a basis for an exact reproduction on preservation-quality media, such as acid-free permanent or archival paper."@en .

<http://rdaregistry.info/Elements/u/P60300>
    reg:hasSubproperty <http://rdaregistry.info/Elements/m/P30046> ;
    reg:lexicalAlias <http://rdaregistry.info/Elements/u/facsimileContainerOf.en> ;
    reg:name "facsimileContainerOf"@en ;
    reg:status <http://metadataregistry.org/uri/RegStatus/1001> ;
    a rdf:Property ;
    rdfs:isDefinedBy <http://rdaregistry.info/Elements/u/> ;
    rdfs:label "is facsimile container of"@en ;
    rdfs:subPropertyOf <http://rdaregistry.info/Elements/u/P60249> ;
    owl:inverseOf <http://rdaregistry.info/Elements/u/P60100> ;
    skos:definition "Relates a resource to a resource used as a basis for an exact reproduction that is a discrete component of a larger entity."@en .

<http://rdaregistry.info/Elements/u/P60301>
    reg:hasSubproperty <http://rdaregistry.info/Elements/i/P40045>, <http://rdaregistry.info/Elements/m/P30047>, <http://rdaregistry.info/Elements/u/P60299> ;
    reg:lexicalAlias <http://rdaregistry.info/Elements/u/facsimileOf.en> ;
    reg:name "facsimileOf"@en ;
    reg:status <http://metadataregistry.org/uri/RegStatus/1001> ;
    a rdf:Property ;
    rdfs:isDefinedBy <http://rdaregistry.info/Elements/u/> ;
    rdfs:label "is facsimile of"@en ;
    rdfs:subPropertyOf <http://rdaregistry.info/Elements/u/P60297> ;
    owl:inverseOf <http://rdaregistry.info/Elements/u/P60217> ;
    skos:definition "Relates a resource to a resource that is used as a basis for an exact reproduction."@en .

<http://rdaregistry.info/Elements/u/P60302>
    reg:hasSubproperty <http://rdaregistry.info/Elements/e/P20188> ;
    reg:lexicalAlias <http://rdaregistry.info/Elements/u/indexTo.en> ;
    reg:name "indexTo"@en ;
    reg:status <http://metadataregistry.org/uri/RegStatus/1001> ;
    a rdf:Property ;
    rdfs:isDefinedBy <http://rdaregistry.info/Elements/u/> ;
    rdfs:label "is index to"@en ;
    rdfs:subPropertyOf <http://rdaregistry.info/Elements/u/P60307> ;
    owl:inverseOf <http://rdaregistry.info/Elements/u/P60263> ;
    skos:definition "Relates a resource to a resource used as a basis for an index, i.e., a systematic, alphabetical guide to the contents of a predominant resource, usually keyed to page numbers or other reference codes."@en .

<http://rdaregistry.info/Elements/u/P60303>
    reg:hasSubproperty <http://rdaregistry.info/Elements/e/P20189> ;
    reg:lexicalAlias <http://rdaregistry.info/Elements/u/revisionOf.en> ;
    reg:name "revisionOf"@en ;
    reg:status <http://metadataregistry.org/uri/RegStatus/1001> ;
    a rdf:Property ;
    rdfs:isDefinedBy <http://rdaregistry.info/Elements/u/> ;
    rdfs:label "is revision of"@en ;
    rdfs:subPropertyOf <http://rdaregistry.info/Elements/u/P60305> ;
    owl:inverseOf <http://rdaregistry.info/Elements/u/P60245> ;
    skos:definition "Relates a resource to a resource used as a basis for an updated, corrected, or expanded version."@en .

<http://rdaregistry.info/Elements/u/P60304>
    reg:hasSubproperty <http://rdaregistry.info/Elements/e/P20190> ;
    reg:lexicalAlias <http://rdaregistry.info/Elements/u/librettoBasedOn.en> ;
    reg:name "librettoBasedOn"@en ;
    reg:status <http://metadataregistry.org/uri/RegStatus/1001> ;
    a rdf:Property ;
    rdfs:isDefinedBy <http://rdaregistry.info/Elements/u/> ;
    rdfs:label "is libretto based on"@en ;
    rdfs:subPropertyOf <http://rdaregistry.info/Elements/u/P60305> ;
    owl:inverseOf <http://rdaregistry.info/Elements/u/P60210> ;
    skos:definition "Relates a resource to a resource that has been adapted as a text of an opera or other resource for the musical stage, or an oratorio."@en .

<http://rdaregistry.info/Elements/u/P60305>
    reg:hasSubproperty <http://rdaregistry.info/Elements/e/P20204>, <http://rdaregistry.info/Elements/u/P60114>, <http://rdaregistry.info/Elements/u/P60223>, <http://rdaregistry.info/Elements/u/P60224>, <http://rdaregistry.info/Elements/u/P60238>, <http://rdaregistry.info/Elements/u/P60241>, <http://rdaregistry.info/Elements/u/P60242>, <http://rdaregistry.info/Elements/u/P60243>, <http://rdaregistry.info/Elements/u/P60244>, <http://rdaregistry.info/Elements/u/P60266>, <http://rdaregistry.info/Elements/u/P60289>, <http://rdaregistry.info/Elements/u/P60293>, <http://rdaregistry.info/Elements/u/P60294>, <http://rdaregistry.info/Elements/u/P60295>, <http://rdaregistry.info/Elements/u/P60296>, <http://rdaregistry.info/Elements/u/P60303>, <http://rdaregistry.info/Elements/u/P60304>, <http://rdaregistry.info/Elements/u/P60308>, <http://rdaregistry.info/Elements/u/P60309>, <http://rdaregistry.info/Elements/u/P60311>, <http://rdaregistry.info/Elements/u/P60830>, <http://rdaregistry.info/Elements/u/P60832> ;
    reg:lexicalAlias <http://rdaregistry.info/Elements/u/basedOn.en> ;
    reg:name "basedOn"@en ;
    reg:status <http://metadataregistry.org/uri/RegStatus/1001> ;
    a rdf:Property ;
    rdfs:isDefinedBy <http://rdaregistry.info/Elements/u/> ;
    rdfs:label "is based on"@en ;
    rdfs:subPropertyOf <http://rdaregistry.info/Elements/u/P60710> ;
    owl:inverseOf <http://rdaregistry.info/Elements/u/P60250> ;
    skos:definition "Relates a resource to a resource used as a source for a derivative resource."@en .

<http://rdaregistry.info/Elements/u/P60306>
    reg:hasSubproperty <http://rdaregistry.info/Elements/e/P20191> ;
    reg:lexicalAlias <http://rdaregistry.info/Elements/u/continuedBy.en> ;
    reg:name "continuedBy"@en ;
    reg:status <http://metadataregistry.org/uri/RegStatus/1001> ;
    a rdf:Property ;
    rdfs:isDefinedBy <http://rdaregistry.info/Elements/u/> ;
    rdfs:label "is continued by"@en ;
    rdfs:subPropertyOf <http://rdaregistry.info/Elements/u/P60278> ;
    owl:inverseOf <http://rdaregistry.info/Elements/u/P60576> ;
    skos:definition "Relates a resource to a resource whose content continues an earlier resource under a new title."@en ;
    skos:scopeNote "This relationship applies generally to serials."@en .

<http://rdaregistry.info/Elements/u/P60307>
    reg:hasSubproperty <http://rdaregistry.info/Elements/e/P20192>, <http://rdaregistry.info/Elements/u/P60116>, <http://rdaregistry.info/Elements/u/P60251>, <http://rdaregistry.info/Elements/u/P60252>, <http://rdaregistry.info/Elements/u/P60253>, <http://rdaregistry.info/Elements/u/P60254>, <http://rdaregistry.info/Elements/u/P60259>, <http://rdaregistry.info/Elements/u/P60286>, <http://rdaregistry.info/Elements/u/P60290>, <http://rdaregistry.info/Elements/u/P60291>, <http://rdaregistry.info/Elements/u/P60302>, <http://rdaregistry.info/Elements/u/P60474> ;
    reg:lexicalAlias <http://rdaregistry.info/Elements/u/augmentationOf.en> ;
    reg:name "augmentationOf"@en ;
    reg:status <http://metadataregistry.org/uri/RegStatus/1001> ;
    a rdf:Property ;
    rdfs:isDefinedBy <http://rdaregistry.info/Elements/u/> ;
    rdfs:label "is augmentation of"@en ;
    rdfs:subPropertyOf <http://rdaregistry.info/Elements/u/P60709> ;
    owl:inverseOf <http://rdaregistry.info/Elements/u/P60204> ;
    skos:definition "Relates a resource to a resource whose content is added to by another resource."@en .

<http://rdaregistry.info/Elements/u/P60308>
    reg:hasSubproperty <http://rdaregistry.info/Elements/e/P20193> ;
    reg:lexicalAlias <http://rdaregistry.info/Elements/u/abstractsFor.en> ;
    reg:name "abstractsFor"@en ;
    reg:status <http://metadataregistry.org/uri/RegStatus/1001> ;
    a rdf:Property ;
    rdfs:isDefinedBy <http://rdaregistry.info/Elements/u/> ;
    rdfs:label "is abstracts for"@en ;
    rdfs:subPropertyOf <http://rdaregistry.info/Elements/u/P60305> ;
    owl:inverseOf <http://rdaregistry.info/Elements/u/P60177> ;
    skos:definition "Relates a resource to a resource whose contents have been abstracted by an abstracting and indexing service."@en .

<http://rdaregistry.info/Elements/u/P60309>
    reg:hasSubproperty <http://rdaregistry.info/Elements/e/P20194> ;
    reg:lexicalAlias <http://rdaregistry.info/Elements/u/indexingFor.en> ;
    reg:name "indexingFor"@en ;
    reg:status <http://metadataregistry.org/uri/RegStatus/1001> ;
    a rdf:Property ;
    rdfs:isDefinedBy <http://rdaregistry.info/Elements/u/> ;
    rdfs:label "is indexing for"@en ;
    rdfs:subPropertyOf <http://rdaregistry.info/Elements/u/P60305> ;
    owl:inverseOf <http://rdaregistry.info/Elements/u/P60178> ;
    skos:definition "Relates a resource to a resource whose contents have been indexed by an abstracting and indexing service."@en .

<http://rdaregistry.info/Elements/u/P60310>
    reg:lexicalAlias <http://rdaregistry.info/Elements/u/prequelTo.en> ;
    reg:name "prequelTo"@en ;
    reg:status <http://metadataregistry.org/uri/RegStatus/1001> ;
    a rdf:Property ;
    rdfs:isDefinedBy <http://rdaregistry.info/Elements/u/> ;
    rdfs:label "is prequel to"@en ;
    rdfs:subPropertyOf <http://rdaregistry.info/Elements/u/P60278> ;
    owl:inverseOf <http://rdaregistry.info/Elements/u/P60220> ;
    skos:definition "Relates a resource to a resource whose narrative is extended backwards in time by the later resource."@en .

<http://rdaregistry.info/Elements/u/P60311>
    reg:hasSubproperty <http://rdaregistry.info/Elements/e/P20195>, <http://rdaregistry.info/Elements/u/P60312> ;
    reg:lexicalAlias <http://rdaregistry.info/Elements/u/imitationOf.en> ;
    reg:name "imitationOf"@en ;
    reg:status <http://metadataregistry.org/uri/RegStatus/1001> ;
    a rdf:Property ;
    rdfs:isDefinedBy <http://rdaregistry.info/Elements/u/> ;
    rdfs:label "is imitation of"@en ;
    rdfs:subPropertyOf <http://rdaregistry.info/Elements/u/P60305> ;
    owl:inverseOf <http://rdaregistry.info/Elements/u/P60214> ;
    skos:definition "Relates a resource to a resource whose style or content is copied in a derivative resource."@en .

<http://rdaregistry.info/Elements/u/P60312>
    reg:hasSubproperty <http://rdaregistry.info/Elements/e/P20196> ;
    reg:lexicalAlias <http://rdaregistry.info/Elements/u/parodyOf.en> ;
    reg:name "parodyOf"@en ;
    reg:status <http://metadataregistry.org/uri/RegStatus/1001> ;
    a rdf:Property ;
    rdfs:isDefinedBy <http://rdaregistry.info/Elements/u/> ;
    rdfs:label "is parody of"@en ;
    rdfs:subPropertyOf <http://rdaregistry.info/Elements/u/P60311> ;
    owl:inverseOf <http://rdaregistry.info/Elements/u/P60246> ;
    skos:definition "Relates a resource to a resource whose style or content is imitated for comic effect."@en .

<http://rdaregistry.info/Elements/u/P60313>
    reg:hasSubproperty <http://rdaregistry.info/Elements/e/P20205>, <http://rdaregistry.info/Elements/i/P40046>, <http://rdaregistry.info/Elements/i/P40069>, <http://rdaregistry.info/Elements/i/P40070>, <http://rdaregistry.info/Elements/i/P40071>, <http://rdaregistry.info/Elements/m/P30048>, <http://rdaregistry.info/Elements/m/P30140>, <http://rdaregistry.info/Elements/m/P30265>, <http://rdaregistry.info/Elements/m/P30266> ;
    reg:lexicalAlias <http://rdaregistry.info/Elements/u/relatedResource.en> ;
    reg:name "relatedResource"@en ;
    reg:status <http://metadataregistry.org/uri/RegStatus/1001> ;
    a rdf:Property ;
    rdfs:isDefinedBy <http://rdaregistry.info/Elements/u/> ;
    rdfs:label "has related resource"@en ;
    skos:definition "Relates a resource to a resource that is related to a resource being described."@en .

<http://rdaregistry.info/Elements/u/P60314>
    reg:hasSubproperty <http://rdaregistry.info/Elements/m/P30096> ;
    reg:lexicalAlias <http://rdaregistry.info/Elements/u/encodingFormat.en> ;
    reg:name "encodingFormat"@en ;
    reg:status <http://metadataregistry.org/uri/RegStatus/1001> ;
    a rdf:Property ;
    rdfs:isDefinedBy <http://rdaregistry.info/Elements/u/> ;
    rdfs:label "has encoding format"@en ;
    rdfs:subPropertyOf <http://rdaregistry.info/Elements/u/P60350> ;
    skos:definition "Relates a resource to a schema, standard, etc., used to encode the digital content of a resource."@en .

<http://rdaregistry.info/Elements/u/P60315>
    reg:lexicalAlias <http://rdaregistry.info/Elements/u/numericDesignationOfMusicalResource.en> ;
    reg:name "numericDesignationOfMusicalResource"@en ;
    reg:status <http://metadataregistry.org/uri/RegStatus/1001> ;
    a rdf:Property ;
    rdfs:isDefinedBy <http://rdaregistry.info/Elements/u/> ;
    rdfs:label "has numeric designation of musical resource"@en ;
    skos:definition "Relates a resource to a serial number, opus number, or thematic index number assigned to a musical resource by a composer, publisher, or a musicologist."@en ;
    skos:scopeNote "A numeric designation of a musical resource includes a caption such as e.g., no., op., BWV, and it may include a numeral, a letter, a word, any other character, or the combination of these."@en .

<http://rdaregistry.info/Elements/u/P60316>
    reg:lexicalAlias <http://rdaregistry.info/Elements/u/subseries.en> ;
    reg:name "subseries"@en ;
    reg:status <http://metadataregistry.org/uri/RegStatus/1001> ;
    a rdf:Property ;
    rdfs:isDefinedBy <http://rdaregistry.info/Elements/u/> ;
    rdfs:label "is subseries"@en ;
    rdfs:subPropertyOf <http://rdaregistry.info/Elements/u/P60249> ;
    owl:inverseOf <http://rdaregistry.info/Elements/u/P60192> ;
    skos:definition "Relates a resource to a serial or multipart resource that consistently appears in a larger resource; a title of the larger resource appears on all issues or parts of a subseries"@en .

<http://rdaregistry.info/Elements/u/P60317>
    reg:hasSubproperty <http://rdaregistry.info/Elements/m/P30101> ;
    reg:lexicalAlias <http://rdaregistry.info/Elements/u/specialIssueOf.en> ;
    reg:name "specialIssueOf"@en ;
    reg:status <http://metadataregistry.org/uri/RegStatus/1001> ;
    a rdf:Property ;
    rdfs:isDefinedBy <http://rdaregistry.info/Elements/u/> ;
    rdfs:label "is special issue of"@en ;
    rdfs:subPropertyOf <http://rdaregistry.info/Elements/u/P60101> ;
    owl:inverseOf <http://rdaregistry.info/Elements/u/P60207> ;
    skos:definition "Relates a resource to a serial or newspaper containing a single issue or a supplementary section devoted to a special subject, with or without serial numbering, such as an anniversary number of a periodical or newspaper."@en .

<http://rdaregistry.info/Elements/u/P60318>
    reg:hasSubproperty <http://rdaregistry.info/Elements/e/P20061> ;
    reg:lexicalAlias <http://rdaregistry.info/Elements/u/formOfTactileNotation.en> ;
    reg:name "formOfTactileNotation"@en ;
    reg:status <http://metadataregistry.org/uri/RegStatus/1001> ;
    a rdf:Property ;
    rdfs:isDefinedBy <http://rdaregistry.info/Elements/u/> ;
    rdfs:label "has form of tactile notation"@en ;
    rdfs:subPropertyOf <http://rdaregistry.info/Elements/u/P60319> ;
    skos:definition "Relates a resource to a set of characters or symbols used to express the content of a resource in a form that can be perceived through touch."@en .

<http://rdaregistry.info/Elements/u/P60319>
    reg:hasSubproperty <http://rdaregistry.info/Elements/e/P20062>, <http://rdaregistry.info/Elements/u/P60318>, <http://rdaregistry.info/Elements/u/P60320>, <http://rdaregistry.info/Elements/u/P60321>, <http://rdaregistry.info/Elements/u/P60322> ;
    reg:lexicalAlias <http://rdaregistry.info/Elements/u/formOfNotation.en> ;
    reg:name "formOfNotation"@en ;
    reg:status <http://metadataregistry.org/uri/RegStatus/1001> ;
    a rdf:Property ;
    rdfs:isDefinedBy <http://rdaregistry.info/Elements/u/> ;
    rdfs:label "has form of notation"@en ;
    skos:definition "Relates a resource to a set of characters or symbols used to express the content of a resource."@en .

<http://rdaregistry.info/Elements/u/P60320>
    reg:hasSubproperty <http://rdaregistry.info/Elements/e/P20063> ;
    reg:lexicalAlias <http://rdaregistry.info/Elements/u/formOfNotatedMovement.en> ;
    reg:name "formOfNotatedMovement"@en ;
    reg:status <http://metadataregistry.org/uri/RegStatus/1001> ;
    a rdf:Property ;
    rdfs:isDefinedBy <http://rdaregistry.info/Elements/u/> ;
    rdfs:label "has form of notated movement"@en ;
    rdfs:subPropertyOf <http://rdaregistry.info/Elements/u/P60319> ;
    skos:definition "Relates a resource to a set of characters or symbols used to express movement content of a resource."@en .

<http://rdaregistry.info/Elements/u/P60321>
    reg:hasSubproperty <http://rdaregistry.info/Elements/e/P20064> ;
    reg:lexicalAlias <http://rdaregistry.info/Elements/u/formOfMusicalNotation.en> ;
    reg:name "formOfMusicalNotation"@en ;
    reg:status <http://metadataregistry.org/uri/RegStatus/1001> ;
    a rdf:Property ;
    rdfs:isDefinedBy <http://rdaregistry.info/Elements/u/> ;
    rdfs:label "has form of musical notation"@en ;
    rdfs:subPropertyOf <http://rdaregistry.info/Elements/u/P60319> ;
    skos:definition "Relates a resource to a set of characters or symbols used to express musical content of a resource."@en .

<http://rdaregistry.info/Elements/u/P60322>
    reg:hasSubproperty <http://rdaregistry.info/Elements/e/P20065> ;
    reg:lexicalAlias <http://rdaregistry.info/Elements/u/script.en> ;
    reg:name "script"@en ;
    reg:status <http://metadataregistry.org/uri/RegStatus/1001> ;
    a rdf:Property ;
    rdfs:isDefinedBy <http://rdaregistry.info/Elements/u/> ;
    rdfs:label "has script"@en ;
    rdfs:subPropertyOf <http://rdaregistry.info/Elements/u/P60319> ;
    skos:definition "Relates a resource to a set of characters or symbols used to express written language content of a resource."@en .

<http://rdaregistry.info/Elements/u/P60323>
    reg:hasSubproperty <http://rdaregistry.info/Elements/m/P30102> ;
    reg:lexicalAlias <http://rdaregistry.info/Elements/u/digitalRepresentationOfCartographicContent.en> ;
    reg:name "digitalRepresentationOfCartographicContent"@en ;
    reg:status <http://metadataregistry.org/uri/RegStatus/1001> ;
    a rdf:Property ;
    rdfs:isDefinedBy <http://rdaregistry.info/Elements/u/> ;
    rdfs:label "has digital representation of cartographic content"@en ;
    rdfs:subPropertyOf <http://rdaregistry.info/Elements/u/P60350> ;
    skos:definition "Relates a resource to a set of technical details relating to an encoding of geospatial information in a cartographic resource."@en .

<http://rdaregistry.info/Elements/u/P60324>
    reg:hasSubproperty <http://rdaregistry.info/Elements/a/P50040>, <http://rdaregistry.info/Elements/a/P50058>, <http://rdaregistry.info/Elements/a/P50107>, <http://rdaregistry.info/Elements/u/P60076>, <http://rdaregistry.info/Elements/u/P60524>, <http://rdaregistry.info/Elements/u/P60525>, <http://rdaregistry.info/Elements/u/P60526>, <http://rdaregistry.info/Elements/u/P60598>, <http://rdaregistry.info/Elements/u/P60599> ;
    reg:lexicalAlias <http://rdaregistry.info/Elements/u/dateAssociatedWithAgent.en> ;
    reg:name "dateAssociatedWithAgent"@en ;
    reg:status <http://metadataregistry.org/uri/RegStatus/1001> ;
    a rdf:Property ;
    rdfs:isDefinedBy <http://rdaregistry.info/Elements/u/> ;
    rdfs:label "has date associated with agent"@en ;
    skos:definition "Relates a resource to a significant date associated with the history of an agent, or the date or range of dates on which a conference, etc., was held, or a date with which an agent is otherwise associated."@en .

<http://rdaregistry.info/Elements/u/P60325>
    reg:hasSubproperty <http://rdaregistry.info/Elements/a/P50031>, <http://rdaregistry.info/Elements/a/P50057>, <http://rdaregistry.info/Elements/a/P50260>, <http://rdaregistry.info/Elements/u/P60064>, <http://rdaregistry.info/Elements/u/P60107> ;
    reg:lexicalAlias <http://rdaregistry.info/Elements/u/placeAssociatedWithAgent.en> ;
    reg:name "placeAssociatedWithAgent"@en ;
    reg:status <http://metadataregistry.org/uri/RegStatus/1001> ;
    a rdf:Property ;
    rdfs:isDefinedBy <http://rdaregistry.info/Elements/u/> ;
    rdfs:label "has place associated with agent"@en ;
    skos:definition "Relates a resource to a significant location associated with an agent, or a place where an agent resides or has resided or has some connection."@en .

<http://rdaregistry.info/Elements/u/P60326>
    reg:hasSubproperty <http://rdaregistry.info/Elements/m/P30104> ;
    reg:lexicalAlias <http://rdaregistry.info/Elements/u/videoFormat.en> ;
    reg:name "videoFormat"@en ;
    reg:status <http://metadataregistry.org/uri/RegStatus/1001> ;
    a rdf:Property ;
    rdfs:isDefinedBy <http://rdaregistry.info/Elements/u/> ;
    rdfs:label "has video format"@en ;
    rdfs:subPropertyOf <http://rdaregistry.info/Elements/u/P60352> ;
    skos:definition "Relates a resource to a standard, etc., used to encode the analog video content of a resource."@en .

<http://rdaregistry.info/Elements/u/P60327>
    reg:hasSubproperty <http://rdaregistry.info/Elements/m/P30105> ;
    reg:lexicalAlias <http://rdaregistry.info/Elements/u/statementOfResponsibilityRelatingToTitleProper.en> ;
    reg:name "statementOfResponsibilityRelatingToTitleProper"@en ;
    reg:status <http://metadataregistry.org/uri/RegStatus/1001> ;
    a rdf:Property ;
    rdfs:isDefinedBy <http://rdaregistry.info/Elements/u/> ;
    rdfs:label "has statement of responsibility relating to title proper"@en ;
    rdfs:subPropertyOf <http://rdaregistry.info/Elements/u/P60339> ;
    skos:definition "Relates a resource to a statement associated with a title proper of a resource that relates to an identification or function of agents responsible for the creation of, or contributing to a realization of, the intellectual or artistic content of a resource."@en .

<http://rdaregistry.info/Elements/u/P60328>
    reg:hasSubproperty <http://rdaregistry.info/Elements/m/P30106> ;
    reg:lexicalAlias <http://rdaregistry.info/Elements/u/seriesStatement.en> ;
    reg:name "seriesStatement"@en ;
    reg:status <http://metadataregistry.org/uri/RegStatus/1001> ;
    a rdf:Property ;
    rdfs:isDefinedBy <http://rdaregistry.info/Elements/u/> ;
    rdfs:label "has series statement"@en ;
    skos:definition "Relates a resource to a statement identifying a series to which a resource belongs and a numbering of a resource within the series."@en ;
    skos:scopeNote "A series statement may also include information identifying one or more subseries to which the resource being described belongs. A series statement sometimes includes statements of responsibility relating to a series or subseries."@en .

<http://rdaregistry.info/Elements/u/P60329>
    reg:hasSubproperty <http://rdaregistry.info/Elements/m/P30107> ;
    reg:lexicalAlias <http://rdaregistry.info/Elements/u/editionStatement.en> ;
    reg:name "editionStatement"@en ;
    reg:status <http://metadataregistry.org/uri/RegStatus/1001> ;
    a rdf:Property ;
    rdfs:isDefinedBy <http://rdaregistry.info/Elements/u/> ;
    rdfs:label "has edition statement"@en ;
    skos:definition "Relates a resource to a statement identifying an edition to which a resource belongs."@en .

<http://rdaregistry.info/Elements/u/P60330>
    reg:hasSubproperty <http://rdaregistry.info/Elements/m/P30108> ;
    reg:lexicalAlias <http://rdaregistry.info/Elements/u/distributionStatement.en> ;
    reg:name "distributionStatement"@en ;
    reg:status <http://metadataregistry.org/uri/RegStatus/1001> ;
    a rdf:Property ;
    rdfs:isDefinedBy <http://rdaregistry.info/Elements/u/> ;
    rdfs:label "has distribution statement"@en ;
    skos:definition "Relates a resource to a statement identifying a place or places of distribution, distributor or distributors, and date or dates of distribution of a resource in a published form."@en .

<http://rdaregistry.info/Elements/u/P60331>
    reg:hasSubproperty <http://rdaregistry.info/Elements/m/P30109> ;
    reg:lexicalAlias <http://rdaregistry.info/Elements/u/manufactureStatement.en> ;
    reg:name "manufactureStatement"@en ;
    reg:status <http://metadataregistry.org/uri/RegStatus/1001> ;
    a rdf:Property ;
    rdfs:isDefinedBy <http://rdaregistry.info/Elements/u/> ;
    rdfs:label "has manufacture statement"@en ;
    skos:definition "Relates a resource to a statement identifying a place or places of manufacture, manufacturer or manufacturers, and date or dates of manufacture of a resource in a published form."@en .

<http://rdaregistry.info/Elements/u/P60332>
    reg:hasSubproperty <http://rdaregistry.info/Elements/m/P30110> ;
    reg:lexicalAlias <http://rdaregistry.info/Elements/u/productionStatement.en> ;
    reg:name "productionStatement"@en ;
    reg:status <http://metadataregistry.org/uri/RegStatus/1001> ;
    a rdf:Property ;
    rdfs:isDefinedBy <http://rdaregistry.info/Elements/u/> ;
    rdfs:label "has production statement"@en ;
    skos:definition "Relates a resource to a statement identifying a place or places of production, producer or producers, and date or dates of production of a resource in an unpublished form."@en .

<http://rdaregistry.info/Elements/u/P60333>
    reg:hasSubproperty <http://rdaregistry.info/Elements/m/P30111> ;
    reg:lexicalAlias <http://rdaregistry.info/Elements/u/publicationStatement.en> ;
    reg:name "publicationStatement"@en ;
    reg:status <http://metadataregistry.org/uri/RegStatus/1001> ;
    a rdf:Property ;
    rdfs:isDefinedBy <http://rdaregistry.info/Elements/u/> ;
    rdfs:label "has publication statement"@en ;
    skos:definition "Relates a resource to a statement identifying a place or places of publication, publisher or publishers, and date or dates of publication of a resource."@en .

<http://rdaregistry.info/Elements/u/P60334>
    reg:hasSubproperty <http://rdaregistry.info/Elements/m/P30112> ;
    reg:lexicalAlias <http://rdaregistry.info/Elements/u/parallelStatementOfResponsibilityRelatingToNamedRevisionOfEdition.en> ;
    reg:name "parallelStatementOfResponsibilityRelatingToNamedRevisionOfEdition"@en ;
    reg:status <http://metadataregistry.org/uri/RegStatus/1001> ;
    a rdf:Property ;
    rdfs:isDefinedBy <http://rdaregistry.info/Elements/u/> ;
    rdfs:label "has parallel statement of responsibility relating to named revision of edition"@en ;
    skos:definition "Relates a resource to a statement of responsibility relating to a named revision of an edition in a language or script that differs from that recorded in a statement of responsibility relating to a named revision of an edition element."@en .

<http://rdaregistry.info/Elements/u/P60335>
    reg:hasSubproperty <http://rdaregistry.info/Elements/m/P30113> ;
    reg:lexicalAlias <http://rdaregistry.info/Elements/u/parallelStatementOfResponsibilityRelatingToSeries.en> ;
    reg:name "parallelStatementOfResponsibilityRelatingToSeries"@en ;
    reg:status <http://metadataregistry.org/uri/RegStatus/1001> ;
    a rdf:Property ;
    rdfs:isDefinedBy <http://rdaregistry.info/Elements/u/> ;
    rdfs:label "has parallel statement of responsibility relating to series"@en ;
    skos:definition "Relates a resource to a statement of responsibility relating to series in a language or script that differs from that recorded in a statement of responsibility relating to series element."@en .

<http://rdaregistry.info/Elements/u/P60336>
    reg:hasSubproperty <http://rdaregistry.info/Elements/m/P30114> ;
    reg:lexicalAlias <http://rdaregistry.info/Elements/u/parallelStatementOfResponsibilityRelatingToSubseries.en> ;
    reg:name "parallelStatementOfResponsibilityRelatingToSubseries"@en ;
    reg:status <http://metadataregistry.org/uri/RegStatus/1001> ;
    a rdf:Property ;
    rdfs:isDefinedBy <http://rdaregistry.info/Elements/u/> ;
    rdfs:label "has parallel statement of responsibility relating to subseries"@en ;
    skos:definition "Relates a resource to a statement of responsibility relating to subseries in a language or script that differs from that recorded in a statement of responsibility relating to subseries element."@en .

<http://rdaregistry.info/Elements/u/P60337>
    reg:hasSubproperty <http://rdaregistry.info/Elements/m/P30115> ;
    reg:lexicalAlias <http://rdaregistry.info/Elements/u/parallelStatementOfResponsibilityRelatingToEdition.en> ;
    reg:name "parallelStatementOfResponsibilityRelatingToEdition"@en ;
    reg:status <http://metadataregistry.org/uri/RegStatus/1001> ;
    a rdf:Property ;
    rdfs:isDefinedBy <http://rdaregistry.info/Elements/u/> ;
    rdfs:label "has parallel statement of responsibility relating to edition"@en ;
    skos:definition "Relates a resource to a statement of responsibility relating to an edition in a language or script that differs from that recorded in a statement of responsibility relating to an edition element."@en .

<http://rdaregistry.info/Elements/u/P60338>
    reg:hasSubproperty <http://rdaregistry.info/Elements/m/P30116> ;
    reg:lexicalAlias <http://rdaregistry.info/Elements/u/parallelStatementOfResponsibilityRelatingToTitleProper.en> ;
    reg:name "parallelStatementOfResponsibilityRelatingToTitleProper"@en ;
    reg:status <http://metadataregistry.org/uri/RegStatus/1001> ;
    a rdf:Property ;
    rdfs:isDefinedBy <http://rdaregistry.info/Elements/u/> ;
    rdfs:label "has parallel statement of responsibility relating to title proper"@en ;
    rdfs:subPropertyOf <http://rdaregistry.info/Elements/u/P60339> ;
    skos:definition "Relates a resource to a statement of responsibility relating to title proper in a language or script that differs from that recorded in a statement of responsibility relating to title proper element."@en .

<http://rdaregistry.info/Elements/u/P60339>
    reg:hasSubproperty <http://rdaregistry.info/Elements/m/P30117>, <http://rdaregistry.info/Elements/u/P60327>, <http://rdaregistry.info/Elements/u/P60338> ;
    reg:lexicalAlias <http://rdaregistry.info/Elements/u/statementOfResponsibility.en> ;
    reg:name "statementOfResponsibility"@en ;
    reg:status <http://metadataregistry.org/uri/RegStatus/1001> ;
    a rdf:Property ;
    rdfs:isDefinedBy <http://rdaregistry.info/Elements/u/> ;
    rdfs:label "has statement of responsibility"@en ;
    skos:definition "Relates a resource to a statement relating to anidentification or function of any agents responsible for the creation of, or contributing to a realization of, the intellectual or artistic content of a resource."@en .

<http://rdaregistry.info/Elements/u/P60340>
    reg:hasSubproperty <http://rdaregistry.info/Elements/m/P30118> ;
    reg:lexicalAlias <http://rdaregistry.info/Elements/u/statementOfResponsibilityRelatingToNamedRevisionOfEdition.en> ;
    reg:name "statementOfResponsibilityRelatingToNamedRevisionOfEdition"@en ;
    reg:status <http://metadataregistry.org/uri/RegStatus/1001> ;
    a rdf:Property ;
    rdfs:isDefinedBy <http://rdaregistry.info/Elements/u/> ;
    rdfs:label "has statement of responsibility relating to named revision of edition"@en ;
    skos:definition "Relates a resource to a statement relating to an identification of agents responsible for a named revision of an edition."@en .

<http://rdaregistry.info/Elements/u/P60341>
    reg:hasSubproperty <http://rdaregistry.info/Elements/m/P30119> ;
    reg:lexicalAlias <http://rdaregistry.info/Elements/u/statementOfResponsibilityRelatingToSeries.en> ;
    reg:name "statementOfResponsibilityRelatingToSeries"@en ;
    reg:status <http://metadataregistry.org/uri/RegStatus/1001> ;
    a rdf:Property ;
    rdfs:isDefinedBy <http://rdaregistry.info/Elements/u/> ;
    rdfs:label "has statement of responsibility relating to series"@en ;
    skos:definition "Relates a resource to a statement relating to an identification of agents responsible for a series."@en .

<http://rdaregistry.info/Elements/u/P60342>
    reg:hasSubproperty <http://rdaregistry.info/Elements/m/P30120> ;
    reg:lexicalAlias <http://rdaregistry.info/Elements/u/statementOfResponsibilityRelatingToSubseries.en> ;
    reg:name "statementOfResponsibilityRelatingToSubseries"@en ;
    reg:status <http://metadataregistry.org/uri/RegStatus/1001> ;
    a rdf:Property ;
    rdfs:isDefinedBy <http://rdaregistry.info/Elements/u/> ;
    rdfs:label "has statement of responsibility relating to subseries"@en ;
    skos:definition "Relates a resource to a statement relating to an identification of agents responsible for a subseries."@en .

<http://rdaregistry.info/Elements/u/P60343>
    reg:hasSubproperty <http://rdaregistry.info/Elements/m/P30121> ;
    reg:lexicalAlias <http://rdaregistry.info/Elements/u/statementOfResponsibilityRelatingToEdition.en> ;
    reg:name "statementOfResponsibilityRelatingToEdition"@en ;
    reg:status <http://metadataregistry.org/uri/RegStatus/1001> ;
    a rdf:Property ;
    rdfs:isDefinedBy <http://rdaregistry.info/Elements/u/> ;
    rdfs:label "has statement of responsibility relating to edition"@en ;
    skos:definition "Relates a resource to a statement relating to an identification of agents responsible for an edition being described but not to all editions."@en .

<http://rdaregistry.info/Elements/u/P60344>
    reg:hasSubproperty <http://rdaregistry.info/Elements/m/P30122> ;
    reg:lexicalAlias <http://rdaregistry.info/Elements/u/emulsionOnMicrofilmAndMicrofiche.en> ;
    reg:name "emulsionOnMicrofilmAndMicrofiche"@en ;
    reg:status <http://metadataregistry.org/uri/RegStatus/1001> ;
    a rdf:Property ;
    rdfs:isDefinedBy <http://rdaregistry.info/Elements/u/> ;
    rdfs:label "has emulsion on microfilm and microfiche"@en ;
    rdfs:subPropertyOf <http://rdaregistry.info/Elements/u/P60159> ;
    skos:definition "Relates a resource to a suspension of light-sensitive chemicals used as a coating on a microfilm or microfiche."@en .

<http://rdaregistry.info/Elements/u/P60345>
    reg:lexicalAlias <http://rdaregistry.info/Elements/u/longitudeAndLatitude.en> ;
    reg:name "longitudeAndLatitude"@en ;
    reg:status <http://metadataregistry.org/uri/RegStatus/1001> ;
    a rdf:Property ;
    rdfs:isDefinedBy <http://rdaregistry.info/Elements/u/> ;
    rdfs:label "has longitude and latitude"@en ;
    rdfs:subPropertyOf <http://rdaregistry.info/Elements/u/P60109> ;
    skos:definition "Relates a resource to a system for identifying the area covered by the cartographic content of a resource using longitude of the westernmost and easternmost boundaries and latitude of the northernmost and southernmost boundaries."@en .

<http://rdaregistry.info/Elements/u/P60346>
    reg:lexicalAlias <http://rdaregistry.info/Elements/u/rightAscensionAndDeclination.en> ;
    reg:name "rightAscensionAndDeclination"@en ;
    reg:status <http://metadataregistry.org/uri/RegStatus/1001> ;
    a rdf:Property ;
    rdfs:isDefinedBy <http://rdaregistry.info/Elements/u/> ;
    rdfs:label "has right ascension and declination"@en ;
    rdfs:subPropertyOf <http://rdaregistry.info/Elements/u/P60109> ;
    skos:definition "Relates a resource to a system for identifying the location of a celestial object in the sky covered by the cartographic content of a resource using angles of right ascension and declination."@en .

<http://rdaregistry.info/Elements/u/P60347>
    reg:lexicalAlias <http://rdaregistry.info/Elements/u/stringsOfCoordinatePairs.en> ;
    reg:name "stringsOfCoordinatePairs"@en ;
    reg:status <http://metadataregistry.org/uri/RegStatus/1001> ;
    a rdf:Property ;
    rdfs:isDefinedBy <http://rdaregistry.info/Elements/u/> ;
    rdfs:label "has strings of coordinate pairs"@en ;
    rdfs:subPropertyOf <http://rdaregistry.info/Elements/u/P60109> ;
    skos:definition "Relates a resource to a system for identifying the precise area covered by the cartographic content of a resource using coordinates for each vertex of a polygon."@en .

<http://rdaregistry.info/Elements/u/P60348>
    reg:lexicalAlias <http://rdaregistry.info/Elements/u/systemOfOrganization.en> ;
    reg:name "systemOfOrganization"@en ;
    reg:status <http://metadataregistry.org/uri/RegStatus/1001> ;
    a rdf:Property ;
    rdfs:isDefinedBy <http://rdaregistry.info/Elements/u/> ;
    rdfs:label "has system of organization"@en ;
    skos:definition "Relates a resource to a system of arranging materials in an archival resource or a collection."@en .

<http://rdaregistry.info/Elements/u/P60349>
    reg:hasSubproperty <http://rdaregistry.info/Elements/m/P30123> ;
    reg:lexicalAlias <http://rdaregistry.info/Elements/u/broadcastStandard.en> ;
    reg:name "broadcastStandard"@en ;
    reg:status <http://metadataregistry.org/uri/RegStatus/1001> ;
    a rdf:Property ;
    rdfs:isDefinedBy <http://rdaregistry.info/Elements/u/> ;
    rdfs:label "has broadcast standard"@en ;
    rdfs:subPropertyOf <http://rdaregistry.info/Elements/u/P60352> ;
    skos:definition "Relates a resource to a system used to format a video resource for television broadcast."@en .

<http://rdaregistry.info/Elements/u/P60350>
    reg:hasSubproperty <http://rdaregistry.info/Elements/m/P30124>, <http://rdaregistry.info/Elements/u/P60059>, <http://rdaregistry.info/Elements/u/P60093>, <http://rdaregistry.info/Elements/u/P60314>, <http://rdaregistry.info/Elements/u/P60323>, <http://rdaregistry.info/Elements/u/P60519>, <http://rdaregistry.info/Elements/u/P60551>, <http://rdaregistry.info/Elements/u/P60587> ;
    reg:lexicalAlias <http://rdaregistry.info/Elements/u/digitalFileCharacteristic.en> ;
    reg:name "digitalFileCharacteristic"@en ;
    reg:status <http://metadataregistry.org/uri/RegStatus/1001> ;
    a rdf:Property ;
    rdfs:isDefinedBy <http://rdaregistry.info/Elements/u/> ;
    rdfs:label "has digital file characteristic"@en ;
    skos:definition "Relates a resource to a technical specification relating to a digital encoding of text, image, audio, video, and other types of data in a resource."@en .

<http://rdaregistry.info/Elements/u/P60351>
    reg:hasSubproperty <http://rdaregistry.info/Elements/m/P30125>, <http://rdaregistry.info/Elements/u/P60481>, <http://rdaregistry.info/Elements/u/P60522>, <http://rdaregistry.info/Elements/u/P60532>, <http://rdaregistry.info/Elements/u/P60543>, <http://rdaregistry.info/Elements/u/P60552>, <http://rdaregistry.info/Elements/u/P60553>, <http://rdaregistry.info/Elements/u/P60586>, <http://rdaregistry.info/Elements/u/P60594> ;
    reg:lexicalAlias <http://rdaregistry.info/Elements/u/soundCharacteristic.en> ;
    reg:name "soundCharacteristic"@en ;
    reg:status <http://metadataregistry.org/uri/RegStatus/1001> ;
    a rdf:Property ;
    rdfs:isDefinedBy <http://rdaregistry.info/Elements/u/> ;
    rdfs:label "has sound characteristic"@en ;
    skos:definition "Relates a resource to a technical specification relating to an encoding of sound in a resource."@en .

<http://rdaregistry.info/Elements/u/P60352>
    reg:hasSubproperty <http://rdaregistry.info/Elements/m/P30126>, <http://rdaregistry.info/Elements/u/P60326>, <http://rdaregistry.info/Elements/u/P60349> ;
    reg:lexicalAlias <http://rdaregistry.info/Elements/u/videoCharacteristic.en> ;
    reg:name "videoCharacteristic"@en ;
    reg:status <http://metadataregistry.org/uri/RegStatus/1001> ;
    a rdf:Property ;
    rdfs:isDefinedBy <http://rdaregistry.info/Elements/u/> ;
    rdfs:label "has video characteristic"@en ;
    skos:definition "Relates a resource to a technical specification relating to an encoding of video images in a resource."@en .

<http://rdaregistry.info/Elements/u/P60353>
    reg:hasSubproperty <http://rdaregistry.info/Elements/m/P30127>, <http://rdaregistry.info/Elements/u/P60529>, <http://rdaregistry.info/Elements/u/P60585> ;
    reg:lexicalAlias <http://rdaregistry.info/Elements/u/projectionCharacteristicOfMotionPictureFilm.en> ;
    reg:name "projectionCharacteristicOfMotionPictureFilm"@en ;
    reg:status <http://metadataregistry.org/uri/RegStatus/1001> ;
    a rdf:Property ;
    rdfs:isDefinedBy <http://rdaregistry.info/Elements/u/> ;
    rdfs:label "has projection characteristic of motion picture film"@en ;
    skos:definition "Relates a resource to a technical specification relating to the projection of a motion picture film."@en .

<http://rdaregistry.info/Elements/u/P60354>
    reg:hasSubproperty <http://rdaregistry.info/Elements/e/P20066> ;
    reg:lexicalAlias <http://rdaregistry.info/Elements/u/adaptedAsATelevisionProgram.en> ;
    reg:name "adaptedAsATelevisionProgram"@en ;
    reg:status <http://metadataregistry.org/uri/RegStatus/1001> ;
    a rdf:Property ;
    rdfs:isDefinedBy <http://rdaregistry.info/Elements/u/> ;
    rdfs:label "is adapted as television program"@en ;
    rdfs:subPropertyOf <http://rdaregistry.info/Elements/u/P60260> ;
    owl:inverseOf <http://rdaregistry.info/Elements/u/P60230> ;
    skos:definition "Relates a resource to a television program based on a source resource."@en .

<http://rdaregistry.info/Elements/u/P60355>
    reg:hasSubproperty <http://rdaregistry.info/Elements/m/P30128> ;
    reg:lexicalAlias <http://rdaregistry.info/Elements/u/variantTitle.en> ;
    reg:name "variantTitle"@en ;
    reg:status <http://metadataregistry.org/uri/RegStatus/1001> ;
    a rdf:Property ;
    rdfs:isDefinedBy <http://rdaregistry.info/Elements/u/> ;
    rdfs:label "has variant title"@en ;
    rdfs:subPropertyOf <http://rdaregistry.info/Elements/u/P60369> ;
    skos:definition "Relates a resource to a title associated with a resource that differs from a title recorded as a preferred title, title proper, a parallel title proper, other title information, parallel other title information, earlier title proper, later title proper, key title, or abbreviated title."@en .

<http://rdaregistry.info/Elements/u/P60356>
    reg:hasSubproperty <http://rdaregistry.info/Elements/a/P50059> ;
    reg:lexicalAlias <http://rdaregistry.info/Elements/u/hereditaryTitle.en> ;
    reg:name "hereditaryTitle"@en ;
    reg:status <http://metadataregistry.org/uri/RegStatus/1001> ;
    a rdf:Property ;
    rdfs:isDefinedBy <http://rdaregistry.info/Elements/u/> ;
    rdfs:label "has hereditary title"@en ;
    skos:definition "Relates a resource to a title of nobility, etc., associated with an agent."@en .

<http://rdaregistry.info/Elements/u/P60357>
    reg:hasSubproperty <http://rdaregistry.info/Elements/m/P30129> ;
    reg:lexicalAlias <http://rdaregistry.info/Elements/u/laterTitleProper.en> ;
    reg:name "laterTitleProper"@en ;
    reg:status <http://metadataregistry.org/uri/RegStatus/1001> ;
    a rdf:Property ;
    rdfs:isDefinedBy <http://rdaregistry.info/Elements/u/> ;
    rdfs:label "has later title proper"@en ;
    rdfs:subPropertyOf <http://rdaregistry.info/Elements/u/P60369> ;
    skos:definition "Relates a resource to a title proper appearing on a later issue or part of a multipart monograph or serial that differs from that on the first or earliest issue or part."@en .

<http://rdaregistry.info/Elements/u/P60358>
    reg:hasSubproperty <http://rdaregistry.info/Elements/m/P30130> ;
    reg:lexicalAlias <http://rdaregistry.info/Elements/u/earlierTitleProper.en> ;
    reg:name "earlierTitleProper"@en ;
    reg:status <http://metadataregistry.org/uri/RegStatus/1001> ;
    a rdf:Property ;
    rdfs:isDefinedBy <http://rdaregistry.info/Elements/u/> ;
    rdfs:label "has earlier title proper"@en ;
    rdfs:subPropertyOf <http://rdaregistry.info/Elements/u/P60369> ;
    skos:definition "Relates a resource to a title proper appearing on an earlier iteration of an integrating resource that differs from that on a current iteration."@en .

<http://rdaregistry.info/Elements/u/P60359>
    reg:hasSubproperty <http://rdaregistry.info/Elements/m/P30131> ;
    reg:lexicalAlias <http://rdaregistry.info/Elements/u/abbreviatedTitle.en> ;
    reg:name "abbreviatedTitle"@en ;
    reg:status <http://metadataregistry.org/uri/RegStatus/1001> ;
    a rdf:Property ;
    rdfs:isDefinedBy <http://rdaregistry.info/Elements/u/> ;
    rdfs:label "has abbreviated title"@en ;
    rdfs:subPropertyOf <http://rdaregistry.info/Elements/u/P60369> ;
    skos:definition "Relates a resource to a title that has been abbreviated for purposes of indexing or identification."@en .

<http://rdaregistry.info/Elements/u/P60360>
    reg:hasSubproperty <http://rdaregistry.info/Elements/a/P50109> ;
    reg:lexicalAlias <http://rdaregistry.info/Elements/u/placeOfResidenceEtc.en> ;
    reg:name "placeOfResidenceEtc"@en ;
    reg:status <http://metadataregistry.org/uri/RegStatus/1001> ;
    a rdf:Property ;
    rdfs:isDefinedBy <http://rdaregistry.info/Elements/u/> ;
    rdfs:label "has place of residence, etc."@en ;
    skos:definition "Relates a resource to a town, city, province, state, or country in which an agent resides or has resided, or another significant place associated with an agent other than place of birth, place of death, or residence."@en ;
    skos:scopeNote "A place where an agent has worked or studied is included."@en .

<http://rdaregistry.info/Elements/u/P60361>
    reg:hasSubproperty <http://rdaregistry.info/Elements/e/P20067> ;
    reg:lexicalAlias <http://rdaregistry.info/Elements/u/adaptedAsAVideo.en> ;
    reg:name "adaptedAsAVideo"@en ;
    reg:status <http://metadataregistry.org/uri/RegStatus/1001> ;
    a rdf:Property ;
    rdfs:isDefinedBy <http://rdaregistry.info/Elements/u/> ;
    rdfs:label "is adapted as video"@en ;
    rdfs:subPropertyOf <http://rdaregistry.info/Elements/u/P60260> ;
    owl:inverseOf <http://rdaregistry.info/Elements/u/P60236> ;
    skos:definition "Relates a resource to a video based on a source resource."@en .

<http://rdaregistry.info/Elements/u/P60362>
    reg:hasSubproperty <http://rdaregistry.info/Elements/a/P50060> ;
    reg:lexicalAlias <http://rdaregistry.info/Elements/u/prominentMemberOfTheFamily.en> ;
    reg:name "prominentMemberOfAgent"@en ;
    reg:status <http://metadataregistry.org/uri/RegStatus/1001> ;
    a rdf:Property ;
    rdfs:isDefinedBy <http://rdaregistry.info/Elements/u/> ;
    rdfs:label "has prominent member of agent"@en ;
    skos:definition "Relates a resource to a well-known individual who is a member of an agent."@en .

<http://rdaregistry.info/Elements/u/P60363>
    reg:hasSubproperty <http://rdaregistry.info/Elements/a/P50110> ;
    reg:lexicalAlias <http://rdaregistry.info/Elements/u/titleOfAgent.en> ;
    reg:name "titleOfAgent"@en ;
    reg:status <http://metadataregistry.org/uri/RegStatus/1001> ;
    a rdf:Property ;
    rdfs:isDefinedBy <http://rdaregistry.info/Elements/u/> ;
    rdfs:label "has title of agent"@en ;
    skos:definition "Relates a resource to a word or phrase indicative of royalty, nobility, or ecclesiastical rank or office, a term of address for an agent of religious vocation, or another term indicative of rank, honour, or office."@en .

<http://rdaregistry.info/Elements/u/P60364>
    reg:hasSubproperty <http://rdaregistry.info/Elements/m/P30132> ;
    reg:lexicalAlias <http://rdaregistry.info/Elements/u/designationOfNamedRevisionOfEdition.en> ;
    reg:name "designationOfNamedRevisionOfEdition"@en ;
    reg:status <http://metadataregistry.org/uri/RegStatus/1001> ;
    a rdf:Property ;
    rdfs:isDefinedBy <http://rdaregistry.info/Elements/u/> ;
    rdfs:label "has designation of named revision of edition"@en ;
    skos:definition "Relates a resource to a word, character or group of words or characters, identifying a particular revision of a named edition."@en .

<http://rdaregistry.info/Elements/u/P60365>
    reg:hasSubproperty <http://rdaregistry.info/Elements/m/P30133> ;
    reg:lexicalAlias <http://rdaregistry.info/Elements/u/designationOfEdition.en> ;
    reg:name "designationOfEdition"@en ;
    reg:status <http://metadataregistry.org/uri/RegStatus/1001> ;
    a rdf:Property ;
    rdfs:isDefinedBy <http://rdaregistry.info/Elements/u/> ;
    rdfs:label "has designation of edition"@en ;
    skos:definition "Relates a resource to a word, character or group of words or characters, identifying an edition to which a resource belongs."@en .

<http://rdaregistry.info/Elements/u/P60366>
    reg:hasSubproperty <http://rdaregistry.info/Elements/p/P70001>, <http://rdaregistry.info/Elements/u/P60548> ;
    reg:lexicalAlias <http://rdaregistry.info/Elements/u/nameOfPlace.en> ;
    reg:name "nameOfPlace"@en ;
    reg:status <http://metadataregistry.org/uri/RegStatus/1001> ;
    a rdf:Property ;
    rdfs:isDefinedBy <http://rdaregistry.info/Elements/u/> ;
    rdfs:label "has name of place"@en ;
    skos:definition "Relates a resource to a word, character, or group of words or characters by which a place is known."@en .

<http://rdaregistry.info/Elements/u/P60367>
    reg:hasSubproperty <http://rdaregistry.info/Elements/u/P60588> ;
    reg:lexicalAlias <http://rdaregistry.info/Elements/u/titleOfResource.en> ;
    reg:name "titleOfResource"@en ;
    reg:status <http://metadataregistry.org/uri/RegStatus/1001> ;
    a rdf:Property ;
    rdfs:isDefinedBy <http://rdaregistry.info/Elements/u/> ;
    rdfs:label "has title of resource"@en ;
    skos:definition "Relates a resource to a word, character, or group of words or characters by which a resource is known."@en .

<http://rdaregistry.info/Elements/u/P60368>
    reg:hasSubproperty <http://rdaregistry.info/Elements/a/P50032>, <http://rdaregistry.info/Elements/a/P50061>, <http://rdaregistry.info/Elements/a/P50111>, <http://rdaregistry.info/Elements/u/P60119>, <http://rdaregistry.info/Elements/u/P60549> ;
    reg:lexicalAlias <http://rdaregistry.info/Elements/u/nameOfAgent.en> ;
    reg:name "nameOfAgent"@en ;
    reg:status <http://metadataregistry.org/uri/RegStatus/1001> ;
    a rdf:Property ;
    rdfs:isDefinedBy <http://rdaregistry.info/Elements/u/> ;
    rdfs:label "has name of agent"@en ;
    skos:definition "Relates a resource to a word, character, or group of words or characters by which an agent is known."@en .

<http://rdaregistry.info/Elements/u/P60369>
    reg:hasSubproperty <http://rdaregistry.info/Elements/m/P30134>, <http://rdaregistry.info/Elements/u/P60355>, <http://rdaregistry.info/Elements/u/P60357>, <http://rdaregistry.info/Elements/u/P60358>, <http://rdaregistry.info/Elements/u/P60359>, <http://rdaregistry.info/Elements/u/P60493>, <http://rdaregistry.info/Elements/u/P60507>, <http://rdaregistry.info/Elements/u/P60515>, <http://rdaregistry.info/Elements/u/P60589>, <http://rdaregistry.info/Elements/u/P60597> ;
    reg:lexicalAlias <http://rdaregistry.info/Elements/u/title.en> ;
    reg:name "title"@en ;
    reg:status <http://metadataregistry.org/uri/RegStatus/1001> ;
    a rdf:Property ;
    rdfs:isDefinedBy <http://rdaregistry.info/Elements/u/> ;
    rdfs:label "has title"@en ;
    skos:definition "Relates a resource to a word, character, or group of words or characters that names a resource or a resource embodied in it."@en .

<http://rdaregistry.info/Elements/u/P60370>
    reg:hasSubproperty <http://rdaregistry.info/Elements/a/P50033>, <http://rdaregistry.info/Elements/a/P50108>, <http://rdaregistry.info/Elements/a/P50239> ;
    reg:lexicalAlias <http://rdaregistry.info/Elements/u/otherDesignationAssociatedWithAgent.en> ;
    reg:name "otherDesignationAssociatedWithAgent"@en ;
    reg:status <http://metadataregistry.org/uri/RegStatus/1001> ;
    a rdf:Property ;
    rdfs:isDefinedBy <http://rdaregistry.info/Elements/u/> ;
    rdfs:label "has other designation associated with agent"@en ;
    skos:definition "Relates a resource to a word, phrase, or abbreviation indicating incorporation or legal status of an agent, or any term serving to differentiate a an agent from other agents, etc., or a term other than a title that is associated with an agents name."@en .

<http://rdaregistry.info/Elements/u/P60371>
    rdakit:seeAlso <http://rdaregistry.info/Elements/u/P60477> ;
    reg:hasSubproperty <http://rdaregistry.info/Elements/e/P20068> ;
    reg:lexicalAlias <http://rdaregistry.info/Elements/u/writerOfAddedLyrics.en> ;
    reg:name "writerOfAddedLyrics"@en ;
    reg:status <http://metadataregistry.org/uri/RegStatus/1001> ;
    a rdf:Property ;
    rdfs:isDefinedBy <http://rdaregistry.info/Elements/u/> ;
    rdfs:label "has writer of added lyrics"@en ;
    rdfs:subPropertyOf <http://rdaregistry.info/Elements/u/P60380> ;
    owl:inverseOf <http://rdaregistry.info/Elements/u/P60600> ;
    skos:definition "Relates a resource to a writer of words added to a musical resource."@en ;
    skos:scopeNote "Writing of lyrics in collaboration with a composer to form an original resource is excluded."@en .

<http://rdaregistry.info/Elements/u/P60372>
    reg:hasSubproperty <http://rdaregistry.info/Elements/e/P20069> ;
    reg:lexicalAlias <http://rdaregistry.info/Elements/u/summarizationOfContent.en> ;
    reg:name "summarizationOfContent"@en ;
    reg:status <http://metadataregistry.org/uri/RegStatus/1001> ;
    a rdf:Property ;
    rdfs:isDefinedBy <http://rdaregistry.info/Elements/u/> ;
    rdfs:label "has summarization of content"@en ;
    skos:definition "Relates a resource to an abstract, summary, synopsis, etc., of the content of a resource."@en .

<http://rdaregistry.info/Elements/u/P60373>
    reg:lexicalAlias <http://rdaregistry.info/Elements/u/appellee.en> ;
    reg:name "appellee"@en ;
    reg:status <http://metadataregistry.org/uri/RegStatus/1001> ;
    a rdf:Property ;
    rdfs:isDefinedBy <http://rdaregistry.info/Elements/u/> ;
    rdfs:label "has appellee"@en ;
    rdfs:subPropertyOf <http://rdaregistry.info/Elements/u/P60374> ;
    owl:inverseOf <http://rdaregistry.info/Elements/u/P60601> ;
    skos:definition "Relates a resource to an agent against whom an appeal is taken on a decision of a lower court recorded in a legal resource of a higher court."@en .

<http://rdaregistry.info/Elements/u/P60374>
    reg:hasSubproperty <http://rdaregistry.info/Elements/i/P40023>, <http://rdaregistry.info/Elements/m/P30079>, <http://rdaregistry.info/Elements/u/P60060>, <http://rdaregistry.info/Elements/u/P60061>, <http://rdaregistry.info/Elements/u/P60062>, <http://rdaregistry.info/Elements/u/P60065>, <http://rdaregistry.info/Elements/u/P60097>, <http://rdaregistry.info/Elements/u/P60157>, <http://rdaregistry.info/Elements/u/P60373>, <http://rdaregistry.info/Elements/u/P60375>, <http://rdaregistry.info/Elements/u/P60376>, <http://rdaregistry.info/Elements/u/P60406>, <http://rdaregistry.info/Elements/u/P60421>, <http://rdaregistry.info/Elements/u/P60441>, <http://rdaregistry.info/Elements/u/P60449>, <http://rdaregistry.info/Elements/u/P60450>, <http://rdaregistry.info/Elements/u/P60451>, <http://rdaregistry.info/Elements/u/P60455>, <http://rdaregistry.info/Elements/u/P60456>, <http://rdaregistry.info/Elements/u/P60457>, <http://rdaregistry.info/Elements/u/P60458>, <http://rdaregistry.info/Elements/u/P60459>, <http://rdaregistry.info/Elements/u/P60460>, <http://rdaregistry.info/Elements/u/P60461>, <http://rdaregistry.info/Elements/u/P60462>, <http://rdaregistry.info/Elements/u/P60464>, <http://rdaregistry.info/Elements/u/P60466>, <http://rdaregistry.info/Elements/u/P60467>, <http://rdaregistry.info/Elements/u/P60815>, <http://rdaregistry.info/Elements/u/P60834>, <http://rdaregistry.info/Elements/u/P60836>, <http://rdaregistry.info/Elements/u/P60849>, <http://rdaregistry.info/Elements/u/P60869>, <http://rdaregistry.info/Elements/u/P60871> ;
    reg:lexicalAlias <http://rdaregistry.info/Elements/u/otherAgentAssociatedWithResource.en> ;
    reg:name "otherAgentAssociatedWithResource"@en ;
    reg:status <http://metadataregistry.org/uri/RegStatus/1001> ;
    a rdf:Property ;
    rdfs:isDefinedBy <http://rdaregistry.info/Elements/u/> ;
    rdfs:label "has other agent associated with resource"@en ;
    owl:inverseOf <http://rdaregistry.info/Elements/u/P60602> ;
    skos:definition "Relates a resource to an agent other than a creator, custodian, owner, producer, publisher, distributor, or manufacturer associated with a resource."@en .

<http://rdaregistry.info/Elements/u/P60375>
    reg:lexicalAlias <http://rdaregistry.info/Elements/u/dedicator.en> ;
    reg:name "dedicator"@en ;
    reg:status <http://metadataregistry.org/uri/RegStatus/1001> ;
    a rdf:Property ;
    rdfs:isDefinedBy <http://rdaregistry.info/Elements/u/> ;
    rdfs:label "has dedicator"@en ;
    rdfs:subPropertyOf <http://rdaregistry.info/Elements/u/P60374> ;
    owl:inverseOf <http://rdaregistry.info/Elements/u/P60603> ;
    skos:definition "Relates a resource to an agent by whom a resource is dedicated."@en .

<http://rdaregistry.info/Elements/u/P60376>
    reg:hasSubproperty <http://rdaregistry.info/Elements/i/P40017>, <http://rdaregistry.info/Elements/u/P60066>, <http://rdaregistry.info/Elements/u/P60067> ;
    reg:lexicalAlias <http://rdaregistry.info/Elements/u/curator.en> ;
    reg:name "curator"@en ;
    reg:status <http://metadataregistry.org/uri/RegStatus/1001> ;
    a rdf:Property ;
    rdfs:isDefinedBy <http://rdaregistry.info/Elements/u/> ;
    rdfs:label "has curator"@en ;
    rdfs:subPropertyOf <http://rdaregistry.info/Elements/u/P60374> ;
    owl:inverseOf <http://rdaregistry.info/Elements/u/P60604> ;
    skos:definition "Relates a resource to an agent conceiving, aggregating, or organizing an exhibition, collection, or other resource."@en .

<http://rdaregistry.info/Elements/u/P60377>
    reg:hasSubproperty <http://rdaregistry.info/Elements/e/P20027> ;
    reg:lexicalAlias <http://rdaregistry.info/Elements/u/surveyor.en> ;
    reg:name "surveyor"@en ;
    reg:status <http://metadataregistry.org/uri/RegStatus/1001> ;
    a rdf:Property ;
    rdfs:isDefinedBy <http://rdaregistry.info/Elements/u/> ;
    rdfs:label "has surveyor"@en ;
    rdfs:subPropertyOf <http://rdaregistry.info/Elements/u/P60398> ;
    owl:inverseOf <http://rdaregistry.info/Elements/u/P60605> ;
    skos:definition "Relates a resource to an agent contributing to a cartographic resource by providing measurements or dimensional relationships for a geographic area represented."@en .

<http://rdaregistry.info/Elements/u/P60378>
    rdakit:seeAlso <http://rdaregistry.info/Elements/u/P60431> ;
    reg:hasSubproperty <http://rdaregistry.info/Elements/e/P20028> ;
    reg:lexicalAlias <http://rdaregistry.info/Elements/u/animator.en> ;
    reg:name "animator"@en ;
    reg:status <http://metadataregistry.org/uri/RegStatus/1001> ;
    a rdf:Property ;
    rdfs:isDefinedBy <http://rdaregistry.info/Elements/u/> ;
    rdfs:label "has animator"@en ;
    rdfs:subPropertyOf <http://rdaregistry.info/Elements/u/P60398> ;
    owl:inverseOf <http://rdaregistry.info/Elements/u/P60606> ;
    skos:definition "Relates a resource to an agent contributing to a moving image resource or computer program by giving apparent movement to inanimate objects or drawings."@en ;
    skos:scopeNote "Creation of the drawings that are animated is excluded."@en .

<http://rdaregistry.info/Elements/u/P60379>
    rdakit:seeAlso <http://rdaregistry.info/Elements/u/P60426> ;
    reg:hasSubproperty <http://rdaregistry.info/Elements/e/P20029> ;
    reg:lexicalAlias <http://rdaregistry.info/Elements/u/arrangerOfMusic.en> ;
    reg:name "arrangerOfMusic"@en ;
    reg:status <http://metadataregistry.org/uri/RegStatus/1001> ;
    a rdf:Property ;
    rdfs:isDefinedBy <http://rdaregistry.info/Elements/u/> ;
    rdfs:label "has arranger of music"@en ;
    rdfs:subPropertyOf <http://rdaregistry.info/Elements/u/P60398> ;
    owl:inverseOf <http://rdaregistry.info/Elements/u/P60607> ;
    skos:definition "Relates a resource to an agent contributing to a musical resource by rewriting a composition for a medium of performance different from that for which a resource was originally intended."@en ;
    skos:scopeNote "Modification of the resource for the same medium of performance, etc., keeping the musical substance of the original composition essentially unchanged, is included.  Substantial modification that results in the creation of a new musical resource is excluded."@en .

<http://rdaregistry.info/Elements/u/P60380>
    reg:hasSubproperty <http://rdaregistry.info/Elements/e/P20030>, <http://rdaregistry.info/Elements/u/P60371> ;
    reg:lexicalAlias <http://rdaregistry.info/Elements/u/writerOfAddedText.en> ;
    reg:name "writerOfAddedText"@en ;
    reg:status <http://metadataregistry.org/uri/RegStatus/1001> ;
    a rdf:Property ;
    rdfs:isDefinedBy <http://rdaregistry.info/Elements/u/> ;
    rdfs:label "has writer of added text"@en ;
    rdfs:subPropertyOf <http://rdaregistry.info/Elements/u/P60392> ;
    owl:inverseOf <http://rdaregistry.info/Elements/u/P60608> ;
    skos:definition "Relates a resource to an agent contributing to a primarily non-textual resource by providing text, such as writing captions for photographs or descriptions of maps."@en .

<http://rdaregistry.info/Elements/u/P60381>
    reg:hasSubproperty <http://rdaregistry.info/Elements/e/P20033> ;
    reg:lexicalAlias <http://rdaregistry.info/Elements/u/draftsman.en> ;
    reg:name "draftsman"@en ;
    reg:status <http://metadataregistry.org/uri/RegStatus/1001> ;
    a rdf:Property ;
    rdfs:isDefinedBy <http://rdaregistry.info/Elements/u/> ;
    rdfs:label "has draftsman"@en ;
    rdfs:subPropertyOf <http://rdaregistry.info/Elements/u/P60398> ;
    owl:inverseOf <http://rdaregistry.info/Elements/u/P60609> ;
    skos:definition "Relates a resource to an agent contributing to a resource by an architect, inventor, etc., by making detailed plans or drawings for buildings, ships, aircraft, machines, objects, etc."@en .

<http://rdaregistry.info/Elements/u/P60382>
    rdakit:seeAlso <http://rdaregistry.info/Elements/u/P60379> ;
    reg:hasSubproperty <http://rdaregistry.info/Elements/e/P20034> ;
    reg:lexicalAlias <http://rdaregistry.info/Elements/u/transcriber.en> ;
    reg:name "transcriber"@en ;
    reg:status <http://metadataregistry.org/uri/RegStatus/1001> ;
    a rdf:Property ;
    rdfs:isDefinedBy <http://rdaregistry.info/Elements/u/> ;
    rdfs:label "has transcriber"@en ;
    rdfs:subPropertyOf <http://rdaregistry.info/Elements/u/P60398> ;
    owl:inverseOf <http://rdaregistry.info/Elements/u/P60610> ;
    skos:definition "Relates a resource to an agent contributing to a resource by writing down or notating unwritten or unnotated content, or by changing it from one system of notation to another."@en ;
    skos:scopeNote "Transcription of a musical resource for a different instrument or performing group is excluded."@en .

<http://rdaregistry.info/Elements/u/P60383>
    reg:hasSubproperty <http://rdaregistry.info/Elements/e/P20035> ;
    reg:lexicalAlias <http://rdaregistry.info/Elements/u/musicalDirector.en> ;
    reg:name "musicalDirector"@en ;
    reg:status <http://metadataregistry.org/uri/RegStatus/1001> ;
    a rdf:Property ;
    rdfs:isDefinedBy <http://rdaregistry.info/Elements/u/> ;
    rdfs:label "has musical director"@en ;
    rdfs:subPropertyOf <http://rdaregistry.info/Elements/u/P60398> ;
    owl:inverseOf <http://rdaregistry.info/Elements/u/P60611> ;
    skos:definition "Relates a resource to an agent contributing to a resource by coordinating the activities of composers, sound editors, and sound mixers for a moving image production or for a musical or dramatic presentation or entertainment."@en .

<http://rdaregistry.info/Elements/u/P60384>
    reg:hasSubproperty <http://rdaregistry.info/Elements/e/P20036> ;
    reg:lexicalAlias <http://rdaregistry.info/Elements/u/costumeDesigner.en> ;
    reg:name "costumeDesigner"@en ;
    reg:status <http://metadataregistry.org/uri/RegStatus/1001> ;
    a rdf:Property ;
    rdfs:isDefinedBy <http://rdaregistry.info/Elements/u/> ;
    rdfs:label "has costume designer"@en ;
    rdfs:subPropertyOf <http://rdaregistry.info/Elements/u/P60398> ;
    owl:inverseOf <http://rdaregistry.info/Elements/u/P60612> ;
    skos:definition "Relates a resource to an agent contributing to a resource by designing costumes for a moving image production or for a musical or dramatic presentation or entertainment."@en .

<http://rdaregistry.info/Elements/u/P60385>
    reg:hasSubproperty <http://rdaregistry.info/Elements/e/P20037> ;
    reg:lexicalAlias <http://rdaregistry.info/Elements/u/translator.en> ;
    reg:name "translator"@en ;
    reg:status <http://metadataregistry.org/uri/RegStatus/1001> ;
    a rdf:Property ;
    rdfs:isDefinedBy <http://rdaregistry.info/Elements/u/> ;
    rdfs:label "has translator"@en ;
    rdfs:subPropertyOf <http://rdaregistry.info/Elements/u/P60398> ;
    owl:inverseOf <http://rdaregistry.info/Elements/u/P60613> ;
    skos:definition "Relates a resource to an agent contributing to an expression of a resource by expressing linguistic content of a resource in a language different from that of previous expressions of an original resource."@en ;
    skos:scopeNote "Translation of linguistic content between forms of the same language from different time periods is included."@en .

<http://rdaregistry.info/Elements/u/P60386>
    reg:hasSubproperty <http://rdaregistry.info/Elements/e/P20038> ;
    reg:lexicalAlias <http://rdaregistry.info/Elements/u/artDirector.en> ;
    reg:name "artDirector"@en ;
    reg:status <http://metadataregistry.org/uri/RegStatus/1001> ;
    a rdf:Property ;
    rdfs:isDefinedBy <http://rdaregistry.info/Elements/u/> ;
    rdfs:label "has art director"@en ;
    rdfs:subPropertyOf <http://rdaregistry.info/Elements/u/P60398> ;
    owl:inverseOf <http://rdaregistry.info/Elements/u/P60614> ;
    skos:definition "Relates a resource to an agent contributing to a resource by overseeing artists and craftspeople who build sets for moving image productions."@en .

<http://rdaregistry.info/Elements/u/P60387>
    reg:hasSubproperty <http://rdaregistry.info/Elements/e/P20039>, <http://rdaregistry.info/Elements/u/P60141>, <http://rdaregistry.info/Elements/u/P60142>, <http://rdaregistry.info/Elements/u/P60143>, <http://rdaregistry.info/Elements/u/P60144>, <http://rdaregistry.info/Elements/u/P60145>, <http://rdaregistry.info/Elements/u/P60146>, <http://rdaregistry.info/Elements/u/P60147>, <http://rdaregistry.info/Elements/u/P60148>, <http://rdaregistry.info/Elements/u/P60149>, <http://rdaregistry.info/Elements/u/P60150>, <http://rdaregistry.info/Elements/u/P60151>, <http://rdaregistry.info/Elements/u/P60153>, <http://rdaregistry.info/Elements/u/P60154>, <http://rdaregistry.info/Elements/u/P60155>, <http://rdaregistry.info/Elements/u/P60156> ;
    reg:lexicalAlias <http://rdaregistry.info/Elements/u/performer.en> ;
    reg:name "performer"@en ;
    reg:status <http://metadataregistry.org/uri/RegStatus/1001> ;
    a rdf:Property ;
    rdfs:isDefinedBy <http://rdaregistry.info/Elements/u/> ;
    rdfs:label "has performer"@en ;
    rdfs:subPropertyOf <http://rdaregistry.info/Elements/u/P60398> ;
    owl:inverseOf <http://rdaregistry.info/Elements/u/P60615> ;
    skos:definition "Relates a resource to an agent contributing to a resource by performing music, acting, dancing, speaking, etc., often in a musical or dramatic presentation, etc."@en .

<http://rdaregistry.info/Elements/u/P60388>
    reg:hasSubproperty <http://rdaregistry.info/Elements/e/P20040> ;
    reg:lexicalAlias <http://rdaregistry.info/Elements/u/courtReporter.en> ;
    reg:name "courtReporter"@en ;
    reg:status <http://metadataregistry.org/uri/RegStatus/1001> ;
    a rdf:Property ;
    rdfs:isDefinedBy <http://rdaregistry.info/Elements/u/> ;
    rdfs:label "has court reporter"@en ;
    rdfs:subPropertyOf <http://rdaregistry.info/Elements/u/P60398> ;
    owl:inverseOf <http://rdaregistry.info/Elements/u/P60616> ;
    skos:definition "Relates a resource to an agent contributing to a resource by preparing a court's opinions for publication."@en .

<http://rdaregistry.info/Elements/u/P60389>
    reg:hasSubproperty <http://rdaregistry.info/Elements/e/P20041> ;
    reg:lexicalAlias <http://rdaregistry.info/Elements/u/writerOfPreface.en> ;
    reg:name "writerOfPreface"@en ;
    reg:status <http://metadataregistry.org/uri/RegStatus/1001> ;
    a rdf:Property ;
    rdfs:isDefinedBy <http://rdaregistry.info/Elements/u/> ;
    rdfs:label "has writer of preface"@en ;
    rdfs:subPropertyOf <http://rdaregistry.info/Elements/u/P60392> ;
    owl:inverseOf <http://rdaregistry.info/Elements/u/P60617> ;
    skos:definition "Relates a resource to an agent contributing to a resource by providing a preface to an original resource."@en .

<http://rdaregistry.info/Elements/u/P60390>
    reg:hasSubproperty <http://rdaregistry.info/Elements/e/P20044> ;
    reg:lexicalAlias <http://rdaregistry.info/Elements/u/writerOfAddedCommentary.en> ;
    reg:name "writerOfAddedCommentary"@en ;
    reg:status <http://metadataregistry.org/uri/RegStatus/1001> ;
    a rdf:Property ;
    rdfs:isDefinedBy <http://rdaregistry.info/Elements/u/> ;
    rdfs:label "has writer of added commentary"@en ;
    rdfs:subPropertyOf <http://rdaregistry.info/Elements/u/P60392> ;
    owl:inverseOf <http://rdaregistry.info/Elements/u/P60618> ;
    skos:definition "Relates a resource to an agent contributing to a resource by providing an interpretation or critical explanation of an original resource."@en .

<http://rdaregistry.info/Elements/u/P60391>
    reg:hasSubproperty <http://rdaregistry.info/Elements/e/P20045> ;
    reg:lexicalAlias <http://rdaregistry.info/Elements/u/writerOfIntroduction.en> ;
    reg:name "writerOfIntroduction"@en ;
    reg:status <http://metadataregistry.org/uri/RegStatus/1001> ;
    a rdf:Property ;
    rdfs:isDefinedBy <http://rdaregistry.info/Elements/u/> ;
    rdfs:label "has writer of introduction"@en ;
    rdfs:subPropertyOf <http://rdaregistry.info/Elements/u/P60392> ;
    owl:inverseOf <http://rdaregistry.info/Elements/u/P60619> ;
    skos:definition "Relates a resource to an agent contributing to a resource by providing an introduction to an original resource."@en .

<http://rdaregistry.info/Elements/u/P60392>
    reg:hasSubproperty <http://rdaregistry.info/Elements/e/P20046>, <http://rdaregistry.info/Elements/u/P60380>, <http://rdaregistry.info/Elements/u/P60389>, <http://rdaregistry.info/Elements/u/P60390>, <http://rdaregistry.info/Elements/u/P60391> ;
    reg:lexicalAlias <http://rdaregistry.info/Elements/u/writerOfSupplementaryTextualContent.en> ;
    reg:name "writerOfSupplementaryTextualContent"@en ;
    reg:status <http://metadataregistry.org/uri/RegStatus/1001> ;
    a rdf:Property ;
    rdfs:isDefinedBy <http://rdaregistry.info/Elements/u/> ;
    rdfs:label "has writer of supplementary textual content"@en ;
    rdfs:subPropertyOf <http://rdaregistry.info/Elements/u/P60398> ;
    owl:inverseOf <http://rdaregistry.info/Elements/u/P60620> ;
    skos:definition "Relates a resource to an agent contributing to a resource by providing supplementary textual content (e.g., an appendix, an introduction, a preface) to an original resource."@en .

<http://rdaregistry.info/Elements/u/P60393>
    rdakit:seeAlso <http://rdaregistry.info/Elements/u/P60434> ;
    reg:hasSubproperty <http://rdaregistry.info/Elements/e/P20048> ;
    reg:lexicalAlias <http://rdaregistry.info/Elements/u/editor.en> ;
    reg:name "editor"@en ;
    reg:status <http://metadataregistry.org/uri/RegStatus/1001> ;
    a rdf:Property ;
    rdfs:isDefinedBy <http://rdaregistry.info/Elements/u/> ;
    rdfs:label "has editor"@en ;
    rdfs:subPropertyOf <http://rdaregistry.info/Elements/u/P60398> ;
    owl:inverseOf <http://rdaregistry.info/Elements/u/P60621> ;
    skos:definition "Relates a resource to an agent contributing to a resource by revising or clarifying the content, or by selecting and putting together resources, or parts of resources, by one or more creators."@en ;
    skos:scopeNote "Addition of an introduction, notes, or other critical matter, or preparing a resource for production, publication, or distribution is included. Major revision, adaptation, etc., that substantially changes the nature and content of the original resource, resulting in a new resource, is excluded."@en .

<http://rdaregistry.info/Elements/u/P60394>
    rdakit:seeAlso <http://rdaregistry.info/Elements/u/P60434> ;
    reg:hasSubproperty <http://rdaregistry.info/Elements/e/P20049> ;
    reg:lexicalAlias <http://rdaregistry.info/Elements/u/abridger.en> ;
    reg:name "abridger"@en ;
    reg:status <http://metadataregistry.org/uri/RegStatus/1001> ;
    a rdf:Property ;
    rdfs:isDefinedBy <http://rdaregistry.info/Elements/u/> ;
    rdfs:label "has abridger"@en ;
    rdfs:subPropertyOf <http://rdaregistry.info/Elements/u/P60398> ;
    owl:inverseOf <http://rdaregistry.info/Elements/u/P60622> ;
    skos:definition "Relates a resource to an agent contributing to a resource by shortening or condensing an original resource but leaving the nature and content substantially unchanged."@en ;
    skos:scopeNote "Substantial modification that results in the creation of a new resource is excluded."@en .

<http://rdaregistry.info/Elements/u/P60395>
    reg:hasSubproperty <http://rdaregistry.info/Elements/e/P20050> ;
    reg:lexicalAlias <http://rdaregistry.info/Elements/u/recordingEngineer.en> ;
    reg:name "recordingEngineer"@en ;
    reg:status <http://metadataregistry.org/uri/RegStatus/1001> ;
    a rdf:Property ;
    rdfs:isDefinedBy <http://rdaregistry.info/Elements/u/> ;
    rdfs:label "has recording engineer"@en ;
    rdfs:subPropertyOf <http://rdaregistry.info/Elements/u/P60398> ;
    owl:inverseOf <http://rdaregistry.info/Elements/u/P60623> ;
    skos:definition "Relates a resource to an agent contributing to a resource by supervising the technical aspects of a sound or video recording session."@en .

<http://rdaregistry.info/Elements/u/P60396>
    reg:hasSubproperty <http://rdaregistry.info/Elements/e/P20051>, <http://rdaregistry.info/Elements/u/P60750> ;
    reg:lexicalAlias <http://rdaregistry.info/Elements/u/illustrator.en> ;
    reg:name "illustrator"@en ;
    reg:status <http://metadataregistry.org/uri/RegStatus/1001> ;
    a rdf:Property ;
    rdfs:isDefinedBy <http://rdaregistry.info/Elements/u/> ;
    rdfs:label "has illustrator"@en ;
    rdfs:subPropertyOf <http://rdaregistry.info/Elements/u/P60398> ;
    owl:inverseOf <http://rdaregistry.info/Elements/u/P60624> ;
    skos:definition "Relates a resource to an agent contributing to a resource by supplementing a primary content with drawings, diagrams, photographs, etc."@en ;
    skos:scopeNote "Creation of content that is primarily artistic is excluded."@en .

<http://rdaregistry.info/Elements/u/P60397>
    reg:hasSubproperty <http://rdaregistry.info/Elements/e/P20052> ;
    reg:lexicalAlias <http://rdaregistry.info/Elements/u/recordist.en> ;
    reg:name "recordist"@en ;
    reg:status <http://metadataregistry.org/uri/RegStatus/1001> ;
    a rdf:Property ;
    rdfs:isDefinedBy <http://rdaregistry.info/Elements/u/> ;
    rdfs:label "has recordist"@en ;
    rdfs:subPropertyOf <http://rdaregistry.info/Elements/u/P60398> ;
    owl:inverseOf <http://rdaregistry.info/Elements/u/P60625> ;
    skos:definition "Relates a resource to an agent contributing to a resource by using a recording device to capture sound or video during a recording session, including field recordings of natural sounds, folkloric events, music, etc."@en .

<http://rdaregistry.info/Elements/u/P60398>
    reg:hasSubproperty <http://rdaregistry.info/Elements/e/P20053>, <http://rdaregistry.info/Elements/u/P60377>, <http://rdaregistry.info/Elements/u/P60378>, <http://rdaregistry.info/Elements/u/P60379>, <http://rdaregistry.info/Elements/u/P60381>, <http://rdaregistry.info/Elements/u/P60382>, <http://rdaregistry.info/Elements/u/P60383>, <http://rdaregistry.info/Elements/u/P60384>, <http://rdaregistry.info/Elements/u/P60385>, <http://rdaregistry.info/Elements/u/P60386>, <http://rdaregistry.info/Elements/u/P60387>, <http://rdaregistry.info/Elements/u/P60388>, <http://rdaregistry.info/Elements/u/P60392>, <http://rdaregistry.info/Elements/u/P60393>, <http://rdaregistry.info/Elements/u/P60394>, <http://rdaregistry.info/Elements/u/P60395>, <http://rdaregistry.info/Elements/u/P60396>, <http://rdaregistry.info/Elements/u/P60397>, <http://rdaregistry.info/Elements/u/P60399>, <http://rdaregistry.info/Elements/u/P60419>, <http://rdaregistry.info/Elements/u/P60422>, <http://rdaregistry.info/Elements/u/P60437>, <http://rdaregistry.info/Elements/u/P60446>, <http://rdaregistry.info/Elements/u/P60748>, <http://rdaregistry.info/Elements/u/P60749>, <http://rdaregistry.info/Elements/u/P60809>, <http://rdaregistry.info/Elements/u/P60811>, <http://rdaregistry.info/Elements/u/P60813>, <http://rdaregistry.info/Elements/u/P60824>, <http://rdaregistry.info/Elements/u/P60828>, <http://rdaregistry.info/Elements/u/P60838>, <http://rdaregistry.info/Elements/u/P60840>, <http://rdaregistry.info/Elements/u/P60851>, <http://rdaregistry.info/Elements/u/P60892>, <http://rdaregistry.info/Elements/u/P60894>, <http://rdaregistry.info/Elements/u/P60895>, <http://rdaregistry.info/Elements/u/P60896> ;
    reg:lexicalAlias <http://rdaregistry.info/Elements/u/contributor.en> ;
    reg:name "contributor"@en ;
    reg:status <http://metadataregistry.org/uri/RegStatus/1001> ;
    a rdf:Property ;
    rdfs:isDefinedBy <http://rdaregistry.info/Elements/u/> ;
    rdfs:label "has contributor"@en ;
    owl:inverseOf <http://rdaregistry.info/Elements/u/P60626> ;
    skos:definition "Relates a resource to an agent contributing to a resource."@en ;
    skos:scopeNote "Contributors include editors, translators, arrangers of music, performers, etc."@en .

<http://rdaregistry.info/Elements/u/P60399>
    reg:hasSubproperty <http://rdaregistry.info/Elements/e/P20031> ;
    reg:lexicalAlias <http://rdaregistry.info/Elements/u/stageDirector.en> ;
    reg:name "stageDirector"@en ;
    reg:status <http://metadataregistry.org/uri/RegStatus/1001> ;
    a rdf:Property ;
    rdfs:isDefinedBy <http://rdaregistry.info/Elements/u/> ;
    rdfs:label "has stage director"@en ;
    rdfs:subPropertyOf <http://rdaregistry.info/Elements/u/P60398> ;
    owl:inverseOf <http://rdaregistry.info/Elements/u/P60627> ;
    skos:definition "Relates a resource to an agent contributing to a stage resource through the general management and supervision of a performance."@en .

<http://rdaregistry.info/Elements/u/P60400>
    reg:hasSubproperty <http://rdaregistry.info/Elements/i/P40018>, <http://rdaregistry.info/Elements/u/P60068> ;
    reg:lexicalAlias <http://rdaregistry.info/Elements/u/currentOwner.en> ;
    reg:name "currentOwner"@en ;
    reg:status <http://metadataregistry.org/uri/RegStatus/1001> ;
    a rdf:Property ;
    rdfs:isDefinedBy <http://rdaregistry.info/Elements/u/> ;
    rdfs:label "has current owner"@en ;
    rdfs:subPropertyOf <http://rdaregistry.info/Elements/u/P60404> ;
    owl:inverseOf <http://rdaregistry.info/Elements/u/P60628> ;
    skos:definition "Relates a resource to an agent currently having legal possession of a resource."@en .

<http://rdaregistry.info/Elements/u/P60401>
    reg:hasSubproperty <http://rdaregistry.info/Elements/i/P40019>, <http://rdaregistry.info/Elements/u/P60091>, <http://rdaregistry.info/Elements/u/P60092> ;
    reg:lexicalAlias <http://rdaregistry.info/Elements/u/formerOwner.en> ;
    reg:name "formerOwner"@en ;
    reg:status <http://metadataregistry.org/uri/RegStatus/1001> ;
    a rdf:Property ;
    rdfs:isDefinedBy <http://rdaregistry.info/Elements/u/> ;
    rdfs:label "has former owner"@en ;
    rdfs:subPropertyOf <http://rdaregistry.info/Elements/u/P60404> ;
    owl:inverseOf <http://rdaregistry.info/Elements/u/P60630> ;
    skos:definition "Relates a resource to an agent formerly having legal possession of a resource."@en .

<http://rdaregistry.info/Elements/u/P60402>
    reg:hasSubproperty <http://rdaregistry.info/Elements/i/P40020> ;
    reg:lexicalAlias <http://rdaregistry.info/Elements/u/custodian.en> ;
    reg:name "custodian"@en ;
    reg:status <http://metadataregistry.org/uri/RegStatus/1001> ;
    a rdf:Property ;
    rdfs:isDefinedBy <http://rdaregistry.info/Elements/u/> ;
    rdfs:label "has custodian"@en ;
    owl:inverseOf <http://rdaregistry.info/Elements/u/P60631> ;
    skos:definition "Relates a resource to an agent having legal custody of a resource."@en .

<http://rdaregistry.info/Elements/u/P60404>
    reg:hasSubproperty <http://rdaregistry.info/Elements/i/P40021>, <http://rdaregistry.info/Elements/u/P60400>, <http://rdaregistry.info/Elements/u/P60401> ;
    reg:lexicalAlias <http://rdaregistry.info/Elements/u/owner.en> ;
    reg:name "owner"@en ;
    reg:status <http://metadataregistry.org/uri/RegStatus/1001> ;
    a rdf:Property ;
    rdfs:isDefinedBy <http://rdaregistry.info/Elements/u/> ;
    rdfs:label "has owner"@en ;
    owl:inverseOf <http://rdaregistry.info/Elements/u/P60632> ;
    skos:definition "Relates a resource to an agent having legal possession of a resource."@en .

<http://rdaregistry.info/Elements/u/P60406>
    reg:hasSubproperty <http://rdaregistry.info/Elements/i/P40022> ;
    reg:lexicalAlias <http://rdaregistry.info/Elements/u/honouree.en> ;
    reg:name "honouree"@en ;
    reg:status <http://metadataregistry.org/uri/RegStatus/1001> ;
    a rdf:Property ;
    rdfs:isDefinedBy <http://rdaregistry.info/Elements/u/> ;
    rdfs:label "has honouree"@en ;
    rdfs:subPropertyOf <http://rdaregistry.info/Elements/u/P60374> ;
    owl:inverseOf <http://rdaregistry.info/Elements/u/P60634> ;
    skos:altLabel "has honoree"@en ;
    skos:definition "Relates a resource to an agent honoured by a resource."@en .

<http://rdaregistry.info/Elements/u/P60407>
    reg:hasSubproperty <http://rdaregistry.info/Elements/m/P30067> ;
    reg:lexicalAlias <http://rdaregistry.info/Elements/u/broadcaster.en> ;
    reg:name "broadcaster"@en ;
    reg:status <http://metadataregistry.org/uri/RegStatus/1001> ;
    a rdf:Property ;
    rdfs:isDefinedBy <http://rdaregistry.info/Elements/u/> ;
    rdfs:label "has broadcaster"@en ;
    rdfs:subPropertyOf <http://rdaregistry.info/Elements/u/P60444> ;
    owl:inverseOf <http://rdaregistry.info/Elements/u/P60635> ;
    skos:definition "Relates a resource to an agent involved in broadcasting a resource to an audience via radio, television, webcast, etc."@en .

<http://rdaregistry.info/Elements/u/P60408>
    reg:hasSubproperty <http://rdaregistry.info/Elements/m/P30068> ;
    reg:lexicalAlias <http://rdaregistry.info/Elements/u/filmDistributor.en> ;
    reg:name "filmDistributor"@en ;
    reg:status <http://metadataregistry.org/uri/RegStatus/1001> ;
    a rdf:Property ;
    rdfs:isDefinedBy <http://rdaregistry.info/Elements/u/> ;
    rdfs:label "has film distributor"@en ;
    rdfs:subPropertyOf <http://rdaregistry.info/Elements/u/P60438> ;
    owl:inverseOf <http://rdaregistry.info/Elements/u/P60636> ;
    skos:definition "Relates a resource to an agent involved in distributing a moving image resource to theatres or other distribution channels."@en .

<http://rdaregistry.info/Elements/u/P60409>
    reg:hasSubproperty <http://rdaregistry.info/Elements/m/P30069> ;
    reg:lexicalAlias <http://rdaregistry.info/Elements/u/bookDesigner.en> ;
    reg:name "bookDesigner"@en ;
    reg:status <http://metadataregistry.org/uri/RegStatus/1001> ;
    a rdf:Property ;
    rdfs:isDefinedBy <http://rdaregistry.info/Elements/u/> ;
    rdfs:label "has book designer"@en ;
    rdfs:subPropertyOf <http://rdaregistry.info/Elements/u/P60443> ;
    owl:inverseOf <http://rdaregistry.info/Elements/u/P60637> ;
    skos:definition "Relates a resource to an agent involved in manufacturing a resource by being responsible for the entire graphic design of a book, including arrangement of type and illustration, choice of materials, and process used."@en .

<http://rdaregistry.info/Elements/u/P60410>
    reg:hasSubproperty <http://rdaregistry.info/Elements/m/P30070> ;
    reg:lexicalAlias <http://rdaregistry.info/Elements/u/engraver.en> ;
    reg:name "engraver"@en ;
    reg:status <http://metadataregistry.org/uri/RegStatus/1001> ;
    a rdf:Property ;
    rdfs:isDefinedBy <http://rdaregistry.info/Elements/u/> ;
    rdfs:label "has engraver"@en ;
    rdfs:subPropertyOf <http://rdaregistry.info/Elements/u/P60443> ;
    owl:inverseOf <http://rdaregistry.info/Elements/u/P60638> ;
    skos:definition "Relates a resource to an agent involved in manufacturing a resource by cutting letters, figures, etc., on a surface such as a wooden or metal plate used for printing."@en .

<http://rdaregistry.info/Elements/u/P60411>
    reg:hasSubproperty <http://rdaregistry.info/Elements/m/P30071> ;
    reg:lexicalAlias <http://rdaregistry.info/Elements/u/brailleEmbosser.en> ;
    reg:name "brailleEmbosser"@en ;
    reg:status <http://metadataregistry.org/uri/RegStatus/1001> ;
    a rdf:Property ;
    rdfs:isDefinedBy <http://rdaregistry.info/Elements/u/> ;
    rdfs:label "has braille embosser"@en ;
    rdfs:subPropertyOf <http://rdaregistry.info/Elements/u/P60443> ;
    owl:inverseOf <http://rdaregistry.info/Elements/u/P60639> ;
    skos:definition "Relates a resource to an agent involved in manufacturing a resource by embossing braille cells using a stylus, special embossing printer, or other device."@en .

<http://rdaregistry.info/Elements/u/P60412>
    reg:hasSubproperty <http://rdaregistry.info/Elements/m/P30072> ;
    reg:lexicalAlias <http://rdaregistry.info/Elements/u/printmaker.en> ;
    reg:name "printmaker"@en ;
    reg:status <http://metadataregistry.org/uri/RegStatus/1001> ;
    a rdf:Property ;
    rdfs:isDefinedBy <http://rdaregistry.info/Elements/u/> ;
    rdfs:label "has printmaker"@en ;
    rdfs:subPropertyOf <http://rdaregistry.info/Elements/u/P60443> ;
    owl:inverseOf <http://rdaregistry.info/Elements/u/P60640> ;
    skos:definition "Relates a resource to an agent involved in manufacturing a resource by making a relief, intaglio, or planographic printing surface."@en .

<http://rdaregistry.info/Elements/u/P60413>
    reg:hasSubproperty <http://rdaregistry.info/Elements/m/P30073> ;
    reg:lexicalAlias <http://rdaregistry.info/Elements/u/caster.en> ;
    reg:name "caster"@en ;
    reg:status <http://metadataregistry.org/uri/RegStatus/1001> ;
    a rdf:Property ;
    rdfs:isDefinedBy <http://rdaregistry.info/Elements/u/> ;
    rdfs:label "has caster"@en ;
    rdfs:subPropertyOf <http://rdaregistry.info/Elements/u/P60443> ;
    owl:inverseOf <http://rdaregistry.info/Elements/u/P60641> ;
    skos:definition "Relates a resource to an agent involved in manufacturing a resource by pouring a liquid or molten substance into a mold and leaving it to solidify to take the shape of the mold."@en .

<http://rdaregistry.info/Elements/u/P60414>
    reg:hasSubproperty <http://rdaregistry.info/Elements/m/P30074> ;
    reg:lexicalAlias <http://rdaregistry.info/Elements/u/lithographer.en> ;
    reg:name "lithographer"@en ;
    reg:status <http://metadataregistry.org/uri/RegStatus/1001> ;
    a rdf:Property ;
    rdfs:isDefinedBy <http://rdaregistry.info/Elements/u/> ;
    rdfs:label "has lithographer"@en ;
    rdfs:subPropertyOf <http://rdaregistry.info/Elements/u/P60443> ;
    owl:inverseOf <http://rdaregistry.info/Elements/u/P60642> ;
    skos:definition "Relates a resource to an agent involved in manufacturing a resource by preparing a stone or plate for lithographic printing."@en ;
    skos:scopeNote "A lithographer includes a graphic artist creating a design directly on the surface from which printing will be done."@en .

<http://rdaregistry.info/Elements/u/P60415>
    reg:hasSubproperty <http://rdaregistry.info/Elements/m/P30075> ;
    reg:lexicalAlias <http://rdaregistry.info/Elements/u/platemaker.en> ;
    reg:name "platemaker"@en ;
    reg:status <http://metadataregistry.org/uri/RegStatus/1001> ;
    a rdf:Property ;
    rdfs:isDefinedBy <http://rdaregistry.info/Elements/u/> ;
    rdfs:label "has platemaker"@en ;
    rdfs:subPropertyOf <http://rdaregistry.info/Elements/u/P60443> ;
    owl:inverseOf <http://rdaregistry.info/Elements/u/P60643> ;
    skos:definition "Relates a resource to an agent involved in manufacturing a resource by preparing plates used in the production of printed images or text."@en .

<http://rdaregistry.info/Elements/u/P60416>
    reg:hasSubproperty <http://rdaregistry.info/Elements/m/P30076> ;
    reg:lexicalAlias <http://rdaregistry.info/Elements/u/etcher.en> ;
    reg:name "etcher"@en ;
    reg:status <http://metadataregistry.org/uri/RegStatus/1001> ;
    a rdf:Property ;
    rdfs:isDefinedBy <http://rdaregistry.info/Elements/u/> ;
    rdfs:label "has etcher"@en ;
    rdfs:subPropertyOf <http://rdaregistry.info/Elements/u/P60443> ;
    owl:inverseOf <http://rdaregistry.info/Elements/u/P60644> ;
    skos:definition "Relates a resource to an agent involved in manufacturing a resource by subjecting metal, glass, or some other surface used for printing, to acid or another corrosive substance."@en .

<http://rdaregistry.info/Elements/u/P60417>
    reg:hasSubproperty <http://rdaregistry.info/Elements/m/P30077> ;
    reg:lexicalAlias <http://rdaregistry.info/Elements/u/collotyper.en> ;
    reg:name "collotyper"@en ;
    reg:status <http://metadataregistry.org/uri/RegStatus/1001> ;
    a rdf:Property ;
    rdfs:isDefinedBy <http://rdaregistry.info/Elements/u/> ;
    rdfs:label "has collotyper"@en ;
    rdfs:subPropertyOf <http://rdaregistry.info/Elements/u/P60443> ;
    owl:inverseOf <http://rdaregistry.info/Elements/u/P60645> ;
    skos:definition "Relates a resource to an agent involved in manufacturing a resource using a photomechanical process for making prints directly from a hardened film of gelatin or other colloid that has ink-receptive and ink-repellent surfaces."@en .

<http://rdaregistry.info/Elements/u/P60418>
    reg:hasSubproperty <http://rdaregistry.info/Elements/m/P30078> ;
    reg:lexicalAlias <http://rdaregistry.info/Elements/u/printer.en> ;
    reg:name "printer"@en ;
    reg:status <http://metadataregistry.org/uri/RegStatus/1001> ;
    a rdf:Property ;
    rdfs:isDefinedBy <http://rdaregistry.info/Elements/u/> ;
    rdfs:label "has printer"@en ;
    rdfs:subPropertyOf <http://rdaregistry.info/Elements/u/P60443> ;
    owl:inverseOf <http://rdaregistry.info/Elements/u/P60646> ;
    skos:definition "Relates a resource to an agent involved in manufacturing a resource of printed text, notated music, etc., from type or plates, such as a book, newspaper, magazine, broadside, score, etc."@en .

<http://rdaregistry.info/Elements/u/P60419>
    reg:hasSubproperty <http://rdaregistry.info/Elements/e/P20054> ;
    reg:lexicalAlias <http://rdaregistry.info/Elements/u/presenter.en> ;
    reg:name "presenter"@en ;
    reg:status <http://metadataregistry.org/uri/RegStatus/1001> ;
    a rdf:Property ;
    rdfs:isDefinedBy <http://rdaregistry.info/Elements/u/> ;
    rdfs:label "has presenter"@en ;
    rdfs:subPropertyOf <http://rdaregistry.info/Elements/u/P60398> ;
    owl:inverseOf <http://rdaregistry.info/Elements/u/P60647> ;
    skos:definition "Relates a resource to an agent mentioned in an \"X presents\" credit for moving image materials and who is probably associated with production, finance, or distribution in some way."@en .

<http://rdaregistry.info/Elements/u/P60420>
    reg:lexicalAlias <http://rdaregistry.info/Elements/u/degreeSupervisor.en> ;
    reg:name "degreeSupervisor"@en ;
    reg:status <http://metadataregistry.org/uri/RegStatus/1001> ;
    a rdf:Property ;
    rdfs:isDefinedBy <http://rdaregistry.info/Elements/u/> ;
    rdfs:label "has degree supervisor"@en ;
    rdfs:subPropertyOf <http://rdaregistry.info/Elements/u/P60447> ;
    owl:inverseOf <http://rdaregistry.info/Elements/u/P60649> ;
    skos:definition "Relates a resource to an agent, such as an advisor or supervisor of thesis or dissertation research, overseeing either an academic degree or thesis."@en .

<http://rdaregistry.info/Elements/u/P60421>
    reg:hasSubproperty <http://rdaregistry.info/Elements/i/P40012> ;
    reg:lexicalAlias <http://rdaregistry.info/Elements/u/illuminator.en> ;
    reg:name "illuminator"@en ;
    reg:status <http://metadataregistry.org/uri/RegStatus/1001> ;
    a rdf:Property ;
    rdfs:isDefinedBy <http://rdaregistry.info/Elements/u/> ;
    rdfs:label "has illuminator"@en ;
    rdfs:subPropertyOf <http://rdaregistry.info/Elements/u/P60374> ;
    owl:inverseOf <http://rdaregistry.info/Elements/u/P60650> ;
    skos:definition "Relates a resource to an agent providing decoration to a specific resource using precious metals or color, often with elaborate designs and motifs."@en .

<http://rdaregistry.info/Elements/u/P60422>
    rdakit:seeAlso <http://rdaregistry.info/Elements/u/P60663> ;
    reg:hasSubproperty <http://rdaregistry.info/Elements/e/P20055> ;
    reg:lexicalAlias <http://rdaregistry.info/Elements/u/editorOfMovingImageResource.en> ;
    reg:name "editorOfMovingImageResource"@en ;
    reg:status <http://metadataregistry.org/uri/RegStatus/1001> ;
    a rdf:Property ;
    rdfs:isDefinedBy <http://rdaregistry.info/Elements/u/> ;
    rdfs:label "has editor of moving image work"@en ;
    rdfs:subPropertyOf <http://rdaregistry.info/Elements/u/P60398> ;
    owl:inverseOf <http://rdaregistry.info/Elements/u/P60651> ;
    skos:definition "Relates a resource to an agent responsible for assembling, arranging, and trimming film, video, or other moving image formats, including both visual and audio aspects."@en .

<http://rdaregistry.info/Elements/u/P60423>
    reg:lexicalAlias <http://rdaregistry.info/Elements/u/programmer.en> ;
    reg:name "programmer"@en ;
    reg:status <http://metadataregistry.org/uri/RegStatus/1001> ;
    a rdf:Property ;
    rdfs:isDefinedBy <http://rdaregistry.info/Elements/u/> ;
    rdfs:label "has programmer"@en ;
    rdfs:subPropertyOf <http://rdaregistry.info/Elements/u/P60447> ;
    owl:inverseOf <http://rdaregistry.info/Elements/u/P60652> ;
    skos:definition "Relates a resource to an agent responsible for creating a computer program."@en .

<http://rdaregistry.info/Elements/u/P60424>
    reg:lexicalAlias <http://rdaregistry.info/Elements/u/designer.en> ;
    reg:name "designer"@en ;
    reg:status <http://metadataregistry.org/uri/RegStatus/1001> ;
    a rdf:Property ;
    rdfs:isDefinedBy <http://rdaregistry.info/Elements/u/> ;
    rdfs:label "has designer"@en ;
    rdfs:subPropertyOf <http://rdaregistry.info/Elements/u/P60447> ;
    owl:inverseOf <http://rdaregistry.info/Elements/u/P60653> ;
    skos:definition "Relates a resource to an agent responsible for creating a design for an object."@en .

<http://rdaregistry.info/Elements/u/P60425>
    reg:hasSubproperty <http://rdaregistry.info/Elements/e/P20042> ;
    reg:lexicalAlias <http://rdaregistry.info/Elements/u/cartographer.en> ;
    reg:name "cartographer"@en ;
    reg:status <http://metadataregistry.org/uri/RegStatus/1001> ;
    a rdf:Property ;
    rdfs:isDefinedBy <http://rdaregistry.info/Elements/u/> ;
    rdfs:label "has cartographer"@en ;
    rdfs:subPropertyOf <http://rdaregistry.info/Elements/u/P60447> ;
    owl:inverseOf <http://rdaregistry.info/Elements/u/P60654> ;
    skos:definition "Relates a resource to an agent responsible for creating a map, atlas, globe, or other cartographic resource."@en .

<http://rdaregistry.info/Elements/u/P60426>
    reg:hasSubproperty <http://rdaregistry.info/Elements/e/P20026> ;
    reg:lexicalAlias <http://rdaregistry.info/Elements/u/composer.en> ;
    reg:name "composer"@en ;
    reg:status <http://metadataregistry.org/uri/RegStatus/1001> ;
    a rdf:Property ;
    rdfs:isDefinedBy <http://rdaregistry.info/Elements/u/> ;
    rdfs:label "has composer"@en ;
    rdfs:subPropertyOf <http://rdaregistry.info/Elements/u/P60447> ;
    owl:inverseOf <http://rdaregistry.info/Elements/u/P60655> ;
    skos:definition "Relates a resource to an agent responsible for creating a musical resource."@en ;
    skos:scopeNote "Adaptation of another musical resource to form a distinct alteration, paraphrasing a resource or creating a resource in the general style of another composer, or creating a resource that is based on the music of another composer, is included."@en .

<http://rdaregistry.info/Elements/u/P60427>
    reg:lexicalAlias <http://rdaregistry.info/Elements/u/inventor.en> ;
    reg:name "inventor"@en ;
    reg:status <http://metadataregistry.org/uri/RegStatus/1001> ;
    a rdf:Property ;
    rdfs:isDefinedBy <http://rdaregistry.info/Elements/u/> ;
    rdfs:label "has inventor"@en ;
    rdfs:subPropertyOf <http://rdaregistry.info/Elements/u/P60447> ;
    owl:inverseOf <http://rdaregistry.info/Elements/u/P60656> ;
    skos:definition "Relates a resource to an agent responsible for creating a new device or process."@en .

<http://rdaregistry.info/Elements/u/P60428>
    rdakit:seeAlso <http://rdaregistry.info/Elements/u/P60393> ;
    reg:lexicalAlias <http://rdaregistry.info/Elements/u/compiler.en> ;
    reg:name "compiler"@en ;
    reg:status <http://metadataregistry.org/uri/RegStatus/1001> ;
    a rdf:Property ;
    rdfs:isDefinedBy <http://rdaregistry.info/Elements/u/> ;
    rdfs:label "has compiler"@en ;
    rdfs:subPropertyOf <http://rdaregistry.info/Elements/u/P60447> ;
    owl:inverseOf <http://rdaregistry.info/Elements/u/P60657> ;
    skos:definition "Relates a resource to an agent responsible for creating a new resource such as a bibliography or a directory by selecting, arranging, aggregating, and editing data, information, etc."@en ;
    skos:scopeNote "Revising or clarifying the content, or selecting and putting together resources or parts of resources, by one or more creators is excluded"@en .

<http://rdaregistry.info/Elements/u/P60429>
    reg:hasSubproperty <http://rdaregistry.info/Elements/e/P20288> ;
    reg:lexicalAlias <http://rdaregistry.info/Elements/u/photographer.en> ;
    reg:name "photographer"@en ;
    reg:status <http://metadataregistry.org/uri/RegStatus/1001> ;
    a rdf:Property ;
    rdfs:isDefinedBy <http://rdaregistry.info/Elements/u/> ;
    rdfs:label "has photographer"@en ;
    rdfs:subPropertyOf <http://rdaregistry.info/Elements/u/P60447> ;
    owl:inverseOf <http://rdaregistry.info/Elements/u/P60658> ;
    skos:definition "Relates a resource to an agent responsible for creating a photographic resource."@en .

<http://rdaregistry.info/Elements/u/P60430>
    reg:hasSubproperty <http://rdaregistry.info/Elements/e/P20032> ;
    reg:lexicalAlias <http://rdaregistry.info/Elements/u/interviewer.en> ;
    reg:name "interviewer"@en ;
    reg:status <http://metadataregistry.org/uri/RegStatus/1001> ;
    a rdf:Property ;
    rdfs:isDefinedBy <http://rdaregistry.info/Elements/u/> ;
    rdfs:label "has interviewer"@en ;
    rdfs:subPropertyOf <http://rdaregistry.info/Elements/u/P60447> ;
    owl:inverseOf <http://rdaregistry.info/Elements/u/P60659> ;
    skos:definition "Relates a resource to an agent responsible for creating a resource by acting as an interviewer, reporter, pollster, or some other information gathering agent."@en .

<http://rdaregistry.info/Elements/u/P60431>
    reg:hasSubproperty <http://rdaregistry.info/Elements/u/P60475>, <http://rdaregistry.info/Elements/u/P60752>, <http://rdaregistry.info/Elements/u/P60753> ;
    reg:lexicalAlias <http://rdaregistry.info/Elements/u/artist.en> ;
    reg:name "artist"@en ;
    reg:status <http://metadataregistry.org/uri/RegStatus/1001> ;
    a rdf:Property ;
    rdfs:isDefinedBy <http://rdaregistry.info/Elements/u/> ;
    rdfs:label "has artist"@en ;
    rdfs:subPropertyOf <http://rdaregistry.info/Elements/u/P60447> ;
    owl:inverseOf <http://rdaregistry.info/Elements/u/P60660> ;
    skos:definition "Relates a resource to an agent responsible for creating a resource by conceiving, and often implementing, an original graphic design, drawing, painting, etc."@en .

<http://rdaregistry.info/Elements/u/P60432>
    reg:hasSubproperty <http://rdaregistry.info/Elements/e/P20047> ;
    reg:lexicalAlias <http://rdaregistry.info/Elements/u/interviewee.en> ;
    reg:name "interviewee"@en ;
    reg:status <http://metadataregistry.org/uri/RegStatus/1001> ;
    a rdf:Property ;
    rdfs:isDefinedBy <http://rdaregistry.info/Elements/u/> ;
    rdfs:label "has interviewee"@en ;
    rdfs:subPropertyOf <http://rdaregistry.info/Elements/u/P60447> ;
    owl:inverseOf <http://rdaregistry.info/Elements/u/P60661> ;
    skos:definition "Relates a resource to an agent responsible for creating a resource by responding to an interviewer, usually a reporter, pollster, or some other information gathering agent."@en .

<http://rdaregistry.info/Elements/u/P60433>
    reg:hasSubproperty <http://rdaregistry.info/Elements/e/P20043> ;
    reg:lexicalAlias <http://rdaregistry.info/Elements/u/choreographer.en> ;
    reg:name "choreographer"@en ;
    reg:status <http://metadataregistry.org/uri/RegStatus/1001> ;
    a rdf:Property ;
    rdfs:isDefinedBy <http://rdaregistry.info/Elements/u/> ;
    rdfs:label "has choreographer"@en ;
    rdfs:subPropertyOf <http://rdaregistry.info/Elements/u/P60447> ;
    owl:inverseOf <http://rdaregistry.info/Elements/u/P60662> ;
    skos:definition "Relates a resource to an agent responsible for creating a resource of movement."@en .

<http://rdaregistry.info/Elements/u/P60434>
    reg:hasSubproperty <http://rdaregistry.info/Elements/u/P60476>, <http://rdaregistry.info/Elements/u/P60477>, <http://rdaregistry.info/Elements/u/P60478>, <http://rdaregistry.info/Elements/u/P60751> ;
    reg:lexicalAlias <http://rdaregistry.info/Elements/u/author.en> ;
    reg:name "author"@en ;
    reg:status <http://metadataregistry.org/uri/RegStatus/1001> ;
    a rdf:Property ;
    rdfs:isDefinedBy <http://rdaregistry.info/Elements/u/> ;
    rdfs:label "has author"@en ;
    rdfs:subPropertyOf <http://rdaregistry.info/Elements/u/P60447> ;
    owl:inverseOf <http://rdaregistry.info/Elements/u/P60663> ;
    skos:definition "Relates a resource to an agent responsible for creating a resource that is primarily textual in content, regardless of media type or genre."@en .

<http://rdaregistry.info/Elements/u/P60435>
    reg:hasSubproperty <http://rdaregistry.info/Elements/u/P60473> ;
    reg:lexicalAlias <http://rdaregistry.info/Elements/u/architect.en> ;
    reg:name "architect"@en ;
    reg:status <http://metadataregistry.org/uri/RegStatus/1001> ;
    a rdf:Property ;
    rdfs:isDefinedBy <http://rdaregistry.info/Elements/u/> ;
    rdfs:label "has architect"@en ;
    rdfs:subPropertyOf <http://rdaregistry.info/Elements/u/P60447> ;
    owl:inverseOf <http://rdaregistry.info/Elements/u/P60664> ;
    skos:definition "Relates a resource to an agent responsible for creating an architectural design, including a pictorial representation intended to show how a building, etc., will look when completed."@en .

<http://rdaregistry.info/Elements/u/P60436>
    reg:lexicalAlias <http://rdaregistry.info/Elements/u/filmmaker.en> ;
    reg:name "filmmaker"@en ;
    reg:status <http://metadataregistry.org/uri/RegStatus/1001> ;
    a rdf:Property ;
    rdfs:isDefinedBy <http://rdaregistry.info/Elements/u/> ;
    rdfs:label "has filmmaker"@en ;
    rdfs:subPropertyOf <http://rdaregistry.info/Elements/u/P60447> ;
    owl:inverseOf <http://rdaregistry.info/Elements/u/P60665> ;
    skos:definition "Relates a resource to an agent responsible for creating an independent or personal film."@en .

<http://rdaregistry.info/Elements/u/P60437>
    reg:hasSubproperty <http://rdaregistry.info/Elements/e/P20056> ;
    reg:lexicalAlias <http://rdaregistry.info/Elements/u/productionDesigner.en> ;
    reg:name "productionDesigner"@en ;
    reg:status <http://metadataregistry.org/uri/RegStatus/1001> ;
    a rdf:Property ;
    rdfs:isDefinedBy <http://rdaregistry.info/Elements/u/> ;
    rdfs:label "has production designer"@en ;
    rdfs:subPropertyOf <http://rdaregistry.info/Elements/u/P60398> ;
    owl:inverseOf <http://rdaregistry.info/Elements/u/P60666> ;
    skos:definition "Relates a resource to an agent responsible for designing the overall visual appearance of a moving image production."@en .

<http://rdaregistry.info/Elements/u/P60438>
    reg:hasSubproperty <http://rdaregistry.info/Elements/m/P30080>, <http://rdaregistry.info/Elements/u/P60408> ;
    reg:lexicalAlias <http://rdaregistry.info/Elements/u/distributor.en> ;
    reg:name "distributor"@en ;
    reg:status <http://metadataregistry.org/uri/RegStatus/1001> ;
    a rdf:Property ;
    rdfs:isDefinedBy <http://rdaregistry.info/Elements/u/> ;
    rdfs:label "has distributor"@en ;
    owl:inverseOf <http://rdaregistry.info/Elements/u/P60667> ;
    skos:definition "Relates a resource to an agent responsible for distributing a resource."@en .

<http://rdaregistry.info/Elements/u/P60440>
    reg:hasSubproperty <http://rdaregistry.info/Elements/m/P30081> ;
    reg:lexicalAlias <http://rdaregistry.info/Elements/u/producerOfUnpublishedResource.en> ;
    reg:name "producerOfUnpublishedResource"@en ;
    reg:status <http://metadataregistry.org/uri/RegStatus/1001> ;
    a rdf:Property ;
    rdfs:isDefinedBy <http://rdaregistry.info/Elements/u/> ;
    rdfs:label "has producer of unpublished resource"@en ;
    skos:definition "Relates a resource to an agent responsible for inscribing, fabricating, constructing, etc., a resource in an unpublished form."@en .

<http://rdaregistry.info/Elements/u/P60441>
    reg:hasSubproperty <http://rdaregistry.info/Elements/u/P60169>, <http://rdaregistry.info/Elements/u/P60170>, <http://rdaregistry.info/Elements/u/P60171>, <http://rdaregistry.info/Elements/u/P60889> ;
    reg:lexicalAlias <http://rdaregistry.info/Elements/u/producer.en> ;
    reg:name "producer"@en ;
    reg:status <http://metadataregistry.org/uri/RegStatus/1001> ;
    a rdf:Property ;
    rdfs:isDefinedBy <http://rdaregistry.info/Elements/u/> ;
    rdfs:label "has producer"@en ;
    rdfs:subPropertyOf <http://rdaregistry.info/Elements/u/P60374> ;
    owl:inverseOf <http://rdaregistry.info/Elements/u/P60668> ;
    skos:definition "Relates a resource to an agent responsible for most of the business aspects of a production for screen, sound recording, television, webcast, etc. a producer is generally responsible for fund raising, managing the production, hiring key personnel, arranging for distributors, etc."@en .

<http://rdaregistry.info/Elements/u/P60442>
    reg:status <http://metadataregistry.org/uri/RegStatus/1008> ;
    rdfs:isDefinedBy <http://rdaregistry.info/Elements/u/> .

<http://rdaregistry.info/Elements/u/P60443>
    reg:hasSubproperty <http://rdaregistry.info/Elements/m/P30082>, <http://rdaregistry.info/Elements/u/P60409>, <http://rdaregistry.info/Elements/u/P60410>, <http://rdaregistry.info/Elements/u/P60411>, <http://rdaregistry.info/Elements/u/P60412>, <http://rdaregistry.info/Elements/u/P60413>, <http://rdaregistry.info/Elements/u/P60414>, <http://rdaregistry.info/Elements/u/P60415>, <http://rdaregistry.info/Elements/u/P60416>, <http://rdaregistry.info/Elements/u/P60417>, <http://rdaregistry.info/Elements/u/P60418>, <http://rdaregistry.info/Elements/u/P60746> ;
    reg:lexicalAlias <http://rdaregistry.info/Elements/u/manufacturer.en> ;
    reg:name "manufacturer"@en ;
    reg:status <http://metadataregistry.org/uri/RegStatus/1001> ;
    a rdf:Property ;
    rdfs:isDefinedBy <http://rdaregistry.info/Elements/u/> ;
    rdfs:label "has manufacturer"@en ;
    owl:inverseOf <http://rdaregistry.info/Elements/u/P60669> ;
    skos:definition "Relates a resource to an agent responsible for printing, duplicating, casting, etc., a resource in a published form."@en .

<http://rdaregistry.info/Elements/u/P60444>
    reg:hasSubproperty <http://rdaregistry.info/Elements/m/P30083>, <http://rdaregistry.info/Elements/u/P60407> ;
    reg:lexicalAlias <http://rdaregistry.info/Elements/u/publisher.en> ;
    reg:name "publisher"@en ;
    reg:status <http://metadataregistry.org/uri/RegStatus/1001> ;
    a rdf:Property ;
    rdfs:isDefinedBy <http://rdaregistry.info/Elements/u/> ;
    rdfs:label "has publisher"@en ;
    owl:inverseOf <http://rdaregistry.info/Elements/u/P60670> ;
    skos:definition "Relates a resource to an agent responsible for publishing, releasing, or issuing a resource."@en .

<http://rdaregistry.info/Elements/u/P60446>
    reg:hasSubproperty <http://rdaregistry.info/Elements/e/P20058> ;
    reg:lexicalAlias <http://rdaregistry.info/Elements/u/minuteTaker.en> ;
    reg:name "minuteTaker"@en ;
    reg:status <http://metadataregistry.org/uri/RegStatus/1001> ;
    a rdf:Property ;
    rdfs:isDefinedBy <http://rdaregistry.info/Elements/u/> ;
    rdfs:label "has minute taker"@en ;
    rdfs:subPropertyOf <http://rdaregistry.info/Elements/u/P60398> ;
    owl:inverseOf <http://rdaregistry.info/Elements/u/P60671> ;
    skos:definition "Relates a resource to an agent responsible for recording the minutes of a meeting."@en .

<http://rdaregistry.info/Elements/u/P60447>
    reg:hasSubproperty <http://rdaregistry.info/Elements/u/P60045>, <http://rdaregistry.info/Elements/u/P60096>, <http://rdaregistry.info/Elements/u/P60420>, <http://rdaregistry.info/Elements/u/P60423>, <http://rdaregistry.info/Elements/u/P60424>, <http://rdaregistry.info/Elements/u/P60425>, <http://rdaregistry.info/Elements/u/P60426>, <http://rdaregistry.info/Elements/u/P60427>, <http://rdaregistry.info/Elements/u/P60428>, <http://rdaregistry.info/Elements/u/P60429>, <http://rdaregistry.info/Elements/u/P60430>, <http://rdaregistry.info/Elements/u/P60431>, <http://rdaregistry.info/Elements/u/P60432>, <http://rdaregistry.info/Elements/u/P60433>, <http://rdaregistry.info/Elements/u/P60434>, <http://rdaregistry.info/Elements/u/P60435>, <http://rdaregistry.info/Elements/u/P60436>, <http://rdaregistry.info/Elements/u/P60463>, <http://rdaregistry.info/Elements/u/P60465>, <http://rdaregistry.info/Elements/u/P60826>, <http://rdaregistry.info/Elements/u/P60891> ;
    reg:lexicalAlias <http://rdaregistry.info/Elements/u/creator.en> ;
    reg:name "creator"@en ;
    reg:status <http://metadataregistry.org/uri/RegStatus/1001> ;
    a rdf:Property ;
    rdfs:isDefinedBy <http://rdaregistry.info/Elements/u/> ;
    rdfs:label "has creator"@en ;
    owl:inverseOf <http://rdaregistry.info/Elements/u/P60672> ;
    skos:definition "Relates a resource to an agent responsible for the creation of a resource"@en ;
    skos:scopeNote "Creators include agents who are jointly responsible for the creation of a resource either performing the same role, such as in a collaboration between two writers, or performing different roles, such as in a collaboration between a composer and a lyricist."@en .

<http://rdaregistry.info/Elements/u/P60449>
    reg:hasSubproperty <http://rdaregistry.info/Elements/u/P60084>, <http://rdaregistry.info/Elements/u/P60085>, <http://rdaregistry.info/Elements/u/P60086> ;
    reg:lexicalAlias <http://rdaregistry.info/Elements/u/director.en> ;
    reg:name "director"@en ;
    reg:status <http://metadataregistry.org/uri/RegStatus/1001> ;
    a rdf:Property ;
    rdfs:isDefinedBy <http://rdaregistry.info/Elements/u/> ;
    rdfs:label "has director"@en ;
    rdfs:subPropertyOf <http://rdaregistry.info/Elements/u/P60374> ;
    owl:inverseOf <http://rdaregistry.info/Elements/u/P60452> ;
    skos:definition "Relates a resource to an agent responsible for the general management and supervision of a filmed performance, a radio or television program, etc."@en .

<http://rdaregistry.info/Elements/u/P60450>
    reg:hasSubproperty <http://rdaregistry.info/Elements/e/P20289>, <http://rdaregistry.info/Elements/i/P40024> ;
    reg:lexicalAlias <http://rdaregistry.info/Elements/u/restorationist.en> ;
    reg:name "restorationist"@en ;
    reg:status <http://metadataregistry.org/uri/RegStatus/1001> ;
    a rdf:Property ;
    rdfs:isDefinedBy <http://rdaregistry.info/Elements/u/> ;
    rdfs:label "has restorationist"@en ;
    rdfs:subPropertyOf <http://rdaregistry.info/Elements/u/P60374> ;
    owl:inverseOf <http://rdaregistry.info/Elements/u/P60674> ;
    skos:definition "Relates a resource to an agent responsible for the set of technical, editorial, and intellectual procedures aimed at compensating for the degradation of a resource by bringing it back to a state as close as possible to its original condition."@en .

<http://rdaregistry.info/Elements/u/P60451>
    reg:lexicalAlias <http://rdaregistry.info/Elements/u/sponsoringBody.en> ;
    reg:name "sponsoringBody"@en ;
    reg:status <http://metadataregistry.org/uri/RegStatus/1001> ;
    a rdf:Property ;
    rdfs:isDefinedBy <http://rdaregistry.info/Elements/u/> ;
    rdfs:label "has sponsoring body"@en ;
    rdfs:subPropertyOf <http://rdaregistry.info/Elements/u/P60374> ;
    owl:inverseOf <http://rdaregistry.info/Elements/u/P60675> ;
    skos:definition "Relates a resource to an agent sponsoring some aspect of a resource, such as funding research or sponsoring an event."@en .

<http://rdaregistry.info/Elements/u/P60452>
    reg:hasSubproperty <http://rdaregistry.info/Elements/u/P60009>, <http://rdaregistry.info/Elements/u/P60010>, <http://rdaregistry.info/Elements/u/P60011> ;
    reg:lexicalAlias <http://rdaregistry.info/Elements/u/directorOfPhotography.en> ;
    reg:name "directorOfPhotography"@en ;
    reg:status <http://metadataregistry.org/uri/RegStatus/1001> ;
    a rdf:Property ;
    rdfs:isDefinedBy <http://rdaregistry.info/Elements/u/> ;
    rdfs:label "has director of photography"@en ;
    rdfs:subPropertyOf <http://rdaregistry.info/Elements/u/P60374> ;
    owl:inverseOf <http://rdaregistry.info/Elements/u/P60678> ;
    skos:definition "Relates a resource to an agent that captures images, either electronically or on film or video stock, and often selects and arranges lighting. a director of photography for a movie is also called a chief cinematographer."@en .

<http://rdaregistry.info/Elements/u/P60454>
    reg:hasSubproperty <http://rdaregistry.info/Elements/u/P60633>, <http://rdaregistry.info/Elements/u/P60737>, <http://rdaregistry.info/Elements/u/P60853>, <http://rdaregistry.info/Elements/u/P60854>, <http://rdaregistry.info/Elements/u/P60855>, <http://rdaregistry.info/Elements/u/P60856>, <http://rdaregistry.info/Elements/u/P60861>, <http://rdaregistry.info/Elements/u/P60862>, <http://rdaregistry.info/Elements/u/P60863> ;
    reg:lexicalAlias <http://rdaregistry.info/Elements/u/relatedAgent.en> ;
    reg:name "relatedAgent"@en ;
    reg:status <http://metadataregistry.org/uri/RegStatus/1001> ;
    a rdf:Property ;
    rdfs:isDefinedBy <http://rdaregistry.info/Elements/u/> ;
    rdfs:label "has related agent"@en ;
    skos:definition "Relates an agent to an agent that is associated with an agent being described."@en .

<http://rdaregistry.info/Elements/u/P60455>
    reg:hasSubproperty <http://rdaregistry.info/Elements/i/P40025> ;
    reg:lexicalAlias <http://rdaregistry.info/Elements/u/dedicatee.en> ;
    reg:name "dedicatee"@en ;
    reg:status <http://metadataregistry.org/uri/RegStatus/1001> ;
    a rdf:Property ;
    rdfs:isDefinedBy <http://rdaregistry.info/Elements/u/> ;
    rdfs:label "has dedicatee"@en ;
    rdfs:subPropertyOf <http://rdaregistry.info/Elements/u/P60374> ;
    owl:inverseOf <http://rdaregistry.info/Elements/u/P60689> ;
    skos:definition "Relates a resource to an agent to whom a resource is dedicated."@en .

<http://rdaregistry.info/Elements/u/P60456>
    reg:lexicalAlias <http://rdaregistry.info/Elements/u/addressee.en> ;
    reg:name "addressee"@en ;
    reg:status <http://metadataregistry.org/uri/RegStatus/1001> ;
    a rdf:Property ;
    rdfs:isDefinedBy <http://rdaregistry.info/Elements/u/> ;
    rdfs:label "has addressee"@en ;
    rdfs:subPropertyOf <http://rdaregistry.info/Elements/u/P60374> ;
    owl:inverseOf <http://rdaregistry.info/Elements/u/P60690> ;
    skos:definition "Relates a resource to an agent to whom a resource or part of a resource is addressed."@en .

<http://rdaregistry.info/Elements/u/P60457>
    reg:lexicalAlias <http://rdaregistry.info/Elements/u/appellant.en> ;
    reg:name "appellant"@en ;
    reg:status <http://metadataregistry.org/uri/RegStatus/1001> ;
    a rdf:Property ;
    rdfs:isDefinedBy <http://rdaregistry.info/Elements/u/> ;
    rdfs:label "has appellant"@en ;
    rdfs:subPropertyOf <http://rdaregistry.info/Elements/u/P60374> ;
    owl:inverseOf <http://rdaregistry.info/Elements/u/P60691> ;
    skos:definition "Relates a resource to an agent who appeals a decision of a lower court recorded in a legal resource of a higher court."@en .

<http://rdaregistry.info/Elements/u/P60458>
    reg:hasSubproperty <http://rdaregistry.info/Elements/i/P40013> ;
    reg:lexicalAlias <http://rdaregistry.info/Elements/u/binder.en> ;
    reg:name "binder"@en ;
    reg:status <http://metadataregistry.org/uri/RegStatus/1001> ;
    a rdf:Property ;
    rdfs:isDefinedBy <http://rdaregistry.info/Elements/u/> ;
    rdfs:label "has binder"@en ;
    rdfs:subPropertyOf <http://rdaregistry.info/Elements/u/P60374> ;
    owl:inverseOf <http://rdaregistry.info/Elements/u/P60692> ;
    skos:definition "Relates a resource to an agent who binds a resource."@en .

<http://rdaregistry.info/Elements/u/P60459>
    reg:lexicalAlias <http://rdaregistry.info/Elements/u/plaintiff.en> ;
    reg:name "plaintiff"@en ;
    reg:status <http://metadataregistry.org/uri/RegStatus/1001> ;
    a rdf:Property ;
    rdfs:isDefinedBy <http://rdaregistry.info/Elements/u/> ;
    rdfs:label "has plaintiff"@en ;
    rdfs:subPropertyOf <http://rdaregistry.info/Elements/u/P60374> ;
    owl:inverseOf <http://rdaregistry.info/Elements/u/P60693> ;
    skos:definition "Relates a resource to an agent who brings a suit in a civil proceeding."@en .

<http://rdaregistry.info/Elements/u/P60460>
    reg:hasSubproperty <http://rdaregistry.info/Elements/i/P40014> ;
    reg:lexicalAlias <http://rdaregistry.info/Elements/u/inscriber.en> ;
    reg:name "inscriber"@en ;
    reg:status <http://metadataregistry.org/uri/RegStatus/1001> ;
    a rdf:Property ;
    rdfs:isDefinedBy <http://rdaregistry.info/Elements/u/> ;
    rdfs:label "has inscriber"@en ;
    rdfs:subPropertyOf <http://rdaregistry.info/Elements/u/P60374> ;
    owl:inverseOf <http://rdaregistry.info/Elements/u/P60695> ;
    skos:definition "Relates a resource to an agent who has written a statement of dedication or gift on a resource."@en .

<http://rdaregistry.info/Elements/u/P60461>
    reg:lexicalAlias <http://rdaregistry.info/Elements/u/judge.en> ;
    reg:name "judge"@en ;
    reg:status <http://metadataregistry.org/uri/RegStatus/1001> ;
    a rdf:Property ;
    rdfs:isDefinedBy <http://rdaregistry.info/Elements/u/> ;
    rdfs:label "has judge"@en ;
    rdfs:subPropertyOf <http://rdaregistry.info/Elements/u/P60374> ;
    owl:inverseOf <http://rdaregistry.info/Elements/u/P60696> ;
    skos:definition "Relates a resource to an agent who hears and decides on legal matters in court."@en .

<http://rdaregistry.info/Elements/u/P60462>
    reg:hasSubproperty <http://rdaregistry.info/Elements/w/P10285>, <http://rdaregistry.info/Elements/w/P10286> ;
    reg:lexicalAlias <http://rdaregistry.info/Elements/u/defendant.en> ;
    reg:name "defendant"@en ;
    reg:status <http://metadataregistry.org/uri/RegStatus/1001> ;
    a rdf:Property ;
    rdfs:isDefinedBy <http://rdaregistry.info/Elements/u/> ;
    rdfs:label "has defendant"@en ;
    rdfs:subPropertyOf <http://rdaregistry.info/Elements/u/P60374> ;
    owl:inverseOf <http://rdaregistry.info/Elements/u/P60698> ;
    skos:definition "Relates a resource to an agent who is accused in a criminal proceeding or sued in a civil proceeding."@en .

<http://rdaregistry.info/Elements/u/P60463>
    reg:lexicalAlias <http://rdaregistry.info/Elements/u/praeses.en> ;
    reg:name "praeses"@en ;
    reg:status <http://metadataregistry.org/uri/RegStatus/1001> ;
    a rdf:Property ;
    rdfs:isDefinedBy <http://rdaregistry.info/Elements/u/> ;
    rdfs:label "has praeses"@en ;
    rdfs:subPropertyOf <http://rdaregistry.info/Elements/u/P60447> ;
    owl:inverseOf <http://rdaregistry.info/Elements/u/P60699> ;
    skos:definition "Relates a resource to an agent who is a faculty moderator of an academic disputation, normally proposing a thesis and participating in an ensuing disputation."@en .

<http://rdaregistry.info/Elements/u/P60464>
    reg:hasSubproperty <http://rdaregistry.info/Elements/i/P40015> ;
    reg:lexicalAlias <http://rdaregistry.info/Elements/u/annotator.en> ;
    reg:name "annotator"@en ;
    reg:status <http://metadataregistry.org/uri/RegStatus/1001> ;
    a rdf:Property ;
    rdfs:isDefinedBy <http://rdaregistry.info/Elements/u/> ;
    rdfs:label "has annotator"@en ;
    rdfs:subPropertyOf <http://rdaregistry.info/Elements/u/P60374> ;
    owl:inverseOf <http://rdaregistry.info/Elements/u/P60700> ;
    skos:definition "Relates a resource to an agent who makes manuscript annotations on a resource."@en .

<http://rdaregistry.info/Elements/u/P60465>
    reg:lexicalAlias <http://rdaregistry.info/Elements/u/consultant.en> ;
    reg:name "consultant"@en ;
    reg:status <http://metadataregistry.org/uri/RegStatus/1001> ;
    a rdf:Property ;
    rdfs:isDefinedBy <http://rdaregistry.info/Elements/u/> ;
    rdfs:label "has consultant"@en ;
    rdfs:subPropertyOf <http://rdaregistry.info/Elements/u/P60447> ;
    owl:inverseOf <http://rdaregistry.info/Elements/u/P60701> ;
    skos:definition "Relates a resource to an agent who provides consultation services, and often makes recommendations, for another agent that is represented as a creator of a resource."@en .

<http://rdaregistry.info/Elements/u/P60466>
    reg:hasSubproperty <http://rdaregistry.info/Elements/i/P40016> ;
    reg:lexicalAlias <http://rdaregistry.info/Elements/u/autographer.en> ;
    reg:name "autographer"@en ;
    reg:status <http://metadataregistry.org/uri/RegStatus/1001> ;
    a rdf:Property ;
    rdfs:isDefinedBy <http://rdaregistry.info/Elements/u/> ;
    rdfs:label "has autographer"@en ;
    rdfs:subPropertyOf <http://rdaregistry.info/Elements/u/P60374> ;
    owl:inverseOf <http://rdaregistry.info/Elements/u/P60702> ;
    skos:definition "Relates a resource to an agent whose manuscript signature appears on a resource."@en .

<http://rdaregistry.info/Elements/u/P60467>
    reg:lexicalAlias <http://rdaregistry.info/Elements/u/issuingBody.en> ;
    reg:name "issuingBody"@en ;
    reg:status <http://metadataregistry.org/uri/RegStatus/1001> ;
    a rdf:Property ;
    rdfs:isDefinedBy <http://rdaregistry.info/Elements/u/> ;
    rdfs:label "has issuing body"@en ;
    rdfs:subPropertyOf <http://rdaregistry.info/Elements/u/P60374> ;
    owl:inverseOf <http://rdaregistry.info/Elements/u/P60703> ;
    skos:definition "Relates a resource to an agent issuing a resource, such as an official organ of the agent."@en .

<http://rdaregistry.info/Elements/u/P60468>
    reg:hasSubproperty <http://rdaregistry.info/Elements/a/P50104> ;
    reg:lexicalAlias <http://rdaregistry.info/Elements/u/professionOrOccupation.en> ;
    reg:name "professionOrOccupation"@en ;
    reg:status <http://metadataregistry.org/uri/RegStatus/1001> ;
    a rdf:Property ;
    rdfs:isDefinedBy <http://rdaregistry.info/Elements/u/> ;
    rdfs:label "has profession or occupation"@en ;
    skos:definition "Relates a resource to an agent's vocation or avocation."@en .

<http://rdaregistry.info/Elements/u/P60469>
    reg:hasSubproperty <http://rdaregistry.info/Elements/i/P40027>, <http://rdaregistry.info/Elements/m/P30136> ;
    reg:lexicalAlias <http://rdaregistry.info/Elements/u/electronicReproductionOf.en> ;
    reg:name "electronicReproductionOf"@en ;
    reg:status <http://metadataregistry.org/uri/RegStatus/1001> ;
    a rdf:Property ;
    rdfs:isDefinedBy <http://rdaregistry.info/Elements/u/> ;
    rdfs:label "is electronic reproduction of"@en ;
    rdfs:subPropertyOf <http://rdaregistry.info/Elements/u/P60297> ;
    owl:inverseOf <http://rdaregistry.info/Elements/u/P60083> ;
    skos:definition "Relates a resource to a resource in an analog format that is transferred to a digital format."@en .

<http://rdaregistry.info/Elements/u/P60470>
    reg:hasSubproperty <http://rdaregistry.info/Elements/e/P20071>, <http://rdaregistry.info/Elements/i/P40028>, <http://rdaregistry.info/Elements/m/P30137>, <http://rdaregistry.info/Elements/m/P30214>, <http://rdaregistry.info/Elements/u/P60122>, <http://rdaregistry.info/Elements/u/P60123>, <http://rdaregistry.info/Elements/u/P60124>, <http://rdaregistry.info/Elements/u/P60125>, <http://rdaregistry.info/Elements/u/P60126>, <http://rdaregistry.info/Elements/u/P60127>, <http://rdaregistry.info/Elements/u/P60128>, <http://rdaregistry.info/Elements/u/P60129>, <http://rdaregistry.info/Elements/u/P60130>, <http://rdaregistry.info/Elements/u/P60131>, <http://rdaregistry.info/Elements/u/P60132>, <http://rdaregistry.info/Elements/u/P60133>, <http://rdaregistry.info/Elements/u/P60134>, <http://rdaregistry.info/Elements/u/P60135>, <http://rdaregistry.info/Elements/u/P60136>, <http://rdaregistry.info/Elements/u/P60137>, <http://rdaregistry.info/Elements/u/P60868>, <http://rdaregistry.info/Elements/u/P60905> ;
    reg:lexicalAlias <http://rdaregistry.info/Elements/u/noteOnResource.en> ;
    reg:name "noteOnResource"@en ;
    reg:status <http://metadataregistry.org/uri/RegStatus/1001> ;
    a rdf:Property ;
    rdfs:isDefinedBy <http://rdaregistry.info/Elements/u/> ;
    rdfs:label "has note on resource"@en ;
    skos:definition "Relates a resource to a note providing additional information about content recorded as a resource attribute."@en .

<http://rdaregistry.info/Elements/u/P60471>
    reg:status <http://metadataregistry.org/uri/RegStatus/1008> ;
    rdfs:isDefinedBy <http://rdaregistry.info/Elements/u/> .

<http://rdaregistry.info/Elements/u/P60472>
    reg:lexicalAlias <http://rdaregistry.info/Elements/u/epoch.en> ;
    reg:name "epoch"@en ;
    reg:status <http://metadataregistry.org/uri/RegStatus/1001> ;
    a rdf:Property ;
    rdfs:isDefinedBy <http://rdaregistry.info/Elements/u/> ;
    rdfs:label "has epoch"@en ;
    skos:definition "Relates a resource to an arbitrary moment in time to which measurements of position for a body or orientation for an orbit are referred."@en .

<http://rdaregistry.info/Elements/u/P60473>
    reg:lexicalAlias <http://rdaregistry.info/Elements/u/landscapeArchitect.en> ;
    reg:name "landscapeArchitect"@en ;
    reg:status <http://metadataregistry.org/uri/RegStatus/1001> ;
    a rdf:Property ;
    rdfs:isDefinedBy <http://rdaregistry.info/Elements/u/> ;
    rdfs:label "has landscape architect"@en ;
    rdfs:subPropertyOf <http://rdaregistry.info/Elements/u/P60435> ;
    owl:inverseOf <http://rdaregistry.info/Elements/u/P60704> ;
    skos:definition "Relates a resource to an architect responsible for creating landscape resources."@en .

<http://rdaregistry.info/Elements/u/P60474>
    reg:hasSubproperty <http://rdaregistry.info/Elements/e/P20197> ;
    reg:lexicalAlias <http://rdaregistry.info/Elements/u/findingAidFor.en> ;
    reg:name "findingAidFor"@en ;
    reg:status <http://metadataregistry.org/uri/RegStatus/1001> ;
    a rdf:Property ;
    rdfs:isDefinedBy <http://rdaregistry.info/Elements/u/> ;
    rdfs:label "is finding aid for"@en ;
    rdfs:subPropertyOf <http://rdaregistry.info/Elements/u/P60307> ;
    owl:inverseOf <http://rdaregistry.info/Elements/u/P60262> ;
    skos:definition "Relates a resource to an archival collection that is described in a finding aid, i.e., a guide to an organization, arrangement, and contents of a collection."@en .

<http://rdaregistry.info/Elements/u/P60475>
    reg:lexicalAlias <http://rdaregistry.info/Elements/u/sculptor.en> ;
    reg:name "sculptor"@en ;
    reg:status <http://metadataregistry.org/uri/RegStatus/1001> ;
    a rdf:Property ;
    rdfs:isDefinedBy <http://rdaregistry.info/Elements/u/> ;
    rdfs:label "has sculptor"@en ;
    rdfs:subPropertyOf <http://rdaregistry.info/Elements/u/P60431> ;
    owl:inverseOf <http://rdaregistry.info/Elements/u/P60705> ;
    skos:definition "Relates a resource to an artist responsible for creating a three-dimensional resource by modeling, carving, or similar technique."@en .

<http://rdaregistry.info/Elements/u/P60476>
    reg:lexicalAlias <http://rdaregistry.info/Elements/u/screenwriter.en> ;
    reg:name "screenwriter"@en ;
    reg:status <http://metadataregistry.org/uri/RegStatus/1001> ;
    a rdf:Property ;
    rdfs:isDefinedBy <http://rdaregistry.info/Elements/u/> ;
    rdfs:label "has screenwriter"@en ;
    rdfs:subPropertyOf <http://rdaregistry.info/Elements/u/P60434> ;
    owl:inverseOf <http://rdaregistry.info/Elements/u/P60706> ;
    skos:definition "Relates a resource to an author of a screenplay, script, or scene."@en .

<http://rdaregistry.info/Elements/u/P60477>
    rdakit:seeAlso <http://rdaregistry.info/Elements/u/P60478> ;
    reg:lexicalAlias <http://rdaregistry.info/Elements/u/lyricist.en> ;
    reg:name "lyricist"@en ;
    reg:status <http://metadataregistry.org/uri/RegStatus/1001> ;
    a rdf:Property ;
    rdfs:isDefinedBy <http://rdaregistry.info/Elements/u/> ;
    rdfs:label "has lyricist"@en ;
    rdfs:subPropertyOf <http://rdaregistry.info/Elements/u/P60434> ;
    owl:inverseOf <http://rdaregistry.info/Elements/u/P60707> ;
    skos:definition "Relates a resource to an author of the words of a popular song, including a song or songs from a musical."@en ;
    skos:scopeNote "Authoring of just dialogue from a musical is excluded"@en .

<http://rdaregistry.info/Elements/u/P60478>
    rdakit:seeAlso <http://rdaregistry.info/Elements/u/P60477> ;
    reg:lexicalAlias <http://rdaregistry.info/Elements/u/librettist.en> ;
    reg:name "librettist"@en ;
    reg:status <http://metadataregistry.org/uri/RegStatus/1001> ;
    a rdf:Property ;
    rdfs:isDefinedBy <http://rdaregistry.info/Elements/u/> ;
    rdfs:label "has librettist"@en ;
    rdfs:subPropertyOf <http://rdaregistry.info/Elements/u/P60434> ;
    owl:inverseOf <http://rdaregistry.info/Elements/u/P60708> ;
    skos:definition "Relates a resource to an author of words of an opera or other musical stage resource or an oratorio."@en ;
    skos:scopeNote "Authoring of the words of just the songs from a musical is excluded."@en .

<http://rdaregistry.info/Elements/u/P60479>
    reg:hasSubproperty <http://rdaregistry.info/Elements/e/P20198> ;
    reg:lexicalAlias <http://rdaregistry.info/Elements/u/replacementInPartOf.en> ;
    reg:name "replacementInPartOf"@en ;
    reg:status <http://metadataregistry.org/uri/RegStatus/1001> ;
    a rdf:Property ;
    rdfs:isDefinedBy <http://rdaregistry.info/Elements/u/> ;
    rdfs:label "is replacement in part of"@en ;
    rdfs:subPropertyOf <http://rdaregistry.info/Elements/u/P60261> ;
    owl:inverseOf <http://rdaregistry.info/Elements/u/P60103> ;
    skos:definition "Relates a resource to an earlier resource whose content has been partially replaced by a later resource, usually because the later resource contains updated or new information that makes the earlier resource obsolete."@en ;
    skos:scopeNote "This relationship applies generally to single-part units, multipart monographs, and integrating resources."@en .

<http://rdaregistry.info/Elements/u/P60480>
    reg:hasSubproperty <http://rdaregistry.info/Elements/e/P20199> ;
    reg:lexicalAlias <http://rdaregistry.info/Elements/u/replacementOf.en> ;
    reg:name "replacementOf"@en ;
    reg:status <http://metadataregistry.org/uri/RegStatus/1001> ;
    a rdf:Property ;
    rdfs:isDefinedBy <http://rdaregistry.info/Elements/u/> ;
    rdfs:label "is replacement of"@en ;
    rdfs:subPropertyOf <http://rdaregistry.info/Elements/u/P60261> ;
    owl:inverseOf <http://rdaregistry.info/Elements/u/P60104> ;
    skos:definition "Relates a resource to an earlier resource whose content has been replaced by a later resource, usually because the later resource contains updated or new information that makes the earlier resource obsolete."@en ;
    skos:scopeNote "This relationship applies generally to single-part units, multipart monographs, and integrating resources."@en .

<http://rdaregistry.info/Elements/u/P60481>
    reg:hasSubproperty <http://rdaregistry.info/Elements/m/P30138> ;
    reg:lexicalAlias <http://rdaregistry.info/Elements/u/specialPlaybackCharacteristic.en> ;
    reg:name "specialPlaybackCharacteristic"@en ;
    reg:status <http://metadataregistry.org/uri/RegStatus/1001> ;
    a rdf:Property ;
    rdfs:isDefinedBy <http://rdaregistry.info/Elements/u/> ;
    rdfs:label "has special playback characteristic"@en ;
    rdfs:subPropertyOf <http://rdaregistry.info/Elements/u/P60351> ;
    skos:definition "Relates a resource to an equalization system, noise reduction system, etc., used in making an audio recording."@en .

<http://rdaregistry.info/Elements/u/P60482>
    reg:hasSubproperty <http://rdaregistry.info/Elements/a/P50034> ;
    reg:lexicalAlias <http://rdaregistry.info/Elements/u/associatedInstitution.en> ;
    reg:name "associatedInstitution"@en ;
    reg:status <http://metadataregistry.org/uri/RegStatus/1001> ;
    a rdf:Property ;
    rdfs:isDefinedBy <http://rdaregistry.info/Elements/u/> ;
    rdfs:label "has associated institution"@en ;
    skos:definition "Relates a resource to an institution commonly associated with an agent."@en .

<http://rdaregistry.info/Elements/u/P60483>
    reg:lexicalAlias <http://rdaregistry.info/Elements/u/grantingInstitutionOrFaculty.en> ;
    reg:name "grantingInstitutionOrFaculty"@en ;
    reg:status <http://metadataregistry.org/uri/RegStatus/1001> ;
    a rdf:Property ;
    rdfs:isDefinedBy <http://rdaregistry.info/Elements/u/> ;
    rdfs:label "has granting institution or faculty"@en ;
    skos:definition "Relates a resource to an institution or faculty conferring an academic degree on a candidate."@en .

<http://rdaregistry.info/Elements/u/P60484>
    reg:hasSubproperty <http://rdaregistry.info/Elements/a/P50035>, <http://rdaregistry.info/Elements/a/P50064> ;
    reg:lexicalAlias <http://rdaregistry.info/Elements/u/agentHistory.en> ;
    reg:name "agentHistory"@en ;
    reg:status <http://metadataregistry.org/uri/RegStatus/1001> ;
    a rdf:Property ;
    rdfs:isDefinedBy <http://rdaregistry.info/Elements/u/> ;
    rdfs:label "has agent history"@en ;
    skos:definition "Relates a resource to biographical or historical information about an agent."@en .

<http://rdaregistry.info/Elements/u/P60485>
    reg:hasSubproperty <http://rdaregistry.info/Elements/e/P20206> ;
    reg:lexicalAlias <http://rdaregistry.info/Elements/u/supplementaryContent.en> ;
    reg:name "supplementaryContent"@en ;
    reg:status <http://metadataregistry.org/uri/RegStatus/1001> ;
    a rdf:Property ;
    rdfs:isDefinedBy <http://rdaregistry.info/Elements/u/> ;
    rdfs:label "has supplementary content"@en ;
    skos:definition "Relates a resource to an indication of content that updates or complements a primary content of a resource."@en ;
    skos:scopeNote "Supplementary content may include an index, a bibliography, or an appendix."@en .

<http://rdaregistry.info/Elements/u/P60486>
    reg:hasSubproperty <http://rdaregistry.info/Elements/e/P20207> ;
    reg:lexicalAlias <http://rdaregistry.info/Elements/u/illustrativeContent.en> ;
    reg:name "illustrativeContent"@en ;
    reg:status <http://metadataregistry.org/uri/RegStatus/1001> ;
    a rdf:Property ;
    rdfs:isDefinedBy <http://rdaregistry.info/Elements/u/> ;
    rdfs:label "has illustrative content"@en ;
    skos:definition "Relates a resource to a presence of one or more still images that accompany a primary content of a resource."@en .

<http://rdaregistry.info/Elements/u/P60487>
    reg:hasSubproperty <http://rdaregistry.info/Elements/e/P20208> ;
    reg:lexicalAlias <http://rdaregistry.info/Elements/u/accessibilityContent.en> ;
    reg:name "accessibilityContent"@en ;
    reg:status <http://metadataregistry.org/uri/RegStatus/1001> ;
    a rdf:Property ;
    rdfs:isDefinedBy <http://rdaregistry.info/Elements/u/> ;
    rdfs:label "has accessibility content"@en ;
    skos:definition "Relates a resource to an indication of content that provides alternative sensory modes to perceive a primary content of a resource."@en ;
    skos:scopeNote "Accessibility content includes accessible labels, audio description, captioning, image description, sign language, and subtitles. Accessibility content does not include subtitles in a language different from the spoken content."@en .

<http://rdaregistry.info/Elements/u/P60488>
    reg:hasSubproperty <http://rdaregistry.info/Elements/e/P20209> ;
    reg:lexicalAlias <http://rdaregistry.info/Elements/u/formatOfNotatedMusic.en> ;
    reg:name "formatOfNotatedMusic"@en ;
    reg:status <http://metadataregistry.org/uri/RegStatus/1001> ;
    a rdf:Property ;
    rdfs:isDefinedBy <http://rdaregistry.info/Elements/u/> ;
    rdfs:label "has format of notated music"@en ;
    skos:definition "Relates a resource to a musical or physical layout of the content of a resource that is presented in the form of musical notation."@en .

<http://rdaregistry.info/Elements/u/P60489>
    reg:lexicalAlias <http://rdaregistry.info/Elements/u/dissertationOrThesisInformation.en> ;
    reg:name "dissertationOrThesisInformation"@en ;
    reg:status <http://metadataregistry.org/uri/RegStatus/1001> ;
    a rdf:Property ;
    rdfs:isDefinedBy <http://rdaregistry.info/Elements/u/> ;
    rdfs:label "has dissertation or thesis information"@en ;
    skos:definition "Relates a resource to a statement identifying an academic institution, degree, and year for which a resource was presented."@en .

<http://rdaregistry.info/Elements/u/P60490>
    reg:hasSubproperty <http://rdaregistry.info/Elements/m/P30141> ;
    reg:lexicalAlias <http://rdaregistry.info/Elements/u/contactInformation.en> ;
    reg:name "contactInformation"@en ;
    reg:status <http://metadataregistry.org/uri/RegStatus/1001> ;
    a rdf:Property ;
    rdfs:isDefinedBy <http://rdaregistry.info/Elements/u/> ;
    rdfs:label "has contact information"@en ;
    skos:definition "Relates a resource to a name, address, etc., of an organization, etc., from which a resource may be obtained."@en ;
    skos:scopeNote "Contact information includes the name, address, etc. of the publisher, distributor, etc. of a published resource, or of the archival repository that holds the resource."@en .

<http://rdaregistry.info/Elements/u/P60491>
    reg:lexicalAlias <http://rdaregistry.info/Elements/u/historyOfTheResource.en> ;
    reg:name "historyOfResource"@en ;
    reg:status <http://metadataregistry.org/uri/RegStatus/1001> ;
    a rdf:Property ;
    rdfs:isDefinedBy <http://rdaregistry.info/Elements/u/> ;
    rdfs:label "has history of resource"@en ;
    skos:definition "Relates a resource to a summary of information about the history of a resource."@en .

<http://rdaregistry.info/Elements/u/P60492>
    reg:hasSubproperty <http://rdaregistry.info/Elements/a/P50113> ;
    reg:lexicalAlias <http://rdaregistry.info/Elements/u/biographicalInformation.en> ;
    reg:name "biographicalInformation"@en ;
    reg:status <http://metadataregistry.org/uri/RegStatus/1001> ;
    a rdf:Property ;
    rdfs:isDefinedBy <http://rdaregistry.info/Elements/u/> ;
    rdfs:label "has biographical information"@en ;
    skos:definition "Relates an agent to a summary of information about the life or history of an agent."@en .

<http://rdaregistry.info/Elements/u/P60493>
    reg:hasSubproperty <http://rdaregistry.info/Elements/m/P30142> ;
    reg:lexicalAlias <http://rdaregistry.info/Elements/u/otherTitleInformation.en> ;
    reg:name "otherTitleInformation"@en ;
    reg:status <http://metadataregistry.org/uri/RegStatus/1001> ;
    a rdf:Property ;
    rdfs:isDefinedBy <http://rdaregistry.info/Elements/u/> ;
    rdfs:label "has other title information"@en ;
    rdfs:subPropertyOf <http://rdaregistry.info/Elements/u/P60369> ;
    skos:definition "Relates a resource to a word, character, or group of words or characters that appears in conjunction with, and is subordinate to, a title proper of a resource."@en .

<http://rdaregistry.info/Elements/u/P60494>
    reg:hasSubproperty <http://rdaregistry.info/Elements/m/P30143> ;
    reg:lexicalAlias <http://rdaregistry.info/Elements/u/otherTitleInformationOfSeries.en> ;
    reg:name "otherTitleInformationOfSeries"@en ;
    reg:status <http://metadataregistry.org/uri/RegStatus/1001> ;
    a rdf:Property ;
    rdfs:isDefinedBy <http://rdaregistry.info/Elements/u/> ;
    rdfs:label "has other title information of series"@en ;
    skos:definition "Relates a resource to a word, character, or group of words or characters that appears in conjunction with, and is subordinate to, a title proper of a series."@en .

<http://rdaregistry.info/Elements/u/P60495>
    reg:hasSubproperty <http://rdaregistry.info/Elements/m/P30144> ;
    reg:lexicalAlias <http://rdaregistry.info/Elements/u/otherTitleInformationOfSubseries.en> ;
    reg:name "otherTitleInformationOfSubseries"@en ;
    reg:status <http://metadataregistry.org/uri/RegStatus/1001> ;
    a rdf:Property ;
    rdfs:isDefinedBy <http://rdaregistry.info/Elements/u/> ;
    rdfs:label "has other title information of subseries"@en ;
    skos:definition "Relates a resource to a word, character, or group of words or characters that appears in conjunction with, and is subordinate to, a title proper of a subseries."@en .

<http://rdaregistry.info/Elements/u/P60496>
    reg:hasSubproperty <http://rdaregistry.info/Elements/i/P40047>, <http://rdaregistry.info/Elements/m/P30145> ;
    reg:lexicalAlias <http://rdaregistry.info/Elements/u/restrictionsOnAccess.en> ;
    reg:name "restrictionsOnAccess"@en ;
    reg:status <http://metadataregistry.org/uri/RegStatus/1001> ;
    a rdf:Property ;
    rdfs:isDefinedBy <http://rdaregistry.info/Elements/u/> ;
    rdfs:label "has restrictions on access"@en ;
    skos:definition "Relates a resource to limitations placed on access to a resource."@en .

<http://rdaregistry.info/Elements/u/P60497>
    reg:hasSubproperty <http://rdaregistry.info/Elements/i/P40048>, <http://rdaregistry.info/Elements/m/P30146> ;
    reg:lexicalAlias <http://rdaregistry.info/Elements/u/restrictionsOnUse.en> ;
    reg:name "restrictionsOnUse"@en ;
    reg:status <http://metadataregistry.org/uri/RegStatus/1001> ;
    a rdf:Property ;
    rdfs:isDefinedBy <http://rdaregistry.info/Elements/u/> ;
    rdfs:label "has restrictions on use"@en ;
    skos:definition "Relates a resource to a limitation placed on reproduction, publication, exhibition, etc., of a resource."@en .

<http://rdaregistry.info/Elements/u/P60498>
    reg:hasSubproperty <http://rdaregistry.info/Elements/e/P20210> ;
    reg:lexicalAlias <http://rdaregistry.info/Elements/u/otherDetailsOfCartographicContent.en> ;
    reg:name "otherDetailsOfCartographicContent"@en ;
    reg:status <http://metadataregistry.org/uri/RegStatus/1001> ;
    a rdf:Property ;
    rdfs:isDefinedBy <http://rdaregistry.info/Elements/u/> ;
    rdfs:label "has other details of cartographic content"@en ;
    skos:definition "Relates a resource to an indication of mathematical data and other features of the cartographic content of a resource not recorded in statements of scale, projection, and coordinates."@en .

<http://rdaregistry.info/Elements/u/P60499>
    reg:hasSubproperty <http://rdaregistry.info/Elements/m/P30147> ;
    reg:lexicalAlias <http://rdaregistry.info/Elements/u/numericAndOrAlphabeticDesignationOfFirstIssueOrPartOfSequence.en> ;
    reg:name "numericAndOrAlphabeticDesignationOfFirstIssueOrPartOfSequence"@en ;
    reg:status <http://metadataregistry.org/uri/RegStatus/1001> ;
    a rdf:Property ;
    rdfs:isDefinedBy <http://rdaregistry.info/Elements/u/> ;
    rdfs:label "has numeric and/or alphabetic designation of first issue or part of sequence"@en ;
    rdfs:subPropertyOf <http://rdaregistry.info/Elements/u/P60533> ;
    skos:definition "Relates a resource to a designation in numeric or alphabetic form presented on the first issue or part of a serial issued in a sequence of numbering."@en .

<http://rdaregistry.info/Elements/u/P60500>
    reg:hasSubproperty <http://rdaregistry.info/Elements/m/P30148> ;
    reg:lexicalAlias <http://rdaregistry.info/Elements/u/numericAndOrAlphabeticDesignationOfLastIssueOrPartOfSequence.en> ;
    reg:name "numericAndOrAlphabeticDesignationOfLastIssueOrPartOfSequence"@en ;
    reg:status <http://metadataregistry.org/uri/RegStatus/1001> ;
    a rdf:Property ;
    rdfs:isDefinedBy <http://rdaregistry.info/Elements/u/> ;
    rdfs:label "has numeric and/or alphabetic designation of last issue or part of sequence"@en ;
    rdfs:subPropertyOf <http://rdaregistry.info/Elements/u/P60533> ;
    skos:definition "Relates a resource to a designation in numeric or alphabetic form presented on the last issue or part of a serial issued in a sequence of numbering."@en .

<http://rdaregistry.info/Elements/u/P60501>
    reg:hasSubproperty <http://rdaregistry.info/Elements/m/P30149> ;
    reg:lexicalAlias <http://rdaregistry.info/Elements/u/chronologicalDesignationOfFirstIssueOrPartOfSequence.en> ;
    reg:name "chronologicalDesignationOfFirstIssueOrPartOfSequence"@en ;
    reg:status <http://metadataregistry.org/uri/RegStatus/1001> ;
    a rdf:Property ;
    rdfs:isDefinedBy <http://rdaregistry.info/Elements/u/> ;
    rdfs:label "has chronological designation of first issue or part of sequence"@en ;
    rdfs:subPropertyOf <http://rdaregistry.info/Elements/u/P60533> ;
    skos:definition "Relates a resource to a designation in date form presented on the first issue or part of a serial issued in a sequence of numbering."@en ;
    skos:scopeNote "Designation includes a year; year and month; month, day, and year."@en .

<http://rdaregistry.info/Elements/u/P60502>
    reg:hasSubproperty <http://rdaregistry.info/Elements/m/P30150> ;
    reg:lexicalAlias <http://rdaregistry.info/Elements/u/chronologicalDesignationOfLastIssueOrPartOfSequence.en> ;
    reg:name "chronologicalDesignationOfLastIssueOrPartOfSequence"@en ;
    reg:status <http://metadataregistry.org/uri/RegStatus/1001> ;
    a rdf:Property ;
    rdfs:isDefinedBy <http://rdaregistry.info/Elements/u/> ;
    rdfs:label "has chronological designation of last issue or part of sequence"@en ;
    rdfs:subPropertyOf <http://rdaregistry.info/Elements/u/P60533> ;
    skos:definition "Relates a resource to a designation in date form presented on the last issue or part of a serial issued in a sequence of numbering."@en ;
    skos:scopeNote "Designation includes a year; year and month; month, day, and year."@en .

<http://rdaregistry.info/Elements/u/P60503>
    reg:hasSubproperty <http://rdaregistry.info/Elements/e/P20200> ;
    reg:lexicalAlias <http://rdaregistry.info/Elements/u/splitInto.en> ;
    reg:name "splitInto"@en ;
    reg:status <http://metadataregistry.org/uri/RegStatus/1001> ;
    a rdf:Property ;
    rdfs:isDefinedBy <http://rdaregistry.info/Elements/u/> ;
    rdfs:label "is split into"@en ;
    rdfs:subPropertyOf <http://rdaregistry.info/Elements/u/P60278> ;
    owl:inverseOf <http://rdaregistry.info/Elements/u/P60276> ;
    skos:definition "Relates a resource to a resource resulting from a division of an earlier resource into two or more separate resources."@en .

<http://rdaregistry.info/Elements/u/P60504>
    reg:hasSubproperty <http://rdaregistry.info/Elements/e/P20212> ;
    reg:lexicalAlias <http://rdaregistry.info/Elements/u/mergedToForm.en> ;
    reg:name "mergedToForm"@en ;
    reg:status <http://metadataregistry.org/uri/RegStatus/1001> ;
    a rdf:Property ;
    rdfs:isDefinedBy <http://rdaregistry.info/Elements/u/> ;
    rdfs:label "is merged to form"@en ;
    rdfs:subPropertyOf <http://rdaregistry.info/Elements/u/P60278> ;
    owl:inverseOf <http://rdaregistry.info/Elements/u/P60505> ;
    skos:definition "Relates a resource to a resource formed from a coming together of two or more resources."@en .

<http://rdaregistry.info/Elements/u/P60505>
    reg:hasSubproperty <http://rdaregistry.info/Elements/e/P20201> ;
    reg:lexicalAlias <http://rdaregistry.info/Elements/u/mergerOf.en> ;
    reg:name "mergerOf"@en ;
    reg:status <http://metadataregistry.org/uri/RegStatus/1001> ;
    a rdf:Property ;
    rdfs:isDefinedBy <http://rdaregistry.info/Elements/u/> ;
    rdfs:label "is merger of"@en ;
    rdfs:subPropertyOf <http://rdaregistry.info/Elements/u/P60261> ;
    owl:inverseOf <http://rdaregistry.info/Elements/u/P60504> ;
    skos:definition "Relates a resource to a resource that came together with one or more other resources to form a new resource."@en .

<http://rdaregistry.info/Elements/u/P60506>
    reg:lexicalAlias <http://rdaregistry.info/Elements/u/equinox.en> ;
    reg:name "equinox"@en ;
    reg:status <http://metadataregistry.org/uri/RegStatus/1001> ;
    a rdf:Property ;
    rdfs:isDefinedBy <http://rdaregistry.info/Elements/u/> ;
    rdfs:label "has equinox"@en ;
    skos:definition "Relates a resource to a point of intersection of the ecliptic and the celestial equator, occupied by the sun when its declination is 0."@en .

<http://rdaregistry.info/Elements/u/P60507>
    reg:hasSubproperty <http://rdaregistry.info/Elements/m/P30151> ;
    reg:lexicalAlias <http://rdaregistry.info/Elements/u/parallelOtherTitleInformation.en> ;
    reg:name "parallelOtherTitleInformation"@en ;
    reg:status <http://metadataregistry.org/uri/RegStatus/1001> ;
    a rdf:Property ;
    rdfs:isDefinedBy <http://rdaregistry.info/Elements/u/> ;
    rdfs:label "has parallel other title information"@en ;
    rdfs:subPropertyOf <http://rdaregistry.info/Elements/u/P60369> ;
    skos:definition "Relates a resource to an other title information in a language or script that differs from that recorded in an other title information element."@en .

<http://rdaregistry.info/Elements/u/P60508>
    reg:hasSubproperty <http://rdaregistry.info/Elements/m/P30152> ;
    reg:lexicalAlias <http://rdaregistry.info/Elements/u/parallelOtherTitleInformationOfSeries.en> ;
    reg:name "parallelOtherTitleInformationOfSeries"@en ;
    reg:status <http://metadataregistry.org/uri/RegStatus/1001> ;
    a rdf:Property ;
    rdfs:isDefinedBy <http://rdaregistry.info/Elements/u/> ;
    rdfs:label "has parallel other title information of series"@en ;
    skos:definition "Relates a resource to an other title information of a series in a language or script that differs from that recorded in an other title information of series element."@en .

<http://rdaregistry.info/Elements/u/P60509>
    reg:hasSubproperty <http://rdaregistry.info/Elements/m/P30153> ;
    reg:lexicalAlias <http://rdaregistry.info/Elements/u/parallelOtherTitleInformationOfSubseries.en> ;
    reg:name "parallelOtherTitleInformationOfSubseries"@en ;
    reg:status <http://metadataregistry.org/uri/RegStatus/1001> ;
    a rdf:Property ;
    rdfs:isDefinedBy <http://rdaregistry.info/Elements/u/> ;
    rdfs:label "has parallel other title information of subseries"@en ;
    skos:definition "Relates a resource to an other title information of a subseries in a language or script that differs from that recorded in an other title information of subseries element."@en .

<http://rdaregistry.info/Elements/u/P60510>
    reg:hasSubproperty <http://rdaregistry.info/Elements/e/P20213> ;
    reg:lexicalAlias <http://rdaregistry.info/Elements/u/additionalScaleInformation.en> ;
    reg:name "additionalScaleInformation"@en ;
    reg:status <http://metadataregistry.org/uri/RegStatus/1001> ;
    a rdf:Property ;
    rdfs:isDefinedBy <http://rdaregistry.info/Elements/u/> ;
    rdfs:label "has additional scale information"@en ;
    rdfs:subPropertyOf <http://rdaregistry.info/Elements/u/P60565> ;
    skos:definition "Relates a resource to an indication of supplemental information about scale."@en ;
    skos:scopeNote "Statement of comparative measurements or limitation of the scale to particular parts of the content of a resource are included."@en .

<http://rdaregistry.info/Elements/u/P60511>
    reg:hasSubproperty <http://rdaregistry.info/Elements/m/P30154> ;
    reg:lexicalAlias <http://rdaregistry.info/Elements/u/uniformResourceLocator.en> ;
    reg:name "uniformResourceLocator"@en ;
    reg:status <http://metadataregistry.org/uri/RegStatus/1001> ;
    a rdf:Property ;
    rdfs:isDefinedBy <http://rdaregistry.info/Elements/u/> ;
    rdfs:label "has uniform resource locator"@en ;
    skos:altLabel "URL"@en ;
    skos:definition "Relates a resource to an address of an online resource."@en ;
    skos:scopeNote "A Uniform Resource Locators includes all resource identifiers intended to provide online access to a resource using a standard Internet browser."@en .

<http://rdaregistry.info/Elements/u/P60512>
    reg:hasSubproperty <http://rdaregistry.info/Elements/a/P50036>, <http://rdaregistry.info/Elements/a/P50114> ;
    reg:lexicalAlias <http://rdaregistry.info/Elements/u/addressOfAgent.en> ;
    reg:name "addressOfAgent"@en ;
    reg:status <http://metadataregistry.org/uri/RegStatus/1001> ;
    a rdf:Property ;
    rdfs:isDefinedBy <http://rdaregistry.info/Elements/u/> ;
    rdfs:label "has address of agent"@en ;
    skos:definition "Relates a resource to an address of an agent's place of residence, business, or employer, headquarters or offices, or an e-mail or internet address."@en .

<http://rdaregistry.info/Elements/u/P60513>
    reg:hasSubproperty <http://rdaregistry.info/Elements/m/P30155> ;
    reg:lexicalAlias <http://rdaregistry.info/Elements/u/layout.en> ;
    reg:name "layout"@en ;
    reg:status <http://metadataregistry.org/uri/RegStatus/1001> ;
    a rdf:Property ;
    rdfs:isDefinedBy <http://rdaregistry.info/Elements/u/> ;
    rdfs:label "has layout"@en ;
    skos:definition "Relates a resource to an arrangement of text, images, tactile notation, etc., in a resource."@en .

<http://rdaregistry.info/Elements/u/P60514>
    reg:lexicalAlias <http://rdaregistry.info/Elements/u/yearDegreeGranted.en> ;
    reg:name "yearDegreeGranted"@en ;
    reg:status <http://metadataregistry.org/uri/RegStatus/1001> ;
    a rdf:Property ;
    rdfs:isDefinedBy <http://rdaregistry.info/Elements/u/> ;
    rdfs:label "has year degree granted"@en ;
    skos:definition "Relates a resource to a calendar year in which a granting institution or faculty conferred an academic degree on a candidate."@en .

<http://rdaregistry.info/Elements/u/P60515>
    reg:hasSubproperty <http://rdaregistry.info/Elements/m/P30156> ;
    reg:lexicalAlias <http://rdaregistry.info/Elements/u/titleProper.en> ;
    reg:name "titleProper"@en ;
    reg:status <http://metadataregistry.org/uri/RegStatus/1001> ;
    a rdf:Property ;
    rdfs:isDefinedBy <http://rdaregistry.info/Elements/u/> ;
    rdfs:label "has title proper"@en ;
    rdfs:subPropertyOf <http://rdaregistry.info/Elements/u/P60369> ;
    skos:definition "Relates a resource to a chief name of a resource, that is, a title normally used when naming a resource."@en ;
    skos:scopeNote "An alternative title is treated as part of the title proper."@en .

<http://rdaregistry.info/Elements/u/P60516>
    reg:hasSubproperty <http://rdaregistry.info/Elements/m/P30157> ;
    reg:lexicalAlias <http://rdaregistry.info/Elements/u/titleProperOfSeries.en> ;
    reg:name "titleProperOfSeries"@en ;
    reg:status <http://metadataregistry.org/uri/RegStatus/1001> ;
    a rdf:Property ;
    rdfs:isDefinedBy <http://rdaregistry.info/Elements/u/> ;
    rdfs:label "has title proper of series"@en ;
    skos:definition "Relates a resource to a name of a series appearing on a resource of a part of a series."@en .

<http://rdaregistry.info/Elements/u/P60517>
    reg:hasSubproperty <http://rdaregistry.info/Elements/m/P30158> ;
    reg:lexicalAlias <http://rdaregistry.info/Elements/u/titleProperOfSubseries.en> ;
    reg:name "titleProperOfSubseries"@en ;
    reg:status <http://metadataregistry.org/uri/RegStatus/1001> ;
    a rdf:Property ;
    rdfs:isDefinedBy <http://rdaregistry.info/Elements/u/> ;
    rdfs:label "has title proper of subseries"@en ;
    skos:definition "Relates a resource to a name of a series appearing on a resource of a part of a subseries."@en .

<http://rdaregistry.info/Elements/u/P60518>
    reg:lexicalAlias <http://rdaregistry.info/Elements/u/coverageOfContent.en> ;
    reg:name "coverageOfContent"@en ;
    reg:status <http://metadataregistry.org/uri/RegStatus/1001> ;
    a rdf:Property ;
    rdfs:isDefinedBy <http://rdaregistry.info/Elements/u/> ;
    rdfs:label "has coverage of content"@en ;
    skos:definition "Relates a resource to a chronological or geographic coverage of the content of a resource."@en .

<http://rdaregistry.info/Elements/u/P60519>
    reg:hasSubproperty <http://rdaregistry.info/Elements/m/P30159> ;
    reg:lexicalAlias <http://rdaregistry.info/Elements/u/resolution.en> ;
    reg:name "resolution"@en ;
    reg:status <http://metadataregistry.org/uri/RegStatus/1001> ;
    a rdf:Property ;
    rdfs:isDefinedBy <http://rdaregistry.info/Elements/u/> ;
    rdfs:label "has resolution"@en ;
    rdfs:subPropertyOf <http://rdaregistry.info/Elements/u/P60350> ;
    skos:definition "Relates a resource to a clarity or fineness of detail in a digital image, expressed by a measurement of the image in pixels, etc."@en .

<http://rdaregistry.info/Elements/u/P60520>
    reg:lexicalAlias <http://rdaregistry.info/Elements/u/intendedAudience.en> ;
    reg:name "intendedAudience"@en ;
    reg:status <http://metadataregistry.org/uri/RegStatus/1001> ;
    a rdf:Property ;
    rdfs:isDefinedBy <http://rdaregistry.info/Elements/u/> ;
    rdfs:label "has intended audience"@en ;
    skos:definition "Relates a resource to a category of user for which the content of a resource is intended, or for whom the content is considered suitable."@en .

<http://rdaregistry.info/Elements/u/P60521>
    reg:hasSubproperty <http://rdaregistry.info/Elements/m/P30160> ;
    reg:lexicalAlias <http://rdaregistry.info/Elements/u/termsOfAvailability.en> ;
    reg:name "termsOfAvailability"@en ;
    reg:status <http://metadataregistry.org/uri/RegStatus/1001> ;
    a rdf:Property ;
    rdfs:isDefinedBy <http://rdaregistry.info/Elements/u/> ;
    rdfs:label "has terms of availability"@en ;
    skos:definition "Relates a resource to a condition under which a publisher, distributor, etc., will normally supply a resource or the price of a resource."@en .

<http://rdaregistry.info/Elements/u/P60522>
    reg:hasSubproperty <http://rdaregistry.info/Elements/m/P30161> ;
    reg:lexicalAlias <http://rdaregistry.info/Elements/u/trackConfiguration.en> ;
    reg:name "trackConfiguration"@en ;
    reg:status <http://metadataregistry.org/uri/RegStatus/1001> ;
    a rdf:Property ;
    rdfs:isDefinedBy <http://rdaregistry.info/Elements/u/> ;
    rdfs:label "has track configuration"@en ;
    rdfs:subPropertyOf <http://rdaregistry.info/Elements/u/P60351> ;
    skos:definition "Relates a reource to a configuration of an audio track on a sound-track film."@en .

<http://rdaregistry.info/Elements/u/P60523>
    reg:lexicalAlias <http://rdaregistry.info/Elements/u/placeOfOriginOfResource.en> ;
    reg:name "placeOfOriginOfResource"@en ;
    reg:status <http://metadataregistry.org/uri/RegStatus/1001> ;
    a rdf:Property ;
    rdfs:isDefinedBy <http://rdaregistry.info/Elements/u/> ;
    rdfs:label "has place of origin of resource"@en ;
    skos:definition "Relates a resource to a country or other territorial jurisdiction from which a resource originated."@en .

<http://rdaregistry.info/Elements/u/P60524>
    reg:hasSubproperty <http://rdaregistry.info/Elements/a/P50037> ;
    reg:lexicalAlias <http://rdaregistry.info/Elements/u/dateOfEstablishment.en> ;
    reg:name "dateOfEstablishment"@en ;
    reg:status <http://metadataregistry.org/uri/RegStatus/1001> ;
    a rdf:Property ;
    rdfs:isDefinedBy <http://rdaregistry.info/Elements/u/> ;
    rdfs:label "has date of establishment"@en ;
    rdfs:subPropertyOf <http://rdaregistry.info/Elements/u/P60324> ;
    skos:definition "Relates a resource to a date on which an agent was established or founded."@en .

<http://rdaregistry.info/Elements/u/P60525>
    reg:hasSubproperty <http://rdaregistry.info/Elements/a/P50038> ;
    reg:lexicalAlias <http://rdaregistry.info/Elements/u/dateOfTermination.en> ;
    reg:name "dateOfTermination"@en ;
    reg:status <http://metadataregistry.org/uri/RegStatus/1001> ;
    a rdf:Property ;
    rdfs:isDefinedBy <http://rdaregistry.info/Elements/u/> ;
    rdfs:label "has date of termination"@en ;
    rdfs:subPropertyOf <http://rdaregistry.info/Elements/u/P60324> ;
    skos:definition "Relates a resource to a date on which an agent was terminated or dissolved."@en .

<http://rdaregistry.info/Elements/u/P60526>
    reg:hasSubproperty <http://rdaregistry.info/Elements/a/P50039> ;
    reg:lexicalAlias <http://rdaregistry.info/Elements/u/dateOfConferenceEtc.en> ;
    reg:name "dateOfConferenceEtc"@en ;
    reg:status <http://metadataregistry.org/uri/RegStatus/1001> ;
    a rdf:Property ;
    rdfs:isDefinedBy <http://rdaregistry.info/Elements/u/> ;
    rdfs:label "has date of conference, etc."@en ;
    rdfs:subPropertyOf <http://rdaregistry.info/Elements/u/P60324> ;
    skos:definition "Relates a resource to a date or range of dates on which a conference, congress, meeting, exhibition, fair, festival, etc., was held."@en .

<http://rdaregistry.info/Elements/u/P60527>
    reg:hasSubproperty <http://rdaregistry.info/Elements/e/P20214> ;
    reg:lexicalAlias <http://rdaregistry.info/Elements/u/dateOfResource.en> ;
    reg:name "dateOfResource"@en ;
    reg:status <http://metadataregistry.org/uri/RegStatus/1001> ;
    a rdf:Property ;
    rdfs:isDefinedBy <http://rdaregistry.info/Elements/u/> ;
    rdfs:label "has date of resource"@en ;
    skos:definition "Relates a resource to an earliest date associated with a resource."@en .

<http://rdaregistry.info/Elements/u/P60528>
    reg:hasSubproperty <http://rdaregistry.info/Elements/m/P30162> ;
    reg:lexicalAlias <http://rdaregistry.info/Elements/u/equipmentOrSystemRequirement.en> ;
    reg:name "equipmentOrSystemRequirement"@en ;
    reg:status <http://metadataregistry.org/uri/RegStatus/1001> ;
    a rdf:Property ;
    rdfs:isDefinedBy <http://rdaregistry.info/Elements/u/> ;
    rdfs:label "has equipment or system requirement"@en ;
    skos:definition "Relates a resource to a system or equipment required for use, playback, etc., of an analog, digital, etc., resource."@en .

<http://rdaregistry.info/Elements/u/P60529>
    reg:hasSubproperty <http://rdaregistry.info/Elements/m/P30163> ;
    reg:lexicalAlias <http://rdaregistry.info/Elements/u/presentationFormat.en> ;
    reg:name "presentationFormat"@en ;
    reg:status <http://metadataregistry.org/uri/RegStatus/1001> ;
    a rdf:Property ;
    rdfs:isDefinedBy <http://rdaregistry.info/Elements/u/> ;
    rdfs:label "has presentation format"@en ;
    rdfs:subPropertyOf <http://rdaregistry.info/Elements/u/P60353> ;
    skos:definition "Relates a resource to a format used in the production of a projected image."@en .

<http://rdaregistry.info/Elements/u/P60530>
    reg:hasSubproperty <http://rdaregistry.info/Elements/a/P50115> ;
    reg:lexicalAlias <http://rdaregistry.info/Elements/u/fullerFormOfName.en> ;
    reg:name "fullerFormOfName"@en ;
    reg:status <http://metadataregistry.org/uri/RegStatus/1001> ;
    a rdf:Property ;
    rdfs:isDefinedBy <http://rdaregistry.info/Elements/u/> ;
    rdfs:label "has fuller form of name"@en ;
    skos:definition "Relates a resource to a full form of a part of a name represented only by an initial or abbreviation in a form chosen as a preferred name, or a part of a name not included in a form chosen as a preferred name."@en .

<http://rdaregistry.info/Elements/u/P60531>
    reg:hasSubproperty <http://rdaregistry.info/Elements/a/P50116> ;
    reg:lexicalAlias <http://rdaregistry.info/Elements/u/gender.en> ;
    reg:name "gender"@en ;
    reg:status <http://metadataregistry.org/uri/RegStatus/1001> ;
    a rdf:Property ;
    rdfs:isDefinedBy <http://rdaregistry.info/Elements/u/> ;
    rdfs:label "has gender"@en ;
    skos:definition "Relates a resource to a gender with which an agent identifies."@en .

<http://rdaregistry.info/Elements/u/P60532>
    reg:hasSubproperty <http://rdaregistry.info/Elements/m/P30164> ;
    reg:lexicalAlias <http://rdaregistry.info/Elements/u/grooveCharacteristic.en> ;
    reg:name "grooveCharacteristic"@en ;
    reg:status <http://metadataregistry.org/uri/RegStatus/1001> ;
    a rdf:Property ;
    rdfs:isDefinedBy <http://rdaregistry.info/Elements/u/> ;
    rdfs:label "has groove characteristic"@en ;
    rdfs:subPropertyOf <http://rdaregistry.info/Elements/u/P60351> ;
    skos:definition "Relates a resource to a groove width of an analog disc or a groove pitch of an analog cylinder."@en .

<http://rdaregistry.info/Elements/u/P60533>
    reg:hasSubproperty <http://rdaregistry.info/Elements/m/P30165>, <http://rdaregistry.info/Elements/u/P60499>, <http://rdaregistry.info/Elements/u/P60500>, <http://rdaregistry.info/Elements/u/P60501>, <http://rdaregistry.info/Elements/u/P60502>, <http://rdaregistry.info/Elements/u/P60818>, <http://rdaregistry.info/Elements/u/P60819>, <http://rdaregistry.info/Elements/u/P60820>, <http://rdaregistry.info/Elements/u/P60821> ;
    reg:lexicalAlias <http://rdaregistry.info/Elements/u/numberingOfSerials.en> ;
    reg:name "numberingOfSerials"@en ;
    reg:status <http://metadataregistry.org/uri/RegStatus/1001> ;
    a rdf:Property ;
    rdfs:isDefinedBy <http://rdaregistry.info/Elements/u/> ;
    rdfs:label "has numbering of serials"@en ;
    skos:definition "Relates a resource to a designation for each of the issues or parts of a serial."@en ;
    skos:scopeNote "Numbering includes a numeral, a letter, any other character, or the combination of these with or without an accompanying caption and/or a chronological designation."@en .

<http://rdaregistry.info/Elements/u/P60534>
    reg:hasSubproperty <http://rdaregistry.info/Elements/m/P30166> ;
    reg:lexicalAlias <http://rdaregistry.info/Elements/u/issnOfSeries.en> ;
    reg:name "issnOfSeries"@en ;
    reg:status <http://metadataregistry.org/uri/RegStatus/1001> ;
    a rdf:Property ;
    rdfs:isDefinedBy <http://rdaregistry.info/Elements/u/> ;
    rdfs:label "has ISSN of series"@en ;
    skos:definition "Relates a resource to an identifier assigned to a series by an ISSN registration agency."@en .

<http://rdaregistry.info/Elements/u/P60535>
    reg:hasSubproperty <http://rdaregistry.info/Elements/m/P30167> ;
    reg:lexicalAlias <http://rdaregistry.info/Elements/u/issnOfSubseries.en> ;
    reg:name "issnOfSubseries"@en ;
    reg:status <http://metadataregistry.org/uri/RegStatus/1001> ;
    a rdf:Property ;
    rdfs:isDefinedBy <http://rdaregistry.info/Elements/u/> ;
    rdfs:label "has ISSN of subseries"@en ;
    skos:definition "Relates a resource to an identifier assigned to a subseries by an ISSN registration agency."@en .

<http://rdaregistry.info/Elements/u/P60536>
    reg:lexicalAlias <http://rdaregistry.info/Elements/u/mediumOfPerformance.en> ;
    reg:name "mediumOfPerformance"@en ;
    reg:status <http://metadataregistry.org/uri/RegStatus/1001> ;
    a rdf:Property ;
    rdfs:isDefinedBy <http://rdaregistry.info/Elements/u/> ;
    rdfs:label "has medium of performance"@en ;
    skos:definition "Relates a resource to an instrument, voice, or ensemble for which a musical resource was originally conceived."@en .

<http://rdaregistry.info/Elements/u/P60537>
    reg:hasSubproperty <http://rdaregistry.info/Elements/e/P20215> ;
    reg:lexicalAlias <http://rdaregistry.info/Elements/u/mediumOfPerformanceOfMusicalContent.en> ;
    reg:name "mediumOfPerformanceOfMusicalContent"@en ;
    reg:status <http://metadataregistry.org/uri/RegStatus/1001> ;
    a rdf:Property ;
    rdfs:isDefinedBy <http://rdaregistry.info/Elements/u/> ;
    rdfs:label "has medium of performance of musical content"@en ;
    skos:definition "Relates a resource to an instrument, voice, or ensemble used, or intended to be used, for performance of musical content."@en .

<http://rdaregistry.info/Elements/u/P60538>
    reg:hasSubproperty <http://rdaregistry.info/Elements/m/P30168> ;
    reg:lexicalAlias <http://rdaregistry.info/Elements/u/frequency.en> ;
    reg:name "frequency"@en ;
    reg:status <http://metadataregistry.org/uri/RegStatus/1001> ;
    a rdf:Property ;
    rdfs:isDefinedBy <http://rdaregistry.info/Elements/u/> ;
    rdfs:label "has frequency"@en ;
    skos:definition "Relates a resource to an interval at which an issue or part of a serial or an update to an integrating resource is issued."@en .

<http://rdaregistry.info/Elements/u/P60539>
    reg:hasSubproperty <http://rdaregistry.info/Elements/m/P30169>, <http://rdaregistry.info/Elements/u/P60540>, <http://rdaregistry.info/Elements/u/P60541> ;
    reg:lexicalAlias <http://rdaregistry.info/Elements/u/dimensions.en> ;
    reg:name "dimensions"@en ;
    reg:status <http://metadataregistry.org/uri/RegStatus/1001> ;
    a rdf:Property ;
    rdfs:isDefinedBy <http://rdaregistry.info/Elements/u/> ;
    rdfs:label "has dimensions"@en ;
    skos:definition "Relates a resource to a measurement of a carrier or a container of a resource."@en .

<http://rdaregistry.info/Elements/u/P60540>
    reg:hasSubproperty <http://rdaregistry.info/Elements/m/P30170> ;
    reg:lexicalAlias <http://rdaregistry.info/Elements/u/dimensionsOfMapEtc.en> ;
    reg:name "dimensionsOfMapEtc"@en ;
    reg:status <http://metadataregistry.org/uri/RegStatus/1001> ;
    a rdf:Property ;
    rdfs:isDefinedBy <http://rdaregistry.info/Elements/u/> ;
    rdfs:label "has dimensions of map, etc."@en ;
    rdfs:subPropertyOf <http://rdaregistry.info/Elements/u/P60539> ;
    skos:definition "Relates a resource to a measurement of a face of a map, etc."@en .

<http://rdaregistry.info/Elements/u/P60541>
    reg:hasSubproperty <http://rdaregistry.info/Elements/m/P30171> ;
    reg:lexicalAlias <http://rdaregistry.info/Elements/u/dimensionsOfStillImage.en> ;
    reg:name "dimensionsOfStillImage"@en ;
    reg:status <http://metadataregistry.org/uri/RegStatus/1001> ;
    a rdf:Property ;
    rdfs:isDefinedBy <http://rdaregistry.info/Elements/u/> ;
    rdfs:label "has dimensions of still image"@en ;
    rdfs:subPropertyOf <http://rdaregistry.info/Elements/u/P60539> ;
    skos:definition "Relates a resource to a measurement of the pictorial area of a still image."@en .

<http://rdaregistry.info/Elements/u/P60542>
    reg:hasSubproperty <http://rdaregistry.info/Elements/e/P20216> ;
    reg:lexicalAlias <http://rdaregistry.info/Elements/u/projectionOfCartographicContent.en> ;
    reg:name "projectionOfCartographicContent"@en ;
    reg:status <http://metadataregistry.org/uri/RegStatus/1001> ;
    a rdf:Property ;
    rdfs:isDefinedBy <http://rdaregistry.info/Elements/u/> ;
    rdfs:label "has projection of cartographic content"@en ;
    skos:definition "Relates a resource to a method or system used to represent the surface of the earth or of a celestial sphere on a plane."@en .

<http://rdaregistry.info/Elements/u/P60543>
    reg:hasSubproperty <http://rdaregistry.info/Elements/m/P30172> ;
    reg:lexicalAlias <http://rdaregistry.info/Elements/u/typeOfRecording.en> ;
    reg:name "typeOfRecording"@en ;
    reg:status <http://metadataregistry.org/uri/RegStatus/1001> ;
    a rdf:Property ;
    rdfs:isDefinedBy <http://rdaregistry.info/Elements/u/> ;
    rdfs:label "has type of recording"@en ;
    rdfs:subPropertyOf <http://rdaregistry.info/Elements/u/P60351> ;
    skos:definition "Relates a resource to a method used to encode audio content for playback."@en .

<http://rdaregistry.info/Elements/u/P60544>
    reg:hasSubproperty <http://rdaregistry.info/Elements/m/P30173> ;
    reg:lexicalAlias <http://rdaregistry.info/Elements/u/distributorsName.en> ;
    reg:name "distributorsName"@en ;
    reg:status <http://metadataregistry.org/uri/RegStatus/1001> ;
    a rdf:Property ;
    rdfs:isDefinedBy <http://rdaregistry.info/Elements/u/> ;
    rdfs:label "has distributors name"@en ;
    skos:definition "Relates a resource to a name of an agent responsible for distributing a resource in a published form."@en .

<http://rdaregistry.info/Elements/u/P60545>
    reg:hasSubproperty <http://rdaregistry.info/Elements/m/P30174> ;
    reg:lexicalAlias <http://rdaregistry.info/Elements/u/producersName.en> ;
    reg:name "producersName"@en ;
    reg:status <http://metadataregistry.org/uri/RegStatus/1001> ;
    a rdf:Property ;
    rdfs:isDefinedBy <http://rdaregistry.info/Elements/u/> ;
    rdfs:label "has producers name"@en ;
    skos:definition "Relates a resource to a name of an agent responsible for inscribing, fabricating, constructing, etc., a resource in an unpublished form."@en .

<http://rdaregistry.info/Elements/u/P60546>
    reg:hasSubproperty <http://rdaregistry.info/Elements/m/P30175> ;
    reg:lexicalAlias <http://rdaregistry.info/Elements/u/manufacturersName.en> ;
    reg:name "manufacturersName"@en ;
    reg:status <http://metadataregistry.org/uri/RegStatus/1001> ;
    a rdf:Property ;
    rdfs:isDefinedBy <http://rdaregistry.info/Elements/u/> ;
    rdfs:label "has manufacturers name"@en ;
    skos:definition "Relates a resource to a name of an agent responsible for printing, duplicating, casting, etc., a resource in a published form."@en .

<http://rdaregistry.info/Elements/u/P60547>
    reg:hasSubproperty <http://rdaregistry.info/Elements/m/P30176> ;
    reg:lexicalAlias <http://rdaregistry.info/Elements/u/publishersName.en> ;
    reg:name "publishersName"@en ;
    reg:status <http://metadataregistry.org/uri/RegStatus/1001> ;
    a rdf:Property ;
    rdfs:isDefinedBy <http://rdaregistry.info/Elements/u/> ;
    rdfs:label "has publishers name"@en ;
    skos:definition "Relates a resource to a name of an agent responsible for publishing, releasing, or issuing a resource."@en .

<http://rdaregistry.info/Elements/u/P60548>
    reg:hasSubproperty <http://rdaregistry.info/Elements/p/P70002> ;
    reg:lexicalAlias <http://rdaregistry.info/Elements/u/preferredNameOfPlace.en> ;
    reg:name "preferredNameOfPlace"@en ;
    reg:status <http://metadataregistry.org/uri/RegStatus/1001> ;
    a rdf:Property ;
    rdfs:isDefinedBy <http://rdaregistry.info/Elements/u/> ;
    rdfs:label "has preferred name of place"@en ;
    rdfs:subPropertyOf <http://rdaregistry.info/Elements/u/P60366> ;
    skos:definition "Relates a resource to a name or form of name chosen to identify a place."@en .

<http://rdaregistry.info/Elements/u/P60549>
    reg:hasSubproperty <http://rdaregistry.info/Elements/a/P50041>, <http://rdaregistry.info/Elements/a/P50065>, <http://rdaregistry.info/Elements/a/P50117> ;
    reg:lexicalAlias <http://rdaregistry.info/Elements/u/preferredNameForAgent.en> ;
    reg:name "preferredNameForAgent"@en ;
    reg:status <http://metadataregistry.org/uri/RegStatus/1001> ;
    a rdf:Property ;
    rdfs:isDefinedBy <http://rdaregistry.info/Elements/u/> ;
    rdfs:label "has preferred name for agent"@en ;
    rdfs:subPropertyOf <http://rdaregistry.info/Elements/u/P60368> ;
    skos:definition "Relates a resource to a name or form of name chosen to identify an agent."@en .

<http://rdaregistry.info/Elements/u/P60550>
    reg:hasSubproperty <http://rdaregistry.info/Elements/m/P30177>, <http://rdaregistry.info/Elements/m/P30178>, <http://rdaregistry.info/Elements/m/P30179>, <http://rdaregistry.info/Elements/m/P30180>, <http://rdaregistry.info/Elements/m/P30181>, <http://rdaregistry.info/Elements/m/P30182> ;
    reg:lexicalAlias <http://rdaregistry.info/Elements/u/extent.en> ;
    reg:name "extent"@en ;
    reg:status <http://metadataregistry.org/uri/RegStatus/1001> ;
    a rdf:Property ;
    rdfs:isDefinedBy <http://rdaregistry.info/Elements/u/> ;
    rdfs:label "has extent"@en ;
    skos:definition "Relates a resource to a number and type of unit or subunit of a resource."@en .

<http://rdaregistry.info/Elements/u/P60551>
    reg:hasSubproperty <http://rdaregistry.info/Elements/m/P30183> ;
    reg:lexicalAlias <http://rdaregistry.info/Elements/u/fileSize.en> ;
    reg:name "fileSize"@en ;
    reg:status <http://metadataregistry.org/uri/RegStatus/1001> ;
    a rdf:Property ;
    rdfs:isDefinedBy <http://rdaregistry.info/Elements/u/> ;
    rdfs:label "has file size"@en ;
    rdfs:subPropertyOf <http://rdaregistry.info/Elements/u/P60350> ;
    skos:definition "Relates a resource to a number of bytes in a digital file."@en .

<http://rdaregistry.info/Elements/u/P60552>
    reg:hasSubproperty <http://rdaregistry.info/Elements/m/P30184> ;
    reg:lexicalAlias <http://rdaregistry.info/Elements/u/configurationOfPlaybackChannels.en> ;
    reg:name "configurationOfPlaybackChannels"@en ;
    reg:status <http://metadataregistry.org/uri/RegStatus/1001> ;
    a rdf:Property ;
    rdfs:isDefinedBy <http://rdaregistry.info/Elements/u/> ;
    rdfs:label "has configuration of playback channels"@en ;
    rdfs:subPropertyOf <http://rdaregistry.info/Elements/u/P60351> ;
    skos:definition "Relates a resource to a number of sound channels used to make a recording."@en .

<http://rdaregistry.info/Elements/u/P60553>
    reg:hasSubproperty <http://rdaregistry.info/Elements/m/P30185> ;
    reg:lexicalAlias <http://rdaregistry.info/Elements/u/tapeConfiguration.en> ;
    reg:name "tapeConfiguration"@en ;
    reg:status <http://metadataregistry.org/uri/RegStatus/1001> ;
    a rdf:Property ;
    rdfs:isDefinedBy <http://rdaregistry.info/Elements/u/> ;
    rdfs:label "has tape configuration"@en ;
    rdfs:subPropertyOf <http://rdaregistry.info/Elements/u/P60351> ;
    skos:definition "Relates a resource to a number of tracks on an audiotape."@en .

<http://rdaregistry.info/Elements/u/P60554>
    reg:hasSubproperty <http://rdaregistry.info/Elements/m/P30186> ;
    reg:lexicalAlias <http://rdaregistry.info/Elements/u/mount.en> ;
    reg:name "mount"@en ;
    reg:status <http://metadataregistry.org/uri/RegStatus/1001> ;
    a rdf:Property ;
    rdfs:isDefinedBy <http://rdaregistry.info/Elements/u/> ;
    rdfs:label "has mount"@en ;
    skos:definition "Relates a resource to a physical material used for the support or backing to which the base material of a resource has been attached."@en .

<http://rdaregistry.info/Elements/u/P60555>
    reg:hasSubproperty <http://rdaregistry.info/Elements/e/P20217> ;
    reg:lexicalAlias <http://rdaregistry.info/Elements/u/captureInformation.en> ;
    reg:name "captureInformation"@en ;
    reg:status <http://metadataregistry.org/uri/RegStatus/1001> ;
    a rdf:Property ;
    rdfs:isDefinedBy <http://rdaregistry.info/Elements/u/> ;
    rdfs:label "has capture information"@en ;
    skos:definition "Relates a resource to a place, date, or other information associated with the recording, filming, etc., of the content of a resource."@en .

<http://rdaregistry.info/Elements/u/P60556>
    reg:hasSubproperty <http://rdaregistry.info/Elements/e/P20218> ;
    reg:lexicalAlias <http://rdaregistry.info/Elements/u/placeOfCapture.en> ;
    reg:name "placeOfCapture"@en ;
    reg:status <http://metadataregistry.org/uri/RegStatus/1001> ;
    a rdf:Property ;
    rdfs:isDefinedBy <http://rdaregistry.info/Elements/u/> ;
    rdfs:label "has place of capture"@en ;
    skos:definition "Relates a resource to a place associated with the capture (i.e., recording, filming, etc.) of the content of a resource."@en .

<http://rdaregistry.info/Elements/u/P60557>
    reg:hasSubproperty <http://rdaregistry.info/Elements/e/P20219> ;
    reg:lexicalAlias <http://rdaregistry.info/Elements/u/duration.en> ;
    reg:name "duration"@en ;
    reg:status <http://metadataregistry.org/uri/RegStatus/1001> ;
    a rdf:Property ;
    rdfs:isDefinedBy <http://rdaregistry.info/Elements/u/> ;
    rdfs:label "has duration"@en ;
    skos:definition "Relates a resource to a playing time, running time, etc., of a content of a resource."@en .

<http://rdaregistry.info/Elements/u/P60558>
    reg:hasSubproperty <http://rdaregistry.info/Elements/e/P20224> ;
    reg:lexicalAlias <http://rdaregistry.info/Elements/u/colourContent.en> ;
    reg:name "colourContent"@en ;
    reg:status <http://metadataregistry.org/uri/RegStatus/1001> ;
    a rdf:Property ;
    rdfs:isDefinedBy <http://rdaregistry.info/Elements/u/> ;
    rdfs:label "has colour content"@en ;
    skos:definition "Relates a resource to a presence of colour, tone, etc., in the content of a resource."@en ;
    skos:scopeNote "Black, white, single colour shades of black, single colour tints of white, and single colour tones of gray are considered to be single colours."@en .

<http://rdaregistry.info/Elements/u/P60559>
    reg:hasSubproperty <http://rdaregistry.info/Elements/e/P20225> ;
    reg:lexicalAlias <http://rdaregistry.info/Elements/u/soundContent.en> ;
    reg:name "soundContent"@en ;
    reg:status <http://metadataregistry.org/uri/RegStatus/1001> ;
    a rdf:Property ;
    rdfs:isDefinedBy <http://rdaregistry.info/Elements/u/> ;
    rdfs:label "has sound content"@en ;
    skos:definition "Relates a resource to a presence or absence of sound in a resource."@en .

<http://rdaregistry.info/Elements/u/P60560>
    reg:hasSubproperty <http://rdaregistry.info/Elements/m/P30187>, <http://rdaregistry.info/Elements/u/P60561>, <http://rdaregistry.info/Elements/u/P60562> ;
    reg:lexicalAlias <http://rdaregistry.info/Elements/u/productionMethod.en> ;
    reg:name "productionMethod"@en ;
    reg:status <http://metadataregistry.org/uri/RegStatus/1001> ;
    a rdf:Property ;
    rdfs:isDefinedBy <http://rdaregistry.info/Elements/u/> ;
    rdfs:label "has production method"@en ;
    skos:definition "Relates a resource to a process used to produce a resource."@en .

<http://rdaregistry.info/Elements/u/P60561>
    reg:hasSubproperty <http://rdaregistry.info/Elements/m/P30188> ;
    reg:lexicalAlias <http://rdaregistry.info/Elements/u/productionMethodForTactileResource.en> ;
    reg:name "productionMethodForTactileResource"@en ;
    reg:status <http://metadataregistry.org/uri/RegStatus/1008> ;
    a rdf:Property ;
    rdfs:isDefinedBy <http://rdaregistry.info/Elements/u/> ;
    rdfs:subPropertyOf <http://rdaregistry.info/Elements/u/P60560> ;
    skos:definition "Relates a resource to the process used to produce a tactile resource (e.g., embossing, thermoform)."@en .

<http://rdaregistry.info/Elements/u/P60562>
    reg:hasSubproperty <http://rdaregistry.info/Elements/m/P30189> ;
    reg:lexicalAlias <http://rdaregistry.info/Elements/u/productionMethodForManuscript.en> ;
    reg:name "productionMethodForManuscript"@en ;
    reg:status <http://metadataregistry.org/uri/RegStatus/1008> ;
    a rdf:Property ;
    rdfs:isDefinedBy <http://rdaregistry.info/Elements/u/> ;
    rdfs:subPropertyOf <http://rdaregistry.info/Elements/u/P60560> ;
    skos:definition "Relates a resource to the process used to produce an original manuscript or a copy."@en .

<http://rdaregistry.info/Elements/u/P60563>
    reg:hasSubproperty <http://rdaregistry.info/Elements/e/P20226> ;
    reg:lexicalAlias <http://rdaregistry.info/Elements/u/horizontalScaleOfCartographicContent.en> ;
    reg:name "horizontalScaleOfCartographicContent"@en ;
    reg:status <http://metadataregistry.org/uri/RegStatus/1001> ;
    a rdf:Property ;
    rdfs:isDefinedBy <http://rdaregistry.info/Elements/u/> ;
    rdfs:label "has horizontal scale of cartographic content"@en ;
    rdfs:subPropertyOf <http://rdaregistry.info/Elements/u/P60565> ;
    skos:definition "Relates a resource to a ratio of horizontal distances in the cartographic content of a resource to the actual distances they represent."@en .

<http://rdaregistry.info/Elements/u/P60564>
    reg:hasSubproperty <http://rdaregistry.info/Elements/e/P20227> ;
    reg:lexicalAlias <http://rdaregistry.info/Elements/u/scaleOfStillImageOrThreeDimensionalForm.en> ;
    reg:name "scaleOfStillImageOrThreeDimensionalForm"@en ;
    reg:status <http://metadataregistry.org/uri/RegStatus/1001> ;
    a rdf:Property ;
    rdfs:isDefinedBy <http://rdaregistry.info/Elements/u/> ;
    rdfs:label "has scale of still image or three-dimensional form"@en ;
    rdfs:subPropertyOf <http://rdaregistry.info/Elements/u/P60565> ;
    skos:definition "Relates a resource to a ratio of the dimensions of a still image or three-dimensional form contained or embodied in a resource to the dimensions of the thing it represents."@en .

<http://rdaregistry.info/Elements/u/P60565>
    reg:hasSubproperty <http://rdaregistry.info/Elements/e/P20228>, <http://rdaregistry.info/Elements/u/P60510>, <http://rdaregistry.info/Elements/u/P60563>, <http://rdaregistry.info/Elements/u/P60564>, <http://rdaregistry.info/Elements/u/P60579> ;
    reg:lexicalAlias <http://rdaregistry.info/Elements/u/scale.en> ;
    reg:name "scale"@en ;
    reg:status <http://metadataregistry.org/uri/RegStatus/1001> ;
    a rdf:Property ;
    rdfs:isDefinedBy <http://rdaregistry.info/Elements/u/> ;
    rdfs:label "has scale"@en ;
    skos:definition "Relates a resource to a ratio of the dimensions of the content of an image or three-dimensional form to the dimensions of the thing it represents"@en ;
    skos:scopeNote "Scale can apply to horizontal, vertical, angular, and/or other measurements represented in the resource."@en .

<http://rdaregistry.info/Elements/u/P60566>
    reg:hasSubproperty <http://rdaregistry.info/Elements/e/P20229> ;
    reg:lexicalAlias <http://rdaregistry.info/Elements/u/aspectRatio.en> ;
    reg:name "aspectRatio"@en ;
    reg:status <http://metadataregistry.org/uri/RegStatus/1001> ;
    a rdf:Property ;
    rdfs:isDefinedBy <http://rdaregistry.info/Elements/u/> ;
    rdfs:label "has aspect ratio"@en ;
    skos:definition "Relates a resource to a numerical ratio of the width to the height of a moving image."@en .

<http://rdaregistry.info/Elements/u/P60567>
    reg:hasSubproperty <http://rdaregistry.info/Elements/m/P30190> ;
    reg:lexicalAlias <http://rdaregistry.info/Elements/u/generationOfAudioRecording.en> ;
    reg:name "generationOfAudioRecording"@en ;
    reg:status <http://metadataregistry.org/uri/RegStatus/1008> ;
    a rdf:Property ;
    rdfs:isDefinedBy <http://rdaregistry.info/Elements/u/> ;
    rdfs:subPropertyOf <http://rdaregistry.info/Elements/u/P60568> ;
    skos:definition "Relates a resource to the relationship between an original audio carrier and the carrier of a reproduction made from the original (e.g., a tape duplication master, a test pressing)."@en .

<http://rdaregistry.info/Elements/u/P60568>
    reg:hasSubproperty <http://rdaregistry.info/Elements/m/P30191>, <http://rdaregistry.info/Elements/u/P60567>, <http://rdaregistry.info/Elements/u/P60569>, <http://rdaregistry.info/Elements/u/P60570>, <http://rdaregistry.info/Elements/u/P60571>, <http://rdaregistry.info/Elements/u/P60572> ;
    reg:lexicalAlias <http://rdaregistry.info/Elements/u/generation.en> ;
    reg:name "generation"@en ;
    reg:status <http://metadataregistry.org/uri/RegStatus/1001> ;
    a rdf:Property ;
    rdfs:isDefinedBy <http://rdaregistry.info/Elements/u/> ;
    rdfs:label "has generation"@en ;
    skos:definition "Relates a resource to a relationship between an original carrier and a carrier of a reproduction made from an original."@en .

<http://rdaregistry.info/Elements/u/P60569>
    reg:hasSubproperty <http://rdaregistry.info/Elements/m/P30192> ;
    reg:lexicalAlias <http://rdaregistry.info/Elements/u/generationOfDigitalResource.en> ;
    reg:name "generationOfDigitalResource"@en ;
    reg:status <http://metadataregistry.org/uri/RegStatus/1008> ;
    a rdf:Property ;
    rdfs:isDefinedBy <http://rdaregistry.info/Elements/u/> ;
    rdfs:subPropertyOf <http://rdaregistry.info/Elements/u/P60568> ;
    skos:definition "Relates a resource to the relationship between an original carrier of a digital resource and the carrier of a reproduction made from the original (e.g., a derivative master)."@en .

<http://rdaregistry.info/Elements/u/P60570>
    reg:hasSubproperty <http://rdaregistry.info/Elements/m/P30193> ;
    reg:lexicalAlias <http://rdaregistry.info/Elements/u/generationOfMotionPictureFilm.en> ;
    reg:name "generationOfMotionPictureFilm"@en ;
    reg:status <http://metadataregistry.org/uri/RegStatus/1008> ;
    a rdf:Property ;
    rdfs:isDefinedBy <http://rdaregistry.info/Elements/u/> ;
    rdfs:subPropertyOf <http://rdaregistry.info/Elements/u/P60568> ;
    skos:definition "Relates a resource to the relationship between an original carrier of a motion picture film resource and the carrier of a reproduction made from the original (e.g., a reference print)."@en .

<http://rdaregistry.info/Elements/u/P60571>
    reg:hasSubproperty <http://rdaregistry.info/Elements/m/P30194> ;
    reg:lexicalAlias <http://rdaregistry.info/Elements/u/generationOfVideotape.en> ;
    reg:name "generationOfVideotape"@en ;
    reg:status <http://metadataregistry.org/uri/RegStatus/1008> ;
    a rdf:Property ;
    rdfs:isDefinedBy <http://rdaregistry.info/Elements/u/> ;
    rdfs:subPropertyOf <http://rdaregistry.info/Elements/u/P60568> ;
    skos:definition "Relates a resource to the relationship between an original carrier of a videotape resource and the carrier of a reproduction made from the original (e.g., a show copy)."@en .

<http://rdaregistry.info/Elements/u/P60572>
    reg:hasSubproperty <http://rdaregistry.info/Elements/m/P30195> ;
    reg:lexicalAlias <http://rdaregistry.info/Elements/u/generationOfMicroform.en> ;
    reg:name "generationOfMicroform"@en ;
    reg:status <http://metadataregistry.org/uri/RegStatus/1008> ;
    a rdf:Property ;
    rdfs:isDefinedBy <http://rdaregistry.info/Elements/u/> ;
    rdfs:subPropertyOf <http://rdaregistry.info/Elements/u/P60568> ;
    skos:definition "Relates a resource to the relationship between an original microform carrier and the carrier of a reproduction made from the original (e.g., a printing master)."@en .

<http://rdaregistry.info/Elements/u/P60573>
    reg:hasSubproperty <http://rdaregistry.info/Elements/m/P30196> ;
    reg:lexicalAlias <http://rdaregistry.info/Elements/u/polarity.en> ;
    reg:name "polarity"@en ;
    reg:status <http://metadataregistry.org/uri/RegStatus/1001> ;
    a rdf:Property ;
    rdfs:isDefinedBy <http://rdaregistry.info/Elements/u/> ;
    rdfs:label "has polarity"@en ;
    skos:definition "Relates a resource to a relationship of the colours and tones in an image to the colours and tones of the object reproduced."@en .

<http://rdaregistry.info/Elements/u/P60574>
    reg:hasSubproperty <http://rdaregistry.info/Elements/e/P20137> ;
    reg:lexicalAlias <http://rdaregistry.info/Elements/u/absorptionOf.en> ;
    reg:name "absorptionOf"@en ;
    reg:status <http://metadataregistry.org/uri/RegStatus/1001> ;
    a rdf:Property ;
    rdfs:isDefinedBy <http://rdaregistry.info/Elements/u/> ;
    rdfs:label "is absorption of"@en ;
    rdfs:subPropertyOf <http://rdaregistry.info/Elements/u/P60261> ;
    owl:inverseOf <http://rdaregistry.info/Elements/u/P60247> ;
    skos:definition "Relates a resource to a resource that has been incorporated into another resource."@en .

<http://rdaregistry.info/Elements/u/P60575>
    reg:hasSubproperty <http://rdaregistry.info/Elements/e/P20138> ;
    reg:lexicalAlias <http://rdaregistry.info/Elements/u/absorptionInPartOf.en> ;
    reg:name "absorptionInPartOf"@en ;
    reg:status <http://metadataregistry.org/uri/RegStatus/1001> ;
    a rdf:Property ;
    rdfs:isDefinedBy <http://rdaregistry.info/Elements/u/> ;
    rdfs:label "is absorption in part of"@en ;
    rdfs:subPropertyOf <http://rdaregistry.info/Elements/u/P60261> ;
    owl:inverseOf <http://rdaregistry.info/Elements/u/P60248> ;
    skos:definition "Relates a resource to a resource that has been partially incorporated into another resource."@en .

<http://rdaregistry.info/Elements/u/P60576>
    reg:hasSubproperty <http://rdaregistry.info/Elements/e/P20149> ;
    reg:lexicalAlias <http://rdaregistry.info/Elements/u/continuationOf.en> ;
    reg:name "continuationOf"@en ;
    reg:status <http://metadataregistry.org/uri/RegStatus/1001> ;
    a rdf:Property ;
    rdfs:isDefinedBy <http://rdaregistry.info/Elements/u/> ;
    rdfs:label "is continuation of"@en ;
    rdfs:subPropertyOf <http://rdaregistry.info/Elements/u/P60261> ;
    owl:inverseOf <http://rdaregistry.info/Elements/u/P60306> ;
    skos:definition "Relates a resource to a resource that is continued by the content of a later resource."@en ;
    skos:scopeNote "This relationship applies generally to serials."@en .

<http://rdaregistry.info/Elements/u/P60577>
    reg:lexicalAlias <http://rdaregistry.info/Elements/u/sequelTo.en> ;
    reg:name "sequelTo"@en ;
    reg:status <http://metadataregistry.org/uri/RegStatus/1001> ;
    a rdf:Property ;
    rdfs:isDefinedBy <http://rdaregistry.info/Elements/u/> ;
    rdfs:label "is sequel to"@en ;
    rdfs:subPropertyOf <http://rdaregistry.info/Elements/u/P60261> ;
    owl:inverseOf <http://rdaregistry.info/Elements/u/P60102> ;
    skos:definition "Relates a resource to a resource whose narrative is continued by a later resource."@en .

<http://rdaregistry.info/Elements/u/P60578>
    reg:hasSubproperty <http://rdaregistry.info/Elements/m/P30197> ;
    reg:lexicalAlias <http://rdaregistry.info/Elements/u/bibliographicFormat.en> ;
    reg:name "bibliographicFormat"@en ;
    reg:status <http://metadataregistry.org/uri/RegStatus/1001> ;
    a rdf:Property ;
    rdfs:isDefinedBy <http://rdaregistry.info/Elements/u/> ;
    rdfs:label "has bibliographic format"@en ;
    skos:definition "Relates a resource to a proportional relationship between a whole sheet in a printed or manuscript resource, and the individual leaves that result if that sheet is left full, cut, or folded."@en .

<http://rdaregistry.info/Elements/u/P60579>
    reg:hasSubproperty <http://rdaregistry.info/Elements/e/P20230> ;
    reg:lexicalAlias <http://rdaregistry.info/Elements/u/verticalScaleOfCartographicContent.en> ;
    reg:name "verticalScaleOfCartographicContent"@en ;
    reg:status <http://metadataregistry.org/uri/RegStatus/1001> ;
    a rdf:Property ;
    rdfs:isDefinedBy <http://rdaregistry.info/Elements/u/> ;
    rdfs:label "has vertical scale of cartographic content"@en ;
    rdfs:subPropertyOf <http://rdaregistry.info/Elements/u/P60565> ;
    skos:definition "Relates a resource to a scale of elevation or vertical dimension of the cartographic content of a resource."@en .

<http://rdaregistry.info/Elements/u/P60580>
    reg:lexicalAlias <http://rdaregistry.info/Elements/u/key.en> ;
    reg:name "key"@en ;
    reg:status <http://metadataregistry.org/uri/RegStatus/1001> ;
    a rdf:Property ;
    rdfs:isDefinedBy <http://rdaregistry.info/Elements/u/> ;
    rdfs:label "has key"@en ;
    skos:definition "Relates a resource to a set of pitch relationships that establishes a tonal centre, or principal tonal centre, of a musical resource."@en .

<http://rdaregistry.info/Elements/u/P60581>
    reg:hasSubproperty <http://rdaregistry.info/Elements/m/P30198> ;
    reg:lexicalAlias <http://rdaregistry.info/Elements/u/reductionRatio.en> ;
    reg:name "reductionRatio"@en ;
    reg:status <http://metadataregistry.org/uri/RegStatus/1001> ;
    a rdf:Property ;
    rdfs:isDefinedBy <http://rdaregistry.info/Elements/u/> ;
    rdfs:label "has reduction ratio"@en ;
    skos:definition "Relates a resource to a numerical ratio of the size of a micro-image in relation to an original from which it was produced."@en .

<http://rdaregistry.info/Elements/u/P60582>
    reg:hasSubproperty <http://rdaregistry.info/Elements/m/P30199> ;
    reg:lexicalAlias <http://rdaregistry.info/Elements/u/fontSize.en> ;
    reg:name "fontSize"@en ;
    reg:status <http://metadataregistry.org/uri/RegStatus/1001> ;
    a rdf:Property ;
    rdfs:isDefinedBy <http://rdaregistry.info/Elements/u/> ;
    rdfs:label "has font size"@en ;
    skos:definition "Relates a resource to a size of the type used to represent characters and symbols in a resource."@en .

<http://rdaregistry.info/Elements/u/P60583>
    reg:hasSubproperty <http://rdaregistry.info/Elements/i/P40050> ;
    reg:lexicalAlias <http://rdaregistry.info/Elements/u/immediateSourceOfAcquisitionOfResource.en> ;
    reg:name "immediateSourceOfAcquisitionOfResource"@en ;
    reg:status <http://metadataregistry.org/uri/RegStatus/1001> ;
    a rdf:Property ;
    rdfs:isDefinedBy <http://rdaregistry.info/Elements/u/> ;
    rdfs:label "has immediate source of acquisition of resource"@en ;
    skos:definition "Relates a resource to a source from which an agency directly acquired a resource and the circumstances under which it was received."@en .

<http://rdaregistry.info/Elements/u/P60584>
    reg:lexicalAlias <http://rdaregistry.info/Elements/u/natureOfContent.en> ;
    reg:name "natureOfContent"@en ;
    reg:status <http://metadataregistry.org/uri/RegStatus/1001> ;
    a rdf:Property ;
    rdfs:isDefinedBy <http://rdaregistry.info/Elements/u/> ;
    rdfs:label "has nature of content"@en ;
    skos:definition "Relates a resource to a specific character of a primary content of a resource."@en .

<http://rdaregistry.info/Elements/u/P60585>
    reg:hasSubproperty <http://rdaregistry.info/Elements/m/P30200> ;
    reg:lexicalAlias <http://rdaregistry.info/Elements/u/projectionSpeed.en> ;
    reg:name "projectionSpeed"@en ;
    reg:status <http://metadataregistry.org/uri/RegStatus/1001> ;
    a rdf:Property ;
    rdfs:isDefinedBy <http://rdaregistry.info/Elements/u/> ;
    rdfs:label "has projection speed"@en ;
    rdfs:subPropertyOf <http://rdaregistry.info/Elements/u/P60353> ;
    skos:definition "Relates a resource to a speed at which a projected carrier must be operated to produce the moving image intended."@en .

<http://rdaregistry.info/Elements/u/P60586>
    reg:hasSubproperty <http://rdaregistry.info/Elements/m/P30201> ;
    reg:lexicalAlias <http://rdaregistry.info/Elements/u/playingSpeed.en> ;
    reg:name "playingSpeed"@en ;
    reg:status <http://metadataregistry.org/uri/RegStatus/1001> ;
    a rdf:Property ;
    rdfs:isDefinedBy <http://rdaregistry.info/Elements/u/> ;
    rdfs:label "has playing speed"@en ;
    rdfs:subPropertyOf <http://rdaregistry.info/Elements/u/P60351> ;
    skos:definition "Relates a resource to a speed at which an audio carrier must be operated to produce the sound intended."@en .

<http://rdaregistry.info/Elements/u/P60587>
    reg:hasSubproperty <http://rdaregistry.info/Elements/m/P30202> ;
    reg:lexicalAlias <http://rdaregistry.info/Elements/u/encodedBitrate.en> ;
    reg:name "encodedBitrate"@en ;
    reg:status <http://metadataregistry.org/uri/RegStatus/1001> ;
    a rdf:Property ;
    rdfs:isDefinedBy <http://rdaregistry.info/Elements/u/> ;
    rdfs:label "has encoded bitrate"@en ;
    rdfs:subPropertyOf <http://rdaregistry.info/Elements/u/P60350> ;
    owl:inverseOf <http://rdaregistry.info/Elements/u/P60858> ;
    skos:definition "Relates a resource to a speed at which streaming audio, video, etc., is designed to play."@en .

<http://rdaregistry.info/Elements/u/P60588>
    reg:lexicalAlias <http://rdaregistry.info/Elements/u/preferredTitleForResource.en> ;
    reg:name "preferredTitleForResource"@en ;
    reg:status <http://metadataregistry.org/uri/RegStatus/1001> ;
    a rdf:Property ;
    rdfs:isDefinedBy <http://rdaregistry.info/Elements/u/> ;
    rdfs:label "has preferred title for resource"@en ;
    rdfs:subPropertyOf <http://rdaregistry.info/Elements/u/P60367> ;
    owl:inverseOf <http://rdaregistry.info/Elements/u/P60857> ;
    skos:definition "Relates a resource to a title or form of title chosen to identify a resource."@en .

<http://rdaregistry.info/Elements/u/P60589>
    reg:hasSubproperty <http://rdaregistry.info/Elements/m/P30203> ;
    reg:lexicalAlias <http://rdaregistry.info/Elements/u/parallelTitleProper.en> ;
    reg:name "parallelTitleProper"@en ;
    reg:status <http://metadataregistry.org/uri/RegStatus/1001> ;
    a rdf:Property ;
    rdfs:isDefinedBy <http://rdaregistry.info/Elements/u/> ;
    rdfs:label "has parallel title proper"@en ;
    rdfs:subPropertyOf <http://rdaregistry.info/Elements/u/P60369> ;
    skos:definition "Relates a resource to a title proper in another language or script."@en ;
    skos:scopeNote "An alternative title in another language and/or script is treated as part of the parallel title proper."@en .

<http://rdaregistry.info/Elements/u/P60590>
    reg:hasSubproperty <http://rdaregistry.info/Elements/m/P30204> ;
    reg:lexicalAlias <http://rdaregistry.info/Elements/u/parallelTitleProperOfSeries.en> ;
    reg:name "parallelTitleProperOfSeries"@en ;
    reg:status <http://metadataregistry.org/uri/RegStatus/1001> ;
    a rdf:Property ;
    rdfs:isDefinedBy <http://rdaregistry.info/Elements/u/> ;
    rdfs:label "has parallel title proper of series"@en ;
    skos:definition "Relates a resource to a title proper of a series in another language or script."@en .

<http://rdaregistry.info/Elements/u/P60591>
    reg:hasSubproperty <http://rdaregistry.info/Elements/m/P30205> ;
    reg:lexicalAlias <http://rdaregistry.info/Elements/u/parallelTitleProperOfSubseries.en> ;
    reg:name "parallelTitleProperOfSubseries"@en ;
    reg:status <http://metadataregistry.org/uri/RegStatus/1001> ;
    a rdf:Property ;
    rdfs:isDefinedBy <http://rdaregistry.info/Elements/u/> ;
    rdfs:label "has parallel title proper of subseries"@en ;
    skos:definition "Relates a resource to a title proper of a subseries in another language or script."@en .

<http://rdaregistry.info/Elements/u/P60592>
    reg:hasSubproperty <http://rdaregistry.info/Elements/a/P50118> ;
    reg:lexicalAlias <http://rdaregistry.info/Elements/u/placeOfDeath.en> ;
    reg:name "placeOfDeath"@en ;
    reg:status <http://metadataregistry.org/uri/RegStatus/1001> ;
    a rdf:Property ;
    rdfs:isDefinedBy <http://rdaregistry.info/Elements/u/> ;
    rdfs:label "has place of death"@en ;
    skos:definition "Relates a resource to a town, city, province, state, or country in which an agent died."@en .

<http://rdaregistry.info/Elements/u/P60593>
    reg:hasSubproperty <http://rdaregistry.info/Elements/a/P50119> ;
    reg:lexicalAlias <http://rdaregistry.info/Elements/u/placeOfBirth.en> ;
    reg:name "placeOfBirth"@en ;
    reg:status <http://metadataregistry.org/uri/RegStatus/1001> ;
    a rdf:Property ;
    rdfs:isDefinedBy <http://rdaregistry.info/Elements/u/> ;
    rdfs:label "has place of birth"@en ;
    skos:definition "Relates a resource to a town, city, province, state, or country in which an agent was born."@en .

<http://rdaregistry.info/Elements/u/P60594>
    reg:hasSubproperty <http://rdaregistry.info/Elements/m/P30206> ;
    reg:lexicalAlias <http://rdaregistry.info/Elements/u/recordingMedium.en> ;
    reg:name "recordingMedium"@en ;
    reg:status <http://metadataregistry.org/uri/RegStatus/1001> ;
    a rdf:Property ;
    rdfs:isDefinedBy <http://rdaregistry.info/Elements/u/> ;
    rdfs:label "has recording medium"@en ;
    rdfs:subPropertyOf <http://rdaregistry.info/Elements/u/P60351> ;
    skos:definition "Relates a resource to a type of medium used to record sound on an audio carrier."@en .

<http://rdaregistry.info/Elements/u/P60595>
    reg:status <http://metadataregistry.org/uri/RegStatus/1008> ;
    rdfs:isDefinedBy <http://rdaregistry.info/Elements/u/> .

<http://rdaregistry.info/Elements/u/P60596>
    reg:hasSubproperty <http://rdaregistry.info/Elements/m/P30208> ;
    reg:lexicalAlias <http://rdaregistry.info/Elements/u/baseMaterial.en> ;
    reg:name "baseMaterial"@en ;
    reg:status <http://metadataregistry.org/uri/RegStatus/1001> ;
    a rdf:Property ;
    rdfs:isDefinedBy <http://rdaregistry.info/Elements/u/> ;
    rdfs:label "has base material"@en ;
    skos:definition "Relates a resource to an underlying physical material of a resource."@en .

<http://rdaregistry.info/Elements/u/P60597>
    reg:hasSubproperty <http://rdaregistry.info/Elements/m/P30209> ;
    reg:lexicalAlias <http://rdaregistry.info/Elements/u/keyTitle.en> ;
    reg:name "keyTitle"@en ;
    reg:status <http://metadataregistry.org/uri/RegStatus/1001> ;
    a rdf:Property ;
    rdfs:isDefinedBy <http://rdaregistry.info/Elements/u/> ;
    rdfs:label "has key title"@en ;
    rdfs:subPropertyOf <http://rdaregistry.info/Elements/u/P60369> ;
    skos:definition "Relates a resource to a unique name assigned to a resource by an ISSN registration agency."@en .

<http://rdaregistry.info/Elements/u/P60598>
    reg:hasSubproperty <http://rdaregistry.info/Elements/a/P50120> ;
    reg:lexicalAlias <http://rdaregistry.info/Elements/u/dateOfDeath.en> ;
    reg:name "dateOfDeath"@en ;
    reg:status <http://metadataregistry.org/uri/RegStatus/1001> ;
    a rdf:Property ;
    rdfs:isDefinedBy <http://rdaregistry.info/Elements/u/> ;
    rdfs:label "has date of death"@en ;
    rdfs:subPropertyOf <http://rdaregistry.info/Elements/u/P60324> ;
    skos:definition "Relates a resource to a year an agent died."@en .

<http://rdaregistry.info/Elements/u/P60599>
    reg:hasSubproperty <http://rdaregistry.info/Elements/a/P50121> ;
    reg:lexicalAlias <http://rdaregistry.info/Elements/u/dateOfBirth.en> ;
    reg:name "dateOfBirth"@en ;
    reg:status <http://metadataregistry.org/uri/RegStatus/1001> ;
    a rdf:Property ;
    rdfs:isDefinedBy <http://rdaregistry.info/Elements/u/> ;
    rdfs:label "has date of birth"@en ;
    rdfs:subPropertyOf <http://rdaregistry.info/Elements/u/P60324> ;
    skos:definition "Relates a resource to a year an agent was born."@en .

<http://rdaregistry.info/Elements/u/P60600>
    rdakit:seeAlso <http://rdaregistry.info/Elements/u/P60707> ;
    reg:hasSubproperty <http://rdaregistry.info/Elements/a/P50216> ;
    reg:lexicalAlias <http://rdaregistry.info/Elements/u/writerOfAddedLyricsOf.en> ;
    reg:name "writerOfAddedLyricsOf"@en ;
    reg:status <http://metadataregistry.org/uri/RegStatus/1001> ;
    a rdf:Property ;
    rdfs:isDefinedBy <http://rdaregistry.info/Elements/u/> ;
    rdfs:label "is writer of added lyrics of"@en ;
    rdfs:subPropertyOf <http://rdaregistry.info/Elements/u/P60608> ;
    owl:inverseOf <http://rdaregistry.info/Elements/u/P60371> ;
    skos:definition "Relates a writer of words added to a musical resource to a resource."@en ;
    skos:scopeNote "Writing of lyrics in collaboration with a composer to form an original resource is excluded."@en .

<http://rdaregistry.info/Elements/u/P60601>
    reg:hasSubproperty <http://rdaregistry.info/Elements/a/P50002>, <http://rdaregistry.info/Elements/a/P50085>, <http://rdaregistry.info/Elements/a/P50087> ;
    reg:lexicalAlias <http://rdaregistry.info/Elements/u/appelleeOf.en> ;
    reg:name "appelleeOf"@en ;
    reg:status <http://metadataregistry.org/uri/RegStatus/1001> ;
    a rdf:Property ;
    rdfs:isDefinedBy <http://rdaregistry.info/Elements/u/> ;
    rdfs:label "is appellee of"@en ;
    rdfs:subPropertyOf <http://rdaregistry.info/Elements/u/P60602> ;
    owl:inverseOf <http://rdaregistry.info/Elements/u/P60373> ;
    skos:definition "Relates an agent against whom an appeal is taken on a decision of a lower court recorded in a legal resource of a higher court to a resource."@en .

<http://rdaregistry.info/Elements/u/P60602>
    reg:hasSubproperty <http://rdaregistry.info/Elements/a/P50131>, <http://rdaregistry.info/Elements/a/P50181>, <http://rdaregistry.info/Elements/a/P50182>, <http://rdaregistry.info/Elements/u/P60002>, <http://rdaregistry.info/Elements/u/P60003>, <http://rdaregistry.info/Elements/u/P60004>, <http://rdaregistry.info/Elements/u/P60005>, <http://rdaregistry.info/Elements/u/P60015>, <http://rdaregistry.info/Elements/u/P60032>, <http://rdaregistry.info/Elements/u/P60601>, <http://rdaregistry.info/Elements/u/P60603>, <http://rdaregistry.info/Elements/u/P60604>, <http://rdaregistry.info/Elements/u/P60634>, <http://rdaregistry.info/Elements/u/P60650>, <http://rdaregistry.info/Elements/u/P60668>, <http://rdaregistry.info/Elements/u/P60673>, <http://rdaregistry.info/Elements/u/P60674>, <http://rdaregistry.info/Elements/u/P60675>, <http://rdaregistry.info/Elements/u/P60678>, <http://rdaregistry.info/Elements/u/P60689>, <http://rdaregistry.info/Elements/u/P60690>, <http://rdaregistry.info/Elements/u/P60691>, <http://rdaregistry.info/Elements/u/P60692>, <http://rdaregistry.info/Elements/u/P60693>, <http://rdaregistry.info/Elements/u/P60695>, <http://rdaregistry.info/Elements/u/P60696>, <http://rdaregistry.info/Elements/u/P60698>, <http://rdaregistry.info/Elements/u/P60700>, <http://rdaregistry.info/Elements/u/P60702>, <http://rdaregistry.info/Elements/u/P60703>, <http://rdaregistry.info/Elements/u/P60816>, <http://rdaregistry.info/Elements/u/P60835>, <http://rdaregistry.info/Elements/u/P60837>, <http://rdaregistry.info/Elements/u/P60850>, <http://rdaregistry.info/Elements/u/P60870>, <http://rdaregistry.info/Elements/u/P60872> ;
    reg:lexicalAlias <http://rdaregistry.info/Elements/u/otherAgentAssociatedWithResourceOf.en> ;
    reg:name "otherAgentAssociatedWithResourceOf"@en ;
    reg:status <http://metadataregistry.org/uri/RegStatus/1001> ;
    a rdf:Property ;
    rdfs:isDefinedBy <http://rdaregistry.info/Elements/u/> ;
    rdfs:label "is other agent associated with resource of"@en ;
    owl:inverseOf <http://rdaregistry.info/Elements/u/P60374> ;
    skos:definition "Relates an agent other than a creator, custodian, owner, producer, publisher, distributor or manufacturer associated with a resource to a resource."@en .

<http://rdaregistry.info/Elements/u/P60603>
    reg:hasSubproperty <http://rdaregistry.info/Elements/a/P50132> ;
    reg:lexicalAlias <http://rdaregistry.info/Elements/u/dedicatorOf.en> ;
    reg:name "dedicatorOf"@en ;
    reg:status <http://metadataregistry.org/uri/RegStatus/1001> ;
    a rdf:Property ;
    rdfs:isDefinedBy <http://rdaregistry.info/Elements/u/> ;
    rdfs:label "is dedicator of"@en ;
    rdfs:subPropertyOf <http://rdaregistry.info/Elements/u/P60602> ;
    owl:inverseOf <http://rdaregistry.info/Elements/u/P60375> ;
    skos:definition "Relates an agent by whom a resource is dedicated to a resource."@en .

<http://rdaregistry.info/Elements/u/P60604>
    reg:hasSubproperty <http://rdaregistry.info/Elements/a/P50133>, <http://rdaregistry.info/Elements/u/P60006>, <http://rdaregistry.info/Elements/u/P60007> ;
    reg:lexicalAlias <http://rdaregistry.info/Elements/u/curatorOf.en> ;
    reg:name "curatorOf"@en ;
    reg:status <http://metadataregistry.org/uri/RegStatus/1001> ;
    a rdf:Property ;
    rdfs:isDefinedBy <http://rdaregistry.info/Elements/u/> ;
    rdfs:label "is curator of"@en ;
    rdfs:subPropertyOf <http://rdaregistry.info/Elements/u/P60602> ;
    owl:inverseOf <http://rdaregistry.info/Elements/u/P60376> ;
    skos:definition "Relates an agent conceiving, aggregating, or organizing an exhibition, collection, or other resource to a resource."@en .

<http://rdaregistry.info/Elements/u/P60605>
    reg:hasSubproperty <http://rdaregistry.info/Elements/a/P50135> ;
    reg:lexicalAlias <http://rdaregistry.info/Elements/u/surveyorOf.en> ;
    reg:name "surveyorOf"@en ;
    reg:status <http://metadataregistry.org/uri/RegStatus/1001> ;
    a rdf:Property ;
    rdfs:isDefinedBy <http://rdaregistry.info/Elements/u/> ;
    rdfs:label "is surveyor of"@en ;
    rdfs:subPropertyOf <http://rdaregistry.info/Elements/u/P60626> ;
    owl:inverseOf <http://rdaregistry.info/Elements/u/P60377> ;
    skos:definition "Relates an agent contributing to a cartographic resource by providing measurements or dimensional relationships for a geographic area represented to a resource."@en .

<http://rdaregistry.info/Elements/u/P60606>
    rdakit:seeAlso <http://rdaregistry.info/Elements/u/P60660> ;
    reg:hasSubproperty <http://rdaregistry.info/Elements/a/P50136> ;
    reg:lexicalAlias <http://rdaregistry.info/Elements/u/animatorOf.en> ;
    reg:name "animatorOf"@en ;
    reg:status <http://metadataregistry.org/uri/RegStatus/1001> ;
    a rdf:Property ;
    rdfs:isDefinedBy <http://rdaregistry.info/Elements/u/> ;
    rdfs:label "is animator of"@en ;
    rdfs:subPropertyOf <http://rdaregistry.info/Elements/u/P60626> ;
    owl:inverseOf <http://rdaregistry.info/Elements/u/P60378> ;
    skos:definition "Relates an agent contributing to a moving image resource or computer program by giving apparent movement to inanimate objects or drawings to a resource."@en ;
    skos:scopeNote "Creation of the drawings that are animated is excluded."@en .

<http://rdaregistry.info/Elements/u/P60607>
    rdakit:seeAlso <http://rdaregistry.info/Elements/u/P60655> ;
    reg:hasSubproperty <http://rdaregistry.info/Elements/a/P50137> ;
    reg:lexicalAlias <http://rdaregistry.info/Elements/u/arrangerOfMusicOf.en> ;
    reg:name "arrangerOfMusicOf"@en ;
    reg:status <http://metadataregistry.org/uri/RegStatus/1001> ;
    a rdf:Property ;
    rdfs:isDefinedBy <http://rdaregistry.info/Elements/u/> ;
    rdfs:label "is arranger of music of"@en ;
    rdfs:subPropertyOf <http://rdaregistry.info/Elements/u/P60626> ;
    owl:inverseOf <http://rdaregistry.info/Elements/u/P60379> ;
    skos:definition "Relates an agent contributing to a musical resource by rewriting a composition for a medium of performance different from that for which a resource was originally intended to a resource."@en .

<http://rdaregistry.info/Elements/u/P60608>
    reg:hasSubproperty <http://rdaregistry.info/Elements/a/P50138>, <http://rdaregistry.info/Elements/u/P60600> ;
    reg:lexicalAlias <http://rdaregistry.info/Elements/u/writerOfAddedTextOf.en> ;
    reg:name "writerOfAddedTextOf"@en ;
    reg:status <http://metadataregistry.org/uri/RegStatus/1001> ;
    a rdf:Property ;
    rdfs:isDefinedBy <http://rdaregistry.info/Elements/u/> ;
    rdfs:label "is writer of added text of"@en ;
    rdfs:subPropertyOf <http://rdaregistry.info/Elements/u/P60620> ;
    owl:inverseOf <http://rdaregistry.info/Elements/u/P60380> ;
    skos:definition "Relates an agent contributing to a primarily non-textual resource by providing text, such as captions for photographs or descriptions of maps to a resource."@en .

<http://rdaregistry.info/Elements/u/P60609>
    reg:hasSubproperty <http://rdaregistry.info/Elements/a/P50141> ;
    reg:lexicalAlias <http://rdaregistry.info/Elements/u/draftsmanOf.en> ;
    reg:name "draftsmanOf"@en ;
    reg:status <http://metadataregistry.org/uri/RegStatus/1001> ;
    a rdf:Property ;
    rdfs:isDefinedBy <http://rdaregistry.info/Elements/u/> ;
    rdfs:label "is draftsman of"@en ;
    rdfs:subPropertyOf <http://rdaregistry.info/Elements/u/P60626> ;
    owl:inverseOf <http://rdaregistry.info/Elements/u/P60381> ;
    skos:definition "Relates an agent contributing to a resource by an architect, inventor, etc., by making detailed plans or drawings for buildings, ships, aircraft, machines, objects, etc. to a resource."@en .

<http://rdaregistry.info/Elements/u/P60610>
    rdakit:seeAlso <http://rdaregistry.info/Elements/u/P60607> ;
    reg:hasSubproperty <http://rdaregistry.info/Elements/a/P50142> ;
    reg:lexicalAlias <http://rdaregistry.info/Elements/u/transcriberOf.en> ;
    reg:name "transcriberOf"@en ;
    reg:status <http://metadataregistry.org/uri/RegStatus/1001> ;
    a rdf:Property ;
    rdfs:isDefinedBy <http://rdaregistry.info/Elements/u/> ;
    rdfs:label "is transcriber of"@en ;
    rdfs:subPropertyOf <http://rdaregistry.info/Elements/u/P60626> ;
    owl:inverseOf <http://rdaregistry.info/Elements/u/P60382> ;
    skos:definition "Relates an agent contributing to a resource by writing down or notating previously unwritten or unnotated content, or by changing it from one system of notation to another to a resource."@en ;
    skos:scopeNote "Transcription of a musical resource for a different instrument or performing group is excluded."@en .

<http://rdaregistry.info/Elements/u/P60611>
    reg:hasSubproperty <http://rdaregistry.info/Elements/a/P50143> ;
    reg:lexicalAlias <http://rdaregistry.info/Elements/u/musicalDirectorOf.en> ;
    reg:name "musicalDirectorOf"@en ;
    reg:status <http://metadataregistry.org/uri/RegStatus/1001> ;
    a rdf:Property ;
    rdfs:isDefinedBy <http://rdaregistry.info/Elements/u/> ;
    rdfs:label "is musical director of"@en ;
    rdfs:subPropertyOf <http://rdaregistry.info/Elements/u/P60626> ;
    owl:inverseOf <http://rdaregistry.info/Elements/u/P60383> ;
    skos:definition "Relates an agent contributing to a resource by coordinating the activities of composers, sound editors, and sound mixers for a moving image production or for a musical or dramatic presentation or entertainment to a resource."@en .

<http://rdaregistry.info/Elements/u/P60612>
    reg:hasSubproperty <http://rdaregistry.info/Elements/a/P50144> ;
    reg:lexicalAlias <http://rdaregistry.info/Elements/u/costumeDesignerOf.en> ;
    reg:name "costumeDesignerOf"@en ;
    reg:status <http://metadataregistry.org/uri/RegStatus/1001> ;
    a rdf:Property ;
    rdfs:isDefinedBy <http://rdaregistry.info/Elements/u/> ;
    rdfs:label "is costume designer of"@en ;
    rdfs:subPropertyOf <http://rdaregistry.info/Elements/u/P60626> ;
    owl:inverseOf <http://rdaregistry.info/Elements/u/P60384> ;
    skos:definition "Relates an agent contributing to a resource by designing costumes for a moving image production or for a musical or dramatic presentation or entertainment to a resource."@en .

<http://rdaregistry.info/Elements/u/P60613>
    reg:hasSubproperty <http://rdaregistry.info/Elements/a/P50145> ;
    reg:lexicalAlias <http://rdaregistry.info/Elements/u/translatorOf.en> ;
    reg:name "translatorOf"@en ;
    reg:status <http://metadataregistry.org/uri/RegStatus/1001> ;
    a rdf:Property ;
    rdfs:isDefinedBy <http://rdaregistry.info/Elements/u/> ;
    rdfs:label "is translator of"@en ;
    rdfs:subPropertyOf <http://rdaregistry.info/Elements/u/P60626> ;
    owl:inverseOf <http://rdaregistry.info/Elements/u/P60385> ;
    skos:definition "Relates an agent contributing to a resource by expressing linguistic content of a resource in a language different from that of previous expressions of an original resource to a resource."@en ;
    skos:scopeNote "Translation of linguistic content between forms of the same language from different time periods is included."@en .

<http://rdaregistry.info/Elements/u/P60614>
    reg:hasSubproperty <http://rdaregistry.info/Elements/a/P50146> ;
    reg:lexicalAlias <http://rdaregistry.info/Elements/u/artDirectorOf.en> ;
    reg:name "artDirectorOf"@en ;
    reg:status <http://metadataregistry.org/uri/RegStatus/1001> ;
    a rdf:Property ;
    rdfs:isDefinedBy <http://rdaregistry.info/Elements/u/> ;
    rdfs:label "is art director of"@en ;
    rdfs:subPropertyOf <http://rdaregistry.info/Elements/u/P60626> ;
    owl:inverseOf <http://rdaregistry.info/Elements/u/P60386> ;
    skos:definition "Relates an agent contributing to a resource by overseeing artists and craftspeople who build sets for moving image productions to a resource."@en .

<http://rdaregistry.info/Elements/u/P60615>
    reg:hasSubproperty <http://rdaregistry.info/Elements/a/P50147>, <http://rdaregistry.info/Elements/u/P60016>, <http://rdaregistry.info/Elements/u/P60017>, <http://rdaregistry.info/Elements/u/P60018>, <http://rdaregistry.info/Elements/u/P60019>, <http://rdaregistry.info/Elements/u/P60020>, <http://rdaregistry.info/Elements/u/P60021>, <http://rdaregistry.info/Elements/u/P60022>, <http://rdaregistry.info/Elements/u/P60023>, <http://rdaregistry.info/Elements/u/P60024>, <http://rdaregistry.info/Elements/u/P60025>, <http://rdaregistry.info/Elements/u/P60026>, <http://rdaregistry.info/Elements/u/P60028>, <http://rdaregistry.info/Elements/u/P60029>, <http://rdaregistry.info/Elements/u/P60030>, <http://rdaregistry.info/Elements/u/P60031> ;
    reg:lexicalAlias <http://rdaregistry.info/Elements/u/performerOf.en> ;
    reg:name "performerOf"@en ;
    reg:status <http://metadataregistry.org/uri/RegStatus/1001> ;
    a rdf:Property ;
    rdfs:isDefinedBy <http://rdaregistry.info/Elements/u/> ;
    rdfs:label "is performer of"@en ;
    rdfs:subPropertyOf <http://rdaregistry.info/Elements/u/P60626> ;
    owl:inverseOf <http://rdaregistry.info/Elements/u/P60387> ;
    skos:definition "Relates an agent contributing to a resource by performing music, acting, dancing, speaking, etc., often in a musical or dramatic presentation, etc. to a resource."@en .

<http://rdaregistry.info/Elements/u/P60616>
    reg:hasSubproperty <http://rdaregistry.info/Elements/a/P50148> ;
    reg:lexicalAlias <http://rdaregistry.info/Elements/u/courtReporterOf.en> ;
    reg:name "courtReporterOf"@en ;
    reg:status <http://metadataregistry.org/uri/RegStatus/1001> ;
    a rdf:Property ;
    rdfs:isDefinedBy <http://rdaregistry.info/Elements/u/> ;
    rdfs:label "is court reporter of"@en ;
    rdfs:subPropertyOf <http://rdaregistry.info/Elements/u/P60626> ;
    owl:inverseOf <http://rdaregistry.info/Elements/u/P60388> ;
    skos:definition "Relates an agent contributing to a resource by preparing a court's opinions for publication to a resource."@en .

<http://rdaregistry.info/Elements/u/P60617>
    reg:hasSubproperty <http://rdaregistry.info/Elements/a/P50149> ;
    reg:lexicalAlias <http://rdaregistry.info/Elements/u/writerOfPrefaceOf.en> ;
    reg:name "writerOfPrefaceOf"@en ;
    reg:status <http://metadataregistry.org/uri/RegStatus/1001> ;
    a rdf:Property ;
    rdfs:isDefinedBy <http://rdaregistry.info/Elements/u/> ;
    rdfs:label "is writer of introduction of"@en ;
    rdfs:subPropertyOf <http://rdaregistry.info/Elements/u/P60620> ;
    owl:inverseOf <http://rdaregistry.info/Elements/u/P60389> ;
    skos:definition "Relates an agent contributing to a resource by providing an introduction to an original resource to a resource."@en .

<http://rdaregistry.info/Elements/u/P60618>
    reg:hasSubproperty <http://rdaregistry.info/Elements/a/P50152> ;
    reg:lexicalAlias <http://rdaregistry.info/Elements/u/writerOfAddedCommentaryOf.en> ;
    reg:name "writerOfAddedCommentaryOf"@en ;
    reg:status <http://metadataregistry.org/uri/RegStatus/1001> ;
    a rdf:Property ;
    rdfs:isDefinedBy <http://rdaregistry.info/Elements/u/> ;
    rdfs:label "is writer of added commentary of"@en ;
    rdfs:subPropertyOf <http://rdaregistry.info/Elements/u/P60620> ;
    owl:inverseOf <http://rdaregistry.info/Elements/u/P60390> ;
    skos:definition "Relates an agent contributing to a resource by providing an interpretation or critical explanation of an original resource to a resource."@en .

<http://rdaregistry.info/Elements/u/P60619>
    reg:hasSubproperty <http://rdaregistry.info/Elements/a/P50153> ;
    reg:lexicalAlias <http://rdaregistry.info/Elements/u/writerOfIntroductionOf.en> ;
    reg:name "writerOfIntroductionOf"@en ;
    reg:status <http://metadataregistry.org/uri/RegStatus/1001> ;
    a rdf:Property ;
    rdfs:isDefinedBy <http://rdaregistry.info/Elements/u/> ;
    rdfs:label "is writer of afterword of"@en ;
    rdfs:subPropertyOf <http://rdaregistry.info/Elements/u/P60620> ;
    owl:inverseOf <http://rdaregistry.info/Elements/u/P60391> ;
    skos:definition "Relates an agent contributing to a resource by providing an afterword to an original resource to a resource."@en .

<http://rdaregistry.info/Elements/u/P60620>
    reg:hasSubproperty <http://rdaregistry.info/Elements/a/P50154>, <http://rdaregistry.info/Elements/u/P60608>, <http://rdaregistry.info/Elements/u/P60617>, <http://rdaregistry.info/Elements/u/P60618>, <http://rdaregistry.info/Elements/u/P60619> ;
    reg:lexicalAlias <http://rdaregistry.info/Elements/u/writerOfSupplementaryTextualContentOf.en> ;
    reg:name "writerOfSupplementaryTextualContentOf"@en ;
    reg:status <http://metadataregistry.org/uri/RegStatus/1001> ;
    a rdf:Property ;
    rdfs:isDefinedBy <http://rdaregistry.info/Elements/u/> ;
    rdfs:label "is writer of postface of"@en ;
    rdfs:subPropertyOf <http://rdaregistry.info/Elements/u/P60626> ;
    owl:inverseOf <http://rdaregistry.info/Elements/u/P60392> ;
    skos:definition "Relates an agent contributing to a resource by providing supplementary textual content, such as an introduction or a preface, to an original resource to a resource."@en .

<http://rdaregistry.info/Elements/u/P60621>
    reg:hasSubproperty <http://rdaregistry.info/Elements/a/P50156> ;
    reg:lexicalAlias <http://rdaregistry.info/Elements/u/editorOf.en> ;
    reg:name "editorOf"@en ;
    reg:status <http://metadataregistry.org/uri/RegStatus/1001> ;
    a rdf:Property ;
    rdfs:isDefinedBy <http://rdaregistry.info/Elements/u/> ;
    rdfs:label "is editor of"@en ;
    rdfs:subPropertyOf <http://rdaregistry.info/Elements/u/P60626> ;
    owl:inverseOf <http://rdaregistry.info/Elements/u/P60393> ;
    skos:definition "Relates an agent contributing to a resource by revising or clarifying the content, e.g., adding an introduction, notes, or other critical matter to a resource."@en .

<http://rdaregistry.info/Elements/u/P60622>
    rdakit:seeAlso <http://rdaregistry.info/Elements/u/P60663> ;
    reg:hasSubproperty <http://rdaregistry.info/Elements/a/P50157> ;
    reg:lexicalAlias <http://rdaregistry.info/Elements/u/abridgerOf.en> ;
    reg:name "abridgerOf"@en ;
    reg:status <http://metadataregistry.org/uri/RegStatus/1001> ;
    a rdf:Property ;
    rdfs:isDefinedBy <http://rdaregistry.info/Elements/u/> ;
    rdfs:label "is abridger of"@en ;
    rdfs:subPropertyOf <http://rdaregistry.info/Elements/u/P60626> ;
    owl:inverseOf <http://rdaregistry.info/Elements/u/P60394> ;
    skos:definition "Relates an agent contributing to a resource by shortening or condensing an original resource but leaving the nature and content substantially unchanged to a resource."@en .

<http://rdaregistry.info/Elements/u/P60623>
    reg:hasSubproperty <http://rdaregistry.info/Elements/a/P50158> ;
    reg:lexicalAlias <http://rdaregistry.info/Elements/u/recordingEngineerOf.en> ;
    reg:name "recordingEngineerOf"@en ;
    reg:status <http://metadataregistry.org/uri/RegStatus/1001> ;
    a rdf:Property ;
    rdfs:isDefinedBy <http://rdaregistry.info/Elements/u/> ;
    rdfs:label "is recording engineer of"@en ;
    rdfs:subPropertyOf <http://rdaregistry.info/Elements/u/P60626> ;
    owl:inverseOf <http://rdaregistry.info/Elements/u/P60395> ;
    skos:definition "Relates an agent contributing to a resource by supervising the technical aspects of a sound or video recording session to a resource."@en .

<http://rdaregistry.info/Elements/u/P60624>
    rdakit:seeAlso <http://rdaregistry.info/Elements/u/P60660> ;
    reg:hasSubproperty <http://rdaregistry.info/Elements/a/P50159>, <http://rdaregistry.info/Elements/u/P60756> ;
    reg:lexicalAlias <http://rdaregistry.info/Elements/u/illustratorOf.en> ;
    reg:name "illustratorOf"@en ;
    reg:status <http://metadataregistry.org/uri/RegStatus/1001> ;
    a rdf:Property ;
    rdfs:isDefinedBy <http://rdaregistry.info/Elements/u/> ;
    rdfs:label "is illustrator of"@en ;
    rdfs:subPropertyOf <http://rdaregistry.info/Elements/u/P60626> ;
    owl:inverseOf <http://rdaregistry.info/Elements/u/P60396> ;
    skos:definition "Relates an agent contributing to a resource by supplementing a primary content with drawings, diagrams, photographs, etc. to a resource."@en ;
    skos:scopeNote "Creation of content that is primarily artistic is excluded."@en .

<http://rdaregistry.info/Elements/u/P60625>
    reg:hasSubproperty <http://rdaregistry.info/Elements/a/P50160> ;
    reg:lexicalAlias <http://rdaregistry.info/Elements/u/recordistOf.en> ;
    reg:name "recordistOf"@en ;
    reg:status <http://metadataregistry.org/uri/RegStatus/1001> ;
    a rdf:Property ;
    rdfs:isDefinedBy <http://rdaregistry.info/Elements/u/> ;
    rdfs:label "is recordist of"@en ;
    rdfs:subPropertyOf <http://rdaregistry.info/Elements/u/P60626> ;
    owl:inverseOf <http://rdaregistry.info/Elements/u/P60397> ;
    skos:definition "Relates an agent contributing to a resource by using a recording device to capture sound or video during a recording session, including field recordings of natural sounds, folkloric events, music, etc. to a resource."@en .

<http://rdaregistry.info/Elements/u/P60626>
    reg:hasSubproperty <http://rdaregistry.info/Elements/a/P50161>, <http://rdaregistry.info/Elements/u/P60605>, <http://rdaregistry.info/Elements/u/P60606>, <http://rdaregistry.info/Elements/u/P60607>, <http://rdaregistry.info/Elements/u/P60609>, <http://rdaregistry.info/Elements/u/P60610>, <http://rdaregistry.info/Elements/u/P60611>, <http://rdaregistry.info/Elements/u/P60612>, <http://rdaregistry.info/Elements/u/P60613>, <http://rdaregistry.info/Elements/u/P60614>, <http://rdaregistry.info/Elements/u/P60615>, <http://rdaregistry.info/Elements/u/P60616>, <http://rdaregistry.info/Elements/u/P60620>, <http://rdaregistry.info/Elements/u/P60621>, <http://rdaregistry.info/Elements/u/P60622>, <http://rdaregistry.info/Elements/u/P60623>, <http://rdaregistry.info/Elements/u/P60624>, <http://rdaregistry.info/Elements/u/P60625>, <http://rdaregistry.info/Elements/u/P60627>, <http://rdaregistry.info/Elements/u/P60647>, <http://rdaregistry.info/Elements/u/P60651>, <http://rdaregistry.info/Elements/u/P60666>, <http://rdaregistry.info/Elements/u/P60671>, <http://rdaregistry.info/Elements/u/P60754>, <http://rdaregistry.info/Elements/u/P60755>, <http://rdaregistry.info/Elements/u/P60810>, <http://rdaregistry.info/Elements/u/P60812>, <http://rdaregistry.info/Elements/u/P60814>, <http://rdaregistry.info/Elements/u/P60825>, <http://rdaregistry.info/Elements/u/P60829>, <http://rdaregistry.info/Elements/u/P60839>, <http://rdaregistry.info/Elements/u/P60841>, <http://rdaregistry.info/Elements/u/P60852> ;
    reg:lexicalAlias <http://rdaregistry.info/Elements/u/contributorOf.en> ;
    reg:name "contributorOf"@en ;
    reg:status <http://metadataregistry.org/uri/RegStatus/1001> ;
    a rdf:Property ;
    rdfs:isDefinedBy <http://rdaregistry.info/Elements/u/> ;
    rdfs:label "is contributor of"@en ;
    owl:inverseOf <http://rdaregistry.info/Elements/u/P60398> ;
    skos:definition "Relates an agent contributing to an expression to a resource."@en .

<http://rdaregistry.info/Elements/u/P60627>
    reg:hasSubproperty <http://rdaregistry.info/Elements/a/P50139> ;
    reg:lexicalAlias <http://rdaregistry.info/Elements/u/stageDirectorOf.en> ;
    reg:name "stageDirectorOf"@en ;
    reg:status <http://metadataregistry.org/uri/RegStatus/1001> ;
    a rdf:Property ;
    rdfs:isDefinedBy <http://rdaregistry.info/Elements/u/> ;
    rdfs:label "is stage director of"@en ;
    rdfs:subPropertyOf <http://rdaregistry.info/Elements/u/P60626> ;
    owl:inverseOf <http://rdaregistry.info/Elements/u/P60399> ;
    skos:definition "Relates an agent contributing to a stage resource through the general management and supervision of a performance to a resource."@en .

<http://rdaregistry.info/Elements/u/P60628>
    reg:hasSubproperty <http://rdaregistry.info/Elements/a/P50162>, <http://rdaregistry.info/Elements/u/P60008> ;
    reg:lexicalAlias <http://rdaregistry.info/Elements/u/currentOwnerOf.en> ;
    reg:name "currentOwnerOf"@en ;
    reg:status <http://metadataregistry.org/uri/RegStatus/1001> ;
    a rdf:Property ;
    rdfs:isDefinedBy <http://rdaregistry.info/Elements/u/> ;
    rdfs:label "is current owner of"@en ;
    rdfs:subPropertyOf <http://rdaregistry.info/Elements/u/P60632> ;
    owl:inverseOf <http://rdaregistry.info/Elements/u/P60400> ;
    skos:definition "Relates an agent currently having legal possession of a resource to a resource."@en .

<http://rdaregistry.info/Elements/u/P60629>
    reg:hasSubproperty <http://rdaregistry.info/Elements/a/P50026> ;
    reg:lexicalAlias <http://rdaregistry.info/Elements/u/employee.en> ;
    reg:name "employee"@en ;
    reg:status <http://metadataregistry.org/uri/RegStatus/1001> ;
    a rdf:Property ;
    rdfs:isDefinedBy <http://rdaregistry.info/Elements/u/> ;
    rdfs:label "has employee"@en ;
    owl:inverseOf <http://rdaregistry.info/Elements/u/P60679> ;
    skos:definition "Relates an agent employed by an agent to an agent."@en .

<http://rdaregistry.info/Elements/u/P60630>
    reg:hasSubproperty <http://rdaregistry.info/Elements/a/P50163>, <http://rdaregistry.info/Elements/u/P60012>, <http://rdaregistry.info/Elements/u/P60013> ;
    reg:lexicalAlias <http://rdaregistry.info/Elements/u/formerOwnerOf.en> ;
    reg:name "formerOwnerOf"@en ;
    reg:status <http://metadataregistry.org/uri/RegStatus/1001> ;
    a rdf:Property ;
    rdfs:isDefinedBy <http://rdaregistry.info/Elements/u/> ;
    rdfs:label "is former owner of"@en ;
    rdfs:subPropertyOf <http://rdaregistry.info/Elements/u/P60632> ;
    owl:inverseOf <http://rdaregistry.info/Elements/u/P60401> ;
    skos:definition "Relates an agent formerly having legal possession of a resource to a resource."@en .

<http://rdaregistry.info/Elements/u/P60631>
    reg:hasSubproperty <http://rdaregistry.info/Elements/a/P50164> ;
    reg:lexicalAlias <http://rdaregistry.info/Elements/u/custodianOf.en> ;
    reg:name "custodianOf"@en ;
    reg:status <http://metadataregistry.org/uri/RegStatus/1001> ;
    a rdf:Property ;
    rdfs:isDefinedBy <http://rdaregistry.info/Elements/u/> ;
    rdfs:label "is custodian of"@en ;
    owl:inverseOf <http://rdaregistry.info/Elements/u/P60402> ;
    skos:definition "Relates an agent having legal custody of a resource to a resource."@en .

<http://rdaregistry.info/Elements/u/P60632>
    reg:hasSubproperty <http://rdaregistry.info/Elements/a/P50165>, <http://rdaregistry.info/Elements/u/P60628>, <http://rdaregistry.info/Elements/u/P60630> ;
    reg:lexicalAlias <http://rdaregistry.info/Elements/u/ownerOf.en> ;
    reg:name "ownerOf"@en ;
    reg:status <http://metadataregistry.org/uri/RegStatus/1001> ;
    a rdf:Property ;
    rdfs:isDefinedBy <http://rdaregistry.info/Elements/u/> ;
    rdfs:label "is owner of"@en ;
    owl:inverseOf <http://rdaregistry.info/Elements/u/P60404> ;
    skos:definition "Relates an agent having legal possession of a resource to a resource."@en .

<http://rdaregistry.info/Elements/u/P60633>
    reg:hasSubproperty <http://rdaregistry.info/Elements/a/P50027>, <http://rdaregistry.info/Elements/u/P60864>, <http://rdaregistry.info/Elements/u/P60866> ;
    reg:lexicalAlias <http://rdaregistry.info/Elements/u/officer.en> ;
    reg:name "officer"@en ;
    reg:status <http://metadataregistry.org/uri/RegStatus/1001> ;
    a rdf:Property ;
    rdfs:isDefinedBy <http://rdaregistry.info/Elements/u/> ;
    rdfs:label "has officer"@en ;
    rdfs:subPropertyOf <http://rdaregistry.info/Elements/u/P60454> ;
    owl:inverseOf <http://rdaregistry.info/Elements/u/P60737> ;
    skos:definition "Relates an agent holding an office in or commanding an agent to an agent."@en .

<http://rdaregistry.info/Elements/u/P60634>
    reg:hasSubproperty <http://rdaregistry.info/Elements/a/P50166>, <http://rdaregistry.info/Elements/a/P50167> ;
    reg:lexicalAlias <http://rdaregistry.info/Elements/u/honoureeOf.en> ;
    reg:name "honoureeOf"@en ;
    reg:status <http://metadataregistry.org/uri/RegStatus/1001> ;
    a rdf:Property ;
    rdfs:isDefinedBy <http://rdaregistry.info/Elements/u/> ;
    rdfs:label "is honouree of"@en ;
    rdfs:subPropertyOf <http://rdaregistry.info/Elements/u/P60602> ;
    owl:inverseOf <http://rdaregistry.info/Elements/u/P60406> ;
    skos:altLabel "honoree of"@en ;
    skos:definition "Relates an agent honoured by a resource to a resource."@en .

<http://rdaregistry.info/Elements/u/P60635>
    reg:hasSubproperty <http://rdaregistry.info/Elements/a/P50168> ;
    reg:lexicalAlias <http://rdaregistry.info/Elements/u/broadcasterOf.en> ;
    reg:name "broadcasterOf"@en ;
    reg:status <http://metadataregistry.org/uri/RegStatus/1001> ;
    a rdf:Property ;
    rdfs:isDefinedBy <http://rdaregistry.info/Elements/u/> ;
    rdfs:label "is broadcaster of"@en ;
    rdfs:subPropertyOf <http://rdaregistry.info/Elements/u/P60670> ;
    owl:inverseOf <http://rdaregistry.info/Elements/u/P60407> ;
    skos:definition "Relates an agent involved in broadcasting a resource to an audience via radio, television, webcast, etc. to a resource."@en .

<http://rdaregistry.info/Elements/u/P60636>
    reg:hasSubproperty <http://rdaregistry.info/Elements/a/P50169> ;
    reg:lexicalAlias <http://rdaregistry.info/Elements/u/filmDistributorOf.en> ;
    reg:name "filmDistributorOf"@en ;
    reg:status <http://metadataregistry.org/uri/RegStatus/1001> ;
    a rdf:Property ;
    rdfs:isDefinedBy <http://rdaregistry.info/Elements/u/> ;
    rdfs:label "is film distributor of"@en ;
    rdfs:subPropertyOf <http://rdaregistry.info/Elements/u/P60667> ;
    owl:inverseOf <http://rdaregistry.info/Elements/u/P60408> ;
    skos:definition "Relates an agent involved in distributing a moving image resource to theatres or other distribution channels to a resource."@en .

<http://rdaregistry.info/Elements/u/P60637>
    reg:hasSubproperty <http://rdaregistry.info/Elements/a/P50170> ;
    reg:lexicalAlias <http://rdaregistry.info/Elements/u/bookDesignerOf.en> ;
    reg:name "bookDesignerOf"@en ;
    reg:status <http://metadataregistry.org/uri/RegStatus/1001> ;
    a rdf:Property ;
    rdfs:isDefinedBy <http://rdaregistry.info/Elements/u/> ;
    rdfs:label "is book designer of"@en ;
    rdfs:subPropertyOf <http://rdaregistry.info/Elements/u/P60669> ;
    owl:inverseOf <http://rdaregistry.info/Elements/u/P60409> ;
    skos:definition "Relates an agent involved in manufacturing a resource by being responsible for the entire graphic design of a book, including arrangement of type and illustration, choice of materials, and process used to a resource."@en .

<http://rdaregistry.info/Elements/u/P60638>
    reg:hasSubproperty <http://rdaregistry.info/Elements/a/P50171> ;
    reg:lexicalAlias <http://rdaregistry.info/Elements/u/engraverOf.en> ;
    reg:name "engraverOf"@en ;
    reg:status <http://metadataregistry.org/uri/RegStatus/1001> ;
    a rdf:Property ;
    rdfs:isDefinedBy <http://rdaregistry.info/Elements/u/> ;
    rdfs:label "is engraver of"@en ;
    rdfs:subPropertyOf <http://rdaregistry.info/Elements/u/P60669> ;
    owl:inverseOf <http://rdaregistry.info/Elements/u/P60410> ;
    skos:definition "Relates an agent involved in manufacturing a resource by cutting letters, figures, etc., on a surface such as a wooden or metal plate used for printing to a resource."@en .

<http://rdaregistry.info/Elements/u/P60639>
    reg:hasSubproperty <http://rdaregistry.info/Elements/a/P50172> ;
    reg:lexicalAlias <http://rdaregistry.info/Elements/u/brailleEmbosserOf.en> ;
    reg:name "brailleEmbosserOf"@en ;
    reg:status <http://metadataregistry.org/uri/RegStatus/1001> ;
    a rdf:Property ;
    rdfs:isDefinedBy <http://rdaregistry.info/Elements/u/> ;
    rdfs:label "is braille embosser of"@en ;
    rdfs:subPropertyOf <http://rdaregistry.info/Elements/u/P60669> ;
    owl:inverseOf <http://rdaregistry.info/Elements/u/P60411> ;
    skos:definition "Relates an agent involved in manufacturing a resource by embossing braille cells using a stylus, special embossing printer, or other device to a resource."@en .

<http://rdaregistry.info/Elements/u/P60640>
    reg:hasSubproperty <http://rdaregistry.info/Elements/a/P50173> ;
    reg:lexicalAlias <http://rdaregistry.info/Elements/u/printmakerOf.en> ;
    reg:name "printmakerOf"@en ;
    reg:status <http://metadataregistry.org/uri/RegStatus/1001> ;
    a rdf:Property ;
    rdfs:isDefinedBy <http://rdaregistry.info/Elements/u/> ;
    rdfs:label "is printmaker of"@en ;
    rdfs:subPropertyOf <http://rdaregistry.info/Elements/u/P60669> ;
    owl:inverseOf <http://rdaregistry.info/Elements/u/P60412> ;
    skos:definition "Relates an agent involved in manufacturing a resource by making a relief, intaglio, or planographic printing surface to a resource."@en .

<http://rdaregistry.info/Elements/u/P60641>
    reg:hasSubproperty <http://rdaregistry.info/Elements/a/P50174> ;
    reg:lexicalAlias <http://rdaregistry.info/Elements/u/casterOf.en> ;
    reg:name "casterOf"@en ;
    reg:status <http://metadataregistry.org/uri/RegStatus/1001> ;
    a rdf:Property ;
    rdfs:isDefinedBy <http://rdaregistry.info/Elements/u/> ;
    rdfs:label "is caster of"@en ;
    rdfs:subPropertyOf <http://rdaregistry.info/Elements/u/P60669> ;
    owl:inverseOf <http://rdaregistry.info/Elements/u/P60413> ;
    skos:definition "Relates an agent involved in manufacturing a resource by pouring a liquid or molten substance into a mold and leaving it to solidify to take the shape of the mold to a resource."@en .

<http://rdaregistry.info/Elements/u/P60642>
    reg:hasSubproperty <http://rdaregistry.info/Elements/a/P50175> ;
    reg:lexicalAlias <http://rdaregistry.info/Elements/u/lithographerOf.en> ;
    reg:name "lithographerOf"@en ;
    reg:status <http://metadataregistry.org/uri/RegStatus/1001> ;
    a rdf:Property ;
    rdfs:isDefinedBy <http://rdaregistry.info/Elements/u/> ;
    rdfs:label "is lithographer of"@en ;
    rdfs:subPropertyOf <http://rdaregistry.info/Elements/u/P60669> ;
    owl:inverseOf <http://rdaregistry.info/Elements/u/P60414> ;
    skos:definition "Relates an agent involved in manufacturing a resource by preparing a stone or plate for lithographic printing."@en ;
    skos:scopeNote "A lithographer includes a graphic artist creating a design directly on the surface from which printing will be done."@en .

<http://rdaregistry.info/Elements/u/P60643>
    reg:hasSubproperty <http://rdaregistry.info/Elements/a/P50176> ;
    reg:lexicalAlias <http://rdaregistry.info/Elements/u/platemakerOf.en> ;
    reg:name "platemakerOf"@en ;
    reg:status <http://metadataregistry.org/uri/RegStatus/1001> ;
    a rdf:Property ;
    rdfs:isDefinedBy <http://rdaregistry.info/Elements/u/> ;
    rdfs:label "is platemaker of"@en ;
    rdfs:subPropertyOf <http://rdaregistry.info/Elements/u/P60669> ;
    owl:inverseOf <http://rdaregistry.info/Elements/u/P60415> ;
    skos:definition "Relates an agent involved in manufacturing a resource by preparing plates used in the production of printed images or text to a resource."@en .

<http://rdaregistry.info/Elements/u/P60644>
    reg:hasSubproperty <http://rdaregistry.info/Elements/a/P50177> ;
    reg:lexicalAlias <http://rdaregistry.info/Elements/u/etcherOf.en> ;
    reg:name "etcherOf"@en ;
    reg:status <http://metadataregistry.org/uri/RegStatus/1001> ;
    a rdf:Property ;
    rdfs:isDefinedBy <http://rdaregistry.info/Elements/u/> ;
    rdfs:label "is etcher of"@en ;
    rdfs:subPropertyOf <http://rdaregistry.info/Elements/u/P60669> ;
    owl:inverseOf <http://rdaregistry.info/Elements/u/P60416> ;
    skos:definition "Relates an agent involved in manufacturing a resource by subjecting metal, glass, or some other surface used for printing, to acid or another corrosive substance to a resource."@en .

<http://rdaregistry.info/Elements/u/P60645>
    reg:hasSubproperty <http://rdaregistry.info/Elements/a/P50178> ;
    reg:lexicalAlias <http://rdaregistry.info/Elements/u/collotyperOf.en> ;
    reg:name "collotyperOf"@en ;
    reg:status <http://metadataregistry.org/uri/RegStatus/1001> ;
    a rdf:Property ;
    rdfs:isDefinedBy <http://rdaregistry.info/Elements/u/> ;
    rdfs:label "is collotyper of"@en ;
    rdfs:subPropertyOf <http://rdaregistry.info/Elements/u/P60669> ;
    owl:inverseOf <http://rdaregistry.info/Elements/u/P60417> ;
    skos:definition "Relates an agent involved in manufacturing a resource using a photomechanical process for making prints directly from a hardened film of gelatin or other colloid that has ink-receptive and ink-repellent surfaces to a resource."@en .

<http://rdaregistry.info/Elements/u/P60646>
    reg:hasSubproperty <http://rdaregistry.info/Elements/a/P50179> ;
    reg:lexicalAlias <http://rdaregistry.info/Elements/u/printerOf.en> ;
    reg:name "printerOf"@en ;
    reg:status <http://metadataregistry.org/uri/RegStatus/1001> ;
    a rdf:Property ;
    rdfs:isDefinedBy <http://rdaregistry.info/Elements/u/> ;
    rdfs:label "is printer of"@en ;
    rdfs:subPropertyOf <http://rdaregistry.info/Elements/u/P60669> ;
    owl:inverseOf <http://rdaregistry.info/Elements/u/P60418> ;
    skos:definition "Relates an agent involved in manufacturing a resource of printed text, notated music, etc., from type or plates, such as a book, newspaper, magazine, broadside, score, etc. to a resource."@en .

<http://rdaregistry.info/Elements/u/P60647>
    reg:hasSubproperty <http://rdaregistry.info/Elements/a/P50180> ;
    reg:lexicalAlias <http://rdaregistry.info/Elements/u/presenterOf.en> ;
    reg:name "presenterOf"@en ;
    reg:status <http://metadataregistry.org/uri/RegStatus/1001> ;
    a rdf:Property ;
    rdfs:isDefinedBy <http://rdaregistry.info/Elements/u/> ;
    rdfs:label "is presenter of"@en ;
    rdfs:subPropertyOf <http://rdaregistry.info/Elements/u/P60626> ;
    owl:inverseOf <http://rdaregistry.info/Elements/u/P60419> ;
    skos:definition "Relates an agent mentioned in an \"X presents\" credit for moving image materials and who is probably associated with production, finance, or distribution in some way to a resource."@en .

<http://rdaregistry.info/Elements/u/P60648>
    reg:hasSubproperty <http://rdaregistry.info/Elements/a/P50056>, <http://rdaregistry.info/Elements/a/P50095>, <http://rdaregistry.info/Elements/a/P50230> ;
    reg:lexicalAlias <http://rdaregistry.info/Elements/u/memberOf.en> ;
    reg:name "memberOf"@en ;
    reg:status <http://metadataregistry.org/uri/RegStatus/1001> ;
    a rdf:Property ;
    rdfs:isDefinedBy <http://rdaregistry.info/Elements/u/> ;
    rdfs:label "has member of"@en ;
    owl:inverseOf <http://rdaregistry.info/Elements/u/P60697> ;
    skos:definition "Relates an agent of which an agent is a member to an agent."@en .

<http://rdaregistry.info/Elements/u/P60649>
    reg:hasSubproperty <http://rdaregistry.info/Elements/a/P50091> ;
    reg:lexicalAlias <http://rdaregistry.info/Elements/u/degreeSupervisorOf.en> ;
    reg:name "degreeSupervisorOf"@en ;
    reg:status <http://metadataregistry.org/uri/RegStatus/1001> ;
    a rdf:Property ;
    rdfs:isDefinedBy <http://rdaregistry.info/Elements/u/> ;
    rdfs:label "is degree supervisor of"@en ;
    rdfs:subPropertyOf <http://rdaregistry.info/Elements/u/P60672> ;
    owl:inverseOf <http://rdaregistry.info/Elements/u/P60420> ;
    skos:definition "Relates an agent, such as an advisor or supervisor of thesis or dissertation research, overseeing either an academic degree or thesis to a resource."@en .

<http://rdaregistry.info/Elements/u/P60650>
    reg:hasSubproperty <http://rdaregistry.info/Elements/a/P50092> ;
    reg:lexicalAlias <http://rdaregistry.info/Elements/u/illuminatorOf.en> ;
    reg:name "illuminatorOf"@en ;
    reg:status <http://metadataregistry.org/uri/RegStatus/1001> ;
    a rdf:Property ;
    rdfs:isDefinedBy <http://rdaregistry.info/Elements/u/> ;
    rdfs:label "is illuminator of"@en ;
    rdfs:subPropertyOf <http://rdaregistry.info/Elements/u/P60602> ;
    owl:inverseOf <http://rdaregistry.info/Elements/u/P60421> ;
    skos:definition "Relates an agent providing decoration to a specific resource using precious metals or color, often with elaborate designs and motifs to a resource."@en .

<http://rdaregistry.info/Elements/u/P60651>
    reg:hasSubproperty <http://rdaregistry.info/Elements/a/P50183> ;
    reg:lexicalAlias <http://rdaregistry.info/Elements/u/editorOfMovingImageResourceOf.en> ;
    reg:name "editorOfMovingImageResourceOf"@en ;
    reg:status <http://metadataregistry.org/uri/RegStatus/1001> ;
    a rdf:Property ;
    rdfs:isDefinedBy <http://rdaregistry.info/Elements/u/> ;
    rdfs:label "is editor of moving image resource of"@en ;
    rdfs:subPropertyOf <http://rdaregistry.info/Elements/u/P60626> ;
    owl:inverseOf <http://rdaregistry.info/Elements/u/P60422> ;
    skos:definition "Relates an agent responsible for assembling, arranging, and trimming film, video, or other moving image formats, including both visual and audio aspects to a resource."@en .

<http://rdaregistry.info/Elements/u/P60652>
    reg:hasSubproperty <http://rdaregistry.info/Elements/a/P50184> ;
    reg:lexicalAlias <http://rdaregistry.info/Elements/u/programmerOf.en> ;
    reg:name "programmerOf"@en ;
    reg:status <http://metadataregistry.org/uri/RegStatus/1001> ;
    a rdf:Property ;
    rdfs:isDefinedBy <http://rdaregistry.info/Elements/u/> ;
    rdfs:label "is programmer of"@en ;
    rdfs:subPropertyOf <http://rdaregistry.info/Elements/u/P60672> ;
    owl:inverseOf <http://rdaregistry.info/Elements/u/P60423> ;
    skos:definition "Relates an agent responsible for creating a computer program to a resource."@en .

<http://rdaregistry.info/Elements/u/P60653>
    reg:hasSubproperty <http://rdaregistry.info/Elements/a/P50185> ;
    reg:lexicalAlias <http://rdaregistry.info/Elements/u/designerOf.en> ;
    reg:name "designerOf"@en ;
    reg:status <http://metadataregistry.org/uri/RegStatus/1001> ;
    a rdf:Property ;
    rdfs:isDefinedBy <http://rdaregistry.info/Elements/u/> ;
    rdfs:label "is designer of"@en ;
    rdfs:subPropertyOf <http://rdaregistry.info/Elements/u/P60672> ;
    owl:inverseOf <http://rdaregistry.info/Elements/u/P60424> ;
    skos:definition "Relates an agent responsible for creating a design for an object to a resource."@en .

<http://rdaregistry.info/Elements/u/P60654>
    reg:hasSubproperty <http://rdaregistry.info/Elements/a/P50150>, <http://rdaregistry.info/Elements/a/P50186> ;
    reg:lexicalAlias <http://rdaregistry.info/Elements/u/cartographerOf.en> ;
    reg:name "cartographerOf"@en ;
    reg:status <http://metadataregistry.org/uri/RegStatus/1001> ;
    a rdf:Property ;
    rdfs:isDefinedBy <http://rdaregistry.info/Elements/u/> ;
    rdfs:label "is cartographer of"@en ;
    rdfs:subPropertyOf <http://rdaregistry.info/Elements/u/P60672> ;
    owl:inverseOf <http://rdaregistry.info/Elements/u/P60425> ;
    skos:definition "Relates an agent responsible for creating a map, atlas, globe, or other cartographic resource to a resource."@en .

<http://rdaregistry.info/Elements/u/P60655>
    reg:hasSubproperty <http://rdaregistry.info/Elements/a/P50134>, <http://rdaregistry.info/Elements/a/P50187> ;
    reg:lexicalAlias <http://rdaregistry.info/Elements/u/composerOf.en> ;
    reg:name "composerOf"@en ;
    reg:status <http://metadataregistry.org/uri/RegStatus/1001> ;
    a rdf:Property ;
    rdfs:isDefinedBy <http://rdaregistry.info/Elements/u/> ;
    rdfs:label "is composer of"@en ;
    rdfs:subPropertyOf <http://rdaregistry.info/Elements/u/P60672> ;
    owl:inverseOf <http://rdaregistry.info/Elements/u/P60426> ;
    skos:definition "Relates an agent responsible for creating a musical resource to a resource."@en .

<http://rdaregistry.info/Elements/u/P60656>
    reg:hasSubproperty <http://rdaregistry.info/Elements/a/P50188> ;
    reg:lexicalAlias <http://rdaregistry.info/Elements/u/inventorOf.en> ;
    reg:name "inventorOf"@en ;
    reg:status <http://metadataregistry.org/uri/RegStatus/1001> ;
    a rdf:Property ;
    rdfs:isDefinedBy <http://rdaregistry.info/Elements/u/> ;
    rdfs:label "is inventor of"@en ;
    rdfs:subPropertyOf <http://rdaregistry.info/Elements/u/P60672> ;
    owl:inverseOf <http://rdaregistry.info/Elements/u/P60427> ;
    skos:definition "Relates an agent responsible for creating a new device or process to a resource."@en .

<http://rdaregistry.info/Elements/u/P60657>
    rdakit:seeAlso <http://rdaregistry.info/Elements/u/P60621> ;
    reg:hasSubproperty <http://rdaregistry.info/Elements/a/P50189> ;
    reg:lexicalAlias <http://rdaregistry.info/Elements/u/compilerOf.en> ;
    reg:name "compilerOf"@en ;
    reg:status <http://metadataregistry.org/uri/RegStatus/1001> ;
    a rdf:Property ;
    rdfs:isDefinedBy <http://rdaregistry.info/Elements/u/> ;
    rdfs:label "is compiler of"@en ;
    rdfs:subPropertyOf <http://rdaregistry.info/Elements/u/P60672> ;
    owl:inverseOf <http://rdaregistry.info/Elements/u/P60428> ;
    skos:definition "Relates an agent responsible for creating a new resource such as a bibliography or a directory by selecting, arranging, aggregating, and editing data, information, etc., to a resource."@en .

<http://rdaregistry.info/Elements/u/P60658>
    reg:hasSubproperty <http://rdaregistry.info/Elements/a/P50190>, <http://rdaregistry.info/Elements/a/P50272> ;
    reg:lexicalAlias <http://rdaregistry.info/Elements/u/photographerOf.en> ;
    reg:name "photographerOf"@en ;
    reg:status <http://metadataregistry.org/uri/RegStatus/1001> ;
    a rdf:Property ;
    rdfs:isDefinedBy <http://rdaregistry.info/Elements/u/> ;
    rdfs:label "is photographer of"@en ;
    rdfs:subPropertyOf <http://rdaregistry.info/Elements/u/P60672> ;
    owl:inverseOf <http://rdaregistry.info/Elements/u/P60429> ;
    skos:definition "Relates an agent responsible for creating a photographic resource to a resource."@en .

<http://rdaregistry.info/Elements/u/P60659>
    reg:hasSubproperty <http://rdaregistry.info/Elements/a/P50140>, <http://rdaregistry.info/Elements/a/P50191> ;
    reg:lexicalAlias <http://rdaregistry.info/Elements/u/interviewerOf.en> ;
    reg:name "interviewerOf"@en ;
    reg:status <http://metadataregistry.org/uri/RegStatus/1001> ;
    a rdf:Property ;
    rdfs:isDefinedBy <http://rdaregistry.info/Elements/u/> ;
    rdfs:label "is interviewer of"@en ;
    rdfs:subPropertyOf <http://rdaregistry.info/Elements/u/P60672> ;
    owl:inverseOf <http://rdaregistry.info/Elements/u/P60430> ;
    skos:definition "Relates an agent responsible for creating a resource by acting as an interviewer, reporter, pollster, or some other information gathering agent to a resource."@en .

<http://rdaregistry.info/Elements/u/P60660>
    reg:hasSubproperty <http://rdaregistry.info/Elements/a/P50192>, <http://rdaregistry.info/Elements/u/P60705>, <http://rdaregistry.info/Elements/u/P60758>, <http://rdaregistry.info/Elements/u/P60759> ;
    reg:lexicalAlias <http://rdaregistry.info/Elements/u/artistOf.en> ;
    reg:name "artistOf"@en ;
    reg:status <http://metadataregistry.org/uri/RegStatus/1001> ;
    a rdf:Property ;
    rdfs:isDefinedBy <http://rdaregistry.info/Elements/u/> ;
    rdfs:label "is artist of"@en ;
    rdfs:subPropertyOf <http://rdaregistry.info/Elements/u/P60672> ;
    owl:inverseOf <http://rdaregistry.info/Elements/u/P60431> ;
    skos:definition "Relates an agent responsible for creating a resource by conceiving, and often implementing, an original graphic design, drawing, painting, etc. to a resource."@en .

<http://rdaregistry.info/Elements/u/P60661>
    reg:hasSubproperty <http://rdaregistry.info/Elements/a/P50155>, <http://rdaregistry.info/Elements/a/P50193> ;
    reg:lexicalAlias <http://rdaregistry.info/Elements/u/intervieweeOf.en> ;
    reg:name "intervieweeOf"@en ;
    reg:status <http://metadataregistry.org/uri/RegStatus/1001> ;
    a rdf:Property ;
    rdfs:isDefinedBy <http://rdaregistry.info/Elements/u/> ;
    rdfs:label "is interviewee of"@en ;
    rdfs:subPropertyOf <http://rdaregistry.info/Elements/u/P60672> ;
    owl:inverseOf <http://rdaregistry.info/Elements/u/P60432> ;
    skos:definition "Relates an agent responsible for creating a resource by responding to an interviewer, usually a reporter, pollster, or some other information gathering agent to a resource."@en .

<http://rdaregistry.info/Elements/u/P60662>
    reg:hasSubproperty <http://rdaregistry.info/Elements/a/P50151>, <http://rdaregistry.info/Elements/a/P50194> ;
    reg:lexicalAlias <http://rdaregistry.info/Elements/u/choreographerOf.en> ;
    reg:name "choreographerOf"@en ;
    reg:status <http://metadataregistry.org/uri/RegStatus/1001> ;
    a rdf:Property ;
    rdfs:isDefinedBy <http://rdaregistry.info/Elements/u/> ;
    rdfs:label "is choreographer of"@en ;
    rdfs:subPropertyOf <http://rdaregistry.info/Elements/u/P60672> ;
    owl:inverseOf <http://rdaregistry.info/Elements/u/P60433> ;
    skos:definition "Relates an agent responsible for creating a resource of movement to a resource."@en .

<http://rdaregistry.info/Elements/u/P60663>
    reg:hasSubproperty <http://rdaregistry.info/Elements/a/P50195>, <http://rdaregistry.info/Elements/u/P60706>, <http://rdaregistry.info/Elements/u/P60707>, <http://rdaregistry.info/Elements/u/P60708>, <http://rdaregistry.info/Elements/u/P60757> ;
    reg:lexicalAlias <http://rdaregistry.info/Elements/u/authorOf.en> ;
    reg:name "authorOf"@en ;
    reg:status <http://metadataregistry.org/uri/RegStatus/1001> ;
    a rdf:Property ;
    rdfs:isDefinedBy <http://rdaregistry.info/Elements/u/> ;
    rdfs:label "is author of"@en ;
    rdfs:subPropertyOf <http://rdaregistry.info/Elements/u/P60672> ;
    owl:inverseOf <http://rdaregistry.info/Elements/u/P60434> ;
    skos:definition "Relates an agent responsible for creating a resource that is primarily textual in content, regardless of media  type or genre to a resource."@en .

<http://rdaregistry.info/Elements/u/P60664>
    reg:hasSubproperty <http://rdaregistry.info/Elements/a/P50196>, <http://rdaregistry.info/Elements/u/P60704> ;
    reg:lexicalAlias <http://rdaregistry.info/Elements/u/architectOf.en> ;
    reg:name "architectOf"@en ;
    reg:status <http://metadataregistry.org/uri/RegStatus/1001> ;
    a rdf:Property ;
    rdfs:isDefinedBy <http://rdaregistry.info/Elements/u/> ;
    rdfs:label "is architect of"@en ;
    rdfs:subPropertyOf <http://rdaregistry.info/Elements/u/P60672> ;
    owl:inverseOf <http://rdaregistry.info/Elements/u/P60435> ;
    skos:definition "Relates an agent responsible for creating an architectural design, including a pictorial representation intended to show how a building, etc., will look when completed to a resource."@en .

<http://rdaregistry.info/Elements/u/P60665>
    reg:hasSubproperty <http://rdaregistry.info/Elements/a/P50197> ;
    reg:lexicalAlias <http://rdaregistry.info/Elements/u/filmmakerOf.en> ;
    reg:name "filmmakerOf"@en ;
    reg:status <http://metadataregistry.org/uri/RegStatus/1001> ;
    a rdf:Property ;
    rdfs:isDefinedBy <http://rdaregistry.info/Elements/u/> ;
    rdfs:label "is filmmaker of"@en ;
    rdfs:subPropertyOf <http://rdaregistry.info/Elements/u/P60672> ;
    owl:inverseOf <http://rdaregistry.info/Elements/u/P60436> ;
    skos:definition "Relates an agent responsible for creating an independent or personal film to a resource."@en .

<http://rdaregistry.info/Elements/u/P60666>
    reg:hasSubproperty <http://rdaregistry.info/Elements/a/P50198> ;
    reg:lexicalAlias <http://rdaregistry.info/Elements/u/productionDesignerOf.en> ;
    reg:name "productionDesignerOf"@en ;
    reg:status <http://metadataregistry.org/uri/RegStatus/1001> ;
    a rdf:Property ;
    rdfs:isDefinedBy <http://rdaregistry.info/Elements/u/> ;
    rdfs:label "is production designer of"@en ;
    rdfs:subPropertyOf <http://rdaregistry.info/Elements/u/P60626> ;
    owl:inverseOf <http://rdaregistry.info/Elements/u/P60437> ;
    skos:definition "Relates an agent responsible for designing the overall visual appearance of a moving image production to a resource."@en .

<http://rdaregistry.info/Elements/u/P60667>
    reg:hasSubproperty <http://rdaregistry.info/Elements/a/P50199>, <http://rdaregistry.info/Elements/u/P60636> ;
    reg:lexicalAlias <http://rdaregistry.info/Elements/u/distributorOf.en> ;
    reg:name "distributorOf"@en ;
    reg:status <http://metadataregistry.org/uri/RegStatus/1001> ;
    a rdf:Property ;
    rdfs:isDefinedBy <http://rdaregistry.info/Elements/u/> ;
    rdfs:label "is distributor of"@en ;
    owl:inverseOf <http://rdaregistry.info/Elements/u/P60438> ;
    skos:definition "Relates an agent responsible for distributing a resource to a resource."@en .

<http://rdaregistry.info/Elements/u/P60668>
    reg:hasSubproperty <http://rdaregistry.info/Elements/a/P50201>, <http://rdaregistry.info/Elements/u/P60033>, <http://rdaregistry.info/Elements/u/P60034>, <http://rdaregistry.info/Elements/u/P60035>, <http://rdaregistry.info/Elements/u/P60883> ;
    reg:lexicalAlias <http://rdaregistry.info/Elements/u/producerOf.en> ;
    reg:name "producerOf"@en ;
    reg:status <http://metadataregistry.org/uri/RegStatus/1001> ;
    a rdf:Property ;
    rdfs:isDefinedBy <http://rdaregistry.info/Elements/u/> ;
    rdfs:label "is producer of"@en ;
    rdfs:subPropertyOf <http://rdaregistry.info/Elements/u/P60602> ;
    owl:inverseOf <http://rdaregistry.info/Elements/u/P60441> ;
    skos:definition "Relates an agent responsible for most of the business aspects of a production for screen, sound recording, television, webcast, etc. to a resource."@en .

<http://rdaregistry.info/Elements/u/P60669>
    reg:hasSubproperty <http://rdaregistry.info/Elements/a/P50202>, <http://rdaregistry.info/Elements/u/P60637>, <http://rdaregistry.info/Elements/u/P60638>, <http://rdaregistry.info/Elements/u/P60639>, <http://rdaregistry.info/Elements/u/P60640>, <http://rdaregistry.info/Elements/u/P60641>, <http://rdaregistry.info/Elements/u/P60642>, <http://rdaregistry.info/Elements/u/P60643>, <http://rdaregistry.info/Elements/u/P60644>, <http://rdaregistry.info/Elements/u/P60645>, <http://rdaregistry.info/Elements/u/P60646>, <http://rdaregistry.info/Elements/u/P60747> ;
    reg:lexicalAlias <http://rdaregistry.info/Elements/u/manufacturerOf.en> ;
    reg:name "manufacturerOf"@en ;
    reg:status <http://metadataregistry.org/uri/RegStatus/1001> ;
    a rdf:Property ;
    rdfs:isDefinedBy <http://rdaregistry.info/Elements/u/> ;
    rdfs:label "is manufacturer of"@en ;
    owl:inverseOf <http://rdaregistry.info/Elements/u/P60443> ;
    skos:definition "Relates an agent responsible for printing, duplicating, casting, etc., a resource in a published form to a resource."@en .

<http://rdaregistry.info/Elements/u/P60670>
    reg:hasSubproperty <http://rdaregistry.info/Elements/a/P50203>, <http://rdaregistry.info/Elements/u/P60635> ;
    reg:lexicalAlias <http://rdaregistry.info/Elements/u/publisherOf.en> ;
    reg:name "publisherOf"@en ;
    reg:status <http://metadataregistry.org/uri/RegStatus/1001> ;
    a rdf:Property ;
    rdfs:isDefinedBy <http://rdaregistry.info/Elements/u/> ;
    rdfs:label "is publisher of"@en ;
    owl:inverseOf <http://rdaregistry.info/Elements/u/P60444> ;
    skos:definition "Relates an agent responsible for publishing, releasing, or issuing a resource to a resource."@en .

<http://rdaregistry.info/Elements/u/P60671>
    reg:hasSubproperty <http://rdaregistry.info/Elements/a/P50212> ;
    reg:lexicalAlias <http://rdaregistry.info/Elements/u/minuteTakerOf.en> ;
    reg:name "minuteTakerOf"@en ;
    reg:status <http://metadataregistry.org/uri/RegStatus/1001> ;
    a rdf:Property ;
    rdfs:isDefinedBy <http://rdaregistry.info/Elements/u/> ;
    rdfs:label "is minute taker of"@en ;
    rdfs:subPropertyOf <http://rdaregistry.info/Elements/u/P60626> ;
    owl:inverseOf <http://rdaregistry.info/Elements/u/P60446> ;
    skos:definition "Relates an agent responsible for recording the minutes of a meeting to a resource."@en .

<http://rdaregistry.info/Elements/u/P60672>
    reg:hasSubproperty <http://rdaregistry.info/Elements/a/P50204>, <http://rdaregistry.info/Elements/u/P60001>, <http://rdaregistry.info/Elements/u/P60014>, <http://rdaregistry.info/Elements/u/P60649>, <http://rdaregistry.info/Elements/u/P60652>, <http://rdaregistry.info/Elements/u/P60653>, <http://rdaregistry.info/Elements/u/P60654>, <http://rdaregistry.info/Elements/u/P60655>, <http://rdaregistry.info/Elements/u/P60656>, <http://rdaregistry.info/Elements/u/P60657>, <http://rdaregistry.info/Elements/u/P60658>, <http://rdaregistry.info/Elements/u/P60659>, <http://rdaregistry.info/Elements/u/P60660>, <http://rdaregistry.info/Elements/u/P60661>, <http://rdaregistry.info/Elements/u/P60662>, <http://rdaregistry.info/Elements/u/P60663>, <http://rdaregistry.info/Elements/u/P60664>, <http://rdaregistry.info/Elements/u/P60665>, <http://rdaregistry.info/Elements/u/P60699>, <http://rdaregistry.info/Elements/u/P60701>, <http://rdaregistry.info/Elements/u/P60827>, <http://rdaregistry.info/Elements/u/P60881>, <http://rdaregistry.info/Elements/u/P60882> ;
    reg:lexicalAlias <http://rdaregistry.info/Elements/u/creatorOf.en> ;
    reg:name "creatorOf"@en ;
    reg:status <http://metadataregistry.org/uri/RegStatus/1001> ;
    a rdf:Property ;
    rdfs:isDefinedBy <http://rdaregistry.info/Elements/u/> ;
    rdfs:label "is creator of"@en ;
    owl:inverseOf <http://rdaregistry.info/Elements/u/P60447> ;
    skos:definition "Relates an agent responsible for the creation of a resource to a resource."@en .

<http://rdaregistry.info/Elements/u/P60673>
    reg:hasSubproperty <http://rdaregistry.info/Elements/a/P50205> ;
    reg:lexicalAlias <http://rdaregistry.info/Elements/u/directorOf.en> ;
    reg:name "directorOf"@en ;
    reg:status <http://metadataregistry.org/uri/RegStatus/1001> ;
    a rdf:Property ;
    rdfs:isDefinedBy <http://rdaregistry.info/Elements/u/> ;
    rdfs:label "is director of"@en ;
    rdfs:subPropertyOf <http://rdaregistry.info/Elements/u/P60602> ;
    owl:inverseOf <http://rdaregistry.info/Elements/u/P60449> ;
    skos:definition "Relates an agent responsible for the general management and supervision of a filmed performance, a radio or television program, etc. to a resource."@en .

<http://rdaregistry.info/Elements/u/P60674>
    reg:hasSubproperty <http://rdaregistry.info/Elements/a/P50206>, <http://rdaregistry.info/Elements/a/P50273> ;
    reg:lexicalAlias <http://rdaregistry.info/Elements/u/restorationistOf.en> ;
    reg:name "restorationistOf"@en ;
    reg:status <http://metadataregistry.org/uri/RegStatus/1001> ;
    a rdf:Property ;
    rdfs:isDefinedBy <http://rdaregistry.info/Elements/u/> ;
    rdfs:label "is restorationist of"@en ;
    rdfs:subPropertyOf <http://rdaregistry.info/Elements/u/P60602> ;
    owl:inverseOf <http://rdaregistry.info/Elements/u/P60450> ;
    skos:definition "Relates an agent responsible for the set of technical, editorial, and intellectual procedures aimed at compensating for the degradation of a resource by bringing it back to a state as close as possible to its original condition to a resource."@en .

<http://rdaregistry.info/Elements/u/P60675>
    reg:hasSubproperty <http://rdaregistry.info/Elements/a/P50226> ;
    reg:lexicalAlias <http://rdaregistry.info/Elements/u/sponsoringBodyOf.en> ;
    reg:name "sponsoringBodyOf"@en ;
    reg:status <http://metadataregistry.org/uri/RegStatus/1001> ;
    a rdf:Property ;
    rdfs:isDefinedBy <http://rdaregistry.info/Elements/u/> ;
    rdfs:label "is sponsoring body of"@en ;
    rdfs:subPropertyOf <http://rdaregistry.info/Elements/u/P60602> ;
    owl:inverseOf <http://rdaregistry.info/Elements/u/P60451> ;
    skos:definition "Relates an agent sponsoring some aspect of a resource, e.g., funding research, sponsoring an event to a resource."@en .

<http://rdaregistry.info/Elements/u/P60676>
    reg:hasSubproperty <http://rdaregistry.info/Elements/a/P50015>, <http://rdaregistry.info/Elements/a/P50021>, <http://rdaregistry.info/Elements/a/P50028> ;
    reg:lexicalAlias <http://rdaregistry.info/Elements/u/sponsor.en> ;
    reg:name "sponsor"@en ;
    reg:status <http://metadataregistry.org/uri/RegStatus/1001> ;
    a rdf:Property ;
    rdfs:isDefinedBy <http://rdaregistry.info/Elements/u/> ;
    rdfs:label "has sponsor"@en ;
    owl:inverseOf <http://rdaregistry.info/Elements/u/P60688> ;
    skos:definition "Relates an agent sponsoring an agent to an agent."@en .

<http://rdaregistry.info/Elements/u/P60678>
    reg:hasSubproperty <http://rdaregistry.info/Elements/a/P50207> ;
    reg:lexicalAlias <http://rdaregistry.info/Elements/u/directorOfPhotographyOf.en> ;
    reg:name "directorOfPhotographyOf"@en ;
    reg:status <http://metadataregistry.org/uri/RegStatus/1001> ;
    a rdf:Property ;
    rdfs:isDefinedBy <http://rdaregistry.info/Elements/u/> ;
    rdfs:label "is director of photography of"@en ;
    rdfs:subPropertyOf <http://rdaregistry.info/Elements/u/P60602> ;
    owl:inverseOf <http://rdaregistry.info/Elements/u/P60452> ;
    skos:definition "Relates an agent that captures images, either electronically or on film or video stock, and often selects and arranges lighting. a director of photography for a movie is also called a chief cinematographer to a resource."@en .

<http://rdaregistry.info/Elements/u/P60679>
    reg:hasSubproperty <http://rdaregistry.info/Elements/a/P50096> ;
    reg:lexicalAlias <http://rdaregistry.info/Elements/u/employer.en> ;
    reg:name "employer"@en ;
    reg:status <http://metadataregistry.org/uri/RegStatus/1001> ;
    a rdf:Property ;
    rdfs:isDefinedBy <http://rdaregistry.info/Elements/u/> ;
    rdfs:label "has employer"@en ;
    owl:inverseOf <http://rdaregistry.info/Elements/u/P60629> ;
    skos:definition "Relates an agent that employs an agent to an agent."@en .

<http://rdaregistry.info/Elements/u/P60680>
    reg:hasSubproperty <http://rdaregistry.info/Elements/a/P50008> ;
    reg:lexicalAlias <http://rdaregistry.info/Elements/u/hierarchicalSuperior.en> ;
    reg:name "hierarchicalSuperior"@en ;
    reg:status <http://metadataregistry.org/uri/RegStatus/1001> ;
    a rdf:Property ;
    rdfs:isDefinedBy <http://rdaregistry.info/Elements/u/> ;
    rdfs:label "has hierarchical superior"@en ;
    owl:inverseOf <http://rdaregistry.info/Elements/u/P60681> ;
    skos:definition "Relates an agent that is hierarchically superior to another agent to an agent."@en .

<http://rdaregistry.info/Elements/u/P60681>
    reg:hasSubproperty <http://rdaregistry.info/Elements/a/P50010> ;
    reg:lexicalAlias <http://rdaregistry.info/Elements/u/hierarchicalSubordinate.en> ;
    reg:name "hierarchicalSubordinate"@en ;
    reg:status <http://metadataregistry.org/uri/RegStatus/1001> ;
    a rdf:Property ;
    rdfs:isDefinedBy <http://rdaregistry.info/Elements/u/> ;
    rdfs:label "has hierarchical subordinate"@en ;
    owl:inverseOf <http://rdaregistry.info/Elements/u/P60680> ;
    skos:definition "Relates an agent that is subordinate to another agent to an agent."@en .

<http://rdaregistry.info/Elements/u/P60682>
    reg:hasSubproperty <http://rdaregistry.info/Elements/a/P50011> ;
    reg:lexicalAlias <http://rdaregistry.info/Elements/u/mergee.en> ;
    reg:name "mergee"@en ;
    reg:status <http://metadataregistry.org/uri/RegStatus/1001> ;
    a rdf:Property ;
    rdfs:isDefinedBy <http://rdaregistry.info/Elements/u/> ;
    rdfs:label "has mergee"@en ;
    owl:inverseOf <http://rdaregistry.info/Elements/u/P60682> ;
    skos:definition "Relates a agent that merged with another agent to form a third to an agent."@en .

<http://rdaregistry.info/Elements/u/P60683>
    reg:hasSubproperty <http://rdaregistry.info/Elements/a/P50012>, <http://rdaregistry.info/Elements/a/P50055> ;
    reg:lexicalAlias <http://rdaregistry.info/Elements/u/predecessor.en> ;
    reg:name "predecessor"@en ;
    reg:status <http://metadataregistry.org/uri/RegStatus/1001> ;
    a rdf:Property ;
    rdfs:isDefinedBy <http://rdaregistry.info/Elements/u/> ;
    rdfs:label "has predecessor"@en ;
    owl:inverseOf <http://rdaregistry.info/Elements/u/P60686> ;
    skos:definition "Relates an agent that precedes another agent to an agent."@en .

<http://rdaregistry.info/Elements/u/P60684>
    reg:hasSubproperty <http://rdaregistry.info/Elements/a/P50013> ;
    reg:lexicalAlias <http://rdaregistry.info/Elements/u/productOfAMerger.en> ;
    reg:name "productOfAMerger"@en ;
    reg:status <http://metadataregistry.org/uri/RegStatus/1001> ;
    a rdf:Property ;
    rdfs:isDefinedBy <http://rdaregistry.info/Elements/u/> ;
    rdfs:label "has product of merger"@en ;
    owl:inverseOf <http://rdaregistry.info/Elements/u/P60736> ;
    skos:definition "Relates a agent that resulted from a merger of two or more other agents to an agent."@en .

<http://rdaregistry.info/Elements/u/P60685>
    reg:hasSubproperty <http://rdaregistry.info/Elements/a/P50014> ;
    reg:lexicalAlias <http://rdaregistry.info/Elements/u/productOfASplit.en> ;
    reg:name "productOfASplit"@en ;
    reg:status <http://metadataregistry.org/uri/RegStatus/1001> ;
    a rdf:Property ;
    rdfs:isDefinedBy <http://rdaregistry.info/Elements/u/> ;
    rdfs:label "has product of split"@en ;
    owl:inverseOf <http://rdaregistry.info/Elements/u/P60733> ;
    skos:definition "Relates a agent that resulted from a split or division of another agent to an agent."@en .

<http://rdaregistry.info/Elements/u/P60686>
    reg:hasSubproperty <http://rdaregistry.info/Elements/a/P50016>, <http://rdaregistry.info/Elements/a/P50053>, <http://rdaregistry.info/Elements/a/P50099> ;
    reg:lexicalAlias <http://rdaregistry.info/Elements/u/successor.en> ;
    reg:name "successor"@en ;
    reg:status <http://metadataregistry.org/uri/RegStatus/1001> ;
    a rdf:Property ;
    rdfs:isDefinedBy <http://rdaregistry.info/Elements/u/> ;
    rdfs:label "has successor"@en ;
    owl:inverseOf <http://rdaregistry.info/Elements/u/P60683> ;
    skos:definition "Relates an agent that succeeds or follows another agent to an agent."@en .

<http://rdaregistry.info/Elements/u/P60687>
    reg:hasSubproperty <http://rdaregistry.info/Elements/a/P50017>, <http://rdaregistry.info/Elements/a/P50062>, <http://rdaregistry.info/Elements/a/P50112> ;
    reg:lexicalAlias <http://rdaregistry.info/Elements/u/foundedEntity.en> ;
    reg:name "foundedEntity"@en ;
    reg:status <http://metadataregistry.org/uri/RegStatus/1001> ;
    a rdf:Property ;
    rdfs:isDefinedBy <http://rdaregistry.info/Elements/u/> ;
    rdfs:label "has founded entity"@en ;
    owl:inverseOf <http://rdaregistry.info/Elements/u/P60694> ;
    skos:definition "Relates an agent that an agent founded to an agent."@en .

<http://rdaregistry.info/Elements/u/P60688>
    reg:hasSubproperty <http://rdaregistry.info/Elements/a/P50009>, <http://rdaregistry.info/Elements/a/P50063> ;
    reg:lexicalAlias <http://rdaregistry.info/Elements/u/sponsoredEntity.en> ;
    reg:name "sponsoredEntity"@en ;
    reg:status <http://metadataregistry.org/uri/RegStatus/1001> ;
    a rdf:Property ;
    rdfs:isDefinedBy <http://rdaregistry.info/Elements/u/> ;
    rdfs:label "has sponsored entity"@en ;
    owl:inverseOf <http://rdaregistry.info/Elements/u/P60676> ;
    skos:definition "Relates an agent that an agent sponsors to an agent."@en .

<http://rdaregistry.info/Elements/u/P60689>
    reg:hasSubproperty <http://rdaregistry.info/Elements/a/P50208>, <http://rdaregistry.info/Elements/a/P50210> ;
    reg:lexicalAlias <http://rdaregistry.info/Elements/u/dedicateeOf.en> ;
    reg:name "dedicateeOf"@en ;
    reg:status <http://metadataregistry.org/uri/RegStatus/1001> ;
    a rdf:Property ;
    rdfs:isDefinedBy <http://rdaregistry.info/Elements/u/> ;
    rdfs:label "is dedicatee of"@en ;
    rdfs:subPropertyOf <http://rdaregistry.info/Elements/u/P60602> ;
    owl:inverseOf <http://rdaregistry.info/Elements/u/P60455> ;
    skos:definition "Relates an agent to whom a resource is dedicated to a resource."@en .

<http://rdaregistry.info/Elements/u/P60690>
    reg:hasSubproperty <http://rdaregistry.info/Elements/a/P50209> ;
    reg:lexicalAlias <http://rdaregistry.info/Elements/u/addresseeOf.en> ;
    reg:name "addresseeOf"@en ;
    reg:status <http://metadataregistry.org/uri/RegStatus/1001> ;
    a rdf:Property ;
    rdfs:isDefinedBy <http://rdaregistry.info/Elements/u/> ;
    rdfs:label "is addressee of"@en ;
    rdfs:subPropertyOf <http://rdaregistry.info/Elements/u/P60602> ;
    owl:inverseOf <http://rdaregistry.info/Elements/u/P60456> ;
    skos:definition "Relates an agent to whom a resource or part of a resource is addressed to a resource."@en .

<http://rdaregistry.info/Elements/u/P60691>
    reg:hasSubproperty <http://rdaregistry.info/Elements/a/P50042>, <http://rdaregistry.info/Elements/a/P50088>, <http://rdaregistry.info/Elements/a/P50122> ;
    reg:lexicalAlias <http://rdaregistry.info/Elements/u/appellantOf.en> ;
    reg:name "appellantOf"@en ;
    reg:status <http://metadataregistry.org/uri/RegStatus/1001> ;
    a rdf:Property ;
    rdfs:isDefinedBy <http://rdaregistry.info/Elements/u/> ;
    rdfs:label "is appellant of"@en ;
    rdfs:subPropertyOf <http://rdaregistry.info/Elements/u/P60602> ;
    owl:inverseOf <http://rdaregistry.info/Elements/u/P60457> ;
    skos:definition "Relates an agent who appeals a decision of a lower court recorded in a legal resource of a higher court to a resource."@en .

<http://rdaregistry.info/Elements/u/P60692>
    reg:hasSubproperty <http://rdaregistry.info/Elements/a/P50123> ;
    reg:lexicalAlias <http://rdaregistry.info/Elements/u/binderOf.en> ;
    reg:name "binderOf"@en ;
    reg:status <http://metadataregistry.org/uri/RegStatus/1001> ;
    a rdf:Property ;
    rdfs:isDefinedBy <http://rdaregistry.info/Elements/u/> ;
    rdfs:label "is binder of"@en ;
    rdfs:subPropertyOf <http://rdaregistry.info/Elements/u/P60602> ;
    owl:inverseOf <http://rdaregistry.info/Elements/u/P60458> ;
    skos:definition "Relates an agent who binds a resource to a resource."@en .

<http://rdaregistry.info/Elements/u/P60693>
    reg:hasSubproperty <http://rdaregistry.info/Elements/a/P50043>, <http://rdaregistry.info/Elements/a/P50089>, <http://rdaregistry.info/Elements/a/P50124> ;
    reg:lexicalAlias <http://rdaregistry.info/Elements/u/plaintiffOf.en> ;
    reg:name "plaintiffOf"@en ;
    reg:status <http://metadataregistry.org/uri/RegStatus/1001> ;
    a rdf:Property ;
    rdfs:isDefinedBy <http://rdaregistry.info/Elements/u/> ;
    rdfs:label "is plaintiff of"@en ;
    rdfs:subPropertyOf <http://rdaregistry.info/Elements/u/P60602> ;
    owl:inverseOf <http://rdaregistry.info/Elements/u/P60459> ;
    skos:definition "Relates an agent who brings a suit in a civil proceeding to a resource."@en .

<http://rdaregistry.info/Elements/u/P60694>
    reg:hasSubproperty <http://rdaregistry.info/Elements/a/P50007>, <http://rdaregistry.info/Elements/a/P50020>, <http://rdaregistry.info/Elements/a/P50029> ;
    reg:lexicalAlias <http://rdaregistry.info/Elements/u/founder.en> ;
    reg:name "founder"@en ;
    reg:status <http://metadataregistry.org/uri/RegStatus/1001> ;
    a rdf:Property ;
    rdfs:isDefinedBy <http://rdaregistry.info/Elements/u/> ;
    rdfs:label "has founder"@en ;
    owl:inverseOf <http://rdaregistry.info/Elements/u/P60687> ;
    skos:definition "Relates an agent who founded an agent to an agent."@en .

<http://rdaregistry.info/Elements/u/P60695>
    reg:hasSubproperty <http://rdaregistry.info/Elements/a/P50125> ;
    reg:lexicalAlias <http://rdaregistry.info/Elements/u/inscriberOf.en> ;
    reg:name "inscriberOf"@en ;
    reg:status <http://metadataregistry.org/uri/RegStatus/1001> ;
    a rdf:Property ;
    rdfs:isDefinedBy <http://rdaregistry.info/Elements/u/> ;
    rdfs:label "is inscriber of"@en ;
    rdfs:subPropertyOf <http://rdaregistry.info/Elements/u/P60602> ;
    owl:inverseOf <http://rdaregistry.info/Elements/u/P60460> ;
    skos:definition "Relates an agent who has written a statement of dedication or gift on a resource to a resource."@en .

<http://rdaregistry.info/Elements/u/P60696>
    reg:hasSubproperty <http://rdaregistry.info/Elements/a/P50126> ;
    reg:lexicalAlias <http://rdaregistry.info/Elements/u/judgeOf.en> ;
    reg:name "judgeOf"@en ;
    reg:status <http://metadataregistry.org/uri/RegStatus/1001> ;
    a rdf:Property ;
    rdfs:isDefinedBy <http://rdaregistry.info/Elements/u/> ;
    rdfs:label "is judge of"@en ;
    rdfs:subPropertyOf <http://rdaregistry.info/Elements/u/P60602> ;
    owl:inverseOf <http://rdaregistry.info/Elements/u/P60461> ;
    skos:definition "Relates an agent who hears and decides on legal matters in court to a resource."@en .

<http://rdaregistry.info/Elements/u/P60697>
    reg:hasSubproperty <http://rdaregistry.info/Elements/a/P50030>, <http://rdaregistry.info/Elements/a/P50231>, <http://rdaregistry.info/Elements/a/P50233> ;
    reg:lexicalAlias <http://rdaregistry.info/Elements/u/member.en> ;
    reg:name "member"@en ;
    reg:status <http://metadataregistry.org/uri/RegStatus/1001> ;
    a rdf:Property ;
    rdfs:isDefinedBy <http://rdaregistry.info/Elements/u/> ;
    rdfs:label "has member"@en ;
    owl:inverseOf <http://rdaregistry.info/Elements/u/P60648> ;
    skos:definition "Relates an agent who is a member of an agent to an agent."@en .

<http://rdaregistry.info/Elements/u/P60698>
    reg:hasSubproperty <http://rdaregistry.info/Elements/a/P50090>, <http://rdaregistry.info/Elements/a/P50258>, <http://rdaregistry.info/Elements/a/P50259> ;
    reg:lexicalAlias <http://rdaregistry.info/Elements/u/defendantOf.en> ;
    reg:name "defendantOf"@en ;
    reg:status <http://metadataregistry.org/uri/RegStatus/1001> ;
    a rdf:Property ;
    rdfs:isDefinedBy <http://rdaregistry.info/Elements/u/> ;
    rdfs:label "is defendant of"@en ;
    rdfs:subPropertyOf <http://rdaregistry.info/Elements/u/P60602> ;
    owl:inverseOf <http://rdaregistry.info/Elements/u/P60462> ;
    skos:definition "Relates an agent who is accused in a criminal proceeding or sued in a civil proceeding to a resource."@en .

<http://rdaregistry.info/Elements/u/P60699>
    reg:hasSubproperty <http://rdaregistry.info/Elements/a/P50127> ;
    reg:lexicalAlias <http://rdaregistry.info/Elements/u/praesesOf.en> ;
    reg:name "praesesOf"@en ;
    reg:status <http://metadataregistry.org/uri/RegStatus/1001> ;
    a rdf:Property ;
    rdfs:isDefinedBy <http://rdaregistry.info/Elements/u/> ;
    rdfs:label "is praeses of"@en ;
    rdfs:subPropertyOf <http://rdaregistry.info/Elements/u/P60672> ;
    owl:inverseOf <http://rdaregistry.info/Elements/u/P60463> ;
    skos:definition "Relates an agent who is a faculty moderator of an academic disputation, normally proposing a thesis and participating in an ensuing disputation to a resource."@en .

<http://rdaregistry.info/Elements/u/P60700>
    reg:hasSubproperty <http://rdaregistry.info/Elements/a/P50128> ;
    reg:lexicalAlias <http://rdaregistry.info/Elements/u/annotatorOf.en> ;
    reg:name "annotatorOf"@en ;
    reg:status <http://metadataregistry.org/uri/RegStatus/1001> ;
    a rdf:Property ;
    rdfs:isDefinedBy <http://rdaregistry.info/Elements/u/> ;
    rdfs:label "is annotator of"@en ;
    rdfs:subPropertyOf <http://rdaregistry.info/Elements/u/P60602> ;
    owl:inverseOf <http://rdaregistry.info/Elements/u/P60464> ;
    skos:definition "Relates an agent who makes manuscript annotations on a resource to a resource."@en .

<http://rdaregistry.info/Elements/u/P60701>
    reg:hasSubproperty <http://rdaregistry.info/Elements/a/P50211> ;
    reg:lexicalAlias <http://rdaregistry.info/Elements/u/consultantOf.en> ;
    reg:name "consultantOf"@en ;
    reg:status <http://metadataregistry.org/uri/RegStatus/1001> ;
    a rdf:Property ;
    rdfs:isDefinedBy <http://rdaregistry.info/Elements/u/> ;
    rdfs:label "is consultant of"@en ;
    rdfs:subPropertyOf <http://rdaregistry.info/Elements/u/P60672> ;
    owl:inverseOf <http://rdaregistry.info/Elements/u/P60465> ;
    skos:definition "Relates an agent who provides consultation services, and often makes recommendations, for another agent that is represented as a creator of a resource to a resource."@en .

<http://rdaregistry.info/Elements/u/P60702>
    reg:hasSubproperty <http://rdaregistry.info/Elements/a/P50129> ;
    reg:lexicalAlias <http://rdaregistry.info/Elements/u/autographerOf.en> ;
    reg:name "autographerOf"@en ;
    reg:status <http://metadataregistry.org/uri/RegStatus/1001> ;
    a rdf:Property ;
    rdfs:isDefinedBy <http://rdaregistry.info/Elements/u/> ;
    rdfs:label "is autographer of"@en ;
    rdfs:subPropertyOf <http://rdaregistry.info/Elements/u/P60602> ;
    owl:inverseOf <http://rdaregistry.info/Elements/u/P60466> ;
    skos:definition "Relates an agent whose manuscript signature appears on a resource to a resource."@en .

<http://rdaregistry.info/Elements/u/P60703>
    reg:hasSubproperty <http://rdaregistry.info/Elements/a/P50130> ;
    reg:lexicalAlias <http://rdaregistry.info/Elements/u/issuingBodyOf.en> ;
    reg:name "issuingBodyOf"@en ;
    reg:status <http://metadataregistry.org/uri/RegStatus/1001> ;
    a rdf:Property ;
    rdfs:isDefinedBy <http://rdaregistry.info/Elements/u/> ;
    rdfs:label "is issuing body of"@en ;
    rdfs:subPropertyOf <http://rdaregistry.info/Elements/u/P60602> ;
    owl:inverseOf <http://rdaregistry.info/Elements/u/P60467> ;
    skos:definition "Relates an agent issuing a resource, such as an official organ of the agent, to a resource."@en .

<http://rdaregistry.info/Elements/u/P60704>
    reg:hasSubproperty <http://rdaregistry.info/Elements/a/P50221> ;
    reg:lexicalAlias <http://rdaregistry.info/Elements/u/landscapeArchitectOf.en> ;
    reg:name "landscapeArchitectOf"@en ;
    reg:status <http://metadataregistry.org/uri/RegStatus/1001> ;
    a rdf:Property ;
    rdfs:isDefinedBy <http://rdaregistry.info/Elements/u/> ;
    rdfs:label "is landscape architect of"@en ;
    rdfs:subPropertyOf <http://rdaregistry.info/Elements/u/P60664> ;
    owl:inverseOf <http://rdaregistry.info/Elements/u/P60473> ;
    skos:definition "Relates an architect responsible for creating landscape resources to a resource."@en .

<http://rdaregistry.info/Elements/u/P60705>
    reg:hasSubproperty <http://rdaregistry.info/Elements/a/P50222> ;
    reg:lexicalAlias <http://rdaregistry.info/Elements/u/sculptorOf.en> ;
    reg:name "sculptorOf"@en ;
    reg:status <http://metadataregistry.org/uri/RegStatus/1001> ;
    a rdf:Property ;
    rdfs:isDefinedBy <http://rdaregistry.info/Elements/u/> ;
    rdfs:label "is sculptor of"@en ;
    rdfs:subPropertyOf <http://rdaregistry.info/Elements/u/P60660> ;
    owl:inverseOf <http://rdaregistry.info/Elements/u/P60475> ;
    skos:definition "Relates an artist responsible for creating a three-dimensional resource by modeling, carving, or similar technique to a resource."@en .

<http://rdaregistry.info/Elements/u/P60706>
    reg:hasSubproperty <http://rdaregistry.info/Elements/a/P50223> ;
    reg:lexicalAlias <http://rdaregistry.info/Elements/u/screenwriterOf.en> ;
    reg:name "screenwriterOf"@en ;
    reg:status <http://metadataregistry.org/uri/RegStatus/1001> ;
    a rdf:Property ;
    rdfs:isDefinedBy <http://rdaregistry.info/Elements/u/> ;
    rdfs:label "is screenwriter of"@en ;
    rdfs:subPropertyOf <http://rdaregistry.info/Elements/u/P60663> ;
    owl:inverseOf <http://rdaregistry.info/Elements/u/P60476> ;
    skos:definition "Relates an author of a screenplay, script, or scene to a resource."@en .

<http://rdaregistry.info/Elements/u/P60707>
    rdakit:seeAlso <http://rdaregistry.info/Elements/u/P60708> ;
    reg:hasSubproperty <http://rdaregistry.info/Elements/a/P50224> ;
    reg:lexicalAlias <http://rdaregistry.info/Elements/u/lyricistOf.en> ;
    reg:name "lyricistOf"@en ;
    reg:status <http://metadataregistry.org/uri/RegStatus/1001> ;
    a rdf:Property ;
    rdfs:isDefinedBy <http://rdaregistry.info/Elements/u/> ;
    rdfs:label "is lyricist of"@en ;
    rdfs:subPropertyOf <http://rdaregistry.info/Elements/u/P60663> ;
    owl:inverseOf <http://rdaregistry.info/Elements/u/P60477> ;
    skos:definition "Relates an author of the words of a popular song, including a song or songs from a musical to a resource."@en .

<http://rdaregistry.info/Elements/u/P60708>
    rdakit:seeAlso <http://rdaregistry.info/Elements/u/P60707> ;
    reg:hasSubproperty <http://rdaregistry.info/Elements/a/P50225> ;
    reg:lexicalAlias <http://rdaregistry.info/Elements/u/librettistOf.en> ;
    reg:name "librettistOf"@en ;
    reg:status <http://metadataregistry.org/uri/RegStatus/1001> ;
    a rdf:Property ;
    rdfs:isDefinedBy <http://rdaregistry.info/Elements/u/> ;
    rdfs:label "is librettist of"@en ;
    rdfs:subPropertyOf <http://rdaregistry.info/Elements/u/P60663> ;
    owl:inverseOf <http://rdaregistry.info/Elements/u/P60478> ;
    skos:definition "Relates an author of words of an opera or other musical stage resource or an oratorio to a resource."@en .

<http://rdaregistry.info/Elements/u/P60709>
    reg:hasSubproperty <http://rdaregistry.info/Elements/e/P20232>, <http://rdaregistry.info/Elements/i/P40051>, <http://rdaregistry.info/Elements/m/P30210>, <http://rdaregistry.info/Elements/u/P60196>, <http://rdaregistry.info/Elements/u/P60198>, <http://rdaregistry.info/Elements/u/P60204>, <http://rdaregistry.info/Elements/u/P60307> ;
    reg:lexicalAlias <http://rdaregistry.info/Elements/u/accompanyingResourceRelationshipWith.en> ;
    reg:name "accompanyingResourceRelationshipWith"@en ;
    reg:status <http://metadataregistry.org/uri/RegStatus/1001> ;
    a rdf:Property ;
    rdfs:isDefinedBy <http://rdaregistry.info/Elements/u/> ;
    rdfs:label "has accompanying resource relationship with"@en ;
    owl:inverseOf <http://rdaregistry.info/Elements/u/P60709> ;
    skos:definition "Relates a resource to a resource that is an augmentation of, or is augmented by, or is complemented by, or accompanies, or is accompanied by a resource."@en .

<http://rdaregistry.info/Elements/u/P60710>
    reg:hasSubproperty <http://rdaregistry.info/Elements/u/P60250>, <http://rdaregistry.info/Elements/u/P60305> ;
    reg:lexicalAlias <http://rdaregistry.info/Elements/u/derivativeResourceRelationshipWith.en> ;
    reg:name "derivativeResourceRelationshipWith"@en ;
    reg:status <http://metadataregistry.org/uri/RegStatus/1001> ;
    a rdf:Property ;
    rdfs:isDefinedBy <http://rdaregistry.info/Elements/u/> ;
    rdfs:label "has derivative resource relationship with"@en ;
    owl:inverseOf <http://rdaregistry.info/Elements/u/P60710> ;
    skos:definition "Relates a resource to a resource that is based on or is a derivative of another resource."@en .

<http://rdaregistry.info/Elements/u/P60711>
    reg:hasSubproperty <http://rdaregistry.info/Elements/u/P60190>, <http://rdaregistry.info/Elements/u/P60215> ;
    reg:status <http://metadataregistry.org/uri/RegStatus/1008> ;
    rdfs:isDefinedBy <http://rdaregistry.info/Elements/u/> .

<http://rdaregistry.info/Elements/u/P60712>
    reg:hasSubproperty <http://rdaregistry.info/Elements/i/P40053>, <http://rdaregistry.info/Elements/m/P30212>, <http://rdaregistry.info/Elements/u/P60191> ;
    reg:lexicalAlias <http://rdaregistry.info/Elements/u/equivalentResourceRelationshipWith.en> ;
    reg:name "equivalentResourceRelationshipWith"@en ;
    reg:status <http://metadataregistry.org/uri/RegStatus/1001> ;
    a rdf:Property ;
    rdfs:isDefinedBy <http://rdaregistry.info/Elements/u/> ;
    rdfs:label "has equivalent resource relationship with"@en ;
    owl:inverseOf <http://rdaregistry.info/Elements/u/P60712> ;
    skos:definition "Relates a resource to a resource that is equivalent to another resource."@en .

<http://rdaregistry.info/Elements/u/P60713>
    reg:hasSubproperty <http://rdaregistry.info/Elements/u/P60261>, <http://rdaregistry.info/Elements/u/P60278> ;
    reg:lexicalAlias <http://rdaregistry.info/Elements/u/sequentialResourceRelationshipWith.en> ;
    reg:name "sequentialResourceRelationshipWith"@en ;
    reg:status <http://metadataregistry.org/uri/RegStatus/1001> ;
    a rdf:Property ;
    rdfs:isDefinedBy <http://rdaregistry.info/Elements/u/> ;
    rdfs:label "has sequential resource relationship with"@en ;
    owl:inverseOf <http://rdaregistry.info/Elements/u/P60713> ;
    skos:definition "Relates a resource to a resource that is preceded by or succeeded by another resource."@en .

<http://rdaregistry.info/Elements/u/P60714>
    reg:hasSubproperty <http://rdaregistry.info/Elements/i/P40054>, <http://rdaregistry.info/Elements/m/P30213>, <http://rdaregistry.info/Elements/u/P60101>, <http://rdaregistry.info/Elements/u/P60249> ;
    reg:lexicalAlias <http://rdaregistry.info/Elements/u/wholePartResourceRelationshipWith.en> ;
    reg:name "wholePartResourceRelationshipWith"@en ;
    reg:status <http://metadataregistry.org/uri/RegStatus/1001> ;
    a rdf:Property ;
    rdfs:isDefinedBy <http://rdaregistry.info/Elements/u/> ;
    rdfs:label "has whole-part resource relationship with"@en ;
    owl:inverseOf <http://rdaregistry.info/Elements/u/P60714> ;
    skos:definition "Relates a resource to a resource that is contained in or contains another resource."@en .

<http://rdaregistry.info/Elements/u/P60715>
    reg:hasSubproperty <http://rdaregistry.info/Elements/e/P20237> ;
    reg:lexicalAlias <http://rdaregistry.info/Elements/u/writerOfAfterword.en> ;
    reg:name "writerOfAfterword"@en ;
    reg:status <http://metadataregistry.org/uri/RegStatus/1001> ;
    a rdf:Property ;
    rdfs:isDefinedBy <http://rdaregistry.info/Elements/u/> ;
    rdfs:label "has writer of afterword"@en ;
    rdfs:subPropertyOf <http://rdaregistry.info/Elements/u/P60392> ;
    owl:inverseOf <http://rdaregistry.info/Elements/u/P60717> ;
    skos:definition "Relates a resource to an agent contributing to a resource by providing an afterword to an original resource."@en .

<http://rdaregistry.info/Elements/u/P60716>
    reg:hasSubproperty <http://rdaregistry.info/Elements/e/P20238> ;
    reg:lexicalAlias <http://rdaregistry.info/Elements/u/writerOfPostface.en> ;
    reg:name "writerOfPostface"@en ;
    reg:status <http://metadataregistry.org/uri/RegStatus/1001> ;
    a rdf:Property ;
    rdfs:isDefinedBy <http://rdaregistry.info/Elements/u/> ;
    rdfs:label "has writer of postface"@en ;
    rdfs:subPropertyOf <http://rdaregistry.info/Elements/u/P60392> ;
    owl:inverseOf <http://rdaregistry.info/Elements/u/P60718> ;
    skos:definition "Relates a resource to an agent contributing to a resource by providing a postface to an original resource."@en .

<http://rdaregistry.info/Elements/u/P60717>
    reg:hasSubproperty <http://rdaregistry.info/Elements/a/P50227> ;
    reg:lexicalAlias <http://rdaregistry.info/Elements/u/writerOfAfterwordOf.en> ;
    reg:name "writerOfAfterwordOf"@en ;
    reg:status <http://metadataregistry.org/uri/RegStatus/1001> ;
    a rdf:Property ;
    rdfs:isDefinedBy <http://rdaregistry.info/Elements/u/> ;
    rdfs:label "is writer of preface of"@en ;
    rdfs:subPropertyOf <http://rdaregistry.info/Elements/u/P60620> ;
    owl:inverseOf <http://rdaregistry.info/Elements/u/P60715> ;
    skos:definition "Relates an agent contributing to a resource by providing a preface to an original resource to a resource."@en .

<http://rdaregistry.info/Elements/u/P60718>
    reg:hasSubproperty <http://rdaregistry.info/Elements/a/P50228> ;
    reg:lexicalAlias <http://rdaregistry.info/Elements/u/writerOfPostfaceOf.en> ;
    reg:name "writerOfPostfaceOf"@en ;
    reg:status <http://metadataregistry.org/uri/RegStatus/1001> ;
    a rdf:Property ;
    rdfs:isDefinedBy <http://rdaregistry.info/Elements/u/> ;
    rdfs:label "is writer of supplementary textual content of"@en ;
    rdfs:subPropertyOf <http://rdaregistry.info/Elements/u/P60620> ;
    owl:inverseOf <http://rdaregistry.info/Elements/u/P60716> ;
    skos:definition "Relates an agent contributing to a resource by providing supplementary textual content (e.g., an appendix, an introduction, a preface) to an original resource to a resource."@en .

<http://rdaregistry.info/Elements/u/P60719>
    reg:hasSubproperty <http://rdaregistry.info/Elements/e/P20239> ;
    reg:lexicalAlias <http://rdaregistry.info/Elements/u/musicalTheatreAdaptationOf.en> ;
    reg:name "musicalTheatreAdaptationOf"@en ;
    reg:status <http://metadataregistry.org/uri/RegStatus/1001> ;
    a rdf:Property ;
    rdfs:isDefinedBy <http://rdaregistry.info/Elements/u/> ;
    rdfs:label "is musical theatre adaptation of"@en ;
    rdfs:subPropertyOf <http://rdaregistry.info/Elements/u/P60241> ;
    owl:inverseOf <http://rdaregistry.info/Elements/u/P60721> ;
    skos:definition "Relates a resource to a resource that has been adapted as a musical theatre resource."@en .

<http://rdaregistry.info/Elements/u/P60720>
    reg:hasSubproperty <http://rdaregistry.info/Elements/e/P20240> ;
    reg:lexicalAlias <http://rdaregistry.info/Elements/u/operaAdaptationOf.en> ;
    reg:name "operaAdaptationOf"@en ;
    reg:status <http://metadataregistry.org/uri/RegStatus/1001> ;
    a rdf:Property ;
    rdfs:isDefinedBy <http://rdaregistry.info/Elements/u/> ;
    rdfs:label "is opera adaptation of"@en ;
    rdfs:subPropertyOf <http://rdaregistry.info/Elements/u/P60241> ;
    owl:inverseOf <http://rdaregistry.info/Elements/u/P60722> ;
    skos:definition "Relates a resource to a resource that has been adapted as an opera."@en .

<http://rdaregistry.info/Elements/u/P60721>
    reg:hasSubproperty <http://rdaregistry.info/Elements/e/P20241> ;
    reg:lexicalAlias <http://rdaregistry.info/Elements/u/adaptedAsMusicalTheatre.en> ;
    reg:name "adaptedAsMusicalTheatre"@en ;
    reg:status <http://metadataregistry.org/uri/RegStatus/1001> ;
    a rdf:Property ;
    rdfs:isDefinedBy <http://rdaregistry.info/Elements/u/> ;
    rdfs:label "is adapted as musical theatre"@en ;
    rdfs:subPropertyOf <http://rdaregistry.info/Elements/u/P60260> ;
    owl:inverseOf <http://rdaregistry.info/Elements/u/P60719> ;
    skos:definition "Relates a resource to a musical theatre resource based on a source resource."@en .

<http://rdaregistry.info/Elements/u/P60722>
    reg:hasSubproperty <http://rdaregistry.info/Elements/e/P20242> ;
    reg:lexicalAlias <http://rdaregistry.info/Elements/u/adaptedAsOpera.en> ;
    reg:name "adaptedAsOpera"@en ;
    reg:status <http://metadataregistry.org/uri/RegStatus/1001> ;
    a rdf:Property ;
    rdfs:isDefinedBy <http://rdaregistry.info/Elements/u/> ;
    rdfs:label "is adapted as opera"@en ;
    rdfs:subPropertyOf <http://rdaregistry.info/Elements/u/P60260> ;
    owl:inverseOf <http://rdaregistry.info/Elements/u/P60720> ;
    skos:definition "Relates a resource to an opera based on a source resource."@en .

<http://rdaregistry.info/Elements/u/P60723>
    reg:hasSubproperty <http://rdaregistry.info/Elements/e/P20243>, <http://rdaregistry.info/Elements/u/P60118>, <http://rdaregistry.info/Elements/w/P10237> ;
    reg:lexicalAlias <http://rdaregistry.info/Elements/u/music.en> ;
    reg:name "music"@en ;
    reg:status <http://metadataregistry.org/uri/RegStatus/1001> ;
    a rdf:Property ;
    rdfs:isDefinedBy <http://rdaregistry.info/Elements/u/> ;
    rdfs:label "is music"@en ;
    rdfs:subPropertyOf <http://rdaregistry.info/Elements/u/P60198> ;
    owl:inverseOf <http://rdaregistry.info/Elements/u/P60724> ;
    skos:definition "Relates a resource to a musical resource that is used in a motion picture, play, television program, etc."@en .

<http://rdaregistry.info/Elements/u/P60724>
    reg:hasSubproperty <http://rdaregistry.info/Elements/e/P20244>, <http://rdaregistry.info/Elements/u/P60202>, <http://rdaregistry.info/Elements/w/P10238> ;
    reg:lexicalAlias <http://rdaregistry.info/Elements/u/musicFor.en> ;
    reg:name "musicFor"@en ;
    reg:status <http://metadataregistry.org/uri/RegStatus/1001> ;
    a rdf:Property ;
    rdfs:isDefinedBy <http://rdaregistry.info/Elements/u/> ;
    rdfs:label "is music for"@en ;
    rdfs:subPropertyOf <http://rdaregistry.info/Elements/u/P60198> ;
    owl:inverseOf <http://rdaregistry.info/Elements/u/P60723> ;
    skos:definition "Relates a resource to a resource such as a motion picture, play, television program, etc., that uses a musical resource."@en .

<http://rdaregistry.info/Elements/u/P60725>
    reg:hasSubproperty <http://rdaregistry.info/Elements/e/P20245> ;
    reg:lexicalAlias <http://rdaregistry.info/Elements/u/videoMusic.en> ;
    reg:name "videoMusic"@en ;
    reg:status <http://metadataregistry.org/uri/RegStatus/1001> ;
    a rdf:Property ;
    rdfs:isDefinedBy <http://rdaregistry.info/Elements/u/> ;
    rdfs:label "is video music"@en ;
    rdfs:subPropertyOf <http://rdaregistry.info/Elements/u/P60723> ;
    owl:inverseOf <http://rdaregistry.info/Elements/u/P60726> ;
    skos:definition "Relates a resource to a musical resource that is used in a video."@en .

<http://rdaregistry.info/Elements/u/P60726>
    reg:hasSubproperty <http://rdaregistry.info/Elements/e/P20246> ;
    reg:lexicalAlias <http://rdaregistry.info/Elements/u/musicForVideo.en> ;
    reg:name "musicForVideo"@en ;
    reg:status <http://metadataregistry.org/uri/RegStatus/1001> ;
    a rdf:Property ;
    rdfs:isDefinedBy <http://rdaregistry.info/Elements/u/> ;
    rdfs:label "is music for video"@en ;
    rdfs:subPropertyOf <http://rdaregistry.info/Elements/u/P60724> ;
    owl:inverseOf <http://rdaregistry.info/Elements/u/P60725> ;
    skos:definition "Relates a resource to a resource that uses a musical resource in a video."@en .

<http://rdaregistry.info/Elements/u/P60727>
    reg:hasSubproperty <http://rdaregistry.info/Elements/e/P20247> ;
    reg:lexicalAlias <http://rdaregistry.info/Elements/u/televisionProgramMusic.en> ;
    reg:name "televisionProgramMusic"@en ;
    reg:status <http://metadataregistry.org/uri/RegStatus/1001> ;
    a rdf:Property ;
    rdfs:isDefinedBy <http://rdaregistry.info/Elements/u/> ;
    rdfs:label "is television program music"@en ;
    rdfs:subPropertyOf <http://rdaregistry.info/Elements/u/P60723> ;
    owl:inverseOf <http://rdaregistry.info/Elements/u/P60728> ;
    skos:definition "Relates a resource to a musical resource that is used in a television program."@en .

<http://rdaregistry.info/Elements/u/P60728>
    reg:hasSubproperty <http://rdaregistry.info/Elements/e/P20248> ;
    reg:lexicalAlias <http://rdaregistry.info/Elements/u/musicForTelevisionProgram.en> ;
    reg:name "musicForTelevisionProgram"@en ;
    reg:status <http://metadataregistry.org/uri/RegStatus/1001> ;
    a rdf:Property ;
    rdfs:isDefinedBy <http://rdaregistry.info/Elements/u/> ;
    rdfs:label "is music for television program"@en ;
    rdfs:subPropertyOf <http://rdaregistry.info/Elements/u/P60724> ;
    owl:inverseOf <http://rdaregistry.info/Elements/u/P60727> ;
    skos:definition "Relates a resource to a resource that uses a musical resource in a television program."@en .

<http://rdaregistry.info/Elements/u/P60729>
    reg:hasSubproperty <http://rdaregistry.info/Elements/e/P20249> ;
    reg:lexicalAlias <http://rdaregistry.info/Elements/u/radioProgramMusic.en> ;
    reg:name "radioProgramMusic"@en ;
    reg:status <http://metadataregistry.org/uri/RegStatus/1001> ;
    a rdf:Property ;
    rdfs:isDefinedBy <http://rdaregistry.info/Elements/u/> ;
    rdfs:label "is radio program music"@en ;
    rdfs:subPropertyOf <http://rdaregistry.info/Elements/u/P60723> ;
    owl:inverseOf <http://rdaregistry.info/Elements/u/P60730> ;
    skos:definition "Relates a resource to a musical resource that is used in a radio program."@en .

<http://rdaregistry.info/Elements/u/P60730>
    reg:hasSubproperty <http://rdaregistry.info/Elements/e/P20250> ;
    reg:lexicalAlias <http://rdaregistry.info/Elements/u/musicForRadioProgram.en> ;
    reg:name "musicForRadioProgram"@en ;
    reg:status <http://metadataregistry.org/uri/RegStatus/1001> ;
    a rdf:Property ;
    rdfs:isDefinedBy <http://rdaregistry.info/Elements/u/> ;
    rdfs:label "is music for radio program"@en ;
    rdfs:subPropertyOf <http://rdaregistry.info/Elements/u/P60724> ;
    owl:inverseOf <http://rdaregistry.info/Elements/u/P60729> ;
    skos:definition "Relates a resource to a resource that uses a musical resource in a radio program."@en .

<http://rdaregistry.info/Elements/u/P60731>
    reg:hasSubproperty <http://rdaregistry.info/Elements/e/P20251> ;
    reg:lexicalAlias <http://rdaregistry.info/Elements/u/musicForMotionPicture.en> ;
    reg:name "musicForMotionPicture"@en ;
    reg:status <http://metadataregistry.org/uri/RegStatus/1001> ;
    a rdf:Property ;
    rdfs:isDefinedBy <http://rdaregistry.info/Elements/u/> ;
    rdfs:label "is music for motion picture"@en ;
    rdfs:subPropertyOf <http://rdaregistry.info/Elements/u/P60723> ;
    owl:inverseOf <http://rdaregistry.info/Elements/u/P60732> ;
    skos:definition "Relates a resource to a resource that uses a musical resource in a motion picture."@en .

<http://rdaregistry.info/Elements/u/P60732>
    reg:hasSubproperty <http://rdaregistry.info/Elements/e/P20252> ;
    reg:lexicalAlias <http://rdaregistry.info/Elements/u/motionPictureMusic.en> ;
    reg:name "motionPictureMusic"@en ;
    reg:status <http://metadataregistry.org/uri/RegStatus/1001> ;
    a rdf:Property ;
    rdfs:isDefinedBy <http://rdaregistry.info/Elements/u/> ;
    rdfs:label "is motion picture music"@en ;
    rdfs:subPropertyOf <http://rdaregistry.info/Elements/u/P60723> ;
    owl:inverseOf <http://rdaregistry.info/Elements/u/P60731> ;
    skos:definition "Relates a resource to a musical resource that is used in a motion picture."@en .

<http://rdaregistry.info/Elements/u/P60733>
    reg:hasSubproperty <http://rdaregistry.info/Elements/a/P50229> ;
    reg:lexicalAlias <http://rdaregistry.info/Elements/u/predecessorOfSplit.en> ;
    reg:name "predecessorOfSplit"@en ;
    reg:status <http://metadataregistry.org/uri/RegStatus/1001> ;
    a rdf:Property ;
    rdfs:isDefinedBy <http://rdaregistry.info/Elements/u/> ;
    rdfs:label "has predecessor of split"@en ;
    owl:inverseOf <http://rdaregistry.info/Elements/u/P60685> ;
    skos:definition "Relates an agent that split or divided into another agent to an agent."@en .

<http://rdaregistry.info/Elements/u/P60736>
    reg:hasSubproperty <http://rdaregistry.info/Elements/a/P50232> ;
    reg:lexicalAlias <http://rdaregistry.info/Elements/u/componentOfMerger.en> ;
    reg:name "componentOfMerger"@en ;
    reg:status <http://metadataregistry.org/uri/RegStatus/1001> ;
    a rdf:Property ;
    rdfs:isDefinedBy <http://rdaregistry.info/Elements/u/> ;
    rdfs:label "has component of merger"@en ;
    owl:inverseOf <http://rdaregistry.info/Elements/u/P60684> ;
    skos:definition "Relates an agent that formed another agent by merging with one or more other agents to an agent."@en .

<http://rdaregistry.info/Elements/u/P60737>
    reg:hasSubproperty <http://rdaregistry.info/Elements/a/P50234>, <http://rdaregistry.info/Elements/u/P60865>, <http://rdaregistry.info/Elements/u/P60867> ;
    reg:lexicalAlias <http://rdaregistry.info/Elements/u/officerOf.en> ;
    reg:name "officerOf"@en ;
    reg:status <http://metadataregistry.org/uri/RegStatus/1001> ;
    a rdf:Property ;
    rdfs:isDefinedBy <http://rdaregistry.info/Elements/u/> ;
    rdfs:label "has officer of"@en ;
    rdfs:subPropertyOf <http://rdaregistry.info/Elements/u/P60454> ;
    owl:inverseOf <http://rdaregistry.info/Elements/u/P60633> ;
    skos:definition "Relates an agent to an agent holding an office in or commanding an agent."@en .

<http://rdaregistry.info/Elements/u/P60738>
    reg:lexicalAlias <http://rdaregistry.info/Elements/u/broaderAffiliatedAgent.en> ;
    reg:name "broaderAffiliatedAgent"@en ;
    reg:status <http://metadataregistry.org/uri/RegStatus/1001> ;
    a rdf:Property ;
    rdfs:isDefinedBy <http://rdaregistry.info/Elements/u/> ;
    rdfs:label "has broader affiliated agent"@en ;
    skos:definition "Relates an agent that acts for a local affiliated agent and others at a broader organizational level to an agent."@en .

<http://rdaregistry.info/Elements/u/P60739>
    reg:lexicalAlias <http://rdaregistry.info/Elements/u/localAffiliate.en> ;
    reg:name "localAffiliate"@en ;
    reg:status <http://metadataregistry.org/uri/RegStatus/1001> ;
    a rdf:Property ;
    rdfs:isDefinedBy <http://rdaregistry.info/Elements/u/> ;
    rdfs:label "has local affiliate"@en ;
    skos:definition "Relates a local agent affiliated with a broader agent which acts for it and others at a broader organizational level to an agent."@en .

<http://rdaregistry.info/Elements/u/P60740>
    reg:lexicalAlias <http://rdaregistry.info/Elements/u/choreography.en> ;
    reg:name "choreography"@en ;
    reg:status <http://metadataregistry.org/uri/RegStatus/1001> ;
    a rdf:Property ;
    rdfs:isDefinedBy <http://rdaregistry.info/Elements/u/> ;
    rdfs:label "is choreography"@en ;
    rdfs:subPropertyOf <http://rdaregistry.info/Elements/u/P60198> ;
    owl:inverseOf <http://rdaregistry.info/Elements/u/P60741> ;
    skos:definition "Relates a resource to a resource that provides choreography for use in a related resource."@en .

<http://rdaregistry.info/Elements/u/P60741>
    reg:lexicalAlias <http://rdaregistry.info/Elements/u/choreographyFor.en> ;
    reg:name "choreographyFor"@en ;
    reg:status <http://metadataregistry.org/uri/RegStatus/1001> ;
    a rdf:Property ;
    rdfs:isDefinedBy <http://rdaregistry.info/Elements/u/> ;
    rdfs:label "is choreography for"@en ;
    rdfs:subPropertyOf <http://rdaregistry.info/Elements/u/P60198> ;
    owl:inverseOf <http://rdaregistry.info/Elements/u/P60740> ;
    skos:definition "Relates a resource to a resource that uses choreography of a related resource."@en .

<http://rdaregistry.info/Elements/u/P60742>
    reg:lexicalAlias <http://rdaregistry.info/Elements/u/adaptedAsGraphicNovel.en> ;
    reg:name "adaptedAsGraphicNovel"@en ;
    reg:status <http://metadataregistry.org/uri/RegStatus/1001> ;
    a rdf:Property ;
    rdfs:isDefinedBy <http://rdaregistry.info/Elements/u/> ;
    rdfs:label "is adapted as graphic novel"@en ;
    rdfs:subPropertyOf <http://rdaregistry.info/Elements/u/P60260> ;
    owl:inverseOf <http://rdaregistry.info/Elements/u/P60743> ;
    skos:definition "Relates a resource to a graphic novel based on a source resource"@en .

<http://rdaregistry.info/Elements/u/P60743>
    reg:lexicalAlias <http://rdaregistry.info/Elements/u/graphicNovelizationOf.en> ;
    reg:name "graphicNovelizationOf"@en ;
    reg:status <http://metadataregistry.org/uri/RegStatus/1001> ;
    a rdf:Property ;
    rdfs:isDefinedBy <http://rdaregistry.info/Elements/u/> ;
    rdfs:label "is graphic novelization of"@en ;
    rdfs:subPropertyOf <http://rdaregistry.info/Elements/u/P60241> ;
    owl:inverseOf <http://rdaregistry.info/Elements/u/P60742> ;
    skos:definition "Relates a resourcce to a resource that has been adapted as a graphic novel."@en .

<http://rdaregistry.info/Elements/u/P60744>
    reg:lexicalAlias <http://rdaregistry.info/Elements/u/adaptedAsVideoGame.en> ;
    reg:name "adaptedAsVideoGame"@en ;
    reg:status <http://metadataregistry.org/uri/RegStatus/1001> ;
    a rdf:Property ;
    rdfs:isDefinedBy <http://rdaregistry.info/Elements/u/> ;
    rdfs:label "is adapted as video game"@en ;
    rdfs:subPropertyOf <http://rdaregistry.info/Elements/u/P60260> ;
    owl:inverseOf <http://rdaregistry.info/Elements/u/P60745> ;
    skos:definition "Relates a resource to relates a resource to a video game based on a source resource."@en .

<http://rdaregistry.info/Elements/u/P60745>
    reg:lexicalAlias <http://rdaregistry.info/Elements/u/videoGameAdaptationOf.en> ;
    reg:name "videoGameAdaptationOf"@en ;
    reg:status <http://metadataregistry.org/uri/RegStatus/1001> ;
    a rdf:Property ;
    rdfs:isDefinedBy <http://rdaregistry.info/Elements/u/> ;
    rdfs:label "is video game adaptation of"@en ;
    rdfs:subPropertyOf <http://rdaregistry.info/Elements/u/P60241> ;
    owl:inverseOf <http://rdaregistry.info/Elements/u/P60744> ;
    skos:definition "Relates a resource to a resource that has been adapted as a video game."@en .

<http://rdaregistry.info/Elements/u/P60746>
    reg:lexicalAlias <http://rdaregistry.info/Elements/u/papermaker.en> ;
    reg:name "papermaker"@en ;
    reg:status <http://metadataregistry.org/uri/RegStatus/1001> ;
    a rdf:Property ;
    rdfs:isDefinedBy <http://rdaregistry.info/Elements/u/> ;
    rdfs:label "has papermaker"@en ;
    rdfs:subPropertyOf <http://rdaregistry.info/Elements/u/P60443> ;
    owl:inverseOf <http://rdaregistry.info/Elements/u/P60747> ;
    skos:definition "Relates a resource to an agent responsible for the production of paper used to manufacture a resource."@en .

<http://rdaregistry.info/Elements/u/P60747>
    reg:lexicalAlias <http://rdaregistry.info/Elements/u/papermakerOf.en> ;
    reg:name "papermakerOf"@en ;
    reg:status <http://metadataregistry.org/uri/RegStatus/1001> ;
    a rdf:Property ;
    rdfs:isDefinedBy <http://rdaregistry.info/Elements/u/> ;
    rdfs:label "is papermaker of"@en ;
    rdfs:subPropertyOf <http://rdaregistry.info/Elements/u/P60669> ;
    owl:inverseOf <http://rdaregistry.info/Elements/u/P60746> ;
    skos:definition "Relates an agent responsible for the production of paper used to manufacture a resource to a resource."@en .

<http://rdaregistry.info/Elements/u/P60748>
    reg:lexicalAlias <http://rdaregistry.info/Elements/u/visualEffectsProvider.en> ;
    reg:name "visualEffectsProvider"@en ;
    reg:status <http://metadataregistry.org/uri/RegStatus/1001> ;
    a rdf:Property ;
    rdfs:isDefinedBy <http://rdaregistry.info/Elements/u/> ;
    rdfs:label "has visual effects provider"@en ;
    rdfs:subPropertyOf <http://rdaregistry.info/Elements/u/P60398> ;
    owl:inverseOf <http://rdaregistry.info/Elements/u/P60754> ;
    skos:definition "Relates a resource to an agent contributing to an expression of a moving image resource by designing and creating post-production visual effects."@en .

<http://rdaregistry.info/Elements/u/P60749>
    reg:lexicalAlias <http://rdaregistry.info/Elements/u/specialEffectsProvider.en> ;
    reg:name "specialEffectsProvider"@en ;
    reg:status <http://metadataregistry.org/uri/RegStatus/1001> ;
    a rdf:Property ;
    rdfs:isDefinedBy <http://rdaregistry.info/Elements/u/> ;
    rdfs:label "has special effects provider"@en ;
    rdfs:subPropertyOf <http://rdaregistry.info/Elements/u/P60398> ;
    owl:inverseOf <http://rdaregistry.info/Elements/u/P60755> ;
    skos:definition "Relates a resource to an agent contributing to a moving image or audio resource by designing and creating on-set special effects such as on-set mechanical effects and in-camera optical effects."@en .

<http://rdaregistry.info/Elements/u/P60750>
    reg:lexicalAlias <http://rdaregistry.info/Elements/u/letterer.en> ;
    reg:name "letterer"@en ;
    reg:status <http://metadataregistry.org/uri/RegStatus/1001> ;
    a rdf:Property ;
    rdfs:isDefinedBy <http://rdaregistry.info/Elements/u/> ;
    rdfs:label "has letterer"@en ;
    rdfs:subPropertyOf <http://rdaregistry.info/Elements/u/P60396> ;
    owl:inverseOf <http://rdaregistry.info/Elements/u/P60756> ;
    skos:definition "Relates a resource to an illustrator contributing to a comic book, graphic novel, etc., by drawing text and graphic sound effects."@en .

<http://rdaregistry.info/Elements/u/P60751>
    rdakit:seeAlso <http://rdaregistry.info/Elements/u/P60446> ;
    reg:lexicalAlias <http://rdaregistry.info/Elements/u/rapporteur.en> ;
    reg:name "rapporteur"@en ;
    reg:status <http://metadataregistry.org/uri/RegStatus/1001> ;
    a rdf:Property ;
    rdfs:isDefinedBy <http://rdaregistry.info/Elements/u/> ;
    rdfs:label "has rapporteur"@en ;
    rdfs:subPropertyOf <http://rdaregistry.info/Elements/u/P60434> ;
    owl:inverseOf <http://rdaregistry.info/Elements/u/P60757> ;
    skos:definition "Relates a resource to an author who is appointed by an organization to report on the proceedings of its meetings."@en ;
    skos:scopeNote "Responsibility limited to taking minutes is excluded."@en .

<http://rdaregistry.info/Elements/u/P60752>
    reg:lexicalAlias <http://rdaregistry.info/Elements/u/calligrapher.en> ;
    reg:name "calligrapher"@en ;
    reg:status <http://metadataregistry.org/uri/RegStatus/1001> ;
    a rdf:Property ;
    rdfs:isDefinedBy <http://rdaregistry.info/Elements/u/> ;
    rdfs:label "has calligrapher"@en ;
    rdfs:subPropertyOf <http://rdaregistry.info/Elements/u/P60431> ;
    owl:inverseOf <http://rdaregistry.info/Elements/u/P60758> ;
    skos:definition "Relates a resource to an artist responsible for creating a resource of calligraphy where a focus of interest lies in the aesthetic value of its penmanship or graphic artistry, regardless of whether the same agent also authored the inscribed text."@en .

<http://rdaregistry.info/Elements/u/P60753>
    reg:lexicalAlias <http://rdaregistry.info/Elements/u/bookArtist.en> ;
    reg:name "bookArtist"@en ;
    reg:status <http://metadataregistry.org/uri/RegStatus/1001> ;
    a rdf:Property ;
    rdfs:isDefinedBy <http://rdaregistry.info/Elements/u/> ;
    rdfs:label "has book artist"@en ;
    rdfs:subPropertyOf <http://rdaregistry.info/Elements/u/P60431> ;
    owl:inverseOf <http://rdaregistry.info/Elements/u/P60759> ;
    skos:definition "Relates a resource to an artist responsible for creating art resources that exploit a book form or alter its physical structure as part of a content of a resource."@en .

<http://rdaregistry.info/Elements/u/P60754>
    reg:lexicalAlias <http://rdaregistry.info/Elements/u/visualEffectsProviderOf.en> ;
    reg:name "visualEffectsProviderOf"@en ;
    reg:status <http://metadataregistry.org/uri/RegStatus/1001> ;
    a rdf:Property ;
    rdfs:isDefinedBy <http://rdaregistry.info/Elements/u/> ;
    rdfs:label "is visual effects provider of"@en ;
    rdfs:subPropertyOf <http://rdaregistry.info/Elements/u/P60626> ;
    owl:inverseOf <http://rdaregistry.info/Elements/u/P60748> ;
    skos:definition "Relates an agent contributing to an expression of a moving image resource by designing and creating post-production visual effects to a resource."@en .

<http://rdaregistry.info/Elements/u/P60755>
    reg:lexicalAlias <http://rdaregistry.info/Elements/u/specialEffectsProviderOf.en> ;
    reg:name "specialEffectsProviderOf"@en ;
    reg:status <http://metadataregistry.org/uri/RegStatus/1001> ;
    a rdf:Property ;
    rdfs:isDefinedBy <http://rdaregistry.info/Elements/u/> ;
    rdfs:label "is special effects provider of"@en ;
    rdfs:subPropertyOf <http://rdaregistry.info/Elements/u/P60626> ;
    owl:inverseOf <http://rdaregistry.info/Elements/u/P60749> ;
    skos:definition "Relates an agent contributing to a moving image or audio resource by designing and creating on-set special effects, such as on-set mechanical effects and in-camera optical effects, to a resource."@en .

<http://rdaregistry.info/Elements/u/P60756>
    reg:lexicalAlias <http://rdaregistry.info/Elements/u/lettererOf.en> ;
    reg:name "lettererOf"@en ;
    reg:status <http://metadataregistry.org/uri/RegStatus/1001> ;
    a rdf:Property ;
    rdfs:isDefinedBy <http://rdaregistry.info/Elements/u/> ;
    rdfs:label "is letterer of"@en ;
    rdfs:subPropertyOf <http://rdaregistry.info/Elements/u/P60624> ;
    owl:inverseOf <http://rdaregistry.info/Elements/u/P60750> ;
    skos:definition "Relates an illustrator contributing to a comic book, graphic novel, etc., by drawing text and graphic sound effects to a resource."@en .

<http://rdaregistry.info/Elements/u/P60757>
    rdakit:seeAlso <http://rdaregistry.info/Elements/u/P60708> ;
    reg:lexicalAlias <http://rdaregistry.info/Elements/u/rapporteurOf.en> ;
    reg:name "rapporteurOf"@en ;
    reg:status <http://metadataregistry.org/uri/RegStatus/1001> ;
    a rdf:Property ;
    rdfs:isDefinedBy <http://rdaregistry.info/Elements/u/> ;
    rdfs:label "is rapporteur of"@en ;
    rdfs:subPropertyOf <http://rdaregistry.info/Elements/u/P60663> ;
    owl:inverseOf <http://rdaregistry.info/Elements/u/P60751> ;
    skos:definition "Relates an author who is appointed by an organization to report on the proceedings of its meetings to a resource."@en .

<http://rdaregistry.info/Elements/u/P60758>
    reg:lexicalAlias <http://rdaregistry.info/Elements/u/calligrapherOf.en> ;
    reg:name "calligrapherOf"@en ;
    reg:status <http://metadataregistry.org/uri/RegStatus/1001> ;
    a rdf:Property ;
    rdfs:isDefinedBy <http://rdaregistry.info/Elements/u/> ;
    rdfs:label "is calligrapher of"@en ;
    rdfs:subPropertyOf <http://rdaregistry.info/Elements/u/P60660> ;
    owl:inverseOf <http://rdaregistry.info/Elements/u/P60752> ;
    skos:definition "Relates an artist responsible for creating a resource of calligraphy where a focus of interest lies in the aesthetic value of its penmanship or graphic artistry, regardless of whether the same agent also authored the inscribed text to a resource."@en .

<http://rdaregistry.info/Elements/u/P60759>
    reg:lexicalAlias <http://rdaregistry.info/Elements/u/bookArtistOf.en> ;
    reg:name "bookArtistOf"@en ;
    reg:status <http://metadataregistry.org/uri/RegStatus/1001> ;
    a rdf:Property ;
    rdfs:isDefinedBy <http://rdaregistry.info/Elements/u/> ;
    rdfs:label "is book artist of"@en ;
    rdfs:subPropertyOf <http://rdaregistry.info/Elements/u/P60660> ;
    owl:inverseOf <http://rdaregistry.info/Elements/u/P60753> ;
    skos:definition "Relates an artist responsible for creating art resources that exploit a book form or alter its physical structure as part of the content of a resource to a resource."@en .

<http://rdaregistry.info/Elements/u/P60760>
    reg:lexicalAlias <http://rdaregistry.info/Elements/u/detailsOfAspectRatioDesignation.en> ;
    reg:name "detailsOfAspectRatioDesignation"@en ;
    reg:status <http://metadataregistry.org/uri/RegStatus/1001> ;
    a rdf:Property ;
    rdfs:isDefinedBy <http://rdaregistry.info/Elements/u/> ;
    rdfs:label "has details of aspect ratio designation"@en ;
    skos:definition "Relates a resource to details of the ratio of the width to the height of a moving image."@en .

<http://rdaregistry.info/Elements/u/P60761>
    reg:lexicalAlias <http://rdaregistry.info/Elements/u/detailsOfColourContent.en> ;
    reg:name "detailsOfColourContent"@en ;
    reg:status <http://metadataregistry.org/uri/RegStatus/1001> ;
    a rdf:Property ;
    rdfs:isDefinedBy <http://rdaregistry.info/Elements/u/> ;
    rdfs:label "has details of colour content"@en ;
    skos:altLabel "has details of color content"@en ;
    skos:definition "Relates a resource to details of the presence of colour, tone, etc., in the content of a resource, and the specific colours, tones, etc., including black and white, present."@en .

<http://rdaregistry.info/Elements/u/P60762>
    reg:lexicalAlias <http://rdaregistry.info/Elements/u/detailsOfFormOfMusicalNotation.en> ;
    reg:name "detailsOfFormOfMusicalNotation"@en ;
    reg:status <http://metadataregistry.org/uri/RegStatus/1001> ;
    a rdf:Property ;
    rdfs:isDefinedBy <http://rdaregistry.info/Elements/u/> ;
    rdfs:label "has details of form of musical notation"@en ;
    skos:definition "Relates a resource to details of a set of characters or symbols used to express musical content of a resource."@en .

<http://rdaregistry.info/Elements/u/P60763>
    reg:lexicalAlias <http://rdaregistry.info/Elements/u/detailsOfFormOfNotatedMovement.en> ;
    reg:name "detailsOfFormOfNotatedMovement"@en ;
    reg:status <http://metadataregistry.org/uri/RegStatus/1001> ;
    a rdf:Property ;
    rdfs:isDefinedBy <http://rdaregistry.info/Elements/u/> ;
    rdfs:label "has details of form of notated movement"@en ;
    skos:definition "Relates a resource to details of a set of characters or symbols used to express movement content of a resource."@en .

<http://rdaregistry.info/Elements/u/P60764>
    reg:lexicalAlias <http://rdaregistry.info/Elements/u/detailsOfFormatOfNotatedMusic.en> ;
    reg:name "detailsOfFormatOfNotatedMusic"@en ;
    reg:status <http://metadataregistry.org/uri/RegStatus/1001> ;
    a rdf:Property ;
    rdfs:isDefinedBy <http://rdaregistry.info/Elements/u/> ;
    rdfs:label "has details of format of notated music"@en ;
    skos:definition "Relates a resource to details of a musical or physical layout of the content of a resource that is presented in a form of musical notation."@en .

<http://rdaregistry.info/Elements/u/P60765>
    reg:lexicalAlias <http://rdaregistry.info/Elements/u/detailsOfFormOfTactileNotation.en> ;
    reg:name "detailsOfFormOfTactileNotation"@en ;
    reg:status <http://metadataregistry.org/uri/RegStatus/1001> ;
    a rdf:Property ;
    rdfs:isDefinedBy <http://rdaregistry.info/Elements/u/> ;
    rdfs:label "has details of form of tactile notation"@en ;
    skos:definition "Relates a resource to details of a set of characters or symbols used to express the content of a resource in a form that can be perceived through touch."@en .

<http://rdaregistry.info/Elements/u/P60766>
    reg:lexicalAlias <http://rdaregistry.info/Elements/u/detailsOfScript.en> ;
    reg:name "detailsOfScript"@en ;
    reg:status <http://metadataregistry.org/uri/RegStatus/1001> ;
    a rdf:Property ;
    rdfs:isDefinedBy <http://rdaregistry.info/Elements/u/> ;
    rdfs:label "has details of script"@en ;
    skos:definition "Relates a resource to details of set of characters or symbols used to express written language content of a resource."@en .

<http://rdaregistry.info/Elements/u/P60767>
    reg:hasSubproperty <http://rdaregistry.info/Elements/u/P60774> ;
    reg:lexicalAlias <http://rdaregistry.info/Elements/u/detailsOfAppliedMaterial.en> ;
    reg:name "detailsOfAppliedMaterial"@en ;
    reg:status <http://metadataregistry.org/uri/RegStatus/1001> ;
    a rdf:Property ;
    rdfs:isDefinedBy <http://rdaregistry.info/Elements/u/> ;
    rdfs:label "has details of applied material"@en ;
    skos:definition "Relates a resource to details of a physical or chemical substance applied to a base material of a resource."@en .

<http://rdaregistry.info/Elements/u/P60768>
    reg:lexicalAlias <http://rdaregistry.info/Elements/u/detailsOfBaseMaterial.en> ;
    reg:name "detailsOfBaseMaterial"@en ;
    reg:status <http://metadataregistry.org/uri/RegStatus/1001> ;
    a rdf:Property ;
    rdfs:isDefinedBy <http://rdaregistry.info/Elements/u/> ;
    rdfs:label "has details of base material"@en ;
    skos:definition "Relates a resource to details of an underlying physical material of a resource."@en .

<http://rdaregistry.info/Elements/u/P60769>
    reg:lexicalAlias <http://rdaregistry.info/Elements/u/detailsOfBibliographicFormat.en> ;
    reg:name "detailsOfBibliographicFormat"@en ;
    reg:status <http://metadataregistry.org/uri/RegStatus/1001> ;
    a rdf:Property ;
    rdfs:isDefinedBy <http://rdaregistry.info/Elements/u/> ;
    rdfs:label "has details of bibliographic format"@en ;
    skos:definition "Relates a resource to details of the proportional relationship between a whole sheet in a printed or manuscript resource, and the individual leaves that result if that sheet is left full, cut, or folded."@en .

<http://rdaregistry.info/Elements/u/P60770>
    reg:lexicalAlias <http://rdaregistry.info/Elements/u/detailsOfBroadcastStandard.en> ;
    reg:name "detailsOfBroadcastStandard"@en ;
    reg:status <http://metadataregistry.org/uri/RegStatus/1001> ;
    a rdf:Property ;
    rdfs:isDefinedBy <http://rdaregistry.info/Elements/u/> ;
    rdfs:label "has details of broadcast standard"@en ;
    rdfs:subPropertyOf <http://rdaregistry.info/Elements/u/P60801> ;
    skos:definition "Relates a resource to details of a system used to format a video resource for television broadcast."@en .

<http://rdaregistry.info/Elements/u/P60771>
    reg:lexicalAlias <http://rdaregistry.info/Elements/u/detailsOfConfigurationOfPlaybackChannels.en> ;
    reg:name "detailsOfConfigurationOfPlaybackChannels"@en ;
    reg:status <http://metadataregistry.org/uri/RegStatus/1001> ;
    a rdf:Property ;
    rdfs:isDefinedBy <http://rdaregistry.info/Elements/u/> ;
    rdfs:label "has details of configuration of playback channels"@en ;
    rdfs:subPropertyOf <http://rdaregistry.info/Elements/u/P60796> ;
    skos:definition "Relates a resource to details of a number of sound channels used to make a recording."@en .

<http://rdaregistry.info/Elements/u/P60772>
    reg:hasSubproperty <http://rdaregistry.info/Elements/u/P60773>, <http://rdaregistry.info/Elements/u/P60775>, <http://rdaregistry.info/Elements/u/P60776> ;
    reg:lexicalAlias <http://rdaregistry.info/Elements/u/detailsOfDigitalFileCharacteristic.en> ;
    reg:name "detailsOfDigitalFileCharacteristic"@en ;
    reg:status <http://metadataregistry.org/uri/RegStatus/1001> ;
    a rdf:Property ;
    rdfs:isDefinedBy <http://rdaregistry.info/Elements/u/> ;
    rdfs:label "has details of digital file characteristic"@en ;
    skos:definition "Relates a resource to details of a technical specification relating to a digital encoding of text, image, audio, video, and other types of data in a resource."@en .

<http://rdaregistry.info/Elements/u/P60773>
    reg:lexicalAlias <http://rdaregistry.info/Elements/u/detailsOfDigitalRepresentationOfCartographicContent.en> ;
    reg:name "detailsOfDigitalRepresentationOfCartographicContent"@en ;
    reg:status <http://metadataregistry.org/uri/RegStatus/1001> ;
    a rdf:Property ;
    rdfs:isDefinedBy <http://rdaregistry.info/Elements/u/> ;
    rdfs:label "has details of digital representation of cartographic content"@en ;
    rdfs:subPropertyOf <http://rdaregistry.info/Elements/u/P60772> ;
    skos:definition "Relates a resource to details of an encoding of geospatial information in a cartographic resource."@en .

<http://rdaregistry.info/Elements/u/P60774>
    reg:lexicalAlias <http://rdaregistry.info/Elements/u/detailsOfEmulsionOnMicrofilmAndMicrofiche.en> ;
    reg:name "detailsOfEmulsionOnMicrofilmAndMicrofiche"@en ;
    reg:status <http://metadataregistry.org/uri/RegStatus/1001> ;
    a rdf:Property ;
    rdfs:isDefinedBy <http://rdaregistry.info/Elements/u/> ;
    rdfs:label "has details of emulsion on microfilm and microfiche"@en ;
    rdfs:subPropertyOf <http://rdaregistry.info/Elements/u/P60767> ;
    skos:definition "Relates a resource to details of a suspension of light-sensitive chemicals used as a coating on a microfilm or microfiche."@en .

<http://rdaregistry.info/Elements/u/P60775>
    reg:lexicalAlias <http://rdaregistry.info/Elements/u/detailsOfEncodingFormat.en> ;
    reg:name "detailsOfEncodingFormat"@en ;
    reg:status <http://metadataregistry.org/uri/RegStatus/1001> ;
    a rdf:Property ;
    rdfs:isDefinedBy <http://rdaregistry.info/Elements/u/> ;
    rdfs:label "has details of encoding format"@en ;
    rdfs:subPropertyOf <http://rdaregistry.info/Elements/u/P60772> ;
    skos:definition "Relates a resource to details of a schema, standard, etc., used to encode the digital content of a resource."@en .

<http://rdaregistry.info/Elements/u/P60776>
    reg:lexicalAlias <http://rdaregistry.info/Elements/u/detailsOfFileType.en> ;
    reg:name "detailsOfFileType"@en ;
    reg:status <http://metadataregistry.org/uri/RegStatus/1001> ;
    a rdf:Property ;
    rdfs:isDefinedBy <http://rdaregistry.info/Elements/u/> ;
    rdfs:label "has details of file type"@en ;
    rdfs:subPropertyOf <http://rdaregistry.info/Elements/u/P60772> ;
    skos:definition "Relates a resource to details of a general type of data content encoded in a computer file."@en .

<http://rdaregistry.info/Elements/u/P60777>
    reg:lexicalAlias <http://rdaregistry.info/Elements/u/detailsOfFontSize.en> ;
    reg:name "detailsOfFontSize"@en ;
    reg:status <http://metadataregistry.org/uri/RegStatus/1001> ;
    a rdf:Property ;
    rdfs:isDefinedBy <http://rdaregistry.info/Elements/u/> ;
    rdfs:label "has details of font size"@en ;
    skos:definition "Relates a resource to details of a size of the type used to represent characters and symbols in a resource."@en .

<http://rdaregistry.info/Elements/u/P60778>
    reg:lexicalAlias <http://rdaregistry.info/Elements/u/detailsOfGenerationOfAudioRecording.en> ;
    reg:name "detailsOfGenerationOfAudioRecording"@en ;
    reg:status <http://metadataregistry.org/uri/RegStatus/1008> ;
    a rdf:Property ;
    rdfs:isDefinedBy <http://rdaregistry.info/Elements/u/> ;
    rdfs:subPropertyOf <http://rdaregistry.info/Elements/u/P60803> ;
    skos:definition "Relates a resource to details of the relationship between an original audio carrier and the carrier of a reproduction made from the original (e.g., a tape duplication master, a test pressing)."@en .

<http://rdaregistry.info/Elements/u/P60779>
    reg:lexicalAlias <http://rdaregistry.info/Elements/u/detailsOfGenerationOfDigitalResource.en> ;
    reg:name "detailsOfGenerationOfDigitalResource"@en ;
    reg:status <http://metadataregistry.org/uri/RegStatus/1008> ;
    a rdf:Property ;
    rdfs:isDefinedBy <http://rdaregistry.info/Elements/u/> ;
    rdfs:subPropertyOf <http://rdaregistry.info/Elements/u/P60803> ;
    skos:definition "Relates a resource to details of the relationship between an original carrier of a digital resource and the carrier of a reproduction made from the original (e.g., a derivative master)."@en .

<http://rdaregistry.info/Elements/u/P60780>
    reg:lexicalAlias <http://rdaregistry.info/Elements/u/detailsOfGenerationOfMicroform.en> ;
    reg:name "detailsOfGenerationOfMicroform"@en ;
    reg:status <http://metadataregistry.org/uri/RegStatus/1008> ;
    a rdf:Property ;
    rdfs:isDefinedBy <http://rdaregistry.info/Elements/u/> ;
    rdfs:subPropertyOf <http://rdaregistry.info/Elements/u/P60803> ;
    skos:definition "Relates a resource to details of the relationship between an original microform carrier and the carrier of a reproduction made from the original (e.g., a printing master)."@en .

<http://rdaregistry.info/Elements/u/P60781>
    reg:lexicalAlias <http://rdaregistry.info/Elements/u/detailsOfGenerationOfMotionPictureFilm.en> ;
    reg:name "detailsOfGenerationOfMotionPictureFilm"@en ;
    reg:status <http://metadataregistry.org/uri/RegStatus/1008> ;
    a rdf:Property ;
    rdfs:isDefinedBy <http://rdaregistry.info/Elements/u/> ;
    rdfs:subPropertyOf <http://rdaregistry.info/Elements/u/P60803> ;
    skos:definition "Relates a resource to details of the relationship between an original carrier of a motion picture film resource and the carrier of a reproduction made from the original (e.g., a reference print)."@en .

<http://rdaregistry.info/Elements/u/P60782>
    reg:lexicalAlias <http://rdaregistry.info/Elements/u/detailsOfGenerationOfVideotape.en> ;
    reg:name "detailsOfGenerationOfVideotape"@en ;
    reg:status <http://metadataregistry.org/uri/RegStatus/1008> ;
    a rdf:Property ;
    rdfs:isDefinedBy <http://rdaregistry.info/Elements/u/> ;
    rdfs:subPropertyOf <http://rdaregistry.info/Elements/u/P60803> ;
    skos:definition "Relates a resource to details of the relationship between an original carrier of a videotape resource and the carrier of a reproduction made from the original (e.g., a show copy)."@en .

<http://rdaregistry.info/Elements/u/P60783>
    reg:lexicalAlias <http://rdaregistry.info/Elements/u/detailsOfGrooveCharacteristic.en> ;
    reg:name "detailsOfGrooveCharacteristic"@en ;
    reg:status <http://metadataregistry.org/uri/RegStatus/1001> ;
    a rdf:Property ;
    rdfs:isDefinedBy <http://rdaregistry.info/Elements/u/> ;
    rdfs:label "has details of groove characteristic"@en ;
    rdfs:subPropertyOf <http://rdaregistry.info/Elements/u/P60796> ;
    skos:definition "Relates a resource to details of a groove width of an analog disc or a groove pitch of an analog cylinder."@en .

<http://rdaregistry.info/Elements/u/P60784>
    reg:lexicalAlias <http://rdaregistry.info/Elements/u/detailsOfLayout.en> ;
    reg:name "detailsOfLayout"@en ;
    reg:status <http://metadataregistry.org/uri/RegStatus/1001> ;
    a rdf:Property ;
    rdfs:isDefinedBy <http://rdaregistry.info/Elements/u/> ;
    rdfs:label "has details of layout"@en ;
    skos:definition "Relates a resource to details of an arrangement of text, images, tactile notation, etc., in a resource."@en .

<http://rdaregistry.info/Elements/u/P60785>
    reg:lexicalAlias <http://rdaregistry.info/Elements/u/detailsOfMount.en> ;
    reg:name "detailsOfMount"@en ;
    reg:status <http://metadataregistry.org/uri/RegStatus/1001> ;
    a rdf:Property ;
    rdfs:isDefinedBy <http://rdaregistry.info/Elements/u/> ;
    rdfs:label "has details of mount"@en ;
    skos:definition "Relates a resource to details of a physical material used for the support or backing to which the base material of a resource has been attached."@en .

<http://rdaregistry.info/Elements/u/P60786>
    reg:lexicalAlias <http://rdaregistry.info/Elements/u/detailsOfPlayingSpeed.en> ;
    reg:name "detailsOfPlayingSpeed"@en ;
    reg:status <http://metadataregistry.org/uri/RegStatus/1001> ;
    a rdf:Property ;
    rdfs:isDefinedBy <http://rdaregistry.info/Elements/u/> ;
    rdfs:label "has details of playing speed"@en ;
    skos:definition "Relates a resource to details of a speed at which an audio carrier must be operated to produce the sound intended."@en .

<http://rdaregistry.info/Elements/u/P60787>
    reg:lexicalAlias <http://rdaregistry.info/Elements/u/detailsOfPolarity.en> ;
    reg:name "detailsOfPolarity"@en ;
    reg:status <http://metadataregistry.org/uri/RegStatus/1001> ;
    a rdf:Property ;
    rdfs:isDefinedBy <http://rdaregistry.info/Elements/u/> ;
    rdfs:label "has details of polarity"@en ;
    skos:definition "Relates a resource to details of a relationship of the colours and tones in an image to the colours and tones of the object reproduced."@en .

<http://rdaregistry.info/Elements/u/P60788>
    reg:lexicalAlias <http://rdaregistry.info/Elements/u/detailsOfPresentationFormat.en> ;
    reg:name "detailsOfPresentationFormat"@en ;
    reg:status <http://metadataregistry.org/uri/RegStatus/1001> ;
    a rdf:Property ;
    rdfs:isDefinedBy <http://rdaregistry.info/Elements/u/> ;
    rdfs:label "has details of presentation format"@en ;
    skos:definition "Relates a resource to details of a format used in the production of a projected image."@en .

<http://rdaregistry.info/Elements/u/P60789>
    reg:lexicalAlias <http://rdaregistry.info/Elements/u/detailsOfProductionMethod.en> ;
    reg:name "detailsOfProductionMethod"@en ;
    reg:status <http://metadataregistry.org/uri/RegStatus/1001> ;
    a rdf:Property ;
    rdfs:isDefinedBy <http://rdaregistry.info/Elements/u/> ;
    rdfs:label "has details of production method"@en ;
    skos:definition "Relates a resource to details of a process used to produce a resource."@en .

<http://rdaregistry.info/Elements/u/P60790>
    reg:lexicalAlias <http://rdaregistry.info/Elements/u/detailsOfProductionMethodForManuscript.en> ;
    reg:name "detailsOfProductionMethodForManuscript"@en ;
    reg:status <http://metadataregistry.org/uri/RegStatus/1008> ;
    a rdf:Property ;
    rdfs:isDefinedBy <http://rdaregistry.info/Elements/u/> .

<http://rdaregistry.info/Elements/u/P60791>
    reg:lexicalAlias <http://rdaregistry.info/Elements/u/detailsOfProductionMethodForTactileResource.en> ;
    reg:name "detailsOfProductionMethodForTactileResource"@en ;
    reg:status <http://metadataregistry.org/uri/RegStatus/1008> ;
    a rdf:Property ;
    rdfs:isDefinedBy <http://rdaregistry.info/Elements/u/> .

<http://rdaregistry.info/Elements/u/P60792>
    reg:hasSubproperty <http://rdaregistry.info/Elements/u/P60793> ;
    reg:lexicalAlias <http://rdaregistry.info/Elements/u/detailsOfProjectionCharacteristicOfMotionPictureFilm.en> ;
    reg:name "detailsOfProjectionCharacteristicOfMotionPictureFilm"@en ;
    reg:status <http://metadataregistry.org/uri/RegStatus/1001> ;
    a rdf:Property ;
    rdfs:isDefinedBy <http://rdaregistry.info/Elements/u/> ;
    rdfs:label "has details of projection characteristic of motion picture film"@en ;
    skos:definition "Relates a resource to details of a technical specification relating to the projection of a motion picture film."@en .

<http://rdaregistry.info/Elements/u/P60793>
    reg:lexicalAlias <http://rdaregistry.info/Elements/u/detailsOfProjectionSpeed.en> ;
    reg:name "detailsOfProjectionSpeed"@en ;
    reg:status <http://metadataregistry.org/uri/RegStatus/1001> ;
    a rdf:Property ;
    rdfs:isDefinedBy <http://rdaregistry.info/Elements/u/> ;
    rdfs:label "has details of projection speed"@en ;
    rdfs:subPropertyOf <http://rdaregistry.info/Elements/u/P60792> ;
    skos:definition "Relates a resource to details of a speed at which a projected carrier must be operated to produce the moving image intended."@en .

<http://rdaregistry.info/Elements/u/P60794>
    reg:lexicalAlias <http://rdaregistry.info/Elements/u/detailsOfRecordingMedium.en> ;
    reg:name "detailsOfRecordingMedium"@en ;
    reg:status <http://metadataregistry.org/uri/RegStatus/1001> ;
    a rdf:Property ;
    rdfs:isDefinedBy <http://rdaregistry.info/Elements/u/> ;
    rdfs:label "has details of recording medium"@en ;
    rdfs:subPropertyOf <http://rdaregistry.info/Elements/u/P60796> ;
    skos:definition "Relates a resource to details of a type of medium used to record sound on an audio carrier."@en .

<http://rdaregistry.info/Elements/u/P60795>
    reg:lexicalAlias <http://rdaregistry.info/Elements/u/detailsOfReductionRatioDesignation.en> ;
    reg:name "detailsOfReductionRatioDesignation"@en ;
    reg:status <http://metadataregistry.org/uri/RegStatus/1001> ;
    a rdf:Property ;
    rdfs:isDefinedBy <http://rdaregistry.info/Elements/u/> ;
    rdfs:label "has details of reduction ratio designation"@en ;
    skos:definition "Relates a resource to details of a designation of the size of a micro-image to an original from which it was produced."@en .

<http://rdaregistry.info/Elements/u/P60796>
    reg:hasSubproperty <http://rdaregistry.info/Elements/u/P60771>, <http://rdaregistry.info/Elements/u/P60783>, <http://rdaregistry.info/Elements/u/P60794>, <http://rdaregistry.info/Elements/u/P60797>, <http://rdaregistry.info/Elements/u/P60798>, <http://rdaregistry.info/Elements/u/P60799>, <http://rdaregistry.info/Elements/u/P60800> ;
    reg:lexicalAlias <http://rdaregistry.info/Elements/u/detailsOfSoundCharacteristic.en> ;
    reg:name "detailsOfSoundCharacteristic"@en ;
    reg:status <http://metadataregistry.org/uri/RegStatus/1001> ;
    a rdf:Property ;
    rdfs:isDefinedBy <http://rdaregistry.info/Elements/u/> ;
    rdfs:label "has details of sound characteristic"@en ;
    skos:definition "Relates a resource to details of a technical specification relating to the encoding of sound in a resource."@en .

<http://rdaregistry.info/Elements/u/P60797>
    reg:lexicalAlias <http://rdaregistry.info/Elements/u/detailsOfSpecialPlaybackCharacteristic.en> ;
    reg:name "detailsOfSpecialPlaybackCharacteristic"@en ;
    reg:status <http://metadataregistry.org/uri/RegStatus/1001> ;
    a rdf:Property ;
    rdfs:isDefinedBy <http://rdaregistry.info/Elements/u/> ;
    rdfs:label "has details of special playback characteristic"@en ;
    rdfs:subPropertyOf <http://rdaregistry.info/Elements/u/P60796> ;
    skos:definition "Relates a resource to details of an equalization system, noise reduction system, etc., used in making an audio recording."@en .

<http://rdaregistry.info/Elements/u/P60798>
    reg:lexicalAlias <http://rdaregistry.info/Elements/u/detailsOfTapeConfiguration.en> ;
    reg:name "detailsOfTapeConfiguration"@en ;
    reg:status <http://metadataregistry.org/uri/RegStatus/1001> ;
    a rdf:Property ;
    rdfs:isDefinedBy <http://rdaregistry.info/Elements/u/> ;
    rdfs:label "has details of tape configuration"@en ;
    rdfs:subPropertyOf <http://rdaregistry.info/Elements/u/P60796> ;
    skos:definition "Relates a resource to details of a number of tracks on an audiotape."@en .

<http://rdaregistry.info/Elements/u/P60799>
    reg:lexicalAlias <http://rdaregistry.info/Elements/u/detailsOfTrackConfiguration.en> ;
    reg:name "detailsOfTrackConfiguration"@en ;
    reg:status <http://metadataregistry.org/uri/RegStatus/1001> ;
    a rdf:Property ;
    rdfs:isDefinedBy <http://rdaregistry.info/Elements/u/> ;
    rdfs:label "has details of track configuration"@en ;
    rdfs:subPropertyOf <http://rdaregistry.info/Elements/u/P60796> ;
    skos:definition "Relates a resource to details of a configuration of the audio track on a sound-track film."@en .

<http://rdaregistry.info/Elements/u/P60800>
    reg:lexicalAlias <http://rdaregistry.info/Elements/u/detailsOfTypeOfRecording.en> ;
    reg:name "detailsOfTypeOfRecording"@en ;
    reg:status <http://metadataregistry.org/uri/RegStatus/1001> ;
    a rdf:Property ;
    rdfs:isDefinedBy <http://rdaregistry.info/Elements/u/> ;
    rdfs:label "has details of type of recording"@en ;
    rdfs:subPropertyOf <http://rdaregistry.info/Elements/u/P60796> ;
    skos:definition "Relates a resource to details of a method used to encode audio content for playback."@en .

<http://rdaregistry.info/Elements/u/P60801>
    reg:hasSubproperty <http://rdaregistry.info/Elements/u/P60770>, <http://rdaregistry.info/Elements/u/P60802> ;
    reg:lexicalAlias <http://rdaregistry.info/Elements/u/detailsOfVideoCharacteristic.en> ;
    reg:name "detailsOfVideoCharacteristic"@en ;
    reg:status <http://metadataregistry.org/uri/RegStatus/1001> ;
    a rdf:Property ;
    rdfs:isDefinedBy <http://rdaregistry.info/Elements/u/> ;
    rdfs:label "has details of video characteristic"@en ;
    skos:definition "Relates a resource to details of a technical specification relating to an encoding of video images in a resource."@en .

<http://rdaregistry.info/Elements/u/P60802>
    reg:lexicalAlias <http://rdaregistry.info/Elements/u/detailsOfVideoFormat.en> ;
    reg:name "detailsOfVideoFormat"@en ;
    reg:status <http://metadataregistry.org/uri/RegStatus/1001> ;
    a rdf:Property ;
    rdfs:isDefinedBy <http://rdaregistry.info/Elements/u/> ;
    rdfs:label "has details of video format"@en ;
    rdfs:subPropertyOf <http://rdaregistry.info/Elements/u/P60801> ;
    skos:definition "Relates a resource to details of a standard, etc., used to encode the analog video content of a resource."@en .

<http://rdaregistry.info/Elements/u/P60803>
    reg:hasSubproperty <http://rdaregistry.info/Elements/u/P60778>, <http://rdaregistry.info/Elements/u/P60779>, <http://rdaregistry.info/Elements/u/P60780>, <http://rdaregistry.info/Elements/u/P60781>, <http://rdaregistry.info/Elements/u/P60782> ;
    reg:lexicalAlias <http://rdaregistry.info/Elements/u/detailsOfGeneration.en> ;
    reg:name "detailsOfGeneration"@en ;
    reg:status <http://metadataregistry.org/uri/RegStatus/1001> ;
    a rdf:Property ;
    rdfs:isDefinedBy <http://rdaregistry.info/Elements/u/> ;
    rdfs:label "has details of generation"@en ;
    skos:definition "Relates a resource to details of a relationship between an original carrier and a carrier of a reproduction made from an original."@en .

<http://rdaregistry.info/Elements/u/P60804>
    reg:lexicalAlias <http://rdaregistry.info/Elements/u/detailsOfIllustrativeContent.en> ;
    reg:name "detailsOfIllustrativeContent"@en ;
    reg:status <http://metadataregistry.org/uri/RegStatus/1001> ;
    a rdf:Property ;
    rdfs:isDefinedBy <http://rdaregistry.info/Elements/u/> ;
    rdfs:label "has details of illustrative content"@en ;
    skos:definition "Relates a resource to details of a presence of one or more still images that accompany the primary content of a resource."@en, "Relates a resource to details of content intended to illustrate a primary content of a resource."@en .

<http://rdaregistry.info/Elements/u/P60805>
    reg:hasSubproperty <http://rdaregistry.info/Elements/w/P10324> ;
    reg:lexicalAlias <http://rdaregistry.info/Elements/u/subject.en> ;
    reg:name "subject"@en ;
    reg:status <http://metadataregistry.org/uri/RegStatus/1001> ;
    a rdf:Property ;
    rdfs:isDefinedBy <http://rdaregistry.info/Elements/u/> ;
    rdfs:label "has subject"@en ;
    owl:inverseOf <http://rdaregistry.info/Elements/u/P60806> ;
    skos:definition "Relates a resource to a subject of a resource; i.e., an indication of what a resource is about."@en .

<http://rdaregistry.info/Elements/u/P60806>
    reg:lexicalAlias <http://rdaregistry.info/Elements/u/subjectOf.en> ;
    reg:name "subjectOf"@en ;
    reg:status <http://metadataregistry.org/uri/RegStatus/1001> ;
    a rdf:Property ;
    rdfs:isDefinedBy <http://rdaregistry.info/Elements/u/> ;
    rdfs:label "is subject of"@en ;
    owl:inverseOf <http://rdaregistry.info/Elements/u/P60805> ;
    skos:definition "Relates a resource to a resource that is about a resource."@en .

<http://rdaregistry.info/Elements/u/P60807>
    reg:lexicalAlias <http://rdaregistry.info/Elements/u/graduate.en> ;
    reg:name "graduate"@en ;
    reg:status <http://metadataregistry.org/uri/RegStatus/1001> ;
    a rdf:Property ;
    rdfs:isDefinedBy <http://rdaregistry.info/Elements/u/> ;
    rdfs:label "has graduate"@en ;
    owl:inverseOf <http://rdaregistry.info/Elements/u/P60808> ;
    skos:definition "Relates an agent to an agent who receives an academic degree from a granting institution or faculty."@en .

<http://rdaregistry.info/Elements/u/P60808>
    reg:lexicalAlias <http://rdaregistry.info/Elements/u/graduateOf.en> ;
    reg:name "graduateOf"@en ;
    reg:status <http://metadataregistry.org/uri/RegStatus/1001> ;
    a rdf:Property ;
    rdfs:isDefinedBy <http://rdaregistry.info/Elements/u/> ;
    rdfs:label "is graduate of"@en ;
    owl:inverseOf <http://rdaregistry.info/Elements/u/P60807> ;
    skos:definition "Relates an agent to an institution or faculty that granted an academic degree to an agent."@en .

<http://rdaregistry.info/Elements/u/P60809>
    reg:lexicalAlias <http://rdaregistry.info/Elements/u/writerOfForeword.en> ;
    reg:name "writerOfForeword"@en ;
    reg:status <http://metadataregistry.org/uri/RegStatus/1001> ;
    a rdf:Property ;
    rdfs:isDefinedBy <http://rdaregistry.info/Elements/u/> ;
    rdfs:label "has writer of foreword"@en ;
    rdfs:subPropertyOf <http://rdaregistry.info/Elements/u/P60398> ;
    owl:inverseOf <http://rdaregistry.info/Elements/u/P60810> ;
    skos:definition "Relates a resource to an agent contributing to a resource by providing a foreword to an original resource."@en .

<http://rdaregistry.info/Elements/u/P60810>
    reg:lexicalAlias <http://rdaregistry.info/Elements/u/writerOfForewordOf.en> ;
    reg:name "writerOfForewordOf"@en ;
    reg:status <http://metadataregistry.org/uri/RegStatus/1001> ;
    a rdf:Property ;
    rdfs:isDefinedBy <http://rdaregistry.info/Elements/u/> ;
    rdfs:label "is writer of foreword of"@en ;
    rdfs:subPropertyOf <http://rdaregistry.info/Elements/u/P60626> ;
    owl:inverseOf <http://rdaregistry.info/Elements/u/P60809> ;
    skos:definition "Relates an agent contributing to a resource by providing a foreword to an original resource to a resource."@en .

<http://rdaregistry.info/Elements/u/P60811>
    reg:lexicalAlias <http://rdaregistry.info/Elements/u/soundDesigner.en> ;
    reg:name "soundDesigner"@en ;
    reg:status <http://metadataregistry.org/uri/RegStatus/1001> ;
    a rdf:Property ;
    rdfs:isDefinedBy <http://rdaregistry.info/Elements/u/> ;
    rdfs:label "has sound designer"@en ;
    rdfs:subPropertyOf <http://rdaregistry.info/Elements/u/P60398> ;
    owl:inverseOf <http://rdaregistry.info/Elements/u/P60812> ;
    skos:definition "Relates a resource to an agent contributing to a resource by designing and creating audio/sound components."@en .

<http://rdaregistry.info/Elements/u/P60812>
    reg:lexicalAlias <http://rdaregistry.info/Elements/u/soundDesignerOf.en> ;
    reg:name "soundDesignerOf"@en ;
    reg:status <http://metadataregistry.org/uri/RegStatus/1001> ;
    a rdf:Property ;
    rdfs:isDefinedBy <http://rdaregistry.info/Elements/u/> ;
    rdfs:label "is sound designer of"@en ;
    rdfs:subPropertyOf <http://rdaregistry.info/Elements/u/P60626> ;
    owl:inverseOf <http://rdaregistry.info/Elements/u/P60811> ;
    skos:definition "Relates an agent contributing to a resource by designing and creating audio/sound components to a resource."@en .

<http://rdaregistry.info/Elements/u/P60813>
    reg:lexicalAlias <http://rdaregistry.info/Elements/u/lightingDesigner.en> ;
    reg:name "lightingDesigner"@en ;
    reg:status <http://metadataregistry.org/uri/RegStatus/1001> ;
    a rdf:Property ;
    rdfs:isDefinedBy <http://rdaregistry.info/Elements/u/> ;
    rdfs:label "has lighting designer"@en ;
    rdfs:subPropertyOf <http://rdaregistry.info/Elements/u/P60398> ;
    owl:inverseOf <http://rdaregistry.info/Elements/u/P60814> ;
    skos:definition "Relates a resource to an agent contributing to a resource by designing and creating lighting components."@en .

<http://rdaregistry.info/Elements/u/P60814>
    reg:lexicalAlias <http://rdaregistry.info/Elements/u/lightingDesignerOf.en> ;
    reg:name "lightingDesignerOf"@en ;
    reg:status <http://metadataregistry.org/uri/RegStatus/1001> ;
    a rdf:Property ;
    rdfs:isDefinedBy <http://rdaregistry.info/Elements/u/> ;
    rdfs:label "is lighting designer of"@en ;
    rdfs:subPropertyOf <http://rdaregistry.info/Elements/u/P60626> ;
    owl:inverseOf <http://rdaregistry.info/Elements/u/P60813> ;
    skos:definition "Relates an agent contributing to a resource by designing and creating lighting components to a resource."@en .

<http://rdaregistry.info/Elements/u/P60815>
    reg:lexicalAlias <http://rdaregistry.info/Elements/u/degreeCommitteeMember.en> ;
    reg:name "degreeCommitteeMember"@en ;
    reg:status <http://metadataregistry.org/uri/RegStatus/1001> ;
    a rdf:Property ;
    rdfs:isDefinedBy <http://rdaregistry.info/Elements/u/> ;
    rdfs:label "has degree committee member"@en ;
    rdfs:subPropertyOf <http://rdaregistry.info/Elements/u/P60374> ;
    owl:inverseOf <http://rdaregistry.info/Elements/u/P60816> ;
    skos:definition "Relates a resource to an agent serving on a committee that supervises a students thesis or dissertation."@en .

<http://rdaregistry.info/Elements/u/P60816>
    reg:lexicalAlias <http://rdaregistry.info/Elements/u/degreeCommitteeMemberOf.en> ;
    reg:name "degreeCommitteeMemberOf"@en ;
    reg:status <http://metadataregistry.org/uri/RegStatus/1001> ;
    a rdf:Property ;
    rdfs:isDefinedBy <http://rdaregistry.info/Elements/u/> ;
    rdfs:label "is degree committee member of"@en ;
    rdfs:subPropertyOf <http://rdaregistry.info/Elements/u/P60602> ;
    owl:inverseOf <http://rdaregistry.info/Elements/u/P60815> ;
    skos:definition "Relates an agent serving on a committee that supervises a students thesis or dissertation to a resource."@en .

<http://rdaregistry.info/Elements/u/P60817>
    reg:lexicalAlias <http://rdaregistry.info/Elements/u/producerOfUnpublishedResourceOf.en> ;
    reg:name "producerOfUnpublishedResourceOf"@en ;
    reg:status <http://metadataregistry.org/uri/RegStatus/1001> ;
    a rdf:Property ;
    rdfs:isDefinedBy <http://rdaregistry.info/Elements/u/> ;
    rdfs:label "is producer of unpublished resource of"@en ;
    skos:definition "Relates an agent responsible for inscribing, fabricating, constructing, etc. to a resource."@en .

<http://rdaregistry.info/Elements/u/P60818>
    reg:lexicalAlias <http://rdaregistry.info/Elements/u/alternativeChronologicalDesignationOfFirstIssueOrPartOfSequence.en> ;
    reg:name "alternativeChronologicalDesignationOfFirstIssueOrPartOfSequence"@en ;
    reg:status <http://metadataregistry.org/uri/RegStatus/1001> ;
    a rdf:Property ;
    rdfs:isDefinedBy <http://rdaregistry.info/Elements/u/> ;
    rdfs:label "has alternative chronological designation of first issue or part of sequence"@en ;
    rdfs:subPropertyOf <http://rdaregistry.info/Elements/u/P60533> ;
    skos:definition "Relates a resource to a second or subsequent system of numbering presented in the form of a date on the first issue or part of a sequence of numbering for a serial."@en ;
    skos:scopeNote "Designation includes a year; year and month; month, day, and year. An alternative chronological designation may include a date in a different calendar."@en .

<http://rdaregistry.info/Elements/u/P60819>
    reg:lexicalAlias <http://rdaregistry.info/Elements/u/alternativeChronologicalDesignationOfLastIssueOrPartOfSequence.en> ;
    reg:name "alternativeChronologicalDesignationOfLastIssueOrPartOfSequence"@en ;
    reg:status <http://metadataregistry.org/uri/RegStatus/1001> ;
    a rdf:Property ;
    rdfs:isDefinedBy <http://rdaregistry.info/Elements/u/> ;
    rdfs:label "has alternative chronological designation of last issue or part of sequence"@en ;
    rdfs:subPropertyOf <http://rdaregistry.info/Elements/u/P60533> ;
    skos:definition "Relates a resource to a second or subsequent system of numbering presented in the form of a date on the last issue or part of a sequence of numbering for a serial."@en ;
    skos:scopeNote "Designational includes a year; year and month; month, day, and year. An alternative chronological designation may include a date in a different calendar."@en .

<http://rdaregistry.info/Elements/u/P60820>
    reg:lexicalAlias <http://rdaregistry.info/Elements/u/alternativeNumericAndOrAlphabeticDesignationOfFirstIssueOrPartOfSequence.en> ;
    reg:name "alternativeNumericAndOrAlphabeticDesignationOfFirstIssueOrPartOfSequence"@en ;
    reg:status <http://metadataregistry.org/uri/RegStatus/1001> ;
    a rdf:Property ;
    rdfs:isDefinedBy <http://rdaregistry.info/Elements/u/> ;
    rdfs:label "has alternative numeric and/or alphabetic designation of first issue or part of sequence"@en ;
    rdfs:subPropertyOf <http://rdaregistry.info/Elements/u/P60533> ;
    skos:definition "Relates a resource to a second or subsequent system of numbering presented in numeric or alphabetic form on the first issue or part of a sequence of numbering for a serial."@en .

<http://rdaregistry.info/Elements/u/P60821>
    reg:lexicalAlias <http://rdaregistry.info/Elements/u/alternativeNumericAndOrAlphabeticDesignationOfLastIssueOrPartOfSequence.en> ;
    reg:name "alternativeNumericAndOrAlphabeticDesignationOfLastIssueOrPartOfSequence"@en ;
    reg:status <http://metadataregistry.org/uri/RegStatus/1001> ;
    a rdf:Property ;
    rdfs:isDefinedBy <http://rdaregistry.info/Elements/u/> ;
    rdfs:label "has alternative numeric and/or alphabetic designation of last issue or part of sequence"@en ;
    rdfs:subPropertyOf <http://rdaregistry.info/Elements/u/P60533> ;
    skos:definition "Relates a resource to a second or subsequent system of numbering presented in numeric or alphabetic form on the last issue or part of a sequence of numbering for a serial."@en .

<http://rdaregistry.info/Elements/u/P60822>
    reg:lexicalAlias <http://rdaregistry.info/Elements/u/scopeOfUsage.en> ;
    reg:name "scopeOfUsage"@en ;
    reg:status <http://metadataregistry.org/uri/RegStatus/1001> ;
    a rdf:Property ;
    rdfs:isDefinedBy <http://rdaregistry.info/Elements/u/> ;
    rdfs:label "has scope of usage"@en ;
    skos:definition "Relates a name to a type or form of resource associated with a name chosen as a preferred name for an agent."@en .

<http://rdaregistry.info/Elements/u/P60823>
    reg:lexicalAlias <http://rdaregistry.info/Elements/u/detailsOfDuration.en> ;
    reg:name "detailsOfDuration"@en ;
    reg:status <http://metadataregistry.org/uri/RegStatus/1001> ;
    a rdf:Property ;
    rdfs:isDefinedBy <http://rdaregistry.info/Elements/u/> ;
    rdfs:label "has details of duration"@en ;
    skos:definition "Relates a resource to details of the playing time, running time, performance time, etc., of the content of a resource."@en .

<http://rdaregistry.info/Elements/u/P60824>
    rdakit:seeAlso <http://rdaregistry.info/Elements/u/P60143> ;
    reg:hasSubproperty <http://rdaregistry.info/Elements/e/P20279> ;
    reg:lexicalAlias <http://rdaregistry.info/Elements/u/onScreenParticipant.en> ;
    reg:name "onScreenParticipant"@en ;
    reg:status <http://metadataregistry.org/uri/RegStatus/1001> ;
    a rdf:Property ;
    rdfs:isDefinedBy <http://rdaregistry.info/Elements/u/> ;
    rdfs:label "has on-screen participant"@en ;
    rdfs:subPropertyOf <http://rdaregistry.info/Elements/u/P60398> ;
    owl:inverseOf <http://rdaregistry.info/Elements/u/P60825> ;
    skos:definition "Relates a resource to an agent contributing to a nonfiction moving image resource by taking an active role as a participant."@en ;
    skos:scopeNote "Appearance on screen to provide contextual or background information is excluded."@en .

<http://rdaregistry.info/Elements/u/P60825>
    rdakit:seeAlso <http://rdaregistry.info/Elements/u/P60018> ;
    reg:hasSubproperty <http://rdaregistry.info/Elements/a/P50261> ;
    reg:lexicalAlias <http://rdaregistry.info/Elements/u/onScreenParticipantOf.en> ;
    reg:name "onScreenParticipantOf"@en ;
    reg:status <http://metadataregistry.org/uri/RegStatus/1001> ;
    a rdf:Property ;
    rdfs:isDefinedBy <http://rdaregistry.info/Elements/u/> ;
    rdfs:label "is on-screen participant of"@en ;
    rdfs:subPropertyOf <http://rdaregistry.info/Elements/u/P60626> ;
    owl:inverseOf <http://rdaregistry.info/Elements/u/P60824> ;
    skos:definition "Relates an agent contributing to a nonfiction moving image resource by taking an active role as a participant to a resource."@en ;
    skos:scopeNote "Appearance on screen to provide contextual or background information is excluded."@en .

<http://rdaregistry.info/Elements/u/P60826>
    reg:lexicalAlias <http://rdaregistry.info/Elements/u/commissioningBody.en> ;
    reg:name "commissioningBody"@en ;
    reg:status <http://metadataregistry.org/uri/RegStatus/1001> ;
    a rdf:Property ;
    rdfs:isDefinedBy <http://rdaregistry.info/Elements/u/> ;
    rdfs:label "has commissioning body"@en ;
    rdfs:subPropertyOf <http://rdaregistry.info/Elements/u/P60447> ;
    owl:inverseOf <http://rdaregistry.info/Elements/u/P60827> ;
    skos:definition "Relates a resource to an agent responsible for commissioning a resource."@en .

<http://rdaregistry.info/Elements/u/P60827>
    reg:hasSubproperty <http://rdaregistry.info/Elements/a/P50262> ;
    reg:lexicalAlias <http://rdaregistry.info/Elements/u/commissioningBodyOf.en> ;
    reg:name "commissioningBodyOf"@en ;
    reg:status <http://metadataregistry.org/uri/RegStatus/1001> ;
    a rdf:Property ;
    rdfs:isDefinedBy <http://rdaregistry.info/Elements/u/> ;
    rdfs:label "is commissioning body of"@en ;
    rdfs:subPropertyOf <http://rdaregistry.info/Elements/u/P60672> ;
    owl:inverseOf <http://rdaregistry.info/Elements/u/P60826> ;
    skos:definition "Relates an agent responsible for commissioning a resource to a resource."@en .

<http://rdaregistry.info/Elements/u/P60828>
    reg:hasSubproperty <http://rdaregistry.info/Elements/e/P20280> ;
    reg:lexicalAlias <http://rdaregistry.info/Elements/u/softwareDeveloper.en> ;
    reg:name "softwareDeveloper"@en ;
    reg:status <http://metadataregistry.org/uri/RegStatus/1001> ;
    a rdf:Property ;
    rdfs:isDefinedBy <http://rdaregistry.info/Elements/u/> ;
    rdfs:label "has software developer"@en ;
    rdfs:subPropertyOf <http://rdaregistry.info/Elements/u/P60398> ;
    owl:inverseOf <http://rdaregistry.info/Elements/u/P60829> ;
    skos:definition "Relates a resource to an agent contributing to a resource by researching, designing, implementing, or testing software."@en .

<http://rdaregistry.info/Elements/u/P60829>
    reg:hasSubproperty <http://rdaregistry.info/Elements/a/P50263> ;
    reg:lexicalAlias <http://rdaregistry.info/Elements/u/softwareDeveloperOf.en> ;
    reg:name "softwareDeveloperOf"@en ;
    reg:status <http://metadataregistry.org/uri/RegStatus/1001> ;
    a rdf:Property ;
    rdfs:isDefinedBy <http://rdaregistry.info/Elements/u/> ;
    rdfs:label "is software developer of"@en ;
    rdfs:subPropertyOf <http://rdaregistry.info/Elements/u/P60626> ;
    owl:inverseOf <http://rdaregistry.info/Elements/u/P60828> ;
    skos:definition "Relates an agent contributing to a resource by researching, designing, implementing, or testing software to a resource."@en .

<http://rdaregistry.info/Elements/u/P60830>
    reg:hasSubproperty <http://rdaregistry.info/Elements/e/P20281> ;
    reg:lexicalAlias <http://rdaregistry.info/Elements/u/oratorioAdaptationOf.en> ;
    reg:name "oratorioAdaptationOf"@en ;
    reg:status <http://metadataregistry.org/uri/RegStatus/1001> ;
    a rdf:Property ;
    rdfs:isDefinedBy <http://rdaregistry.info/Elements/u/> ;
    rdfs:label "is oratorio adaptation of"@en ;
    rdfs:subPropertyOf <http://rdaregistry.info/Elements/u/P60305> ;
    owl:inverseOf <http://rdaregistry.info/Elements/u/P60831> ;
    skos:definition "Relates a resource to a resource that has been adapted as an oratorio."@en .

<http://rdaregistry.info/Elements/u/P60831>
    reg:hasSubproperty <http://rdaregistry.info/Elements/e/P20282> ;
    reg:lexicalAlias <http://rdaregistry.info/Elements/u/adaptedAsOratorio.en> ;
    reg:name "adaptedAsOratorio"@en ;
    reg:status <http://metadataregistry.org/uri/RegStatus/1001> ;
    a rdf:Property ;
    rdfs:isDefinedBy <http://rdaregistry.info/Elements/u/> ;
    rdfs:label "is adapted as oratorio"@en ;
    rdfs:subPropertyOf <http://rdaregistry.info/Elements/u/P60250> ;
    owl:inverseOf <http://rdaregistry.info/Elements/u/P60830> ;
    skos:definition "Relates a resource to an oratorio based on a source resource."@en .

<http://rdaregistry.info/Elements/u/P60832>
    reg:lexicalAlias <http://rdaregistry.info/Elements/u/inspiredBy.en> ;
    reg:name "inspiredBy"@en ;
    reg:status <http://metadataregistry.org/uri/RegStatus/1001> ;
    a rdf:Property ;
    rdfs:isDefinedBy <http://rdaregistry.info/Elements/u/> ;
    rdfs:label "is inspired by"@en ;
    rdfs:subPropertyOf <http://rdaregistry.info/Elements/u/P60305> ;
    owl:inverseOf <http://rdaregistry.info/Elements/u/P60833> ;
    skos:definition "Relates a resource to a resource which serves as the inspiration for another resource."@en .

<http://rdaregistry.info/Elements/u/P60833>
    reg:lexicalAlias <http://rdaregistry.info/Elements/u/inspirationFor.en> ;
    reg:name "inspirationFor"@en ;
    reg:status <http://metadataregistry.org/uri/RegStatus/1001> ;
    a rdf:Property ;
    rdfs:isDefinedBy <http://rdaregistry.info/Elements/u/> ;
    rdfs:label "is inspiration for"@en ;
    rdfs:subPropertyOf <http://rdaregistry.info/Elements/u/P60250> ;
    owl:inverseOf <http://rdaregistry.info/Elements/u/P60832> ;
    skos:definition "Relates a resource to a resource which was inspired by another resource."@en .

<http://rdaregistry.info/Elements/u/P60834>
    reg:lexicalAlias <http://rdaregistry.info/Elements/u/participantInTreaty.en> ;
    reg:name "participantInTreaty"@en ;
    reg:status <http://metadataregistry.org/uri/RegStatus/1001> ;
    a rdf:Property ;
    rdfs:isDefinedBy <http://rdaregistry.info/Elements/u/> ;
    rdfs:label "has participant in treaty"@en ;
    rdfs:subPropertyOf <http://rdaregistry.info/Elements/u/P60374> ;
    owl:inverseOf <http://rdaregistry.info/Elements/u/P60835> ;
    skos:definition "Relates a resource to a government, international intergovernmental body, or other agent that has signed, ratified, or acceded to a treaty."@en .

<http://rdaregistry.info/Elements/u/P60835>
    reg:hasSubproperty <http://rdaregistry.info/Elements/a/P50264> ;
    reg:lexicalAlias <http://rdaregistry.info/Elements/u/participantInTreatyOf.en> ;
    reg:name "participantInTreatyOf"@en ;
    reg:status <http://metadataregistry.org/uri/RegStatus/1001> ;
    a rdf:Property ;
    rdfs:isDefinedBy <http://rdaregistry.info/Elements/u/> ;
    rdfs:label "is participant in treaty of"@en ;
    rdfs:subPropertyOf <http://rdaregistry.info/Elements/u/P60602> ;
    owl:inverseOf <http://rdaregistry.info/Elements/u/P60834> ;
    skos:definition "Relates a government, international intergovernmental body, or other agent that has signed, ratified, or acceded to a treaty to a resource."@en .

<http://rdaregistry.info/Elements/u/P60836>
    reg:lexicalAlias <http://rdaregistry.info/Elements/u/researcher.en> ;
    reg:name "researcher"@en ;
    reg:status <http://metadataregistry.org/uri/RegStatus/1001> ;
    a rdf:Property ;
    rdfs:isDefinedBy <http://rdaregistry.info/Elements/u/> ;
    rdfs:label "has researcher"@en ;
    rdfs:subPropertyOf <http://rdaregistry.info/Elements/u/P60374> ;
    owl:inverseOf <http://rdaregistry.info/Elements/u/P60837> ;
    skos:definition "Relates a resource to an agent who does research in support of the creation of a resource."@en .

<http://rdaregistry.info/Elements/u/P60837>
    reg:hasSubproperty <http://rdaregistry.info/Elements/a/P50265> ;
    reg:lexicalAlias <http://rdaregistry.info/Elements/u/researchOf.en> ;
    reg:name "researcherOf"@en ;
    reg:status <http://metadataregistry.org/uri/RegStatus/1001> ;
    a rdf:Property ;
    rdfs:isDefinedBy <http://rdaregistry.info/Elements/u/> ;
    rdfs:label "is researcher of"@en ;
    rdfs:subPropertyOf <http://rdaregistry.info/Elements/u/P60602> ;
    owl:inverseOf <http://rdaregistry.info/Elements/u/P60836> ;
    skos:definition "Relates an agent who does research in support of the creation of a resource to a resource."@en .

<http://rdaregistry.info/Elements/u/P60838>
    reg:hasSubproperty <http://rdaregistry.info/Elements/e/P20283> ;
    reg:lexicalAlias <http://rdaregistry.info/Elements/u/colourist.en> ;
    reg:name "colourist"@en ;
    reg:status <http://metadataregistry.org/uri/RegStatus/1001> ;
    a rdf:Property ;
    rdfs:isDefinedBy <http://rdaregistry.info/Elements/u/> ;
    rdfs:label "has colourist"@en ;
    rdfs:subPropertyOf <http://rdaregistry.info/Elements/u/P60398> ;
    owl:inverseOf <http://rdaregistry.info/Elements/u/P60839> ;
    skos:definition "Relates a resource to an agent contributing to a resource by applying colour to drawings, prints, photographs, maps, moving images, etc."@en .

<http://rdaregistry.info/Elements/u/P60839>
    reg:hasSubproperty <http://rdaregistry.info/Elements/a/P50266> ;
    reg:lexicalAlias <http://rdaregistry.info/Elements/u/colouristOf.en> ;
    reg:name "colouristOf"@en ;
    reg:status <http://metadataregistry.org/uri/RegStatus/1001> ;
    a rdf:Property ;
    rdfs:isDefinedBy <http://rdaregistry.info/Elements/u/> ;
    rdfs:label "is colourist of"@en ;
    rdfs:subPropertyOf <http://rdaregistry.info/Elements/u/P60626> ;
    owl:inverseOf <http://rdaregistry.info/Elements/u/P60838> ;
    skos:definition "Relates an agent contributing to a resource by applying colour to drawings, prints, photographs, maps, moving images, etc. to a resource."@en .

<http://rdaregistry.info/Elements/u/P60840>
    reg:hasSubproperty <http://rdaregistry.info/Elements/e/P20284> ;
    reg:lexicalAlias <http://rdaregistry.info/Elements/u/makeUpArtist.en> ;
    reg:name "makeUpArtist"@en ;
    reg:status <http://metadataregistry.org/uri/RegStatus/1001> ;
    a rdf:Property ;
    rdfs:isDefinedBy <http://rdaregistry.info/Elements/u/> ;
    rdfs:label "has make-up artist"@en ;
    rdfs:subPropertyOf <http://rdaregistry.info/Elements/u/P60398> ;
    owl:inverseOf <http://rdaregistry.info/Elements/u/P60841> ;
    skos:definition "Relates a resource to an agent contributing to a resource by applying make-up and prosthetics for a moving image production or for a musical or dramatic presentation or entertainment."@en .

<http://rdaregistry.info/Elements/u/P60841>
    reg:hasSubproperty <http://rdaregistry.info/Elements/a/P50267> ;
    reg:lexicalAlias <http://rdaregistry.info/Elements/u/makeUpArtistOf.en> ;
    reg:name "makeUpArtistOf"@en ;
    reg:status <http://metadataregistry.org/uri/RegStatus/1001> ;
    a rdf:Property ;
    rdfs:isDefinedBy <http://rdaregistry.info/Elements/u/> ;
    rdfs:label "is make-up artist of"@en ;
    rdfs:subPropertyOf <http://rdaregistry.info/Elements/u/P60626> ;
    owl:inverseOf <http://rdaregistry.info/Elements/u/P60840> ;
    skos:definition "Relates an agent contributing to a resource by applying make-up and prosthetics for a moving image production or for a musical or dramatic presentation or entertainment to a resource."@en .

<http://rdaregistry.info/Elements/u/P60842>
    reg:hasSubproperty <http://rdaregistry.info/Elements/e/P20285> ;
    reg:lexicalAlias <http://rdaregistry.info/Elements/u/choralConductor.en> ;
    reg:name "choralConductor"@en ;
    reg:status <http://metadataregistry.org/uri/RegStatus/1001> ;
    a rdf:Property ;
    rdfs:isDefinedBy <http://rdaregistry.info/Elements/u/> ;
    rdfs:label "has choral conductor"@en ;
    rdfs:subPropertyOf <http://rdaregistry.info/Elements/u/P60141> ;
    owl:inverseOf <http://rdaregistry.info/Elements/u/P60843> ;
    skos:definition "Relates a resource to a conductor contributing to a musical resource by leading a choral performing group in a musical or dramatic presentation, etc."@en .

<http://rdaregistry.info/Elements/u/P60843>
    reg:hasSubproperty <http://rdaregistry.info/Elements/a/P50268> ;
    reg:lexicalAlias <http://rdaregistry.info/Elements/u/choralConductorOf.en> ;
    reg:name "choralConductorOf"@en ;
    reg:status <http://metadataregistry.org/uri/RegStatus/1001> ;
    a rdf:Property ;
    rdfs:isDefinedBy <http://rdaregistry.info/Elements/u/> ;
    rdfs:label "is choral conductor of"@en ;
    rdfs:subPropertyOf <http://rdaregistry.info/Elements/u/P60016> ;
    owl:inverseOf <http://rdaregistry.info/Elements/u/P60842> ;
    skos:definition "Relates a conductor contributing to a musical resource by leading a choral performing group in a musical or dramatic presentation, etc. to a resource."@en .

<http://rdaregistry.info/Elements/u/P60844>
    reg:hasSubproperty <http://rdaregistry.info/Elements/e/P20286> ;
    reg:lexicalAlias <http://rdaregistry.info/Elements/u/instrumentalConductor.en> ;
    reg:name "instrumentalConductor"@en ;
    reg:status <http://metadataregistry.org/uri/RegStatus/1001> ;
    a rdf:Property ;
    rdfs:isDefinedBy <http://rdaregistry.info/Elements/u/> ;
    rdfs:label "has instrumental conductor"@en ;
    rdfs:subPropertyOf <http://rdaregistry.info/Elements/u/P60141> ;
    owl:inverseOf <http://rdaregistry.info/Elements/u/P60845> ;
    skos:definition "Relates a resource to a conductor contributing to a musical resource by leading an instrumental performing group in a musical or dramatic presentation, etc."@en .

<http://rdaregistry.info/Elements/u/P60845>
    reg:hasSubproperty <http://rdaregistry.info/Elements/a/P50269> ;
    reg:lexicalAlias <http://rdaregistry.info/Elements/u/instrumentalConductorOf.en> ;
    reg:name "instrumentalConductorOf"@en ;
    reg:status <http://metadataregistry.org/uri/RegStatus/1001> ;
    a rdf:Property ;
    rdfs:isDefinedBy <http://rdaregistry.info/Elements/u/> ;
    rdfs:label "is instrumental conductor of"@en ;
    rdfs:subPropertyOf <http://rdaregistry.info/Elements/u/P60016> ;
    owl:inverseOf <http://rdaregistry.info/Elements/u/P60844> ;
    skos:definition "Relates a conductor contributing to a musical resource by leading an instrumental performing group in a musical or dramatic presentation, etc. to a resource"@en .

<http://rdaregistry.info/Elements/u/P60846>
    reg:lexicalAlias <http://rdaregistry.info/Elements/u/commemoration.en> ;
    reg:name "commemoration"@en ;
    reg:status <http://metadataregistry.org/uri/RegStatus/1001> ;
    a rdf:Property ;
    rdfs:isDefinedBy <http://rdaregistry.info/Elements/u/> ;
    rdfs:label "has commemoration"@en ;
    rdfs:subPropertyOf <http://rdaregistry.info/Elements/u/P60848> ;
    owl:inverseOf <http://rdaregistry.info/Elements/u/P60847> ;
    skos:definition "Relates a resource to a resource created to commemorate an earlier resource."@en .

<http://rdaregistry.info/Elements/u/P60847>
    reg:lexicalAlias <http://rdaregistry.info/Elements/u/commemorationOf.en> ;
    reg:name "commemorationOf"@en ;
    reg:status <http://metadataregistry.org/uri/RegStatus/1001> ;
    a rdf:Property ;
    rdfs:isDefinedBy <http://rdaregistry.info/Elements/u/> ;
    rdfs:label "is commemoration of"@en ;
    rdfs:subPropertyOf <http://rdaregistry.info/Elements/u/P60848> ;
    owl:inverseOf <http://rdaregistry.info/Elements/u/P60846> ;
    skos:definition "Relates a resource to a resource commemorated in a later resource."@en .

<http://rdaregistry.info/Elements/u/P60848>
    reg:hasSubproperty <http://rdaregistry.info/Elements/u/P60846>, <http://rdaregistry.info/Elements/u/P60847> ;
    reg:lexicalAlias <http://rdaregistry.info/Elements/u/referentialResourceRelationship.en> ;
    reg:name "referentialResourceRelationship"@en ;
    reg:status <http://metadataregistry.org/uri/RegStatus/1001> ;
    a rdf:Property ;
    rdfs:isDefinedBy <http://rdaregistry.info/Elements/u/> ;
    rdfs:label "has referential resource relationship with"@en ;
    owl:inverseOf <http://rdaregistry.info/Elements/u/P60848> ;
    skos:definition "Relates a resource to a resource that references another resource."@en .

<http://rdaregistry.info/Elements/u/P60849>
    reg:hasSubproperty <http://rdaregistry.info/Elements/w/P10297> ;
    reg:lexicalAlias <http://rdaregistry.info/Elements/u/organizer.en> ;
    reg:name "organizer"@en ;
    reg:status <http://metadataregistry.org/uri/RegStatus/1001> ;
    a rdf:Property ;
    rdfs:isDefinedBy <http://rdaregistry.info/Elements/u/> ;
    rdfs:label "has organizer"@en ;
    rdfs:subPropertyOf <http://rdaregistry.info/Elements/u/P60374> ;
    owl:inverseOf <http://rdaregistry.info/Elements/u/P60850> ;
    skos:definition "Relates a resource to an agent organizing an exhibit, event, conference, course, program, etc., which gave rise to a resource."@en .

<http://rdaregistry.info/Elements/u/P60850>
    reg:hasSubproperty <http://rdaregistry.info/Elements/a/P50270> ;
    reg:lexicalAlias <http://rdaregistry.info/Elements/u/organizerOf.en> ;
    reg:name "organizerOf"@en ;
    reg:status <http://metadataregistry.org/uri/RegStatus/1001> ;
    a rdf:Property ;
    rdfs:isDefinedBy <http://rdaregistry.info/Elements/u/> ;
    rdfs:label "is organizer of"@en ;
    rdfs:subPropertyOf <http://rdaregistry.info/Elements/u/P60602> ;
    owl:inverseOf <http://rdaregistry.info/Elements/u/P60849> ;
    skos:definition "Relates an agent organizing an exhibit, event, conference, course, program, etc., which gave rise to a resource to a resource."@en .

<http://rdaregistry.info/Elements/u/P60851>
    rdakit:seeAlso <http://rdaregistry.info/Elements/u/P60434> ;
    reg:hasSubproperty <http://rdaregistry.info/Elements/e/P20287> ;
    reg:lexicalAlias <http://rdaregistry.info/Elements/u/censor.en> ;
    reg:name "censor"@en ;
    reg:status <http://metadataregistry.org/uri/RegStatus/1001> ;
    a rdf:Property ;
    rdfs:isDefinedBy <http://rdaregistry.info/Elements/u/> ;
    rdfs:label "has censor"@en ;
    rdfs:subPropertyOf <http://rdaregistry.info/Elements/u/P60398> ;
    owl:inverseOf <http://rdaregistry.info/Elements/u/P60852> ;
    skos:definition "Relates a resource to an agent contributing to a resource by revising the content for the purpose of suppressing parts deemed objectionable on moral, political, military, or other grounds, but leaving the nature and content substantially unchanged."@en ;
    skos:scopeNote "Substantial modification that results in the creation of a new resource is excluded."@en .

<http://rdaregistry.info/Elements/u/P60852>
    rdakit:seeAlso <http://rdaregistry.info/Elements/u/P60663> ;
    reg:hasSubproperty <http://rdaregistry.info/Elements/a/P50271> ;
    reg:lexicalAlias <http://rdaregistry.info/Elements/u/censorOf.en> ;
    reg:name "censorOf"@en ;
    reg:status <http://metadataregistry.org/uri/RegStatus/1001> ;
    a rdf:Property ;
    rdfs:isDefinedBy <http://rdaregistry.info/Elements/u/> ;
    rdfs:label "is censor of"@en ;
    rdfs:subPropertyOf <http://rdaregistry.info/Elements/u/P60626> ;
    owl:inverseOf <http://rdaregistry.info/Elements/u/P60851> ;
    skos:definition "Relates an agent contributing to a resource by revising the content for the purpose of suppressing parts deemed objectionable on moral, political, military, or other grounds, but leaving the nature and content substantially unchanged to a resource."@en ;
    skos:scopeNote "Substantial modification that results in the creation of a new resource is excluded."@en .

<http://rdaregistry.info/Elements/u/P60853>
    reg:hasSubproperty <http://rdaregistry.info/Elements/a/P50274>, <http://rdaregistry.info/Elements/u/P60857>, <http://rdaregistry.info/Elements/u/P60858>, <http://rdaregistry.info/Elements/u/P60859>, <http://rdaregistry.info/Elements/u/P60860> ;
    reg:lexicalAlias <http://rdaregistry.info/Elements/u/colleague.en> ;
    reg:name "colleague"@en ;
    reg:status <http://metadataregistry.org/uri/RegStatus/1001> ;
    a rdf:Property ;
    rdfs:isDefinedBy <http://rdaregistry.info/Elements/u/> ;
    rdfs:label "has colleague"@en ;
    rdfs:subPropertyOf <http://rdaregistry.info/Elements/u/P60454> ;
    owl:inverseOf <http://rdaregistry.info/Elements/u/P60853> ;
    skos:definition "Relates an agent to a fellow member of a profession, staff, or academic faculty."@en .

<http://rdaregistry.info/Elements/u/P60854>
    reg:hasSubproperty <http://rdaregistry.info/Elements/a/P50280> ;
    reg:lexicalAlias <http://rdaregistry.info/Elements/u/friend.en> ;
    reg:name "friend"@en ;
    reg:status <http://metadataregistry.org/uri/RegStatus/1001> ;
    a rdf:Property ;
    rdfs:isDefinedBy <http://rdaregistry.info/Elements/u/> ;
    rdfs:label "has friend"@en ;
    rdfs:subPropertyOf <http://rdaregistry.info/Elements/u/P60454> ;
    owl:inverseOf <http://rdaregistry.info/Elements/u/P60854> ;
    skos:definition "Relates an agent to an agent who shares a bond of mutual affection or regard with another agent."@en .

<http://rdaregistry.info/Elements/u/P60855>
    reg:hasSubproperty <http://rdaregistry.info/Elements/a/P50283> ;
    reg:lexicalAlias <http://rdaregistry.info/Elements/u/enrolledStudent.en> ;
    reg:name "enrolledStudent"@en ;
    reg:status <http://metadataregistry.org/uri/RegStatus/1001> ;
    a rdf:Property ;
    rdfs:isDefinedBy <http://rdaregistry.info/Elements/u/> ;
    rdfs:label "has enrolled student"@en ;
    rdfs:subPropertyOf <http://rdaregistry.info/Elements/u/P60454> ;
    owl:inverseOf <http://rdaregistry.info/Elements/u/P60856> ;
    skos:definition "Relates an agent to an agent who receives instruction at an educational institution."@en .

<http://rdaregistry.info/Elements/u/P60856>
    reg:hasSubproperty <http://rdaregistry.info/Elements/a/P50288> ;
    reg:lexicalAlias <http://rdaregistry.info/Elements/u/studentAt.en> ;
    reg:name "studentAt"@en ;
    reg:status <http://metadataregistry.org/uri/RegStatus/1001> ;
    a rdf:Property ;
    rdfs:isDefinedBy <http://rdaregistry.info/Elements/u/> ;
    rdfs:label "is student at"@en ;
    rdfs:subPropertyOf <http://rdaregistry.info/Elements/u/P60454> ;
    owl:inverseOf <http://rdaregistry.info/Elements/u/P60855> ;
    skos:definition "Relates an agent to an educational institution that provides instruction to an agent."@en .

<http://rdaregistry.info/Elements/u/P60857>
    reg:hasSubproperty <http://rdaregistry.info/Elements/a/P50275> ;
    reg:lexicalAlias <http://rdaregistry.info/Elements/u/assistant.en> ;
    reg:name "assistant"@en ;
    reg:status <http://metadataregistry.org/uri/RegStatus/1001> ;
    a rdf:Property ;
    rdfs:isDefinedBy <http://rdaregistry.info/Elements/u/> ;
    rdfs:label "has assistant"@en ;
    rdfs:subPropertyOf <http://rdaregistry.info/Elements/u/P60853> ;
    owl:inverseOf <http://rdaregistry.info/Elements/u/P60588> ;
    skos:definition "Relates an agent to a colleague who helps another agent."@en .

<http://rdaregistry.info/Elements/u/P60858>
    reg:hasSubproperty <http://rdaregistry.info/Elements/a/P50276> ;
    reg:lexicalAlias <http://rdaregistry.info/Elements/u/assistantTo.en> ;
    reg:name "assistantTo"@en ;
    reg:status <http://metadataregistry.org/uri/RegStatus/1001> ;
    a rdf:Property ;
    rdfs:isDefinedBy <http://rdaregistry.info/Elements/u/> ;
    rdfs:label "is assistant to"@en ;
    rdfs:subPropertyOf <http://rdaregistry.info/Elements/u/P60853> ;
    owl:inverseOf <http://rdaregistry.info/Elements/u/P60587> ;
    skos:definition "Relates an agent to a colleague who is helped by another agent."@en .

<http://rdaregistry.info/Elements/u/P60859>
    reg:hasSubproperty <http://rdaregistry.info/Elements/a/P50277> ;
    reg:lexicalAlias <http://rdaregistry.info/Elements/u/coworker.en> ;
    reg:name "coworker"@en ;
    reg:status <http://metadataregistry.org/uri/RegStatus/1001> ;
    a rdf:Property ;
    rdfs:isDefinedBy <http://rdaregistry.info/Elements/u/> ;
    rdfs:label "has co-worker"@en ;
    rdfs:subPropertyOf <http://rdaregistry.info/Elements/u/P60853> ;
    owl:inverseOf <http://rdaregistry.info/Elements/u/P60859> ;
    skos:definition "Relates an agent to a colleague who works with or shares a task with another agent."@en .

<http://rdaregistry.info/Elements/u/P60860>
    reg:hasSubproperty <http://rdaregistry.info/Elements/a/P50278> ;
    reg:lexicalAlias <http://rdaregistry.info/Elements/u/partner.en> ;
    reg:name "partner"@en ;
    reg:status <http://metadataregistry.org/uri/RegStatus/1001> ;
    a rdf:Property ;
    rdfs:isDefinedBy <http://rdaregistry.info/Elements/u/> ;
    rdfs:label "has partner"@en ;
    rdfs:subPropertyOf <http://rdaregistry.info/Elements/u/P60853> ;
    owl:inverseOf <http://rdaregistry.info/Elements/u/P60860> ;
    skos:definition "Relates an agent to a colleague working with another agent in an activity of common interest, most often a business partnership."@en .

<http://rdaregistry.info/Elements/u/P60861>
    reg:hasSubproperty <http://rdaregistry.info/Elements/a/P50279> ;
    reg:lexicalAlias <http://rdaregistry.info/Elements/u/fellowStudent.en> ;
    reg:name "fellowStudent"@en ;
    reg:status <http://metadataregistry.org/uri/RegStatus/1001> ;
    a rdf:Property ;
    rdfs:isDefinedBy <http://rdaregistry.info/Elements/u/> ;
    rdfs:label "has fellow student"@en ;
    rdfs:subPropertyOf <http://rdaregistry.info/Elements/u/P60454> ;
    owl:inverseOf <http://rdaregistry.info/Elements/u/P60861> ;
    skos:definition "Relates an agent to an associate of another student who is also formally engaged in learning."@en .

<http://rdaregistry.info/Elements/u/P60862>
    reg:hasSubproperty <http://rdaregistry.info/Elements/a/P50281> ;
    reg:lexicalAlias <http://rdaregistry.info/Elements/u/student.en> ;
    reg:name "student"@en ;
    reg:status <http://metadataregistry.org/uri/RegStatus/1001> ;
    a rdf:Property ;
    rdfs:isDefinedBy <http://rdaregistry.info/Elements/u/> ;
    rdfs:label "has student"@en ;
    rdfs:subPropertyOf <http://rdaregistry.info/Elements/u/P60454> ;
    owl:inverseOf <http://rdaregistry.info/Elements/u/P60863> ;
    skos:definition "Relates an agent to an agent who receives instruction from another agent."@en .

<http://rdaregistry.info/Elements/u/P60863>
    reg:hasSubproperty <http://rdaregistry.info/Elements/a/P50282> ;
    reg:lexicalAlias <http://rdaregistry.info/Elements/u/teacher.en> ;
    reg:name "teacher"@en ;
    reg:status <http://metadataregistry.org/uri/RegStatus/1001> ;
    a rdf:Property ;
    rdfs:isDefinedBy <http://rdaregistry.info/Elements/u/> ;
    rdfs:label "has teacher"@en ;
    rdfs:subPropertyOf <http://rdaregistry.info/Elements/u/P60454> ;
    owl:inverseOf <http://rdaregistry.info/Elements/u/P60862> ;
    skos:definition "Relates an agent to an agent who instructs another agent."@en .

<http://rdaregistry.info/Elements/u/P60864>
    reg:hasSubproperty <http://rdaregistry.info/Elements/a/P50284> ;
    reg:lexicalAlias <http://rdaregistry.info/Elements/u/chiefExecutive.en> ;
    reg:name "chiefExecutive"@en ;
    reg:status <http://metadataregistry.org/uri/RegStatus/1001> ;
    a rdf:Property ;
    rdfs:isDefinedBy <http://rdaregistry.info/Elements/u/> ;
    rdfs:label "has chief executive"@en ;
    rdfs:subPropertyOf <http://rdaregistry.info/Elements/u/P60633> ;
    owl:inverseOf <http://rdaregistry.info/Elements/u/P60865> ;
    skos:definition "Relates an agent to an officer who is a top ranking official of an agent."@en .

<http://rdaregistry.info/Elements/u/P60865>
    reg:hasSubproperty <http://rdaregistry.info/Elements/a/P50286> ;
    reg:lexicalAlias <http://rdaregistry.info/Elements/u/chiefExecutiveOf.en> ;
    reg:name "chiefExecutiveOf"@en ;
    reg:status <http://metadataregistry.org/uri/RegStatus/1001> ;
    a rdf:Property ;
    rdfs:isDefinedBy <http://rdaregistry.info/Elements/u/> ;
    rdfs:label "is chief executive of"@en ;
    rdfs:subPropertyOf <http://rdaregistry.info/Elements/u/P60737> ;
    owl:inverseOf <http://rdaregistry.info/Elements/u/P60864> ;
    skos:definition "Relates an agent to an agent in which an officer is a top ranking official."@en .

<http://rdaregistry.info/Elements/u/P60866>
    reg:hasSubproperty <http://rdaregistry.info/Elements/a/P50285> ;
    reg:lexicalAlias <http://rdaregistry.info/Elements/u/trustee.en> ;
    reg:name "trustee"@en ;
    reg:status <http://metadataregistry.org/uri/RegStatus/1001> ;
    a rdf:Property ;
    rdfs:isDefinedBy <http://rdaregistry.info/Elements/u/> ;
    rdfs:label "has trustee"@en ;
    rdfs:subPropertyOf <http://rdaregistry.info/Elements/u/P60633> ;
    owl:inverseOf <http://rdaregistry.info/Elements/u/P60867> ;
    skos:definition "Relates an agent to an officer granted powers of administration in an agent in order to act for its benefit."@en .

<http://rdaregistry.info/Elements/u/P60867>
    reg:hasSubproperty <http://rdaregistry.info/Elements/a/P50287> ;
    reg:lexicalAlias <http://rdaregistry.info/Elements/u/trusteeOf.en> ;
    reg:name "trusteeOf"@en ;
    reg:status <http://metadataregistry.org/uri/RegStatus/1001> ;
    a rdf:Property ;
    rdfs:isDefinedBy <http://rdaregistry.info/Elements/u/> ;
    rdfs:label "is trustee of"@en ;
    rdfs:subPropertyOf <http://rdaregistry.info/Elements/u/P60737> ;
    owl:inverseOf <http://rdaregistry.info/Elements/u/P60866> ;
    skos:definition "Relates an agent to an agent that grants powers of administration to an officer in order to act for its benefit."@en .

<http://rdaregistry.info/Elements/u/P60868>
    reg:lexicalAlias <http://rdaregistry.info/Elements/u/noteOnIdentifierForResource.en> ;
    reg:name "noteOnIdentifierForResource"@en ;
    reg:status <http://metadataregistry.org/uri/RegStatus/1001> ;
    a rdf:Property ;
    rdfs:isDefinedBy <http://rdaregistry.info/Elements/u/> ;
    rdfs:label "has note on identifier for resource"@en ;
    rdfs:subPropertyOf <http://rdaregistry.info/Elements/u/P60470> ;
    skos:definition "Relates a resource to a note providing information on identifiers for a resource not recorded as part of an identifier for a resource element."@en .

<http://rdaregistry.info/Elements/u/P60869>
    rdakit:seeAlso <http://rdaregistry.info/Elements/u/P60393> ;
    reg:hasSubproperty <http://rdaregistry.info/Elements/w/P10298> ;
    reg:lexicalAlias <http://rdaregistry.info/Elements/u/editorialDirector.en> ;
    reg:name "editorialDirector"@en ;
    reg:status <http://metadataregistry.org/uri/RegStatus/1001> ;
    a rdf:Property ;
    rdfs:isDefinedBy <http://rdaregistry.info/Elements/u/> ;
    rdfs:label "has editorial director"@en ;
    rdfs:subPropertyOf <http://rdaregistry.info/Elements/u/P60374> ;
    owl:inverseOf <http://rdaregistry.info/Elements/u/P60870> ;
    skos:definition "Relates a resource to an agent having legal or intellectual responsibility other than creation for the content of a serial, integrating resource, or multipart monographic resource."@en .

<http://rdaregistry.info/Elements/u/P60870>
    rdakit:seeAlso <http://rdaregistry.info/Elements/u/P60621> ;
    reg:lexicalAlias <http://rdaregistry.info/Elements/u/editorialDirectorOf.en> ;
    reg:name "editorialDirectorOf"@en ;
    reg:status <http://metadataregistry.org/uri/RegStatus/1001> ;
    a rdf:Property ;
    rdfs:isDefinedBy <http://rdaregistry.info/Elements/u/> ;
    rdfs:label "is editorial director of"@en ;
    rdfs:subPropertyOf <http://rdaregistry.info/Elements/u/P60602> ;
    owl:inverseOf <http://rdaregistry.info/Elements/u/P60869> ;
    skos:definition "Relates an agent responsible for a legal or intellectual responsibility other than creation for the content of a serial, integrating resource, or multipart monographic resource to a resource."@en .

<http://rdaregistry.info/Elements/u/P60871>
    reg:hasSubproperty <http://rdaregistry.info/Elements/w/P10299> ;
    reg:lexicalAlias <http://rdaregistry.info/Elements/u/founderOfResource.en> ;
    reg:name "founderOfResource"@en ;
    reg:status <http://metadataregistry.org/uri/RegStatus/1001> ;
    a rdf:Property ;
    rdfs:isDefinedBy <http://rdaregistry.info/Elements/u/> ;
    rdfs:label "has founder of resource"@en ;
    rdfs:subPropertyOf <http://rdaregistry.info/Elements/u/P60374> ;
    owl:inverseOf <http://rdaregistry.info/Elements/u/P60872> ;
    skos:definition "Relates a resource to an agent responsible for establishing a serial, integrating resource, or multipart monographic resource."@en .

<http://rdaregistry.info/Elements/u/P60872>
    reg:lexicalAlias <http://rdaregistry.info/Elements/u/founderOfResourceOf.en> ;
    reg:name "founderOfResourceOf"@en ;
    reg:status <http://metadataregistry.org/uri/RegStatus/1001> ;
    a rdf:Property ;
    rdfs:isDefinedBy <http://rdaregistry.info/Elements/u/> ;
    rdfs:label "is founder of resource of"@en ;
    rdfs:subPropertyOf <http://rdaregistry.info/Elements/u/P60602> ;
    owl:inverseOf <http://rdaregistry.info/Elements/u/P60871> ;
    skos:definition "Relates an agent responsible for establishing a serial, integrating resource, or multipart monograph to a resource."@en .

<http://rdaregistry.info/Elements/u/P60873>
    reg:hasSubproperty <http://rdaregistry.info/Elements/e/P20290> ;
    reg:lexicalAlias <http://rdaregistry.info/Elements/u/aspectRatioDesignation.en> ;
    reg:name "aspectRatioDesignation"@en ;
    reg:status <http://metadataregistry.org/uri/RegStatus/1001> ;
    a rdf:Property ;
    rdfs:isDefinedBy <http://rdaregistry.info/Elements/u/> ;
    rdfs:label "has aspect ratio designation"@en ;
    skos:definition "Relates a resource to a general designation of the ratio of the width to the height of a moving image."@en .

<http://rdaregistry.info/Elements/u/P60874>
    reg:hasSubproperty <http://rdaregistry.info/Elements/e/P20291> ;
    reg:lexicalAlias <http://rdaregistry.info/Elements/u/scaleDesignation.en> ;
    reg:name "scaleDesignation"@en ;
    reg:status <http://metadataregistry.org/uri/RegStatus/1001> ;
    a rdf:Property ;
    rdfs:isDefinedBy <http://rdaregistry.info/Elements/u/> ;
    rdfs:label "has scale designation"@en ;
    skos:definition "Relates a resource to a general designation of a lack of a ratio of the dimensions of the content of an image or three-dimensional form to the dimensions of the thing it represents."@en .

<http://rdaregistry.info/Elements/u/P60875>
    reg:hasSubproperty <http://rdaregistry.info/Elements/m/P30261> ;
    reg:lexicalAlias <http://rdaregistry.info/Elements/u/cartographicDataType.en> ;
    reg:name "cartographicDataType"@en ;
    reg:status <http://metadataregistry.org/uri/RegStatus/1001> ;
    a rdf:Property ;
    rdfs:isDefinedBy <http://rdaregistry.info/Elements/u/> ;
    rdfs:label "has cartographic data type"@en ;
    skos:definition "Relates a resource to a machine-readable representation of geospatial features."@en .

<http://rdaregistry.info/Elements/u/P60876>
    reg:hasSubproperty <http://rdaregistry.info/Elements/m/P30262> ;
    reg:lexicalAlias <http://rdaregistry.info/Elements/u/detailsOfCartographicDataType.en> ;
    reg:name "detailsOfCartographicDataType"@en ;
    reg:status <http://metadataregistry.org/uri/RegStatus/1001> ;
    a rdf:Property ;
    rdfs:isDefinedBy <http://rdaregistry.info/Elements/u/> ;
    rdfs:label "has details of cartographic data type"@en ;
    skos:definition "Relates a resource to details of a machine-readable representation of geospatial features."@en .

<http://rdaregistry.info/Elements/u/P60877>
    reg:hasSubproperty <http://rdaregistry.info/Elements/m/P30263> ;
    reg:lexicalAlias <http://rdaregistry.info/Elements/u/reductionRatioDesignation.en> ;
    reg:name "reductionRatioDesignation"@en ;
    reg:status <http://metadataregistry.org/uri/RegStatus/1001> ;
    a rdf:Property ;
    rdfs:isDefinedBy <http://rdaregistry.info/Elements/u/> ;
    rdfs:label "has reduction ratio designation"@en ;
    skos:definition "Relates a resource to a general designation of the size of a micro-image in relation to an original from which it was produced."@en .

<http://rdaregistry.info/Elements/u/P60878>
    reg:hasSubproperty <http://rdaregistry.info/Elements/a/P50291> ;
    reg:lexicalAlias <http://rdaregistry.info/Elements/u/surname.en> ;
    reg:name "surname"@en ;
    reg:status <http://metadataregistry.org/uri/RegStatus/1001> ;
    a rdf:Property ;
    rdfs:isDefinedBy <http://rdaregistry.info/Elements/u/> ;
    rdfs:label "has surname"@en ;
    skos:definition "Relates an agent to a name used as a family name."@en .

<http://rdaregistry.info/Elements/u/P60879>
    reg:hasSubproperty <http://rdaregistry.info/Elements/a/P50292> ;
    reg:lexicalAlias <http://rdaregistry.info/Elements/u/givenName.en> ;
    reg:name "givenName"@en ;
    reg:status <http://metadataregistry.org/uri/RegStatus/1001> ;
    a rdf:Property ;
    rdfs:isDefinedBy <http://rdaregistry.info/Elements/u/> ;
    rdfs:label "has given name"@en ;
    skos:definition "Relates an agent to a name given to an agent at birth or at some later point in addition to, or instead of, a surname."@en .

<http://rdaregistry.info/Elements/u/P60880>
    reg:hasSubproperty <http://rdaregistry.info/Elements/p/P70003> ;
    reg:lexicalAlias <http://rdaregistry.info/Elements/u/variantNameOfPlace.en> ;
    reg:name "variantNameOfPlace"@en ;
    reg:status <http://metadataregistry.org/uri/RegStatus/1001> ;
    a rdf:Property ;
    rdfs:isDefinedBy <http://rdaregistry.info/Elements/u/> ;
    rdfs:label "has variant name of place"@en ;
    skos:definition "Relates a place to a name or form of name by which a place is known that differs from a name or form of name chosen as a preferred name."@en .

<http://rdaregistry.info/Elements/u/P60881>
    rdakit:seeAlso <http://rdaregistry.info/Elements/u/P60886> ;
    reg:hasSubproperty <http://rdaregistry.info/Elements/a/P50293> ;
    reg:lexicalAlias <http://rdaregistry.info/Elements/u/remixArtistOf.en> ;
    reg:name "remixArtistOf"@en ;
    reg:status <http://metadataregistry.org/uri/RegStatus/1001> ;
    a rdf:Property ;
    rdfs:isDefinedBy <http://rdaregistry.info/Elements/u/> ;
    rdfs:label "is remix artist of"@en ;
    rdfs:subPropertyOf <http://rdaregistry.info/Elements/u/P60672> ;
    owl:inverseOf <http://rdaregistry.info/Elements/u/P60891> ;
    skos:definition "Relates an agent to an audio resource created by manipulating, recombining, mixing, and reproducing previously recorded sounds to a resource."@en ;
    skos:scopeNote "Remixing activities that do not substantially change the nature and content of the original resource, and mixing recorded tracks together to appear as one continuous track are excluded."@en .

<http://rdaregistry.info/Elements/u/P60882>
    reg:hasSubproperty <http://rdaregistry.info/Elements/a/P50294> ;
    reg:lexicalAlias <http://rdaregistry.info/Elements/u/castingDirectorOf.en> ;
    reg:name "castingDirectorOf"@en ;
    reg:status <http://metadataregistry.org/uri/RegStatus/1001> ;
    a rdf:Property ;
    rdfs:isDefinedBy <http://rdaregistry.info/Elements/u/> ;
    rdfs:label "is casting director of"@en ;
    rdfs:subPropertyOf <http://rdaregistry.info/Elements/u/P60672> ;
    owl:inverseOf <http://rdaregistry.info/Elements/u/P60890> ;
    skos:definition "Relates an agent to a resource that incorporates a contribution of responsibility for most aspects of assigning parts and duties to performers."@en .

<http://rdaregistry.info/Elements/u/P60883>
    reg:hasSubproperty <http://rdaregistry.info/Elements/a/P50295> ;
    reg:lexicalAlias <http://rdaregistry.info/Elements/u/audioProducerOf.en> ;
    reg:name "audioProducerOf"@en ;
    reg:status <http://metadataregistry.org/uri/RegStatus/1001> ;
    a rdf:Property ;
    rdfs:isDefinedBy <http://rdaregistry.info/Elements/u/> ;
    rdfs:label "is audio producer of"@en ;
    rdfs:subPropertyOf <http://rdaregistry.info/Elements/u/P60668> ;
    owl:inverseOf <http://rdaregistry.info/Elements/u/P60889> ;
    skos:definition "Relates an agent to a resource that involves a responsibility for most of the business aspects of an audio recording."@en .

<http://rdaregistry.info/Elements/u/P60884>
    reg:hasSubproperty <http://rdaregistry.info/Elements/a/P50296>, <http://rdaregistry.info/Elements/u/P60885> ;
    reg:lexicalAlias <http://rdaregistry.info/Elements/u/audioEngineerOf.en> ;
    reg:name "audioEngineerOf"@en ;
    reg:status <http://metadataregistry.org/uri/RegStatus/1001> ;
    a rdf:Property ;
    rdfs:isDefinedBy <http://rdaregistry.info/Elements/u/> ;
    rdfs:label "is audio engineer of"@en ;
    rdfs:subPropertyOf <http://rdaregistry.info/Elements/u/P60158> ;
    owl:inverseOf <http://rdaregistry.info/Elements/u/P60892> ;
    skos:definition "Relates an agent to a resource that incorporates a contribution to the audio content of managing the technical aspects of sound during the processes of recording, mixing, and reproduction."@en .

<http://rdaregistry.info/Elements/u/P60885>
    rdakit:seeAlso <http://rdaregistry.info/Elements/u/P60881> ;
    reg:hasSubproperty <http://rdaregistry.info/Elements/a/P50297> ;
    reg:lexicalAlias <http://rdaregistry.info/Elements/u/mixingEngineerOf.en> ;
    reg:name "mixingEngineerOf"@en ;
    reg:status <http://metadataregistry.org/uri/RegStatus/1001> ;
    a rdf:Property ;
    rdfs:isDefinedBy <http://rdaregistry.info/Elements/u/> ;
    rdfs:label "is mixing engineer of"@en ;
    rdfs:subPropertyOf <http://rdaregistry.info/Elements/u/P60884> ;
    owl:inverseOf <http://rdaregistry.info/Elements/u/P60893> ;
    skos:definition "Relates an agent to a resource that incorporates a contribution to the audio content of manipulating, mixing and assembling the multiple tracks of a recording."@en ;
    skos:scopeNote "Remixing activities that substantially change the nature and content of the original resource, resulting in a new resource, are excluded."@en .

<http://rdaregistry.info/Elements/u/P60886>
    rdakit:seeAlso <http://rdaregistry.info/Elements/u/P60885> ;
    reg:hasSubproperty <http://rdaregistry.info/Elements/a/P50298> ;
    reg:lexicalAlias <http://rdaregistry.info/Elements/u/DJOf.en> ;
    reg:name "DJOf"@en ;
    reg:status <http://metadataregistry.org/uri/RegStatus/1001> ;
    a rdf:Property ;
    rdfs:isDefinedBy <http://rdaregistry.info/Elements/u/> ;
    rdfs:label "is DJ of"@en ;
    rdfs:subPropertyOf <http://rdaregistry.info/Elements/u/P60158> ;
    owl:inverseOf <http://rdaregistry.info/Elements/u/P60896> ;
    skos:definition "Relates an agent to a resource that incorporates a contribution of mixing recorded tracks together during a live performance or in a recording studio to appear as one continuous track."@en ;
    skos:scopeNote "Remixing activities that substantially change the nature and content of the original resource, resulting in a new resource, and mixing and assembling the multiple tracks of a recording are excluded."@en .

<http://rdaregistry.info/Elements/u/P60887>
    reg:hasSubproperty <http://rdaregistry.info/Elements/a/P50299> ;
    reg:lexicalAlias <http://rdaregistry.info/Elements/u/dubbingDirectorOf.en> ;
    reg:name "dubbingDirectorOf"@en ;
    reg:status <http://metadataregistry.org/uri/RegStatus/1001> ;
    a rdf:Property ;
    rdfs:isDefinedBy <http://rdaregistry.info/Elements/u/> ;
    rdfs:label "is dubbing director of"@en ;
    rdfs:subPropertyOf <http://rdaregistry.info/Elements/u/P60158> ;
    owl:inverseOf <http://rdaregistry.info/Elements/u/P60895> ;
    skos:definition "Relates an agent to a resource that incorporates a contribution of responsibility for the general management and supervision of the process of adding new dialogue or other sounds to complete a sound track."@en .

<http://rdaregistry.info/Elements/u/P60888>
    rdakit:seeAlso <http://rdaregistry.info/Elements/u/P60655> ;
    reg:hasSubproperty <http://rdaregistry.info/Elements/a/P50300> ;
    reg:lexicalAlias <http://rdaregistry.info/Elements/u/musicProgrammerOf.en> ;
    reg:name "musicProgrammerOf"@en ;
    reg:status <http://metadataregistry.org/uri/RegStatus/1001> ;
    a rdf:Property ;
    rdfs:isDefinedBy <http://rdaregistry.info/Elements/u/> ;
    rdfs:label "is music programmer of"@en ;
    rdfs:subPropertyOf <http://rdaregistry.info/Elements/u/P60158> ;
    owl:inverseOf <http://rdaregistry.info/Elements/u/P60894> ;
    skos:definition "Relates an agent to a musical resource that incorporates a contribution of using electronic audio devices or computer software to generate sounds."@en .

<http://rdaregistry.info/Elements/u/P60889>
    reg:hasSubproperty <http://rdaregistry.info/Elements/w/P10304> ;
    reg:lexicalAlias <http://rdaregistry.info/Elements/u/audioProducer.en> ;
    reg:name "audioProducer"@en ;
    reg:status <http://metadataregistry.org/uri/RegStatus/1001> ;
    a rdf:Property ;
    rdfs:isDefinedBy <http://rdaregistry.info/Elements/u/> ;
    rdfs:label "has audio producer"@en ;
    rdfs:subPropertyOf <http://rdaregistry.info/Elements/u/P60441> ;
    owl:inverseOf <http://rdaregistry.info/Elements/u/P60883> ;
    skos:definition "Relates a resource to a producer responsible for most of the business aspects of an audio recording."@en .

<http://rdaregistry.info/Elements/u/P60890>
    reg:hasSubproperty <http://rdaregistry.info/Elements/w/P10305> ;
    reg:lexicalAlias <http://rdaregistry.info/Elements/u/castingDirector.en> ;
    reg:name "castingDIrector"@en ;
    reg:status <http://metadataregistry.org/uri/RegStatus/1001> ;
    a rdf:Property ;
    rdfs:isDefinedBy <http://rdaregistry.info/Elements/u/> ;
    rdfs:label "has casting director"@en ;
    rdfs:subPropertyOf <http://rdaregistry.info/Elements/u/P60158> ;
    owl:inverseOf <http://rdaregistry.info/Elements/u/P60882> ;
    skos:definition "Relates a resource to an agent responsible for most aspects of assigning parts and duties to performers."@en .

<http://rdaregistry.info/Elements/u/P60891>
    rdakit:seeAlso <http://rdaregistry.info/Elements/u/P60896> ;
    reg:hasSubproperty <http://rdaregistry.info/Elements/w/P10306> ;
    reg:lexicalAlias <http://rdaregistry.info/Elements/u/remixArtist.en> ;
    reg:name "remixArtist"@en ;
    reg:status <http://metadataregistry.org/uri/RegStatus/1001> ;
    a rdf:Property ;
    rdfs:isDefinedBy <http://rdaregistry.info/Elements/u/> ;
    rdfs:label "has remix artist"@en ;
    rdfs:subPropertyOf <http://rdaregistry.info/Elements/u/P60447> ;
    owl:inverseOf <http://rdaregistry.info/Elements/u/P60881> ;
    skos:definition "Relates a resource to an agent responsible for creating an audio resource by manipulating, recombining, mixing, and reproducing previously recorded sounds."@en ;
    skos:scopeNote "Remixing activities that do not substantially change the nature and content of the original resource, and mixing recorded tracks together to appear as one continuous track are excluded."@en .

<http://rdaregistry.info/Elements/u/P60892>
    reg:hasSubproperty <http://rdaregistry.info/Elements/e/P20292>, <http://rdaregistry.info/Elements/u/P60893> ;
    reg:lexicalAlias <http://rdaregistry.info/Elements/u/audioEngineer.en> ;
    reg:name "audioEngineer"@en ;
    reg:status <http://metadataregistry.org/uri/RegStatus/1001> ;
    a rdf:Property ;
    rdfs:isDefinedBy <http://rdaregistry.info/Elements/u/> ;
    rdfs:label "has audio engineer"@en ;
    rdfs:subPropertyOf <http://rdaregistry.info/Elements/u/P60398> ;
    owl:inverseOf <http://rdaregistry.info/Elements/u/P60884> ;
    skos:definition "Relates a resource to an agent contributing to the audio content of a resource by managing the technical aspects of sound during the processes of recording, mixing, and reproduction."@en .

<http://rdaregistry.info/Elements/u/P60893>
    rdakit:seeAlso <http://rdaregistry.info/Elements/u/P60891> ;
    reg:hasSubproperty <http://rdaregistry.info/Elements/e/P20293> ;
    reg:lexicalAlias <http://rdaregistry.info/Elements/u/mixingEngineer.en> ;
    reg:name "mixingEngineer"@en ;
    reg:status <http://metadataregistry.org/uri/RegStatus/1001> ;
    a rdf:Property ;
    rdfs:isDefinedBy <http://rdaregistry.info/Elements/u/> ;
    rdfs:label "has mixing engineer"@en ;
    rdfs:subPropertyOf <http://rdaregistry.info/Elements/u/P60892> ;
    owl:inverseOf <http://rdaregistry.info/Elements/u/P60885> ;
    skos:definition "Relates a resource to an audio engineer contributing to the audio content of a resource by manipulating, mixing, and assembling the multiple tracks of a recording."@en ;
    skos:scopeNote "Remixing activities that substantially change the nature and content of the original resource, resulting in a new resource, are excluded."@en .

<http://rdaregistry.info/Elements/u/P60894>
    rdakit:seeAlso <http://rdaregistry.info/Elements/u/P60426> ;
    reg:hasSubproperty <http://rdaregistry.info/Elements/e/P20294> ;
    reg:lexicalAlias <http://rdaregistry.info/Elements/u/musicProgrammer.en> ;
    reg:name "musicProgrammer"@en ;
    reg:status <http://metadataregistry.org/uri/RegStatus/1001> ;
    a rdf:Property ;
    rdfs:isDefinedBy <http://rdaregistry.info/Elements/u/> ;
    rdfs:label "has music programmer"@en ;
    rdfs:subPropertyOf <http://rdaregistry.info/Elements/u/P60398> ;
    owl:inverseOf <http://rdaregistry.info/Elements/u/P60888> ;
    skos:definition "Relates a resource to an agent contributing to a musical resource by using electronic audio devices or computer software to generate sounds."@en ;
    skos:scopeNote "The creation of a new musical resource is excluded."@en .

<http://rdaregistry.info/Elements/u/P60895>
    reg:hasSubproperty <http://rdaregistry.info/Elements/e/P20295> ;
    reg:lexicalAlias <http://rdaregistry.info/Elements/u/dubbingDirector.en> ;
    reg:name "dubbingDirector"@en ;
    reg:status <http://metadataregistry.org/uri/RegStatus/1001> ;
    a rdf:Property ;
    rdfs:isDefinedBy <http://rdaregistry.info/Elements/u/> ;
    rdfs:label "has dubbing director"@en ;
    rdfs:subPropertyOf <http://rdaregistry.info/Elements/u/P60398> ;
    owl:inverseOf <http://rdaregistry.info/Elements/u/P60887> ;
    skos:definition "Relates a resource to an agent responsible for the general management and supervision of the process of adding new dialogue or other sounds to complete a sound track for a resource"@en .

<http://rdaregistry.info/Elements/u/P60896>
    rdakit:seeAlso <http://rdaregistry.info/Elements/u/P60893> ;
    reg:hasSubproperty <http://rdaregistry.info/Elements/e/P20296> ;
    reg:lexicalAlias <http://rdaregistry.info/Elements/u/DJ.en> ;
    reg:name "DJ"@en ;
    reg:status <http://metadataregistry.org/uri/RegStatus/1001> ;
    a rdf:Property ;
    rdfs:isDefinedBy <http://rdaregistry.info/Elements/u/> ;
    rdfs:label "has DJ"@en ;
    rdfs:subPropertyOf <http://rdaregistry.info/Elements/u/P60398> ;
    owl:inverseOf <http://rdaregistry.info/Elements/u/P60886> ;
    skos:definition "Relates a resource to an agent who mixes recorded tracks together during a live performance or in a recording studio to appear as one continuous track."@en ;
    skos:scopeNote "Remixing activities that substantially change the nature and content of the original resource, resulting in a new resource, and mixing and assembling the multiple tracks of a recording are excluded."@en .

<http://rdaregistry.info/Elements/u/P60897>
    reg:lexicalAlias <http://rdaregistry.info/Elements/u/latitude.en> ;
    reg:name "latitude"@en ;
    reg:status <http://metadataregistry.org/uri/RegStatus/1001> ;
    a rdf:Property ;
    rdfs:isDefinedBy <http://rdaregistry.info/Elements/u/> ;
    rdfs:label "has latitude"@en ;
    skos:definition "Relates a resource to a distance of a point on a planet or satellite measured north and south from the equator."@en .

<http://rdaregistry.info/Elements/u/P60898>
    reg:lexicalAlias <http://rdaregistry.info/Elements/u/longitude.en> ;
    reg:name "longitude"@en ;
    reg:status <http://metadataregistry.org/uri/RegStatus/1001> ;
    a rdf:Property ;
    rdfs:isDefinedBy <http://rdaregistry.info/Elements/u/> ;
    rdfs:label "has longitude"@en ;
    skos:definition "Relates a resource to a distance of a point on a planet or satellite measured east and west from a reference meridian."@en .

<http://rdaregistry.info/Elements/u/P60899>
    reg:lexicalAlias <http://rdaregistry.info/Elements/u/rightAscension.en> ;
    reg:name "rightAscension"@en ;
    reg:status <http://metadataregistry.org/uri/RegStatus/1001> ;
    a rdf:Property ;
    rdfs:isDefinedBy <http://rdaregistry.info/Elements/u/> ;
    rdfs:label "has right ascension"@en ;
    skos:definition "Relates a resource to an angular distance measured eastward on the equator from the vernal equinox to the hour circle through a celestial body, from 0 to 24 hours.."@en .

<http://rdaregistry.info/Elements/u/P60900>
    reg:lexicalAlias <http://rdaregistry.info/Elements/u/declination.en> ;
    reg:name "declination"@en ;
    reg:status <http://metadataregistry.org/uri/RegStatus/1001> ;
    a rdf:Property ;
    rdfs:isDefinedBy <http://rdaregistry.info/Elements/u/> ;
    rdfs:label "has declination"@en ;
    skos:definition "Relates a resource to an angular distance to a body on the celestial sphere measured north or south through 90 from the celestial equator along the hour circle of the body."@en .

<http://rdaregistry.info/Elements/u/P60901>
    reg:lexicalAlias <http://rdaregistry.info/Elements/u/absorbedAgent.en> ;
    reg:name "absorbedAgent"@en ;
    reg:status <http://metadataregistry.org/uri/RegStatus/1001> ;
    a rdf:Property ;
    rdfs:isDefinedBy <http://rdaregistry.info/Elements/u/> ;
    rdfs:label "has absorbed agent"@en ;
    owl:inverseOf <http://rdaregistry.info/Elements/u/P60902> ;
    skos:definition "Relates an agent to an agent that was absorbed by another agent."@en .

<http://rdaregistry.info/Elements/u/P60902>
    reg:lexicalAlias <http://rdaregistry.info/Elements/u/absorbingAgent.en> ;
    reg:name "absorbingAgent"@en ;
    reg:status <http://metadataregistry.org/uri/RegStatus/1001> ;
    a rdf:Property ;
    rdfs:isDefinedBy <http://rdaregistry.info/Elements/u/> ;
    rdfs:label "has absorbing agent"@en ;
    owl:inverseOf <http://rdaregistry.info/Elements/u/P60901> ;
    skos:definition "Relates an agent to an agent that absorbed another agent."@en .

<http://rdaregistry.info/Elements/u/P60903>
    reg:lexicalAlias <http://rdaregistry.info/Elements/u/jointlyHeldConference.en> ;
    reg:name "jointlyHeldConference"@en ;
    reg:status <http://metadataregistry.org/uri/RegStatus/1001> ;
    a rdf:Property ;
    rdfs:isDefinedBy <http://rdaregistry.info/Elements/u/> ;
    rdfs:label "has jointly held conference"@en ;
    owl:inverseOf <http://rdaregistry.info/Elements/u/P60903> ;
    skos:definition "Relates a conference to a conference that is jointly held with another conference."@en .

<http://rdaregistry.info/Elements/u/P60904>
    reg:lexicalAlias <http://rdaregistry.info/Elements/u/detailsOfRegionalEncoding.en> ;
    reg:name "detailsOfRegionalEncoding"@en ;
    reg:status <http://metadataregistry.org/uri/RegStatus/1001> ;
    a rdf:Property ;
    rdfs:isDefinedBy <http://rdaregistry.info/Elements/u/> ;
    rdfs:label "has details of regional encoding"@en ;
    rdfs:subPropertyOf <http://rdaregistry.info/Elements/u/P60772> ;
    skos:definition "Relates a resource to details of a designation for one or more regions of the world for which a videodisc or video game carrier has been encoded, indicating that playback is restricted to a device configured to decode it."@en .

<http://rdaregistry.info/Elements/u/P60905>
    reg:lexicalAlias <http://rdaregistry.info/Elements/u/noteOnCapture.en> ;
    reg:name "noteOnCapture"@en ;
    reg:status <http://metadataregistry.org/uri/RegStatus/1001> ;
    a rdf:Property ;
    rdfs:isDefinedBy <http://rdaregistry.info/Elements/u/> ;
    rdfs:label "has note on capture"@en ;
    rdfs:subPropertyOf <http://rdaregistry.info/Elements/u/P60470> ;
    skos:definition "Relates a resource to a note providing information associated with the recording, filming, etc., of the content of a resource."@en ;
    skos:scopeNote "Note on capture includes the circumstances such as a live or studio recording, the equipment used, etc."@en .

