@prefix dc: <http://purl.org/dc/elements/1.1/> .
@prefix dcterms: <http://purl.org/dc/terms/> .
@prefix foaf: <http://xmlns.com/foaf/0.1/> .
@prefix owl: <http://www.w3.org/2002/07/owl#> .
@prefix rdf: <http://www.w3.org/1999/02/22-rdf-syntax-ns#> .
@prefix rdfs: <http://www.w3.org/2000/01/rdf-schema#> .
@prefix reg: <http://metadataregistry.org/uri/profile/RegAp/> .
@prefix skos: <http://www.w3.org/2004/02/skos/core#> .
@prefix status: <http://metadataregistry.org/uri/RegStatus/> .
@prefix xml: <http://www.w3.org/XML/1998/namespace> .
@prefix xsd: <http://www.w3.org/2001/XMLSchema#> .

<http://rdaregistry.info/Elements/e/P20001> a rdf:Property ;
    rdfs:label "has content type"@en ;
    reg:hasUnconstrained <http://rdaregistry.info/Elements/u/P60049> ;
    reg:lexicalAlias "http://rdaregistry.info/Elements/e/contentType"@en ;
    reg:name "contentType"@en ;
    reg:status <http://metadataregistry.org/uri/RegStatus/1001> ;
    rdfs:domain <http://rdaregistry.info/Elements/c/C10006> ;
    rdfs:isDefinedBy <http://rdaregistry.info/Elements/e/> ;
    skos:definition "Relates an expression to a categorization reflecting the fundamental form of communication in which the content is expressed and the human sense through which it is intended to be perceived."@en ;
    skos:scopeNote "For content expressed in the form of an image or images, content type also reflects the number of spatial dimensions in which the content is intended to be perceived and the perceived presence or absence of movement."@en .

<http://rdaregistry.info/Elements/e/P20002> a rdf:Property ;
    rdfs:label "has identifier for the expression"@en ;
    reg:hasUnconstrained <http://rdaregistry.info/Elements/u/P60052> ;
    reg:lexicalAlias "http://rdaregistry.info/Elements/e/identifierForTheExpression"@en ;
    reg:name "identifierForTheExpression"@en ;
    reg:status <http://metadataregistry.org/uri/RegStatus/1001> ;
    rdfs:domain <http://rdaregistry.info/Elements/c/C10006> ;
    rdfs:isDefinedBy <http://rdaregistry.info/Elements/e/> ;
    skos:definition "Relates an expression to a character string uniquely associated with an expression, or with a surrogate for an expression (e.g., an authority record)."@en ;
    skos:scopeNote "The identifier serves to differentiate that expression from other expressions."@en .

<http://rdaregistry.info/Elements/e/P20003> a rdf:Property ;
    rdfs:label "has other distinguishing characteristic of the expression"@en ;
    reg:hasUnconstrained <http://rdaregistry.info/Elements/u/P60054> ;
    reg:lexicalAlias "http://rdaregistry.info/Elements/e/otherDistinguishingCharacteristicOfTheExpression"@en ;
    reg:name "otherDistinguishingCharacteristicOfTheExpression"@en ;
    reg:status <http://metadataregistry.org/uri/RegStatus/1001> ;
    rdfs:domain <http://rdaregistry.info/Elements/c/C10006> ;
    rdfs:isDefinedBy <http://rdaregistry.info/Elements/e/> ;
    skos:definition "Relates an expression to a characteristic other than content type, language of expression, or date of expression."@en ;
    skos:scopeNote "It serves to differentiate an expression from another expression of the same work."@en .

<http://rdaregistry.info/Elements/e/P20004> a rdf:Property ;
    rdfs:label "has date of capture"@en ;
    reg:hasUnconstrained <http://rdaregistry.info/Elements/u/P60074> ;
    reg:lexicalAlias "http://rdaregistry.info/Elements/e/dateOfCapture"@en ;
    reg:name "dateOfCapture"@en ;
    reg:status <http://metadataregistry.org/uri/RegStatus/1001> ;
    rdfs:domain <http://rdaregistry.info/Elements/c/C10006> ;
    rdfs:isDefinedBy <http://rdaregistry.info/Elements/e/> ;
    skos:definition "Relates an expression to a date or range of dates associated with the capture (i.e., recording, filming, etc.) of the content of a resource."@en .

<http://rdaregistry.info/Elements/e/P20005> a rdf:Property ;
    rdfs:label "has award"@en ;
    reg:hasUnconstrained <http://rdaregistry.info/Elements/u/P60090> ;
    reg:lexicalAlias "http://rdaregistry.info/Elements/e/award"@en ;
    reg:name "award"@en ;
    reg:status <http://metadataregistry.org/uri/RegStatus/1001> ;
    rdfs:domain <http://rdaregistry.info/Elements/c/C10006> ;
    rdfs:isDefinedBy <http://rdaregistry.info/Elements/e/> ;
    skos:definition "Relates an expression to a formal recognition of excellence, etc., given by an award- or prize-granting body, for the content of a resource."@en .

<http://rdaregistry.info/Elements/e/P20006> a rdf:Property ;
    rdfs:label "has language of expression"@en ;
    reg:hasUnconstrained <http://rdaregistry.info/Elements/u/P60099> ;
    reg:lexicalAlias "http://rdaregistry.info/Elements/e/languageOfExpression"@en ;
    reg:name "languageOfExpression"@en ;
    reg:status <http://metadataregistry.org/uri/RegStatus/1001> ;
    rdfs:domain <http://rdaregistry.info/Elements/c/C10006> ;
    rdfs:isDefinedBy <http://rdaregistry.info/Elements/e/> ;
    skos:definition "Relates an expression to a language in which a work is expressed."@en .

<http://rdaregistry.info/Elements/e/P20007> a rdf:Property ;
    rdfs:label "has language of the content"@en ;
    reg:hasUnconstrained <http://rdaregistry.info/Elements/u/P60099> ;
    reg:lexicalAlias "http://rdaregistry.info/Elements/e/languageOfTheContent"@en ;
    reg:name "languageOfTheContent"@en ;
    reg:status <http://metadataregistry.org/uri/RegStatus/1001> ;
    rdfs:domain <http://rdaregistry.info/Elements/c/C10006> ;
    rdfs:isDefinedBy <http://rdaregistry.info/Elements/e/> ;
    skos:definition "Relates an expression to a language used to express the content of a resource."@en .

<http://rdaregistry.info/Elements/e/P20008> a rdf:Property ;
    rdfs:label "has artistic and/or technical credit"@en ;
    reg:name "artisticAndOrTechnicalCredit"@en ;
    reg:status <http://metadataregistry.org/uri/RegStatus/1008> ;
    rdfs:domain <http://rdaregistry.info/Elements/c/C10006> ;
    rdfs:isDefinedBy <http://rdaregistry.info/Elements/e/> ;
    rdfs:subPropertyOf <http://rdaregistry.info/Elements/u/P60105> ;
    = <http://rdaregistry.info/Elements/e/artisticAndOrTechnicalCredit> ;
    skos:definition "Relates an expression to a listing of persons, families, or corporate bodies making contributions to the artistic and/or technical production of a resource."@en .

<http://rdaregistry.info/Elements/e/P20040> a rdf:Property ;
    rdfs:label "has court reporter "@en ;
    reg:hasUnconstrained <http://rdaregistry.info/Elements/u/P60388> ;
    reg:lexicalAlias "http://rdaregistry.info/Elements/e/courtReporter"@en ;
    reg:name "courtReporter"@en ;
    reg:status <http://metadataregistry.org/uri/RegStatus/1001> ;
    rdfs:domain <http://rdaregistry.info/Elements/c/C10006> ;
    rdfs:isDefinedBy <http://rdaregistry.info/Elements/e/> ;
    rdfs:range <http://rdaregistry.info/Elements/c/C10002> ;
    rdfs:subPropertyOf <http://rdaregistry.info/Elements/e/P20053> ;
    owl:inverseOf <http://rdaregistry.info/Elements/a/P50148> ;
    skos:definition "Relates an expression to a person, family, or corporate body contributing to an expression of a work by preparing a court’s opinions for publication."@en .

<http://rdaregistry.info/Elements/e/P20054> a rdf:Property ;
    rdfs:label "has presenter "@en ;
    reg:hasUnconstrained <http://rdaregistry.info/Elements/u/P60419> ;
    reg:lexicalAlias "http://rdaregistry.info/Elements/e/presenter"@en ;
    reg:name "presenter"@en ;
    reg:status <http://metadataregistry.org/uri/RegStatus/1001> ;
    rdfs:domain <http://rdaregistry.info/Elements/c/C10006> ;
    rdfs:isDefinedBy <http://rdaregistry.info/Elements/e/> ;
    rdfs:range <http://rdaregistry.info/Elements/c/C10002> ;
    rdfs:subPropertyOf <http://rdaregistry.info/Elements/e/P20053> ;
    owl:inverseOf <http://rdaregistry.info/Elements/a/P50180> ;
    skos:definition "Relates an expression to a person, family, or corporate body mentioned in an \"X presents&quot: credit for moving image materials and who is probably associated with production, finance, or distribution in some way."@en .

<http://rdaregistry.info/Elements/e/P20057> a rdf:Property ;
    rdfs:label "has performer, narrator, and/or presenter"@en ;
    reg:name "performerNarratorAndOrPresenter"@en ;
    reg:status <http://metadataregistry.org/uri/RegStatus/1008> ;
    rdfs:domain <http://rdaregistry.info/Elements/c/C10006> ;
    rdfs:isDefinedBy <http://rdaregistry.info/Elements/e/> ;
    rdfs:subPropertyOf <http://rdaregistry.info/Elements/u/P60442> ;
    = <http://rdaregistry.info/Elements/e/performerNarratorAndOrPresenter> ;
    skos:definition "Relates an expression to a person, family, or corporate body responsible for performing, narrating, and/or presenting a work."@en .

<http://rdaregistry.info/Elements/e/P20059> a rdf:Property ;
    rdfs:label "has manifestation of expression"@en ;
    reg:lexicalAlias "http://rdaregistry.info/Elements/e/manifestationOfExpression"@en ;
    reg:name "manifestationOfExpression"@en ;
    reg:status <http://metadataregistry.org/uri/RegStatus/1001> ;
    rdfs:domain <http://rdaregistry.info/Elements/c/C10006> ;
    rdfs:isDefinedBy <http://rdaregistry.info/Elements/e/> ;
    rdfs:range <http://rdaregistry.info/Elements/c/C10007> ;
    owl:inverseOf <http://rdaregistry.info/Elements/m/P30139> ;
    skos:definition "Relates an expression to a physical embodiment of an expression."@en .

<http://rdaregistry.info/Elements/e/P20069> a rdf:Property ;
    rdfs:label "has summarization of the content"@en ;
    reg:hasUnconstrained <http://rdaregistry.info/Elements/u/P60372> ;
    reg:lexicalAlias "http://rdaregistry.info/Elements/e/summarizationOfTheContent"@en ;
    reg:name "summarizationOfTheContent"@en ;
    reg:status <http://metadataregistry.org/uri/RegStatus/1001> ;
    rdfs:domain <http://rdaregistry.info/Elements/c/C10006> ;
    rdfs:isDefinedBy <http://rdaregistry.info/Elements/e/> ;
    skos:definition "Relates an expression to an abstract, summary, synopsis, etc., of the content of a resource."@en .

<http://rdaregistry.info/Elements/e/P20178> a rdf:Property ;
    reg:status <http://metadataregistry.org/uri/RegStatus/1001> ;
    rdfs:isDefinedBy <http://rdaregistry.info/Elements/e/> .

<http://rdaregistry.info/Elements/e/P20182> a rdf:Property ;
    reg:status <http://metadataregistry.org/uri/RegStatus/1001> ;
    rdfs:isDefinedBy <http://rdaregistry.info/Elements/e/> .

<http://rdaregistry.info/Elements/e/P20187> a rdf:Property ;
    reg:status <http://metadataregistry.org/uri/RegStatus/1001> ;
    rdfs:isDefinedBy <http://rdaregistry.info/Elements/e/> .

<http://rdaregistry.info/Elements/e/P20206> a rdf:Property ;
    rdfs:label "has supplementary content"@en ;
    reg:hasUnconstrained <http://rdaregistry.info/Elements/u/P60485> ;
    reg:lexicalAlias "http://rdaregistry.info/Elements/e/supplementaryContent"@en ;
    reg:name "supplementaryContent"@en ;
    reg:status <http://metadataregistry.org/uri/RegStatus/1001> ;
    rdfs:domain <http://rdaregistry.info/Elements/c/C10006> ;
    rdfs:isDefinedBy <http://rdaregistry.info/Elements/e/> ;
    skos:definition "Relates an expression to content (e.g., an index, a bibliography, an appendix) intended to supplement the primary content of a resource."@en .

<http://rdaregistry.info/Elements/e/P20207> a rdf:Property ;
    rdfs:label "has illustrative content"@en ;
    reg:hasUnconstrained <http://rdaregistry.info/Elements/u/P60486> ;
    reg:lexicalAlias "http://rdaregistry.info/Elements/e/illustrativeContent"@en ;
    reg:name "illustrativeContent"@en ;
    reg:status <http://metadataregistry.org/uri/RegStatus/1001> ;
    rdfs:domain <http://rdaregistry.info/Elements/c/C10006> ;
    rdfs:isDefinedBy <http://rdaregistry.info/Elements/e/> ;
    skos:definition "Relates an expression to content intended to illustrate the primary content of a resource."@en .

<http://rdaregistry.info/Elements/e/P20208> a rdf:Property ;
    rdfs:label "has accessibility content"@en ;
    reg:hasUnconstrained <http://rdaregistry.info/Elements/u/P60487> ;
    reg:lexicalAlias "http://rdaregistry.info/Elements/e/accessibilityContent"@en ;
    reg:name "accessibilityContent"@en ;
    reg:status <http://metadataregistry.org/uri/RegStatus/1001> ;
    rdfs:domain <http://rdaregistry.info/Elements/c/C10006> ;
    rdfs:isDefinedBy <http://rdaregistry.info/Elements/e/> ;
    skos:definition "Relates an expression to content that assists those with a sensory impairment in the greater understanding of content which their impairment prevents them fully seeing or hearing."@en .

<http://rdaregistry.info/Elements/e/P20209> a rdf:Property ;
    rdfs:label "has format of notated music"@en ;
    reg:hasUnconstrained <http://rdaregistry.info/Elements/u/P60488> ;
    reg:lexicalAlias "http://rdaregistry.info/Elements/e/formatOfNotatedMusic"@en ;
    reg:name "formatOfNotatedMusic"@en ;
    reg:status <http://metadataregistry.org/uri/RegStatus/1001> ;
    rdfs:domain <http://rdaregistry.info/Elements/c/C10006> ;
    rdfs:isDefinedBy <http://rdaregistry.info/Elements/e/> ;
    skos:definition "Relates an expression to the musical or physical layout of the content of a resource that is presented in the form of musical notation."@en .

<http://rdaregistry.info/Elements/e/P20210> a rdf:Property ;
    rdfs:label "has other details of cartographic content"@en ;
    reg:hasUnconstrained <http://rdaregistry.info/Elements/u/P60498> ;
    reg:lexicalAlias "http://rdaregistry.info/Elements/e/otherDetailsOfCartographicContent"@en ;
    reg:name "otherDetailsOfCartographicContent"@en ;
    reg:status <http://metadataregistry.org/uri/RegStatus/1001> ;
    rdfs:domain <http://rdaregistry.info/Elements/c/C10006> ;
    rdfs:isDefinedBy <http://rdaregistry.info/Elements/e/> ;
    skos:definition "Relates an expression to mathematical data and other features of the cartographic content of a resource not recorded in statements of scale, projection, and coordinates."@en .

<http://rdaregistry.info/Elements/e/P20214> a rdf:Property ;
    rdfs:label "has date of expression"@en ;
    reg:hasUnconstrained <http://rdaregistry.info/Elements/u/P60527> ;
    reg:lexicalAlias "http://rdaregistry.info/Elements/e/dateOfExpression"@en ;
    reg:name "dateOfExpression"@en ;
    reg:status <http://metadataregistry.org/uri/RegStatus/1001> ;
    rdfs:domain <http://rdaregistry.info/Elements/c/C10006> ;
    rdfs:isDefinedBy <http://rdaregistry.info/Elements/e/> ;
    skos:definition "Relates an expression to the earliest date associated with an expression."@en .

<http://rdaregistry.info/Elements/e/P20215> a rdf:Property ;
    rdfs:label "has medium of performance of musical content"@en ;
    reg:hasUnconstrained <http://rdaregistry.info/Elements/u/P60537> ;
    reg:lexicalAlias "http://rdaregistry.info/Elements/e/mediumOfPerformanceOfMusicalContent"@en ;
    reg:name "mediumOfPerformanceOfMusicalContent"@en ;
    reg:status <http://metadataregistry.org/uri/RegStatus/1001> ;
    rdfs:domain <http://rdaregistry.info/Elements/c/C10006> ;
    rdfs:isDefinedBy <http://rdaregistry.info/Elements/e/> ;
    skos:definition "Relates an expression to the instrument, instruments, voice, voices, etc., used (or intended to be used) for performance of musical content."@en .

<http://rdaregistry.info/Elements/e/P20216> a rdf:Property ;
    rdfs:label "has projection of cartographic content"@en ;
    reg:hasUnconstrained <http://rdaregistry.info/Elements/u/P60542> ;
    reg:lexicalAlias "http://rdaregistry.info/Elements/e/projectionOfCartographicContent"@en ;
    reg:name "projectionOfCartographicContent"@en ;
    reg:status <http://metadataregistry.org/uri/RegStatus/1001> ;
    rdfs:domain <http://rdaregistry.info/Elements/c/C10006> ;
    rdfs:isDefinedBy <http://rdaregistry.info/Elements/e/> ;
    skos:definition "Relates an expression to the method or system used to represent the surface of the earth or of a celestial sphere on a plane."@en .

<http://rdaregistry.info/Elements/e/P20217> a rdf:Property ;
    rdfs:label "has place and date of capture"@en ;
    reg:hasUnconstrained <http://rdaregistry.info/Elements/u/P60555> ;
    reg:lexicalAlias "http://rdaregistry.info/Elements/e/placeAndDateOfCapture"@en ;
    reg:name "placeAndDateOfCapture"@en ;
    reg:status <http://metadataregistry.org/uri/RegStatus/1001> ;
    rdfs:domain <http://rdaregistry.info/Elements/c/C10006> ;
    rdfs:isDefinedBy <http://rdaregistry.info/Elements/e/> ;
    skos:definition "Relates an expression to the place and date associated with the capture (i.e., recording, filming, etc.) of the content of a resource."@en .

<http://rdaregistry.info/Elements/e/P20218> a rdf:Property ;
    rdfs:label "has place of capture"@en ;
    reg:hasUnconstrained <http://rdaregistry.info/Elements/u/P60556> ;
    reg:lexicalAlias "http://rdaregistry.info/Elements/e/placeOfCapture"@en ;
    reg:name "placeOfCapture"@en ;
    reg:status <http://metadataregistry.org/uri/RegStatus/1001> ;
    rdfs:domain <http://rdaregistry.info/Elements/c/C10006> ;
    rdfs:isDefinedBy <http://rdaregistry.info/Elements/e/> ;
    skos:definition "Relates an expression to the place associated with the capture (i.e., recording, filming, etc.) of the content of a resource."@en .

<http://rdaregistry.info/Elements/e/P20219> a rdf:Property ;
    rdfs:label "has duration"@en ;
    reg:hasUnconstrained <http://rdaregistry.info/Elements/u/P60557> ;
    reg:lexicalAlias "http://rdaregistry.info/Elements/e/duration"@en ;
    reg:name "duration"@en ;
    reg:status <http://metadataregistry.org/uri/RegStatus/1001> ;
    rdfs:domain <http://rdaregistry.info/Elements/c/C10006> ;
    rdfs:isDefinedBy <http://rdaregistry.info/Elements/e/> ;
    skos:definition "Relates an expression to the playing time, performance time, running time, etc., of the content of a resource."@en .

<http://rdaregistry.info/Elements/e/P20220> a rdf:Property ;
    reg:status <http://metadataregistry.org/uri/RegStatus/1001> ;
    rdfs:isDefinedBy <http://rdaregistry.info/Elements/e/> .

<http://rdaregistry.info/Elements/e/P20221> a rdf:Property ;
    reg:status <http://metadataregistry.org/uri/RegStatus/1001> ;
    rdfs:isDefinedBy <http://rdaregistry.info/Elements/e/> .

<http://rdaregistry.info/Elements/e/P20222> a rdf:Property ;
    reg:status <http://metadataregistry.org/uri/RegStatus/1001> ;
    rdfs:isDefinedBy <http://rdaregistry.info/Elements/e/> .

<http://rdaregistry.info/Elements/e/P20223> a rdf:Property ;
    reg:status <http://metadataregistry.org/uri/RegStatus/1001> ;
    rdfs:isDefinedBy <http://rdaregistry.info/Elements/e/> .

<http://rdaregistry.info/Elements/e/P20224> a rdf:Property ;
    rdfs:label "has colour content"@en ;
    reg:hasUnconstrained <http://rdaregistry.info/Elements/u/P60558> ;
    reg:lexicalAlias "http://rdaregistry.info/Elements/e/colourContent"@en ;
    reg:name "colourContent"@en ;
    reg:status <http://metadataregistry.org/uri/RegStatus/1001> ;
    rdfs:domain <http://rdaregistry.info/Elements/c/C10006> ;
    rdfs:isDefinedBy <http://rdaregistry.info/Elements/e/> ;
    skos:definition "Relates an expression to the presence of colour, tone, etc., in the content of a resource. "@en .

<http://rdaregistry.info/Elements/e/P20225> a rdf:Property ;
    rdfs:label "has sound content"@en ;
    reg:hasUnconstrained <http://rdaregistry.info/Elements/u/P60559> ;
    reg:lexicalAlias "http://rdaregistry.info/Elements/e/soundContent"@en ;
    reg:name "soundContent"@en ;
    reg:status <http://metadataregistry.org/uri/RegStatus/1001> ;
    rdfs:domain <http://rdaregistry.info/Elements/c/C10006> ;
    rdfs:isDefinedBy <http://rdaregistry.info/Elements/e/> ;
    skos:definition "Relates an expression to the presence of sound in a resource other than one that consists primarily of recorded sound."@en .

<http://rdaregistry.info/Elements/e/P20229> a rdf:Property ;
    rdfs:label "has aspect ratio"@en ;
    reg:hasUnconstrained <http://rdaregistry.info/Elements/u/P60566> ;
    reg:lexicalAlias "http://rdaregistry.info/Elements/e/aspectRatio"@en ;
    reg:name "aspectRatio"@en ;
    reg:status <http://metadataregistry.org/uri/RegStatus/1001> ;
    rdfs:domain <http://rdaregistry.info/Elements/c/C10006> ;
    rdfs:isDefinedBy <http://rdaregistry.info/Elements/e/> ;
    skos:definition "Relates an expression to the ratio of the width to the height of a moving image."@en .

<http://rdaregistry.info/Elements/e/P20231> a rdf:Property ;
    rdfs:label "has work expressed"@en ;
    reg:lexicalAlias "http://rdaregistry.info/Elements/e/workExpressed"@en ;
    reg:name "workExpressed"@en ;
    reg:status <http://metadataregistry.org/uri/RegStatus/1001> ;
    rdfs:domain <http://rdaregistry.info/Elements/c/C10006> ;
    rdfs:isDefinedBy <http://rdaregistry.info/Elements/e/> ;
    rdfs:range <http://rdaregistry.info/Elements/c/C10001> ;
    owl:inverseOf <http://rdaregistry.info/Elements/w/P10078> ;
    skos:definition "Relates an expression to the work realized through an expression."@en .

<http://rdaregistry.info/Elements/e/P20237> a rdf:Property ;
    rdfs:label "has writer of afterword"@en ;
    reg:hasUnconstrained <http://rdaregistry.info/Elements/u/P60715> ;
    reg:lexicalAlias "http://rdaregistry.info/Elements/e/writerOfAfterword"@en ;
    reg:name "writerOfAfterword"@en ;
    reg:status <http://metadataregistry.org/uri/RegStatus/1001> ;
    rdfs:domain <http://rdaregistry.info/Elements/c/C10006> ;
    rdfs:isDefinedBy <http://rdaregistry.info/Elements/e/> ;
    rdfs:range <http://rdaregistry.info/Elements/c/C10002> ;
    rdfs:subPropertyOf <http://rdaregistry.info/Elements/e/P20046>,
        <http://rdaregistry.info/Elements/u/P60715> ;
    owl:inverseOf <http://rdaregistry.info/Elements/a/P50227> ;
    skos:definition "Relates an expression to a person, family, or corporate body contributing to an expression of a work by providing an afterword to the original work."@en .

<http://rdaregistry.info/Elements/e/P20238> a rdf:Property ;
    rdfs:label "has writer of postface"@en ;
    reg:hasUnconstrained <http://rdaregistry.info/Elements/u/P60716> ;
    reg:lexicalAlias "http://rdaregistry.info/Elements/e/writerOfPostface"@en ;
    reg:name "writerOfPostface"@en ;
    reg:status <http://metadataregistry.org/uri/RegStatus/1001> ;
    rdfs:domain <http://rdaregistry.info/Elements/c/C10006> ;
    rdfs:isDefinedBy <http://rdaregistry.info/Elements/e/> ;
    rdfs:range <http://rdaregistry.info/Elements/c/C10002> ;
    rdfs:subPropertyOf <http://rdaregistry.info/Elements/e/P20046>,
        <http://rdaregistry.info/Elements/u/P60716> ;
    owl:inverseOf <http://rdaregistry.info/Elements/a/P50228> ;
    skos:definition "Relates an expression to a person, family, or corporate body contributing to an expression of a work by providing a postface to the original work."@en .

<http://rdaregistry.info/Elements/e/P20260> a rdf:Property ;
    rdfs:label "has details of aspect ratio"@en ;
    reg:hasUnconstrained <http://rdaregistry.info/Elements/u/P60760> ;
    reg:lexicalAlias "http://rdaregistry.info/Elements/e/detailsOfAspectRatio"@en ;
    reg:name "detailsOfAspectRatio"@en ;
    reg:status <http://metadataregistry.org/uri/RegStatus/1001> ;
    rdfs:domain <http://rdaregistry.info/Elements/c/C10006> ;
    rdfs:isDefinedBy <http://rdaregistry.info/Elements/e/> ;
    skos:definition "Relates an expression to details of the ratio of the width to the height of a moving image."@en .

<http://rdaregistry.info/Elements/e/P20261> a rdf:Property ;
    rdfs:label "has details of colour content"@en ;
    reg:hasUnconstrained <http://rdaregistry.info/Elements/u/P60761> ;
    reg:lexicalAlias "http://rdaregistry.info/Elements/e/detailsOfColourContent"@en ;
    reg:name "detailsOfColourContent"@en ;
    reg:status <http://metadataregistry.org/uri/RegStatus/1001> ;
    rdfs:domain <http://rdaregistry.info/Elements/c/C10006> ;
    rdfs:isDefinedBy <http://rdaregistry.info/Elements/e/> ;
    skos:definition "Relates an expression to details of the presence of colour, tone, etc., in the content of a resource, and the specific colours, tones, etc., (including black and white) present."@en .

<http://rdaregistry.info/Elements/e/P20262> a rdf:Property ;
    rdfs:label "has details of form of musical notation"@en ;
    reg:hasUnconstrained <http://rdaregistry.info/Elements/u/P60762> ;
    reg:lexicalAlias "http://rdaregistry.info/Elements/e/detailsOfFormOfMusicalNotation"@en ;
    reg:name "detailsOfFormOfMusicalNotation"@en ;
    reg:status <http://metadataregistry.org/uri/RegStatus/1001> ;
    rdfs:domain <http://rdaregistry.info/Elements/c/C10006> ;
    rdfs:isDefinedBy <http://rdaregistry.info/Elements/e/> ;
    skos:definition "Relates an expression to details of the set of characters and/or symbols used to express the musical content of a resource."@en .

<http://rdaregistry.info/Elements/e/P20263> a rdf:Property ;
    rdfs:label "has details of form of notated movement"@en ;
    reg:hasUnconstrained <http://rdaregistry.info/Elements/u/P60763> ;
    reg:lexicalAlias "http://rdaregistry.info/Elements/e/detailsOfFormOfNotatedMovement"@en ;
    reg:name "detailsOfFormOfNotatedMovement"@en ;
    reg:status <http://metadataregistry.org/uri/RegStatus/1001> ;
    rdfs:domain <http://rdaregistry.info/Elements/c/C10006> ;
    rdfs:isDefinedBy <http://rdaregistry.info/Elements/e/> ;
    skos:definition "Relates an expression to details of the set of characters and/or symbols used to express the movement content of a resource."@en .

<http://rdaregistry.info/Elements/e/P20264> a rdf:Property ;
    rdfs:label "has details of format of notated music"@en ;
    reg:hasUnconstrained <http://rdaregistry.info/Elements/u/P60764> ;
    reg:lexicalAlias "http://rdaregistry.info/Elements/e/detailsOfFormatOfNotatedMusic"@en ;
    reg:name "detailsOfFormatOfNotatedMusic"@en ;
    reg:status <http://metadataregistry.org/uri/RegStatus/1001> ;
    rdfs:domain <http://rdaregistry.info/Elements/c/C10006> ;
    rdfs:isDefinedBy <http://rdaregistry.info/Elements/e/> ;
    skos:definition "Relates an expression to details of the musical or physical layout of the content of a resource that is presented in the form of musical notation."@en .

<http://rdaregistry.info/Elements/e/P20265> a rdf:Property ;
    rdfs:label "has details of form of tactile notation"@en ;
    reg:hasUnconstrained <http://rdaregistry.info/Elements/u/P60765> ;
    reg:lexicalAlias "http://rdaregistry.info/Elements/e/detailsOfFormOfTactileNotation"@en ;
    reg:name "detailsOfFormOfTactileNotation"@en ;
    reg:status <http://metadataregistry.org/uri/RegStatus/1001> ;
    rdfs:domain <http://rdaregistry.info/Elements/c/C10006> ;
    rdfs:isDefinedBy <http://rdaregistry.info/Elements/e/> ;
    skos:definition "Relates an expression to details of the set of characters and/or symbols used to express the content of a resource in a form that can be perceived through touch."@en .

<http://rdaregistry.info/Elements/e/P20266> a rdf:Property ;
    rdfs:label "has details of script"@en ;
    reg:hasUnconstrained <http://rdaregistry.info/Elements/u/P60766> ;
    reg:lexicalAlias "http://rdaregistry.info/Elements/e/detailsOfScript"@en ;
    reg:name "detailsOfScript"@en ;
    reg:status <http://metadataregistry.org/uri/RegStatus/1001> ;
    rdfs:domain <http://rdaregistry.info/Elements/c/C10006> ;
    rdfs:isDefinedBy <http://rdaregistry.info/Elements/e/> ;
    skos:definition "Relates an expression to details of the set of characters and/or symbols used to express the written language content of a resource."@en .

<http://rdaregistry.info/Elements/e/P20267> a rdf:Property ;
    rdfs:label "has details of illustrative content"@en ;
    reg:hasUnconstrained <http://rdaregistry.info/Elements/u/P60804> ;
    reg:lexicalAlias "http://rdaregistry.info/Elements/e/detailsOfIllustrativeContent"@en ;
    reg:name "detailsOfIllustrativeContent"@en ;
    reg:status <http://metadataregistry.org/uri/RegStatus/1001> ;
    rdfs:domain <http://rdaregistry.info/Elements/c/C10006> ;
    rdfs:isDefinedBy <http://rdaregistry.info/Elements/e/> ;
    skos:definition "Relates an expression to details of content intended to illustrate the primary content of a resource."@en .

<http://rdaregistry.info/Elements/e/P20010> a rdf:Property ;
    rdfs:label "has note on changes in content characteristics"@en ;
    reg:hasUnconstrained <http://rdaregistry.info/Elements/u/P60123> ;
    reg:lexicalAlias "http://rdaregistry.info/Elements/e/noteOnChangesInContentCharacteristics"@en ;
    reg:name "noteOnChangesInContentCharacteristics"@en ;
    reg:status <http://metadataregistry.org/uri/RegStatus/1001> ;
    rdfs:domain <http://rdaregistry.info/Elements/c/C10006> ;
    rdfs:isDefinedBy <http://rdaregistry.info/Elements/e/> ;
    rdfs:subPropertyOf <http://rdaregistry.info/Elements/e/P20071>,
        <http://rdaregistry.info/Elements/u/P60123> ;
    skos:definition "Relates an expression to a note on changes in content characteristics that occur in subsequent issues or parts of a resource issued in successive parts or between iterations of an integrating resource."@en .

<http://rdaregistry.info/Elements/e/P20011> a rdf:Property ;
    rdfs:label "has conductor"@en ;
    reg:hasUnconstrained <http://rdaregistry.info/Elements/u/P60141> ;
    reg:lexicalAlias "http://rdaregistry.info/Elements/e/conductor"@en ;
    reg:name "conductor"@en ;
    reg:status <http://metadataregistry.org/uri/RegStatus/1001> ;
    rdfs:domain <http://rdaregistry.info/Elements/c/C10006> ;
    rdfs:isDefinedBy <http://rdaregistry.info/Elements/e/> ;
    rdfs:range <http://rdaregistry.info/Elements/c/C10002> ;
    rdfs:subPropertyOf <http://rdaregistry.info/Elements/e/P20039>,
        <http://rdaregistry.info/Elements/u/P60141> ;
    owl:inverseOf <http://rdaregistry.info/Elements/a/P50070> ;
    skos:definition "Relates an expression to a performer contributing to an expression of a musical work by leading a performing group (orchestra, chorus, opera, etc.) in a musical or dramatic presentation, etc."@en .

<http://rdaregistry.info/Elements/e/P20013> a rdf:Property ;
    rdfs:label "has on-screen presenter"@en ;
    reg:hasUnconstrained <http://rdaregistry.info/Elements/u/P60143> ;
    reg:lexicalAlias "http://rdaregistry.info/Elements/e/onScreenPresenter"@en ;
    reg:name "onScreenPresenter"@en ;
    reg:status <http://metadataregistry.org/uri/RegStatus/1001> ;
    rdfs:domain <http://rdaregistry.info/Elements/c/C10006> ;
    rdfs:isDefinedBy <http://rdaregistry.info/Elements/e/> ;
    rdfs:range <http://rdaregistry.info/Elements/c/C10002> ;
    rdfs:subPropertyOf <http://rdaregistry.info/Elements/e/P20039>,
        <http://rdaregistry.info/Elements/u/P60143> ;
    owl:inverseOf <http://rdaregistry.info/Elements/a/P50072> ;
    skos:definition "Relates an expression to a performer contributing to an expression of a work by appearing on screen to provide contextual or background information."@en ;
    skos:scopeNote "An on-screen presenter may appear in nonfiction moving image materials or in introductions to fiction moving image materials."@en .

<http://rdaregistry.info/Elements/e/P20014> a rdf:Property ;
    rdfs:label "has dancer"@en ;
    reg:hasUnconstrained <http://rdaregistry.info/Elements/u/P60144> ;
    reg:lexicalAlias "http://rdaregistry.info/Elements/e/dancer"@en ;
    reg:name "dancer"@en ;
    reg:status <http://metadataregistry.org/uri/RegStatus/1001> ;
    rdfs:domain <http://rdaregistry.info/Elements/c/C10006> ;
    rdfs:isDefinedBy <http://rdaregistry.info/Elements/e/> ;
    rdfs:range <http://rdaregistry.info/Elements/c/C10002> ;
    rdfs:subPropertyOf <http://rdaregistry.info/Elements/e/P20039>,
        <http://rdaregistry.info/Elements/u/P60144> ;
    owl:inverseOf <http://rdaregistry.info/Elements/a/P50073> ;
    skos:definition "Relates an expression to a performer contributing to an expression of a work by dancing in a musical, dramatic, etc., presentation."@en .

<http://rdaregistry.info/Elements/e/P20015> a rdf:Property ;
    rdfs:label "has teacher "@en ;
    reg:hasUnconstrained <http://rdaregistry.info/Elements/u/P60145> ;
    reg:lexicalAlias "http://rdaregistry.info/Elements/e/teacher"@en ;
    reg:name "teacher"@en ;
    reg:status <http://metadataregistry.org/uri/RegStatus/1001> ;
    rdfs:domain <http://rdaregistry.info/Elements/c/C10006> ;
    rdfs:isDefinedBy <http://rdaregistry.info/Elements/e/> ;
    rdfs:range <http://rdaregistry.info/Elements/c/C10002> ;
    rdfs:subPropertyOf <http://rdaregistry.info/Elements/e/P20039>,
        <http://rdaregistry.info/Elements/u/P60145> ;
    owl:inverseOf <http://rdaregistry.info/Elements/a/P50074> ;
    skos:definition "Relates an expression to a performer contributing to an expression of a work by giving instruction or providing a demonstration."@en .

<http://rdaregistry.info/Elements/e/P20016> a rdf:Property ;
    rdfs:label "has host "@en ;
    reg:hasUnconstrained <http://rdaregistry.info/Elements/u/P60146> ;
    reg:lexicalAlias "http://rdaregistry.info/Elements/e/host"@en ;
    reg:name "host"@en ;
    reg:status <http://metadataregistry.org/uri/RegStatus/1001> ;
    rdfs:domain <http://rdaregistry.info/Elements/c/C10006> ;
    rdfs:isDefinedBy <http://rdaregistry.info/Elements/e/> ;
    rdfs:range <http://rdaregistry.info/Elements/c/C10002> ;
    rdfs:subPropertyOf <http://rdaregistry.info/Elements/e/P20039>,
        <http://rdaregistry.info/Elements/u/P60146> ;
    owl:inverseOf <http://rdaregistry.info/Elements/a/P50075> ;
    skos:definition "Relates an expression to a performer contributing to an expression of a work by leading a program (often broadcast) that includes other guests, performers, etc. (e.g., talk show host)."@en .

<http://rdaregistry.info/Elements/e/P20017> a rdf:Property ;
    rdfs:label "has moderator"@en ;
    reg:hasUnconstrained <http://rdaregistry.info/Elements/u/P60147> ;
    reg:lexicalAlias "http://rdaregistry.info/Elements/e/moderator"@en ;
    reg:name "moderator"@en ;
    reg:status <http://metadataregistry.org/uri/RegStatus/1001> ;
    rdfs:domain <http://rdaregistry.info/Elements/c/C10006> ;
    rdfs:isDefinedBy <http://rdaregistry.info/Elements/e/> ;
    rdfs:range <http://rdaregistry.info/Elements/c/C10002> ;
    rdfs:subPropertyOf <http://rdaregistry.info/Elements/e/P20039>,
        <http://rdaregistry.info/Elements/u/P60147> ;
    owl:inverseOf <http://rdaregistry.info/Elements/a/P50076> ;
    skos:definition "Relates an expression to a performer contributing to an expression of a work by leading a program (often broadcast) where topics are discussed, usually with participation of experts in fields related to the discussion."@en .

<http://rdaregistry.info/Elements/e/P20018> a rdf:Property ;
    rdfs:label "has puppeteer "@en ;
    reg:hasUnconstrained <http://rdaregistry.info/Elements/u/P60148> ;
    reg:lexicalAlias "http://rdaregistry.info/Elements/e/puppeteer"@en ;
    reg:name "puppeteer"@en ;
    reg:status <http://metadataregistry.org/uri/RegStatus/1001> ;
    rdfs:domain <http://rdaregistry.info/Elements/c/C10006> ;
    rdfs:isDefinedBy <http://rdaregistry.info/Elements/e/> ;
    rdfs:range <http://rdaregistry.info/Elements/c/C10002> ;
    rdfs:subPropertyOf <http://rdaregistry.info/Elements/e/P20039>,
        <http://rdaregistry.info/Elements/u/P60148> ;
    owl:inverseOf <http://rdaregistry.info/Elements/a/P50077> ;
    skos:definition "Relates an expression to a performer contributing to an expression of a work by manipulating, controlling, or directing puppets or marionettes in a moving image production or a musical or dramatic presentation or entertainment."@en .

<http://rdaregistry.info/Elements/e/P20019> a rdf:Property ;
    rdfs:label "has panelist"@en ;
    reg:hasUnconstrained <http://rdaregistry.info/Elements/u/P60149> ;
    reg:lexicalAlias "http://rdaregistry.info/Elements/e/panelist"@en ;
    reg:name "panelist"@en ;
    reg:status <http://metadataregistry.org/uri/RegStatus/1001> ;
    rdfs:domain <http://rdaregistry.info/Elements/c/C10006> ;
    rdfs:isDefinedBy <http://rdaregistry.info/Elements/e/> ;
    rdfs:range <http://rdaregistry.info/Elements/c/C10002> ;
    rdfs:subPropertyOf <http://rdaregistry.info/Elements/e/P20039>,
        <http://rdaregistry.info/Elements/u/P60149> ;
    owl:inverseOf <http://rdaregistry.info/Elements/a/P50078> ;
    skos:definition "Relates an expression to a performer contributing to an expression of a work by participating in a program (often broadcast) where topics are discussed, usually with participation of experts in fields related to the discussion."@en .

<http://rdaregistry.info/Elements/e/P20020> a rdf:Property ;
    rdfs:label "has instrumentalist"@en ;
    reg:hasUnconstrained <http://rdaregistry.info/Elements/u/P60150> ;
    reg:lexicalAlias "http://rdaregistry.info/Elements/e/instrumentalist"@en ;
    reg:name "instrumentalist"@en ;
    reg:status <http://metadataregistry.org/uri/RegStatus/1001> ;
    rdfs:domain <http://rdaregistry.info/Elements/c/C10006> ;
    rdfs:isDefinedBy <http://rdaregistry.info/Elements/e/> ;
    rdfs:range <http://rdaregistry.info/Elements/c/C10002> ;
    rdfs:subPropertyOf <http://rdaregistry.info/Elements/e/P20039>,
        <http://rdaregistry.info/Elements/u/P60150> ;
    owl:inverseOf <http://rdaregistry.info/Elements/a/P50079> ;
    skos:definition "Relates an expression to a performer contributing to an expression of a work by playing a musical instrument."@en .

<http://rdaregistry.info/Elements/e/P20021> a rdf:Property ;
    rdfs:label "has commentator"@en ;
    reg:hasUnconstrained <http://rdaregistry.info/Elements/u/P60151> ;
    reg:lexicalAlias "http://rdaregistry.info/Elements/e/commentator"@en ;
    reg:name "commentator"@en ;
    reg:status <http://metadataregistry.org/uri/RegStatus/1001> ;
    rdfs:domain <http://rdaregistry.info/Elements/c/C10006> ;
    rdfs:isDefinedBy <http://rdaregistry.info/Elements/e/> ;
    rdfs:range <http://rdaregistry.info/Elements/c/C10002> ;
    rdfs:subPropertyOf <http://rdaregistry.info/Elements/e/P20039>,
        <http://rdaregistry.info/Elements/u/P60151> ;
    owl:inverseOf <http://rdaregistry.info/Elements/a/P50080> ;
    skos:definition "Relates an expression to a performer contributing to an expression of a work by providing interpretation, analysis, or a discussion of the subject matter on a recording, film, or other audiovisual medium."@en .

<http://rdaregistry.info/Elements/e/P20022> a rdf:Property ;
    rdfs:label "has narrator "@en ;
    reg:hasUnconstrained <http://rdaregistry.info/Elements/u/P60153> ;
    reg:lexicalAlias "http://rdaregistry.info/Elements/e/narrator"@en ;
    reg:name "narrator"@en ;
    reg:status <http://metadataregistry.org/uri/RegStatus/1001> ;
    rdfs:domain <http://rdaregistry.info/Elements/c/C10006> ;
    rdfs:isDefinedBy <http://rdaregistry.info/Elements/e/> ;
    rdfs:range <http://rdaregistry.info/Elements/c/C10002> ;
    rdfs:subPropertyOf <http://rdaregistry.info/Elements/e/P20039>,
        <http://rdaregistry.info/Elements/u/P60153> ;
    owl:inverseOf <http://rdaregistry.info/Elements/a/P50081> ;
    skos:definition "Relates an expression to a performer contributing to an expression of a work by reading aloud or giving an account of an act, occurrence, course of events, etc."@en .

<http://rdaregistry.info/Elements/e/P20023> a rdf:Property ;
    rdfs:label "has storyteller"@en ;
    reg:hasUnconstrained <http://rdaregistry.info/Elements/u/P60154> ;
    reg:lexicalAlias "http://rdaregistry.info/Elements/e/storyteller"@en ;
    reg:name "storyteller"@en ;
    reg:status <http://metadataregistry.org/uri/RegStatus/1001> ;
    rdfs:domain <http://rdaregistry.info/Elements/c/C10006> ;
    rdfs:isDefinedBy <http://rdaregistry.info/Elements/e/> ;
    rdfs:range <http://rdaregistry.info/Elements/c/C10002> ;
    rdfs:subPropertyOf <http://rdaregistry.info/Elements/e/P20039>,
        <http://rdaregistry.info/Elements/u/P60154> ;
    owl:inverseOf <http://rdaregistry.info/Elements/a/P50082> ;
    skos:definition "Relates an expression to a performer contributing to an expression of a work by relaying a creator’s original story with dramatic or theatrical interpretation."@en .

<http://rdaregistry.info/Elements/e/P20024> a rdf:Property ;
    rdfs:label "has speaker"@en ;
    reg:hasUnconstrained <http://rdaregistry.info/Elements/u/P60155> ;
    reg:lexicalAlias "http://rdaregistry.info/Elements/e/speaker"@en ;
    reg:name "speaker"@en ;
    reg:status <http://metadataregistry.org/uri/RegStatus/1001> ;
    rdfs:domain <http://rdaregistry.info/Elements/c/C10006> ;
    rdfs:isDefinedBy <http://rdaregistry.info/Elements/e/> ;
    rdfs:range <http://rdaregistry.info/Elements/c/C10002> ;
    rdfs:subPropertyOf <http://rdaregistry.info/Elements/e/P20039>,
        <http://rdaregistry.info/Elements/u/P60155> ;
    owl:inverseOf <http://rdaregistry.info/Elements/a/P50083> ;
    skos:definition "Relates an expression to a performer contributing to an expression of a work by speaking words, such as a lecture, speech, etc."@en .

<http://rdaregistry.info/Elements/e/P20025> a rdf:Property ;
    rdfs:label "has singer "@en ;
    reg:hasUnconstrained <http://rdaregistry.info/Elements/u/P60156> ;
    reg:lexicalAlias "http://rdaregistry.info/Elements/e/singer"@en ;
    reg:name "singer"@en ;
    reg:status <http://metadataregistry.org/uri/RegStatus/1001> ;
    rdfs:domain <http://rdaregistry.info/Elements/c/C10006> ;
    rdfs:isDefinedBy <http://rdaregistry.info/Elements/e/> ;
    rdfs:range <http://rdaregistry.info/Elements/c/C10002> ;
    rdfs:subPropertyOf <http://rdaregistry.info/Elements/e/P20039>,
        <http://rdaregistry.info/Elements/u/P60156> ;
    owl:inverseOf <http://rdaregistry.info/Elements/a/P50084> ;
    skos:definition "Relates an expression to a performer contributing to an expression of a work by using his/her/their voice, with or without instrumental accompaniment, to produce music."@en ;
    skos:scopeNote "A singer’s performance may or may not include actual words."@en .

<http://rdaregistry.info/Elements/e/P20026> a rdf:Property ;
    rdfs:label "has composer (expression) "@en ;
    reg:hasUnconstrained <http://rdaregistry.info/Elements/u/P60426> ;
    reg:lexicalAlias "http://rdaregistry.info/Elements/e/composerExpression"@en ;
    reg:name "composerExpression"@en ;
    reg:status <http://metadataregistry.org/uri/RegStatus/1001> ;
    rdfs:domain <http://rdaregistry.info/Elements/c/C10006> ;
    rdfs:isDefinedBy <http://rdaregistry.info/Elements/e/> ;
    rdfs:range <http://rdaregistry.info/Elements/c/C10002> ;
    rdfs:subPropertyOf <http://rdaregistry.info/Elements/e/P20053>,
        <http://rdaregistry.info/Elements/u/P60426> ;
    owl:inverseOf <http://rdaregistry.info/Elements/a/P50134> ;
    skos:definition "Relates an expression to a person, family, or corporate body contributing to an expression by adding music to a work that originally lacked it, by composing new music to substitute for the original music, or by composing new music to supplement the existing music."@en .

<http://rdaregistry.info/Elements/e/P20027> a rdf:Property ;
    rdfs:label "has surveyor"@en ;
    reg:hasUnconstrained <http://rdaregistry.info/Elements/u/P60377> ;
    reg:lexicalAlias "http://rdaregistry.info/Elements/e/surveyor"@en ;
    reg:name "surveyor"@en ;
    reg:status <http://metadataregistry.org/uri/RegStatus/1001> ;
    rdfs:domain <http://rdaregistry.info/Elements/c/C10006> ;
    rdfs:isDefinedBy <http://rdaregistry.info/Elements/e/> ;
    rdfs:range <http://rdaregistry.info/Elements/c/C10002> ;
    rdfs:subPropertyOf <http://rdaregistry.info/Elements/e/P20053>,
        <http://rdaregistry.info/Elements/u/P60377> ;
    owl:inverseOf <http://rdaregistry.info/Elements/a/P50135> ;
    skos:definition "Relates an expression to a person, family, or corporate body contributing to an expression of a cartographic work by providing measurements or dimensional relationships for the geographic area represented."@en .

<http://rdaregistry.info/Elements/e/P20028> a rdf:Property ;
    rdfs:label "has animator"@en ;
    reg:hasUnconstrained <http://rdaregistry.info/Elements/u/P60378> ;
    reg:lexicalAlias "http://rdaregistry.info/Elements/e/animator"@en ;
    reg:name "animator"@en ;
    reg:status <http://metadataregistry.org/uri/RegStatus/1001> ;
    rdfs:domain <http://rdaregistry.info/Elements/c/C10006> ;
    rdfs:isDefinedBy <http://rdaregistry.info/Elements/e/> ;
    rdfs:range <http://rdaregistry.info/Elements/c/C10002> ;
    rdfs:subPropertyOf <http://rdaregistry.info/Elements/e/P20053>,
        <http://rdaregistry.info/Elements/u/P60378> ;
    owl:inverseOf <http://rdaregistry.info/Elements/a/P50136> ;
    skos:definition "Relates an expression to a person, family, or corporate body contributing to an expression of a moving image work or computer program by giving apparent movement to inanimate objects or drawings."@en .

<http://rdaregistry.info/Elements/e/P20029> a rdf:Property ;
    rdfs:label "has arranger of music "@en ;
    reg:hasUnconstrained <http://rdaregistry.info/Elements/u/P60379> ;
    reg:lexicalAlias "http://rdaregistry.info/Elements/e/arrangerOfMusic"@en ;
    reg:name "arrangerOfMusic"@en ;
    reg:status <http://metadataregistry.org/uri/RegStatus/1001> ;
    rdfs:domain <http://rdaregistry.info/Elements/c/C10006> ;
    rdfs:isDefinedBy <http://rdaregistry.info/Elements/e/> ;
    rdfs:range <http://rdaregistry.info/Elements/c/C10002> ;
    rdfs:subPropertyOf <http://rdaregistry.info/Elements/e/P20053>,
        <http://rdaregistry.info/Elements/u/P60379> ;
    owl:inverseOf <http://rdaregistry.info/Elements/a/P50137> ;
    skos:definition "Relates an expression to a person, family, or corporate body contributing to an expression of a musical work by rewriting the composition for a medium of performance different from that for which the work was originally intended."@en ;
    skos:scopeNote "An arranger of music may also modify the work for the same medium of performance, etc., keeping the musical substance of the original composition essentially unchanged."@en .

<http://rdaregistry.info/Elements/e/P20031> a rdf:Property ;
    rdfs:label "has stage director"@en ;
    reg:hasUnconstrained <http://rdaregistry.info/Elements/u/P60399> ;
    reg:lexicalAlias "http://rdaregistry.info/Elements/e/stageDirector"@en ;
    reg:name "stageDirector"@en ;
    reg:status <http://metadataregistry.org/uri/RegStatus/1001> ;
    rdfs:domain <http://rdaregistry.info/Elements/c/C10006> ;
    rdfs:isDefinedBy <http://rdaregistry.info/Elements/e/> ;
    rdfs:range <http://rdaregistry.info/Elements/c/C10002> ;
    rdfs:subPropertyOf <http://rdaregistry.info/Elements/e/P20053>,
        <http://rdaregistry.info/Elements/u/P60399> ;
    owl:inverseOf <http://rdaregistry.info/Elements/a/P50139> ;
    skos:definition "Relates an expression to a person, family, or corporate body contributing to an expression of a stage work through the general management and supervision of a performance."@en .

<http://rdaregistry.info/Elements/e/P20032> a rdf:Property ;
    rdfs:label "has interviewer (expression) "@en ;
    reg:hasUnconstrained <http://rdaregistry.info/Elements/u/P60430> ;
    reg:lexicalAlias "http://rdaregistry.info/Elements/e/interviewerExpression"@en ;
    reg:name "interviewerExpression"@en ;
    reg:status <http://metadataregistry.org/uri/RegStatus/1001> ;
    rdfs:domain <http://rdaregistry.info/Elements/c/C10006> ;
    rdfs:isDefinedBy <http://rdaregistry.info/Elements/e/> ;
    rdfs:range <http://rdaregistry.info/Elements/c/C10002> ;
    rdfs:subPropertyOf <http://rdaregistry.info/Elements/e/P20053>,
        <http://rdaregistry.info/Elements/u/P60430> ;
    owl:inverseOf <http://rdaregistry.info/Elements/a/P50140> ;
    skos:definition "Relates an expression to a person, family, or corporate body contributing to an expression of a work by acting as an interviewer, reporter, pollster, or some other information gathering agent."@en .

<http://rdaregistry.info/Elements/e/P20033> a rdf:Property ;
    rdfs:label "has draftsman "@en ;
    reg:hasUnconstrained <http://rdaregistry.info/Elements/u/P60381> ;
    reg:lexicalAlias "http://rdaregistry.info/Elements/e/draftsman"@en ;
    reg:name "draftsman"@en ;
    reg:status <http://metadataregistry.org/uri/RegStatus/1001> ;
    rdfs:domain <http://rdaregistry.info/Elements/c/C10006> ;
    rdfs:isDefinedBy <http://rdaregistry.info/Elements/e/> ;
    rdfs:range <http://rdaregistry.info/Elements/c/C10002> ;
    rdfs:subPropertyOf <http://rdaregistry.info/Elements/e/P20053>,
        <http://rdaregistry.info/Elements/u/P60381> ;
    owl:inverseOf <http://rdaregistry.info/Elements/a/P50141> ;
    skos:definition "Relates an expression to a person, family, or corporate body contributing to an expression of a work by an architect, inventor, etc., by making detailed plans or drawings for buildings, ships, aircraft, machines, objects, etc."@en .

<http://rdaregistry.info/Elements/e/P20034> a rdf:Property ;
    rdfs:label "has transcriber "@en ;
    reg:hasUnconstrained <http://rdaregistry.info/Elements/u/P60382> ;
    reg:lexicalAlias "http://rdaregistry.info/Elements/e/transcriber"@en ;
    reg:name "transcriber"@en ;
    reg:status <http://metadataregistry.org/uri/RegStatus/1001> ;
    rdfs:domain <http://rdaregistry.info/Elements/c/C10006> ;
    rdfs:isDefinedBy <http://rdaregistry.info/Elements/e/> ;
    rdfs:range <http://rdaregistry.info/Elements/c/C10002> ;
    rdfs:subPropertyOf <http://rdaregistry.info/Elements/e/P20053>,
        <http://rdaregistry.info/Elements/u/P60382> ;
    owl:inverseOf <http://rdaregistry.info/Elements/a/P50142> ;
    skos:definition "Relates an expression to a person, family, or corporate body contributing to an expression of a work by writing down or notating previously unwritten or unnotated content, or by changing it from one system of notation to another."@en .

<http://rdaregistry.info/Elements/e/P20035> a rdf:Property ;
    rdfs:label "has musical director"@en ;
    reg:hasUnconstrained <http://rdaregistry.info/Elements/u/P60383> ;
    reg:lexicalAlias "http://rdaregistry.info/Elements/e/musicalDirector"@en ;
    reg:name "musicalDirector"@en ;
    reg:status <http://metadataregistry.org/uri/RegStatus/1001> ;
    rdfs:domain <http://rdaregistry.info/Elements/c/C10006> ;
    rdfs:isDefinedBy <http://rdaregistry.info/Elements/e/> ;
    rdfs:range <http://rdaregistry.info/Elements/c/C10002> ;
    rdfs:subPropertyOf <http://rdaregistry.info/Elements/e/P20053>,
        <http://rdaregistry.info/Elements/u/P60383> ;
    owl:inverseOf <http://rdaregistry.info/Elements/a/P50143> ;
    skos:definition "Relates an expression to a person, family, or corporate body contributing to an expression of a work by coordinating the activities of the composer, the sound editor, and sound mixers for a moving image production or for a musical or dramatic presentation or entertainment."@en .

<http://rdaregistry.info/Elements/e/P20036> a rdf:Property ;
    rdfs:label "has costume designer"@en ;
    reg:hasUnconstrained <http://rdaregistry.info/Elements/u/P60384> ;
    reg:lexicalAlias "http://rdaregistry.info/Elements/e/costumeDesigner"@en ;
    reg:name "costumeDesigner"@en ;
    reg:status <http://metadataregistry.org/uri/RegStatus/1001> ;
    rdfs:domain <http://rdaregistry.info/Elements/c/C10006> ;
    rdfs:isDefinedBy <http://rdaregistry.info/Elements/e/> ;
    rdfs:range <http://rdaregistry.info/Elements/c/C10002> ;
    rdfs:subPropertyOf <http://rdaregistry.info/Elements/e/P20053>,
        <http://rdaregistry.info/Elements/u/P60384> ;
    owl:inverseOf <http://rdaregistry.info/Elements/a/P50144> ;
    skos:definition "Relates an expression to a person, family, or corporate body contributing to an expression of a work by designing the costumes for a moving image production or for a musical or dramatic presentation or entertainment."@en .

<http://rdaregistry.info/Elements/e/P20037> a rdf:Property ;
    rdfs:label "has translator"@en ;
    reg:hasUnconstrained <http://rdaregistry.info/Elements/u/P60385> ;
    reg:lexicalAlias "http://rdaregistry.info/Elements/e/translator"@en ;
    reg:name "translator"@en ;
    reg:status <http://metadataregistry.org/uri/RegStatus/1001> ;
    rdfs:domain <http://rdaregistry.info/Elements/c/C10006> ;
    rdfs:isDefinedBy <http://rdaregistry.info/Elements/e/> ;
    rdfs:range <http://rdaregistry.info/Elements/c/C10002> ;
    rdfs:subPropertyOf <http://rdaregistry.info/Elements/e/P20053>,
        <http://rdaregistry.info/Elements/u/P60385> ;
    owl:inverseOf <http://rdaregistry.info/Elements/a/P50145> ;
    skos:definition "Relates an expression to a person, family, or corporate body contributing to an expression of a work by expressing the linguistic content of the work in a language different from that of previous expressions of the original work."@en ;
    skos:scopeNote "A translator may also translate linguistic content between forms of the same language from different time periods."@en .

<http://rdaregistry.info/Elements/e/P20038> a rdf:Property ;
    rdfs:label "has art director"@en ;
    reg:hasUnconstrained <http://rdaregistry.info/Elements/u/P60386> ;
    reg:lexicalAlias "http://rdaregistry.info/Elements/e/artDirector"@en ;
    reg:name "artDirector"@en ;
    reg:status <http://metadataregistry.org/uri/RegStatus/1001> ;
    rdfs:domain <http://rdaregistry.info/Elements/c/C10006> ;
    rdfs:isDefinedBy <http://rdaregistry.info/Elements/e/> ;
    rdfs:range <http://rdaregistry.info/Elements/c/C10002> ;
    rdfs:subPropertyOf <http://rdaregistry.info/Elements/e/P20053>,
        <http://rdaregistry.info/Elements/u/P60386> ;
    owl:inverseOf <http://rdaregistry.info/Elements/a/P50146> ;
    skos:definition "Relates an expression to a person, family, or corporate body contributing to an expression of a work by overseeing the artists and craftspeople who build the sets for moving image productions."@en .

<http://rdaregistry.info/Elements/e/P20041> a rdf:Property ;
    rdfs:label "has writer of preface"@en ;
    reg:hasUnconstrained <http://rdaregistry.info/Elements/u/P60389> ;
    reg:lexicalAlias "http://rdaregistry.info/Elements/e/writerOfPreface"@en ;
    reg:name "writerOfPreface"@en ;
    reg:status <http://metadataregistry.org/uri/RegStatus/1001> ;
    rdfs:domain <http://rdaregistry.info/Elements/c/C10006> ;
    rdfs:isDefinedBy <http://rdaregistry.info/Elements/e/> ;
    rdfs:range <http://rdaregistry.info/Elements/c/C10002> ;
    rdfs:subPropertyOf <http://rdaregistry.info/Elements/e/P20046>,
        <http://rdaregistry.info/Elements/u/P60389> ;
    owl:inverseOf <http://rdaregistry.info/Elements/a/P50149> ;
    skos:definition "Relates an expression to a person, family, or corporate body contributing to an expression of a work by providing a preface to the original work."@en .

<http://rdaregistry.info/Elements/e/P20042> a rdf:Property ;
    rdfs:label "has cartographer (expression)"@en ;
    reg:hasUnconstrained <http://rdaregistry.info/Elements/u/P60425> ;
    reg:lexicalAlias "http://rdaregistry.info/Elements/e/cartographerExpression"@en ;
    reg:name "cartographerExpression"@en ;
    reg:status <http://metadataregistry.org/uri/RegStatus/1001> ;
    rdfs:domain <http://rdaregistry.info/Elements/c/C10006> ;
    rdfs:isDefinedBy <http://rdaregistry.info/Elements/e/> ;
    rdfs:range <http://rdaregistry.info/Elements/c/C10002> ;
    rdfs:subPropertyOf <http://rdaregistry.info/Elements/e/P20053>,
        <http://rdaregistry.info/Elements/u/P60425> ;
    owl:inverseOf <http://rdaregistry.info/Elements/a/P50150> ;
    skos:definition "Relates an expression to a person, family, or corporate body contributing to an expression of a work by providing additional cartography, or by modifying the previous cartography."@en .

<http://rdaregistry.info/Elements/e/P20043> a rdf:Property ;
    rdfs:label "has choreographer (expression)"@en ;
    reg:hasUnconstrained <http://rdaregistry.info/Elements/u/P60433> ;
    reg:lexicalAlias "http://rdaregistry.info/Elements/e/choreographerExpression"@en ;
    reg:name "choreographerExpression"@en ;
    reg:status <http://metadataregistry.org/uri/RegStatus/1001> ;
    rdfs:domain <http://rdaregistry.info/Elements/c/C10006> ;
    rdfs:isDefinedBy <http://rdaregistry.info/Elements/e/> ;
    rdfs:range <http://rdaregistry.info/Elements/c/C10002> ;
    rdfs:subPropertyOf <http://rdaregistry.info/Elements/e/P20053>,
        <http://rdaregistry.info/Elements/u/P60433> ;
    owl:inverseOf <http://rdaregistry.info/Elements/a/P50151> ;
    skos:definition "Relates an expression to a person, family, or corporate body contributing to an expression of a work by providing additional choreography, or by modifying the previous choreography."@en .

<http://rdaregistry.info/Elements/e/P20044> a rdf:Property ;
    rdfs:label "has writer of added commentary"@en ;
    reg:hasUnconstrained <http://rdaregistry.info/Elements/u/P60390> ;
    reg:lexicalAlias "http://rdaregistry.info/Elements/e/writerOfAddedCommentary"@en ;
    reg:name "writerOfAddedCommentary"@en ;
    reg:status <http://metadataregistry.org/uri/RegStatus/1001> ;
    rdfs:domain <http://rdaregistry.info/Elements/c/C10006> ;
    rdfs:isDefinedBy <http://rdaregistry.info/Elements/e/> ;
    rdfs:range <http://rdaregistry.info/Elements/c/C10002> ;
    rdfs:subPropertyOf <http://rdaregistry.info/Elements/e/P20046>,
        <http://rdaregistry.info/Elements/u/P60390> ;
    owl:inverseOf <http://rdaregistry.info/Elements/a/P50152> ;
    skos:definition "Relates an expression to a person, family, or corporate body contributing to an expression of a work by providing an interpretation or critical explanation of the original work."@en .

<http://rdaregistry.info/Elements/e/P20045> a rdf:Property ;
    rdfs:label "has writer of introduction"@en ;
    reg:hasUnconstrained <http://rdaregistry.info/Elements/u/P60391> ;
    reg:lexicalAlias "http://rdaregistry.info/Elements/e/writerOfIntroduction"@en ;
    reg:name "writerOfIntroduction"@en ;
    reg:status <http://metadataregistry.org/uri/RegStatus/1001> ;
    rdfs:domain <http://rdaregistry.info/Elements/c/C10006> ;
    rdfs:isDefinedBy <http://rdaregistry.info/Elements/e/> ;
    rdfs:range <http://rdaregistry.info/Elements/c/C10002> ;
    rdfs:subPropertyOf <http://rdaregistry.info/Elements/e/P20046>,
        <http://rdaregistry.info/Elements/u/P60391> ;
    owl:inverseOf <http://rdaregistry.info/Elements/a/P50153> ;
    skos:definition "Relates an expression to a person, family, or corporate body contributing to an expression of a work by providing an introduction to the original work."@en .

<http://rdaregistry.info/Elements/e/P20047> a rdf:Property ;
    rdfs:label "has interviewee (expression) "@en ;
    reg:hasUnconstrained <http://rdaregistry.info/Elements/u/P60432> ;
    reg:lexicalAlias "http://rdaregistry.info/Elements/e/intervieweeExpression"@en ;
    reg:name "intervieweeExpression"@en ;
    reg:status <http://metadataregistry.org/uri/RegStatus/1001> ;
    rdfs:domain <http://rdaregistry.info/Elements/c/C10006> ;
    rdfs:isDefinedBy <http://rdaregistry.info/Elements/e/> ;
    rdfs:range <http://rdaregistry.info/Elements/c/C10002> ;
    rdfs:subPropertyOf <http://rdaregistry.info/Elements/e/P20053>,
        <http://rdaregistry.info/Elements/u/P60432> ;
    owl:inverseOf <http://rdaregistry.info/Elements/a/P50155> ;
    skos:definition "Relates an expression to a person, family, or corporate body contributing to an expression of a work by responding to an interviewer, usually a reporter, pollster, or some other information gathering agent."@en .

<http://rdaregistry.info/Elements/e/P20048> a rdf:Property ;
    rdfs:label "has editor"@en ;
    reg:hasUnconstrained <http://rdaregistry.info/Elements/u/P60393> ;
    reg:lexicalAlias "http://rdaregistry.info/Elements/e/editor"@en ;
    reg:name "editor"@en ;
    reg:status <http://metadataregistry.org/uri/RegStatus/1001> ;
    rdfs:domain <http://rdaregistry.info/Elements/c/C10006> ;
    rdfs:isDefinedBy <http://rdaregistry.info/Elements/e/> ;
    rdfs:range <http://rdaregistry.info/Elements/c/C10002> ;
    rdfs:subPropertyOf <http://rdaregistry.info/Elements/e/P20053>,
        <http://rdaregistry.info/Elements/u/P60393> ;
    owl:inverseOf <http://rdaregistry.info/Elements/a/P50156> ;
    skos:definition "Relates an expression to a person, family, or corporate body contributing to an expression of a work by revising or clarifying the content, e.g., adding an introduction, notes, or other critical matter."@en ;
    skos:scopeNote "An editor may also prepare an expression of a work for production, publication, or distribution."@en .

<http://rdaregistry.info/Elements/e/P20049> a rdf:Property ;
    rdfs:label "has abridger"@en ;
    reg:hasUnconstrained <http://rdaregistry.info/Elements/u/P60394> ;
    reg:lexicalAlias "http://rdaregistry.info/Elements/e/abridger"@en ;
    reg:name "abridger"@en ;
    reg:status <http://metadataregistry.org/uri/RegStatus/1001> ;
    rdfs:domain <http://rdaregistry.info/Elements/c/C10006> ;
    rdfs:isDefinedBy <http://rdaregistry.info/Elements/e/> ;
    rdfs:range <http://rdaregistry.info/Elements/c/C10002> ;
    rdfs:subPropertyOf <http://rdaregistry.info/Elements/e/P20053>,
        <http://rdaregistry.info/Elements/u/P60394> ;
    owl:inverseOf <http://rdaregistry.info/Elements/a/P50157> ;
    skos:definition "Relates an expression to a person, family, or corporate body contributing to an expression of a work by shortening or condensing the original work but leaving the nature and content of the original work substantially unchanged."@en .

<http://rdaregistry.info/Elements/e/P20050> a rdf:Property ;
    rdfs:label "has recording engineer "@en ;
    reg:hasUnconstrained <http://rdaregistry.info/Elements/u/P60395> ;
    reg:lexicalAlias "http://rdaregistry.info/Elements/e/recordingEngineer"@en ;
    reg:name "recordingEngineer"@en ;
    reg:status <http://metadataregistry.org/uri/RegStatus/1001> ;
    rdfs:domain <http://rdaregistry.info/Elements/c/C10006> ;
    rdfs:isDefinedBy <http://rdaregistry.info/Elements/e/> ;
    rdfs:range <http://rdaregistry.info/Elements/c/C10002> ;
    rdfs:subPropertyOf <http://rdaregistry.info/Elements/e/P20053>,
        <http://rdaregistry.info/Elements/u/P60395> ;
    owl:inverseOf <http://rdaregistry.info/Elements/a/P50158> ;
    skos:definition "Relates an expression to a person, family, or corporate body contributing to an expression of a work by supervising the technical aspects of a sound or video recording session."@en .

<http://rdaregistry.info/Elements/e/P20052> a rdf:Property ;
    rdfs:label "has recordist "@en ;
    reg:hasUnconstrained <http://rdaregistry.info/Elements/u/P60397> ;
    reg:lexicalAlias "http://rdaregistry.info/Elements/e/recordist"@en ;
    reg:name "recordist"@en ;
    reg:status <http://metadataregistry.org/uri/RegStatus/1001> ;
    rdfs:domain <http://rdaregistry.info/Elements/c/C10006> ;
    rdfs:isDefinedBy <http://rdaregistry.info/Elements/e/> ;
    rdfs:range <http://rdaregistry.info/Elements/c/C10002> ;
    rdfs:subPropertyOf <http://rdaregistry.info/Elements/e/P20053>,
        <http://rdaregistry.info/Elements/u/P60397> ;
    owl:inverseOf <http://rdaregistry.info/Elements/a/P50160> ;
    skos:definition "Relates an expression to a person, family, or corporate body contributing to an expression of a work by using a recording device to capture sound and/or video during a recording session, including field recordings of natural sounds, folkloric events, music, etc."@en .

<http://rdaregistry.info/Elements/e/P20055> a rdf:Property ;
    rdfs:label "has editor of moving image work "@en ;
    reg:hasUnconstrained <http://rdaregistry.info/Elements/u/P60422> ;
    reg:lexicalAlias "http://rdaregistry.info/Elements/e/editorOfMovingImageWork"@en ;
    reg:name "editorOfMovingImageWork"@en ;
    reg:status <http://metadataregistry.org/uri/RegStatus/1001> ;
    rdfs:domain <http://rdaregistry.info/Elements/c/C10006> ;
    rdfs:isDefinedBy <http://rdaregistry.info/Elements/e/> ;
    rdfs:range <http://rdaregistry.info/Elements/c/C10002> ;
    rdfs:subPropertyOf <http://rdaregistry.info/Elements/e/P20053>,
        <http://rdaregistry.info/Elements/u/P60422> ;
    owl:inverseOf <http://rdaregistry.info/Elements/a/P50183> ;
    skos:definition "Relates an expression to a person, family, or corporate body responsible for assembling, arranging, and trimming film, video, or other moving image formats, including both visual and audio aspects."@en .

<http://rdaregistry.info/Elements/e/P20056> a rdf:Property ;
    rdfs:label "has production designer"@en ;
    reg:hasUnconstrained <http://rdaregistry.info/Elements/u/P60437> ;
    reg:lexicalAlias "http://rdaregistry.info/Elements/e/productionDesigner"@en ;
    reg:name "productionDesigner"@en ;
    reg:status <http://metadataregistry.org/uri/RegStatus/1001> ;
    rdfs:domain <http://rdaregistry.info/Elements/c/C10006> ;
    rdfs:isDefinedBy <http://rdaregistry.info/Elements/e/> ;
    rdfs:range <http://rdaregistry.info/Elements/c/C10002> ;
    rdfs:subPropertyOf <http://rdaregistry.info/Elements/e/P20053>,
        <http://rdaregistry.info/Elements/u/P60437> ;
    owl:inverseOf <http://rdaregistry.info/Elements/a/P50198> ;
    skos:definition "Relates an expression to a person, family, or corporate body responsible for designing the overall visual appearance of a moving image production."@en .

<http://rdaregistry.info/Elements/e/P20058> a rdf:Property ;
    rdfs:label "has minute taker"@en ;
    reg:hasUnconstrained <http://rdaregistry.info/Elements/u/P60446> ;
    reg:lexicalAlias "http://rdaregistry.info/Elements/e/minuteTaker"@en ;
    reg:name "minuteTaker"@en ;
    reg:status <http://metadataregistry.org/uri/RegStatus/1001> ;
    rdfs:domain <http://rdaregistry.info/Elements/c/C10006> ;
    rdfs:isDefinedBy <http://rdaregistry.info/Elements/e/> ;
    rdfs:range <http://rdaregistry.info/Elements/c/C10002> ;
    rdfs:subPropertyOf <http://rdaregistry.info/Elements/e/P20053>,
        <http://rdaregistry.info/Elements/u/P60446> ;
    owl:inverseOf <http://rdaregistry.info/Elements/a/P50212> ;
    skos:definition "Relates an expression to a person, family, or corporate body, responsible for recording the minutes of a meeting."@en .

<http://rdaregistry.info/Elements/e/P20061> a rdf:Property ;
    rdfs:label "has form of tactile notation"@en ;
    reg:hasUnconstrained <http://rdaregistry.info/Elements/u/P60318> ;
    reg:lexicalAlias "http://rdaregistry.info/Elements/e/formOfTactileNotation"@en ;
    reg:name "formOfTactileNotation"@en ;
    reg:status <http://metadataregistry.org/uri/RegStatus/1001> ;
    rdfs:domain <http://rdaregistry.info/Elements/c/C10006> ;
    rdfs:isDefinedBy <http://rdaregistry.info/Elements/e/> ;
    rdfs:subPropertyOf <http://rdaregistry.info/Elements/e/P20062>,
        <http://rdaregistry.info/Elements/u/P60318> ;
    skos:definition "Relates an expression to a set of characters and/or symbols used to express the content of a resource in a form that can be perceived through touch."@en .

<http://rdaregistry.info/Elements/e/P20063> a rdf:Property ;
    rdfs:label "has form of notated movement"@en ;
    reg:hasUnconstrained <http://rdaregistry.info/Elements/u/P60320> ;
    reg:lexicalAlias "http://rdaregistry.info/Elements/e/formOfNotatedMovement"@en ;
    reg:name "formOfNotatedMovement"@en ;
    reg:status <http://metadataregistry.org/uri/RegStatus/1001> ;
    rdfs:domain <http://rdaregistry.info/Elements/c/C10006> ;
    rdfs:isDefinedBy <http://rdaregistry.info/Elements/e/> ;
    rdfs:subPropertyOf <http://rdaregistry.info/Elements/e/P20062>,
        <http://rdaregistry.info/Elements/u/P60320> ;
    skos:definition "Relates an expression to a set of characters and/or symbols used to express the movement content of a resource."@en .

<http://rdaregistry.info/Elements/e/P20064> a rdf:Property ;
    rdfs:label "has form of musical notation"@en ;
    reg:hasUnconstrained <http://rdaregistry.info/Elements/u/P60321> ;
    reg:lexicalAlias "http://rdaregistry.info/Elements/e/formOfMusicalNotation"@en ;
    reg:name "formOfMusicalNotation"@en ;
    reg:status <http://metadataregistry.org/uri/RegStatus/1001> ;
    rdfs:domain <http://rdaregistry.info/Elements/c/C10006> ;
    rdfs:isDefinedBy <http://rdaregistry.info/Elements/e/> ;
    rdfs:subPropertyOf <http://rdaregistry.info/Elements/e/P20062>,
        <http://rdaregistry.info/Elements/u/P60321> ;
    skos:definition "Relates an expression to a set of characters and/or symbols used to express the musical content of a resource."@en .

<http://rdaregistry.info/Elements/e/P20065> a rdf:Property ;
    rdfs:label "has script"@en ;
    reg:hasUnconstrained <http://rdaregistry.info/Elements/u/P60322> ;
    reg:lexicalAlias "http://rdaregistry.info/Elements/e/script"@en ;
    reg:name "script"@en ;
    reg:status <http://metadataregistry.org/uri/RegStatus/1001> ;
    rdfs:domain <http://rdaregistry.info/Elements/c/C10006> ;
    rdfs:isDefinedBy <http://rdaregistry.info/Elements/e/> ;
    rdfs:subPropertyOf <http://rdaregistry.info/Elements/e/P20062>,
        <http://rdaregistry.info/Elements/u/P60322> ;
    skos:definition "Relates an expression to a set of characters and/or symbols used to express the written language content of a resource."@en .

<http://rdaregistry.info/Elements/e/P20068> a rdf:Property ;
    rdfs:label "has writer of added lyrics"@en ;
    reg:hasUnconstrained <http://rdaregistry.info/Elements/u/P60371> ;
    reg:lexicalAlias "http://rdaregistry.info/Elements/e/writerOfAddedLyrics"@en ;
    reg:name "writerOfAddedLyrics"@en ;
    reg:status <http://metadataregistry.org/uri/RegStatus/1001> ;
    rdfs:domain <http://rdaregistry.info/Elements/c/C10006> ;
    rdfs:isDefinedBy <http://rdaregistry.info/Elements/e/> ;
    rdfs:range <http://rdaregistry.info/Elements/c/C10002> ;
    rdfs:subPropertyOf <http://rdaregistry.info/Elements/e/P20030>,
        <http://rdaregistry.info/Elements/u/P60371> ;
    owl:inverseOf <http://rdaregistry.info/Elements/a/P50216> ;
    skos:definition "Relates an expression to a writer of words added to an expression of a musical work."@en .

<http://rdaregistry.info/Elements/e/P20070> a rdf:Property ;
    rdfs:label "has voice actor "@en ;
    reg:hasUnconstrained <http://rdaregistry.info/Elements/u/P60152> ;
    reg:lexicalAlias "http://rdaregistry.info/Elements/e/voiceActor"@en ;
    reg:name "voiceActor"@en ;
    reg:status <http://metadataregistry.org/uri/RegStatus/1001> ;
    rdfs:domain <http://rdaregistry.info/Elements/c/C10006> ;
    rdfs:isDefinedBy <http://rdaregistry.info/Elements/e/> ;
    rdfs:range <http://rdaregistry.info/Elements/c/C10002> ;
    rdfs:subPropertyOf <http://rdaregistry.info/Elements/e/P20012>,
        <http://rdaregistry.info/Elements/u/P60152> ;
    owl:inverseOf <http://rdaregistry.info/Elements/a/P50217> ;
    skos:definition "Relates an expression to an actor contributing to an expression of a work by providing the voice for characters in radio and audio productions and for animated characters in moving image works, as well as by providing voice-overs in radio and television commercials, dubbed resources, etc."@en .

<http://rdaregistry.info/Elements/e/P20071> a rdf:Property ;
    rdfs:label "has note on expression"@en ;
    reg:hasSubproperty <http://rdaregistry.info/Elements/e/P20010> ;
    reg:hasUnconstrained <http://rdaregistry.info/Elements/u/P60470> ;
    reg:lexicalAlias "http://rdaregistry.info/Elements/e/noteOnExpression"@en ;
    reg:name "noteOnExpression"@en ;
    reg:status <http://metadataregistry.org/uri/RegStatus/1001> ;
    rdfs:domain <http://rdaregistry.info/Elements/c/C10006> ;
    rdfs:isDefinedBy <http://rdaregistry.info/Elements/e/> ;
    skos:definition "Relates an expression to an annotation providing additional information about content recorded as an expression attribute."@en .

<http://rdaregistry.info/Elements/e/P20075> a rdf:Property ;
    rdfs:label "is replaced in part by (expression)"@en ;
    reg:hasUnconstrained <http://rdaregistry.info/Elements/u/P60103> ;
    reg:lexicalAlias "http://rdaregistry.info/Elements/e/replacedInPartByExpression"@en ;
    reg:name "replacedInPartByExpression"@en ;
    reg:status <http://metadataregistry.org/uri/RegStatus/1001> ;
    rdfs:domain <http://rdaregistry.info/Elements/c/C10006> ;
    rdfs:isDefinedBy <http://rdaregistry.info/Elements/e/> ;
    rdfs:range <http://rdaregistry.info/Elements/c/C10006> ;
    rdfs:subPropertyOf <http://rdaregistry.info/Elements/e/P20169> ;
    owl:inverseOf <http://rdaregistry.info/Elements/e/P20198> ;
    skos:definition "Relates an expression to an expression of a later work used in part in place of the earlier expression usually because the later work contains updated or new information that makes part of the earlier expression obsolete."@en .

<http://rdaregistry.info/Elements/e/P20085> a rdf:Property ;
    rdfs:label "is incidental music (expression)"@en ;
    reg:hasUnconstrained <http://rdaregistry.info/Elements/u/P60118> ;
    reg:lexicalAlias "http://rdaregistry.info/Elements/e/incidentalMusicExpression"@en ;
    reg:name "incidentalMusicExpression"@en ;
    reg:status <http://metadataregistry.org/uri/RegStatus/1001> ;
    rdfs:domain <http://rdaregistry.info/Elements/c/C10006> ;
    rdfs:isDefinedBy <http://rdaregistry.info/Elements/e/> ;
    rdfs:range <http://rdaregistry.info/Elements/c/C10006> ;
    rdfs:subPropertyOf <http://rdaregistry.info/Elements/e/P20243> ;
    owl:inverseOf <http://rdaregistry.info/Elements/e/P20103> ;
    skos:definition "Relates an expression to an expression of a musical work that that provides the incidental music for a play or other spoken work for the stage."@en .

<http://rdaregistry.info/Elements/e/P20103> a rdf:Property ;
    rdfs:label "is incidental music for (expression)"@en ;
    reg:hasUnconstrained <http://rdaregistry.info/Elements/u/P60202> ;
    reg:lexicalAlias "http://rdaregistry.info/Elements/e/incidentalMusicForExpression"@en ;
    reg:name "incidentalMusicForExpression"@en ;
    reg:status <http://metadataregistry.org/uri/RegStatus/1001> ;
    rdfs:domain <http://rdaregistry.info/Elements/c/C10006> ;
    rdfs:isDefinedBy <http://rdaregistry.info/Elements/e/> ;
    rdfs:range <http://rdaregistry.info/Elements/c/C10006> ;
    rdfs:subPropertyOf <http://rdaregistry.info/Elements/e/P20244> ;
    owl:inverseOf <http://rdaregistry.info/Elements/e/P20085> ;
    skos:definition "Relates an expression to an expression of a work such as a play or other spoken work for the stage that uses the musical work as incidental music."@en .

<http://rdaregistry.info/Elements/e/P20111> a rdf:Property ;
    rdfs:label "is reviewed in (expression)"@en ;
    reg:name "reviewedInExpression"@en ;
    reg:status <http://metadataregistry.org/uri/RegStatus/1008> ;
    rdfs:domain <http://rdaregistry.info/Elements/c/C10006> ;
    rdfs:isDefinedBy <http://rdaregistry.info/Elements/e/> ;
    rdfs:range <http://rdaregistry.info/Elements/c/C10006> ;
    rdfs:subPropertyOf <http://rdaregistry.info/Elements/e/P20202>,
        <http://rdaregistry.info/Elements/u/P60211> ;
    = <http://rdaregistry.info/Elements/e/reviewedInExpression> ;
    skos:definition "Relates an expression to an expression of a work that contains a brief evaluation of the described expression."@en .

<http://rdaregistry.info/Elements/e/P20112> a rdf:Property ;
    rdfs:label "is critiqued in (expression)"@en ;
    reg:name "critiquedInExpression"@en ;
    reg:status <http://metadataregistry.org/uri/RegStatus/1008> ;
    rdfs:domain <http://rdaregistry.info/Elements/c/C10006> ;
    rdfs:isDefinedBy <http://rdaregistry.info/Elements/e/> ;
    rdfs:range <http://rdaregistry.info/Elements/c/C10006> ;
    rdfs:subPropertyOf <http://rdaregistry.info/Elements/e/P20202>,
        <http://rdaregistry.info/Elements/u/P60212> ;
    = <http://rdaregistry.info/Elements/e/critiquedInExpression> ;
    skos:definition "Relates an expression to an expression of a work that contains a critical evaluation of the described expression."@en .

<http://rdaregistry.info/Elements/e/P20113> a rdf:Property ;
    rdfs:label "is commentary in (expression)"@en ;
    reg:name "commentaryInExpression"@en ;
    reg:status <http://metadataregistry.org/uri/RegStatus/1008> ;
    rdfs:domain <http://rdaregistry.info/Elements/c/C10006> ;
    rdfs:isDefinedBy <http://rdaregistry.info/Elements/e/> ;
    rdfs:range <http://rdaregistry.info/Elements/c/C10006> ;
    rdfs:subPropertyOf <http://rdaregistry.info/Elements/e/P20202>,
        <http://rdaregistry.info/Elements/u/P60213> ;
    = <http://rdaregistry.info/Elements/e/commentaryInExpression> ;
    skos:definition "Relates an expression to an expression of a work that contains a set of explanatory or critical notes on the described expression."@en .

<http://rdaregistry.info/Elements/e/P20212> a rdf:Property ;
    rdfs:label "is merged to form (expression)"@en ;
    reg:hasUnconstrained <http://rdaregistry.info/Elements/u/P60504> ;
    reg:lexicalAlias "http://rdaregistry.info/Elements/e/mergedToFormExpression"@en ;
    reg:name "mergedToFormExpression"@en ;
    reg:status <http://metadataregistry.org/uri/RegStatus/1001> ;
    rdfs:domain <http://rdaregistry.info/Elements/c/C10006> ;
    rdfs:isDefinedBy <http://rdaregistry.info/Elements/e/> ;
    rdfs:range <http://rdaregistry.info/Elements/c/C10006> ;
    rdfs:subPropertyOf <http://rdaregistry.info/Elements/e/P20169> ;
    owl:inverseOf <http://rdaregistry.info/Elements/e/P20201> ;
    skos:definition "Relates an expression to an expression of a work formed from the coming together of two or more expressions."@en .

<http://rdaregistry.info/Elements/e/P20213> a rdf:Property ;
    rdfs:label "has additional scale information"@en ;
    reg:hasUnconstrained <http://rdaregistry.info/Elements/u/P60510> ;
    reg:lexicalAlias "http://rdaregistry.info/Elements/e/additionalScaleInformation"@en ;
    reg:name "additionalScaleInformation"@en ;
    reg:status <http://metadataregistry.org/uri/RegStatus/1001> ;
    rdfs:domain <http://rdaregistry.info/Elements/c/C10006> ;
    rdfs:isDefinedBy <http://rdaregistry.info/Elements/e/> ;
    rdfs:subPropertyOf <http://rdaregistry.info/Elements/e/P20228>,
        <http://rdaregistry.info/Elements/u/P60510> ;
    skos:definition "Relates an expression to supplemental information about scale such as a statement of comparative measurements or limitation of the scale to particular parts of the content of a resource."@en .

<http://rdaregistry.info/Elements/e/P20226> a rdf:Property ;
    rdfs:label "has horizontal scale of cartographic content"@en ;
    reg:hasUnconstrained <http://rdaregistry.info/Elements/u/P60563> ;
    reg:lexicalAlias "http://rdaregistry.info/Elements/e/horizontalScaleOfCartographicContent"@en ;
    reg:name "horizontalScaleOfCartographicContent"@en ;
    reg:status <http://metadataregistry.org/uri/RegStatus/1001> ;
    rdfs:domain <http://rdaregistry.info/Elements/c/C10006> ;
    rdfs:isDefinedBy <http://rdaregistry.info/Elements/e/> ;
    rdfs:subPropertyOf <http://rdaregistry.info/Elements/e/P20228>,
        <http://rdaregistry.info/Elements/u/P60563> ;
    skos:definition "Relates an expression to the ratio of horizontal distances in the cartographic content of a resource to the actual distances they represent."@en .

<http://rdaregistry.info/Elements/e/P20227> a rdf:Property ;
    rdfs:label "has scale of still image or three-dimensional form"@en ;
    reg:hasUnconstrained <http://rdaregistry.info/Elements/u/P60564> ;
    reg:lexicalAlias "http://rdaregistry.info/Elements/e/scaleOfStillImageOrThreeDimensionalForm"@en ;
    reg:name "scaleOfStillImageOrThreeDimensionalForm"@en ;
    reg:status <http://metadataregistry.org/uri/RegStatus/1001> ;
    rdfs:domain <http://rdaregistry.info/Elements/c/C10006> ;
    rdfs:isDefinedBy <http://rdaregistry.info/Elements/e/> ;
    rdfs:subPropertyOf <http://rdaregistry.info/Elements/e/P20228>,
        <http://rdaregistry.info/Elements/u/P60564> ;
    skos:definition "Relates an expression to the ratio of the dimensions of a still image or three-dimensional form contained or embodied in a resource to the dimensions of the thing it represents."@en .

<http://rdaregistry.info/Elements/e/P20230> a rdf:Property ;
    rdfs:label "has vertical scale of cartographic content"@en ;
    reg:hasUnconstrained <http://rdaregistry.info/Elements/u/P60579> ;
    reg:lexicalAlias "http://rdaregistry.info/Elements/e/verticalScaleOfCartographicContent"@en ;
    reg:name "verticalScaleOfCartographicContent"@en ;
    reg:status <http://metadataregistry.org/uri/RegStatus/1001> ;
    rdfs:domain <http://rdaregistry.info/Elements/c/C10006> ;
    rdfs:isDefinedBy <http://rdaregistry.info/Elements/e/> ;
    rdfs:subPropertyOf <http://rdaregistry.info/Elements/e/P20228>,
        <http://rdaregistry.info/Elements/u/P60579> ;
    skos:definition "Relates an expression to the scale of elevation or vertical dimension of the cartographic content of a resource."@en .

<http://rdaregistry.info/Elements/e/P20234> a rdf:Property ;
    reg:hasSubproperty <http://rdaregistry.info/Elements/e/P20072> ;
    reg:status <http://metadataregistry.org/uri/RegStatus/1001> ;
    rdfs:isDefinedBy <http://rdaregistry.info/Elements/e/> .

<http://rdaregistry.info/Elements/e/P20239> a rdf:Property ;
    rdfs:label "is musical theatre adaptation of (expression)"@en ;
    reg:hasUnconstrained <http://rdaregistry.info/Elements/u/P60719> ;
    reg:lexicalAlias "http://rdaregistry.info/Elements/e/musicalTheatreAdaptationOfExpression"@en ;
    reg:name "musicalTheatreAdaptationOfExpression"@en ;
    reg:status <http://metadataregistry.org/uri/RegStatus/1001> ;
    rdfs:domain <http://rdaregistry.info/Elements/c/C10006> ;
    rdfs:isDefinedBy <http://rdaregistry.info/Elements/e/> ;
    rdfs:range <http://rdaregistry.info/Elements/c/C10006> ;
    rdfs:subPropertyOf <http://rdaregistry.info/Elements/e/P20152>,
        <http://rdaregistry.info/Elements/u/P60719> ;
    owl:inverseOf <http://rdaregistry.info/Elements/e/P20241> ;
    skos:definition "Relates an expression to an expression of a work that has been adapted as a musical theatre work."@en .

<http://rdaregistry.info/Elements/e/P20240> a rdf:Property ;
    rdfs:label "is opera adaptation of (expression)"@en ;
    reg:hasUnconstrained <http://rdaregistry.info/Elements/u/P60720> ;
    reg:lexicalAlias "http://rdaregistry.info/Elements/e/operaAdaptationOfExpression"@en ;
    reg:name "operaAdaptationOfExpression"@en ;
    reg:status <http://metadataregistry.org/uri/RegStatus/1001> ;
    rdfs:domain <http://rdaregistry.info/Elements/c/C10006> ;
    rdfs:isDefinedBy <http://rdaregistry.info/Elements/e/> ;
    rdfs:range <http://rdaregistry.info/Elements/c/C10006> ;
    rdfs:subPropertyOf <http://rdaregistry.info/Elements/e/P20152>,
        <http://rdaregistry.info/Elements/u/P60720> ;
    owl:inverseOf <http://rdaregistry.info/Elements/e/P20242> ;
    skos:definition "Relates an expression to an expression of a work that has been adapted as an opera."@en .

<http://rdaregistry.info/Elements/e/P20241> a rdf:Property ;
    rdfs:label "is adapted as musical theatre (expression) "@en ;
    reg:hasUnconstrained <http://rdaregistry.info/Elements/u/P60721> ;
    reg:lexicalAlias "http://rdaregistry.info/Elements/e/adaptedAsMusicalTheatreExpression"@en ;
    reg:name "adaptedAsMusicalTheatreExpression"@en ;
    reg:status <http://metadataregistry.org/uri/RegStatus/1001> ;
    rdfs:domain <http://rdaregistry.info/Elements/c/C10006> ;
    rdfs:isDefinedBy <http://rdaregistry.info/Elements/e/> ;
    rdfs:range <http://rdaregistry.info/Elements/c/C10006> ;
    rdfs:subPropertyOf <http://rdaregistry.info/Elements/e/P20153>,
        <http://rdaregistry.info/Elements/u/P60721> ;
    owl:inverseOf <http://rdaregistry.info/Elements/e/P20239> ;
    skos:definition "Relates an expression to an expression of a musical theatre work based on the source expression."@en .

<http://rdaregistry.info/Elements/e/P20242> a rdf:Property ;
    rdfs:label "is adapted as opera (expression) "@en ;
    reg:hasUnconstrained <http://rdaregistry.info/Elements/u/P60722> ;
    reg:lexicalAlias "http://rdaregistry.info/Elements/e/adaptedAsOperaExpression"@en ;
    reg:name "adaptedAsOperaExpression"@en ;
    reg:status <http://metadataregistry.org/uri/RegStatus/1001> ;
    rdfs:domain <http://rdaregistry.info/Elements/c/C10006> ;
    rdfs:isDefinedBy <http://rdaregistry.info/Elements/e/> ;
    rdfs:range <http://rdaregistry.info/Elements/c/C10006> ;
    rdfs:subPropertyOf <http://rdaregistry.info/Elements/e/P20153>,
        <http://rdaregistry.info/Elements/u/P60722> ;
    owl:inverseOf <http://rdaregistry.info/Elements/e/P20240> ;
    skos:definition "Relates an expression to an expression of an opera based on the source expression."@en .

<http://rdaregistry.info/Elements/e/P20245> a rdf:Property ;
    rdfs:label "is video music (expression) "@en ;
    reg:hasUnconstrained <http://rdaregistry.info/Elements/u/P60725> ;
    reg:lexicalAlias "http://rdaregistry.info/Elements/e/videoMusicExpression "@en ;
    reg:name "videoMusicExpression "@en ;
    reg:status <http://metadataregistry.org/uri/RegStatus/1001> ;
    rdfs:domain <http://rdaregistry.info/Elements/c/C10006> ;
    rdfs:isDefinedBy <http://rdaregistry.info/Elements/e/> ;
    rdfs:range <http://rdaregistry.info/Elements/c/C10006> ;
    rdfs:subPropertyOf <http://rdaregistry.info/Elements/e/P20243>,
        <http://rdaregistry.info/Elements/u/P60725> ;
    owl:inverseOf <http://rdaregistry.info/Elements/e/P20246> ;
    skos:definition "Relates an expression to an expression of a musical work that is used in a video."@en .

<http://rdaregistry.info/Elements/e/P20246> a rdf:Property ;
    rdfs:label "is music for video (expression)"@en ;
    reg:hasUnconstrained <http://rdaregistry.info/Elements/u/P60726> ;
    reg:lexicalAlias "http://rdaregistry.info/Elements/e/musicForVideoExpression"@en ;
    reg:name "musicForVideoExpression"@en ;
    reg:status <http://metadataregistry.org/uri/RegStatus/1001> ;
    rdfs:domain <http://rdaregistry.info/Elements/c/C10006> ;
    rdfs:isDefinedBy <http://rdaregistry.info/Elements/e/> ;
    rdfs:range <http://rdaregistry.info/Elements/c/C10006> ;
    rdfs:subPropertyOf <http://rdaregistry.info/Elements/e/P20244>,
        <http://rdaregistry.info/Elements/u/P60726> ;
    owl:inverseOf <http://rdaregistry.info/Elements/e/P20245> ;
    skos:definition "Relates an expression to an expression of a work that uses the musical work in a video. "@en .

<http://rdaregistry.info/Elements/e/P20247> a rdf:Property ;
    rdfs:label "is television program music (expression)"@en ;
    reg:hasUnconstrained <http://rdaregistry.info/Elements/u/P60727> ;
    reg:lexicalAlias "http://rdaregistry.info/Elements/e/televisionProgramMusicExpression"@en ;
    reg:name "televisionProgramMusicExpression"@en ;
    reg:status <http://metadataregistry.org/uri/RegStatus/1001> ;
    rdfs:domain <http://rdaregistry.info/Elements/c/C10006> ;
    rdfs:isDefinedBy <http://rdaregistry.info/Elements/e/> ;
    rdfs:range <http://rdaregistry.info/Elements/c/C10006> ;
    rdfs:subPropertyOf <http://rdaregistry.info/Elements/e/P20243>,
        <http://rdaregistry.info/Elements/u/P60727> ;
    owl:inverseOf <http://rdaregistry.info/Elements/e/P20248> ;
    skos:definition "Relates an expression to an expression of a musical work that is used in a television program. "@en .

<http://rdaregistry.info/Elements/e/P20248> a rdf:Property ;
    rdfs:label "is music for television program (expression)"@en ;
    reg:hasUnconstrained <http://rdaregistry.info/Elements/u/P60728> ;
    reg:lexicalAlias "http://rdaregistry.info/Elements/e/musicForTelevisionProgramExpression"@en ;
    reg:name "musicForTelevisionProgramExpression"@en ;
    reg:status <http://metadataregistry.org/uri/RegStatus/1001> ;
    rdfs:domain <http://rdaregistry.info/Elements/c/C10006> ;
    rdfs:isDefinedBy <http://rdaregistry.info/Elements/e/> ;
    rdfs:range <http://rdaregistry.info/Elements/c/C10006> ;
    rdfs:subPropertyOf <http://rdaregistry.info/Elements/e/P20244>,
        <http://rdaregistry.info/Elements/u/P60728> ;
    owl:inverseOf <http://rdaregistry.info/Elements/e/P20247> ;
    skos:definition "Relates an expression to an expression of a work that uses the musical work in a television program."@en .

<http://rdaregistry.info/Elements/e/P20249> a rdf:Property ;
    rdfs:label "is radio program music (expression)"@en ;
    reg:hasUnconstrained <http://rdaregistry.info/Elements/u/P60729> ;
    reg:lexicalAlias "http://rdaregistry.info/Elements/e/radioProgramMusicExpression"@en ;
    reg:name "radioProgramMusicExpression"@en ;
    reg:status <http://metadataregistry.org/uri/RegStatus/1001> ;
    rdfs:domain <http://rdaregistry.info/Elements/c/C10006> ;
    rdfs:isDefinedBy <http://rdaregistry.info/Elements/e/> ;
    rdfs:range <http://rdaregistry.info/Elements/c/C10006> ;
    rdfs:subPropertyOf <http://rdaregistry.info/Elements/e/P20243>,
        <http://rdaregistry.info/Elements/u/P60729> ;
    owl:inverseOf <http://rdaregistry.info/Elements/e/P20250> ;
    skos:definition "Relates an expression to an expression of a musical work that is used in a radio program."@en .

<http://rdaregistry.info/Elements/e/P20250> a rdf:Property ;
    rdfs:label "is music for radio program (expression)"@en ;
    reg:hasUnconstrained <http://rdaregistry.info/Elements/u/P60730> ;
    reg:lexicalAlias "http://rdaregistry.info/Elements/e/musicForRadioProgramExpression"@en ;
    reg:name "musicForRadioProgramExpression"@en ;
    reg:status <http://metadataregistry.org/uri/RegStatus/1001> ;
    rdfs:domain <http://rdaregistry.info/Elements/c/C10006> ;
    rdfs:isDefinedBy <http://rdaregistry.info/Elements/e/> ;
    rdfs:range <http://rdaregistry.info/Elements/c/C10006> ;
    rdfs:subPropertyOf <http://rdaregistry.info/Elements/e/P20244>,
        <http://rdaregistry.info/Elements/u/P60730> ;
    owl:inverseOf <http://rdaregistry.info/Elements/e/P20249> ;
    skos:definition "Relates an expression to an expression of a work that uses the musical work in a radio program."@en .

<http://rdaregistry.info/Elements/e/P20251> a rdf:Property ;
    rdfs:label "is motion picture music (expression)"@en ;
    reg:hasUnconstrained <http://rdaregistry.info/Elements/u/P60731> ;
    reg:lexicalAlias "http://rdaregistry.info/Elements/e/motionPictureMusicExpression"@en ;
    reg:name "motionPictureMusicExpression"@en ;
    reg:status <http://metadataregistry.org/uri/RegStatus/1001> ;
    rdfs:domain <http://rdaregistry.info/Elements/c/C10006> ;
    rdfs:isDefinedBy <http://rdaregistry.info/Elements/e/> ;
    rdfs:range <http://rdaregistry.info/Elements/c/C10006> ;
    rdfs:subPropertyOf <http://rdaregistry.info/Elements/e/P20243>,
        <http://rdaregistry.info/Elements/u/P60731> ;
    owl:inverseOf <http://rdaregistry.info/Elements/e/P20252> ;
    skos:definition "Relates an expression to an expression of a musical work that is used in a motion picture."@en .

<http://rdaregistry.info/Elements/e/P20252> a rdf:Property ;
    rdfs:label "is music for motion picture (expression)"@en ;
    reg:hasUnconstrained <http://rdaregistry.info/Elements/u/P60732> ;
    reg:lexicalAlias "http://rdaregistry.info/Elements/e/musicForMotionPictureExpression"@en ;
    reg:name "musicForMotionPictureExpression"@en ;
    reg:status <http://metadataregistry.org/uri/RegStatus/1001> ;
    rdfs:domain <http://rdaregistry.info/Elements/c/C10006> ;
    rdfs:isDefinedBy <http://rdaregistry.info/Elements/e/> ;
    rdfs:range <http://rdaregistry.info/Elements/c/C10006> ;
    rdfs:subPropertyOf <http://rdaregistry.info/Elements/e/P20244>,
        <http://rdaregistry.info/Elements/u/P60732> ;
    owl:inverseOf <http://rdaregistry.info/Elements/e/P20251> ;
    skos:definition "Relates an expression to an expression of a work that uses the musical work in a motion picture."@en .

<http://rdaregistry.info/Elements/e/P20257> a rdf:Property ;
    rdfs:label "has visual effects provider"@en ;
    reg:hasUnconstrained <http://rdaregistry.info/Elements/u/P60748> ;
    reg:lexicalAlias "http://rdaregistry.info/Elements/e/visualEffectsProvider"@en ;
    reg:name "visualEffectsProvider"@en ;
    reg:status <http://metadataregistry.org/uri/RegStatus/1001> ;
    rdfs:domain <http://rdaregistry.info/Elements/c/C10006> ;
    rdfs:isDefinedBy <http://rdaregistry.info/Elements/e/> ;
    rdfs:range <http://rdaregistry.info/Elements/c/C10002> ;
    rdfs:subPropertyOf <http://rdaregistry.info/Elements/e/P20053> ;
    owl:inverseOf <http://rdaregistry.info/Elements/a/P50243> ;
    skos:definition "Relates an expression to a person, family, or corporate body contributing to an expression of a moving image work by designing and creating post-production visual effects."@en .

<http://rdaregistry.info/Elements/e/P20258> a rdf:Property ;
    rdfs:label "has special effects provider"@en ;
    reg:hasUnconstrained <http://rdaregistry.info/Elements/u/P60749> ;
    reg:lexicalAlias "http://rdaregistry.info/Elements/e/specialEffectsProvider"@en ;
    reg:name "specialEffectsProvider"@en ;
    reg:status <http://metadataregistry.org/uri/RegStatus/1001> ;
    rdfs:domain <http://rdaregistry.info/Elements/c/C10006> ;
    rdfs:isDefinedBy <http://rdaregistry.info/Elements/e/> ;
    rdfs:range <http://rdaregistry.info/Elements/c/C10002> ;
    rdfs:subPropertyOf <http://rdaregistry.info/Elements/e/P20053> ;
    owl:inverseOf <http://rdaregistry.info/Elements/a/P50244> ;
    skos:definition "Relates an expression to a person, family, or corporate body contributing to an expression of a moving image or audio work by designing and creating on-set special effects (on-set mechanical effects and in-camera optical effects)."@en .

<http://rdaregistry.info/Elements/e/P20259> a rdf:Property ;
    rdfs:label "has letterer"@en ;
    reg:hasUnconstrained <http://rdaregistry.info/Elements/u/P60750> ;
    reg:lexicalAlias "http://rdaregistry.info/Elements/e/letterer"@en ;
    reg:name "letterer"@en ;
    reg:status <http://metadataregistry.org/uri/RegStatus/1001> ;
    rdfs:domain <http://rdaregistry.info/Elements/c/C10006> ;
    rdfs:isDefinedBy <http://rdaregistry.info/Elements/e/> ;
    rdfs:range <http://rdaregistry.info/Elements/c/C10002> ;
    rdfs:subPropertyOf <http://rdaregistry.info/Elements/e/P20051> ;
    owl:inverseOf <http://rdaregistry.info/Elements/a/P50245> ;
    skos:definition "Relates an expression to an illustrator contributing to an expression of a comic book, graphic novel, etc., by drawing the text and graphic sound effects."@en .

<http://rdaregistry.info/Elements/e/P20268> a rdf:Property ;
    rdfs:label "is subject of (expression)"@en ;
    reg:hasSubproperty <http://rdaregistry.info/Elements/e/P20269> ;
    reg:hasUnconstrained <http://rdaregistry.info/Elements/u/P60806> ;
    reg:lexicalAlias "http://rdaregistry.info/Elements/e/subjectOfExpression"@en ;
    reg:name "subjectOfExpression"@en ;
    reg:status <http://metadataregistry.org/uri/RegStatus/1001> ;
    rdfs:domain <http://rdaregistry.info/Elements/c/C10006> ;
    rdfs:isDefinedBy <http://rdaregistry.info/Elements/e/> ;
    rdfs:range <http://rdaregistry.info/Elements/c/C10001> ;
    rdfs:subPropertyOf <http://rdaregistry.info/Elements/w/P10283> ;
    owl:inverseOf <http://rdaregistry.info/Elements/w/P10258> ;
    skos:definition "Relates an expression to a work that is about the expression."@en .

<http://rdaregistry.info/Elements/e/P20270> a rdf:Property ;
    rdfs:label "is analysed in (expression)"@en ;
    reg:hasUnconstrained <http://rdaregistry.info/Elements/u/P60219> ;
    reg:lexicalAlias "http://rdaregistry.info/Elements/e/analysedInExpression"@en ;
    reg:name "analysedInExpression"@en ;
    reg:status <http://metadataregistry.org/uri/RegStatus/1001> ;
    rdfs:domain <http://rdaregistry.info/Elements/c/C10006> ;
    rdfs:isDefinedBy <http://rdaregistry.info/Elements/e/> ;
    rdfs:range <http://rdaregistry.info/Elements/c/C10001> ;
    rdfs:subPropertyOf <http://rdaregistry.info/Elements/e/P20269> ;
    owl:inverseOf <http://rdaregistry.info/Elements/w/P10278> ;
    skos:definition "Relates a expression to a work that examines the source expression to identify its components and their relations."@en .

<http://rdaregistry.info/Elements/e/P20271> a rdf:Property ;
    rdfs:label "is commentary in (expression)"@en ;
    reg:hasUnconstrained <http://rdaregistry.info/Elements/u/P60213> ;
    reg:lexicalAlias "http://rdaregistry.info/Elements/e/commentaryInexpression"@en ;
    reg:name "commentaryInexpression"@en ;
    reg:status <http://metadataregistry.org/uri/RegStatus/1001> ;
    rdfs:domain <http://rdaregistry.info/Elements/c/C10006> ;
    rdfs:isDefinedBy <http://rdaregistry.info/Elements/e/> ;
    rdfs:range <http://rdaregistry.info/Elements/c/C10001> ;
    rdfs:subPropertyOf <http://rdaregistry.info/Elements/e/P20269> ;
    owl:inverseOf <http://rdaregistry.info/Elements/w/P10282> ;
    skos:definition "Relates a expression to a work that contains a set of explanatory or critical notes on the described expression. "@en .

<http://rdaregistry.info/Elements/e/P20272> a rdf:Property ;
    rdfs:label "is critiqued in (expression)"@en ;
    reg:hasUnconstrained <http://rdaregistry.info/Elements/u/P60212> ;
    reg:lexicalAlias "http://rdaregistry.info/Elements/e/critiquedInexpression"@en ;
    reg:name "critiqued in (expression)"@en ;
    reg:status <http://metadataregistry.org/uri/RegStatus/1001> ;
    rdfs:domain <http://rdaregistry.info/Elements/c/C10006> ;
    rdfs:isDefinedBy <http://rdaregistry.info/Elements/e/> ;
    rdfs:range <http://rdaregistry.info/Elements/c/C10001> ;
    rdfs:subPropertyOf <http://rdaregistry.info/Elements/e/P20269> ;
    owl:inverseOf <http://rdaregistry.info/Elements/w/P10281> ;
    skos:definition "Relates a expression to a work that contains a critical evaluation of the described expression."@en .

<http://rdaregistry.info/Elements/e/P20273> a rdf:Property ;
    rdfs:label "is evaluated in (expression)"@en ;
    reg:hasUnconstrained <http://rdaregistry.info/Elements/u/P60218> ;
    reg:lexicalAlias "http://rdaregistry.info/Elements/e/evaluatedInexpression"@en ;
    reg:name "evaluatedInexpression"@en ;
    reg:status <http://metadataregistry.org/uri/RegStatus/1001> ;
    rdfs:domain <http://rdaregistry.info/Elements/c/C10006> ;
    rdfs:isDefinedBy <http://rdaregistry.info/Elements/e/> ;
    rdfs:range <http://rdaregistry.info/Elements/c/C10001> ;
    rdfs:subPropertyOf <http://rdaregistry.info/Elements/e/P20269> ;
    owl:inverseOf <http://rdaregistry.info/Elements/w/P10279> ;
    skos:definition "Relates a expression to a work that examines or judges the described expression."@en .

<http://rdaregistry.info/Elements/e/P20274> a rdf:Property ;
    rdfs:label "is reviewed in (expression)"@en ;
    reg:hasUnconstrained <http://rdaregistry.info/Elements/u/P60211> ;
    reg:lexicalAlias "http://rdaregistry.info/Elements/e/reviewedInexpression"@en ;
    reg:name "reviewedInexpression"@en ;
    reg:status <http://metadataregistry.org/uri/RegStatus/1001> ;
    rdfs:domain <http://rdaregistry.info/Elements/c/C10006> ;
    rdfs:isDefinedBy <http://rdaregistry.info/Elements/e/> ;
    rdfs:range <http://rdaregistry.info/Elements/c/C10001> ;
    rdfs:subPropertyOf <http://rdaregistry.info/Elements/e/P20269> ;
    owl:inverseOf <http://rdaregistry.info/Elements/w/P10280> ;
    skos:definition "Relates a expression to a work that contains a brief evaluation of the described expression."@en .

<http://rdaregistry.info/Elements/e/P20275> a rdf:Property ;
    rdfs:label "has writer of foreword"@en ;
    reg:hasUnconstrained <http://rdaregistry.info/Elements/u/P60809> ;
    reg:lexicalAlias "http://rdaregistry.info/Elements/e/writerOfForeword"@en ;
    reg:name "writerOfForeword"@en ;
    reg:status <http://metadataregistry.org/uri/RegStatus/1001> ;
    rdfs:domain <http://rdaregistry.info/Elements/c/C10006> ;
    rdfs:isDefinedBy <http://rdaregistry.info/Elements/e/> ;
    rdfs:range <http://rdaregistry.info/Elements/c/C10002> ;
    rdfs:subPropertyOf <http://rdaregistry.info/Elements/e/P20046> ;
    owl:inverseOf <http://rdaregistry.info/Elements/a/P50254> ;
    skos:definition "Relates an expression to a person, family, or corporate body contributing to an expression of a work by providing a foreword to the original work."@en .

<http://rdaregistry.info/Elements/e/P20276> a rdf:Property ;
    rdfs:label "has sound designer"@en ;
    reg:hasUnconstrained <http://rdaregistry.info/Elements/u/P60811> ;
    reg:lexicalAlias "http://rdaregistry.info/Elements/e/soundDesigner"@en ;
    reg:name "soundDesigner"@en ;
    reg:status <http://metadataregistry.org/uri/RegStatus/1001> ;
    rdfs:domain <http://rdaregistry.info/Elements/c/C10006> ;
    rdfs:isDefinedBy <http://rdaregistry.info/Elements/e/> ;
    rdfs:range <http://rdaregistry.info/Elements/c/C10002> ;
    rdfs:subPropertyOf <http://rdaregistry.info/Elements/e/P20053> ;
    owl:inverseOf <http://rdaregistry.info/Elements/a/P50255> ;
    skos:definition "Relates an expression to a person, family or corporate body contributing to an expression of a work by designing and creating audio/sound components."@en .

<http://rdaregistry.info/Elements/e/P20277> a rdf:Property ;
    rdfs:label "has lighting designer"@en ;
    reg:hasUnconstrained <http://rdaregistry.info/Elements/u/P60813> ;
    reg:lexicalAlias "http://rdaregistry.info/Elements/e/lightingDesigner"@en ;
    reg:name "lightingDesigner"@en ;
    reg:status <http://metadataregistry.org/uri/RegStatus/1001> ;
    rdfs:domain <http://rdaregistry.info/Elements/c/C10006> ;
    rdfs:isDefinedBy <http://rdaregistry.info/Elements/e/> ;
    rdfs:range <http://rdaregistry.info/Elements/c/C10002> ;
    rdfs:subPropertyOf <http://rdaregistry.info/Elements/e/P20053> ;
    owl:inverseOf <http://rdaregistry.info/Elements/a/P50256> ;
    skos:definition "Relates an expression to a person, family or corporate body contributing to an expression of a work by designing and creating lighting components."@en .

<http://rdaregistry.info/Elements/e/P20009> a rdf:Property ;
    rdfs:label "is adapted as motion picture (expression)"@en ;
    reg:hasUnconstrained <http://rdaregistry.info/Elements/u/P60110> ;
    reg:lexicalAlias "http://rdaregistry.info/Elements/e/adaptedAsMotionPictureExpression"@en ;
    reg:name "adaptedAsMotionPictureExpression"@en ;
    reg:status <http://metadataregistry.org/uri/RegStatus/1001> ;
    rdfs:domain <http://rdaregistry.info/Elements/c/C10006> ;
    rdfs:isDefinedBy <http://rdaregistry.info/Elements/e/> ;
    rdfs:range <http://rdaregistry.info/Elements/c/C10006> ;
    rdfs:subPropertyOf <http://rdaregistry.info/Elements/e/P20153>,
        <http://rdaregistry.info/Elements/u/P60110> ;
    owl:inverseOf <http://rdaregistry.info/Elements/e/P20125> ;
    skos:definition "Relates an expression to a motion picture based on the source expression."@en .

<http://rdaregistry.info/Elements/e/P20012> a rdf:Property ;
    rdfs:label "has actor "@en ;
    reg:hasSubproperty <http://rdaregistry.info/Elements/e/P20070> ;
    reg:hasUnconstrained <http://rdaregistry.info/Elements/u/P60142> ;
    reg:lexicalAlias "http://rdaregistry.info/Elements/e/actor"@en ;
    reg:name "actor"@en ;
    reg:status <http://metadataregistry.org/uri/RegStatus/1001> ;
    rdfs:domain <http://rdaregistry.info/Elements/c/C10006> ;
    rdfs:isDefinedBy <http://rdaregistry.info/Elements/e/> ;
    rdfs:range <http://rdaregistry.info/Elements/c/C10002> ;
    rdfs:subPropertyOf <http://rdaregistry.info/Elements/e/P20039>,
        <http://rdaregistry.info/Elements/u/P60142> ;
    owl:inverseOf <http://rdaregistry.info/Elements/a/P50071> ;
    skos:definition "Relates an expression to a performer contributing to an expression of a work by acting as a cast member or player in a musical or dramatic presentation, etc."@en .

<http://rdaregistry.info/Elements/e/P20030> a rdf:Property ;
    rdfs:label "has writer of added text"@en ;
    reg:hasSubproperty <http://rdaregistry.info/Elements/e/P20068> ;
    reg:hasUnconstrained <http://rdaregistry.info/Elements/u/P60380> ;
    reg:lexicalAlias "http://rdaregistry.info/Elements/e/writerOfAddedText"@en ;
    reg:name "writerOfAddedText"@en ;
    reg:status <http://metadataregistry.org/uri/RegStatus/1001> ;
    rdfs:domain <http://rdaregistry.info/Elements/c/C10006> ;
    rdfs:isDefinedBy <http://rdaregistry.info/Elements/e/> ;
    rdfs:range <http://rdaregistry.info/Elements/c/C10002> ;
    rdfs:subPropertyOf <http://rdaregistry.info/Elements/e/P20046>,
        <http://rdaregistry.info/Elements/u/P60380> ;
    owl:inverseOf <http://rdaregistry.info/Elements/a/P50138> ;
    skos:definition "Relates an expression to a person, family, or corporate body contributing to an expression of a primarily non-textual work by providing text for the non-textual work (e.g., writing captions for photographs, descriptions of maps)."@en .

<http://rdaregistry.info/Elements/e/P20051> a rdf:Property ;
    rdfs:label "has illustrator"@en ;
    reg:hasSubproperty <http://rdaregistry.info/Elements/e/P20259> ;
    reg:hasUnconstrained <http://rdaregistry.info/Elements/u/P60396> ;
    reg:lexicalAlias "http://rdaregistry.info/Elements/e/illustrator"@en ;
    reg:name "illustrator"@en ;
    reg:status <http://metadataregistry.org/uri/RegStatus/1001> ;
    rdfs:domain <http://rdaregistry.info/Elements/c/C10006> ;
    rdfs:isDefinedBy <http://rdaregistry.info/Elements/e/> ;
    rdfs:range <http://rdaregistry.info/Elements/c/C10002> ;
    rdfs:subPropertyOf <http://rdaregistry.info/Elements/e/P20053>,
        <http://rdaregistry.info/Elements/u/P60396> ;
    owl:inverseOf <http://rdaregistry.info/Elements/a/P50159> ;
    skos:definition "Relates an expression to a person, family, or corporate body contributing to an expression of a work by supplementing the primary content with drawings, diagrams, photographs, etc."@en .

<http://rdaregistry.info/Elements/e/P20060> a rdf:Property ;
    rdfs:label "is adapted as radio program (expression)"@en ;
    reg:hasUnconstrained <http://rdaregistry.info/Elements/u/P60174> ;
    reg:lexicalAlias "http://rdaregistry.info/Elements/e/adaptedAsRadioProgramExpression"@en ;
    reg:name "adaptedAsRadioProgramExpression"@en ;
    reg:status <http://metadataregistry.org/uri/RegStatus/1001> ;
    rdfs:domain <http://rdaregistry.info/Elements/c/C10006> ;
    rdfs:isDefinedBy <http://rdaregistry.info/Elements/e/> ;
    rdfs:range <http://rdaregistry.info/Elements/c/C10006> ;
    rdfs:subPropertyOf <http://rdaregistry.info/Elements/e/P20153>,
        <http://rdaregistry.info/Elements/u/P60174> ;
    owl:inverseOf <http://rdaregistry.info/Elements/e/P20127> ;
    skos:definition "Relates an expression to a radio program based on the source expression."@en .

<http://rdaregistry.info/Elements/e/P20066> a rdf:Property ;
    rdfs:label "is adapted as television program (expression)"@en ;
    reg:hasUnconstrained <http://rdaregistry.info/Elements/u/P60354> ;
    reg:lexicalAlias "http://rdaregistry.info/Elements/e/adaptedAsTelevisionProgramExpression"@en ;
    reg:name "adaptedAsTelevisionProgramExpression"@en ;
    reg:status <http://metadataregistry.org/uri/RegStatus/1001> ;
    rdfs:domain <http://rdaregistry.info/Elements/c/C10006> ;
    rdfs:isDefinedBy <http://rdaregistry.info/Elements/e/> ;
    rdfs:range <http://rdaregistry.info/Elements/c/C10006> ;
    rdfs:subPropertyOf <http://rdaregistry.info/Elements/e/P20153>,
        <http://rdaregistry.info/Elements/u/P60354> ;
    owl:inverseOf <http://rdaregistry.info/Elements/e/P20128> ;
    skos:definition "Relates an expression to a television program based on the source expression."@en .

<http://rdaregistry.info/Elements/e/P20067> a rdf:Property ;
    rdfs:label "is adapted as video (expression)"@en ;
    reg:hasUnconstrained <http://rdaregistry.info/Elements/u/P60361> ;
    reg:lexicalAlias "http://rdaregistry.info/Elements/e/adaptedAsVideoExpression"@en ;
    reg:name "adaptedAsVideoExpression"@en ;
    reg:status <http://metadataregistry.org/uri/RegStatus/1001> ;
    rdfs:domain <http://rdaregistry.info/Elements/c/C10006> ;
    rdfs:isDefinedBy <http://rdaregistry.info/Elements/e/> ;
    rdfs:range <http://rdaregistry.info/Elements/c/C10006> ;
    rdfs:subPropertyOf <http://rdaregistry.info/Elements/e/P20153>,
        <http://rdaregistry.info/Elements/u/P60361> ;
    owl:inverseOf <http://rdaregistry.info/Elements/e/P20134> ;
    skos:definition "Relates an expression to a video based on the source expression."@en .

<http://rdaregistry.info/Elements/e/P20073> a rdf:Property ;
    rdfs:label "is dramatized as (expression)"@en ;
    reg:hasUnconstrained <http://rdaregistry.info/Elements/u/P60088> ;
    reg:lexicalAlias "http://rdaregistry.info/Elements/e/dramatizedAsExpression"@en ;
    reg:name "dramatizedAsExpression"@en ;
    reg:status <http://metadataregistry.org/uri/RegStatus/1001> ;
    rdfs:domain <http://rdaregistry.info/Elements/c/C10006> ;
    rdfs:isDefinedBy <http://rdaregistry.info/Elements/e/> ;
    rdfs:range <http://rdaregistry.info/Elements/c/C10006> ;
    rdfs:subPropertyOf <http://rdaregistry.info/Elements/e/P20153>,
        <http://rdaregistry.info/Elements/u/P60088> ;
    owl:inverseOf <http://rdaregistry.info/Elements/e/P20123> ;
    skos:definition "Relates an expression to an expression of a dramatic work adapted from the source expression."@en .

<http://rdaregistry.info/Elements/e/P20074> a rdf:Property ;
    rdfs:label "is contained in (expression)"@en ;
    reg:hasUnconstrained <http://rdaregistry.info/Elements/u/P60101> ;
    reg:lexicalAlias "http://rdaregistry.info/Elements/e/containedInExpression"@en ;
    reg:name "containedInExpression"@en ;
    reg:status <http://metadataregistry.org/uri/RegStatus/1001> ;
    rdfs:domain <http://rdaregistry.info/Elements/c/C10006> ;
    rdfs:isDefinedBy <http://rdaregistry.info/Elements/e/> ;
    rdfs:range <http://rdaregistry.info/Elements/c/C10006> ;
    rdfs:subPropertyOf <http://rdaregistry.info/Elements/e/P20236>,
        <http://rdaregistry.info/Elements/u/P60101> ;
    owl:inverseOf <http://rdaregistry.info/Elements/e/P20145> ;
    skos:definition "Relates an expression to an expression of a larger work of which the expression is a discrete component."@en .

<http://rdaregistry.info/Elements/e/P20076> a rdf:Property ;
    rdfs:label "is replaced by (expression)"@en ;
    reg:hasUnconstrained <http://rdaregistry.info/Elements/u/P60104> ;
    reg:lexicalAlias "http://rdaregistry.info/Elements/e/replacedByExpression"@en ;
    reg:name "replacedByExpression"@en ;
    reg:status <http://metadataregistry.org/uri/RegStatus/1001> ;
    rdfs:domain <http://rdaregistry.info/Elements/c/C10006> ;
    rdfs:isDefinedBy <http://rdaregistry.info/Elements/e/> ;
    rdfs:range <http://rdaregistry.info/Elements/c/C10006> ;
    rdfs:subPropertyOf <http://rdaregistry.info/Elements/e/P20169>,
        <http://rdaregistry.info/Elements/u/P60104> ;
    owl:inverseOf <http://rdaregistry.info/Elements/e/P20199> ;
    skos:definition "Relates an expression to an expression of a later work used in place of the earlier expression, usually because the later work contains updated or new information that makes the earlier expression obsolete."@en .

<http://rdaregistry.info/Elements/e/P20077> a rdf:Property ;
    rdfs:label "is adapted in verse as (expression)"@en ;
    reg:hasUnconstrained <http://rdaregistry.info/Elements/u/P60106> ;
    reg:lexicalAlias "http://rdaregistry.info/Elements/e/adaptedInVerseAsExpression"@en ;
    reg:name "adaptedInVerseAsExpression"@en ;
    reg:status <http://metadataregistry.org/uri/RegStatus/1001> ;
    rdfs:domain <http://rdaregistry.info/Elements/c/C10006> ;
    rdfs:isDefinedBy <http://rdaregistry.info/Elements/e/> ;
    rdfs:range <http://rdaregistry.info/Elements/c/C10006> ;
    rdfs:subPropertyOf <http://rdaregistry.info/Elements/e/P20153>,
        <http://rdaregistry.info/Elements/u/P60106> ;
    owl:inverseOf <http://rdaregistry.info/Elements/e/P20124> ;
    skos:definition "Relates an expression to an expression of a literary composition in verse form adapted from the source expression."@en .

<http://rdaregistry.info/Elements/e/P20078> a rdf:Property ;
    rdfs:label "is dubbed version of"@en ;
    reg:hasUnconstrained <http://rdaregistry.info/Elements/u/P60111> ;
    reg:lexicalAlias "http://rdaregistry.info/Elements/e/dubbedVersionOf"@en ;
    reg:name "dubbedVersionOf"@en ;
    reg:status <http://metadataregistry.org/uri/RegStatus/1001> ;
    rdfs:domain <http://rdaregistry.info/Elements/c/C10006> ;
    rdfs:isDefinedBy <http://rdaregistry.info/Elements/e/> ;
    rdfs:range <http://rdaregistry.info/Elements/c/C10006> ;
    rdfs:subPropertyOf <http://rdaregistry.info/Elements/e/P20141>,
        <http://rdaregistry.info/Elements/u/P60111> ;
    owl:inverseOf <http://rdaregistry.info/Elements/e/P20079> ;
    skos:definition "Relates an expression to an expression of a moving image work in which the spoken dialogue has been translated into a language different from that of the original work."@en .

<http://rdaregistry.info/Elements/e/P20079> a rdf:Property ;
    rdfs:label "is dubbed version"@en ;
    reg:hasUnconstrained <http://rdaregistry.info/Elements/u/P60112> ;
    reg:lexicalAlias "http://rdaregistry.info/Elements/e/dubbedVersion"@en ;
    reg:name "dubbedVersion"@en ;
    reg:status <http://metadataregistry.org/uri/RegStatus/1001> ;
    rdfs:domain <http://rdaregistry.info/Elements/c/C10006> ;
    rdfs:isDefinedBy <http://rdaregistry.info/Elements/e/> ;
    rdfs:range <http://rdaregistry.info/Elements/c/C10006> ;
    rdfs:subPropertyOf <http://rdaregistry.info/Elements/e/P20171>,
        <http://rdaregistry.info/Elements/u/P60112> ;
    owl:inverseOf <http://rdaregistry.info/Elements/e/P20078> ;
    skos:definition "Relates an expression to an expression of a moving image work that translates the spoken dialogue of the original work into a different language."@en .

<http://rdaregistry.info/Elements/e/P20080> a rdf:Property ;
    rdfs:label "is cadenza (expression)"@en ;
    reg:hasUnconstrained <http://rdaregistry.info/Elements/u/P60113> ;
    reg:lexicalAlias "http://rdaregistry.info/Elements/e/cadenzaExpression"@en ;
    reg:name "cadenzaExpression"@en ;
    reg:status <http://metadataregistry.org/uri/RegStatus/1001> ;
    rdfs:domain <http://rdaregistry.info/Elements/c/C10006> ;
    rdfs:isDefinedBy <http://rdaregistry.info/Elements/e/> ;
    rdfs:range <http://rdaregistry.info/Elements/c/C10006> ;
    rdfs:subPropertyOf <http://rdaregistry.info/Elements/e/P20105>,
        <http://rdaregistry.info/Elements/u/P60113> ;
    owl:inverseOf <http://rdaregistry.info/Elements/e/P20083> ;
    skos:definition "Relates an expression to an expression of a musical work consisting of an ornamental passage for a soloist, added to a musical work such as a concerto, either by the same or a different composer."@en .

<http://rdaregistry.info/Elements/e/P20081> a rdf:Property ;
    rdfs:label "is variations based on (expression)"@en ;
    reg:hasUnconstrained <http://rdaregistry.info/Elements/u/P60114> ;
    reg:lexicalAlias "http://rdaregistry.info/Elements/e/variationsBasedOnExpression"@en ;
    reg:name "variationsBasedOnExpression"@en ;
    reg:status <http://metadataregistry.org/uri/RegStatus/1001> ;
    rdfs:domain <http://rdaregistry.info/Elements/c/C10006> ;
    rdfs:isDefinedBy <http://rdaregistry.info/Elements/e/> ;
    rdfs:range <http://rdaregistry.info/Elements/c/C10006> ;
    rdfs:subPropertyOf <http://rdaregistry.info/Elements/e/P20204>,
        <http://rdaregistry.info/Elements/u/P60114> ;
    owl:inverseOf <http://rdaregistry.info/Elements/e/P20082> ;
    skos:definition "Relates an expression to an expression of a musical work from which melodic, thematic, or harmonic material is taken to form a discrete theme, which is repeated one or more times with subsequent modifications."@en .

<http://rdaregistry.info/Elements/e/P20082> a rdf:Property ;
    rdfs:label "is modified by variation as (expression)"@en ;
    reg:hasUnconstrained <http://rdaregistry.info/Elements/u/P60115> ;
    reg:lexicalAlias "http://rdaregistry.info/Elements/e/modifiedByVariationAsExpression"@en ;
    reg:name "modifiedByVariationAsExpression"@en ;
    reg:status <http://metadataregistry.org/uri/RegStatus/1001> ;
    rdfs:domain <http://rdaregistry.info/Elements/c/C10006> ;
    rdfs:isDefinedBy <http://rdaregistry.info/Elements/e/> ;
    rdfs:range <http://rdaregistry.info/Elements/c/C10006> ;
    rdfs:subPropertyOf <http://rdaregistry.info/Elements/e/P20203>,
        <http://rdaregistry.info/Elements/u/P60115> ;
    owl:inverseOf <http://rdaregistry.info/Elements/e/P20081> ;
    skos:definition "Relates an expression to an expression of a musical work in which melodic, thematic, or harmonic material is taken from the source work to form a discrete theme, which is repeated one or more times with subsequent modifications."@en .

<http://rdaregistry.info/Elements/e/P20083> a rdf:Property ;
    rdfs:label "is cadenza composed for (expression)"@en ;
    reg:hasUnconstrained <http://rdaregistry.info/Elements/u/P60116> ;
    reg:lexicalAlias "http://rdaregistry.info/Elements/e/cadenzaComposedForExpression"@en ;
    reg:name "cadenzaComposedForExpression"@en ;
    reg:status <http://metadataregistry.org/uri/RegStatus/1001> ;
    rdfs:domain <http://rdaregistry.info/Elements/c/C10006> ;
    rdfs:isDefinedBy <http://rdaregistry.info/Elements/e/> ;
    rdfs:range <http://rdaregistry.info/Elements/c/C10006> ;
    rdfs:subPropertyOf <http://rdaregistry.info/Elements/e/P20192>,
        <http://rdaregistry.info/Elements/u/P60116> ;
    owl:inverseOf <http://rdaregistry.info/Elements/e/P20080> ;
    skos:definition "Relates an expression to an expression of a musical work such as a concerto for which an ornamental passage for a soloist has been composed, either by the same or a different composer."@en .

<http://rdaregistry.info/Elements/e/P20084> a rdf:Property ;
    rdfs:label "is libretto for (expression)"@en ;
    reg:hasUnconstrained <http://rdaregistry.info/Elements/u/P60117> ;
    reg:lexicalAlias "http://rdaregistry.info/Elements/e/librettoForExpression"@en ;
    reg:name "librettoForExpression"@en ;
    reg:status <http://metadataregistry.org/uri/RegStatus/1001> ;
    rdfs:domain <http://rdaregistry.info/Elements/c/C10006> ;
    rdfs:isDefinedBy <http://rdaregistry.info/Elements/e/> ;
    rdfs:range <http://rdaregistry.info/Elements/c/C10006> ;
    rdfs:subPropertyOf <http://rdaregistry.info/Elements/e/P20100>,
        <http://rdaregistry.info/Elements/u/P60117> ;
    owl:inverseOf <http://rdaregistry.info/Elements/e/P20163> ;
    skos:definition "Relates an expression to an expression of a musical work such as an opera or other work for the musical stage, or an oratorio, that uses the text of the related work."@en .

<http://rdaregistry.info/Elements/e/P20086> a rdf:Property ;
    rdfs:label "is remade as (expression)"@en ;
    reg:hasUnconstrained <http://rdaregistry.info/Elements/u/P60120> ;
    reg:lexicalAlias "http://rdaregistry.info/Elements/e/remadeAsExpression"@en ;
    reg:name "remadeAsExpression"@en ;
    reg:status <http://metadataregistry.org/uri/RegStatus/1001> ;
    rdfs:domain <http://rdaregistry.info/Elements/c/C10006> ;
    rdfs:isDefinedBy <http://rdaregistry.info/Elements/e/> ;
    rdfs:range <http://rdaregistry.info/Elements/c/C10006> ;
    rdfs:subPropertyOf <http://rdaregistry.info/Elements/e/P20203>,
        <http://rdaregistry.info/Elements/u/P60120> ;
    owl:inverseOf <http://rdaregistry.info/Elements/e/P20185> ;
    skos:definition "Relates an expression to an expression of a new motion picture, radio program, television program, or video based on an earlier work."@en .

<http://rdaregistry.info/Elements/e/P20087> a rdf:Property ;
    rdfs:label "is set to music as (expression)"@en ;
    reg:hasUnconstrained <http://rdaregistry.info/Elements/u/P60121> ;
    reg:lexicalAlias "http://rdaregistry.info/Elements/e/setToMusicAsExpression"@en ;
    reg:name "setToMusicAsExpression"@en ;
    reg:status <http://metadataregistry.org/uri/RegStatus/1001> ;
    rdfs:domain <http://rdaregistry.info/Elements/c/C10006> ;
    rdfs:isDefinedBy <http://rdaregistry.info/Elements/e/> ;
    rdfs:range <http://rdaregistry.info/Elements/c/C10006> ;
    rdfs:subPropertyOf <http://rdaregistry.info/Elements/e/P20203>,
        <http://rdaregistry.info/Elements/u/P60121> ;
    owl:inverseOf <http://rdaregistry.info/Elements/e/P20159> ;
    skos:definition "Relates an expression to an expression of a non-dramatic musical work, other than an oratorio, that uses the text of the source work."@en .

<http://rdaregistry.info/Elements/e/P20088> a rdf:Property ;
    rdfs:label "is adapted as novel (expression)"@en ;
    reg:hasUnconstrained <http://rdaregistry.info/Elements/u/P60138> ;
    reg:lexicalAlias "http://rdaregistry.info/Elements/e/adaptedAsNovelExpression"@en ;
    reg:name "adaptedAsNovelExpression"@en ;
    reg:status <http://metadataregistry.org/uri/RegStatus/1001> ;
    rdfs:domain <http://rdaregistry.info/Elements/c/C10006> ;
    rdfs:isDefinedBy <http://rdaregistry.info/Elements/e/> ;
    rdfs:range <http://rdaregistry.info/Elements/c/C10006> ;
    rdfs:subPropertyOf <http://rdaregistry.info/Elements/e/P20153>,
        <http://rdaregistry.info/Elements/u/P60138> ;
    owl:inverseOf <http://rdaregistry.info/Elements/e/P20126> ;
    skos:definition "Relates an expression to an expression of a novel adapted from the source expression."@en .

<http://rdaregistry.info/Elements/e/P20089> a rdf:Property ;
    rdfs:label "is appendix to (expression)"@en ;
    reg:hasUnconstrained <http://rdaregistry.info/Elements/u/P60253> ;
    reg:lexicalAlias "http://rdaregistry.info/Elements/e/appendixToExpression"@en ;
    reg:name "appendixToExpression"@en ;
    reg:status <http://metadataregistry.org/uri/RegStatus/1001> ;
    rdfs:domain <http://rdaregistry.info/Elements/c/C10006> ;
    rdfs:isDefinedBy <http://rdaregistry.info/Elements/e/> ;
    rdfs:range <http://rdaregistry.info/Elements/c/C10006> ;
    rdfs:subPropertyOf <http://rdaregistry.info/Elements/e/P20192>,
        <http://rdaregistry.info/Elements/u/P60253> ;
    owl:inverseOf <http://rdaregistry.info/Elements/e/P20118> ;
    skos:definition "Relates an expression to an expression of a predominant work that is augmented by another work that consists of material that is not essential to the completeness of the content, such as a list of references, statistical tables, and explanatory matter; the augmenting work can either come at the end of the content, or be issued separately."@en .

<http://rdaregistry.info/Elements/e/P20090> a rdf:Property ;
    rdfs:label "is abstracted in (expression)"@en ;
    reg:hasUnconstrained <http://rdaregistry.info/Elements/u/P60177> ;
    reg:lexicalAlias "http://rdaregistry.info/Elements/e/abstractedInExpression"@en ;
    reg:name "abstractedInExpression"@en ;
    reg:status <http://metadataregistry.org/uri/RegStatus/1001> ;
    rdfs:domain <http://rdaregistry.info/Elements/c/C10006> ;
    rdfs:isDefinedBy <http://rdaregistry.info/Elements/e/> ;
    rdfs:range <http://rdaregistry.info/Elements/c/C10006> ;
    rdfs:subPropertyOf <http://rdaregistry.info/Elements/e/P20203>,
        <http://rdaregistry.info/Elements/u/P60177> ;
    owl:inverseOf <http://rdaregistry.info/Elements/e/P20193> ;
    skos:definition "Relates an expression to an expression of a work (an abstracting and indexing service) that abstracts the contents of a source expression."@en .

<http://rdaregistry.info/Elements/e/P20091> a rdf:Property ;
    rdfs:label "is indexed in (expression)"@en ;
    reg:hasUnconstrained <http://rdaregistry.info/Elements/u/P60178> ;
    reg:lexicalAlias "http://rdaregistry.info/Elements/e/indexedInExpression"@en ;
    reg:name "indexedInExpression"@en ;
    reg:status <http://metadataregistry.org/uri/RegStatus/1001> ;
    rdfs:domain <http://rdaregistry.info/Elements/c/C10006> ;
    rdfs:isDefinedBy <http://rdaregistry.info/Elements/e/> ;
    rdfs:range <http://rdaregistry.info/Elements/c/C10006> ;
    rdfs:subPropertyOf <http://rdaregistry.info/Elements/e/P20203>,
        <http://rdaregistry.info/Elements/u/P60178> ;
    owl:inverseOf <http://rdaregistry.info/Elements/e/P20194> ;
    skos:definition "Relates an expression to an expression of a work (an abstracting and indexing service) that indexes the contents of a source expression."@en .

<http://rdaregistry.info/Elements/e/P20092> a rdf:Property ;
    rdfs:label "is adapted as choreography (expression)"@en ;
    reg:hasUnconstrained <http://rdaregistry.info/Elements/u/P60180> ;
    reg:lexicalAlias "http://rdaregistry.info/Elements/e/adaptedAsChoreographyExpression"@en ;
    reg:name "adaptedAsChoreographyExpression"@en ;
    reg:status <http://metadataregistry.org/uri/RegStatus/1001> ;
    rdfs:domain <http://rdaregistry.info/Elements/c/C10006> ;
    rdfs:isDefinedBy <http://rdaregistry.info/Elements/e/> ;
    rdfs:range <http://rdaregistry.info/Elements/c/C10006> ;
    rdfs:subPropertyOf <http://rdaregistry.info/Elements/e/P20153> ;
    owl:inverseOf <http://rdaregistry.info/Elements/e/P20183> ;
    skos:definition "Relates an expression to an expression of a work consisting of movement (e.g., dance) based on the source work."@en .

<http://rdaregistry.info/Elements/e/P20093> a rdf:Property ;
    rdfs:label "is errata (expression)"@en ;
    reg:hasUnconstrained <http://rdaregistry.info/Elements/u/P60181> ;
    reg:lexicalAlias "http://rdaregistry.info/Elements/e/errataExpression"@en ;
    reg:name "errataExpression"@en ;
    reg:status <http://metadataregistry.org/uri/RegStatus/1001> ;
    rdfs:domain <http://rdaregistry.info/Elements/c/C10006> ;
    rdfs:isDefinedBy <http://rdaregistry.info/Elements/e/> ;
    rdfs:range <http://rdaregistry.info/Elements/c/C10006> ;
    rdfs:subPropertyOf <http://rdaregistry.info/Elements/e/P20105>,
        <http://rdaregistry.info/Elements/u/P60181> ;
    owl:inverseOf <http://rdaregistry.info/Elements/e/P20146> ;
    skos:definition "Relates an expression to an expression of a work consisting of errors discovered after the publication of the predominant work, with their corrections."@en .

<http://rdaregistry.info/Elements/e/P20094> a rdf:Property ;
    rdfs:label "is illustrations (expression)"@en ;
    reg:hasUnconstrained <http://rdaregistry.info/Elements/u/P60182> ;
    reg:lexicalAlias "http://rdaregistry.info/Elements/e/illustrationsExpression"@en ;
    reg:name "illustrationsExpression"@en ;
    reg:status <http://metadataregistry.org/uri/RegStatus/1001> ;
    rdfs:domain <http://rdaregistry.info/Elements/c/C10006> ;
    rdfs:isDefinedBy <http://rdaregistry.info/Elements/e/> ;
    rdfs:range <http://rdaregistry.info/Elements/c/C10006> ;
    rdfs:subPropertyOf <http://rdaregistry.info/Elements/e/P20105>,
        <http://rdaregistry.info/Elements/u/P60182> ;
    owl:inverseOf <http://rdaregistry.info/Elements/e/P20148> ;
    skos:definition "Relates an expression to an expression of a work consisting of pictorial content designed to explain or decorate the augmented expression."@en .

<http://rdaregistry.info/Elements/e/P20095> a rdf:Property ;
    rdfs:label "is adapted as motion picture screenplay (expression)"@en ;
    reg:hasUnconstrained <http://rdaregistry.info/Elements/u/P60184> ;
    reg:lexicalAlias "http://rdaregistry.info/Elements/e/adaptedAsMotionPictureScreenplayExpression"@en ;
    reg:name "adaptedAsMotionPictureScreenplayExpression"@en ;
    reg:status <http://metadataregistry.org/uri/RegStatus/1001> ;
    rdfs:domain <http://rdaregistry.info/Elements/c/C10006> ;
    rdfs:isDefinedBy <http://rdaregistry.info/Elements/e/> ;
    rdfs:range <http://rdaregistry.info/Elements/c/C10006> ;
    rdfs:subPropertyOf <http://rdaregistry.info/Elements/e/P20096>,
        <http://rdaregistry.info/Elements/u/P60184> ;
    owl:inverseOf <http://rdaregistry.info/Elements/e/P20130> ;
    skos:definition "Relates an expression to an expression of a work consisting of the screenplay for a motion picture, based on the source work."@en .

<http://rdaregistry.info/Elements/e/P20097> a rdf:Property ;
    rdfs:label "is adapted as television screenplay (expression)"@en ;
    reg:hasUnconstrained <http://rdaregistry.info/Elements/u/P60186> ;
    reg:lexicalAlias "http://rdaregistry.info/Elements/e/adaptedAsTelevisionScreenplayExpression"@en ;
    reg:name "adaptedAsTelevisionScreenplayExpression"@en ;
    reg:status <http://metadataregistry.org/uri/RegStatus/1001> ;
    rdfs:domain <http://rdaregistry.info/Elements/c/C10006> ;
    rdfs:isDefinedBy <http://rdaregistry.info/Elements/e/> ;
    rdfs:range <http://rdaregistry.info/Elements/c/C10006> ;
    rdfs:subPropertyOf <http://rdaregistry.info/Elements/e/P20096>,
        <http://rdaregistry.info/Elements/u/P60186> ;
    owl:inverseOf <http://rdaregistry.info/Elements/e/P20131> ;
    skos:definition "Relates an expression to an expression of a work consisting of the screenplay for a television program, based on the source work."@en .

<http://rdaregistry.info/Elements/e/P20098> a rdf:Property ;
    rdfs:label "is adapted as video screenplay (expression)"@en ;
    reg:hasUnconstrained <http://rdaregistry.info/Elements/u/P60187> ;
    reg:lexicalAlias "http://rdaregistry.info/Elements/e/adaptedAsVideoScreenplayExpression"@en ;
    reg:name "adaptedAsVideoScreenplayExpression"@en ;
    reg:status <http://metadataregistry.org/uri/RegStatus/1001> ;
    rdfs:domain <http://rdaregistry.info/Elements/c/C10006> ;
    rdfs:isDefinedBy <http://rdaregistry.info/Elements/e/> ;
    rdfs:range <http://rdaregistry.info/Elements/c/C10006> ;
    rdfs:subPropertyOf <http://rdaregistry.info/Elements/e/P20096>,
        <http://rdaregistry.info/Elements/u/P60187> ;
    owl:inverseOf <http://rdaregistry.info/Elements/e/P20132> ;
    skos:definition "Relates an expression to an expression of a work consisting of the screenplay for a video, based on the source work."@en .

<http://rdaregistry.info/Elements/e/P20099> a rdf:Property ;
    rdfs:label "is adapted as radio script (expression)"@en ;
    reg:hasUnconstrained <http://rdaregistry.info/Elements/u/P60188> ;
    reg:lexicalAlias "http://rdaregistry.info/Elements/e/adaptedAsRadioScriptExpression"@en ;
    reg:name "adaptedAsRadioScriptExpression"@en ;
    reg:status <http://metadataregistry.org/uri/RegStatus/1001> ;
    rdfs:domain <http://rdaregistry.info/Elements/c/C10006> ;
    rdfs:isDefinedBy <http://rdaregistry.info/Elements/e/> ;
    rdfs:range <http://rdaregistry.info/Elements/c/C10006> ;
    rdfs:subPropertyOf <http://rdaregistry.info/Elements/e/P20153>,
        <http://rdaregistry.info/Elements/u/P60188> ;
    owl:inverseOf <http://rdaregistry.info/Elements/e/P20133> ;
    skos:definition "Relates an expression to an expression of a work consisting of the script for a radio program, based on the source work."@en .

<http://rdaregistry.info/Elements/e/P20101> a rdf:Property ;
    rdfs:label "is continued in part by (expression)"@en ;
    reg:hasUnconstrained <http://rdaregistry.info/Elements/u/P60199> ;
    reg:lexicalAlias "http://rdaregistry.info/Elements/e/continuedInPartByExpression"@en ;
    reg:name "continuedInPartByExpression"@en ;
    reg:status <http://metadataregistry.org/uri/RegStatus/1001> ;
    rdfs:domain <http://rdaregistry.info/Elements/c/C10006> ;
    rdfs:isDefinedBy <http://rdaregistry.info/Elements/e/> ;
    rdfs:range <http://rdaregistry.info/Elements/c/C10006> ;
    rdfs:subPropertyOf <http://rdaregistry.info/Elements/e/P20169>,
        <http://rdaregistry.info/Elements/u/P60199> ;
    owl:inverseOf <http://rdaregistry.info/Elements/e/P20168> ;
    skos:definition "Relates an expression to an expression of a work part of whose content separated from an earlier expression to form a new expression."@en .

<http://rdaregistry.info/Elements/e/P20104> a rdf:Property ;
    rdfs:label "is abstracted as (expression)"@en ;
    reg:hasUnconstrained <http://rdaregistry.info/Elements/u/P60203> ;
    reg:lexicalAlias "http://rdaregistry.info/Elements/e/abstractedAsExpression"@en ;
    reg:name "abstractedAsExpression"@en ;
    reg:status <http://metadataregistry.org/uri/RegStatus/1001> ;
    rdfs:domain <http://rdaregistry.info/Elements/c/C10006> ;
    rdfs:isDefinedBy <http://rdaregistry.info/Elements/e/> ;
    rdfs:range <http://rdaregistry.info/Elements/c/C10006> ;
    rdfs:subPropertyOf <http://rdaregistry.info/Elements/e/P20203>,
        <http://rdaregistry.info/Elements/u/P60203> ;
    owl:inverseOf <http://rdaregistry.info/Elements/e/P20122> ;
    skos:definition "Relates an expression to an expression of a work that abbreviates the source expression in a brief, objective manner."@en .

<http://rdaregistry.info/Elements/e/P20106> a rdf:Property ;
    rdfs:label "is summarized as (expression)"@en ;
    reg:hasUnconstrained <http://rdaregistry.info/Elements/u/P60205> ;
    reg:lexicalAlias "http://rdaregistry.info/Elements/e/summarizedAsExpression"@en ;
    reg:name "summarizedAsExpression"@en ;
    reg:status <http://metadataregistry.org/uri/RegStatus/1001> ;
    rdfs:domain <http://rdaregistry.info/Elements/c/C10006> ;
    rdfs:isDefinedBy <http://rdaregistry.info/Elements/e/> ;
    rdfs:range <http://rdaregistry.info/Elements/c/C10006> ;
    rdfs:subPropertyOf <http://rdaregistry.info/Elements/e/P20203>,
        <http://rdaregistry.info/Elements/u/P60205> ;
    owl:inverseOf <http://rdaregistry.info/Elements/e/P20179> ;
    skos:definition "Relates an expression to an expression of a work that consists of a brief recapitulation of the content of the source expression."@en .

<http://rdaregistry.info/Elements/e/P20107> a rdf:Property ;
    rdfs:label "is catalogue (expression)"@en ;
    reg:hasUnconstrained <http://rdaregistry.info/Elements/u/P60206> ;
    reg:lexicalAlias "http://rdaregistry.info/Elements/e/catalogueExpression"@en ;
    reg:name "catalogueExpression"@en ;
    reg:status <http://metadataregistry.org/uri/RegStatus/1001> ;
    rdfs:domain <http://rdaregistry.info/Elements/c/C10006> ;
    rdfs:isDefinedBy <http://rdaregistry.info/Elements/e/> ;
    rdfs:range <http://rdaregistry.info/Elements/c/C10006> ;
    rdfs:subPropertyOf <http://rdaregistry.info/Elements/e/P20105>,
        <http://rdaregistry.info/Elements/u/P60206> ;
    owl:inverseOf <http://rdaregistry.info/Elements/e/P20180> ;
    skos:definition "Relates an expression to an expression of a work that consists of a complete enumeration of items arranged systematically."@en .

<http://rdaregistry.info/Elements/e/P20108> a rdf:Property ;
    rdfs:label "is concordance (expression)"@en ;
    reg:hasUnconstrained <http://rdaregistry.info/Elements/u/P60208> ;
    reg:lexicalAlias "http://rdaregistry.info/Elements/e/concordanceExpression"@en ;
    reg:name "concordanceExpression"@en ;
    reg:status <http://metadataregistry.org/uri/RegStatus/1001> ;
    rdfs:domain <http://rdaregistry.info/Elements/c/C10006> ;
    rdfs:isDefinedBy <http://rdaregistry.info/Elements/e/> ;
    rdfs:range <http://rdaregistry.info/Elements/c/C10006> ;
    rdfs:subPropertyOf <http://rdaregistry.info/Elements/e/P20105>,
        <http://rdaregistry.info/Elements/u/P60208> ;
    owl:inverseOf <http://rdaregistry.info/Elements/e/P20181> ;
    skos:definition "Relates an expression to an expression of a work that consists of an index of all the words in the predominant expression."@en .

<http://rdaregistry.info/Elements/e/P20109> a rdf:Property ;
    rdfs:label "is addenda (expression)"@en ;
    reg:hasUnconstrained <http://rdaregistry.info/Elements/u/P60209> ;
    reg:lexicalAlias "http://rdaregistry.info/Elements/e/addendaExpression"@en ;
    reg:name "addendaExpression"@en ;
    reg:status <http://metadataregistry.org/uri/RegStatus/1001> ;
    rdfs:domain <http://rdaregistry.info/Elements/c/C10006> ;
    rdfs:isDefinedBy <http://rdaregistry.info/Elements/e/> ;
    rdfs:range <http://rdaregistry.info/Elements/c/C10006> ;
    rdfs:subPropertyOf <http://rdaregistry.info/Elements/e/P20105>,
        <http://rdaregistry.info/Elements/u/P60209> ;
    owl:inverseOf <http://rdaregistry.info/Elements/e/P20177> ;
    skos:definition "Relates an expression to an expression of a work that consists of brief additional material, less extensive than a supplement, but essential to the completeness of the text of the predominant work; it is usually added at the end of the content, but is sometimes issued separately."@en .

<http://rdaregistry.info/Elements/e/P20110> a rdf:Property ;
    rdfs:label "is adapted as libretto (expression)"@en ;
    reg:hasUnconstrained <http://rdaregistry.info/Elements/u/P60210> ;
    reg:lexicalAlias "http://rdaregistry.info/Elements/e/adaptedAsLibrettoExpression"@en ;
    reg:name "adaptedAsLibrettoExpression"@en ;
    reg:status <http://metadataregistry.org/uri/RegStatus/1001> ;
    rdfs:domain <http://rdaregistry.info/Elements/c/C10006> ;
    rdfs:isDefinedBy <http://rdaregistry.info/Elements/e/> ;
    rdfs:range <http://rdaregistry.info/Elements/c/C10006> ;
    rdfs:subPropertyOf <http://rdaregistry.info/Elements/e/P20153> ;
    owl:inverseOf <http://rdaregistry.info/Elements/e/P20190> ;
    skos:definition "Relates an expression to an expression of a work that consists of the text of an opera or other work for the musical stage, or an oratorio, based on the source work."@en .

<http://rdaregistry.info/Elements/e/P20115> a rdf:Property ;
    rdfs:label "is expanded as (expression)"@en ;
    reg:hasUnconstrained <http://rdaregistry.info/Elements/u/P60216> ;
    reg:lexicalAlias "http://rdaregistry.info/Elements/e/expandedAsExpression"@en ;
    reg:name "expandedAsExpression"@en ;
    reg:status <http://metadataregistry.org/uri/RegStatus/1001> ;
    rdfs:domain <http://rdaregistry.info/Elements/c/C10006> ;
    rdfs:isDefinedBy <http://rdaregistry.info/Elements/e/> ;
    rdfs:range <http://rdaregistry.info/Elements/c/C10006> ;
    rdfs:subPropertyOf <http://rdaregistry.info/Elements/e/P20203>,
        <http://rdaregistry.info/Elements/u/P60216> ;
    owl:inverseOf <http://rdaregistry.info/Elements/e/P20184> ;
    skos:definition "Relates an expression to an expression of a work that enlarges upon the content of the source work."@en .

<http://rdaregistry.info/Elements/e/P20116> a rdf:Property ;
    rdfs:label "is evaluated in (expression)"@en ;
    reg:name "evaluatedInExpression"@en ;
    reg:status <http://metadataregistry.org/uri/RegStatus/1008> ;
    rdfs:domain <http://rdaregistry.info/Elements/c/C10006> ;
    rdfs:isDefinedBy <http://rdaregistry.info/Elements/e/> ;
    rdfs:range <http://rdaregistry.info/Elements/c/C10006> ;
    rdfs:subPropertyOf <http://rdaregistry.info/Elements/e/P20202>,
        <http://rdaregistry.info/Elements/u/P60218> ;
    owl:inverseOf <http://rdaregistry.info/Elements/e/P20150> ;
    = <http://rdaregistry.info/Elements/e/evaluatedInExpression> ;
    skos:definition "Relates an expression to an expression of a work that examines or judges the described expression."@en .

<http://rdaregistry.info/Elements/e/P20117> a rdf:Property ;
    rdfs:label "is analysed in (expression)"@en ;
    reg:name "analysedInExpression"@en ;
    reg:status <http://metadataregistry.org/uri/RegStatus/1008> ;
    rdfs:domain <http://rdaregistry.info/Elements/c/C10006> ;
    rdfs:isDefinedBy <http://rdaregistry.info/Elements/e/> ;
    rdfs:range <http://rdaregistry.info/Elements/c/C10006> ;
    rdfs:subPropertyOf <http://rdaregistry.info/Elements/e/P20202>,
        <http://rdaregistry.info/Elements/u/P60219> ;
    owl:inverseOf <http://rdaregistry.info/Elements/e/P20136> ;
    = <http://rdaregistry.info/Elements/e/analysedInExpression> ;
    skos:definition "Relates an expression to an expression of a work that examines the source expression to identify its components and their relations."@en .

<http://rdaregistry.info/Elements/e/P20118> a rdf:Property ;
    rdfs:label "is appendix (expression)"@en ;
    reg:hasUnconstrained <http://rdaregistry.info/Elements/u/P60221> ;
    reg:lexicalAlias "http://rdaregistry.info/Elements/e/appendixExpression"@en ;
    reg:name "appendixExpression"@en ;
    reg:status <http://metadataregistry.org/uri/RegStatus/1001> ;
    rdfs:domain <http://rdaregistry.info/Elements/c/C10006> ;
    rdfs:isDefinedBy <http://rdaregistry.info/Elements/e/> ;
    rdfs:range <http://rdaregistry.info/Elements/c/C10006> ;
    rdfs:subPropertyOf <http://rdaregistry.info/Elements/e/P20105>,
        <http://rdaregistry.info/Elements/u/P60221> ;
    owl:inverseOf <http://rdaregistry.info/Elements/e/P20089> ;
    skos:definition "Relates an expression to an expression of a work that forms an augmenting part of another work which is not essential to the completeness of the content, such as a list of references, statistical tables, and explanatory matter; it can be material which either comes at the end of the content of the predominant work, or is issued separately."@en .

<http://rdaregistry.info/Elements/e/P20119> a rdf:Property ;
    rdfs:label "is freely translated as (expression)"@en ;
    reg:hasUnconstrained <http://rdaregistry.info/Elements/u/P60189> ;
    reg:lexicalAlias "http://rdaregistry.info/Elements/e/freelyTranslatedAsExpression"@en ;
    reg:name "freelyTranslatedAsExpression"@en ;
    reg:status <http://metadataregistry.org/uri/RegStatus/1001> ;
    rdfs:domain <http://rdaregistry.info/Elements/c/C10006> ;
    rdfs:isDefinedBy <http://rdaregistry.info/Elements/e/> ;
    rdfs:range <http://rdaregistry.info/Elements/c/C10006> ;
    rdfs:subPropertyOf <http://rdaregistry.info/Elements/e/P20203>,
        <http://rdaregistry.info/Elements/u/P60189> ;
    owl:inverseOf <http://rdaregistry.info/Elements/e/P20140> ;
    skos:definition "Relates an expression to an expression of a work that freely translates the text into another language, preserving the spirit of the original, but not its linguistic details."@en .

<http://rdaregistry.info/Elements/e/P20120> a rdf:Property ;
    rdfs:label "is guide (expression)"@en ;
    reg:hasUnconstrained <http://rdaregistry.info/Elements/u/P60222> ;
    reg:lexicalAlias "http://rdaregistry.info/Elements/e/guideExpression"@en ;
    reg:name "guideExpression"@en ;
    reg:status <http://metadataregistry.org/uri/RegStatus/1001> ;
    rdfs:domain <http://rdaregistry.info/Elements/c/C10006> ;
    rdfs:isDefinedBy <http://rdaregistry.info/Elements/e/> ;
    rdfs:range <http://rdaregistry.info/Elements/c/C10006> ;
    rdfs:subPropertyOf <http://rdaregistry.info/Elements/e/P20105>,
        <http://rdaregistry.info/Elements/u/P60222> ;
    owl:inverseOf <http://rdaregistry.info/Elements/e/P20147> ;
    skos:definition "Relates an expression to an expression of a work that guides a user through the use of the predominant work, using notes, learning and study aids, exercises, problems, questions and answers, instructor or student materials, etc."@en .

<http://rdaregistry.info/Elements/e/P20121> a rdf:Property ;
    rdfs:label "is abridgement of (expression)"@en ;
    reg:hasUnconstrained <http://rdaregistry.info/Elements/u/P60223> ;
    reg:lexicalAlias "http://rdaregistry.info/Elements/e/abridgementOfExpression"@en ;
    reg:name "abridgementOfExpression"@en ;
    reg:status <http://metadataregistry.org/uri/RegStatus/1001> ;
    rdfs:domain <http://rdaregistry.info/Elements/c/C10006> ;
    rdfs:isDefinedBy <http://rdaregistry.info/Elements/e/> ;
    rdfs:range <http://rdaregistry.info/Elements/c/C10006> ;
    rdfs:subPropertyOf <http://rdaregistry.info/Elements/e/P20204>,
        <http://rdaregistry.info/Elements/u/P60223> ;
    owl:inverseOf <http://rdaregistry.info/Elements/e/P20166> ;
    skos:definition "Relates an expression to an expression of a work that has been abridged, i.e., shortened without changing the general meaning or manner of presentation of the source work."@en .

<http://rdaregistry.info/Elements/e/P20122> a rdf:Property ;
    rdfs:label "is abstract of (expression)"@en ;
    reg:hasUnconstrained <http://rdaregistry.info/Elements/u/P60224> ;
    reg:lexicalAlias "http://rdaregistry.info/Elements/e/abstractOfExpression"@en ;
    reg:name "abstractOfExpression"@en ;
    reg:status <http://metadataregistry.org/uri/RegStatus/1001> ;
    rdfs:domain <http://rdaregistry.info/Elements/c/C10006> ;
    rdfs:isDefinedBy <http://rdaregistry.info/Elements/e/> ;
    rdfs:range <http://rdaregistry.info/Elements/c/C10006> ;
    rdfs:subPropertyOf <http://rdaregistry.info/Elements/e/P20204>,
        <http://rdaregistry.info/Elements/u/P60224> ;
    owl:inverseOf <http://rdaregistry.info/Elements/e/P20104> ;
    skos:definition "Relates an expression to an expression of a work that has been abstracted, i.e., abbreviated in a brief, objective manner."@en .

<http://rdaregistry.info/Elements/e/P20123> a rdf:Property ;
    rdfs:label "is dramatization of (expression)"@en ;
    reg:hasUnconstrained <http://rdaregistry.info/Elements/u/P60225> ;
    reg:lexicalAlias "http://rdaregistry.info/Elements/e/dramatizationOfExpression"@en ;
    reg:name "dramatizationOfExpression"@en ;
    reg:status <http://metadataregistry.org/uri/RegStatus/1001> ;
    rdfs:domain <http://rdaregistry.info/Elements/c/C10006> ;
    rdfs:isDefinedBy <http://rdaregistry.info/Elements/e/> ;
    rdfs:range <http://rdaregistry.info/Elements/c/C10006> ;
    rdfs:subPropertyOf <http://rdaregistry.info/Elements/e/P20152>,
        <http://rdaregistry.info/Elements/u/P60225> ;
    owl:inverseOf <http://rdaregistry.info/Elements/e/P20073> ;
    skos:definition "Relates an expression to an expression of a work that has been adapted as a drama."@en .

<http://rdaregistry.info/Elements/e/P20124> a rdf:Property ;
    rdfs:label "is verse adaptation of (expression)"@en ;
    reg:hasUnconstrained <http://rdaregistry.info/Elements/u/P60226> ;
    reg:lexicalAlias "http://rdaregistry.info/Elements/e/verseAdaptationOfExpression"@en ;
    reg:name "verseAdaptationOfExpression"@en ;
    reg:status <http://metadataregistry.org/uri/RegStatus/1001> ;
    rdfs:domain <http://rdaregistry.info/Elements/c/C10006> ;
    rdfs:isDefinedBy <http://rdaregistry.info/Elements/e/> ;
    rdfs:range <http://rdaregistry.info/Elements/c/C10006> ;
    rdfs:subPropertyOf <http://rdaregistry.info/Elements/e/P20152>,
        <http://rdaregistry.info/Elements/u/P60226> ;
    owl:inverseOf <http://rdaregistry.info/Elements/e/P20077> ;
    skos:definition "Relates an expression to an expression of a work that has been adapted as a literary composition in verse form."@en .

<http://rdaregistry.info/Elements/e/P20125> a rdf:Property ;
    rdfs:label "is motion picture adaptation of (expression)"@en ;
    reg:hasUnconstrained <http://rdaregistry.info/Elements/u/P60227> ;
    reg:lexicalAlias "http://rdaregistry.info/Elements/e/motionPictureAdaptationOfExpression"@en ;
    reg:name "motionPictureAdaptationOfExpression"@en ;
    reg:status <http://metadataregistry.org/uri/RegStatus/1001> ;
    rdfs:domain <http://rdaregistry.info/Elements/c/C10006> ;
    rdfs:isDefinedBy <http://rdaregistry.info/Elements/e/> ;
    rdfs:range <http://rdaregistry.info/Elements/c/C10006> ;
    rdfs:subPropertyOf <http://rdaregistry.info/Elements/e/P20152>,
        <http://rdaregistry.info/Elements/u/P60227> ;
    owl:inverseOf <http://rdaregistry.info/Elements/e/P20009> ;
    skos:definition "Relates an expression to an expression of a work that has been adapted as a motion picture."@en .

<http://rdaregistry.info/Elements/e/P20126> a rdf:Property ;
    rdfs:label "is novelization of (expression)"@en ;
    reg:hasUnconstrained <http://rdaregistry.info/Elements/u/P60228> ;
    reg:lexicalAlias "http://rdaregistry.info/Elements/e/novelizationOfExpression"@en ;
    reg:name "novelizationOfExpression"@en ;
    reg:status <http://metadataregistry.org/uri/RegStatus/1001> ;
    rdfs:domain <http://rdaregistry.info/Elements/c/C10006> ;
    rdfs:isDefinedBy <http://rdaregistry.info/Elements/e/> ;
    rdfs:range <http://rdaregistry.info/Elements/c/C10006> ;
    rdfs:subPropertyOf <http://rdaregistry.info/Elements/e/P20152>,
        <http://rdaregistry.info/Elements/u/P60228> ;
    owl:inverseOf <http://rdaregistry.info/Elements/e/P20088> ;
    skos:definition "Relates an expression to an expression of a work that has been adapted as a novel."@en .

<http://rdaregistry.info/Elements/e/P20127> a rdf:Property ;
    rdfs:label "is radio adaptation of (expression)"@en ;
    reg:hasUnconstrained <http://rdaregistry.info/Elements/u/P60229> ;
    reg:lexicalAlias "http://rdaregistry.info/Elements/e/radioAdaptationOfExpression"@en ;
    reg:name "radioAdaptationOfExpression"@en ;
    reg:status <http://metadataregistry.org/uri/RegStatus/1001> ;
    rdfs:domain <http://rdaregistry.info/Elements/c/C10006> ;
    rdfs:isDefinedBy <http://rdaregistry.info/Elements/e/> ;
    rdfs:range <http://rdaregistry.info/Elements/c/C10006> ;
    rdfs:subPropertyOf <http://rdaregistry.info/Elements/e/P20152>,
        <http://rdaregistry.info/Elements/u/P60229> ;
    owl:inverseOf <http://rdaregistry.info/Elements/e/P20060> ;
    skos:definition "Relates an expression to an expression of a work that has been adapted as a radio program."@en .

<http://rdaregistry.info/Elements/e/P20128> a rdf:Property ;
    rdfs:label "is television adaptation of (expression)"@en ;
    reg:hasUnconstrained <http://rdaregistry.info/Elements/u/P60230> ;
    reg:lexicalAlias "http://rdaregistry.info/Elements/e/televisionAdaptationOfExpression"@en ;
    reg:name "televisionAdaptationOfExpression"@en ;
    reg:status <http://metadataregistry.org/uri/RegStatus/1001> ;
    rdfs:domain <http://rdaregistry.info/Elements/c/C10006> ;
    rdfs:isDefinedBy <http://rdaregistry.info/Elements/e/> ;
    rdfs:range <http://rdaregistry.info/Elements/c/C10006> ;
    rdfs:subPropertyOf <http://rdaregistry.info/Elements/e/P20152>,
        <http://rdaregistry.info/Elements/u/P60230> ;
    owl:inverseOf <http://rdaregistry.info/Elements/e/P20066> ;
    skos:definition "Relates an expression to an expression of a work that has been adapted as a television program."@en .

<http://rdaregistry.info/Elements/e/P20130> a rdf:Property ;
    rdfs:label "is motion picture screenplay based on (expression)"@en ;
    reg:hasUnconstrained <http://rdaregistry.info/Elements/u/P60232> ;
    reg:lexicalAlias "http://rdaregistry.info/Elements/e/motionPictureScreenplayBasedOnExpression"@en ;
    reg:name "motionPictureScreenplayBasedOnExpression"@en ;
    reg:status <http://metadataregistry.org/uri/RegStatus/1001> ;
    rdfs:domain <http://rdaregistry.info/Elements/c/C10006> ;
    rdfs:isDefinedBy <http://rdaregistry.info/Elements/e/> ;
    rdfs:range <http://rdaregistry.info/Elements/c/C10006> ;
    rdfs:subPropertyOf <http://rdaregistry.info/Elements/e/P20129>,
        <http://rdaregistry.info/Elements/u/P60232> ;
    owl:inverseOf <http://rdaregistry.info/Elements/e/P20095> ;
    skos:definition "Relates an expression to an expression of a work that has been adapted as the screenplay for a motion picture."@en .

<http://rdaregistry.info/Elements/e/P20131> a rdf:Property ;
    rdfs:label "is television screenplay based on (expression)"@en ;
    reg:hasUnconstrained <http://rdaregistry.info/Elements/u/P60233> ;
    reg:lexicalAlias "http://rdaregistry.info/Elements/e/televisionScreenplayBasedOnExpression"@en ;
    reg:name "televisionScreenplayBasedOnExpression"@en ;
    reg:status <http://metadataregistry.org/uri/RegStatus/1001> ;
    rdfs:domain <http://rdaregistry.info/Elements/c/C10006> ;
    rdfs:isDefinedBy <http://rdaregistry.info/Elements/e/> ;
    rdfs:range <http://rdaregistry.info/Elements/c/C10006> ;
    rdfs:subPropertyOf <http://rdaregistry.info/Elements/e/P20129>,
        <http://rdaregistry.info/Elements/u/P60233> ;
    owl:inverseOf <http://rdaregistry.info/Elements/e/P20097> ;
    skos:definition "Relates an expression to an expression of a work that has been adapted as the screenplay for a television program."@en .

<http://rdaregistry.info/Elements/e/P20132> a rdf:Property ;
    rdfs:label "is video screenplay based on (expression)"@en ;
    reg:hasUnconstrained <http://rdaregistry.info/Elements/u/P60234> ;
    reg:lexicalAlias "http://rdaregistry.info/Elements/e/videoScreenplayBasedOnExpression"@en ;
    reg:name "videoScreenplayBasedOnExpression"@en ;
    reg:status <http://metadataregistry.org/uri/RegStatus/1001> ;
    rdfs:domain <http://rdaregistry.info/Elements/c/C10006> ;
    rdfs:isDefinedBy <http://rdaregistry.info/Elements/e/> ;
    rdfs:range <http://rdaregistry.info/Elements/c/C10006> ;
    rdfs:subPropertyOf <http://rdaregistry.info/Elements/e/P20129>,
        <http://rdaregistry.info/Elements/u/P60234> ;
    owl:inverseOf <http://rdaregistry.info/Elements/e/P20098> ;
    skos:definition "Relates an expression to an expression of a work that has been adapted as the screenplay for a video."@en .

<http://rdaregistry.info/Elements/e/P20133> a rdf:Property ;
    rdfs:label "is radio script based on (expression)"@en ;
    reg:hasUnconstrained <http://rdaregistry.info/Elements/u/P60235> ;
    reg:lexicalAlias "http://rdaregistry.info/Elements/e/radioScriptBasedOnExpression"@en ;
    reg:name "radioScriptBasedOnExpression"@en ;
    reg:status <http://metadataregistry.org/uri/RegStatus/1001> ;
    rdfs:domain <http://rdaregistry.info/Elements/c/C10006> ;
    rdfs:isDefinedBy <http://rdaregistry.info/Elements/e/> ;
    rdfs:range <http://rdaregistry.info/Elements/c/C10006> ;
    rdfs:subPropertyOf <http://rdaregistry.info/Elements/e/P20152>,
        <http://rdaregistry.info/Elements/u/P60235> ;
    owl:inverseOf <http://rdaregistry.info/Elements/e/P20099> ;
    skos:definition "Relates an expression to an expression of a work that has been adapted as the script for a radio program."@en .

<http://rdaregistry.info/Elements/e/P20134> a rdf:Property ;
    rdfs:label "is video adaptation of (expression)"@en ;
    reg:hasUnconstrained <http://rdaregistry.info/Elements/u/P60236> ;
    reg:lexicalAlias "http://rdaregistry.info/Elements/e/videoAdaptationOfExpression"@en ;
    reg:name "videoAdaptationOfExpression"@en ;
    reg:status <http://metadataregistry.org/uri/RegStatus/1001> ;
    rdfs:domain <http://rdaregistry.info/Elements/c/C10006> ;
    rdfs:isDefinedBy <http://rdaregistry.info/Elements/e/> ;
    rdfs:range <http://rdaregistry.info/Elements/c/C10006> ;
    rdfs:subPropertyOf <http://rdaregistry.info/Elements/e/P20152>,
        <http://rdaregistry.info/Elements/u/P60236> ;
    owl:inverseOf <http://rdaregistry.info/Elements/e/P20067> ;
    skos:definition "Relates an expression to an expression of a work that has been adapted for video."@en .

<http://rdaregistry.info/Elements/e/P20135> a rdf:Property ;
    rdfs:label "is digest of (expression)"@en ;
    reg:hasUnconstrained <http://rdaregistry.info/Elements/u/P60238> ;
    reg:lexicalAlias "http://rdaregistry.info/Elements/e/digestOfExpression"@en ;
    reg:name "digestOfExpression"@en ;
    reg:status <http://metadataregistry.org/uri/RegStatus/1001> ;
    rdfs:domain <http://rdaregistry.info/Elements/c/C10006> ;
    rdfs:isDefinedBy <http://rdaregistry.info/Elements/e/> ;
    rdfs:range <http://rdaregistry.info/Elements/c/C10006> ;
    rdfs:subPropertyOf <http://rdaregistry.info/Elements/e/P20204>,
        <http://rdaregistry.info/Elements/u/P60238> ;
    owl:inverseOf <http://rdaregistry.info/Elements/e/P20170> ;
    skos:definition "Relates an expression to an expression of a work that has been digested, i.e., systematically and comprehensively condensed."@en .

<http://rdaregistry.info/Elements/e/P20136> a rdf:Property ;
    rdfs:label "is analysis of (expression)"@en ;
    reg:name "analysisOfExpression"@en ;
    reg:status <http://metadataregistry.org/uri/RegStatus/1008> ;
    rdfs:domain <http://rdaregistry.info/Elements/c/C10006> ;
    rdfs:isDefinedBy <http://rdaregistry.info/Elements/e/> ;
    rdfs:range <http://rdaregistry.info/Elements/c/C10006> ;
    rdfs:subPropertyOf <http://rdaregistry.info/Elements/e/P20072>,
        <http://rdaregistry.info/Elements/u/P60239> ;
    owl:inverseOf <http://rdaregistry.info/Elements/e/P20117> ;
    = <http://rdaregistry.info/Elements/e/analysisOfExpression> ;
    skos:definition "Relates an expression to an expression of a work that has been examined to identify its components and their relations."@en .

<http://rdaregistry.info/Elements/e/P20137> a rdf:Property ;
    rdfs:label "is absorption of (expression)"@en ;
    reg:hasUnconstrained <http://rdaregistry.info/Elements/u/P60574> ;
    reg:lexicalAlias "http://rdaregistry.info/Elements/e/absorptionOfExpression"@en ;
    reg:name "absorptionOfExpression"@en ;
    reg:status <http://metadataregistry.org/uri/RegStatus/1001> ;
    rdfs:domain <http://rdaregistry.info/Elements/c/C10006> ;
    rdfs:isDefinedBy <http://rdaregistry.info/Elements/e/> ;
    rdfs:range <http://rdaregistry.info/Elements/c/C10006> ;
    rdfs:subPropertyOf <http://rdaregistry.info/Elements/e/P20154>,
        <http://rdaregistry.info/Elements/u/P60574> ;
    owl:inverseOf <http://rdaregistry.info/Elements/e/P20143> ;
    skos:definition "Relates an expression to an expression of a work that has been incorporated into another expression."@en .

<http://rdaregistry.info/Elements/e/P20138> a rdf:Property ;
    rdfs:label "is absorption in part of (expression)"@en ;
    reg:hasUnconstrained <http://rdaregistry.info/Elements/u/P60575> ;
    reg:lexicalAlias "http://rdaregistry.info/Elements/e/absorptionInPartOfExpression"@en ;
    reg:name "absorptionInPartOfExpression"@en ;
    reg:status <http://metadataregistry.org/uri/RegStatus/1001> ;
    rdfs:domain <http://rdaregistry.info/Elements/c/C10006> ;
    rdfs:isDefinedBy <http://rdaregistry.info/Elements/e/> ;
    rdfs:range <http://rdaregistry.info/Elements/c/C10006> ;
    rdfs:subPropertyOf <http://rdaregistry.info/Elements/e/P20154>,
        <http://rdaregistry.info/Elements/u/P60575> ;
    owl:inverseOf <http://rdaregistry.info/Elements/e/P20144> ;
    skos:definition "Relates an expression to an expression of a work that has been partially incorporated into another expression."@en .

<http://rdaregistry.info/Elements/e/P20139> a rdf:Property ;
    rdfs:label "is arrangement of"@en ;
    reg:hasUnconstrained <http://rdaregistry.info/Elements/u/P60242> ;
    reg:lexicalAlias "http://rdaregistry.info/Elements/e/arrangementOf"@en ;
    reg:name "arrangementOf"@en ;
    reg:status <http://metadataregistry.org/uri/RegStatus/1001> ;
    rdfs:domain <http://rdaregistry.info/Elements/c/C10006> ;
    rdfs:isDefinedBy <http://rdaregistry.info/Elements/e/> ;
    rdfs:range <http://rdaregistry.info/Elements/c/C10006> ;
    rdfs:subPropertyOf <http://rdaregistry.info/Elements/e/P20204>,
        <http://rdaregistry.info/Elements/u/P60242> ;
    owl:inverseOf <http://rdaregistry.info/Elements/e/P20165> ;
    skos:definition "Relates an expression to an expression of a musical work that has been rewritten for a medium of performance different from that for which the work was originally intended."@en .

<http://rdaregistry.info/Elements/e/P20140> a rdf:Property ;
    rdfs:label "is free translation of (expression)"@en ;
    reg:hasUnconstrained <http://rdaregistry.info/Elements/u/P60243> ;
    reg:lexicalAlias "http://rdaregistry.info/Elements/e/freeTranslationOfExpression"@en ;
    reg:name "freeTranslationOfExpression"@en ;
    reg:status <http://metadataregistry.org/uri/RegStatus/1001> ;
    rdfs:domain <http://rdaregistry.info/Elements/c/C10006> ;
    rdfs:isDefinedBy <http://rdaregistry.info/Elements/e/> ;
    rdfs:range <http://rdaregistry.info/Elements/c/C10006> ;
    rdfs:subPropertyOf <http://rdaregistry.info/Elements/e/P20204>,
        <http://rdaregistry.info/Elements/u/P60243> ;
    owl:inverseOf <http://rdaregistry.info/Elements/e/P20119> ;
    skos:definition "Relates an expression to an expression of a work that has been translated freely, preserving the spirit of the original, but not its linguistic details."@en .

<http://rdaregistry.info/Elements/e/P20142> a rdf:Property ;
    rdfs:label "is parodied as (expression)"@en ;
    reg:hasUnconstrained <http://rdaregistry.info/Elements/u/P60246> ;
    reg:lexicalAlias "http://rdaregistry.info/Elements/e/parodiedAsExpression"@en ;
    reg:name "parodiedAsExpression"@en ;
    reg:status <http://metadataregistry.org/uri/RegStatus/1001> ;
    rdfs:domain <http://rdaregistry.info/Elements/c/C10006> ;
    rdfs:isDefinedBy <http://rdaregistry.info/Elements/e/> ;
    rdfs:range <http://rdaregistry.info/Elements/c/C10006> ;
    rdfs:subPropertyOf <http://rdaregistry.info/Elements/e/P20114>,
        <http://rdaregistry.info/Elements/u/P60246> ;
    owl:inverseOf <http://rdaregistry.info/Elements/e/P20196> ;
    skos:definition "Relates an expression to an expression of a work that imitates the style or content of the source work for comic effect."@en .

<http://rdaregistry.info/Elements/e/P20143> a rdf:Property ;
    rdfs:label "is absorbed by (expression)"@en ;
    reg:hasUnconstrained <http://rdaregistry.info/Elements/u/P60247> ;
    reg:lexicalAlias "http://rdaregistry.info/Elements/e/absorbedByExpression"@en ;
    reg:name "absorbedByExpression"@en ;
    reg:status <http://metadataregistry.org/uri/RegStatus/1001> ;
    rdfs:domain <http://rdaregistry.info/Elements/c/C10006> ;
    rdfs:isDefinedBy <http://rdaregistry.info/Elements/e/> ;
    rdfs:range <http://rdaregistry.info/Elements/c/C10006> ;
    rdfs:subPropertyOf <http://rdaregistry.info/Elements/e/P20169>,
        <http://rdaregistry.info/Elements/u/P60247> ;
    owl:inverseOf <http://rdaregistry.info/Elements/e/P20137> ;
    skos:definition "Relates an expression to an expression of a work that incorporates another expression."@en .

<http://rdaregistry.info/Elements/e/P20144> a rdf:Property ;
    rdfs:label "is absorbed in part by (expression)"@en ;
    reg:hasUnconstrained <http://rdaregistry.info/Elements/u/P60248> ;
    reg:lexicalAlias "http://rdaregistry.info/Elements/e/absorbedInPartByExpression"@en ;
    reg:name "absorbedInPartByExpression"@en ;
    reg:status <http://metadataregistry.org/uri/RegStatus/1001> ;
    rdfs:domain <http://rdaregistry.info/Elements/c/C10006> ;
    rdfs:isDefinedBy <http://rdaregistry.info/Elements/e/> ;
    rdfs:range <http://rdaregistry.info/Elements/c/C10006> ;
    rdfs:subPropertyOf <http://rdaregistry.info/Elements/e/P20169>,
        <http://rdaregistry.info/Elements/u/P60248> ;
    owl:inverseOf <http://rdaregistry.info/Elements/e/P20138> ;
    skos:definition "Relates an expression to an expression of a work that incorporates part of the content of another expression."@en .

<http://rdaregistry.info/Elements/e/P20145> a rdf:Property ;
    rdfs:label "is container of (expression)"@en ;
    reg:hasUnconstrained <http://rdaregistry.info/Elements/u/P60249> ;
    reg:lexicalAlias "http://rdaregistry.info/Elements/e/containerOfExpression"@en ;
    reg:name "containerOfExpression"@en ;
    reg:status <http://metadataregistry.org/uri/RegStatus/1001> ;
    rdfs:domain <http://rdaregistry.info/Elements/c/C10006> ;
    rdfs:isDefinedBy <http://rdaregistry.info/Elements/e/> ;
    rdfs:range <http://rdaregistry.info/Elements/c/C10006> ;
    rdfs:subPropertyOf <http://rdaregistry.info/Elements/e/P20236>,
        <http://rdaregistry.info/Elements/u/P60249> ;
    owl:inverseOf <http://rdaregistry.info/Elements/e/P20074> ;
    skos:definition "Relates an expression to an expression of a work that is a discrete component of a larger expression."@en .

<http://rdaregistry.info/Elements/e/P20146> a rdf:Property ;
    rdfs:label "is errata to (expression)"@en ;
    reg:hasUnconstrained <http://rdaregistry.info/Elements/u/P60251> ;
    reg:lexicalAlias "http://rdaregistry.info/Elements/e/errataToExpression"@en ;
    reg:name "errataToExpression"@en ;
    reg:status <http://metadataregistry.org/uri/RegStatus/1001> ;
    rdfs:domain <http://rdaregistry.info/Elements/c/C10006> ;
    rdfs:isDefinedBy <http://rdaregistry.info/Elements/e/> ;
    rdfs:range <http://rdaregistry.info/Elements/c/C10006> ;
    rdfs:subPropertyOf <http://rdaregistry.info/Elements/e/P20192>,
        <http://rdaregistry.info/Elements/u/P60251> ;
    owl:inverseOf <http://rdaregistry.info/Elements/e/P20093> ;
    skos:definition "Relates an expression to an expression of a work that is augmented by a list of errors in the predominant work, discovered after publication, with their corrections."@en .

<http://rdaregistry.info/Elements/e/P20147> a rdf:Property ;
    rdfs:label "is guide to (expression)"@en ;
    reg:hasUnconstrained <http://rdaregistry.info/Elements/u/P60252> ;
    reg:lexicalAlias "http://rdaregistry.info/Elements/e/guideToExpression"@en ;
    reg:name "guideToExpression"@en ;
    reg:status <http://metadataregistry.org/uri/RegStatus/1001> ;
    rdfs:domain <http://rdaregistry.info/Elements/c/C10006> ;
    rdfs:isDefinedBy <http://rdaregistry.info/Elements/e/> ;
    rdfs:range <http://rdaregistry.info/Elements/c/C10006> ;
    rdfs:subPropertyOf <http://rdaregistry.info/Elements/e/P20192>,
        <http://rdaregistry.info/Elements/u/P60252> ;
    owl:inverseOf <http://rdaregistry.info/Elements/e/P20120> ;
    skos:definition "Relates an expression to an expression of a work that is augmented by another work consisting of material to help the user of the predominant work, such as notes, learning and study aids, exercises, problems, questions and answers, instructor or student materials, etc."@en .

<http://rdaregistry.info/Elements/e/P20148> a rdf:Property ;
    rdfs:label "is illustrations for (expression)"@en ;
    reg:hasUnconstrained <http://rdaregistry.info/Elements/u/P60254> ;
    reg:lexicalAlias "http://rdaregistry.info/Elements/e/illustrationsForExpression"@en ;
    reg:name "illustrationsForExpression"@en ;
    reg:status <http://metadataregistry.org/uri/RegStatus/1001> ;
    rdfs:domain <http://rdaregistry.info/Elements/c/C10006> ;
    rdfs:isDefinedBy <http://rdaregistry.info/Elements/e/> ;
    rdfs:range <http://rdaregistry.info/Elements/c/C10006> ;
    rdfs:subPropertyOf <http://rdaregistry.info/Elements/e/P20192>,
        <http://rdaregistry.info/Elements/u/P60254> ;
    owl:inverseOf <http://rdaregistry.info/Elements/e/P20094> ;
    skos:definition "Relates an expression to an expression of a work that is augmented by pictorial content designed to explain or decorate it."@en .

<http://rdaregistry.info/Elements/e/P20149> a rdf:Property ;
    rdfs:label "is continuation of (expression)"@en ;
    reg:hasUnconstrained <http://rdaregistry.info/Elements/u/P60576> ;
    reg:lexicalAlias "http://rdaregistry.info/Elements/e/continuationOfExpression"@en ;
    reg:name "continuationOfExpression"@en ;
    reg:status <http://metadataregistry.org/uri/RegStatus/1001> ;
    rdfs:domain <http://rdaregistry.info/Elements/c/C10006> ;
    rdfs:isDefinedBy <http://rdaregistry.info/Elements/e/> ;
    rdfs:range <http://rdaregistry.info/Elements/c/C10006> ;
    rdfs:subPropertyOf <http://rdaregistry.info/Elements/e/P20154>,
        <http://rdaregistry.info/Elements/u/P60576> ;
    owl:inverseOf <http://rdaregistry.info/Elements/e/P20191> ;
    skos:definition "Relates an expression to an expression of a work that is continued by the content of an expression of a later work."@en .

<http://rdaregistry.info/Elements/e/P20150> a rdf:Property ;
    rdfs:label "is evaluation of (expression)"@en ;
    reg:name "evaluationOfExpression"@en ;
    reg:status <http://metadataregistry.org/uri/RegStatus/1008> ;
    rdfs:domain <http://rdaregistry.info/Elements/c/C10006> ;
    rdfs:isDefinedBy <http://rdaregistry.info/Elements/e/> ;
    rdfs:range <http://rdaregistry.info/Elements/c/C10006> ;
    rdfs:subPropertyOf <http://rdaregistry.info/Elements/e/P20072>,
        <http://rdaregistry.info/Elements/u/P60255> ;
    owl:inverseOf <http://rdaregistry.info/Elements/e/P20116> ;
    = <http://rdaregistry.info/Elements/e/evaluationOfExpression> ;
    skos:definition "Relates an expression to an expression of a work that is examined or judged."@en .

<http://rdaregistry.info/Elements/e/P20151> a rdf:Property ;
    rdfs:label "is supplement to (expression)"@en ;
    reg:hasUnconstrained <http://rdaregistry.info/Elements/u/P60259> ;
    reg:lexicalAlias "http://rdaregistry.info/Elements/e/supplementToExpression"@en ;
    reg:name "supplementToExpression"@en ;
    reg:status <http://metadataregistry.org/uri/RegStatus/1001> ;
    rdfs:domain <http://rdaregistry.info/Elements/c/C10006> ;
    rdfs:isDefinedBy <http://rdaregistry.info/Elements/e/> ;
    rdfs:range <http://rdaregistry.info/Elements/c/C10006> ;
    rdfs:subPropertyOf <http://rdaregistry.info/Elements/e/P20192>,
        <http://rdaregistry.info/Elements/u/P60259> ;
    owl:inverseOf <http://rdaregistry.info/Elements/e/P20172> ;
    skos:definition "Relates an expression to an expression of a work that is updated or otherwise complemented by the augmenting expression."@en .

<http://rdaregistry.info/Elements/e/P20155> a rdf:Property ;
    rdfs:label "is finding aid (expression)"@en ;
    reg:hasUnconstrained <http://rdaregistry.info/Elements/u/P60262> ;
    reg:lexicalAlias "http://rdaregistry.info/Elements/e/findingAidExpression"@en ;
    reg:name "findingAidExpression"@en ;
    reg:status <http://metadataregistry.org/uri/RegStatus/1001> ;
    rdfs:domain <http://rdaregistry.info/Elements/c/C10006> ;
    rdfs:isDefinedBy <http://rdaregistry.info/Elements/e/> ;
    rdfs:range <http://rdaregistry.info/Elements/c/C10006> ;
    rdfs:subPropertyOf <http://rdaregistry.info/Elements/e/P20105>,
        <http://rdaregistry.info/Elements/u/P60262> ;
    owl:inverseOf <http://rdaregistry.info/Elements/e/P20197> ;
    skos:definition "Relates an expression to an expression of a work that provides a guide to the organization, arrangement, and contents of an archival collection."@en .

<http://rdaregistry.info/Elements/e/P20156> a rdf:Property ;
    rdfs:label "is index (expression)"@en ;
    reg:hasUnconstrained <http://rdaregistry.info/Elements/u/P60263> ;
    reg:lexicalAlias "http://rdaregistry.info/Elements/e/indexExpression"@en ;
    reg:name "indexExpression"@en ;
    reg:status <http://metadataregistry.org/uri/RegStatus/1001> ;
    rdfs:domain <http://rdaregistry.info/Elements/c/C10006> ;
    rdfs:isDefinedBy <http://rdaregistry.info/Elements/e/> ;
    rdfs:range <http://rdaregistry.info/Elements/c/C10006> ;
    rdfs:subPropertyOf <http://rdaregistry.info/Elements/e/P20105>,
        <http://rdaregistry.info/Elements/u/P60263> ;
    owl:inverseOf <http://rdaregistry.info/Elements/e/P20188> ;
    skos:definition "Relates an expression to an expression of a work that provides a systematic, alphabetical guide to the contents of the predominant expression, usually keyed to page numbers or other reference codes."@en .

<http://rdaregistry.info/Elements/e/P20158> a rdf:Property ;
    rdfs:label "is motion picture screenplay (expression)"@en ;
    reg:hasUnconstrained <http://rdaregistry.info/Elements/u/P60265> ;
    reg:lexicalAlias "http://rdaregistry.info/Elements/e/motionPictureScreenplayExpression"@en ;
    reg:name "motionPictureScreenplayExpression"@en ;
    reg:status <http://metadataregistry.org/uri/RegStatus/1001> ;
    rdfs:domain <http://rdaregistry.info/Elements/c/C10006> ;
    rdfs:isDefinedBy <http://rdaregistry.info/Elements/e/> ;
    rdfs:range <http://rdaregistry.info/Elements/c/C10006> ;
    rdfs:subPropertyOf <http://rdaregistry.info/Elements/e/P20157>,
        <http://rdaregistry.info/Elements/u/P60265> ;
    owl:inverseOf <http://rdaregistry.info/Elements/e/P20173> ;
    skos:definition "Relates an expression to an expression of a work that provides the text for a motion picture."@en .

<http://rdaregistry.info/Elements/e/P20159> a rdf:Property ;
    rdfs:label "is musical setting of (expression)"@en ;
    reg:hasUnconstrained <http://rdaregistry.info/Elements/u/P60266> ;
    reg:lexicalAlias "http://rdaregistry.info/Elements/e/musicalSettingOfExpression"@en ;
    reg:name "musicalSettingOfExpression"@en ;
    reg:status <http://metadataregistry.org/uri/RegStatus/1001> ;
    rdfs:domain <http://rdaregistry.info/Elements/c/C10006> ;
    rdfs:isDefinedBy <http://rdaregistry.info/Elements/e/> ;
    rdfs:range <http://rdaregistry.info/Elements/c/C10006> ;
    rdfs:subPropertyOf <http://rdaregistry.info/Elements/e/P20204>,
        <http://rdaregistry.info/Elements/u/P60266> ;
    owl:inverseOf <http://rdaregistry.info/Elements/e/P20087> ;
    skos:definition "Relates an expression to an expression of a work that provides the text for a non-dramatic musical work, other than an oratorio."@en .

<http://rdaregistry.info/Elements/e/P20160> a rdf:Property ;
    rdfs:label "is radio script (expression)"@en ;
    reg:hasUnconstrained <http://rdaregistry.info/Elements/u/P60267> ;
    reg:lexicalAlias "http://rdaregistry.info/Elements/e/radioScriptExpression"@en ;
    reg:name "radioScriptExpression"@en ;
    reg:status <http://metadataregistry.org/uri/RegStatus/1001> ;
    rdfs:domain <http://rdaregistry.info/Elements/c/C10006> ;
    rdfs:isDefinedBy <http://rdaregistry.info/Elements/e/> ;
    rdfs:range <http://rdaregistry.info/Elements/c/C10006> ;
    rdfs:subPropertyOf <http://rdaregistry.info/Elements/e/P20100>,
        <http://rdaregistry.info/Elements/u/P60267> ;
    owl:inverseOf <http://rdaregistry.info/Elements/e/P20176> ;
    skos:definition "Relates an expression to an expression of a work that provides the text for a radio program."@en .

<http://rdaregistry.info/Elements/e/P20161> a rdf:Property ;
    rdfs:label "is television screenplay (expression)"@en ;
    reg:hasUnconstrained <http://rdaregistry.info/Elements/u/P60268> ;
    reg:lexicalAlias "http://rdaregistry.info/Elements/e/televisionScreenplayExpression"@en ;
    reg:name "televisionScreenplayExpression"@en ;
    reg:status <http://metadataregistry.org/uri/RegStatus/1001> ;
    rdfs:domain <http://rdaregistry.info/Elements/c/C10006> ;
    rdfs:isDefinedBy <http://rdaregistry.info/Elements/e/> ;
    rdfs:range <http://rdaregistry.info/Elements/c/C10006> ;
    rdfs:subPropertyOf <http://rdaregistry.info/Elements/e/P20157>,
        <http://rdaregistry.info/Elements/u/P60268> ;
    owl:inverseOf <http://rdaregistry.info/Elements/e/P20174> ;
    skos:definition "Relates an expression to an expression of a work that provides the text for a television program."@en .

<http://rdaregistry.info/Elements/e/P20162> a rdf:Property ;
    rdfs:label "is video screenplay (expression)"@en ;
    reg:hasUnconstrained <http://rdaregistry.info/Elements/u/P60269> ;
    reg:lexicalAlias "http://rdaregistry.info/Elements/e/videoScreenplayExpression"@en ;
    reg:name "videoScreenplayExpression"@en ;
    reg:status <http://metadataregistry.org/uri/RegStatus/1001> ;
    rdfs:domain <http://rdaregistry.info/Elements/c/C10006> ;
    rdfs:isDefinedBy <http://rdaregistry.info/Elements/e/> ;
    rdfs:range <http://rdaregistry.info/Elements/c/C10006> ;
    rdfs:subPropertyOf <http://rdaregistry.info/Elements/e/P20157>,
        <http://rdaregistry.info/Elements/u/P60269> ;
    owl:inverseOf <http://rdaregistry.info/Elements/e/P20175> ;
    skos:definition "Relates an expression to an expression of a work that provides the text for a video."@en .

<http://rdaregistry.info/Elements/e/P20163> a rdf:Property ;
    rdfs:label "is libretto (expression)"@en ;
    reg:hasUnconstrained <http://rdaregistry.info/Elements/u/P60270> ;
    reg:lexicalAlias "http://rdaregistry.info/Elements/e/librettoExpression"@en ;
    reg:name "librettoExpression"@en ;
    reg:status <http://metadataregistry.org/uri/RegStatus/1001> ;
    rdfs:domain <http://rdaregistry.info/Elements/c/C10006> ;
    rdfs:isDefinedBy <http://rdaregistry.info/Elements/e/> ;
    rdfs:range <http://rdaregistry.info/Elements/c/C10006> ;
    rdfs:subPropertyOf <http://rdaregistry.info/Elements/e/P20100>,
        <http://rdaregistry.info/Elements/u/P60270> ;
    owl:inverseOf <http://rdaregistry.info/Elements/e/P20084> ;
    skos:definition "Relates an expression to an expression of a work that provides the text of an opera or other work for the musical stage, or an oratorio."@en .

<http://rdaregistry.info/Elements/e/P20164> a rdf:Property ;
    rdfs:label "is paraphrased as (expression)"@en ;
    reg:hasUnconstrained <http://rdaregistry.info/Elements/u/P60273> ;
    reg:lexicalAlias "http://rdaregistry.info/Elements/e/paraphrasedAsExpression"@en ;
    reg:name "paraphrasedAsExpression"@en ;
    reg:status <http://metadataregistry.org/uri/RegStatus/1001> ;
    rdfs:domain <http://rdaregistry.info/Elements/c/C10006> ;
    rdfs:isDefinedBy <http://rdaregistry.info/Elements/e/> ;
    rdfs:range <http://rdaregistry.info/Elements/c/C10006> ;
    rdfs:subPropertyOf <http://rdaregistry.info/Elements/e/P20203>,
        <http://rdaregistry.info/Elements/u/P60273> ;
    owl:inverseOf <http://rdaregistry.info/Elements/e/P20186> ;
    skos:definition "Relates an expression to an expression of a work that restates the content of the source work in a different form."@en .

<http://rdaregistry.info/Elements/e/P20165> a rdf:Property ;
    rdfs:label "is arranged as"@en ;
    reg:hasUnconstrained <http://rdaregistry.info/Elements/u/P60274> ;
    reg:lexicalAlias "http://rdaregistry.info/Elements/e/arrangedAs"@en ;
    reg:name "arrangedAs"@en ;
    reg:status <http://metadataregistry.org/uri/RegStatus/1001> ;
    rdfs:domain <http://rdaregistry.info/Elements/c/C10006> ;
    rdfs:isDefinedBy <http://rdaregistry.info/Elements/e/> ;
    rdfs:range <http://rdaregistry.info/Elements/c/C10006> ;
    rdfs:subPropertyOf <http://rdaregistry.info/Elements/e/P20203>,
        <http://rdaregistry.info/Elements/u/P60274> ;
    owl:inverseOf <http://rdaregistry.info/Elements/e/P20139> ;
    skos:definition "Relates an expression to an expression of a musical work that rewrites the source expression for a medium of performance different from that for which the work was originally intended."@en .

<http://rdaregistry.info/Elements/e/P20166> a rdf:Property ;
    rdfs:label "is abridged as (expression)"@en ;
    reg:hasUnconstrained <http://rdaregistry.info/Elements/u/P60275> ;
    reg:lexicalAlias "http://rdaregistry.info/Elements/e/abridgedAsExpression"@en ;
    reg:name "abridgedAsExpression"@en ;
    reg:status <http://metadataregistry.org/uri/RegStatus/1001> ;
    rdfs:domain <http://rdaregistry.info/Elements/c/C10006> ;
    rdfs:isDefinedBy <http://rdaregistry.info/Elements/e/> ;
    rdfs:range <http://rdaregistry.info/Elements/c/C10006> ;
    rdfs:subPropertyOf <http://rdaregistry.info/Elements/e/P20203>,
        <http://rdaregistry.info/Elements/u/P60275> ;
    owl:inverseOf <http://rdaregistry.info/Elements/e/P20121> ;
    skos:definition "Relates an expression to an expression of a work that shortens the source expression without changing the general meaning or manner of presentation."@en .

<http://rdaregistry.info/Elements/e/P20167> a rdf:Property ;
    rdfs:label "is continuation in part of (expression)"@en ;
    reg:hasUnconstrained <http://rdaregistry.info/Elements/u/P60276> ;
    reg:lexicalAlias "http://rdaregistry.info/Elements/e/continuationInPartOfExpression"@en ;
    reg:name "continuationInPartOfExpression"@en ;
    reg:status <http://metadataregistry.org/uri/RegStatus/1001> ;
    rdfs:domain <http://rdaregistry.info/Elements/c/C10006> ;
    rdfs:isDefinedBy <http://rdaregistry.info/Elements/e/> ;
    rdfs:range <http://rdaregistry.info/Elements/c/C10006> ;
    rdfs:subPropertyOf <http://rdaregistry.info/Elements/e/P20154>,
        <http://rdaregistry.info/Elements/u/P60276> ;
    owl:inverseOf <http://rdaregistry.info/Elements/e/P20200> ;
    skos:definition "Relates an expression to an expression of a work that split into two or more separate expressions with new titles."@en .

<http://rdaregistry.info/Elements/e/P20168> a rdf:Property ;
    rdfs:label "is separated from (expression)"@en ;
    reg:hasUnconstrained <http://rdaregistry.info/Elements/u/P60277> ;
    reg:lexicalAlias "http://rdaregistry.info/Elements/e/separatedFromExpression"@en ;
    reg:name "separatedFromExpression"@en ;
    reg:status <http://metadataregistry.org/uri/RegStatus/1001> ;
    rdfs:domain <http://rdaregistry.info/Elements/c/C10006> ;
    rdfs:isDefinedBy <http://rdaregistry.info/Elements/e/> ;
    rdfs:range <http://rdaregistry.info/Elements/c/C10006> ;
    rdfs:subPropertyOf <http://rdaregistry.info/Elements/e/P20154>,
        <http://rdaregistry.info/Elements/u/P60277> ;
    owl:inverseOf <http://rdaregistry.info/Elements/e/P20101> ;
    skos:definition "Relates an expression to an expression of a work that spun off a part of its content to form a new expression."@en .

<http://rdaregistry.info/Elements/e/P20170> a rdf:Property ;
    rdfs:label "is digested as (expression)"@en ;
    reg:hasUnconstrained <http://rdaregistry.info/Elements/u/P60279> ;
    reg:lexicalAlias "http://rdaregistry.info/Elements/e/digestedAsExpression"@en ;
    reg:name "digestedAsExpression"@en ;
    reg:status <http://metadataregistry.org/uri/RegStatus/1001> ;
    rdfs:domain <http://rdaregistry.info/Elements/c/C10006> ;
    rdfs:isDefinedBy <http://rdaregistry.info/Elements/e/> ;
    rdfs:range <http://rdaregistry.info/Elements/c/C10006> ;
    rdfs:subPropertyOf <http://rdaregistry.info/Elements/e/P20203>,
        <http://rdaregistry.info/Elements/u/P60279> ;
    owl:inverseOf <http://rdaregistry.info/Elements/e/P20135> ;
    skos:definition "Relates an expression to an expression of a work that systematically and comprehensively condenses the source expression."@en .

<http://rdaregistry.info/Elements/e/P20172> a rdf:Property ;
    rdfs:label "is supplement (expression)"@en ;
    reg:hasUnconstrained <http://rdaregistry.info/Elements/u/P60281> ;
    reg:lexicalAlias "http://rdaregistry.info/Elements/e/supplementExpression"@en ;
    reg:name "supplementExpression"@en ;
    reg:status <http://metadataregistry.org/uri/RegStatus/1001> ;
    rdfs:domain <http://rdaregistry.info/Elements/c/C10006> ;
    rdfs:isDefinedBy <http://rdaregistry.info/Elements/e/> ;
    rdfs:range <http://rdaregistry.info/Elements/c/C10006> ;
    rdfs:subPropertyOf <http://rdaregistry.info/Elements/e/P20105>,
        <http://rdaregistry.info/Elements/u/P60281> ;
    owl:inverseOf <http://rdaregistry.info/Elements/e/P20151> ;
    skos:definition "Relates an expression to an expression of a work that updates or otherwise complements the predominant expression."@en .

<http://rdaregistry.info/Elements/e/P20173> a rdf:Property ;
    rdfs:label "is screenplay for motion picture (expression)"@en ;
    reg:hasUnconstrained <http://rdaregistry.info/Elements/u/P60282> ;
    reg:lexicalAlias "http://rdaregistry.info/Elements/e/screenplayForMotionPictureExpression"@en ;
    reg:name "screenplayForMotionPictureExpression"@en ;
    reg:status <http://metadataregistry.org/uri/RegStatus/1001> ;
    rdfs:domain <http://rdaregistry.info/Elements/c/C10006> ;
    rdfs:isDefinedBy <http://rdaregistry.info/Elements/e/> ;
    rdfs:range <http://rdaregistry.info/Elements/c/C10006> ;
    rdfs:subPropertyOf <http://rdaregistry.info/Elements/e/P20102>,
        <http://rdaregistry.info/Elements/u/P60282> ;
    owl:inverseOf <http://rdaregistry.info/Elements/e/P20158> ;
    skos:definition "Relates an expression to an expression of a work that uses the text as a screenplay for a motion picture."@en .

<http://rdaregistry.info/Elements/e/P20174> a rdf:Property ;
    rdfs:label "is screenplay for television program (expression)"@en ;
    reg:hasUnconstrained <http://rdaregistry.info/Elements/u/P60283> ;
    reg:lexicalAlias "http://rdaregistry.info/Elements/e/screenplayForTelevisionProgramExpression"@en ;
    reg:name "screenplayForTelevisionProgramExpression"@en ;
    reg:status <http://metadataregistry.org/uri/RegStatus/1001> ;
    rdfs:domain <http://rdaregistry.info/Elements/c/C10006> ;
    rdfs:isDefinedBy <http://rdaregistry.info/Elements/e/> ;
    rdfs:range <http://rdaregistry.info/Elements/c/C10006> ;
    rdfs:subPropertyOf <http://rdaregistry.info/Elements/e/P20102>,
        <http://rdaregistry.info/Elements/u/P60283> ;
    owl:inverseOf <http://rdaregistry.info/Elements/e/P20161> ;
    skos:definition "Relates an expression to an expression of a work that uses the text as a screenplay for a television program."@en .

<http://rdaregistry.info/Elements/e/P20175> a rdf:Property ;
    rdfs:label "is screenplay for video (expression)"@en ;
    reg:hasUnconstrained <http://rdaregistry.info/Elements/u/P60284> ;
    reg:lexicalAlias "http://rdaregistry.info/Elements/e/screenplayForVideoExpression"@en ;
    reg:name "screenplayForVideoExpression"@en ;
    reg:status <http://metadataregistry.org/uri/RegStatus/1001> ;
    rdfs:domain <http://rdaregistry.info/Elements/c/C10006> ;
    rdfs:isDefinedBy <http://rdaregistry.info/Elements/e/> ;
    rdfs:range <http://rdaregistry.info/Elements/c/C10006> ;
    rdfs:subPropertyOf <http://rdaregistry.info/Elements/e/P20102>,
        <http://rdaregistry.info/Elements/u/P60284> ;
    owl:inverseOf <http://rdaregistry.info/Elements/e/P20162> ;
    skos:definition "Relates an expression to an expression of a work that uses the text as a screenplay for a video."@en .

<http://rdaregistry.info/Elements/e/P20176> a rdf:Property ;
    rdfs:label "is script for radio program (expression)"@en ;
    reg:hasUnconstrained <http://rdaregistry.info/Elements/u/P60285> ;
    reg:lexicalAlias "http://rdaregistry.info/Elements/e/scriptForRadioProgramExpression"@en ;
    reg:name "scriptForRadioProgramExpression"@en ;
    reg:status <http://metadataregistry.org/uri/RegStatus/1001> ;
    rdfs:domain <http://rdaregistry.info/Elements/c/C10006> ;
    rdfs:isDefinedBy <http://rdaregistry.info/Elements/e/> ;
    rdfs:range <http://rdaregistry.info/Elements/c/C10006> ;
    rdfs:subPropertyOf <http://rdaregistry.info/Elements/e/P20100>,
        <http://rdaregistry.info/Elements/u/P60285> ;
    owl:inverseOf <http://rdaregistry.info/Elements/e/P20160> ;
    skos:definition "Relates an expression to an expression of a work that uses the text of the source work as the script for a radio program."@en .

<http://rdaregistry.info/Elements/e/P20177> a rdf:Property ;
    rdfs:label "is addenda to (expression)"@en ;
    reg:hasUnconstrained <http://rdaregistry.info/Elements/u/P60286> ;
    reg:lexicalAlias "http://rdaregistry.info/Elements/e/addendaToExpression"@en ;
    reg:name "addendaToExpression"@en ;
    reg:status <http://metadataregistry.org/uri/RegStatus/1001> ;
    rdfs:domain <http://rdaregistry.info/Elements/c/C10006> ;
    rdfs:isDefinedBy <http://rdaregistry.info/Elements/e/> ;
    rdfs:range <http://rdaregistry.info/Elements/c/C10006> ;
    rdfs:subPropertyOf <http://rdaregistry.info/Elements/e/P20192>,
        <http://rdaregistry.info/Elements/u/P60286> ;
    owl:inverseOf <http://rdaregistry.info/Elements/e/P20109> ;
    skos:definition "Relates an expression to an expression of a work to which is added brief additional material, less extensive than a supplement, but essential to the completeness of the content of the work; it is usually added at the end of the content but is sometimes issued separately from it."@en .

<http://rdaregistry.info/Elements/e/P20179> a rdf:Property ;
    rdfs:label "is summary of (expression)"@en ;
    reg:hasUnconstrained <http://rdaregistry.info/Elements/u/P60289> ;
    reg:lexicalAlias "http://rdaregistry.info/Elements/e/summaryOfExpression"@en ;
    reg:name "summaryOfExpression"@en ;
    reg:status <http://metadataregistry.org/uri/RegStatus/1001> ;
    rdfs:domain <http://rdaregistry.info/Elements/c/C10006> ;
    rdfs:isDefinedBy <http://rdaregistry.info/Elements/e/> ;
    rdfs:range <http://rdaregistry.info/Elements/c/C10006> ;
    rdfs:subPropertyOf <http://rdaregistry.info/Elements/e/P20204>,
        <http://rdaregistry.info/Elements/u/P60289> ;
    owl:inverseOf <http://rdaregistry.info/Elements/e/P20106> ;
    skos:definition "Relates an expression to an expression of a work used as the basis for a brief recapitulation of its content."@en .

<http://rdaregistry.info/Elements/e/P20180> a rdf:Property ;
    rdfs:label "is catalogue of (expression)"@en ;
    reg:hasUnconstrained <http://rdaregistry.info/Elements/u/P60290> ;
    reg:lexicalAlias "http://rdaregistry.info/Elements/e/catalogueOfExpression"@en ;
    reg:name "catalogueOfExpression"@en ;
    reg:status <http://metadataregistry.org/uri/RegStatus/1001> ;
    rdfs:domain <http://rdaregistry.info/Elements/c/C10006> ;
    rdfs:isDefinedBy <http://rdaregistry.info/Elements/e/> ;
    rdfs:range <http://rdaregistry.info/Elements/c/C10006> ;
    rdfs:subPropertyOf <http://rdaregistry.info/Elements/e/P20192>,
        <http://rdaregistry.info/Elements/u/P60290> ;
    owl:inverseOf <http://rdaregistry.info/Elements/e/P20107> ;
    skos:definition "Relates an expression to an expression of a work used as the basis for a catalogue, i.e., a complete enumeration of items arranged systematically."@en .

<http://rdaregistry.info/Elements/e/P20181> a rdf:Property ;
    rdfs:label "is concordance to (expression)"@en ;
    reg:hasUnconstrained <http://rdaregistry.info/Elements/u/P60291> ;
    reg:lexicalAlias "http://rdaregistry.info/Elements/e/concordanceToExpression"@en ;
    reg:name "concordanceToExpression"@en ;
    reg:status <http://metadataregistry.org/uri/RegStatus/1001> ;
    rdfs:domain <http://rdaregistry.info/Elements/c/C10006> ;
    rdfs:isDefinedBy <http://rdaregistry.info/Elements/e/> ;
    rdfs:range <http://rdaregistry.info/Elements/c/C10006> ;
    rdfs:subPropertyOf <http://rdaregistry.info/Elements/e/P20192>,
        <http://rdaregistry.info/Elements/u/P60291> ;
    owl:inverseOf <http://rdaregistry.info/Elements/e/P20108> ;
    skos:definition "Relates an expression to an expression of a work used as the basis for a concordance, i.e., an index of all the words in the predominant expression."@en .

<http://rdaregistry.info/Elements/e/P20183> a rdf:Property ;
    rdfs:label "is choreographic adaptation of (expression)"@en ;
    reg:hasUnconstrained <http://rdaregistry.info/Elements/u/P60293> ;
    reg:lexicalAlias "http://rdaregistry.info/Elements/e/choreographicAdaptationOfExpression"@en ;
    reg:name "choreographicAdaptationOfExpression"@en ;
    reg:status <http://metadataregistry.org/uri/RegStatus/1001> ;
    rdfs:domain <http://rdaregistry.info/Elements/c/C10006> ;
    rdfs:isDefinedBy <http://rdaregistry.info/Elements/e/> ;
    rdfs:range <http://rdaregistry.info/Elements/c/C10006> ;
    rdfs:subPropertyOf <http://rdaregistry.info/Elements/e/P20152> ;
    owl:inverseOf <http://rdaregistry.info/Elements/e/P20092> ;
    skos:definition "Relates an expression to an expression of a work that has been adapted as a work consisting of movement (e.g., dance)."@en .

<http://rdaregistry.info/Elements/e/P20184> a rdf:Property ;
    rdfs:label "is expanded version of (expression)"@en ;
    reg:hasUnconstrained <http://rdaregistry.info/Elements/u/P60294> ;
    reg:lexicalAlias "http://rdaregistry.info/Elements/e/expandedVersionOfExpression"@en ;
    reg:name "expandedVersionOfExpression"@en ;
    reg:status <http://metadataregistry.org/uri/RegStatus/1001> ;
    rdfs:domain <http://rdaregistry.info/Elements/c/C10006> ;
    rdfs:isDefinedBy <http://rdaregistry.info/Elements/e/> ;
    rdfs:range <http://rdaregistry.info/Elements/c/C10006> ;
    rdfs:subPropertyOf <http://rdaregistry.info/Elements/e/P20204>,
        <http://rdaregistry.info/Elements/u/P60294> ;
    owl:inverseOf <http://rdaregistry.info/Elements/e/P20115> ;
    skos:definition "Relates an expression to an expression of a work used as the basis for a derivative work that enlarges upon the content of the source work."@en .

<http://rdaregistry.info/Elements/e/P20185> a rdf:Property ;
    rdfs:label "is remake of (expression)"@en ;
    reg:hasUnconstrained <http://rdaregistry.info/Elements/u/P60295> ;
    reg:lexicalAlias "http://rdaregistry.info/Elements/e/remakeOfExpression"@en ;
    reg:name "remakeOfExpression"@en ;
    reg:status <http://metadataregistry.org/uri/RegStatus/1001> ;
    rdfs:domain <http://rdaregistry.info/Elements/c/C10006> ;
    rdfs:isDefinedBy <http://rdaregistry.info/Elements/e/> ;
    rdfs:range <http://rdaregistry.info/Elements/c/C10006> ;
    rdfs:subPropertyOf <http://rdaregistry.info/Elements/e/P20204>,
        <http://rdaregistry.info/Elements/u/P60295> ;
    owl:inverseOf <http://rdaregistry.info/Elements/e/P20086> ;
    skos:definition "Relates an expression to an expression of a work used as the basis for a new motion picture, radio program, television program, or video."@en .

<http://rdaregistry.info/Elements/e/P20186> a rdf:Property ;
    rdfs:label "is paraphrase of (expression)"@en ;
    reg:hasUnconstrained <http://rdaregistry.info/Elements/u/P60296> ;
    reg:lexicalAlias "http://rdaregistry.info/Elements/e/paraphraseOfExpression"@en ;
    reg:name "paraphraseOfExpression"@en ;
    reg:status <http://metadataregistry.org/uri/RegStatus/1001> ;
    rdfs:domain <http://rdaregistry.info/Elements/c/C10006> ;
    rdfs:isDefinedBy <http://rdaregistry.info/Elements/e/> ;
    rdfs:range <http://rdaregistry.info/Elements/c/C10006> ;
    rdfs:subPropertyOf <http://rdaregistry.info/Elements/e/P20204>,
        <http://rdaregistry.info/Elements/u/P60296> ;
    owl:inverseOf <http://rdaregistry.info/Elements/e/P20164> ;
    skos:definition "Relates an expression to an expression of a work used as the basis for a paraphrase, i.e., a restating of the content of the source work in a different form."@en .

<http://rdaregistry.info/Elements/e/P20188> a rdf:Property ;
    rdfs:label "is index to (expression)"@en ;
    reg:hasUnconstrained <http://rdaregistry.info/Elements/u/P60302> ;
    reg:lexicalAlias "http://rdaregistry.info/Elements/e/indexToExpression"@en ;
    reg:name "indexToExpression"@en ;
    reg:status <http://metadataregistry.org/uri/RegStatus/1001> ;
    rdfs:domain <http://rdaregistry.info/Elements/c/C10006> ;
    rdfs:isDefinedBy <http://rdaregistry.info/Elements/e/> ;
    rdfs:range <http://rdaregistry.info/Elements/c/C10006> ;
    rdfs:subPropertyOf <http://rdaregistry.info/Elements/e/P20192>,
        <http://rdaregistry.info/Elements/u/P60302> ;
    owl:inverseOf <http://rdaregistry.info/Elements/e/P20156> ;
    skos:definition "Relates an expression to an expression of a work used as the basis for an index, i.e., a systematic, alphabetical guide to the contents of the predominant expression, usually keyed to page numbers or other reference codes."@en .

<http://rdaregistry.info/Elements/e/P20189> a rdf:Property ;
    rdfs:label "is revision of"@en ;
    reg:hasUnconstrained <http://rdaregistry.info/Elements/u/P60303> ;
    reg:lexicalAlias "http://rdaregistry.info/Elements/e/revisionOf"@en ;
    reg:name "revisionOf"@en ;
    reg:status <http://metadataregistry.org/uri/RegStatus/1001> ;
    rdfs:domain <http://rdaregistry.info/Elements/c/C10006> ;
    rdfs:isDefinedBy <http://rdaregistry.info/Elements/e/> ;
    rdfs:range <http://rdaregistry.info/Elements/c/C10006> ;
    rdfs:subPropertyOf <http://rdaregistry.info/Elements/e/P20204>,
        <http://rdaregistry.info/Elements/u/P60303> ;
    owl:inverseOf <http://rdaregistry.info/Elements/e/P20211> ;
    skos:definition "Relates an expression to an expression of a work used as the basis for an updated, corrected, or expanded version."@en .

<http://rdaregistry.info/Elements/e/P20190> a rdf:Property ;
    rdfs:label "is libretto based on (expression)"@en ;
    reg:hasUnconstrained <http://rdaregistry.info/Elements/u/P60304> ;
    reg:lexicalAlias "http://rdaregistry.info/Elements/e/librettoBasedOnExpression"@en ;
    reg:name "librettoBasedOnExpression"@en ;
    reg:status <http://metadataregistry.org/uri/RegStatus/1001> ;
    rdfs:domain <http://rdaregistry.info/Elements/c/C10006> ;
    rdfs:isDefinedBy <http://rdaregistry.info/Elements/e/> ;
    rdfs:range <http://rdaregistry.info/Elements/c/C10006> ;
    rdfs:subPropertyOf <http://rdaregistry.info/Elements/e/P20152> ;
    owl:inverseOf <http://rdaregistry.info/Elements/e/P20110> ;
    skos:definition "Relates an expression to an expression of a work used as the basis for the text of an opera or other work for the musical stage, or an oratorio."@en .

<http://rdaregistry.info/Elements/e/P20191> a rdf:Property ;
    rdfs:label "is continued by (expression)"@en ;
    reg:hasUnconstrained <http://rdaregistry.info/Elements/u/P60306> ;
    reg:lexicalAlias "http://rdaregistry.info/Elements/e/continuedByExpression"@en ;
    reg:name "continuedByExpression"@en ;
    reg:status <http://metadataregistry.org/uri/RegStatus/1001> ;
    rdfs:domain <http://rdaregistry.info/Elements/c/C10006> ;
    rdfs:isDefinedBy <http://rdaregistry.info/Elements/e/> ;
    rdfs:range <http://rdaregistry.info/Elements/c/C10006> ;
    rdfs:subPropertyOf <http://rdaregistry.info/Elements/e/P20169>,
        <http://rdaregistry.info/Elements/u/P60306> ;
    owl:inverseOf <http://rdaregistry.info/Elements/e/P20149> ;
    skos:definition "Relates an expression to an expression of a work whose content continues an expression of an earlier work."@en .

<http://rdaregistry.info/Elements/e/P20193> a rdf:Property ;
    rdfs:label "is abstracts for (expression)"@en ;
    reg:hasUnconstrained <http://rdaregistry.info/Elements/u/P60308> ;
    reg:lexicalAlias "http://rdaregistry.info/Elements/e/abstractsForExpression"@en ;
    reg:name "abstractsForExpression"@en ;
    reg:status <http://metadataregistry.org/uri/RegStatus/1001> ;
    rdfs:domain <http://rdaregistry.info/Elements/c/C10006> ;
    rdfs:isDefinedBy <http://rdaregistry.info/Elements/e/> ;
    rdfs:range <http://rdaregistry.info/Elements/c/C10006> ;
    rdfs:subPropertyOf <http://rdaregistry.info/Elements/e/P20204>,
        <http://rdaregistry.info/Elements/u/P60308> ;
    owl:inverseOf <http://rdaregistry.info/Elements/e/P20090> ;
    skos:definition "Relates an expression to an expression of a work whose contents have been abstracted by an abstracting and indexing service."@en .

<http://rdaregistry.info/Elements/e/P20194> a rdf:Property ;
    rdfs:label "is indexing for (expression)"@en ;
    reg:hasUnconstrained <http://rdaregistry.info/Elements/u/P60309> ;
    reg:lexicalAlias "http://rdaregistry.info/Elements/e/indexingForExpression"@en ;
    reg:name "indexingForExpression"@en ;
    reg:status <http://metadataregistry.org/uri/RegStatus/1001> ;
    rdfs:domain <http://rdaregistry.info/Elements/c/C10006> ;
    rdfs:isDefinedBy <http://rdaregistry.info/Elements/e/> ;
    rdfs:range <http://rdaregistry.info/Elements/c/C10006> ;
    rdfs:subPropertyOf <http://rdaregistry.info/Elements/e/P20204>,
        <http://rdaregistry.info/Elements/u/P60309> ;
    owl:inverseOf <http://rdaregistry.info/Elements/e/P20091> ;
    skos:definition "Relates an expression to an expression of a work whose contents have been indexed by an abstracting and indexing service."@en .

<http://rdaregistry.info/Elements/e/P20196> a rdf:Property ;
    rdfs:label "is parody of (expression)"@en ;
    reg:hasUnconstrained <http://rdaregistry.info/Elements/u/P60312> ;
    reg:lexicalAlias "http://rdaregistry.info/Elements/e/parodyOfExpression"@en ;
    reg:name "parodyOfExpression"@en ;
    reg:status <http://metadataregistry.org/uri/RegStatus/1001> ;
    rdfs:domain <http://rdaregistry.info/Elements/c/C10006> ;
    rdfs:isDefinedBy <http://rdaregistry.info/Elements/e/> ;
    rdfs:range <http://rdaregistry.info/Elements/c/C10006> ;
    rdfs:subPropertyOf <http://rdaregistry.info/Elements/e/P20195>,
        <http://rdaregistry.info/Elements/u/P60312> ;
    owl:inverseOf <http://rdaregistry.info/Elements/e/P20142> ;
    skos:definition "Relates an expression to an expression of a work whose style or content is imitated for comic effect."@en .

<http://rdaregistry.info/Elements/e/P20197> a rdf:Property ;
    rdfs:label "is finding aid for (expression)"@en ;
    reg:hasUnconstrained <http://rdaregistry.info/Elements/u/P60474> ;
    reg:lexicalAlias "http://rdaregistry.info/Elements/e/findingAidForExpression"@en ;
    reg:name "findingAidForExpression"@en ;
    reg:status <http://metadataregistry.org/uri/RegStatus/1001> ;
    rdfs:domain <http://rdaregistry.info/Elements/c/C10006> ;
    rdfs:isDefinedBy <http://rdaregistry.info/Elements/e/> ;
    rdfs:range <http://rdaregistry.info/Elements/c/C10006> ;
    rdfs:subPropertyOf <http://rdaregistry.info/Elements/e/P20192>,
        <http://rdaregistry.info/Elements/u/P60474> ;
    owl:inverseOf <http://rdaregistry.info/Elements/e/P20155> ;
    skos:definition "Relates an expression to an expression of an archival collection that is described in a finding aid, i.e., a guide to the organization, arrangement, and contents of the collection."@en .

<http://rdaregistry.info/Elements/e/P20198> a rdf:Property ;
    rdfs:label "is replacement in part of (expression)"@en ;
    reg:hasUnconstrained <http://rdaregistry.info/Elements/u/P60479> ;
    reg:lexicalAlias "http://rdaregistry.info/Elements/e/replacementInPartOfExpression"@en ;
    reg:name "replacementInPartOfExpression"@en ;
    reg:status <http://metadataregistry.org/uri/RegStatus/1001> ;
    rdfs:domain <http://rdaregistry.info/Elements/c/C10006> ;
    rdfs:isDefinedBy <http://rdaregistry.info/Elements/e/> ;
    rdfs:range <http://rdaregistry.info/Elements/c/C10006> ;
    rdfs:subPropertyOf <http://rdaregistry.info/Elements/e/P20154>,
        <http://rdaregistry.info/Elements/u/P60479> ;
    owl:inverseOf <http://rdaregistry.info/Elements/e/P20075> ;
    skos:definition "Relates an expression to an expression of an earlier work whose content has been partially replaced by a later expression, usually because the later work contains updated or new information that makes the earlier expression obsolete."@en .

<http://rdaregistry.info/Elements/e/P20199> a rdf:Property ;
    rdfs:label "is replacement of (expression)"@en ;
    reg:hasUnconstrained <http://rdaregistry.info/Elements/u/P60480> ;
    reg:lexicalAlias "http://rdaregistry.info/Elements/e/replacementOfExpression"@en ;
    reg:name "replacementOfExpression"@en ;
    reg:status <http://metadataregistry.org/uri/RegStatus/1001> ;
    rdfs:domain <http://rdaregistry.info/Elements/c/C10006> ;
    rdfs:isDefinedBy <http://rdaregistry.info/Elements/e/> ;
    rdfs:range <http://rdaregistry.info/Elements/c/C10006> ;
    rdfs:subPropertyOf <http://rdaregistry.info/Elements/e/P20154>,
        <http://rdaregistry.info/Elements/u/P60480> ;
    owl:inverseOf <http://rdaregistry.info/Elements/e/P20076> ;
    skos:definition "Relates an expression to an expression of an earlier work whose content has been replaced by a later expression, usually because the later work contains updated or new information that makes the earlier expression obsolete."@en .

<http://rdaregistry.info/Elements/e/P20200> a rdf:Property ;
    rdfs:label "is split into (expression)"@en ;
    reg:hasUnconstrained <http://rdaregistry.info/Elements/u/P60503> ;
    reg:lexicalAlias "http://rdaregistry.info/Elements/e/splitIntoExpression"@en ;
    reg:name "splitIntoExpression"@en ;
    reg:status <http://metadataregistry.org/uri/RegStatus/1001> ;
    rdfs:domain <http://rdaregistry.info/Elements/c/C10006> ;
    rdfs:isDefinedBy <http://rdaregistry.info/Elements/e/> ;
    rdfs:range <http://rdaregistry.info/Elements/c/C10006> ;
    rdfs:subPropertyOf <http://rdaregistry.info/Elements/e/P20169>,
        <http://rdaregistry.info/Elements/u/P60503> ;
    owl:inverseOf <http://rdaregistry.info/Elements/e/P20167> ;
    skos:definition "Relates an expression to an expression of one of two or more works resulting from the division of an earlier expression into separate expressions."@en .

<http://rdaregistry.info/Elements/e/P20201> a rdf:Property ;
    rdfs:label "is merger of (expression)"@en ;
    reg:hasUnconstrained <http://rdaregistry.info/Elements/u/P60505> ;
    reg:lexicalAlias "http://rdaregistry.info/Elements/e/mergerOfExpression"@en ;
    reg:name "mergerOfExpression"@en ;
    reg:status <http://metadataregistry.org/uri/RegStatus/1001> ;
    rdfs:domain <http://rdaregistry.info/Elements/c/C10006> ;
    rdfs:isDefinedBy <http://rdaregistry.info/Elements/e/> ;
    rdfs:range <http://rdaregistry.info/Elements/c/C10006> ;
    rdfs:subPropertyOf <http://rdaregistry.info/Elements/e/P20154>,
        <http://rdaregistry.info/Elements/u/P60505> ;
    owl:inverseOf <http://rdaregistry.info/Elements/e/P20212> ;
    skos:definition "Relates an expression to an expression of a work that came together with one or more other expressions to form the new expression."@en .

<http://rdaregistry.info/Elements/e/P20211> a rdf:Property ;
    rdfs:label "is revised as"@en ;
    reg:hasUnconstrained <http://rdaregistry.info/Elements/u/P60245> ;
    reg:lexicalAlias "http://rdaregistry.info/Elements/e/revisedAs"@en ;
    reg:name "revisedAs"@en ;
    reg:status <http://metadataregistry.org/uri/RegStatus/1001> ;
    rdfs:domain <http://rdaregistry.info/Elements/c/C10006> ;
    rdfs:isDefinedBy <http://rdaregistry.info/Elements/e/> ;
    rdfs:range <http://rdaregistry.info/Elements/c/C10006> ;
    rdfs:subPropertyOf <http://rdaregistry.info/Elements/e/P20203>,
        <http://rdaregistry.info/Elements/u/P60245> ;
    owl:inverseOf <http://rdaregistry.info/Elements/e/P20189> ;
    skos:definition "Relates an expression to an expression of a work that has been updated, corrected, or expanded."@en .

<http://rdaregistry.info/Elements/e/P20253> a rdf:Property ;
    rdfs:label "is choreography (expression)"@en ;
    reg:hasUnconstrained <http://rdaregistry.info/Elements/u/P60740> ;
    reg:lexicalAlias "http://rdaregistry.info/Elements/e/choreographyExpression"@en ;
    reg:name "choreographyExpression"@en ;
    reg:status <http://metadataregistry.org/uri/RegStatus/1001> ;
    rdfs:domain <http://rdaregistry.info/Elements/c/C10006> ;
    rdfs:isDefinedBy <http://rdaregistry.info/Elements/e/> ;
    rdfs:range <http://rdaregistry.info/Elements/c/C10006> ;
    rdfs:subPropertyOf <http://rdaregistry.info/Elements/e/P20100> ;
    owl:inverseOf <http://rdaregistry.info/Elements/e/P20254> ;
    skos:definition "Relates an expression to an expression of a work that provides the choreography for use in the related expression."@en .

<http://rdaregistry.info/Elements/e/P20254> a rdf:Property ;
    rdfs:label "is choreography for (expression)"@en ;
    reg:hasUnconstrained <http://rdaregistry.info/Elements/u/P60741> ;
    reg:lexicalAlias "http://rdaregistry.info/Elements/e/choreographyForExpression"@en ;
    reg:name "choreographyForExpression"@en ;
    reg:status <http://metadataregistry.org/uri/RegStatus/1001> ;
    rdfs:domain <http://rdaregistry.info/Elements/c/C10006> ;
    rdfs:isDefinedBy <http://rdaregistry.info/Elements/e/> ;
    rdfs:range <http://rdaregistry.info/Elements/c/C10006> ;
    rdfs:subPropertyOf <http://rdaregistry.info/Elements/e/P20100> ;
    owl:inverseOf <http://rdaregistry.info/Elements/e/P20253> ;
    skos:definition "Relates an expression to an expression of a work that uses the choreography of the related expression. "@en .

<http://rdaregistry.info/Elements/e/P20255> a rdf:Property ;
    rdfs:label "is adapted as graphic novel (expression)"@en ;
    reg:hasUnconstrained <http://rdaregistry.info/Elements/u/P60742> ;
    reg:lexicalAlias "http://rdaregistry.info/Elements/e/adaptedAsGraphicNovelExpression"@en ;
    reg:name "adaptedAsGraphicNovelExpression"@en ;
    reg:status <http://metadataregistry.org/uri/RegStatus/1001> ;
    rdfs:domain <http://rdaregistry.info/Elements/c/C10006> ;
    rdfs:isDefinedBy <http://rdaregistry.info/Elements/e/> ;
    rdfs:range <http://rdaregistry.info/Elements/c/C10006> ;
    rdfs:subPropertyOf <http://rdaregistry.info/Elements/e/P20153> ;
    owl:inverseOf <http://rdaregistry.info/Elements/e/P20256> ;
    skos:definition "Relates an expression to a graphic novel based on the source expression."@en .

<http://rdaregistry.info/Elements/e/P20256> a rdf:Property ;
    rdfs:label "is graphic novelization of (expression)"@en ;
    reg:hasUnconstrained <http://rdaregistry.info/Elements/u/P60743> ;
    reg:lexicalAlias "http://rdaregistry.info/Elements/e/graphicNovelizationOfExpression"@en ;
    reg:name "graphicNovelizationOfExpression"@en ;
    reg:status <http://metadataregistry.org/uri/RegStatus/1001> ;
    rdfs:domain <http://rdaregistry.info/Elements/c/C10006> ;
    rdfs:isDefinedBy <http://rdaregistry.info/Elements/e/> ;
    rdfs:range <http://rdaregistry.info/Elements/c/C10006> ;
    rdfs:subPropertyOf <http://rdaregistry.info/Elements/e/P20152> ;
    owl:inverseOf <http://rdaregistry.info/Elements/e/P20255> ;
    skos:definition "Relates an expression to an expression of a work that has been adapated as a graphic novel."@en .

<http://rdaregistry.info/Elements/e/P20072> a rdf:Property ;
    rdfs:label "is description of (expression)"@en ;
    reg:hasSubproperty <http://rdaregistry.info/Elements/e/P20136>,
        <http://rdaregistry.info/Elements/e/P20150> ;
    reg:name "descriptionOfExpression"@en ;
    reg:status <http://metadataregistry.org/uri/RegStatus/1008> ;
    rdfs:domain <http://rdaregistry.info/Elements/c/C10006> ;
    rdfs:isDefinedBy <http://rdaregistry.info/Elements/e/> ;
    rdfs:range <http://rdaregistry.info/Elements/c/C10006> ;
    rdfs:subPropertyOf <http://rdaregistry.info/Elements/e/P20234>,
        <http://rdaregistry.info/Elements/u/P60190> ;
    = <http://rdaregistry.info/Elements/e/descriptionOfExpression> ;
    skos:definition "Relates an expression to an expression described by an expression of a describing work."@en .

<http://rdaregistry.info/Elements/e/P20114> a rdf:Property ;
    rdfs:label "is imitated as (expression)"@en ;
    reg:hasSubproperty <http://rdaregistry.info/Elements/e/P20142> ;
    reg:hasUnconstrained <http://rdaregistry.info/Elements/u/P60214> ;
    reg:lexicalAlias "http://rdaregistry.info/Elements/e/imitatedAsExpression"@en ;
    reg:name "imitatedAsExpression"@en ;
    reg:status <http://metadataregistry.org/uri/RegStatus/1001> ;
    rdfs:domain <http://rdaregistry.info/Elements/c/C10006> ;
    rdfs:isDefinedBy <http://rdaregistry.info/Elements/e/> ;
    rdfs:range <http://rdaregistry.info/Elements/c/C10006> ;
    rdfs:subPropertyOf <http://rdaregistry.info/Elements/e/P20203>,
        <http://rdaregistry.info/Elements/u/P60214> ;
    owl:inverseOf <http://rdaregistry.info/Elements/e/P20195> ;
    skos:definition "Relates an expression to an expression of a work that copies the style or content of the source work."@en .

<http://rdaregistry.info/Elements/e/P20141> a rdf:Property ;
    rdfs:label "is translation of"@en ;
    reg:hasSubproperty <http://rdaregistry.info/Elements/e/P20078> ;
    reg:hasUnconstrained <http://rdaregistry.info/Elements/u/P60244> ;
    reg:lexicalAlias "http://rdaregistry.info/Elements/e/translationOf"@en ;
    reg:name "translationOf"@en ;
    reg:status <http://metadataregistry.org/uri/RegStatus/1001> ;
    rdfs:domain <http://rdaregistry.info/Elements/c/C10006> ;
    rdfs:isDefinedBy <http://rdaregistry.info/Elements/e/> ;
    rdfs:range <http://rdaregistry.info/Elements/c/C10006> ;
    rdfs:subPropertyOf <http://rdaregistry.info/Elements/e/P20204>,
        <http://rdaregistry.info/Elements/u/P60244> ;
    owl:inverseOf <http://rdaregistry.info/Elements/e/P20171> ;
    skos:definition "Relates an expression to an expression of a work that has been translated, i.e., the text expressed in a language different from that of the original work."@en .

<http://rdaregistry.info/Elements/e/P20171> a rdf:Property ;
    rdfs:label "is translated as"@en ;
    reg:hasSubproperty <http://rdaregistry.info/Elements/e/P20079> ;
    reg:hasUnconstrained <http://rdaregistry.info/Elements/u/P60280> ;
    reg:lexicalAlias "http://rdaregistry.info/Elements/e/translatedAs"@en ;
    reg:name "translatedAs"@en ;
    reg:status <http://metadataregistry.org/uri/RegStatus/1001> ;
    rdfs:domain <http://rdaregistry.info/Elements/c/C10006> ;
    rdfs:isDefinedBy <http://rdaregistry.info/Elements/e/> ;
    rdfs:range <http://rdaregistry.info/Elements/c/C10006> ;
    rdfs:subPropertyOf <http://rdaregistry.info/Elements/e/P20203>,
        <http://rdaregistry.info/Elements/u/P60280> ;
    owl:inverseOf <http://rdaregistry.info/Elements/e/P20141> ;
    skos:definition "Relates an expression to an expression of a work that translates the text of the source expression into a language different from that of the original work."@en .

<http://rdaregistry.info/Elements/e/P20195> a rdf:Property ;
    rdfs:label "is imitation of (expression)"@en ;
    reg:hasSubproperty <http://rdaregistry.info/Elements/e/P20196> ;
    reg:hasUnconstrained <http://rdaregistry.info/Elements/u/P60311> ;
    reg:lexicalAlias "http://rdaregistry.info/Elements/e/imitationOfExpression"@en ;
    reg:name "imitationOfExpression"@en ;
    reg:status <http://metadataregistry.org/uri/RegStatus/1001> ;
    rdfs:domain <http://rdaregistry.info/Elements/c/C10006> ;
    rdfs:isDefinedBy <http://rdaregistry.info/Elements/e/> ;
    rdfs:range <http://rdaregistry.info/Elements/c/C10006> ;
    rdfs:subPropertyOf <http://rdaregistry.info/Elements/e/P20204>,
        <http://rdaregistry.info/Elements/u/P60311> ;
    owl:inverseOf <http://rdaregistry.info/Elements/e/P20114> ;
    skos:definition "Relates an expression to an expression of a work whose style or content is copied in a derivative work."@en .

<http://rdaregistry.info/Elements/e/P20235> a rdf:Property ;
    rdfs:label "has sequential expression relationship with"@en ;
    reg:hasSubproperty <http://rdaregistry.info/Elements/e/P20154>,
        <http://rdaregistry.info/Elements/e/P20169> ;
    reg:hasUnconstrained <http://rdaregistry.info/Elements/u/P60713> ;
    reg:lexicalAlias "http://rdaregistry.info/Elements/e/sequentialExpressionRelationship"@en ;
    reg:name "sequentialExpressionRelationship"@en ;
    reg:status <http://metadataregistry.org/uri/RegStatus/1001> ;
    rdfs:domain <http://rdaregistry.info/Elements/c/C10006> ;
    rdfs:isDefinedBy <http://rdaregistry.info/Elements/e/> ;
    rdfs:range <http://rdaregistry.info/Elements/c/C10006> ;
    rdfs:subPropertyOf <http://rdaregistry.info/Elements/e/P20205>,
        <http://rdaregistry.info/Elements/u/P60713> ;
    skos:definition "Relates an expression to an expression of a work that is preceded by or succeeded by the expression."@en .

<http://rdaregistry.info/Elements/e/P20236> a rdf:Property ;
    rdfs:label "has whole-part expression relationship with"@en ;
    reg:hasSubproperty <http://rdaregistry.info/Elements/e/P20074>,
        <http://rdaregistry.info/Elements/e/P20145> ;
    reg:hasUnconstrained <http://rdaregistry.info/Elements/u/P60714> ;
    reg:lexicalAlias "http://rdaregistry.info/Elements/e/wholePartExpressionRelationship"@en ;
    reg:name "wholePartExpressionRelationship"@en ;
    reg:status <http://metadataregistry.org/uri/RegStatus/1001> ;
    rdfs:domain <http://rdaregistry.info/Elements/c/C10006> ;
    rdfs:isDefinedBy <http://rdaregistry.info/Elements/e/> ;
    rdfs:range <http://rdaregistry.info/Elements/c/C10006> ;
    rdfs:subPropertyOf <http://rdaregistry.info/Elements/e/P20205>,
        <http://rdaregistry.info/Elements/u/P60714> ;
    skos:definition "Relates an expression to an expression that is contained in or contains the expression."@en .

<http://rdaregistry.info/Elements/e/P20062> a rdf:Property ;
    rdfs:label "has form of notation"@en ;
    reg:hasSubproperty <http://rdaregistry.info/Elements/e/P20061>,
        <http://rdaregistry.info/Elements/e/P20063>,
        <http://rdaregistry.info/Elements/e/P20064>,
        <http://rdaregistry.info/Elements/e/P20065> ;
    reg:hasUnconstrained <http://rdaregistry.info/Elements/u/P60319> ;
    reg:lexicalAlias "http://rdaregistry.info/Elements/e/formOfNotation"@en ;
    reg:name "formOfNotation"@en ;
    reg:status <http://metadataregistry.org/uri/RegStatus/1001> ;
    rdfs:domain <http://rdaregistry.info/Elements/c/C10006> ;
    rdfs:isDefinedBy <http://rdaregistry.info/Elements/e/> ;
    skos:definition "Relates an expression to a set of characters and/or symbols used to express the content of a resource."@en .

<http://rdaregistry.info/Elements/e/P20228> a rdf:Property ;
    rdfs:label "has scale"@en ;
    reg:hasSubproperty <http://rdaregistry.info/Elements/e/P20213>,
        <http://rdaregistry.info/Elements/e/P20226>,
        <http://rdaregistry.info/Elements/e/P20227>,
        <http://rdaregistry.info/Elements/e/P20230> ;
    reg:hasUnconstrained <http://rdaregistry.info/Elements/u/P60565> ;
    reg:lexicalAlias "http://rdaregistry.info/Elements/e/scale"@en ;
    reg:name "scale"@en ;
    reg:status <http://metadataregistry.org/uri/RegStatus/1001> ;
    rdfs:domain <http://rdaregistry.info/Elements/c/C10006> ;
    rdfs:isDefinedBy <http://rdaregistry.info/Elements/e/> ;
    skos:definition "Relates an expression to the ratio of the dimensions of an image or three-dimensional form contained or embodied in a resource to the dimensions of the thing it represents."@en ;
    skos:scopeNote "Scale can apply to horizontal, vertical, angular, and/or other measurements represented in the resource."@en .

<http://rdaregistry.info/Elements/e/P20232> a rdf:Property ;
    rdfs:label "has accompanying expression relationship with"@en ;
    reg:hasSubproperty <http://rdaregistry.info/Elements/e/P20100>,
        <http://rdaregistry.info/Elements/e/P20105>,
        <http://rdaregistry.info/Elements/e/P20192> ;
    reg:hasUnconstrained <http://rdaregistry.info/Elements/u/P60709> ;
    reg:lexicalAlias "http://rdaregistry.info/Elements/e/accompanyingExpressionRelationship"@en ;
    reg:name "accompanyingExpressionRelationship"@en ;
    reg:status <http://metadataregistry.org/uri/RegStatus/1001> ;
    rdfs:domain <http://rdaregistry.info/Elements/c/C10006> ;
    rdfs:isDefinedBy <http://rdaregistry.info/Elements/e/> ;
    rdfs:range <http://rdaregistry.info/Elements/c/C10006> ;
    rdfs:subPropertyOf <http://rdaregistry.info/Elements/e/P20205> ;
    owl:inverseOf <http://rdaregistry.info/Elements/e/P20232> ;
    skos:definition "Relates an expression to an expression of a work that is an augmentation of, or is augmented by, or is complemented by the expression."@en .

<http://rdaregistry.info/Elements/e/P20233> a rdf:Property ;
    rdfs:label "has derivative expression relationship with"@en ;
    reg:hasSubproperty <http://rdaregistry.info/Elements/e/P20203> ;
    reg:hasUnconstrained <http://rdaregistry.info/Elements/u/P60710> ;
    reg:lexicalAlias "http://rdaregistry.info/Elements/e/derivativeExpressionRelationship"@en ;
    reg:name "derivativeExpressionRelationship"@en ;
    reg:status <http://metadataregistry.org/uri/RegStatus/1001> ;
    rdfs:domain <http://rdaregistry.info/Elements/c/C10006> ;
    rdfs:isDefinedBy <http://rdaregistry.info/Elements/e/> ;
    rdfs:range <http://rdaregistry.info/Elements/c/C10006> ;
    rdfs:subPropertyOf <http://rdaregistry.info/Elements/e/P20205>,
        <http://rdaregistry.info/Elements/u/P60710> ;
    owl:inverseOf <http://rdaregistry.info/Elements/e/P20233> ;
    skos:definition "Relates an expression to an expression of a work that is based on or is a derivative of the expression."@en .

<http://rdaregistry.info/Elements/e/P20096> a rdf:Property ;
    rdfs:label "is adapted as screenplay (expression)"@en ;
    reg:hasSubproperty <http://rdaregistry.info/Elements/e/P20095>,
        <http://rdaregistry.info/Elements/e/P20097>,
        <http://rdaregistry.info/Elements/e/P20098> ;
    reg:hasUnconstrained <http://rdaregistry.info/Elements/u/P60185> ;
    reg:lexicalAlias "http://rdaregistry.info/Elements/e/adaptedAsScreenplayExpression"@en ;
    reg:name "adaptedAsScreenplayExpression"@en ;
    reg:status <http://metadataregistry.org/uri/RegStatus/1001> ;
    rdfs:domain <http://rdaregistry.info/Elements/c/C10006> ;
    rdfs:isDefinedBy <http://rdaregistry.info/Elements/e/> ;
    rdfs:range <http://rdaregistry.info/Elements/c/C10006> ;
    rdfs:subPropertyOf <http://rdaregistry.info/Elements/e/P20153>,
        <http://rdaregistry.info/Elements/u/P60185> ;
    owl:inverseOf <http://rdaregistry.info/Elements/e/P20129> ;
    skos:definition "Relates an expression to an expression of a work consisting of the screenplay for a motion picture, television program, or video, based on the source work."@en .

<http://rdaregistry.info/Elements/e/P20102> a rdf:Property ;
    rdfs:label "is screenplay for (expression)"@en ;
    reg:hasSubproperty <http://rdaregistry.info/Elements/e/P20173>,
        <http://rdaregistry.info/Elements/e/P20174>,
        <http://rdaregistry.info/Elements/e/P20175> ;
    reg:hasUnconstrained <http://rdaregistry.info/Elements/u/P60201> ;
    reg:lexicalAlias "http://rdaregistry.info/Elements/e/screenplayForExpression"@en ;
    reg:name "screenplayForExpression"@en ;
    reg:status <http://metadataregistry.org/uri/RegStatus/1001> ;
    rdfs:domain <http://rdaregistry.info/Elements/c/C10006> ;
    rdfs:isDefinedBy <http://rdaregistry.info/Elements/e/> ;
    rdfs:range <http://rdaregistry.info/Elements/c/C10006> ;
    rdfs:subPropertyOf <http://rdaregistry.info/Elements/e/P20100>,
        <http://rdaregistry.info/Elements/u/P60201> ;
    owl:inverseOf <http://rdaregistry.info/Elements/e/P20157> ;
    skos:definition "Relates an expression to an expression of a work such as a motion picture, television program, or video, that uses the text of the work as a screenplay."@en .

<http://rdaregistry.info/Elements/e/P20129> a rdf:Property ;
    rdfs:label "is screenplay based on (expression)"@en ;
    reg:hasSubproperty <http://rdaregistry.info/Elements/e/P20130>,
        <http://rdaregistry.info/Elements/e/P20131>,
        <http://rdaregistry.info/Elements/e/P20132> ;
    reg:hasUnconstrained <http://rdaregistry.info/Elements/u/P60231> ;
    reg:lexicalAlias "http://rdaregistry.info/Elements/e/screenplayBasedOnExpression"@en ;
    reg:name "screenplayBasedOnExpression"@en ;
    reg:status <http://metadataregistry.org/uri/RegStatus/1001> ;
    rdfs:domain <http://rdaregistry.info/Elements/c/C10006> ;
    rdfs:isDefinedBy <http://rdaregistry.info/Elements/e/> ;
    rdfs:range <http://rdaregistry.info/Elements/c/C10006> ;
    rdfs:subPropertyOf <http://rdaregistry.info/Elements/e/P20152>,
        <http://rdaregistry.info/Elements/u/P60231> ;
    owl:inverseOf <http://rdaregistry.info/Elements/e/P20096> ;
    skos:definition "Relates an expression to an expression of a work that has been adapted as the screenplay for a motion picture, television program, or video."@en .

<http://rdaregistry.info/Elements/e/P20157> a rdf:Property ;
    rdfs:label "is screenplay (expression)"@en ;
    reg:hasSubproperty <http://rdaregistry.info/Elements/e/P20158>,
        <http://rdaregistry.info/Elements/e/P20161>,
        <http://rdaregistry.info/Elements/e/P20162> ;
    reg:hasUnconstrained <http://rdaregistry.info/Elements/u/P60264> ;
    reg:lexicalAlias "http://rdaregistry.info/Elements/e/screenplayExpression"@en ;
    reg:name "screenplayExpression"@en ;
    reg:status <http://metadataregistry.org/uri/RegStatus/1001> ;
    rdfs:domain <http://rdaregistry.info/Elements/c/C10006> ;
    rdfs:isDefinedBy <http://rdaregistry.info/Elements/e/> ;
    rdfs:range <http://rdaregistry.info/Elements/c/C10006> ;
    rdfs:subPropertyOf <http://rdaregistry.info/Elements/e/P20100>,
        <http://rdaregistry.info/Elements/u/P60264> ;
    owl:inverseOf <http://rdaregistry.info/Elements/e/P20102> ;
    skos:definition "Relates an expression to an expression of a work that provides the text for a motion picture, television program or video."@en .

<http://rdaregistry.info/Elements/e/P20202> a rdf:Property ;
    reg:hasSubproperty <http://rdaregistry.info/Elements/e/P20111>,
        <http://rdaregistry.info/Elements/e/P20112>,
        <http://rdaregistry.info/Elements/e/P20113>,
        <http://rdaregistry.info/Elements/e/P20116>,
        <http://rdaregistry.info/Elements/e/P20117> ;
    reg:status <http://metadataregistry.org/uri/RegStatus/1001> ;
    rdfs:isDefinedBy <http://rdaregistry.info/Elements/e/> .

<http://rdaregistry.info/Elements/e/P20205> a rdf:Property ;
    rdfs:label "has related expression"@en ;
    reg:hasSubproperty <http://rdaregistry.info/Elements/e/P20233>,
        <http://rdaregistry.info/Elements/e/P20235>,
        <http://rdaregistry.info/Elements/e/P20236> ;
    reg:hasUnconstrained <http://rdaregistry.info/Elements/u/P60313> ;
    reg:lexicalAlias "http://rdaregistry.info/Elements/e/relatedExpression"@en ;
    reg:name "relatedExpression"@en ;
    reg:status <http://metadataregistry.org/uri/RegStatus/1001> ;
    rdfs:domain <http://rdaregistry.info/Elements/c/C10006> ;
    rdfs:isDefinedBy <http://rdaregistry.info/Elements/e/> ;
    rdfs:range <http://rdaregistry.info/Elements/c/C10006> ;
    owl:inverseOf <http://rdaregistry.info/Elements/e/P20205> ;
    skos:definition "Relates an expression to an expression, represented by an identifier, an authorized access point, or a description, that is related to the expression being described (e.g., a revised version, a translation)."@en .

<http://rdaregistry.info/Elements/e/P20243> a rdf:Property ;
    rdfs:label "is music (expression)"@en ;
    reg:hasUnconstrained <http://rdaregistry.info/Elements/u/P60723> ;
    reg:lexicalAlias "http://rdaregistry.info/Elements/e/musicExpression"@en ;
    reg:name "musicExpression"@en ;
    reg:status <http://metadataregistry.org/uri/RegStatus/1001> ;
    rdfs:domain <http://rdaregistry.info/Elements/c/C10006> ;
    rdfs:isDefinedBy <http://rdaregistry.info/Elements/e/> ;
    rdfs:range <http://rdaregistry.info/Elements/c/C10006> ;
    rdfs:subPropertyOf <http://rdaregistry.info/Elements/e/P20100>,
        <http://rdaregistry.info/Elements/u/P60723> ;
    owl:inverseOf <http://rdaregistry.info/Elements/e/P20244> ;
    skos:definition "Relates an expression to an expression of a musical work that is used in a motion picture, play, television program, etc."@en .

<http://rdaregistry.info/Elements/e/P20244> a rdf:Property ;
    rdfs:label "is music for (expression)"@en ;
    reg:hasUnconstrained <http://rdaregistry.info/Elements/u/P60724> ;
    reg:lexicalAlias "http://rdaregistry.info/Elements/e/musicForExpression"@en ;
    reg:name "musicForExpression"@en ;
    reg:status <http://metadataregistry.org/uri/RegStatus/1001> ;
    rdfs:domain <http://rdaregistry.info/Elements/c/C10006> ;
    rdfs:isDefinedBy <http://rdaregistry.info/Elements/e/> ;
    rdfs:range <http://rdaregistry.info/Elements/c/C10006> ;
    rdfs:subPropertyOf <http://rdaregistry.info/Elements/e/P20100>,
        <http://rdaregistry.info/Elements/u/P60724> ;
    owl:inverseOf <http://rdaregistry.info/Elements/e/P20243> ;
    skos:definition "Relates an expression to an expression of a work such as a motion picture, play, television program, etc. that uses the musical work."@en .

<http://rdaregistry.info/Elements/e/P20269> a rdf:Property ;
    rdfs:label "is described in (expression)"@en ;
    reg:hasSubproperty <http://rdaregistry.info/Elements/e/P20270>,
        <http://rdaregistry.info/Elements/e/P20271>,
        <http://rdaregistry.info/Elements/e/P20272>,
        <http://rdaregistry.info/Elements/e/P20273>,
        <http://rdaregistry.info/Elements/e/P20274> ;
    reg:hasUnconstrained <http://rdaregistry.info/Elements/u/P60215> ;
    reg:lexicalAlias "http://rdaregistry.info/Elements/e/describedInExpression"@en ;
    reg:name "describedInExpression"@en ;
    reg:status <http://metadataregistry.org/uri/RegStatus/1001> ;
    rdfs:domain <http://rdaregistry.info/Elements/c/C10006> ;
    rdfs:isDefinedBy <http://rdaregistry.info/Elements/e/> ;
    rdfs:range <http://rdaregistry.info/Elements/c/C10001> ;
    rdfs:subPropertyOf <http://rdaregistry.info/Elements/e/P20268> ;
    owl:inverseOf <http://rdaregistry.info/Elements/w/P10277> ;
    skos:definition "Relates an expression to a work that describes a described expression. "@en .

<http://rdaregistry.info/Elements/e/P20046> a rdf:Property ;
    rdfs:label "has writer of supplementary textual content"@en ;
    reg:hasSubproperty <http://rdaregistry.info/Elements/e/P20030>,
        <http://rdaregistry.info/Elements/e/P20041>,
        <http://rdaregistry.info/Elements/e/P20044>,
        <http://rdaregistry.info/Elements/e/P20045>,
        <http://rdaregistry.info/Elements/e/P20275> ;
    reg:hasUnconstrained <http://rdaregistry.info/Elements/u/P60392> ;
    reg:lexicalAlias "http://rdaregistry.info/Elements/e/writerOfSupplementaryTextualContent"@en ;
    reg:name "writerOfSupplementaryTextualContent"@en ;
    reg:status <http://metadataregistry.org/uri/RegStatus/1001> ;
    rdfs:domain <http://rdaregistry.info/Elements/c/C10006> ;
    rdfs:isDefinedBy <http://rdaregistry.info/Elements/e/> ;
    rdfs:range <http://rdaregistry.info/Elements/c/C10002> ;
    rdfs:subPropertyOf <http://rdaregistry.info/Elements/e/P20053>,
        <http://rdaregistry.info/Elements/u/P60392> ;
    owl:inverseOf <http://rdaregistry.info/Elements/a/P50154> ;
    skos:definition "Relates an expression to a person, family, or corporate body contributing to an expression of a work by providing supplementary textual content (e.g., an appendix, an introduction, a preface) to the original work."@en .

<http://metadataregistry.org/uri/RegStatus/1008> a skos:Concept ;
    skos:prefLabel "Deprecated"@en .

<http://rdaregistry.info/Elements/e/P20154> a rdf:Property ;
    rdfs:label "is preceded by (expression)"@en ;
    reg:hasSubproperty <http://rdaregistry.info/Elements/e/P20137>,
        <http://rdaregistry.info/Elements/e/P20138>,
        <http://rdaregistry.info/Elements/e/P20149>,
        <http://rdaregistry.info/Elements/e/P20167>,
        <http://rdaregistry.info/Elements/e/P20168>,
        <http://rdaregistry.info/Elements/e/P20198>,
        <http://rdaregistry.info/Elements/e/P20199>,
        <http://rdaregistry.info/Elements/e/P20201> ;
    reg:hasUnconstrained <http://rdaregistry.info/Elements/u/P60261> ;
    reg:lexicalAlias "http://rdaregistry.info/Elements/e/precededByExpression"@en ;
    reg:name "precededByExpression"@en ;
    reg:status <http://metadataregistry.org/uri/RegStatus/1001> ;
    rdfs:domain <http://rdaregistry.info/Elements/c/C10006> ;
    rdfs:isDefinedBy <http://rdaregistry.info/Elements/e/> ;
    rdfs:range <http://rdaregistry.info/Elements/c/C10006> ;
    rdfs:subPropertyOf <http://rdaregistry.info/Elements/e/P20235>,
        <http://rdaregistry.info/Elements/u/P60261> ;
    owl:inverseOf <http://rdaregistry.info/Elements/e/P20169> ;
    skos:definition "Relates an expression to an expression of a work that precedes (e.g., is earlier in time or before in narrative) the succeeding expression."@en .

<http://rdaregistry.info/Elements/e/P20169> a rdf:Property ;
    rdfs:label "is succeeded by (expression)"@en ;
    reg:hasSubproperty <http://rdaregistry.info/Elements/e/P20076>,
        <http://rdaregistry.info/Elements/e/P20101>,
        <http://rdaregistry.info/Elements/e/P20143>,
        <http://rdaregistry.info/Elements/e/P20144>,
        <http://rdaregistry.info/Elements/e/P20191>,
        <http://rdaregistry.info/Elements/e/P20200> ;
    reg:hasUnconstrained <http://rdaregistry.info/Elements/u/P60278> ;
    reg:lexicalAlias "http://rdaregistry.info/Elements/e/succeededByExpression"@en ;
    reg:name "succeededByExpression"@en ;
    reg:status <http://metadataregistry.org/uri/RegStatus/1001> ;
    rdfs:domain <http://rdaregistry.info/Elements/c/C10006> ;
    rdfs:isDefinedBy <http://rdaregistry.info/Elements/e/> ;
    rdfs:range <http://rdaregistry.info/Elements/c/C10006> ;
    rdfs:subPropertyOf <http://rdaregistry.info/Elements/e/P20235>,
        <http://rdaregistry.info/Elements/u/P60278> ;
    owl:inverseOf <http://rdaregistry.info/Elements/e/P20154> ;
    skos:definition "Relates an expression to an expression of a work that succeeds (e.g., later in time or after in a narrative) the preceding expression."@en .

<http://rdaregistry.info/Elements/e/P20100> a rdf:Property ;
    rdfs:label "is complemented by (expression)"@en ;
    reg:hasSubproperty <http://rdaregistry.info/Elements/e/P20084>,
        <http://rdaregistry.info/Elements/e/P20102>,
        <http://rdaregistry.info/Elements/e/P20157>,
        <http://rdaregistry.info/Elements/e/P20160>,
        <http://rdaregistry.info/Elements/e/P20163>,
        <http://rdaregistry.info/Elements/e/P20176>,
        <http://rdaregistry.info/Elements/e/P20253>,
        <http://rdaregistry.info/Elements/e/P20254> ;
    reg:hasUnconstrained <http://rdaregistry.info/Elements/u/P60198> ;
    reg:lexicalAlias "http://rdaregistry.info/Elements/e/complementedByExpression"@en ;
    reg:name "complementedByExpression"@en ;
    reg:status <http://metadataregistry.org/uri/RegStatus/1001> ;
    rdfs:domain <http://rdaregistry.info/Elements/c/C10006> ;
    rdfs:isDefinedBy <http://rdaregistry.info/Elements/e/> ;
    rdfs:range <http://rdaregistry.info/Elements/c/C10006> ;
    rdfs:subPropertyOf <http://rdaregistry.info/Elements/e/P20232>,
        <http://rdaregistry.info/Elements/u/P60198> ;
    owl:inverseOf <http://rdaregistry.info/Elements/e/P20100> ;
    skos:definition "Relates an expression to an expression of a work paired with another expression without either expression being considered to predominate."@en .

<http://rdaregistry.info/Elements/e/P20105> a rdf:Property ;
    rdfs:label "is augmented by (expression)"@en ;
    reg:hasSubproperty <http://rdaregistry.info/Elements/e/P20080>,
        <http://rdaregistry.info/Elements/e/P20093>,
        <http://rdaregistry.info/Elements/e/P20094>,
        <http://rdaregistry.info/Elements/e/P20107>,
        <http://rdaregistry.info/Elements/e/P20108>,
        <http://rdaregistry.info/Elements/e/P20109>,
        <http://rdaregistry.info/Elements/e/P20118>,
        <http://rdaregistry.info/Elements/e/P20120>,
        <http://rdaregistry.info/Elements/e/P20155>,
        <http://rdaregistry.info/Elements/e/P20156>,
        <http://rdaregistry.info/Elements/e/P20172> ;
    reg:hasUnconstrained <http://rdaregistry.info/Elements/u/P60204> ;
    reg:lexicalAlias "http://rdaregistry.info/Elements/e/augmentedByExpression"@en ;
    reg:name "augmentedByExpression"@en ;
    reg:status <http://metadataregistry.org/uri/RegStatus/1001> ;
    rdfs:domain <http://rdaregistry.info/Elements/c/C10006> ;
    rdfs:isDefinedBy <http://rdaregistry.info/Elements/e/> ;
    rdfs:range <http://rdaregistry.info/Elements/c/C10006> ;
    rdfs:subPropertyOf <http://rdaregistry.info/Elements/e/P20232>,
        <http://rdaregistry.info/Elements/u/P60204> ;
    owl:inverseOf <http://rdaregistry.info/Elements/e/P20192> ;
    skos:definition "Relates an expression to an expression of a work that adds to the content of a predominant expression."@en .

<http://rdaregistry.info/Elements/e/P20192> a rdf:Property ;
    rdfs:label "is augmentation of (expression)"@en ;
    reg:hasSubproperty <http://rdaregistry.info/Elements/e/P20083>,
        <http://rdaregistry.info/Elements/e/P20089>,
        <http://rdaregistry.info/Elements/e/P20146>,
        <http://rdaregistry.info/Elements/e/P20147>,
        <http://rdaregistry.info/Elements/e/P20148>,
        <http://rdaregistry.info/Elements/e/P20151>,
        <http://rdaregistry.info/Elements/e/P20177>,
        <http://rdaregistry.info/Elements/e/P20180>,
        <http://rdaregistry.info/Elements/e/P20181>,
        <http://rdaregistry.info/Elements/e/P20188>,
        <http://rdaregistry.info/Elements/e/P20197> ;
    reg:hasUnconstrained <http://rdaregistry.info/Elements/u/P60307> ;
    reg:lexicalAlias "http://rdaregistry.info/Elements/e/augmentationOfExpression"@en ;
    reg:name "augmentationOfExpression"@en ;
    reg:status <http://metadataregistry.org/uri/RegStatus/1001> ;
    rdfs:domain <http://rdaregistry.info/Elements/c/C10006> ;
    rdfs:isDefinedBy <http://rdaregistry.info/Elements/e/> ;
    rdfs:range <http://rdaregistry.info/Elements/c/C10006> ;
    rdfs:subPropertyOf <http://rdaregistry.info/Elements/e/P20232>,
        <http://rdaregistry.info/Elements/u/P60307> ;
    owl:inverseOf <http://rdaregistry.info/Elements/e/P20105> ;
    skos:definition "Relates an expression to an expression of a work whose content is added to by another expression."@en .

<http://rdaregistry.info/Elements/e/P20153> a rdf:Property ;
    rdfs:label "is adapted as (expression)"@en ;
    reg:hasSubproperty <http://rdaregistry.info/Elements/e/P20009>,
        <http://rdaregistry.info/Elements/e/P20060>,
        <http://rdaregistry.info/Elements/e/P20066>,
        <http://rdaregistry.info/Elements/e/P20067>,
        <http://rdaregistry.info/Elements/e/P20073>,
        <http://rdaregistry.info/Elements/e/P20077>,
        <http://rdaregistry.info/Elements/e/P20088>,
        <http://rdaregistry.info/Elements/e/P20096>,
        <http://rdaregistry.info/Elements/e/P20099>,
        <http://rdaregistry.info/Elements/e/P20255> ;
    reg:hasUnconstrained <http://rdaregistry.info/Elements/u/P60260> ;
    reg:lexicalAlias "http://rdaregistry.info/Elements/e/adaptedAsExpression"@en ;
    reg:name "adaptedAsExpression"@en ;
    reg:status <http://metadataregistry.org/uri/RegStatus/1001> ;
    rdfs:domain <http://rdaregistry.info/Elements/c/C10006> ;
    rdfs:isDefinedBy <http://rdaregistry.info/Elements/e/> ;
    rdfs:range <http://rdaregistry.info/Elements/c/C10006> ;
    rdfs:subPropertyOf <http://rdaregistry.info/Elements/e/P20203> ;
    owl:inverseOf <http://rdaregistry.info/Elements/e/P20152> ;
    skos:definition "Relates an expression to an expression of a work based on the source expression."@en .

<http://rdaregistry.info/Elements/e/P20039> a rdf:Property ;
    rdfs:label "has performer"@en ;
    reg:hasSubproperty <http://rdaregistry.info/Elements/e/P20011>,
        <http://rdaregistry.info/Elements/e/P20012>,
        <http://rdaregistry.info/Elements/e/P20013>,
        <http://rdaregistry.info/Elements/e/P20014>,
        <http://rdaregistry.info/Elements/e/P20015>,
        <http://rdaregistry.info/Elements/e/P20016>,
        <http://rdaregistry.info/Elements/e/P20017>,
        <http://rdaregistry.info/Elements/e/P20018>,
        <http://rdaregistry.info/Elements/e/P20019>,
        <http://rdaregistry.info/Elements/e/P20020>,
        <http://rdaregistry.info/Elements/e/P20021>,
        <http://rdaregistry.info/Elements/e/P20022>,
        <http://rdaregistry.info/Elements/e/P20023>,
        <http://rdaregistry.info/Elements/e/P20024>,
        <http://rdaregistry.info/Elements/e/P20025> ;
    reg:hasUnconstrained <http://rdaregistry.info/Elements/u/P60387> ;
    reg:lexicalAlias "http://rdaregistry.info/Elements/e/performer"@en ;
    reg:name "performer"@en ;
    reg:status <http://metadataregistry.org/uri/RegStatus/1001> ;
    rdfs:domain <http://rdaregistry.info/Elements/c/C10006> ;
    rdfs:isDefinedBy <http://rdaregistry.info/Elements/e/> ;
    rdfs:range <http://rdaregistry.info/Elements/c/C10002> ;
    rdfs:subPropertyOf <http://rdaregistry.info/Elements/e/P20053>,
        <http://rdaregistry.info/Elements/u/P60387> ;
    owl:inverseOf <http://rdaregistry.info/Elements/a/P50147> ;
    skos:definition "Relates an expression to a person, family, or corporate body contributing to an expression of a work by performing music, acting, dancing, speaking, etc., often in a musical or dramatic presentation, etc."@en .

<http://rdaregistry.info/Elements/e/P20152> a rdf:Property ;
    rdfs:label "is adaptation of (expression)"@en ;
    reg:hasSubproperty <http://rdaregistry.info/Elements/e/P20123>,
        <http://rdaregistry.info/Elements/e/P20124>,
        <http://rdaregistry.info/Elements/e/P20125>,
        <http://rdaregistry.info/Elements/e/P20126>,
        <http://rdaregistry.info/Elements/e/P20127>,
        <http://rdaregistry.info/Elements/e/P20128>,
        <http://rdaregistry.info/Elements/e/P20129>,
        <http://rdaregistry.info/Elements/e/P20133>,
        <http://rdaregistry.info/Elements/e/P20134>,
        <http://rdaregistry.info/Elements/e/P20256> ;
    reg:hasUnconstrained <http://rdaregistry.info/Elements/u/P60241> ;
    reg:lexicalAlias "http://rdaregistry.info/Elements/e/adaptationOfExpression"@en ;
    reg:name "adaptationOfExpression"@en ;
    reg:status <http://metadataregistry.org/uri/RegStatus/1001> ;
    rdfs:domain <http://rdaregistry.info/Elements/c/C10006> ;
    rdfs:isDefinedBy <http://rdaregistry.info/Elements/e/> ;
    rdfs:range <http://rdaregistry.info/Elements/c/C10006> ;
    rdfs:subPropertyOf <http://rdaregistry.info/Elements/e/P20204>,
        <http://rdaregistry.info/Elements/u/P60241> ;
    owl:inverseOf <http://rdaregistry.info/Elements/e/P20153> ;
    skos:definition "Relates an expression to an expression of a work that has been modified for a purpose, use, or medium other than that for which it was originally intended."@en .

<http://rdaregistry.info/Elements/e/P20203> a rdf:Property ;
    rdfs:label "is derivative (expression)"@en ;
    reg:hasSubproperty <http://rdaregistry.info/Elements/e/P20082>,
        <http://rdaregistry.info/Elements/e/P20086>,
        <http://rdaregistry.info/Elements/e/P20087>,
        <http://rdaregistry.info/Elements/e/P20090>,
        <http://rdaregistry.info/Elements/e/P20091>,
        <http://rdaregistry.info/Elements/e/P20092>,
        <http://rdaregistry.info/Elements/e/P20104>,
        <http://rdaregistry.info/Elements/e/P20106>,
        <http://rdaregistry.info/Elements/e/P20110>,
        <http://rdaregistry.info/Elements/e/P20114>,
        <http://rdaregistry.info/Elements/e/P20115>,
        <http://rdaregistry.info/Elements/e/P20119>,
        <http://rdaregistry.info/Elements/e/P20164>,
        <http://rdaregistry.info/Elements/e/P20165>,
        <http://rdaregistry.info/Elements/e/P20166>,
        <http://rdaregistry.info/Elements/e/P20170>,
        <http://rdaregistry.info/Elements/e/P20171>,
        <http://rdaregistry.info/Elements/e/P20204>,
        <http://rdaregistry.info/Elements/e/P20211> ;
    reg:hasUnconstrained <http://rdaregistry.info/Elements/u/P60250> ;
    reg:lexicalAlias "http://rdaregistry.info/Elements/e/derivativeExpression"@en ;
    reg:name "derivativeExpression"@en ;
    reg:status <http://metadataregistry.org/uri/RegStatus/1001> ;
    rdfs:domain <http://rdaregistry.info/Elements/c/C10006> ;
    rdfs:isDefinedBy <http://rdaregistry.info/Elements/e/> ;
    rdfs:range <http://rdaregistry.info/Elements/c/C10006> ;
    rdfs:subPropertyOf <http://rdaregistry.info/Elements/e/P20233>,
        <http://rdaregistry.info/Elements/u/P60250> ;
    owl:inverseOf <http://rdaregistry.info/Elements/e/P20204> ;
    skos:definition "Relates an expression to an expression that is a modification of a source expression."@en .

<http://rdaregistry.info/Elements/e/P20204> a rdf:Property ;
    rdfs:label "is based on (expression)"@en ;
    reg:hasSubproperty <http://rdaregistry.info/Elements/e/P20081>,
        <http://rdaregistry.info/Elements/e/P20121>,
        <http://rdaregistry.info/Elements/e/P20122>,
        <http://rdaregistry.info/Elements/e/P20135>,
        <http://rdaregistry.info/Elements/e/P20139>,
        <http://rdaregistry.info/Elements/e/P20140>,
        <http://rdaregistry.info/Elements/e/P20141>,
        <http://rdaregistry.info/Elements/e/P20152>,
        <http://rdaregistry.info/Elements/e/P20159>,
        <http://rdaregistry.info/Elements/e/P20179>,
        <http://rdaregistry.info/Elements/e/P20183>,
        <http://rdaregistry.info/Elements/e/P20184>,
        <http://rdaregistry.info/Elements/e/P20185>,
        <http://rdaregistry.info/Elements/e/P20186>,
        <http://rdaregistry.info/Elements/e/P20189>,
        <http://rdaregistry.info/Elements/e/P20190>,
        <http://rdaregistry.info/Elements/e/P20193>,
        <http://rdaregistry.info/Elements/e/P20194>,
        <http://rdaregistry.info/Elements/e/P20195> ;
    reg:hasUnconstrained <http://rdaregistry.info/Elements/u/P60305> ;
    reg:lexicalAlias "http://rdaregistry.info/Elements/e/basedOnExpression"@en ;
    reg:name "basedOnExpression"@en ;
    reg:status <http://metadataregistry.org/uri/RegStatus/1001> ;
    rdfs:domain <http://rdaregistry.info/Elements/c/C10006> ;
    rdfs:isDefinedBy <http://rdaregistry.info/Elements/e/> ;
    rdfs:range <http://rdaregistry.info/Elements/c/C10006> ;
    rdfs:subPropertyOf <http://rdaregistry.info/Elements/e/P20233> ;
    owl:inverseOf <http://rdaregistry.info/Elements/e/P20203> ;
    skos:definition "Relates an expression to an expression used as the basis for a derivative expression"@en .

<http://rdaregistry.info/Elements/e/P20053> a rdf:Property ;
    rdfs:label "has contributor"@en ;
    reg:hasSubproperty <http://rdaregistry.info/Elements/e/P20026>,
        <http://rdaregistry.info/Elements/e/P20027>,
        <http://rdaregistry.info/Elements/e/P20028>,
        <http://rdaregistry.info/Elements/e/P20029>,
        <http://rdaregistry.info/Elements/e/P20031>,
        <http://rdaregistry.info/Elements/e/P20032>,
        <http://rdaregistry.info/Elements/e/P20033>,
        <http://rdaregistry.info/Elements/e/P20034>,
        <http://rdaregistry.info/Elements/e/P20035>,
        <http://rdaregistry.info/Elements/e/P20036>,
        <http://rdaregistry.info/Elements/e/P20037>,
        <http://rdaregistry.info/Elements/e/P20038>,
        <http://rdaregistry.info/Elements/e/P20039>,
        <http://rdaregistry.info/Elements/e/P20042>,
        <http://rdaregistry.info/Elements/e/P20043>,
        <http://rdaregistry.info/Elements/e/P20046>,
        <http://rdaregistry.info/Elements/e/P20047>,
        <http://rdaregistry.info/Elements/e/P20048>,
        <http://rdaregistry.info/Elements/e/P20049>,
        <http://rdaregistry.info/Elements/e/P20050>,
        <http://rdaregistry.info/Elements/e/P20051>,
        <http://rdaregistry.info/Elements/e/P20052>,
        <http://rdaregistry.info/Elements/e/P20055>,
        <http://rdaregistry.info/Elements/e/P20056>,
        <http://rdaregistry.info/Elements/e/P20058>,
        <http://rdaregistry.info/Elements/e/P20257>,
        <http://rdaregistry.info/Elements/e/P20258>,
        <http://rdaregistry.info/Elements/e/P20276>,
        <http://rdaregistry.info/Elements/e/P20277> ;
    reg:hasUnconstrained <http://rdaregistry.info/Elements/u/P60398> ;
    reg:lexicalAlias "http://rdaregistry.info/Elements/e/contributor"@en ;
    reg:name "contributor"@en ;
    reg:status <http://metadataregistry.org/uri/RegStatus/1001> ;
    rdfs:domain <http://rdaregistry.info/Elements/c/C10006> ;
    rdfs:isDefinedBy <http://rdaregistry.info/Elements/e/> ;
    rdfs:range <http://rdaregistry.info/Elements/c/C10002> ;
    owl:inverseOf <http://rdaregistry.info/Elements/a/P50161> ;
    skos:definition "Relates an expression to a person, family, or corporate body contributing to an expression."@en ;
    skos:scopeNote "Contributors include editors, translators, arrangers of music, performers, etc."@en .

<http://metadataregistry.org/uri/RegStatus/1001> a skos:Concept ;
    skos:prefLabel "Published"@en .

<http://rdaregistry.info/Elements/e/> dc:title "RDA Expression properties"@en ;
    skos:note "Properties derived from RDA elements and relationship designators with the domain of RDA Expression."@en .

